<?xml version="1.0" encoding="utf-8" ?>
<rdf:RDF xmlns:rdf="http://www.w3.org/1999/02/22-rdf-syntax-ns#"
         xmlns:skos="http://www.w3.org/2004/02/skos/core#"
         xmlns:dc="http://purl.org/dc/terms/"
         xmlns:cc="http://creativecommons.org/ns#">

  <skos:ConceptScheme rdf:about="http://purl.org/heritagedata/schemes/571">
    <dc:issued rdf:datatype="http://www.w3.org/2001/XMLSchema#date">2024-07-01</dc:issued>
    <cc:license rdf:resource="https://www.nationalarchives.gov.uk/doc/open-government-licence/version/3/"/>
    <cc:attributionURL rdf:resource="https://historicengland.org.uk/"/>
    <cc:attributionName xml:lang="en">Historic England</cc:attributionName>
    <dc:publisher rdf:resource="https://historicengland.org.uk/"/>
    <dc:identifier>http://purl.org/heritagedata/schemes/571</dc:identifier>
    <dc:spatial rdf:resource="http://dbpedia.org/resource/England"/>
    <dc:spatial rdf:resource="http://vocab.getty.edu/tgn/7002445"/>
    <dc:title xml:lang="en">Historic Characterization Thesaurus</dc:title>
    <dc:description xml:lang="en">Thesaurus combining Historic Landscape and Historic Seascape Characterization terminology (e.g. reclaimed land, vineyard, dunes).</dc:description>
    <skos:hasTopConcept rdf:resource="http://purl.org/heritagedata/schemes/571/concepts/151445"/>
    <skos:hasTopConcept rdf:resource="http://purl.org/heritagedata/schemes/571/concepts/151446"/>
    <skos:hasTopConcept rdf:resource="http://purl.org/heritagedata/schemes/571/concepts/151447"/>
    <skos:hasTopConcept rdf:resource="http://purl.org/heritagedata/schemes/571/concepts/151448"/>
    <skos:hasTopConcept rdf:resource="http://purl.org/heritagedata/schemes/571/concepts/151449"/>
    <skos:hasTopConcept rdf:resource="http://purl.org/heritagedata/schemes/571/concepts/151450"/>
    <skos:hasTopConcept rdf:resource="http://purl.org/heritagedata/schemes/571/concepts/151451"/>
    <skos:hasTopConcept rdf:resource="http://purl.org/heritagedata/schemes/571/concepts/151452"/>
    <skos:hasTopConcept rdf:resource="http://purl.org/heritagedata/schemes/571/concepts/151453"/>
    <skos:hasTopConcept rdf:resource="http://purl.org/heritagedata/schemes/571/concepts/151456"/>
    <skos:hasTopConcept rdf:resource="http://purl.org/heritagedata/schemes/571/concepts/151457"/>
    <skos:hasTopConcept rdf:resource="http://purl.org/heritagedata/schemes/571/concepts/151458"/>
    <skos:hasTopConcept rdf:resource="http://purl.org/heritagedata/schemes/571/concepts/151459"/>
    <skos:hasTopConcept rdf:resource="http://purl.org/heritagedata/schemes/571/concepts/151460"/>
    <skos:hasTopConcept rdf:resource="http://purl.org/heritagedata/schemes/571/concepts/151666"/>
    <skos:hasTopConcept rdf:resource="http://purl.org/heritagedata/schemes/571/concepts/152326"/>
    <skos:hasTopConcept rdf:resource="http://purl.org/heritagedata/schemes/571/concepts/152394"/>
  </skos:ConceptScheme>

  <skos:Concept rdf:about="http://purl.org/heritagedata/schemes/571/concepts/151054">
    <skos:broader rdf:resource="http://purl.org/heritagedata/schemes/571/concepts/151715"/>
    <skos:inScheme rdf:resource="http://purl.org/heritagedata/schemes/571"/>
    <dc:identifier>http://purl.org/heritagedata/schemes/571/concepts/151054</dc:identifier>
    <dc:issued rdf:datatype="http://www.w3.org/2001/XMLSchema#dateTime">2024-07-01T17:17:33</dc:issued>
    <cc:license rdf:resource="https://www.nationalarchives.gov.uk/doc/open-government-licence/version/3/"/>
    <cc:attributionURL rdf:resource="https://historicengland.org.uk/"/>
    <cc:attributionName xml:lang="en">Historic England</cc:attributionName>
    <dc:publisher rdf:resource="https://historicengland.org.uk/"/>
    <dc:spatial rdf:resource="http://vocab.getty.edu/tgn/7002445"/>
    <dc:spatial rdf:resource="http://dbpedia.org/resource/England"/>
    <skos:prefLabel xml:lang="en">Reservoir</skos:prefLabel>
    <skos:related rdf:resource="http://purl.org/heritagedata/schemes/571/concepts/151057"/>
    <skos:scopeNote xml:lang="en">A body of water or other liquid, wholly or partly artificial and sometimes covered, used to collect and store water, or other liquid for a particular function. Most often for the collection and supply of water for public and industrial use.</skos:scopeNote>
  </skos:Concept>

  <skos:Concept rdf:about="http://purl.org/heritagedata/schemes/571/concepts/151715">
    <skos:narrower rdf:resource="http://purl.org/heritagedata/schemes/571/concepts/151054"/>
    <skos:narrower>
      <skos:Concept rdf:about="http://purl.org/heritagedata/schemes/571/concepts/151056">
        <skos:broader rdf:resource="http://purl.org/heritagedata/schemes/571/concepts/151715"/>
        <skos:inScheme rdf:resource="http://purl.org/heritagedata/schemes/571"/>
        <dc:identifier>http://purl.org/heritagedata/schemes/571/concepts/151056</dc:identifier>
        <dc:issued rdf:datatype="http://www.w3.org/2001/XMLSchema#dateTime">2024-07-01T17:17:33</dc:issued>
        <cc:license rdf:resource="https://www.nationalarchives.gov.uk/doc/open-government-licence/version/3/"/>
        <cc:attributionURL rdf:resource="https://historicengland.org.uk/"/>
        <cc:attributionName xml:lang="en">Historic England</cc:attributionName>
        <dc:publisher rdf:resource="https://historicengland.org.uk/"/>
        <dc:spatial rdf:resource="http://vocab.getty.edu/tgn/7002445"/>
        <dc:spatial rdf:resource="http://dbpedia.org/resource/England"/>
        <skos:prefLabel xml:lang="en">Waterworks</skos:prefLabel>
        <skos:scopeNote xml:lang="en">Buildings, engineering constructions and machinery, used for the purpose of supplying a town, or region with water distributed through pipes.</skos:scopeNote>
      </skos:Concept>
    </skos:narrower>

    <skos:narrower rdf:resource="http://purl.org/heritagedata/schemes/571/concepts/151057"/>
    <skos:broader rdf:resource="http://purl.org/heritagedata/schemes/571/concepts/151460"/>
    <skos:inScheme rdf:resource="http://purl.org/heritagedata/schemes/571"/>
    <dc:identifier>http://purl.org/heritagedata/schemes/571/concepts/151715</dc:identifier>
    <dc:issued rdf:datatype="http://www.w3.org/2001/XMLSchema#dateTime">2024-07-01T17:17:33</dc:issued>
    <cc:license rdf:resource="https://www.nationalarchives.gov.uk/doc/open-government-licence/version/3/"/>
    <cc:attributionURL rdf:resource="https://historicengland.org.uk/"/>
    <cc:attributionName xml:lang="en">Historic England</cc:attributionName>
    <dc:publisher rdf:resource="https://historicengland.org.uk/"/>
    <dc:spatial rdf:resource="http://vocab.getty.edu/tgn/7002445"/>
    <dc:spatial rdf:resource="http://dbpedia.org/resource/England"/>
    <skos:prefLabel xml:lang="en">Water Storage And Supply</skos:prefLabel>
    <skos:scopeNote xml:lang="en">Sites and structures associated with the storage and distribution of water.</skos:scopeNote>
  </skos:Concept>

  <skos:Concept rdf:about="http://purl.org/heritagedata/schemes/571/concepts/151055">
    <skos:broader rdf:resource="http://purl.org/heritagedata/schemes/571/concepts/152561"/>
    <skos:narrower>
      <skos:Concept rdf:about="http://purl.org/heritagedata/schemes/571/concepts/151058">
        <skos:broader rdf:resource="http://purl.org/heritagedata/schemes/571/concepts/151055"/>
        <skos:inScheme rdf:resource="http://purl.org/heritagedata/schemes/571"/>
        <dc:identifier>http://purl.org/heritagedata/schemes/571/concepts/151058</dc:identifier>
        <dc:issued rdf:datatype="http://www.w3.org/2001/XMLSchema#dateTime">2024-07-01T17:17:33</dc:issued>
        <cc:license rdf:resource="https://www.nationalarchives.gov.uk/doc/open-government-licence/version/3/"/>
        <cc:attributionURL rdf:resource="https://historicengland.org.uk/"/>
        <cc:attributionName xml:lang="en">Historic England</cc:attributionName>
        <dc:publisher rdf:resource="https://historicengland.org.uk/"/>
        <dc:spatial rdf:resource="http://vocab.getty.edu/tgn/7002445"/>
        <dc:spatial rdf:resource="http://dbpedia.org/resource/England"/>
        <skos:prefLabel xml:lang="en">Sea Wall</skos:prefLabel>
        <skos:scopeNote xml:lang="en">A form of sea defence, may be of hard and strong material (eg concrete) or an earthen bank constructed on the landward part of a coast to reduce the effects of strong waves.</skos:scopeNote>
      </skos:Concept>
    </skos:narrower>

    <skos:narrower rdf:resource="http://purl.org/heritagedata/schemes/571/concepts/151059"/>
    <skos:narrower>
      <skos:Concept rdf:about="http://purl.org/heritagedata/schemes/571/concepts/151061">
        <skos:broader rdf:resource="http://purl.org/heritagedata/schemes/571/concepts/151055"/>
        <skos:inScheme rdf:resource="http://purl.org/heritagedata/schemes/571"/>
        <dc:identifier>http://purl.org/heritagedata/schemes/571/concepts/151061</dc:identifier>
        <dc:issued rdf:datatype="http://www.w3.org/2001/XMLSchema#dateTime">2024-07-01T17:17:33</dc:issued>
        <cc:license rdf:resource="https://www.nationalarchives.gov.uk/doc/open-government-licence/version/3/"/>
        <cc:attributionURL rdf:resource="https://historicengland.org.uk/"/>
        <cc:attributionName xml:lang="en">Historic England</cc:attributionName>
        <dc:publisher rdf:resource="https://historicengland.org.uk/"/>
        <dc:spatial rdf:resource="http://vocab.getty.edu/tgn/7002445"/>
        <dc:spatial rdf:resource="http://dbpedia.org/resource/England"/>
        <skos:prefLabel xml:lang="en">Groynes</skos:prefLabel>
        <skos:scopeNote xml:lang="en">A series of structures extending into the sea for the purpose of preventing further lateral movement of washed up sand and shingle.</skos:scopeNote>
      </skos:Concept>
    </skos:narrower>

    <skos:inScheme rdf:resource="http://purl.org/heritagedata/schemes/571"/>
    <dc:identifier>http://purl.org/heritagedata/schemes/571/concepts/151055</dc:identifier>
    <dc:issued rdf:datatype="http://www.w3.org/2001/XMLSchema#dateTime">2024-07-01T17:17:33</dc:issued>
    <cc:license rdf:resource="https://www.nationalarchives.gov.uk/doc/open-government-licence/version/3/"/>
    <cc:attributionURL rdf:resource="https://historicengland.org.uk/"/>
    <cc:attributionName xml:lang="en">Historic England</cc:attributionName>
    <dc:publisher rdf:resource="https://historicengland.org.uk/"/>
    <dc:spatial rdf:resource="http://vocab.getty.edu/tgn/7002445"/>
    <dc:spatial rdf:resource="http://dbpedia.org/resource/England"/>
    <skos:prefLabel xml:lang="en">Sea Defence</skos:prefLabel>
    <skos:related rdf:resource="http://purl.org/heritagedata/schemes/571/concepts/151095"/>
    <skos:scopeNote xml:lang="en">Non-military artificial structure designed to counter losses to coastal land from the erosive forces of the sea. May work directly to withstand those forces along a defined line, or they may seek to dissipate them in the inter-tidal zone.</skos:scopeNote>
  </skos:Concept>

  <skos:Concept rdf:about="http://purl.org/heritagedata/schemes/571/concepts/152561">
    <skos:narrower rdf:resource="http://purl.org/heritagedata/schemes/571/concepts/151055"/>
    <skos:narrower>
      <skos:Concept rdf:about="http://purl.org/heritagedata/schemes/571/concepts/152560">
        <skos:broader rdf:resource="http://purl.org/heritagedata/schemes/571/concepts/152561"/>
        <skos:inScheme rdf:resource="http://purl.org/heritagedata/schemes/571"/>
        <dc:identifier>http://purl.org/heritagedata/schemes/571/concepts/152560</dc:identifier>
        <dc:issued rdf:datatype="http://www.w3.org/2001/XMLSchema#dateTime">2024-07-01T17:17:33</dc:issued>
        <cc:license rdf:resource="https://www.nationalarchives.gov.uk/doc/open-government-licence/version/3/"/>
        <cc:attributionURL rdf:resource="https://historicengland.org.uk/"/>
        <cc:attributionName xml:lang="en">Historic England</cc:attributionName>
        <dc:publisher rdf:resource="https://historicengland.org.uk/"/>
        <dc:spatial rdf:resource="http://vocab.getty.edu/tgn/7002445"/>
        <dc:spatial rdf:resource="http://dbpedia.org/resource/England"/>
        <skos:prefLabel xml:lang="en">Flood Defence</skos:prefLabel>
        <skos:scopeNote xml:lang="en">Artificial constructions used to prevent water flooding the surrounding area. Often taking the form of a bank or wall but may be more elaborate (eg the Thames Barrier) and include run-off drains and reservoirs.</skos:scopeNote>
      </skos:Concept>
    </skos:narrower>

    <skos:broader rdf:resource="http://purl.org/heritagedata/schemes/571/concepts/151460"/>
    <skos:inScheme rdf:resource="http://purl.org/heritagedata/schemes/571"/>
    <dc:identifier>http://purl.org/heritagedata/schemes/571/concepts/152561</dc:identifier>
    <dc:issued rdf:datatype="http://www.w3.org/2001/XMLSchema#dateTime">2024-07-01T17:17:33</dc:issued>
    <cc:license rdf:resource="https://www.nationalarchives.gov.uk/doc/open-government-licence/version/3/"/>
    <cc:attributionURL rdf:resource="https://historicengland.org.uk/"/>
    <cc:attributionName xml:lang="en">Historic England</cc:attributionName>
    <dc:publisher rdf:resource="https://historicengland.org.uk/"/>
    <dc:spatial rdf:resource="http://vocab.getty.edu/tgn/7002445"/>
    <dc:spatial rdf:resource="http://dbpedia.org/resource/England"/>
    <skos:prefLabel xml:lang="en">Flood And Erosion Defence</skos:prefLabel>
    <skos:scopeNote xml:lang="en">Provision of structures to remove, reduce or mitigate the risk of coastal, riverine and/or estuarine flooding from the sea, rivers or unchannelled rainfall run-off or to counter losses to coastal land from maritime erosive forces.</skos:scopeNote>
  </skos:Concept>

  <skos:Concept rdf:about="http://purl.org/heritagedata/schemes/571/concepts/151057">
    <skos:broader rdf:resource="http://purl.org/heritagedata/schemes/571/concepts/151715"/>
    <skos:inScheme rdf:resource="http://purl.org/heritagedata/schemes/571"/>
    <dc:identifier>http://purl.org/heritagedata/schemes/571/concepts/151057</dc:identifier>
    <dc:issued rdf:datatype="http://www.w3.org/2001/XMLSchema#dateTime">2024-07-01T17:17:33</dc:issued>
    <cc:license rdf:resource="https://www.nationalarchives.gov.uk/doc/open-government-licence/version/3/"/>
    <cc:attributionURL rdf:resource="https://historicengland.org.uk/"/>
    <cc:attributionName xml:lang="en">Historic England</cc:attributionName>
    <dc:publisher rdf:resource="https://historicengland.org.uk/"/>
    <dc:spatial rdf:resource="http://vocab.getty.edu/tgn/7002445"/>
    <dc:spatial rdf:resource="http://dbpedia.org/resource/England"/>
    <skos:prefLabel xml:lang="en">Dam</skos:prefLabel>
    <skos:related rdf:resource="http://purl.org/heritagedata/schemes/571/concepts/151054"/>
    <skos:scopeNote xml:lang="en">A structure built to form a barrier to restrain water or other liquid (including waste), raising its level on one side, to prevent flooding or to form a reservoir.</skos:scopeNote>
  </skos:Concept>

  <skos:Concept rdf:about="http://purl.org/heritagedata/schemes/571/concepts/151059">
    <skos:broader rdf:resource="http://purl.org/heritagedata/schemes/571/concepts/151055"/>
    <skos:broader rdf:resource="http://purl.org/heritagedata/schemes/571/concepts/151667"/>
    <skos:inScheme rdf:resource="http://purl.org/heritagedata/schemes/571"/>
    <dc:identifier>http://purl.org/heritagedata/schemes/571/concepts/151059</dc:identifier>
    <dc:issued rdf:datatype="http://www.w3.org/2001/XMLSchema#dateTime">2024-07-01T17:17:33</dc:issued>
    <cc:license rdf:resource="https://www.nationalarchives.gov.uk/doc/open-government-licence/version/3/"/>
    <cc:attributionURL rdf:resource="https://historicengland.org.uk/"/>
    <cc:attributionName xml:lang="en">Historic England</cc:attributionName>
    <dc:publisher rdf:resource="https://historicengland.org.uk/"/>
    <dc:spatial rdf:resource="http://vocab.getty.edu/tgn/7002445"/>
    <dc:spatial rdf:resource="http://dbpedia.org/resource/England"/>
    <skos:prefLabel xml:lang="en">Breakwater</skos:prefLabel>
    <skos:related rdf:resource="http://purl.org/heritagedata/schemes/571/concepts/151095"/>
    <skos:scopeNote xml:lang="en">A structure which protects a beach or harbour by breaking the force of waves. It may be constructed entirely offshore at a strategic location or with one end attached to land. Commonly associated with ports and navigable river mouths.</skos:scopeNote>
  </skos:Concept>

  <skos:Concept rdf:about="http://purl.org/heritagedata/schemes/571/concepts/151667">
    <skos:narrower rdf:resource="http://purl.org/heritagedata/schemes/571/concepts/151059"/>
    <skos:narrower rdf:resource="http://purl.org/heritagedata/schemes/571/concepts/151086"/>
    <skos:narrower rdf:resource="http://purl.org/heritagedata/schemes/571/concepts/151091"/>
    <skos:narrower>
      <skos:Concept rdf:about="http://purl.org/heritagedata/schemes/571/concepts/151094">
        <skos:broader rdf:resource="http://purl.org/heritagedata/schemes/571/concepts/151667"/>
        <skos:inScheme rdf:resource="http://purl.org/heritagedata/schemes/571"/>
        <dc:identifier>http://purl.org/heritagedata/schemes/571/concepts/151094</dc:identifier>
        <dc:issued rdf:datatype="http://www.w3.org/2001/XMLSchema#dateTime">2024-07-01T17:17:33</dc:issued>
        <cc:license rdf:resource="https://www.nationalarchives.gov.uk/doc/open-government-licence/version/3/"/>
        <cc:attributionURL rdf:resource="https://historicengland.org.uk/"/>
        <cc:attributionName xml:lang="en">Historic England</cc:attributionName>
        <dc:publisher rdf:resource="https://historicengland.org.uk/"/>
        <dc:spatial rdf:resource="http://vocab.getty.edu/tgn/7002445"/>
        <dc:spatial rdf:resource="http://dbpedia.org/resource/England"/>
        <skos:prefLabel xml:lang="en">Quarantine Area</skos:prefLabel>
        <skos:scopeNote xml:lang="en">An area, often linked to a port, where a period of detention was imposed on travellers or voyagers suspected of carrying infectious diseases before they were allowed to enter a country or town.</skos:scopeNote>
      </skos:Concept>
    </skos:narrower>

    <skos:narrower rdf:resource="http://purl.org/heritagedata/schemes/571/concepts/151096"/>
    <skos:narrower rdf:resource="http://purl.org/heritagedata/schemes/571/concepts/151097"/>
    <skos:narrower>
      <skos:Concept rdf:about="http://purl.org/heritagedata/schemes/571/concepts/151145">
        <skos:broader rdf:resource="http://purl.org/heritagedata/schemes/571/concepts/151667"/>
        <skos:inScheme rdf:resource="http://purl.org/heritagedata/schemes/571"/>
        <dc:identifier>http://purl.org/heritagedata/schemes/571/concepts/151145</dc:identifier>
        <dc:issued rdf:datatype="http://www.w3.org/2001/XMLSchema#dateTime">2024-07-01T17:17:33</dc:issued>
        <cc:license rdf:resource="https://www.nationalarchives.gov.uk/doc/open-government-licence/version/3/"/>
        <cc:attributionURL rdf:resource="https://historicengland.org.uk/"/>
        <cc:attributionName xml:lang="en">Historic England</cc:attributionName>
        <dc:publisher rdf:resource="https://historicengland.org.uk/"/>
        <dc:spatial rdf:resource="http://vocab.getty.edu/tgn/7002445"/>
        <dc:spatial rdf:resource="http://dbpedia.org/resource/England"/>
        <skos:prefLabel xml:lang="en">Marina</skos:prefLabel>
        <skos:scopeNote xml:lang="en">A dock or basin on the coast, an estuary or an inland waterway, used for mooring yachts and other small pleasure craft.</skos:scopeNote>
      </skos:Concept>
    </skos:narrower>

    <skos:narrower rdf:resource="http://purl.org/heritagedata/schemes/571/concepts/151404"/>
    <skos:narrower rdf:resource="http://purl.org/heritagedata/schemes/571/concepts/151405"/>
    <skos:narrower rdf:resource="http://purl.org/heritagedata/schemes/571/concepts/151652"/>
    <skos:narrower rdf:resource="http://purl.org/heritagedata/schemes/571/concepts/151710"/>
    <skos:narrower>
      <skos:Concept rdf:about="http://purl.org/heritagedata/schemes/571/concepts/152563">
        <skos:broader rdf:resource="http://purl.org/heritagedata/schemes/571/concepts/151667"/>
        <skos:inScheme rdf:resource="http://purl.org/heritagedata/schemes/571"/>
        <dc:identifier>http://purl.org/heritagedata/schemes/571/concepts/152563</dc:identifier>
        <dc:issued rdf:datatype="http://www.w3.org/2001/XMLSchema#dateTime">2024-07-01T17:17:33</dc:issued>
        <cc:license rdf:resource="https://www.nationalarchives.gov.uk/doc/open-government-licence/version/3/"/>
        <cc:attributionURL rdf:resource="https://historicengland.org.uk/"/>
        <cc:attributionName xml:lang="en">Historic England</cc:attributionName>
        <dc:publisher rdf:resource="https://historicengland.org.uk/"/>
        <dc:spatial rdf:resource="http://vocab.getty.edu/tgn/7002445"/>
        <dc:spatial rdf:resource="http://dbpedia.org/resource/England"/>
        <skos:prefLabel xml:lang="en">Landing Point</skos:prefLabel>
        <skos:scopeNote xml:lang="en">A place where vessels can land passengers and goods</skos:scopeNote>
      </skos:Concept>
    </skos:narrower>

    <skos:narrower>
      <skos:Concept rdf:about="http://purl.org/heritagedata/schemes/571/concepts/152564">
        <skos:broader rdf:resource="http://purl.org/heritagedata/schemes/571/concepts/151667"/>
        <skos:inScheme rdf:resource="http://purl.org/heritagedata/schemes/571"/>
        <dc:identifier>http://purl.org/heritagedata/schemes/571/concepts/152564</dc:identifier>
        <dc:issued rdf:datatype="http://www.w3.org/2001/XMLSchema#dateTime">2024-07-01T17:17:33</dc:issued>
        <cc:license rdf:resource="https://www.nationalarchives.gov.uk/doc/open-government-licence/version/3/"/>
        <cc:attributionURL rdf:resource="https://historicengland.org.uk/"/>
        <cc:attributionName xml:lang="en">Historic England</cc:attributionName>
        <dc:publisher rdf:resource="https://historicengland.org.uk/"/>
        <dc:spatial rdf:resource="http://vocab.getty.edu/tgn/7002445"/>
        <dc:spatial rdf:resource="http://dbpedia.org/resource/England"/>
        <skos:prefLabel xml:lang="en">Port</skos:prefLabel>
        <skos:scopeNote xml:lang="en">A settlement area that combines a harbour and terminal facilities at the interface between land and water transportation systems.</skos:scopeNote>
      </skos:Concept>
    </skos:narrower>

    <skos:narrower rdf:resource="http://purl.org/heritagedata/schemes/571/concepts/152587"/>
    <skos:broader rdf:resource="http://purl.org/heritagedata/schemes/571/concepts/151648"/>
    <skos:inScheme rdf:resource="http://purl.org/heritagedata/schemes/571"/>
    <dc:identifier>http://purl.org/heritagedata/schemes/571/concepts/151667</dc:identifier>
    <dc:issued rdf:datatype="http://www.w3.org/2001/XMLSchema#dateTime">2024-07-01T17:17:33</dc:issued>
    <cc:license rdf:resource="https://www.nationalarchives.gov.uk/doc/open-government-licence/version/3/"/>
    <cc:attributionURL rdf:resource="https://historicengland.org.uk/"/>
    <cc:attributionName xml:lang="en">Historic England</cc:attributionName>
    <dc:publisher rdf:resource="https://historicengland.org.uk/"/>
    <dc:spatial rdf:resource="http://vocab.getty.edu/tgn/7002445"/>
    <dc:spatial rdf:resource="http://dbpedia.org/resource/England"/>
    <skos:prefLabel xml:lang="en">Port And Dock Installation</skos:prefLabel>
    <skos:scopeNote xml:lang="en">Buildings, sites and structures associated with ports and docks together with their harbours.</skos:scopeNote>
  </skos:Concept>

  <skos:Concept rdf:about="http://purl.org/heritagedata/schemes/571/concepts/151060">
    <skos:broader rdf:resource="http://purl.org/heritagedata/schemes/571/concepts/151717"/>
    <skos:inScheme rdf:resource="http://purl.org/heritagedata/schemes/571"/>
    <dc:identifier>http://purl.org/heritagedata/schemes/571/concepts/151060</dc:identifier>
    <dc:issued rdf:datatype="http://www.w3.org/2001/XMLSchema#dateTime">2024-07-01T17:17:33</dc:issued>
    <cc:license rdf:resource="https://www.nationalarchives.gov.uk/doc/open-government-licence/version/3/"/>
    <cc:attributionURL rdf:resource="https://historicengland.org.uk/"/>
    <cc:attributionName xml:lang="en">Historic England</cc:attributionName>
    <dc:publisher rdf:resource="https://historicengland.org.uk/"/>
    <dc:spatial rdf:resource="http://vocab.getty.edu/tgn/7002445"/>
    <dc:spatial rdf:resource="http://dbpedia.org/resource/England"/>
    <skos:prefLabel xml:lang="en">Sewage Works</skos:prefLabel>
    <skos:scopeNote xml:lang="en">An area in which local sewage is filtered and purified in large rectangular or circular tanks.</skos:scopeNote>
  </skos:Concept>

  <skos:Concept rdf:about="http://purl.org/heritagedata/schemes/571/concepts/151717">
    <skos:narrower rdf:resource="http://purl.org/heritagedata/schemes/571/concepts/151060"/>
    <skos:narrower>
      <skos:Concept rdf:about="http://purl.org/heritagedata/schemes/571/concepts/151718">
        <skos:broader rdf:resource="http://purl.org/heritagedata/schemes/571/concepts/151717"/>
        <skos:inScheme rdf:resource="http://purl.org/heritagedata/schemes/571"/>
        <dc:identifier>http://purl.org/heritagedata/schemes/571/concepts/151718</dc:identifier>
        <dc:issued rdf:datatype="http://www.w3.org/2001/XMLSchema#dateTime">2024-07-01T17:17:33</dc:issued>
        <cc:license rdf:resource="https://www.nationalarchives.gov.uk/doc/open-government-licence/version/3/"/>
        <cc:attributionURL rdf:resource="https://historicengland.org.uk/"/>
        <cc:attributionName xml:lang="en">Historic England</cc:attributionName>
        <dc:publisher rdf:resource="https://historicengland.org.uk/"/>
        <dc:spatial rdf:resource="http://vocab.getty.edu/tgn/7002445"/>
        <dc:spatial rdf:resource="http://dbpedia.org/resource/England"/>
        <skos:prefLabel xml:lang="en">Landfill</skos:prefLabel>
        <skos:scopeNote xml:lang="en">A site for the disposal of waste materials by burial.</skos:scopeNote>
      </skos:Concept>
    </skos:narrower>

    <skos:narrower>
      <skos:Concept rdf:about="http://purl.org/heritagedata/schemes/571/concepts/151719">
        <skos:broader rdf:resource="http://purl.org/heritagedata/schemes/571/concepts/151717"/>
        <skos:inScheme rdf:resource="http://purl.org/heritagedata/schemes/571"/>
        <dc:identifier>http://purl.org/heritagedata/schemes/571/concepts/151719</dc:identifier>
        <dc:issued rdf:datatype="http://www.w3.org/2001/XMLSchema#dateTime">2024-07-01T17:17:33</dc:issued>
        <cc:license rdf:resource="https://www.nationalarchives.gov.uk/doc/open-government-licence/version/3/"/>
        <cc:attributionURL rdf:resource="https://historicengland.org.uk/"/>
        <cc:attributionName xml:lang="en">Historic England</cc:attributionName>
        <dc:publisher rdf:resource="https://historicengland.org.uk/"/>
        <dc:spatial rdf:resource="http://vocab.getty.edu/tgn/7002445"/>
        <dc:spatial rdf:resource="http://dbpedia.org/resource/England"/>
        <skos:prefLabel xml:lang="en">Recycling</skos:prefLabel>
        <skos:scopeNote xml:lang="en">A central point for the deposit, collection and recycling of waste materials.</skos:scopeNote>
      </skos:Concept>
    </skos:narrower>

    <skos:narrower>
      <skos:Concept rdf:about="http://purl.org/heritagedata/schemes/571/concepts/151720">
        <skos:broader rdf:resource="http://purl.org/heritagedata/schemes/571/concepts/151717"/>
        <skos:inScheme rdf:resource="http://purl.org/heritagedata/schemes/571"/>
        <dc:identifier>http://purl.org/heritagedata/schemes/571/concepts/151720</dc:identifier>
        <dc:issued rdf:datatype="http://www.w3.org/2001/XMLSchema#dateTime">2024-07-01T17:17:33</dc:issued>
        <cc:license rdf:resource="https://www.nationalarchives.gov.uk/doc/open-government-licence/version/3/"/>
        <cc:attributionURL rdf:resource="https://historicengland.org.uk/"/>
        <cc:attributionName xml:lang="en">Historic England</cc:attributionName>
        <dc:publisher rdf:resource="https://historicengland.org.uk/"/>
        <dc:spatial rdf:resource="http://vocab.getty.edu/tgn/7002445"/>
        <dc:spatial rdf:resource="http://dbpedia.org/resource/England"/>
        <skos:prefLabel xml:lang="en">Incineration Plant</skos:prefLabel>
        <skos:scopeNote xml:lang="en">A site for burning refuse to ashes using an incinerator.</skos:scopeNote>
      </skos:Concept>
    </skos:narrower>

    <skos:broader rdf:resource="http://purl.org/heritagedata/schemes/571/concepts/151460"/>
    <skos:inScheme rdf:resource="http://purl.org/heritagedata/schemes/571"/>
    <dc:identifier>http://purl.org/heritagedata/schemes/571/concepts/151717</dc:identifier>
    <dc:issued rdf:datatype="http://www.w3.org/2001/XMLSchema#dateTime">2024-07-01T17:17:33</dc:issued>
    <cc:license rdf:resource="https://www.nationalarchives.gov.uk/doc/open-government-licence/version/3/"/>
    <cc:attributionURL rdf:resource="https://historicengland.org.uk/"/>
    <cc:attributionName xml:lang="en">Historic England</cc:attributionName>
    <dc:publisher rdf:resource="https://historicengland.org.uk/"/>
    <dc:spatial rdf:resource="http://vocab.getty.edu/tgn/7002445"/>
    <dc:spatial rdf:resource="http://dbpedia.org/resource/England"/>
    <skos:prefLabel xml:lang="en">Waste Disposal</skos:prefLabel>
    <skos:scopeNote xml:lang="en">Buildings, sites and structures associated with the disposal of domestic and industrial waste.</skos:scopeNote>
  </skos:Concept>

  <skos:Concept rdf:about="http://purl.org/heritagedata/schemes/571/concepts/151062">
    <skos:broader rdf:resource="http://purl.org/heritagedata/schemes/571/concepts/151696"/>
    <skos:inScheme rdf:resource="http://purl.org/heritagedata/schemes/571"/>
    <dc:identifier>http://purl.org/heritagedata/schemes/571/concepts/151062</dc:identifier>
    <dc:issued rdf:datatype="http://www.w3.org/2001/XMLSchema#dateTime">2024-07-01T17:17:33</dc:issued>
    <cc:license rdf:resource="https://www.nationalarchives.gov.uk/doc/open-government-licence/version/3/"/>
    <cc:attributionURL rdf:resource="https://historicengland.org.uk/"/>
    <cc:attributionName xml:lang="en">Historic England</cc:attributionName>
    <dc:publisher rdf:resource="https://historicengland.org.uk/"/>
    <dc:spatial rdf:resource="http://vocab.getty.edu/tgn/7002445"/>
    <dc:spatial rdf:resource="http://dbpedia.org/resource/England"/>
    <skos:prefLabel xml:lang="en">City Hall</skos:prefLabel>
    <skos:related rdf:resource="http://purl.org/heritagedata/schemes/571/concepts/151577"/>
    <skos:related rdf:resource="http://purl.org/heritagedata/schemes/571/concepts/151064"/>
    <skos:scopeNote xml:lang="en">A large building, often with directly associated and usually defined grounds, used for the transaction of the public business of a city, the holding of courts of justice, entertainments and other activities.</skos:scopeNote>
  </skos:Concept>

  <skos:Concept rdf:about="http://purl.org/heritagedata/schemes/571/concepts/151696">
    <skos:narrower rdf:resource="http://purl.org/heritagedata/schemes/571/concepts/151062"/>
    <skos:narrower rdf:resource="http://purl.org/heritagedata/schemes/571/concepts/151063"/>
    <skos:narrower rdf:resource="http://purl.org/heritagedata/schemes/571/concepts/151064"/>
    <skos:narrower rdf:resource="http://purl.org/heritagedata/schemes/571/concepts/151700"/>
    <skos:broader rdf:resource="http://purl.org/heritagedata/schemes/571/concepts/151459"/>
    <skos:inScheme rdf:resource="http://purl.org/heritagedata/schemes/571"/>
    <dc:identifier>http://purl.org/heritagedata/schemes/571/concepts/151696</dc:identifier>
    <dc:issued rdf:datatype="http://www.w3.org/2001/XMLSchema#dateTime">2024-07-01T17:17:33</dc:issued>
    <cc:license rdf:resource="https://www.nationalarchives.gov.uk/doc/open-government-licence/version/3/"/>
    <cc:attributionURL rdf:resource="https://historicengland.org.uk/"/>
    <cc:attributionName xml:lang="en">Historic England</cc:attributionName>
    <dc:publisher rdf:resource="https://historicengland.org.uk/"/>
    <dc:spatial rdf:resource="http://vocab.getty.edu/tgn/7002445"/>
    <dc:spatial rdf:resource="http://dbpedia.org/resource/England"/>
    <skos:prefLabel xml:lang="en">Civil</skos:prefLabel>
    <skos:scopeNote xml:lang="en">Institutions of government that support civil behaviour or habits of personal living which then cement viable relations between individuals and wider society.</skos:scopeNote>
  </skos:Concept>

  <skos:Concept rdf:about="http://purl.org/heritagedata/schemes/571/concepts/151063">
    <skos:broader rdf:resource="http://purl.org/heritagedata/schemes/571/concepts/151696"/>
    <skos:inScheme rdf:resource="http://purl.org/heritagedata/schemes/571"/>
    <dc:identifier>http://purl.org/heritagedata/schemes/571/concepts/151063</dc:identifier>
    <dc:issued rdf:datatype="http://www.w3.org/2001/XMLSchema#dateTime">2024-07-01T17:17:33</dc:issued>
    <cc:license rdf:resource="https://www.nationalarchives.gov.uk/doc/open-government-licence/version/3/"/>
    <cc:attributionURL rdf:resource="https://historicengland.org.uk/"/>
    <cc:attributionName xml:lang="en">Historic England</cc:attributionName>
    <dc:publisher rdf:resource="https://historicengland.org.uk/"/>
    <dc:spatial rdf:resource="http://vocab.getty.edu/tgn/7002445"/>
    <dc:spatial rdf:resource="http://dbpedia.org/resource/England"/>
    <skos:prefLabel xml:lang="en">Town Hall</skos:prefLabel>
    <skos:related rdf:resource="http://purl.org/heritagedata/schemes/571/concepts/151064"/>
    <skos:scopeNote xml:lang="en">A large building and directly associated and usually defined grounds used for the transaction of the public business of a town, the holding of courts of justice, entertainments and other activities.</skos:scopeNote>
  </skos:Concept>

  <skos:Concept rdf:about="http://purl.org/heritagedata/schemes/571/concepts/151064">
    <skos:broader rdf:resource="http://purl.org/heritagedata/schemes/571/concepts/151696"/>
    <skos:inScheme rdf:resource="http://purl.org/heritagedata/schemes/571"/>
    <dc:identifier>http://purl.org/heritagedata/schemes/571/concepts/151064</dc:identifier>
    <dc:issued rdf:datatype="http://www.w3.org/2001/XMLSchema#dateTime">2024-07-01T17:17:33</dc:issued>
    <cc:license rdf:resource="https://www.nationalarchives.gov.uk/doc/open-government-licence/version/3/"/>
    <cc:attributionURL rdf:resource="https://historicengland.org.uk/"/>
    <cc:attributionName xml:lang="en">Historic England</cc:attributionName>
    <dc:publisher rdf:resource="https://historicengland.org.uk/"/>
    <dc:spatial rdf:resource="http://vocab.getty.edu/tgn/7002445"/>
    <dc:spatial rdf:resource="http://dbpedia.org/resource/England"/>
    <skos:prefLabel xml:lang="en">Civic Centre</skos:prefLabel>
    <skos:related rdf:resource="http://purl.org/heritagedata/schemes/571/concepts/151062"/>
    <skos:related rdf:resource="http://purl.org/heritagedata/schemes/571/concepts/151063"/>
    <skos:scopeNote xml:lang="en">A building or complex often with several buildings where municipal offices and other public buildings are situated.</skos:scopeNote>
  </skos:Concept>

  <skos:Concept rdf:about="http://purl.org/heritagedata/schemes/571/concepts/151065">
    <skos:broader rdf:resource="http://purl.org/heritagedata/schemes/571/concepts/151697"/>
    <skos:inScheme rdf:resource="http://purl.org/heritagedata/schemes/571"/>
    <dc:identifier>http://purl.org/heritagedata/schemes/571/concepts/151065</dc:identifier>
    <dc:issued rdf:datatype="http://www.w3.org/2001/XMLSchema#dateTime">2024-07-01T17:17:33</dc:issued>
    <cc:license rdf:resource="https://www.nationalarchives.gov.uk/doc/open-government-licence/version/3/"/>
    <cc:attributionURL rdf:resource="https://historicengland.org.uk/"/>
    <cc:attributionName xml:lang="en">Historic England</cc:attributionName>
    <dc:publisher rdf:resource="https://historicengland.org.uk/"/>
    <dc:spatial rdf:resource="http://vocab.getty.edu/tgn/7002445"/>
    <dc:spatial rdf:resource="http://dbpedia.org/resource/England"/>
    <skos:prefLabel xml:lang="en">School</skos:prefLabel>
    <skos:scopeNote xml:lang="en">Primary and secondary educational establishments, buildings and directly associated and usually defined grounds, including car parking etc.</skos:scopeNote>
  </skos:Concept>

  <skos:Concept rdf:about="http://purl.org/heritagedata/schemes/571/concepts/151697">
    <skos:narrower rdf:resource="http://purl.org/heritagedata/schemes/571/concepts/151065"/>
    <skos:narrower>
      <skos:Concept rdf:about="http://purl.org/heritagedata/schemes/571/concepts/151066">
        <skos:broader rdf:resource="http://purl.org/heritagedata/schemes/571/concepts/151697"/>
        <skos:inScheme rdf:resource="http://purl.org/heritagedata/schemes/571"/>
        <dc:identifier>http://purl.org/heritagedata/schemes/571/concepts/151066</dc:identifier>
        <dc:issued rdf:datatype="http://www.w3.org/2001/XMLSchema#dateTime">2024-07-01T17:17:33</dc:issued>
        <cc:license rdf:resource="https://www.nationalarchives.gov.uk/doc/open-government-licence/version/3/"/>
        <cc:attributionURL rdf:resource="https://historicengland.org.uk/"/>
        <cc:attributionName xml:lang="en">Historic England</cc:attributionName>
        <dc:publisher rdf:resource="https://historicengland.org.uk/"/>
        <dc:spatial rdf:resource="http://vocab.getty.edu/tgn/7002445"/>
        <dc:spatial rdf:resource="http://dbpedia.org/resource/England"/>
        <skos:prefLabel xml:lang="en">University Campus</skos:prefLabel>
        <skos:scopeNote xml:lang="en">Educational establishments awarding degrees and undertaking research. Includes buildings and directly associated and usually defined grounds.</skos:scopeNote>
      </skos:Concept>
    </skos:narrower>

    <skos:narrower>
      <skos:Concept rdf:about="http://purl.org/heritagedata/schemes/571/concepts/151067">
        <skos:broader rdf:resource="http://purl.org/heritagedata/schemes/571/concepts/151697"/>
        <skos:inScheme rdf:resource="http://purl.org/heritagedata/schemes/571"/>
        <dc:identifier>http://purl.org/heritagedata/schemes/571/concepts/151067</dc:identifier>
        <dc:issued rdf:datatype="http://www.w3.org/2001/XMLSchema#dateTime">2024-07-01T17:17:33</dc:issued>
        <cc:license rdf:resource="https://www.nationalarchives.gov.uk/doc/open-government-licence/version/3/"/>
        <cc:attributionURL rdf:resource="https://historicengland.org.uk/"/>
        <cc:attributionName xml:lang="en">Historic England</cc:attributionName>
        <dc:publisher rdf:resource="https://historicengland.org.uk/"/>
        <dc:spatial rdf:resource="http://vocab.getty.edu/tgn/7002445"/>
        <dc:spatial rdf:resource="http://dbpedia.org/resource/England"/>
        <skos:prefLabel xml:lang="en">College Campus</skos:prefLabel>
        <skos:scopeNote xml:lang="en">Buildings and grounds of secondary or tertiary educational establishments, below the status of universities.</skos:scopeNote>
      </skos:Concept>
    </skos:narrower>

    <skos:narrower>
      <skos:Concept rdf:about="http://purl.org/heritagedata/schemes/571/concepts/151703">
        <skos:broader rdf:resource="http://purl.org/heritagedata/schemes/571/concepts/151697"/>
        <skos:inScheme rdf:resource="http://purl.org/heritagedata/schemes/571"/>
        <dc:identifier>http://purl.org/heritagedata/schemes/571/concepts/151703</dc:identifier>
        <dc:issued rdf:datatype="http://www.w3.org/2001/XMLSchema#dateTime">2024-07-01T17:17:33</dc:issued>
        <cc:license rdf:resource="https://www.nationalarchives.gov.uk/doc/open-government-licence/version/3/"/>
        <cc:attributionURL rdf:resource="https://historicengland.org.uk/"/>
        <cc:attributionName xml:lang="en">Historic England</cc:attributionName>
        <dc:publisher rdf:resource="https://historicengland.org.uk/"/>
        <dc:spatial rdf:resource="http://vocab.getty.edu/tgn/7002445"/>
        <dc:spatial rdf:resource="http://dbpedia.org/resource/England"/>
        <skos:prefLabel xml:lang="en">Library Complex</skos:prefLabel>
        <skos:scopeNote xml:lang="en">A building, room or suite of rooms where books, or other materials, are classified by subject and stored for use by the library's members. Includes directly associated and usually defined grounds.</skos:scopeNote>
      </skos:Concept>
    </skos:narrower>

    <skos:narrower rdf:resource="http://purl.org/heritagedata/schemes/571/concepts/151704"/>
    <skos:narrower rdf:resource="http://purl.org/heritagedata/schemes/571/concepts/151705"/>
    <skos:broader rdf:resource="http://purl.org/heritagedata/schemes/571/concepts/151459"/>
    <skos:inScheme rdf:resource="http://purl.org/heritagedata/schemes/571"/>
    <dc:identifier>http://purl.org/heritagedata/schemes/571/concepts/151697</dc:identifier>
    <dc:issued rdf:datatype="http://www.w3.org/2001/XMLSchema#dateTime">2024-07-01T17:17:33</dc:issued>
    <cc:license rdf:resource="https://www.nationalarchives.gov.uk/doc/open-government-licence/version/3/"/>
    <cc:attributionURL rdf:resource="https://historicengland.org.uk/"/>
    <cc:attributionName xml:lang="en">Historic England</cc:attributionName>
    <dc:publisher rdf:resource="https://historicengland.org.uk/"/>
    <dc:spatial rdf:resource="http://vocab.getty.edu/tgn/7002445"/>
    <dc:spatial rdf:resource="http://dbpedia.org/resource/England"/>
    <skos:prefLabel xml:lang="en">Education</skos:prefLabel>
    <skos:scopeNote xml:lang="en">Provision of teaching and related material intended to have a formative, and often also a normative effect on the mind, character and abilities of an individual.</skos:scopeNote>
  </skos:Concept>

  <skos:Concept rdf:about="http://purl.org/heritagedata/schemes/571/concepts/151068">
    <skos:broader rdf:resource="http://purl.org/heritagedata/schemes/571/concepts/151698"/>
    <skos:inScheme rdf:resource="http://purl.org/heritagedata/schemes/571"/>
    <dc:identifier>http://purl.org/heritagedata/schemes/571/concepts/151068</dc:identifier>
    <dc:issued rdf:datatype="http://www.w3.org/2001/XMLSchema#dateTime">2024-07-01T17:17:33</dc:issued>
    <cc:license rdf:resource="https://www.nationalarchives.gov.uk/doc/open-government-licence/version/3/"/>
    <cc:attributionURL rdf:resource="https://historicengland.org.uk/"/>
    <cc:attributionName xml:lang="en">Historic England</cc:attributionName>
    <dc:publisher rdf:resource="https://historicengland.org.uk/"/>
    <dc:spatial rdf:resource="http://vocab.getty.edu/tgn/7002445"/>
    <dc:spatial rdf:resource="http://dbpedia.org/resource/England"/>
    <skos:prefLabel xml:lang="en">Hospital</skos:prefLabel>
    <skos:scopeNote xml:lang="en">Establishment (buildings and directly associated grounds) providing care to casualties and the seriously or chronically ill.</skos:scopeNote>
  </skos:Concept>

  <skos:Concept rdf:about="http://purl.org/heritagedata/schemes/571/concepts/151698">
    <skos:narrower rdf:resource="http://purl.org/heritagedata/schemes/571/concepts/151068"/>
    <skos:narrower rdf:resource="http://purl.org/heritagedata/schemes/571/concepts/151604"/>
    <skos:broader rdf:resource="http://purl.org/heritagedata/schemes/571/concepts/151459"/>
    <skos:inScheme rdf:resource="http://purl.org/heritagedata/schemes/571"/>
    <dc:identifier>http://purl.org/heritagedata/schemes/571/concepts/151698</dc:identifier>
    <dc:issued rdf:datatype="http://www.w3.org/2001/XMLSchema#dateTime">2024-07-01T17:17:33</dc:issued>
    <cc:license rdf:resource="https://www.nationalarchives.gov.uk/doc/open-government-licence/version/3/"/>
    <cc:attributionURL rdf:resource="https://historicengland.org.uk/"/>
    <cc:attributionName xml:lang="en">Historic England</cc:attributionName>
    <dc:publisher rdf:resource="https://historicengland.org.uk/"/>
    <dc:spatial rdf:resource="http://vocab.getty.edu/tgn/7002445"/>
    <dc:spatial rdf:resource="http://dbpedia.org/resource/England"/>
    <skos:prefLabel xml:lang="en">Health</skos:prefLabel>
    <skos:scopeNote xml:lang="en">Helping individuals maintain a satisfactory condition of mind and body, and freedom from sickness, injury and pain.</skos:scopeNote>
  </skos:Concept>

  <skos:Concept rdf:about="http://purl.org/heritagedata/schemes/571/concepts/151069">
    <skos:broader rdf:resource="http://purl.org/heritagedata/schemes/571/concepts/151459"/>
    <skos:inScheme rdf:resource="http://purl.org/heritagedata/schemes/571"/>
    <dc:identifier>http://purl.org/heritagedata/schemes/571/concepts/151069</dc:identifier>
    <dc:issued rdf:datatype="http://www.w3.org/2001/XMLSchema#dateTime">2024-07-01T17:17:33</dc:issued>
    <cc:license rdf:resource="https://www.nationalarchives.gov.uk/doc/open-government-licence/version/3/"/>
    <cc:attributionURL rdf:resource="https://historicengland.org.uk/"/>
    <cc:attributionName xml:lang="en">Historic England</cc:attributionName>
    <dc:publisher rdf:resource="https://historicengland.org.uk/"/>
    <dc:spatial rdf:resource="http://vocab.getty.edu/tgn/7002445"/>
    <dc:spatial rdf:resource="http://dbpedia.org/resource/England"/>
    <skos:prefLabel xml:lang="en">Workhouse</skos:prefLabel>
    <skos:scopeNote xml:lang="en">Establishment (buildings and directly associated and usually defined grounds) where the community's poor were maintained at public expense, and provided with labour.</skos:scopeNote>
  </skos:Concept>

  <skos:Concept rdf:about="http://purl.org/heritagedata/schemes/571/concepts/151459">
    <skos:narrower rdf:resource="http://purl.org/heritagedata/schemes/571/concepts/151069"/>
    <skos:narrower>
      <skos:Concept rdf:about="http://purl.org/heritagedata/schemes/571/concepts/151184">
        <skos:broader rdf:resource="http://purl.org/heritagedata/schemes/571/concepts/151459"/>
        <skos:inScheme rdf:resource="http://purl.org/heritagedata/schemes/571"/>
        <dc:identifier>http://purl.org/heritagedata/schemes/571/concepts/151184</dc:identifier>
        <dc:issued rdf:datatype="http://www.w3.org/2001/XMLSchema#dateTime">2024-07-01T17:17:33</dc:issued>
        <cc:license rdf:resource="https://www.nationalarchives.gov.uk/doc/open-government-licence/version/3/"/>
        <cc:attributionURL rdf:resource="https://historicengland.org.uk/"/>
        <cc:attributionName xml:lang="en">Historic England</cc:attributionName>
        <dc:publisher rdf:resource="https://historicengland.org.uk/"/>
        <dc:spatial rdf:resource="http://vocab.getty.edu/tgn/7002445"/>
        <dc:spatial rdf:resource="http://dbpedia.org/resource/England"/>
        <skos:prefLabel xml:lang="en">Prison</skos:prefLabel>
        <skos:scopeNote xml:lang="en">An establishment (buildings and directly associated and usually defined grounds) where offenders are confined.</skos:scopeNote>
      </skos:Concept>
    </skos:narrower>

    <skos:narrower rdf:resource="http://purl.org/heritagedata/schemes/571/concepts/151696"/>
    <skos:narrower rdf:resource="http://purl.org/heritagedata/schemes/571/concepts/151697"/>
    <skos:narrower rdf:resource="http://purl.org/heritagedata/schemes/571/concepts/151698"/>
    <skos:narrower rdf:resource="http://purl.org/heritagedata/schemes/571/concepts/160129"/>
    <skos:narrower rdf:resource="http://purl.org/heritagedata/schemes/571/concepts/160130"/>
    <skos:inScheme rdf:resource="http://purl.org/heritagedata/schemes/571"/>
    <dc:identifier>http://purl.org/heritagedata/schemes/571/concepts/151459</dc:identifier>
    <dc:issued rdf:datatype="http://www.w3.org/2001/XMLSchema#dateTime">2024-07-01T17:17:33</dc:issued>
    <cc:license rdf:resource="https://www.nationalarchives.gov.uk/doc/open-government-licence/version/3/"/>
    <cc:attributionURL rdf:resource="https://historicengland.org.uk/"/>
    <cc:attributionName xml:lang="en">Historic England</cc:attributionName>
    <dc:publisher rdf:resource="https://historicengland.org.uk/"/>
    <dc:spatial rdf:resource="http://vocab.getty.edu/tgn/7002445"/>
    <dc:spatial rdf:resource="http://dbpedia.org/resource/England"/>
    <skos:prefLabel xml:lang="en">Civic Provision</skos:prefLabel>
    <skos:scopeNote xml:lang="en">-</skos:scopeNote>
    <skos:topConceptOf rdf:resource="http://purl.org/heritagedata/schemes/571"/>
  </skos:Concept>

  <skos:Concept rdf:about="http://purl.org/heritagedata/schemes/571/concepts/151070">
    <skos:broader rdf:resource="http://purl.org/heritagedata/schemes/571/concepts/160129"/>
    <skos:inScheme rdf:resource="http://purl.org/heritagedata/schemes/571"/>
    <dc:identifier>http://purl.org/heritagedata/schemes/571/concepts/151070</dc:identifier>
    <dc:issued rdf:datatype="http://www.w3.org/2001/XMLSchema#dateTime">2024-07-01T17:17:33</dc:issued>
    <cc:license rdf:resource="https://www.nationalarchives.gov.uk/doc/open-government-licence/version/3/"/>
    <cc:attributionURL rdf:resource="https://historicengland.org.uk/"/>
    <cc:attributionName xml:lang="en">Historic England</cc:attributionName>
    <dc:publisher rdf:resource="https://historicengland.org.uk/"/>
    <dc:spatial rdf:resource="http://vocab.getty.edu/tgn/7002445"/>
    <dc:spatial rdf:resource="http://dbpedia.org/resource/England"/>
    <skos:prefLabel xml:lang="en">Cemetery</skos:prefLabel>
    <skos:related rdf:resource="http://purl.org/heritagedata/schemes/571/concepts/151075"/>
    <skos:scopeNote xml:lang="en">Place, usually defined, where the dead are carefully and respectfully placed, usually via interment.</skos:scopeNote>
  </skos:Concept>

  <skos:Concept rdf:about="http://purl.org/heritagedata/schemes/571/concepts/160129">
    <skos:narrower rdf:resource="http://purl.org/heritagedata/schemes/571/concepts/151070"/>
    <skos:narrower>
      <skos:Concept rdf:about="http://purl.org/heritagedata/schemes/571/concepts/160128">
        <skos:broader rdf:resource="http://purl.org/heritagedata/schemes/571/concepts/160129"/>
        <skos:inScheme rdf:resource="http://purl.org/heritagedata/schemes/571"/>
        <dc:identifier>http://purl.org/heritagedata/schemes/571/concepts/160128</dc:identifier>
        <dc:issued rdf:datatype="http://www.w3.org/2001/XMLSchema#dateTime">2024-07-01T17:17:33</dc:issued>
        <cc:license rdf:resource="https://www.nationalarchives.gov.uk/doc/open-government-licence/version/3/"/>
        <cc:attributionURL rdf:resource="https://historicengland.org.uk/"/>
        <cc:attributionName xml:lang="en">Historic England</cc:attributionName>
        <dc:publisher rdf:resource="https://historicengland.org.uk/"/>
        <dc:spatial rdf:resource="http://vocab.getty.edu/tgn/7002445"/>
        <dc:spatial rdf:resource="http://dbpedia.org/resource/England"/>
        <skos:prefLabel xml:lang="en">Crematorium Complex</skos:prefLabel>
        <skos:scopeNote xml:lang="en">Place (building and grounds) where the dead are respectfully incinerated and remembered.</skos:scopeNote>
      </skos:Concept>
    </skos:narrower>

    <skos:broader rdf:resource="http://purl.org/heritagedata/schemes/571/concepts/151459"/>
    <skos:inScheme rdf:resource="http://purl.org/heritagedata/schemes/571"/>
    <dc:identifier>http://purl.org/heritagedata/schemes/571/concepts/160129</dc:identifier>
    <dc:issued rdf:datatype="http://www.w3.org/2001/XMLSchema#dateTime">2024-07-01T17:17:33</dc:issued>
    <cc:license rdf:resource="https://www.nationalarchives.gov.uk/doc/open-government-licence/version/3/"/>
    <cc:attributionURL rdf:resource="https://historicengland.org.uk/"/>
    <cc:attributionName xml:lang="en">Historic England</cc:attributionName>
    <dc:publisher rdf:resource="https://historicengland.org.uk/"/>
    <dc:spatial rdf:resource="http://vocab.getty.edu/tgn/7002445"/>
    <dc:spatial rdf:resource="http://dbpedia.org/resource/England"/>
    <skos:prefLabel xml:lang="en">Funerary</skos:prefLabel>
    <skos:scopeNote xml:lang="en">Related to respectful disposal of the bodies of the dead.</skos:scopeNote>
  </skos:Concept>

  <skos:Concept rdf:about="http://purl.org/heritagedata/schemes/571/concepts/151072">
    <skos:broader rdf:resource="http://purl.org/heritagedata/schemes/571/concepts/151707"/>
    <skos:inScheme rdf:resource="http://purl.org/heritagedata/schemes/571"/>
    <dc:identifier>http://purl.org/heritagedata/schemes/571/concepts/151072</dc:identifier>
    <dc:issued rdf:datatype="http://www.w3.org/2001/XMLSchema#dateTime">2024-07-01T17:17:33</dc:issued>
    <cc:license rdf:resource="https://www.nationalarchives.gov.uk/doc/open-government-licence/version/3/"/>
    <cc:attributionURL rdf:resource="https://historicengland.org.uk/"/>
    <cc:attributionName xml:lang="en">Historic England</cc:attributionName>
    <dc:publisher rdf:resource="https://historicengland.org.uk/"/>
    <dc:spatial rdf:resource="http://vocab.getty.edu/tgn/7002445"/>
    <dc:spatial rdf:resource="http://dbpedia.org/resource/England"/>
    <skos:prefLabel xml:lang="en">Chapel</skos:prefLabel>
    <skos:scopeNote xml:lang="en">Place of Christian worship; can include non-conformist (and non-parochial) churches (q.v.) and privately owned chapels. Includes immediately associated and usually physically defined land.</skos:scopeNote>
  </skos:Concept>

  <skos:Concept rdf:about="http://purl.org/heritagedata/schemes/571/concepts/151707">
    <skos:narrower rdf:resource="http://purl.org/heritagedata/schemes/571/concepts/151072"/>
    <skos:narrower>
      <skos:Concept rdf:about="http://purl.org/heritagedata/schemes/571/concepts/151073">
        <skos:broader rdf:resource="http://purl.org/heritagedata/schemes/571/concepts/151707"/>
        <skos:inScheme rdf:resource="http://purl.org/heritagedata/schemes/571"/>
        <dc:identifier>http://purl.org/heritagedata/schemes/571/concepts/151073</dc:identifier>
        <dc:issued rdf:datatype="http://www.w3.org/2001/XMLSchema#dateTime">2024-07-01T17:17:33</dc:issued>
        <cc:license rdf:resource="https://www.nationalarchives.gov.uk/doc/open-government-licence/version/3/"/>
        <cc:attributionURL rdf:resource="https://historicengland.org.uk/"/>
        <cc:attributionName xml:lang="en">Historic England</cc:attributionName>
        <dc:publisher rdf:resource="https://historicengland.org.uk/"/>
        <dc:spatial rdf:resource="http://vocab.getty.edu/tgn/7002445"/>
        <dc:spatial rdf:resource="http://dbpedia.org/resource/England"/>
        <skos:prefLabel xml:lang="en">Mosque</skos:prefLabel>
        <skos:scopeNote xml:lang="en">Place (buildings and directly associated, usually defined, grounds) of Islamist or Mohammedan worship.</skos:scopeNote>
      </skos:Concept>
    </skos:narrower>

    <skos:narrower>
      <skos:Concept rdf:about="http://purl.org/heritagedata/schemes/571/concepts/151074">
        <skos:broader rdf:resource="http://purl.org/heritagedata/schemes/571/concepts/151707"/>
        <skos:inScheme rdf:resource="http://purl.org/heritagedata/schemes/571"/>
        <dc:identifier>http://purl.org/heritagedata/schemes/571/concepts/151074</dc:identifier>
        <dc:issued rdf:datatype="http://www.w3.org/2001/XMLSchema#dateTime">2024-07-01T17:17:33</dc:issued>
        <cc:license rdf:resource="https://www.nationalarchives.gov.uk/doc/open-government-licence/version/3/"/>
        <cc:attributionURL rdf:resource="https://historicengland.org.uk/"/>
        <cc:attributionName xml:lang="en">Historic England</cc:attributionName>
        <dc:publisher rdf:resource="https://historicengland.org.uk/"/>
        <dc:spatial rdf:resource="http://vocab.getty.edu/tgn/7002445"/>
        <dc:spatial rdf:resource="http://dbpedia.org/resource/England"/>
        <skos:prefLabel xml:lang="en">Synagogue</skos:prefLabel>
        <skos:scopeNote xml:lang="en">Place of worship (buildings and directly associated and usually defined grounds) for communities of Jews.</skos:scopeNote>
      </skos:Concept>
    </skos:narrower>

    <skos:narrower rdf:resource="http://purl.org/heritagedata/schemes/571/concepts/151075"/>
    <skos:narrower rdf:resource="http://purl.org/heritagedata/schemes/571/concepts/151708"/>
    <skos:narrower>
      <skos:Concept rdf:about="http://purl.org/heritagedata/schemes/571/concepts/151709">
        <skos:broader rdf:resource="http://purl.org/heritagedata/schemes/571/concepts/151707"/>
        <skos:inScheme rdf:resource="http://purl.org/heritagedata/schemes/571"/>
        <dc:identifier>http://purl.org/heritagedata/schemes/571/concepts/151709</dc:identifier>
        <dc:issued rdf:datatype="http://www.w3.org/2001/XMLSchema#dateTime">2024-07-01T17:17:33</dc:issued>
        <cc:license rdf:resource="https://www.nationalarchives.gov.uk/doc/open-government-licence/version/3/"/>
        <cc:attributionURL rdf:resource="https://historicengland.org.uk/"/>
        <cc:attributionName xml:lang="en">Historic England</cc:attributionName>
        <dc:publisher rdf:resource="https://historicengland.org.uk/"/>
        <dc:spatial rdf:resource="http://vocab.getty.edu/tgn/7002445"/>
        <dc:spatial rdf:resource="http://dbpedia.org/resource/England"/>
        <skos:prefLabel xml:lang="en">Friends Meeting House</skos:prefLabel>
        <skos:scopeNote xml:lang="en">A place of worship, building and directly associated, often defined, grounds for members of the Society of Friends, a denomination founded by George Fox in c.1650 who believed in pacifist principles and a rejection of the sacrament.</skos:scopeNote>
      </skos:Concept>
    </skos:narrower>

    <skos:broader rdf:resource="http://purl.org/heritagedata/schemes/571/concepts/160130"/>
    <skos:inScheme rdf:resource="http://purl.org/heritagedata/schemes/571"/>
    <dc:identifier>http://purl.org/heritagedata/schemes/571/concepts/151707</dc:identifier>
    <dc:issued rdf:datatype="http://www.w3.org/2001/XMLSchema#dateTime">2024-07-01T17:17:33</dc:issued>
    <cc:license rdf:resource="https://www.nationalarchives.gov.uk/doc/open-government-licence/version/3/"/>
    <cc:attributionURL rdf:resource="https://historicengland.org.uk/"/>
    <cc:attributionName xml:lang="en">Historic England</cc:attributionName>
    <dc:publisher rdf:resource="https://historicengland.org.uk/"/>
    <dc:spatial rdf:resource="http://vocab.getty.edu/tgn/7002445"/>
    <dc:spatial rdf:resource="http://dbpedia.org/resource/England"/>
    <skos:prefLabel xml:lang="en">Place Of Worship</skos:prefLabel>
    <skos:scopeNote xml:lang="en">A place (buildings and directly associated and usually defined grounds) where appropriate acts, rites and ceremonies are performed to honour or revere a supernatural being, power or holy entity. Use specific type where known.</skos:scopeNote>
  </skos:Concept>

  <skos:Concept rdf:about="http://purl.org/heritagedata/schemes/571/concepts/151075">
    <skos:broader rdf:resource="http://purl.org/heritagedata/schemes/571/concepts/151707"/>
    <skos:inScheme rdf:resource="http://purl.org/heritagedata/schemes/571"/>
    <dc:identifier>http://purl.org/heritagedata/schemes/571/concepts/151075</dc:identifier>
    <dc:issued rdf:datatype="http://www.w3.org/2001/XMLSchema#dateTime">2024-07-01T17:17:33</dc:issued>
    <cc:license rdf:resource="https://www.nationalarchives.gov.uk/doc/open-government-licence/version/3/"/>
    <cc:attributionURL rdf:resource="https://historicengland.org.uk/"/>
    <cc:attributionName xml:lang="en">Historic England</cc:attributionName>
    <dc:publisher rdf:resource="https://historicengland.org.uk/"/>
    <dc:spatial rdf:resource="http://vocab.getty.edu/tgn/7002445"/>
    <dc:spatial rdf:resource="http://dbpedia.org/resource/England"/>
    <skos:prefLabel xml:lang="en">Church</skos:prefLabel>
    <skos:related rdf:resource="http://purl.org/heritagedata/schemes/571/concepts/151070"/>
    <skos:scopeNote xml:lang="en">Place of Christian worship, usually serving a parish. includes churchyard and immediately related features.</skos:scopeNote>
  </skos:Concept>

  <skos:Concept rdf:about="http://purl.org/heritagedata/schemes/571/concepts/151076">
    <skos:broader rdf:resource="http://purl.org/heritagedata/schemes/571/concepts/151458"/>
    <skos:inScheme rdf:resource="http://purl.org/heritagedata/schemes/571"/>
    <dc:identifier>http://purl.org/heritagedata/schemes/571/concepts/151076</dc:identifier>
    <dc:issued rdf:datatype="http://www.w3.org/2001/XMLSchema#dateTime">2024-07-01T17:17:33</dc:issued>
    <cc:license rdf:resource="https://www.nationalarchives.gov.uk/doc/open-government-licence/version/3/"/>
    <cc:attributionURL rdf:resource="https://historicengland.org.uk/"/>
    <cc:attributionName xml:lang="en">Historic England</cc:attributionName>
    <dc:publisher rdf:resource="https://historicengland.org.uk/"/>
    <dc:spatial rdf:resource="http://vocab.getty.edu/tgn/7002445"/>
    <dc:spatial rdf:resource="http://dbpedia.org/resource/England"/>
    <skos:prefLabel xml:lang="en">Shopping Street</skos:prefLabel>
    <skos:scopeNote xml:lang="en">Street (often with associated back yards etc) predominantly fitted with retail outlets.</skos:scopeNote>
  </skos:Concept>

  <skos:Concept rdf:about="http://purl.org/heritagedata/schemes/571/concepts/151458">
    <skos:narrower rdf:resource="http://purl.org/heritagedata/schemes/571/concepts/151076"/>
    <skos:narrower rdf:resource="http://purl.org/heritagedata/schemes/571/concepts/151077"/>
    <skos:narrower rdf:resource="http://purl.org/heritagedata/schemes/571/concepts/151078"/>
    <skos:narrower>
      <skos:Concept rdf:about="http://purl.org/heritagedata/schemes/571/concepts/151080">
        <skos:broader rdf:resource="http://purl.org/heritagedata/schemes/571/concepts/151458"/>
        <skos:inScheme rdf:resource="http://purl.org/heritagedata/schemes/571"/>
        <dc:identifier>http://purl.org/heritagedata/schemes/571/concepts/151080</dc:identifier>
        <dc:issued rdf:datatype="http://www.w3.org/2001/XMLSchema#dateTime">2024-07-01T17:17:33</dc:issued>
        <cc:license rdf:resource="https://www.nationalarchives.gov.uk/doc/open-government-licence/version/3/"/>
        <cc:attributionURL rdf:resource="https://historicengland.org.uk/"/>
        <cc:attributionName xml:lang="en">Historic England</cc:attributionName>
        <dc:publisher rdf:resource="https://historicengland.org.uk/"/>
        <dc:spatial rdf:resource="http://vocab.getty.edu/tgn/7002445"/>
        <dc:spatial rdf:resource="http://dbpedia.org/resource/England"/>
        <skos:prefLabel xml:lang="en">Garden Centre</skos:prefLabel>
        <skos:scopeNote xml:lang="en">A place, buildings and directly associated grounds, where gardening tools, plants, etc, are sold.</skos:scopeNote>
      </skos:Concept>
    </skos:narrower>

    <skos:narrower rdf:resource="http://purl.org/heritagedata/schemes/571/concepts/151610"/>
    <skos:narrower rdf:resource="http://purl.org/heritagedata/schemes/571/concepts/151766"/>
    <skos:narrower rdf:resource="http://purl.org/heritagedata/schemes/571/concepts/160132"/>
    <skos:narrower rdf:resource="http://purl.org/heritagedata/schemes/571/concepts/160133"/>
    <skos:inScheme rdf:resource="http://purl.org/heritagedata/schemes/571"/>
    <dc:identifier>http://purl.org/heritagedata/schemes/571/concepts/151458</dc:identifier>
    <dc:issued rdf:datatype="http://www.w3.org/2001/XMLSchema#dateTime">2024-07-01T17:17:33</dc:issued>
    <cc:license rdf:resource="https://www.nationalarchives.gov.uk/doc/open-government-licence/version/3/"/>
    <cc:attributionURL rdf:resource="https://historicengland.org.uk/"/>
    <cc:attributionName xml:lang="en">Historic England</cc:attributionName>
    <dc:publisher rdf:resource="https://historicengland.org.uk/"/>
    <dc:spatial rdf:resource="http://vocab.getty.edu/tgn/7002445"/>
    <dc:spatial rdf:resource="http://dbpedia.org/resource/England"/>
    <skos:prefLabel xml:lang="en">Commerce</skos:prefLabel>
    <skos:scopeNote xml:lang="en">-</skos:scopeNote>
    <skos:topConceptOf rdf:resource="http://purl.org/heritagedata/schemes/571"/>
  </skos:Concept>

  <skos:Concept rdf:about="http://purl.org/heritagedata/schemes/571/concepts/151077">
    <skos:broader rdf:resource="http://purl.org/heritagedata/schemes/571/concepts/151458"/>
    <skos:inScheme rdf:resource="http://purl.org/heritagedata/schemes/571"/>
    <dc:identifier>http://purl.org/heritagedata/schemes/571/concepts/151077</dc:identifier>
    <dc:issued rdf:datatype="http://www.w3.org/2001/XMLSchema#dateTime">2024-07-01T17:17:33</dc:issued>
    <cc:license rdf:resource="https://www.nationalarchives.gov.uk/doc/open-government-licence/version/3/"/>
    <cc:attributionURL rdf:resource="https://historicengland.org.uk/"/>
    <cc:attributionName xml:lang="en">Historic England</cc:attributionName>
    <dc:publisher rdf:resource="https://historicengland.org.uk/"/>
    <dc:spatial rdf:resource="http://vocab.getty.edu/tgn/7002445"/>
    <dc:spatial rdf:resource="http://dbpedia.org/resource/England"/>
    <skos:prefLabel xml:lang="en">Shopping Centre</skos:prefLabel>
    <skos:related rdf:resource="http://purl.org/heritagedata/schemes/571/concepts/151254"/>
    <skos:related rdf:resource="http://purl.org/heritagedata/schemes/571/concepts/151577"/>
    <skos:scopeNote xml:lang="en">Area largely devoted to retail; typically at a hub within a town or city.</skos:scopeNote>
  </skos:Concept>

  <skos:Concept rdf:about="http://purl.org/heritagedata/schemes/571/concepts/151078">
    <skos:broader rdf:resource="http://purl.org/heritagedata/schemes/571/concepts/151458"/>
    <skos:inScheme rdf:resource="http://purl.org/heritagedata/schemes/571"/>
    <dc:identifier>http://purl.org/heritagedata/schemes/571/concepts/151078</dc:identifier>
    <dc:issued rdf:datatype="http://www.w3.org/2001/XMLSchema#dateTime">2024-07-01T17:17:33</dc:issued>
    <cc:license rdf:resource="https://www.nationalarchives.gov.uk/doc/open-government-licence/version/3/"/>
    <cc:attributionURL rdf:resource="https://historicengland.org.uk/"/>
    <cc:attributionName xml:lang="en">Historic England</cc:attributionName>
    <dc:publisher rdf:resource="https://historicengland.org.uk/"/>
    <dc:spatial rdf:resource="http://vocab.getty.edu/tgn/7002445"/>
    <dc:spatial rdf:resource="http://dbpedia.org/resource/England"/>
    <skos:prefLabel xml:lang="en">Retail Park</skos:prefLabel>
    <skos:related rdf:resource="http://purl.org/heritagedata/schemes/571/concepts/151254"/>
    <skos:related rdf:resource="http://purl.org/heritagedata/schemes/571/concepts/151577"/>
    <skos:scopeNote xml:lang="en">Area designed for retailing, often at the edge of an urban area convenient for private transport.</skos:scopeNote>
  </skos:Concept>

  <skos:Concept rdf:about="http://purl.org/heritagedata/schemes/571/concepts/151079">
    <skos:broader rdf:resource="http://purl.org/heritagedata/schemes/571/concepts/160132"/>
    <skos:inScheme rdf:resource="http://purl.org/heritagedata/schemes/571"/>
    <dc:identifier>http://purl.org/heritagedata/schemes/571/concepts/151079</dc:identifier>
    <dc:issued rdf:datatype="http://www.w3.org/2001/XMLSchema#dateTime">2024-07-01T17:17:33</dc:issued>
    <cc:license rdf:resource="https://www.nationalarchives.gov.uk/doc/open-government-licence/version/3/"/>
    <cc:attributionURL rdf:resource="https://historicengland.org.uk/"/>
    <cc:attributionName xml:lang="en">Historic England</cc:attributionName>
    <dc:publisher rdf:resource="https://historicengland.org.uk/"/>
    <dc:spatial rdf:resource="http://vocab.getty.edu/tgn/7002445"/>
    <dc:spatial rdf:resource="http://dbpedia.org/resource/England"/>
    <skos:prefLabel xml:lang="en">Business Park</skos:prefLabel>
    <skos:related rdf:resource="http://purl.org/heritagedata/schemes/571/concepts/151254"/>
    <skos:related rdf:resource="http://purl.org/heritagedata/schemes/571/concepts/151577"/>
    <skos:scopeNote xml:lang="en">Area designed to accommodate several businesses, usually non-industrial, but normally not exclusively retail.</skos:scopeNote>
  </skos:Concept>

  <skos:Concept rdf:about="http://purl.org/heritagedata/schemes/571/concepts/160132">
    <skos:narrower rdf:resource="http://purl.org/heritagedata/schemes/571/concepts/151079"/>
    <skos:narrower>
      <skos:Concept rdf:about="http://purl.org/heritagedata/schemes/571/concepts/151157">
        <skos:broader rdf:resource="http://purl.org/heritagedata/schemes/571/concepts/160132"/>
        <skos:inScheme rdf:resource="http://purl.org/heritagedata/schemes/571"/>
        <dc:identifier>http://purl.org/heritagedata/schemes/571/concepts/151157</dc:identifier>
        <dc:issued rdf:datatype="http://www.w3.org/2001/XMLSchema#dateTime">2024-07-01T17:17:33</dc:issued>
        <cc:license rdf:resource="https://www.nationalarchives.gov.uk/doc/open-government-licence/version/3/"/>
        <cc:attributionURL rdf:resource="https://historicengland.org.uk/"/>
        <cc:attributionName xml:lang="en">Historic England</cc:attributionName>
        <dc:publisher rdf:resource="https://historicengland.org.uk/"/>
        <dc:spatial rdf:resource="http://vocab.getty.edu/tgn/7002445"/>
        <dc:spatial rdf:resource="http://dbpedia.org/resource/England"/>
        <skos:prefLabel xml:lang="en">Conference Centre</skos:prefLabel>
        <skos:scopeNote xml:lang="en">A purpose-built, or modified, building and directly associated grounds for organisations and associations to meet for presentations and consultation.</skos:scopeNote>
      </skos:Concept>
    </skos:narrower>

    <skos:broader rdf:resource="http://purl.org/heritagedata/schemes/571/concepts/151458"/>
    <skos:inScheme rdf:resource="http://purl.org/heritagedata/schemes/571"/>
    <dc:identifier>http://purl.org/heritagedata/schemes/571/concepts/160132</dc:identifier>
    <dc:issued rdf:datatype="http://www.w3.org/2001/XMLSchema#dateTime">2024-07-01T17:17:33</dc:issued>
    <cc:license rdf:resource="https://www.nationalarchives.gov.uk/doc/open-government-licence/version/3/"/>
    <cc:attributionURL rdf:resource="https://historicengland.org.uk/"/>
    <cc:attributionName xml:lang="en">Historic England</cc:attributionName>
    <dc:publisher rdf:resource="https://historicengland.org.uk/"/>
    <dc:spatial rdf:resource="http://vocab.getty.edu/tgn/7002445"/>
    <dc:spatial rdf:resource="http://dbpedia.org/resource/England"/>
    <skos:prefLabel xml:lang="en">Business</skos:prefLabel>
    <skos:scopeNote xml:lang="en">Being in a state of busily undertaking commercially viable work; being a body undertaking such business.</skos:scopeNote>
  </skos:Concept>

  <skos:Concept rdf:about="http://purl.org/heritagedata/schemes/571/concepts/151081">
    <skos:broader rdf:resource="http://purl.org/heritagedata/schemes/571/concepts/151576"/>
    <skos:inScheme rdf:resource="http://purl.org/heritagedata/schemes/571"/>
    <dc:identifier>http://purl.org/heritagedata/schemes/571/concepts/151081</dc:identifier>
    <dc:issued rdf:datatype="http://www.w3.org/2001/XMLSchema#dateTime">2024-07-01T17:17:33</dc:issued>
    <cc:license rdf:resource="https://www.nationalarchives.gov.uk/doc/open-government-licence/version/3/"/>
    <cc:attributionURL rdf:resource="https://historicengland.org.uk/"/>
    <cc:attributionName xml:lang="en">Historic England</cc:attributionName>
    <dc:publisher rdf:resource="https://historicengland.org.uk/"/>
    <dc:spatial rdf:resource="http://vocab.getty.edu/tgn/7002445"/>
    <dc:spatial rdf:resource="http://dbpedia.org/resource/England"/>
    <skos:prefLabel xml:lang="en">Airfield</skos:prefLabel>
    <skos:related rdf:resource="http://purl.org/heritagedata/schemes/571/concepts/151163"/>
    <skos:related rdf:resource="http://purl.org/heritagedata/schemes/571/concepts/151084"/>
    <skos:related rdf:resource="http://purl.org/heritagedata/schemes/571/concepts/151082"/>
    <skos:scopeNote xml:lang="en">Small-scale commercial or private field used for air travel, mainly fixed-wing.</skos:scopeNote>
  </skos:Concept>

  <skos:Concept rdf:about="http://purl.org/heritagedata/schemes/571/concepts/151576">
    <skos:narrower rdf:resource="http://purl.org/heritagedata/schemes/571/concepts/151081"/>
    <skos:narrower rdf:resource="http://purl.org/heritagedata/schemes/571/concepts/151082"/>
    <skos:narrower rdf:resource="http://purl.org/heritagedata/schemes/571/concepts/151084"/>
    <skos:narrower rdf:resource="http://purl.org/heritagedata/schemes/571/concepts/151085"/>
    <skos:narrower rdf:resource="http://purl.org/heritagedata/schemes/571/concepts/151089"/>
    <skos:narrower rdf:resource="http://purl.org/heritagedata/schemes/571/concepts/151646"/>
    <skos:narrower rdf:resource="http://purl.org/heritagedata/schemes/571/concepts/151647"/>
    <skos:broader rdf:resource="http://purl.org/heritagedata/schemes/571/concepts/151449"/>
    <skos:inScheme rdf:resource="http://purl.org/heritagedata/schemes/571"/>
    <dc:identifier>http://purl.org/heritagedata/schemes/571/concepts/151576</dc:identifier>
    <dc:issued rdf:datatype="http://www.w3.org/2001/XMLSchema#dateTime">2024-07-01T17:17:33</dc:issued>
    <cc:license rdf:resource="https://www.nationalarchives.gov.uk/doc/open-government-licence/version/3/"/>
    <cc:attributionURL rdf:resource="https://historicengland.org.uk/"/>
    <cc:attributionName xml:lang="en">Historic England</cc:attributionName>
    <dc:publisher rdf:resource="https://historicengland.org.uk/"/>
    <dc:spatial rdf:resource="http://vocab.getty.edu/tgn/7002445"/>
    <dc:spatial rdf:resource="http://dbpedia.org/resource/England"/>
    <skos:prefLabel xml:lang="en">Air Transport</skos:prefLabel>
    <skos:scopeNote xml:lang="en">Features associated with control, accommodation, servicing and testing of aircraft.</skos:scopeNote>
  </skos:Concept>

  <skos:Concept rdf:about="http://purl.org/heritagedata/schemes/571/concepts/151082">
    <skos:broader rdf:resource="http://purl.org/heritagedata/schemes/571/concepts/151576"/>
    <skos:inScheme rdf:resource="http://purl.org/heritagedata/schemes/571"/>
    <dc:identifier>http://purl.org/heritagedata/schemes/571/concepts/151082</dc:identifier>
    <dc:issued rdf:datatype="http://www.w3.org/2001/XMLSchema#dateTime">2024-07-01T17:17:33</dc:issued>
    <cc:license rdf:resource="https://www.nationalarchives.gov.uk/doc/open-government-licence/version/3/"/>
    <cc:attributionURL rdf:resource="https://historicengland.org.uk/"/>
    <cc:attributionName xml:lang="en">Historic England</cc:attributionName>
    <dc:publisher rdf:resource="https://historicengland.org.uk/"/>
    <dc:spatial rdf:resource="http://vocab.getty.edu/tgn/7002445"/>
    <dc:spatial rdf:resource="http://dbpedia.org/resource/England"/>
    <skos:prefLabel xml:lang="en">Runway</skos:prefLabel>
    <skos:related rdf:resource="http://purl.org/heritagedata/schemes/571/concepts/151081"/>
    <skos:related rdf:resource="http://purl.org/heritagedata/schemes/571/concepts/151084"/>
    <skos:related rdf:resource="http://purl.org/heritagedata/schemes/571/concepts/151233"/>
    <skos:scopeNote xml:lang="en">Take-off and landing lane with permanent surface.</skos:scopeNote>
  </skos:Concept>

  <skos:Concept rdf:about="http://purl.org/heritagedata/schemes/571/concepts/151084">
    <skos:broader rdf:resource="http://purl.org/heritagedata/schemes/571/concepts/151576"/>
    <skos:inScheme rdf:resource="http://purl.org/heritagedata/schemes/571"/>
    <dc:identifier>http://purl.org/heritagedata/schemes/571/concepts/151084</dc:identifier>
    <dc:issued rdf:datatype="http://www.w3.org/2001/XMLSchema#dateTime">2024-07-01T17:17:33</dc:issued>
    <cc:license rdf:resource="https://www.nationalarchives.gov.uk/doc/open-government-licence/version/3/"/>
    <cc:attributionURL rdf:resource="https://historicengland.org.uk/"/>
    <cc:attributionName xml:lang="en">Historic England</cc:attributionName>
    <dc:publisher rdf:resource="https://historicengland.org.uk/"/>
    <dc:spatial rdf:resource="http://vocab.getty.edu/tgn/7002445"/>
    <dc:spatial rdf:resource="http://dbpedia.org/resource/England"/>
    <skos:prefLabel xml:lang="en">Airport</skos:prefLabel>
    <skos:related rdf:resource="http://purl.org/heritagedata/schemes/571/concepts/151081"/>
    <skos:related rdf:resource="http://purl.org/heritagedata/schemes/571/concepts/151082"/>
    <skos:related rdf:resource="http://purl.org/heritagedata/schemes/571/concepts/151647"/>
    <skos:related rdf:resource="http://purl.org/heritagedata/schemes/571/concepts/151085"/>
    <skos:scopeNote xml:lang="en">Large-scale commercial base for air travel.</skos:scopeNote>
  </skos:Concept>

  <skos:Concept rdf:about="http://purl.org/heritagedata/schemes/571/concepts/151085">
    <skos:broader rdf:resource="http://purl.org/heritagedata/schemes/571/concepts/151576"/>
    <skos:inScheme rdf:resource="http://purl.org/heritagedata/schemes/571"/>
    <dc:identifier>http://purl.org/heritagedata/schemes/571/concepts/151085</dc:identifier>
    <dc:issued rdf:datatype="http://www.w3.org/2001/XMLSchema#dateTime">2024-07-01T17:17:33</dc:issued>
    <cc:license rdf:resource="https://www.nationalarchives.gov.uk/doc/open-government-licence/version/3/"/>
    <cc:attributionURL rdf:resource="https://historicengland.org.uk/"/>
    <cc:attributionName xml:lang="en">Historic England</cc:attributionName>
    <dc:publisher rdf:resource="https://historicengland.org.uk/"/>
    <dc:spatial rdf:resource="http://vocab.getty.edu/tgn/7002445"/>
    <dc:spatial rdf:resource="http://dbpedia.org/resource/England"/>
    <skos:prefLabel xml:lang="en">Control Complex</skos:prefLabel>
    <skos:related rdf:resource="http://purl.org/heritagedata/schemes/571/concepts/151084"/>
    <skos:scopeNote xml:lang="en">Buildings and associated structures and areas for safely guiding air traffic into and out of an airport.</skos:scopeNote>
  </skos:Concept>

  <skos:Concept rdf:about="http://purl.org/heritagedata/schemes/571/concepts/151086">
    <skos:broader rdf:resource="http://purl.org/heritagedata/schemes/571/concepts/151647"/>
    <skos:broader rdf:resource="http://purl.org/heritagedata/schemes/571/concepts/151667"/>
    <skos:inScheme rdf:resource="http://purl.org/heritagedata/schemes/571"/>
    <dc:identifier>http://purl.org/heritagedata/schemes/571/concepts/151086</dc:identifier>
    <dc:issued rdf:datatype="http://www.w3.org/2001/XMLSchema#dateTime">2024-07-01T17:17:33</dc:issued>
    <cc:license rdf:resource="https://www.nationalarchives.gov.uk/doc/open-government-licence/version/3/"/>
    <cc:attributionURL rdf:resource="https://historicengland.org.uk/"/>
    <cc:attributionName xml:lang="en">Historic England</cc:attributionName>
    <dc:publisher rdf:resource="https://historicengland.org.uk/"/>
    <dc:spatial rdf:resource="http://vocab.getty.edu/tgn/7002445"/>
    <dc:spatial rdf:resource="http://dbpedia.org/resource/England"/>
    <skos:prefLabel xml:lang="en">Terminal Building</skos:prefLabel>
    <skos:scopeNote xml:lang="en">A building within a transport terminal, often associated with the registration and clearing of incoming and outgoing passengers or freight. Also used for waiting and so often provided with commercial outlets and other facilities.</skos:scopeNote>
  </skos:Concept>

  <skos:Concept rdf:about="http://purl.org/heritagedata/schemes/571/concepts/151647">
    <skos:narrower rdf:resource="http://purl.org/heritagedata/schemes/571/concepts/151086"/>
    <skos:broader rdf:resource="http://purl.org/heritagedata/schemes/571/concepts/151576"/>
    <skos:inScheme rdf:resource="http://purl.org/heritagedata/schemes/571"/>
    <dc:identifier>http://purl.org/heritagedata/schemes/571/concepts/151647</dc:identifier>
    <dc:issued rdf:datatype="http://www.w3.org/2001/XMLSchema#dateTime">2024-07-01T17:17:33</dc:issued>
    <cc:license rdf:resource="https://www.nationalarchives.gov.uk/doc/open-government-licence/version/3/"/>
    <cc:attributionURL rdf:resource="https://historicengland.org.uk/"/>
    <cc:attributionName xml:lang="en">Historic England</cc:attributionName>
    <dc:publisher rdf:resource="https://historicengland.org.uk/"/>
    <dc:spatial rdf:resource="http://vocab.getty.edu/tgn/7002445"/>
    <dc:spatial rdf:resource="http://dbpedia.org/resource/England"/>
    <skos:prefLabel xml:lang="en">Air Terminal</skos:prefLabel>
    <skos:related rdf:resource="http://purl.org/heritagedata/schemes/571/concepts/151084"/>
    <skos:scopeNote xml:lang="en">Buildings and their directly associated grounds at an airport from where passengers await,  embark and disembark from an aircraft.</skos:scopeNote>
  </skos:Concept>

  <skos:Concept rdf:about="http://purl.org/heritagedata/schemes/571/concepts/151087">
    <skos:broader rdf:resource="http://purl.org/heritagedata/schemes/571/concepts/151090"/>
    <skos:inScheme rdf:resource="http://purl.org/heritagedata/schemes/571"/>
    <dc:identifier>http://purl.org/heritagedata/schemes/571/concepts/151087</dc:identifier>
    <dc:issued rdf:datatype="http://www.w3.org/2001/XMLSchema#dateTime">2024-07-01T17:17:33</dc:issued>
    <cc:license rdf:resource="https://www.nationalarchives.gov.uk/doc/open-government-licence/version/3/"/>
    <cc:attributionURL rdf:resource="https://historicengland.org.uk/"/>
    <cc:attributionName xml:lang="en">Historic England</cc:attributionName>
    <dc:publisher rdf:resource="https://historicengland.org.uk/"/>
    <dc:spatial rdf:resource="http://vocab.getty.edu/tgn/7002445"/>
    <dc:spatial rdf:resource="http://dbpedia.org/resource/England"/>
    <skos:prefLabel xml:lang="en">Canal</skos:prefLabel>
    <skos:related rdf:resource="http://purl.org/heritagedata/schemes/571/concepts/151655"/>
    <skos:scopeNote xml:lang="en">Artificial watercourse, usually connecting existing watercourses or bodies, constructed for the purpose of inland navigation and transportation or irrigation. Nowadays also used for recreational purposes.</skos:scopeNote>
  </skos:Concept>

  <skos:Concept rdf:about="http://purl.org/heritagedata/schemes/571/concepts/151090">
    <skos:narrower rdf:resource="http://purl.org/heritagedata/schemes/571/concepts/151087"/>
    <skos:narrower>
      <skos:Concept rdf:about="http://purl.org/heritagedata/schemes/571/concepts/151088">
        <skos:broader rdf:resource="http://purl.org/heritagedata/schemes/571/concepts/151090"/>
        <skos:inScheme rdf:resource="http://purl.org/heritagedata/schemes/571"/>
        <dc:identifier>http://purl.org/heritagedata/schemes/571/concepts/151088</dc:identifier>
        <dc:issued rdf:datatype="http://www.w3.org/2001/XMLSchema#dateTime">2024-07-01T17:17:33</dc:issued>
        <cc:license rdf:resource="https://www.nationalarchives.gov.uk/doc/open-government-licence/version/3/"/>
        <cc:attributionURL rdf:resource="https://historicengland.org.uk/"/>
        <cc:attributionName xml:lang="en">Historic England</cc:attributionName>
        <dc:publisher rdf:resource="https://historicengland.org.uk/"/>
        <dc:spatial rdf:resource="http://vocab.getty.edu/tgn/7002445"/>
        <dc:spatial rdf:resource="http://dbpedia.org/resource/England"/>
        <skos:prefLabel xml:lang="en">Navigable River</skos:prefLabel>
        <skos:scopeNote xml:lang="en">Length of river sufficiently deep for regular use by water transport and traffic.</skos:scopeNote>
      </skos:Concept>
    </skos:narrower>

    <skos:narrower rdf:resource="http://purl.org/heritagedata/schemes/571/concepts/151655"/>
    <skos:broader rdf:resource="http://purl.org/heritagedata/schemes/571/concepts/151648"/>
    <skos:inScheme rdf:resource="http://purl.org/heritagedata/schemes/571"/>
    <dc:identifier>http://purl.org/heritagedata/schemes/571/concepts/151090</dc:identifier>
    <dc:issued rdf:datatype="http://www.w3.org/2001/XMLSchema#dateTime">2024-07-01T17:17:33</dc:issued>
    <cc:license rdf:resource="https://www.nationalarchives.gov.uk/doc/open-government-licence/version/3/"/>
    <cc:attributionURL rdf:resource="https://historicengland.org.uk/"/>
    <cc:attributionName xml:lang="en">Historic England</cc:attributionName>
    <dc:publisher rdf:resource="https://historicengland.org.uk/"/>
    <dc:spatial rdf:resource="http://vocab.getty.edu/tgn/7002445"/>
    <dc:spatial rdf:resource="http://dbpedia.org/resource/England"/>
    <skos:prefLabel xml:lang="en">Inland Waterway</skos:prefLabel>
    <skos:scopeNote xml:lang="en">Natural and artificial passages for inland waterborne travel and transport.</skos:scopeNote>
  </skos:Concept>

  <skos:Concept rdf:about="http://purl.org/heritagedata/schemes/571/concepts/151089">
    <skos:broader rdf:resource="http://purl.org/heritagedata/schemes/571/concepts/151576"/>
    <skos:inScheme rdf:resource="http://purl.org/heritagedata/schemes/571"/>
    <dc:identifier>http://purl.org/heritagedata/schemes/571/concepts/151089</dc:identifier>
    <dc:issued rdf:datatype="http://www.w3.org/2001/XMLSchema#dateTime">2024-07-01T17:17:33</dc:issued>
    <cc:license rdf:resource="https://www.nationalarchives.gov.uk/doc/open-government-licence/version/3/"/>
    <cc:attributionURL rdf:resource="https://historicengland.org.uk/"/>
    <cc:attributionName xml:lang="en">Historic England</cc:attributionName>
    <dc:publisher rdf:resource="https://historicengland.org.uk/"/>
    <dc:spatial rdf:resource="http://vocab.getty.edu/tgn/7002445"/>
    <dc:spatial rdf:resource="http://dbpedia.org/resource/England"/>
    <skos:prefLabel xml:lang="en">Heliport</skos:prefLabel>
    <skos:related rdf:resource="http://purl.org/heritagedata/schemes/571/concepts/151163"/>
    <skos:scopeNote xml:lang="en">Field or plot, often with hangars and other buildings, used for commercial or private helicopter travel.</skos:scopeNote>
  </skos:Concept>

  <skos:Concept rdf:about="http://purl.org/heritagedata/schemes/571/concepts/151648">
    <skos:narrower rdf:resource="http://purl.org/heritagedata/schemes/571/concepts/151090"/>
    <skos:narrower rdf:resource="http://purl.org/heritagedata/schemes/571/concepts/151095"/>
    <skos:narrower>
      <skos:Concept rdf:about="http://purl.org/heritagedata/schemes/571/concepts/151098">
        <skos:broader rdf:resource="http://purl.org/heritagedata/schemes/571/concepts/151648"/>
        <skos:inScheme rdf:resource="http://purl.org/heritagedata/schemes/571"/>
        <dc:identifier>http://purl.org/heritagedata/schemes/571/concepts/151098</dc:identifier>
        <dc:issued rdf:datatype="http://www.w3.org/2001/XMLSchema#dateTime">2024-07-01T17:17:33</dc:issued>
        <cc:license rdf:resource="https://www.nationalarchives.gov.uk/doc/open-government-licence/version/3/"/>
        <cc:attributionURL rdf:resource="https://historicengland.org.uk/"/>
        <cc:attributionName xml:lang="en">Historic England</cc:attributionName>
        <dc:publisher rdf:resource="https://historicengland.org.uk/"/>
        <dc:spatial rdf:resource="http://vocab.getty.edu/tgn/7002445"/>
        <dc:spatial rdf:resource="http://dbpedia.org/resource/England"/>
        <skos:prefLabel xml:lang="en">Slipway</skos:prefLabel>
        <skos:scopeNote xml:lang="en">A structure inclined towards the water on which a ship may be built or lowered into the water.</skos:scopeNote>
      </skos:Concept>
    </skos:narrower>

    <skos:narrower rdf:resource="http://purl.org/heritagedata/schemes/571/concepts/151667"/>
    <skos:narrower rdf:resource="http://purl.org/heritagedata/schemes/571/concepts/151678"/>
    <skos:narrower rdf:resource="http://purl.org/heritagedata/schemes/571/concepts/152539"/>
    <skos:broader rdf:resource="http://purl.org/heritagedata/schemes/571/concepts/151449"/>
    <skos:inScheme rdf:resource="http://purl.org/heritagedata/schemes/571"/>
    <dc:identifier>http://purl.org/heritagedata/schemes/571/concepts/151648</dc:identifier>
    <dc:issued rdf:datatype="http://www.w3.org/2001/XMLSchema#dateTime">2024-07-01T17:17:33</dc:issued>
    <cc:license rdf:resource="https://www.nationalarchives.gov.uk/doc/open-government-licence/version/3/"/>
    <cc:attributionURL rdf:resource="https://historicengland.org.uk/"/>
    <cc:attributionName xml:lang="en">Historic England</cc:attributionName>
    <dc:publisher rdf:resource="https://historicengland.org.uk/"/>
    <dc:spatial rdf:resource="http://vocab.getty.edu/tgn/7002445"/>
    <dc:spatial rdf:resource="http://dbpedia.org/resource/England"/>
    <skos:prefLabel xml:lang="en">Water Transport</skos:prefLabel>
    <skos:scopeNote xml:lang="en">Areas associated with movement of people or goods on or in water.</skos:scopeNote>
  </skos:Concept>

  <skos:Concept rdf:about="http://purl.org/heritagedata/schemes/571/concepts/151091">
    <skos:broader rdf:resource="http://purl.org/heritagedata/schemes/571/concepts/151667"/>
    <skos:broader rdf:resource="http://purl.org/heritagedata/schemes/571/concepts/160188"/>
    <skos:narrower>
      <skos:Concept rdf:about="http://purl.org/heritagedata/schemes/571/concepts/151092">
        <skos:broader rdf:resource="http://purl.org/heritagedata/schemes/571/concepts/151091"/>
        <skos:inScheme rdf:resource="http://purl.org/heritagedata/schemes/571"/>
        <dc:identifier>http://purl.org/heritagedata/schemes/571/concepts/151092</dc:identifier>
        <dc:issued rdf:datatype="http://www.w3.org/2001/XMLSchema#dateTime">2024-07-01T17:17:33</dc:issued>
        <cc:license rdf:resource="https://www.nationalarchives.gov.uk/doc/open-government-licence/version/3/"/>
        <cc:attributionURL rdf:resource="https://historicengland.org.uk/"/>
        <cc:attributionName xml:lang="en">Historic England</cc:attributionName>
        <dc:publisher rdf:resource="https://historicengland.org.uk/"/>
        <dc:spatial rdf:resource="http://vocab.getty.edu/tgn/7002445"/>
        <dc:spatial rdf:resource="http://dbpedia.org/resource/England"/>
        <skos:prefLabel xml:lang="en">Dry Dock</skos:prefLabel>
        <skos:scopeNote xml:lang="en">A stone-faced enclosure, with entrance closed by a floatable caisson or by gates, which can be pumped dry for inspection, maintenance, or repair of the hull or underwater fittings of a ship or ships.</skos:scopeNote>
      </skos:Concept>
    </skos:narrower>

    <skos:narrower>
      <skos:Concept rdf:about="http://purl.org/heritagedata/schemes/571/concepts/151093">
        <skos:broader rdf:resource="http://purl.org/heritagedata/schemes/571/concepts/151091"/>
        <skos:inScheme rdf:resource="http://purl.org/heritagedata/schemes/571"/>
        <dc:identifier>http://purl.org/heritagedata/schemes/571/concepts/151093</dc:identifier>
        <dc:issued rdf:datatype="http://www.w3.org/2001/XMLSchema#dateTime">2024-07-01T17:17:33</dc:issued>
        <cc:license rdf:resource="https://www.nationalarchives.gov.uk/doc/open-government-licence/version/3/"/>
        <cc:attributionURL rdf:resource="https://historicengland.org.uk/"/>
        <cc:attributionName xml:lang="en">Historic England</cc:attributionName>
        <dc:publisher rdf:resource="https://historicengland.org.uk/"/>
        <dc:spatial rdf:resource="http://vocab.getty.edu/tgn/7002445"/>
        <dc:spatial rdf:resource="http://dbpedia.org/resource/England"/>
        <skos:prefLabel xml:lang="en">Wet Dock</skos:prefLabel>
        <skos:scopeNote xml:lang="en">An artificial structure or group of structures enclosing an area of water which was impounded by lock gates to maintain water levels artificially, facilitating the loading, unloading, building or repair of ships.</skos:scopeNote>
      </skos:Concept>
    </skos:narrower>

    <skos:inScheme rdf:resource="http://purl.org/heritagedata/schemes/571"/>
    <dc:identifier>http://purl.org/heritagedata/schemes/571/concepts/151091</dc:identifier>
    <dc:issued rdf:datatype="http://www.w3.org/2001/XMLSchema#dateTime">2024-07-01T17:17:33</dc:issued>
    <cc:license rdf:resource="https://www.nationalarchives.gov.uk/doc/open-government-licence/version/3/"/>
    <cc:attributionURL rdf:resource="https://historicengland.org.uk/"/>
    <cc:attributionName xml:lang="en">Historic England</cc:attributionName>
    <dc:publisher rdf:resource="https://historicengland.org.uk/"/>
    <dc:spatial rdf:resource="http://vocab.getty.edu/tgn/7002445"/>
    <dc:spatial rdf:resource="http://dbpedia.org/resource/England"/>
    <skos:prefLabel xml:lang="en">Dockyard</skos:prefLabel>
    <skos:scopeNote xml:lang="en">An area of wet or dry docks, storage areas and workshops for the building, repair, fitting, loading and unloading of ships and therefore situated on a sea coast or estuary.</skos:scopeNote>
  </skos:Concept>

  <skos:Concept rdf:about="http://purl.org/heritagedata/schemes/571/concepts/160188">
    <skos:narrower rdf:resource="http://purl.org/heritagedata/schemes/571/concepts/151091"/>
    <skos:narrower>
      <skos:Concept rdf:about="http://purl.org/heritagedata/schemes/571/concepts/151222">
        <skos:broader rdf:resource="http://purl.org/heritagedata/schemes/571/concepts/160188"/>
        <skos:inScheme rdf:resource="http://purl.org/heritagedata/schemes/571"/>
        <dc:identifier>http://purl.org/heritagedata/schemes/571/concepts/151222</dc:identifier>
        <dc:issued rdf:datatype="http://www.w3.org/2001/XMLSchema#dateTime">2024-07-01T17:17:33</dc:issued>
        <cc:license rdf:resource="https://www.nationalarchives.gov.uk/doc/open-government-licence/version/3/"/>
        <cc:attributionURL rdf:resource="https://historicengland.org.uk/"/>
        <cc:attributionName xml:lang="en">Historic England</cc:attributionName>
        <dc:publisher rdf:resource="https://historicengland.org.uk/"/>
        <dc:spatial rdf:resource="http://vocab.getty.edu/tgn/7002445"/>
        <dc:spatial rdf:resource="http://dbpedia.org/resource/England"/>
        <skos:prefLabel xml:lang="en">Boatyard</skos:prefLabel>
        <skos:scopeNote xml:lang="en">A place where smaller vessels are built, repaired and stored</skos:scopeNote>
      </skos:Concept>
    </skos:narrower>

    <skos:narrower>
      <skos:Concept rdf:about="http://purl.org/heritagedata/schemes/571/concepts/151223">
        <skos:broader rdf:resource="http://purl.org/heritagedata/schemes/571/concepts/160188"/>
        <skos:inScheme rdf:resource="http://purl.org/heritagedata/schemes/571"/>
        <dc:identifier>http://purl.org/heritagedata/schemes/571/concepts/151223</dc:identifier>
        <dc:issued rdf:datatype="http://www.w3.org/2001/XMLSchema#dateTime">2024-07-01T17:17:33</dc:issued>
        <cc:license rdf:resource="https://www.nationalarchives.gov.uk/doc/open-government-licence/version/3/"/>
        <cc:attributionURL rdf:resource="https://historicengland.org.uk/"/>
        <cc:attributionName xml:lang="en">Historic England</cc:attributionName>
        <dc:publisher rdf:resource="https://historicengland.org.uk/"/>
        <dc:spatial rdf:resource="http://vocab.getty.edu/tgn/7002445"/>
        <dc:spatial rdf:resource="http://dbpedia.org/resource/England"/>
        <skos:prefLabel xml:lang="en">Shipyard</skos:prefLabel>
        <skos:scopeNote xml:lang="en">A place where ships or boats are built, repaired and moored.</skos:scopeNote>
      </skos:Concept>
    </skos:narrower>

    <skos:broader rdf:resource="http://purl.org/heritagedata/schemes/571/concepts/152638"/>
    <skos:inScheme rdf:resource="http://purl.org/heritagedata/schemes/571"/>
    <dc:identifier>http://purl.org/heritagedata/schemes/571/concepts/160188</dc:identifier>
    <dc:issued rdf:datatype="http://www.w3.org/2001/XMLSchema#dateTime">2024-07-01T17:17:33</dc:issued>
    <cc:license rdf:resource="https://www.nationalarchives.gov.uk/doc/open-government-licence/version/3/"/>
    <cc:attributionURL rdf:resource="https://historicengland.org.uk/"/>
    <cc:attributionName xml:lang="en">Historic England</cc:attributionName>
    <dc:publisher rdf:resource="https://historicengland.org.uk/"/>
    <dc:spatial rdf:resource="http://vocab.getty.edu/tgn/7002445"/>
    <dc:spatial rdf:resource="http://dbpedia.org/resource/England"/>
    <skos:prefLabel xml:lang="en">Shipbuilding And Repair</skos:prefLabel>
    <skos:scopeNote xml:lang="en">Buildings, sites and structures associated with the construction and repair of ships and boats.</skos:scopeNote>
  </skos:Concept>

  <skos:Concept rdf:about="http://purl.org/heritagedata/schemes/571/concepts/151095">
    <skos:broader rdf:resource="http://purl.org/heritagedata/schemes/571/concepts/151648"/>
    <skos:inScheme rdf:resource="http://purl.org/heritagedata/schemes/571"/>
    <dc:identifier>http://purl.org/heritagedata/schemes/571/concepts/151095</dc:identifier>
    <dc:issued rdf:datatype="http://www.w3.org/2001/XMLSchema#dateTime">2024-07-01T17:17:33</dc:issued>
    <cc:license rdf:resource="https://www.nationalarchives.gov.uk/doc/open-government-licence/version/3/"/>
    <cc:attributionURL rdf:resource="https://historicengland.org.uk/"/>
    <cc:attributionName xml:lang="en">Historic England</cc:attributionName>
    <dc:publisher rdf:resource="https://historicengland.org.uk/"/>
    <dc:spatial rdf:resource="http://vocab.getty.edu/tgn/7002445"/>
    <dc:spatial rdf:resource="http://dbpedia.org/resource/England"/>
    <skos:prefLabel xml:lang="en">Jetty</skos:prefLabel>
    <skos:related rdf:resource="http://purl.org/heritagedata/schemes/571/concepts/151055"/>
    <skos:related rdf:resource="http://purl.org/heritagedata/schemes/571/concepts/151059"/>
    <skos:related rdf:resource="http://purl.org/heritagedata/schemes/571/concepts/151096"/>
    <skos:related rdf:resource="http://purl.org/heritagedata/schemes/571/concepts/151097"/>
    <skos:scopeNote xml:lang="en">A pier-like structure situated at a harbour entrance or running out into the sea or a lake, whose purpose is often to control tidal flow and sedimentation but may also serve as a berthing point for boats and shipping.</skos:scopeNote>
  </skos:Concept>

  <skos:Concept rdf:about="http://purl.org/heritagedata/schemes/571/concepts/151096">
    <skos:broader rdf:resource="http://purl.org/heritagedata/schemes/571/concepts/151667"/>
    <skos:inScheme rdf:resource="http://purl.org/heritagedata/schemes/571"/>
    <dc:identifier>http://purl.org/heritagedata/schemes/571/concepts/151096</dc:identifier>
    <dc:issued rdf:datatype="http://www.w3.org/2001/XMLSchema#dateTime">2024-07-01T17:17:33</dc:issued>
    <cc:license rdf:resource="https://www.nationalarchives.gov.uk/doc/open-government-licence/version/3/"/>
    <cc:attributionURL rdf:resource="https://historicengland.org.uk/"/>
    <cc:attributionName xml:lang="en">Historic England</cc:attributionName>
    <dc:publisher rdf:resource="https://historicengland.org.uk/"/>
    <dc:spatial rdf:resource="http://vocab.getty.edu/tgn/7002445"/>
    <dc:spatial rdf:resource="http://dbpedia.org/resource/England"/>
    <skos:prefLabel xml:lang="en">Quay</skos:prefLabel>
    <skos:related rdf:resource="http://purl.org/heritagedata/schemes/571/concepts/151095"/>
    <skos:related rdf:resource="http://purl.org/heritagedata/schemes/571/concepts/151405"/>
    <skos:scopeNote xml:lang="en">An artificial bank or landing place, largely of solid construction, built parallel to, or projecting out from, the shoreline to facilitate the loading and unloading of vessels.</skos:scopeNote>
  </skos:Concept>

  <skos:Concept rdf:about="http://purl.org/heritagedata/schemes/571/concepts/151097">
    <skos:broader rdf:resource="http://purl.org/heritagedata/schemes/571/concepts/151667"/>
    <skos:inScheme rdf:resource="http://purl.org/heritagedata/schemes/571"/>
    <dc:identifier>http://purl.org/heritagedata/schemes/571/concepts/151097</dc:identifier>
    <dc:issued rdf:datatype="http://www.w3.org/2001/XMLSchema#dateTime">2024-07-01T17:17:33</dc:issued>
    <cc:license rdf:resource="https://www.nationalarchives.gov.uk/doc/open-government-licence/version/3/"/>
    <cc:attributionURL rdf:resource="https://historicengland.org.uk/"/>
    <cc:attributionName xml:lang="en">Historic England</cc:attributionName>
    <dc:publisher rdf:resource="https://historicengland.org.uk/"/>
    <dc:spatial rdf:resource="http://vocab.getty.edu/tgn/7002445"/>
    <dc:spatial rdf:resource="http://dbpedia.org/resource/England"/>
    <skos:prefLabel xml:lang="en">Working Pier</skos:prefLabel>
    <skos:related rdf:resource="http://purl.org/heritagedata/schemes/571/concepts/151095"/>
    <skos:scopeNote xml:lang="en">A raised platform generally of iron or wood, supported on spaced pillars or props and projecting out into the sea; designed to facilitate the transfer of cargo and/or passengers on and off shipping.</skos:scopeNote>
  </skos:Concept>

  <skos:Concept rdf:about="http://purl.org/heritagedata/schemes/571/concepts/151099">
    <skos:broader rdf:resource="http://purl.org/heritagedata/schemes/571/concepts/151652"/>
    <skos:inScheme rdf:resource="http://purl.org/heritagedata/schemes/571"/>
    <dc:identifier>http://purl.org/heritagedata/schemes/571/concepts/151099</dc:identifier>
    <dc:issued rdf:datatype="http://www.w3.org/2001/XMLSchema#dateTime">2024-07-01T17:17:33</dc:issued>
    <cc:license rdf:resource="https://www.nationalarchives.gov.uk/doc/open-government-licence/version/3/"/>
    <cc:attributionURL rdf:resource="https://historicengland.org.uk/"/>
    <cc:attributionName xml:lang="en">Historic England</cc:attributionName>
    <dc:publisher rdf:resource="https://historicengland.org.uk/"/>
    <dc:spatial rdf:resource="http://vocab.getty.edu/tgn/7002445"/>
    <dc:spatial rdf:resource="http://dbpedia.org/resource/England"/>
    <skos:prefLabel xml:lang="en">Container Terminal</skos:prefLabel>
    <skos:scopeNote xml:lang="en">An area of a port, dock or harbour where cargo vessels load and unload large storage containers. Includes associated container storage areas and rail terminals for containers transported to the terminal by rail.</skos:scopeNote>
  </skos:Concept>

  <skos:Concept rdf:about="http://purl.org/heritagedata/schemes/571/concepts/151652">
    <skos:narrower rdf:resource="http://purl.org/heritagedata/schemes/571/concepts/151099"/>
    <skos:narrower>
      <skos:Concept rdf:about="http://purl.org/heritagedata/schemes/571/concepts/151100">
        <skos:broader rdf:resource="http://purl.org/heritagedata/schemes/571/concepts/151652"/>
        <skos:inScheme rdf:resource="http://purl.org/heritagedata/schemes/571"/>
        <dc:identifier>http://purl.org/heritagedata/schemes/571/concepts/151100</dc:identifier>
        <dc:issued rdf:datatype="http://www.w3.org/2001/XMLSchema#dateTime">2024-07-01T17:17:33</dc:issued>
        <cc:license rdf:resource="https://www.nationalarchives.gov.uk/doc/open-government-licence/version/3/"/>
        <cc:attributionURL rdf:resource="https://historicengland.org.uk/"/>
        <cc:attributionName xml:lang="en">Historic England</cc:attributionName>
        <dc:publisher rdf:resource="https://historicengland.org.uk/"/>
        <dc:spatial rdf:resource="http://vocab.getty.edu/tgn/7002445"/>
        <dc:spatial rdf:resource="http://dbpedia.org/resource/England"/>
        <skos:prefLabel xml:lang="en">Ferry Terminal</skos:prefLabel>
        <skos:scopeNote xml:lang="en">An area of a port, dock or harbour, often including buildings for passport control, customs and for sheltered waiting and storage, where passengers and vehicles using ferry services can embark/disembark and where supplies can be taken on board.</skos:scopeNote>
      </skos:Concept>
    </skos:narrower>

    <skos:broader rdf:resource="http://purl.org/heritagedata/schemes/571/concepts/151667"/>
    <skos:inScheme rdf:resource="http://purl.org/heritagedata/schemes/571"/>
    <dc:identifier>http://purl.org/heritagedata/schemes/571/concepts/151652</dc:identifier>
    <dc:issued rdf:datatype="http://www.w3.org/2001/XMLSchema#dateTime">2024-07-01T17:17:33</dc:issued>
    <cc:license rdf:resource="https://www.nationalarchives.gov.uk/doc/open-government-licence/version/3/"/>
    <cc:attributionURL rdf:resource="https://historicengland.org.uk/"/>
    <cc:attributionName xml:lang="en">Historic England</cc:attributionName>
    <dc:publisher rdf:resource="https://historicengland.org.uk/"/>
    <dc:spatial rdf:resource="http://vocab.getty.edu/tgn/7002445"/>
    <dc:spatial rdf:resource="http://dbpedia.org/resource/England"/>
    <skos:prefLabel xml:lang="en">Sea Terminal</skos:prefLabel>
    <skos:scopeNote xml:lang="en">A port, dock or harbour where ferries, hovercraft, ocean liners and cargo vessels can load and unload. May include road and/or rail terminals for transportation to the port.</skos:scopeNote>
  </skos:Concept>

  <skos:Concept rdf:about="http://purl.org/heritagedata/schemes/571/concepts/151101">
    <skos:broader rdf:resource="http://purl.org/heritagedata/schemes/571/concepts/151678"/>
    <skos:narrower>
      <skos:Concept rdf:about="http://purl.org/heritagedata/schemes/571/concepts/151102">
        <skos:broader rdf:resource="http://purl.org/heritagedata/schemes/571/concepts/151101"/>
        <skos:inScheme rdf:resource="http://purl.org/heritagedata/schemes/571"/>
        <dc:identifier>http://purl.org/heritagedata/schemes/571/concepts/151102</dc:identifier>
        <dc:issued rdf:datatype="http://www.w3.org/2001/XMLSchema#dateTime">2024-07-01T17:17:33</dc:issued>
        <cc:license rdf:resource="https://www.nationalarchives.gov.uk/doc/open-government-licence/version/3/"/>
        <cc:attributionURL rdf:resource="https://historicengland.org.uk/"/>
        <cc:attributionName xml:lang="en">Historic England</cc:attributionName>
        <dc:publisher rdf:resource="https://historicengland.org.uk/"/>
        <dc:spatial rdf:resource="http://vocab.getty.edu/tgn/7002445"/>
        <dc:spatial rdf:resource="http://dbpedia.org/resource/England"/>
        <skos:prefLabel xml:lang="en">Commercial Shipping Route</skos:prefLabel>
        <skos:scopeNote xml:lang="en">Route regularly used by ships engaged in commerce or trade. May be defined by usage or in some areas, formally defined by regulation. Distinguished from the Navigation route Sub-character Type by the association with commerical shipping.</skos:scopeNote>
      </skos:Concept>
    </skos:narrower>

    <skos:narrower>
      <skos:Concept rdf:about="http://purl.org/heritagedata/schemes/571/concepts/151103">
        <skos:broader rdf:resource="http://purl.org/heritagedata/schemes/571/concepts/151101"/>
        <skos:inScheme rdf:resource="http://purl.org/heritagedata/schemes/571"/>
        <dc:identifier>http://purl.org/heritagedata/schemes/571/concepts/151103</dc:identifier>
        <dc:issued rdf:datatype="http://www.w3.org/2001/XMLSchema#dateTime">2024-07-01T17:17:33</dc:issued>
        <cc:license rdf:resource="https://www.nationalarchives.gov.uk/doc/open-government-licence/version/3/"/>
        <cc:attributionURL rdf:resource="https://historicengland.org.uk/"/>
        <cc:attributionName xml:lang="en">Historic England</cc:attributionName>
        <dc:publisher rdf:resource="https://historicengland.org.uk/"/>
        <dc:spatial rdf:resource="http://vocab.getty.edu/tgn/7002445"/>
        <dc:spatial rdf:resource="http://dbpedia.org/resource/England"/>
        <skos:prefLabel xml:lang="en">Ferry Crossing</skos:prefLabel>
        <skos:scopeNote xml:lang="en">A regular commercial passenger route across an area of sea, estuary, river or lake, or an area of port, dock or harbour. Includes chain link ferry crossings.</skos:scopeNote>
      </skos:Concept>
    </skos:narrower>

    <skos:inScheme rdf:resource="http://purl.org/heritagedata/schemes/571"/>
    <dc:identifier>http://purl.org/heritagedata/schemes/571/concepts/151101</dc:identifier>
    <dc:issued rdf:datatype="http://www.w3.org/2001/XMLSchema#dateTime">2024-07-01T17:17:33</dc:issued>
    <cc:license rdf:resource="https://www.nationalarchives.gov.uk/doc/open-government-licence/version/3/"/>
    <cc:attributionURL rdf:resource="https://historicengland.org.uk/"/>
    <cc:attributionName xml:lang="en">Historic England</cc:attributionName>
    <dc:publisher rdf:resource="https://historicengland.org.uk/"/>
    <dc:spatial rdf:resource="http://vocab.getty.edu/tgn/7002445"/>
    <dc:spatial rdf:resource="http://dbpedia.org/resource/England"/>
    <skos:prefLabel xml:lang="en">Navigation Route</skos:prefLabel>
    <skos:scopeNote xml:lang="en">Routes regularly used by vessels of any description while navigating between destinations. May be defined by usage or in some areas, formally defined by regulation.</skos:scopeNote>
  </skos:Concept>

  <skos:Concept rdf:about="http://purl.org/heritagedata/schemes/571/concepts/151678">
    <skos:narrower rdf:resource="http://purl.org/heritagedata/schemes/571/concepts/151101"/>
    <skos:narrower>
      <skos:Concept rdf:about="http://purl.org/heritagedata/schemes/571/concepts/151104">
        <skos:broader rdf:resource="http://purl.org/heritagedata/schemes/571/concepts/151678"/>
        <skos:inScheme rdf:resource="http://purl.org/heritagedata/schemes/571"/>
        <dc:identifier>http://purl.org/heritagedata/schemes/571/concepts/151104</dc:identifier>
        <dc:issued rdf:datatype="http://www.w3.org/2001/XMLSchema#dateTime">2024-07-01T17:17:33</dc:issued>
        <cc:license rdf:resource="https://www.nationalarchives.gov.uk/doc/open-government-licence/version/3/"/>
        <cc:attributionURL rdf:resource="https://historicengland.org.uk/"/>
        <cc:attributionName xml:lang="en">Historic England</cc:attributionName>
        <dc:publisher rdf:resource="https://historicengland.org.uk/"/>
        <dc:spatial rdf:resource="http://vocab.getty.edu/tgn/7002445"/>
        <dc:spatial rdf:resource="http://dbpedia.org/resource/England"/>
        <skos:prefLabel xml:lang="en">Dredged Area</skos:prefLabel>
        <skos:scopeNote xml:lang="en">An area from which sediments have been removed to ensure a safe depth of water in channels and berths for navigational purposes or to mitigate risk of flooding or protect a sensitive habitat.</skos:scopeNote>
      </skos:Concept>
    </skos:narrower>

    <skos:narrower>
      <skos:Concept rdf:about="http://purl.org/heritagedata/schemes/571/concepts/151105">
        <skos:broader rdf:resource="http://purl.org/heritagedata/schemes/571/concepts/151678"/>
        <skos:inScheme rdf:resource="http://purl.org/heritagedata/schemes/571"/>
        <dc:identifier>http://purl.org/heritagedata/schemes/571/concepts/151105</dc:identifier>
        <dc:issued rdf:datatype="http://www.w3.org/2001/XMLSchema#dateTime">2024-07-01T17:17:33</dc:issued>
        <cc:license rdf:resource="https://www.nationalarchives.gov.uk/doc/open-government-licence/version/3/"/>
        <cc:attributionURL rdf:resource="https://historicengland.org.uk/"/>
        <cc:attributionName xml:lang="en">Historic England</cc:attributionName>
        <dc:publisher rdf:resource="https://historicengland.org.uk/"/>
        <dc:spatial rdf:resource="http://vocab.getty.edu/tgn/7002445"/>
        <dc:spatial rdf:resource="http://dbpedia.org/resource/England"/>
        <skos:prefLabel xml:lang="en">Anchorage</skos:prefLabel>
        <skos:scopeNote xml:lang="en">An area of sea or coast where vessels anchor, often provided by sheltered conditions afforded by the topography of the nearby coast. They are often located along coastlines within bays or areas sheltered from prevailing winds and/or strong currents.</skos:scopeNote>
      </skos:Concept>
    </skos:narrower>

    <skos:narrower rdf:resource="http://purl.org/heritagedata/schemes/571/concepts/151681"/>
    <skos:narrower rdf:resource="http://purl.org/heritagedata/schemes/571/concepts/152583"/>
    <skos:broader rdf:resource="http://purl.org/heritagedata/schemes/571/concepts/151648"/>
    <skos:inScheme rdf:resource="http://purl.org/heritagedata/schemes/571"/>
    <dc:identifier>http://purl.org/heritagedata/schemes/571/concepts/151678</dc:identifier>
    <dc:issued rdf:datatype="http://www.w3.org/2001/XMLSchema#dateTime">2024-07-01T17:17:33</dc:issued>
    <cc:license rdf:resource="https://www.nationalarchives.gov.uk/doc/open-government-licence/version/3/"/>
    <cc:attributionURL rdf:resource="https://historicengland.org.uk/"/>
    <cc:attributionName xml:lang="en">Historic England</cc:attributionName>
    <dc:publisher rdf:resource="https://historicengland.org.uk/"/>
    <dc:spatial rdf:resource="http://vocab.getty.edu/tgn/7002445"/>
    <dc:spatial rdf:resource="http://dbpedia.org/resource/England"/>
    <skos:prefLabel xml:lang="en">Navigation</skos:prefLabel>
    <skos:scopeNote xml:lang="en">Areas relating to safe passage and route-finding for travel or transport on or in the water, whether inland, coastal or marine.</skos:scopeNote>
  </skos:Concept>

  <skos:Concept rdf:about="http://purl.org/heritagedata/schemes/571/concepts/151106">
    <skos:broader rdf:resource="http://purl.org/heritagedata/schemes/571/concepts/151681"/>
    <skos:inScheme rdf:resource="http://purl.org/heritagedata/schemes/571"/>
    <dc:identifier>http://purl.org/heritagedata/schemes/571/concepts/151106</dc:identifier>
    <dc:issued rdf:datatype="http://www.w3.org/2001/XMLSchema#dateTime">2024-07-01T17:17:33</dc:issued>
    <cc:license rdf:resource="https://www.nationalarchives.gov.uk/doc/open-government-licence/version/3/"/>
    <cc:attributionURL rdf:resource="https://historicengland.org.uk/"/>
    <cc:attributionName xml:lang="en">Historic England</cc:attributionName>
    <dc:publisher rdf:resource="https://historicengland.org.uk/"/>
    <dc:spatial rdf:resource="http://vocab.getty.edu/tgn/7002445"/>
    <dc:spatial rdf:resource="http://dbpedia.org/resource/England"/>
    <skos:prefLabel xml:lang="en">Wreck Hazard</skos:prefLabel>
    <skos:scopeNote xml:lang="en">Relates to the area of the hazard which may include a single wreck or a cluster of several. Wrecks have greatest relevance from their roles as hazards to navigational activity, or as indicators of areas and routes of past navigational or trading activity.</skos:scopeNote>
  </skos:Concept>

  <skos:Concept rdf:about="http://purl.org/heritagedata/schemes/571/concepts/151681">
    <skos:narrower rdf:resource="http://purl.org/heritagedata/schemes/571/concepts/151106"/>
    <skos:narrower>
      <skos:Concept rdf:about="http://purl.org/heritagedata/schemes/571/concepts/151107">
        <skos:broader rdf:resource="http://purl.org/heritagedata/schemes/571/concepts/151681"/>
        <skos:inScheme rdf:resource="http://purl.org/heritagedata/schemes/571"/>
        <dc:identifier>http://purl.org/heritagedata/schemes/571/concepts/151107</dc:identifier>
        <dc:issued rdf:datatype="http://www.w3.org/2001/XMLSchema#dateTime">2024-07-01T17:17:33</dc:issued>
        <cc:license rdf:resource="https://www.nationalarchives.gov.uk/doc/open-government-licence/version/3/"/>
        <cc:attributionURL rdf:resource="https://historicengland.org.uk/"/>
        <cc:attributionName xml:lang="en">Historic England</cc:attributionName>
        <dc:publisher rdf:resource="https://historicengland.org.uk/"/>
        <dc:spatial rdf:resource="http://vocab.getty.edu/tgn/7002445"/>
        <dc:spatial rdf:resource="http://dbpedia.org/resource/England"/>
        <skos:prefLabel xml:lang="en">Shallows</skos:prefLabel>
        <skos:scopeNote xml:lang="en">An area of the sea, a lake, or a river where the water is not very deep.</skos:scopeNote>
      </skos:Concept>
    </skos:narrower>

    <skos:narrower>
      <skos:Concept rdf:about="http://purl.org/heritagedata/schemes/571/concepts/152529">
        <skos:broader rdf:resource="http://purl.org/heritagedata/schemes/571/concepts/151681"/>
        <skos:inScheme rdf:resource="http://purl.org/heritagedata/schemes/571"/>
        <dc:identifier>http://purl.org/heritagedata/schemes/571/concepts/152529</dc:identifier>
        <dc:issued rdf:datatype="http://www.w3.org/2001/XMLSchema#dateTime">2024-07-01T17:17:33</dc:issued>
        <cc:license rdf:resource="https://www.nationalarchives.gov.uk/doc/open-government-licence/version/3/"/>
        <cc:attributionURL rdf:resource="https://historicengland.org.uk/"/>
        <cc:attributionName xml:lang="en">Historic England</cc:attributionName>
        <dc:publisher rdf:resource="https://historicengland.org.uk/"/>
        <dc:spatial rdf:resource="http://vocab.getty.edu/tgn/7002445"/>
        <dc:spatial rdf:resource="http://dbpedia.org/resource/England"/>
        <skos:prefLabel xml:lang="en">Drying Hazard</skos:prefLabel>
        <skos:scopeNote xml:lang="en">Areas variously submerged but also subject to exposure above the sea surface at various states of the tide, known as 'drying areas' and forming a hazard to the safe passage of shipping.</skos:scopeNote>
      </skos:Concept>
    </skos:narrower>

    <skos:narrower>
      <skos:Concept rdf:about="http://purl.org/heritagedata/schemes/571/concepts/152530">
        <skos:broader rdf:resource="http://purl.org/heritagedata/schemes/571/concepts/151681"/>
        <skos:inScheme rdf:resource="http://purl.org/heritagedata/schemes/571"/>
        <dc:identifier>http://purl.org/heritagedata/schemes/571/concepts/152530</dc:identifier>
        <dc:issued rdf:datatype="http://www.w3.org/2001/XMLSchema#dateTime">2024-07-01T17:17:33</dc:issued>
        <cc:license rdf:resource="https://www.nationalarchives.gov.uk/doc/open-government-licence/version/3/"/>
        <cc:attributionURL rdf:resource="https://historicengland.org.uk/"/>
        <cc:attributionName xml:lang="en">Historic England</cc:attributionName>
        <dc:publisher rdf:resource="https://historicengland.org.uk/"/>
        <dc:spatial rdf:resource="http://vocab.getty.edu/tgn/7002445"/>
        <dc:spatial rdf:resource="http://dbpedia.org/resource/England"/>
        <skos:prefLabel xml:lang="en">Maritime Debris</skos:prefLabel>
        <skos:scopeNote xml:lang="en">An area deemed hazardous due to a predominance of recorded obstructions and fouls not known to be associated with a wreck.</skos:scopeNote>
      </skos:Concept>
    </skos:narrower>

    <skos:narrower>
      <skos:Concept rdf:about="http://purl.org/heritagedata/schemes/571/concepts/152531">
        <skos:broader rdf:resource="http://purl.org/heritagedata/schemes/571/concepts/151681"/>
        <skos:inScheme rdf:resource="http://purl.org/heritagedata/schemes/571"/>
        <dc:identifier>http://purl.org/heritagedata/schemes/571/concepts/152531</dc:identifier>
        <dc:issued rdf:datatype="http://www.w3.org/2001/XMLSchema#dateTime">2024-07-01T17:17:33</dc:issued>
        <cc:license rdf:resource="https://www.nationalarchives.gov.uk/doc/open-government-licence/version/3/"/>
        <cc:attributionURL rdf:resource="https://historicengland.org.uk/"/>
        <cc:attributionName xml:lang="en">Historic England</cc:attributionName>
        <dc:publisher rdf:resource="https://historicengland.org.uk/"/>
        <dc:spatial rdf:resource="http://vocab.getty.edu/tgn/7002445"/>
        <dc:spatial rdf:resource="http://dbpedia.org/resource/England"/>
        <skos:prefLabel xml:lang="en">Rock Outcrops</skos:prefLabel>
        <skos:scopeNote xml:lang="en">An area dominated by rocks rising from the general level of the seabed and breaking the sea surface at some or all states of the tide, posing a risk for navigation.</skos:scopeNote>
      </skos:Concept>
    </skos:narrower>

    <skos:narrower>
      <skos:Concept rdf:about="http://purl.org/heritagedata/schemes/571/concepts/152532">
        <skos:broader rdf:resource="http://purl.org/heritagedata/schemes/571/concepts/151681"/>
        <skos:inScheme rdf:resource="http://purl.org/heritagedata/schemes/571"/>
        <dc:identifier>http://purl.org/heritagedata/schemes/571/concepts/152532</dc:identifier>
        <dc:issued rdf:datatype="http://www.w3.org/2001/XMLSchema#dateTime">2024-07-01T17:17:33</dc:issued>
        <cc:license rdf:resource="https://www.nationalarchives.gov.uk/doc/open-government-licence/version/3/"/>
        <cc:attributionURL rdf:resource="https://historicengland.org.uk/"/>
        <cc:attributionName xml:lang="en">Historic England</cc:attributionName>
        <dc:publisher rdf:resource="https://historicengland.org.uk/"/>
        <dc:spatial rdf:resource="http://vocab.getty.edu/tgn/7002445"/>
        <dc:spatial rdf:resource="http://dbpedia.org/resource/England"/>
        <skos:prefLabel xml:lang="en">Water Turbulence</skos:prefLabel>
        <skos:scopeNote xml:lang="en">Areas of the water column and/or sea surface characterised by heavy swell, strong currents and tidal races which pose a risk for navigation.</skos:scopeNote>
      </skos:Concept>
    </skos:narrower>

    <skos:narrower>
      <skos:Concept rdf:about="http://purl.org/heritagedata/schemes/571/concepts/152533">
        <skos:broader rdf:resource="http://purl.org/heritagedata/schemes/571/concepts/151681"/>
        <skos:inScheme rdf:resource="http://purl.org/heritagedata/schemes/571"/>
        <dc:identifier>http://purl.org/heritagedata/schemes/571/concepts/152533</dc:identifier>
        <dc:issued rdf:datatype="http://www.w3.org/2001/XMLSchema#dateTime">2024-07-01T17:17:33</dc:issued>
        <cc:license rdf:resource="https://www.nationalarchives.gov.uk/doc/open-government-licence/version/3/"/>
        <cc:attributionURL rdf:resource="https://historicengland.org.uk/"/>
        <cc:attributionName xml:lang="en">Historic England</cc:attributionName>
        <dc:publisher rdf:resource="https://historicengland.org.uk/"/>
        <dc:spatial rdf:resource="http://vocab.getty.edu/tgn/7002445"/>
        <dc:spatial rdf:resource="http://dbpedia.org/resource/England"/>
        <skos:prefLabel xml:lang="en">Hazardous Water</skos:prefLabel>
        <skos:scopeNote xml:lang="en">Areas of the water column and/or sea surface above sea floor hazards and in a buffered zone around them.</skos:scopeNote>
      </skos:Concept>
    </skos:narrower>

    <skos:narrower rdf:resource="http://purl.org/heritagedata/schemes/571/concepts/152534"/>
    <skos:narrower>
      <skos:Concept rdf:about="http://purl.org/heritagedata/schemes/571/concepts/152535">
        <skos:broader rdf:resource="http://purl.org/heritagedata/schemes/571/concepts/151681"/>
        <skos:inScheme rdf:resource="http://purl.org/heritagedata/schemes/571"/>
        <dc:identifier>http://purl.org/heritagedata/schemes/571/concepts/152535</dc:identifier>
        <dc:issued rdf:datatype="http://www.w3.org/2001/XMLSchema#dateTime">2024-07-01T17:17:33</dc:issued>
        <cc:license rdf:resource="https://www.nationalarchives.gov.uk/doc/open-government-licence/version/3/"/>
        <cc:attributionURL rdf:resource="https://historicengland.org.uk/"/>
        <cc:attributionName xml:lang="en">Historic England</cc:attributionName>
        <dc:publisher rdf:resource="https://historicengland.org.uk/"/>
        <dc:spatial rdf:resource="http://vocab.getty.edu/tgn/7002445"/>
        <dc:spatial rdf:resource="http://dbpedia.org/resource/England"/>
        <skos:prefLabel xml:lang="en">Submerged Rocks</skos:prefLabel>
        <skos:scopeNote xml:lang="en">Areas dominated by rocks rising from the general level of the seabed but not breaking the surface of the water at any state of the tide, posing a risk for navigation.</skos:scopeNote>
      </skos:Concept>
    </skos:narrower>

    <skos:broader rdf:resource="http://purl.org/heritagedata/schemes/571/concepts/151678"/>
    <skos:inScheme rdf:resource="http://purl.org/heritagedata/schemes/571"/>
    <dc:identifier>http://purl.org/heritagedata/schemes/571/concepts/151681</dc:identifier>
    <dc:issued rdf:datatype="http://www.w3.org/2001/XMLSchema#dateTime">2024-07-01T17:17:33</dc:issued>
    <cc:license rdf:resource="https://www.nationalarchives.gov.uk/doc/open-government-licence/version/3/"/>
    <cc:attributionURL rdf:resource="https://historicengland.org.uk/"/>
    <cc:attributionName xml:lang="en">Historic England</cc:attributionName>
    <dc:publisher rdf:resource="https://historicengland.org.uk/"/>
    <dc:spatial rdf:resource="http://vocab.getty.edu/tgn/7002445"/>
    <dc:spatial rdf:resource="http://dbpedia.org/resource/England"/>
    <skos:prefLabel xml:lang="en">Navigation Hazard</skos:prefLabel>
    <skos:scopeNote xml:lang="en">Areas that contain serious risks to vessels which could lead to their damage or complete loss. Such risks may be directly related to sea floor features and aspects, such as wrecks and other seafloor debris and obstructions.</skos:scopeNote>
  </skos:Concept>

  <skos:Concept rdf:about="http://purl.org/heritagedata/schemes/571/concepts/151108">
    <skos:broader rdf:resource="http://purl.org/heritagedata/schemes/571/concepts/152539"/>
    <skos:inScheme rdf:resource="http://purl.org/heritagedata/schemes/571"/>
    <dc:identifier>http://purl.org/heritagedata/schemes/571/concepts/151108</dc:identifier>
    <dc:issued rdf:datatype="http://www.w3.org/2001/XMLSchema#dateTime">2024-07-01T17:17:33</dc:issued>
    <cc:license rdf:resource="https://www.nationalarchives.gov.uk/doc/open-government-licence/version/3/"/>
    <cc:attributionURL rdf:resource="https://historicengland.org.uk/"/>
    <cc:attributionName xml:lang="en">Historic England</cc:attributionName>
    <dc:publisher rdf:resource="https://historicengland.org.uk/"/>
    <dc:spatial rdf:resource="http://vocab.getty.edu/tgn/7002445"/>
    <dc:spatial rdf:resource="http://dbpedia.org/resource/England"/>
    <skos:prefLabel xml:lang="en">Lighthouse</skos:prefLabel>
    <skos:scopeNote xml:lang="en">A tower or structure, with a powerful light or lights at the top, usually erected at an important or dangerous point on or near the sea-coast for the warning and guidance of mariners, but may also be sited inland.</skos:scopeNote>
  </skos:Concept>

  <skos:Concept rdf:about="http://purl.org/heritagedata/schemes/571/concepts/152539">
    <skos:narrower rdf:resource="http://purl.org/heritagedata/schemes/571/concepts/151108"/>
    <skos:narrower>
      <skos:Concept rdf:about="http://purl.org/heritagedata/schemes/571/concepts/151109">
        <skos:broader rdf:resource="http://purl.org/heritagedata/schemes/571/concepts/152539"/>
        <skos:inScheme rdf:resource="http://purl.org/heritagedata/schemes/571"/>
        <dc:identifier>http://purl.org/heritagedata/schemes/571/concepts/151109</dc:identifier>
        <dc:issued rdf:datatype="http://www.w3.org/2001/XMLSchema#dateTime">2024-07-01T17:17:33</dc:issued>
        <cc:license rdf:resource="https://www.nationalarchives.gov.uk/doc/open-government-licence/version/3/"/>
        <cc:attributionURL rdf:resource="https://historicengland.org.uk/"/>
        <cc:attributionName xml:lang="en">Historic England</cc:attributionName>
        <dc:publisher rdf:resource="https://historicengland.org.uk/"/>
        <dc:spatial rdf:resource="http://vocab.getty.edu/tgn/7002445"/>
        <dc:spatial rdf:resource="http://dbpedia.org/resource/England"/>
        <skos:prefLabel xml:lang="en">Buoyage</skos:prefLabel>
        <skos:scopeNote xml:lang="en">Floating, fixed markers indicating to a navigator a sea area to approach or avoid. Single or arrangements of buoys, beacons and lights are often used to demarcate safely navigable entrances to estuaries and rivers, submerged hazards and foul areas.</skos:scopeNote>
      </skos:Concept>
    </skos:narrower>

    <skos:narrower>
      <skos:Concept rdf:about="http://purl.org/heritagedata/schemes/571/concepts/151110">
        <skos:broader rdf:resource="http://purl.org/heritagedata/schemes/571/concepts/152539"/>
        <skos:inScheme rdf:resource="http://purl.org/heritagedata/schemes/571"/>
        <dc:identifier>http://purl.org/heritagedata/schemes/571/concepts/151110</dc:identifier>
        <dc:issued rdf:datatype="http://www.w3.org/2001/XMLSchema#dateTime">2024-07-01T17:17:33</dc:issued>
        <cc:license rdf:resource="https://www.nationalarchives.gov.uk/doc/open-government-licence/version/3/"/>
        <cc:attributionURL rdf:resource="https://historicengland.org.uk/"/>
        <cc:attributionName xml:lang="en">Historic England</cc:attributionName>
        <dc:publisher rdf:resource="https://historicengland.org.uk/"/>
        <dc:spatial rdf:resource="http://vocab.getty.edu/tgn/7002445"/>
        <dc:spatial rdf:resource="http://dbpedia.org/resource/England"/>
        <skos:prefLabel xml:lang="en">Coastguard Station</skos:prefLabel>
        <skos:scopeNote xml:lang="en">A building or group of buildings situated close to the sea used by coastguards, or a volunteer coastwatch, to enable them to monitor the coastline.</skos:scopeNote>
      </skos:Concept>
    </skos:narrower>

    <skos:narrower>
      <skos:Concept rdf:about="http://purl.org/heritagedata/schemes/571/concepts/151111">
        <skos:broader rdf:resource="http://purl.org/heritagedata/schemes/571/concepts/152539"/>
        <skos:inScheme rdf:resource="http://purl.org/heritagedata/schemes/571"/>
        <dc:identifier>http://purl.org/heritagedata/schemes/571/concepts/151111</dc:identifier>
        <dc:issued rdf:datatype="http://www.w3.org/2001/XMLSchema#dateTime">2024-07-01T17:17:33</dc:issued>
        <cc:license rdf:resource="https://www.nationalarchives.gov.uk/doc/open-government-licence/version/3/"/>
        <cc:attributionURL rdf:resource="https://historicengland.org.uk/"/>
        <cc:attributionName xml:lang="en">Historic England</cc:attributionName>
        <dc:publisher rdf:resource="https://historicengland.org.uk/"/>
        <dc:spatial rdf:resource="http://vocab.getty.edu/tgn/7002445"/>
        <dc:spatial rdf:resource="http://dbpedia.org/resource/England"/>
        <skos:prefLabel xml:lang="en">Lifeboat Station</skos:prefLabel>
        <skos:scopeNote xml:lang="en">A building designed to house a lifeboat, usually with a ramp to launch the boat into the sea.</skos:scopeNote>
      </skos:Concept>
    </skos:narrower>

    <skos:narrower>
      <skos:Concept rdf:about="http://purl.org/heritagedata/schemes/571/concepts/151112">
        <skos:broader rdf:resource="http://purl.org/heritagedata/schemes/571/concepts/152539"/>
        <skos:inScheme rdf:resource="http://purl.org/heritagedata/schemes/571"/>
        <dc:identifier>http://purl.org/heritagedata/schemes/571/concepts/151112</dc:identifier>
        <dc:issued rdf:datatype="http://www.w3.org/2001/XMLSchema#dateTime">2024-07-01T17:17:33</dc:issued>
        <cc:license rdf:resource="https://www.nationalarchives.gov.uk/doc/open-government-licence/version/3/"/>
        <cc:attributionURL rdf:resource="https://historicengland.org.uk/"/>
        <cc:attributionName xml:lang="en">Historic England</cc:attributionName>
        <dc:publisher rdf:resource="https://historicengland.org.uk/"/>
        <dc:spatial rdf:resource="http://vocab.getty.edu/tgn/7002445"/>
        <dc:spatial rdf:resource="http://dbpedia.org/resource/England"/>
        <skos:prefLabel xml:lang="en">Rocket Station</skos:prefLabel>
        <skos:scopeNote xml:lang="en">A coastal site containing equipment that enabled a lifeline to be fired at stricken ships that were close to the coastline.</skos:scopeNote>
      </skos:Concept>
    </skos:narrower>

    <skos:narrower rdf:resource="http://purl.org/heritagedata/schemes/571/concepts/151679"/>
    <skos:narrower rdf:resource="http://purl.org/heritagedata/schemes/571/concepts/152523"/>
    <skos:narrower>
      <skos:Concept rdf:about="http://purl.org/heritagedata/schemes/571/concepts/152540">
        <skos:broader rdf:resource="http://purl.org/heritagedata/schemes/571/concepts/152539"/>
        <skos:inScheme rdf:resource="http://purl.org/heritagedata/schemes/571"/>
        <dc:identifier>http://purl.org/heritagedata/schemes/571/concepts/152540</dc:identifier>
        <dc:issued rdf:datatype="http://www.w3.org/2001/XMLSchema#dateTime">2024-07-01T17:17:33</dc:issued>
        <cc:license rdf:resource="https://www.nationalarchives.gov.uk/doc/open-government-licence/version/3/"/>
        <cc:attributionURL rdf:resource="https://historicengland.org.uk/"/>
        <cc:attributionName xml:lang="en">Historic England</cc:attributionName>
        <dc:publisher rdf:resource="https://historicengland.org.uk/"/>
        <dc:spatial rdf:resource="http://vocab.getty.edu/tgn/7002445"/>
        <dc:spatial rdf:resource="http://dbpedia.org/resource/England"/>
        <skos:prefLabel xml:lang="en">Safety Area</skos:prefLabel>
        <skos:scopeNote xml:lang="en">An area of sea with advised or designated restrictions on navigation, or exclusion from permitted navigation altogether. These areas may respond to a variety of dangers.</skos:scopeNote>
      </skos:Concept>
    </skos:narrower>

    <skos:broader rdf:resource="http://purl.org/heritagedata/schemes/571/concepts/151648"/>
    <skos:inScheme rdf:resource="http://purl.org/heritagedata/schemes/571"/>
    <dc:identifier>http://purl.org/heritagedata/schemes/571/concepts/152539</dc:identifier>
    <dc:issued rdf:datatype="http://www.w3.org/2001/XMLSchema#dateTime">2024-07-01T17:17:33</dc:issued>
    <cc:license rdf:resource="https://www.nationalarchives.gov.uk/doc/open-government-licence/version/3/"/>
    <cc:attributionURL rdf:resource="https://historicengland.org.uk/"/>
    <cc:attributionName xml:lang="en">Historic England</cc:attributionName>
    <dc:publisher rdf:resource="https://historicengland.org.uk/"/>
    <dc:spatial rdf:resource="http://vocab.getty.edu/tgn/7002445"/>
    <dc:spatial rdf:resource="http://dbpedia.org/resource/England"/>
    <skos:prefLabel xml:lang="en">Maritime Safety</skos:prefLabel>
    <skos:scopeNote xml:lang="en">Features or structures sited at important position-finding or dangerous points on the coast, or on inland waters, for the guidance and warning of mariners.</skos:scopeNote>
  </skos:Concept>

  <skos:Concept rdf:about="http://purl.org/heritagedata/schemes/571/concepts/151113">
    <skos:broader rdf:resource="http://purl.org/heritagedata/schemes/571/concepts/151651"/>
    <skos:narrower>
      <skos:Concept rdf:about="http://purl.org/heritagedata/schemes/571/concepts/151117">
        <skos:broader rdf:resource="http://purl.org/heritagedata/schemes/571/concepts/151113"/>
        <skos:inScheme rdf:resource="http://purl.org/heritagedata/schemes/571"/>
        <dc:identifier>http://purl.org/heritagedata/schemes/571/concepts/151117</dc:identifier>
        <dc:issued rdf:datatype="http://www.w3.org/2001/XMLSchema#dateTime">2024-07-01T17:17:33</dc:issued>
        <cc:license rdf:resource="https://www.nationalarchives.gov.uk/doc/open-government-licence/version/3/"/>
        <cc:attributionURL rdf:resource="https://historicengland.org.uk/"/>
        <cc:attributionName xml:lang="en">Historic England</cc:attributionName>
        <dc:publisher rdf:resource="https://historicengland.org.uk/"/>
        <dc:spatial rdf:resource="http://vocab.getty.edu/tgn/7002445"/>
        <dc:spatial rdf:resource="http://dbpedia.org/resource/England"/>
        <skos:prefLabel xml:lang="en">Motorway</skos:prefLabel>
        <skos:scopeNote xml:lang="en">Large multiple carriageway for fast-moving motor traffic, continuing for long distances without traffic intersections and subject to legally specified 'motorway regulations'.</skos:scopeNote>
      </skos:Concept>
    </skos:narrower>

    <skos:narrower>
      <skos:Concept rdf:about="http://purl.org/heritagedata/schemes/571/concepts/151118">
        <skos:broader rdf:resource="http://purl.org/heritagedata/schemes/571/concepts/151113"/>
        <skos:inScheme rdf:resource="http://purl.org/heritagedata/schemes/571"/>
        <dc:identifier>http://purl.org/heritagedata/schemes/571/concepts/151118</dc:identifier>
        <dc:issued rdf:datatype="http://www.w3.org/2001/XMLSchema#dateTime">2024-07-01T17:17:33</dc:issued>
        <cc:license rdf:resource="https://www.nationalarchives.gov.uk/doc/open-government-licence/version/3/"/>
        <cc:attributionURL rdf:resource="https://historicengland.org.uk/"/>
        <cc:attributionName xml:lang="en">Historic England</cc:attributionName>
        <dc:publisher rdf:resource="https://historicengland.org.uk/"/>
        <dc:spatial rdf:resource="http://vocab.getty.edu/tgn/7002445"/>
        <dc:spatial rdf:resource="http://dbpedia.org/resource/England"/>
        <skos:prefLabel xml:lang="en">Trunk Road</skos:prefLabel>
        <skos:scopeNote xml:lang="en">Large road, often multiple carriagewayed, linking significant places.</skos:scopeNote>
      </skos:Concept>
    </skos:narrower>

    <skos:inScheme rdf:resource="http://purl.org/heritagedata/schemes/571"/>
    <dc:identifier>http://purl.org/heritagedata/schemes/571/concepts/151113</dc:identifier>
    <dc:issued rdf:datatype="http://www.w3.org/2001/XMLSchema#dateTime">2024-07-01T17:17:33</dc:issued>
    <cc:license rdf:resource="https://www.nationalarchives.gov.uk/doc/open-government-licence/version/3/"/>
    <cc:attributionURL rdf:resource="https://historicengland.org.uk/"/>
    <cc:attributionName xml:lang="en">Historic England</cc:attributionName>
    <dc:publisher rdf:resource="https://historicengland.org.uk/"/>
    <dc:spatial rdf:resource="http://vocab.getty.edu/tgn/7002445"/>
    <dc:spatial rdf:resource="http://dbpedia.org/resource/England"/>
    <skos:prefLabel xml:lang="en">Road</skos:prefLabel>
    <skos:scopeNote xml:lang="en">A way suitable for wheeled transport.</skos:scopeNote>
  </skos:Concept>

  <skos:Concept rdf:about="http://purl.org/heritagedata/schemes/571/concepts/151651">
    <skos:narrower rdf:resource="http://purl.org/heritagedata/schemes/571/concepts/151113"/>
    <skos:narrower>
      <skos:Concept rdf:about="http://purl.org/heritagedata/schemes/571/concepts/151120">
        <skos:broader rdf:resource="http://purl.org/heritagedata/schemes/571/concepts/151651"/>
        <skos:inScheme rdf:resource="http://purl.org/heritagedata/schemes/571"/>
        <dc:identifier>http://purl.org/heritagedata/schemes/571/concepts/151120</dc:identifier>
        <dc:issued rdf:datatype="http://www.w3.org/2001/XMLSchema#dateTime">2024-07-01T17:17:33</dc:issued>
        <cc:license rdf:resource="https://www.nationalarchives.gov.uk/doc/open-government-licence/version/3/"/>
        <cc:attributionURL rdf:resource="https://historicengland.org.uk/"/>
        <cc:attributionName xml:lang="en">Historic England</cc:attributionName>
        <dc:publisher rdf:resource="https://historicengland.org.uk/"/>
        <dc:spatial rdf:resource="http://vocab.getty.edu/tgn/7002445"/>
        <dc:spatial rdf:resource="http://dbpedia.org/resource/England"/>
        <skos:prefLabel xml:lang="en">Car Park</skos:prefLabel>
        <skos:scopeNote xml:lang="en">Area for parking motor vehicles; usually with permanent surfacing, sometimes in purpose-built multi-storey buildings.</skos:scopeNote>
      </skos:Concept>
    </skos:narrower>

    <skos:narrower>
      <skos:Concept rdf:about="http://purl.org/heritagedata/schemes/571/concepts/151164">
        <skos:broader rdf:resource="http://purl.org/heritagedata/schemes/571/concepts/151651"/>
        <skos:inScheme rdf:resource="http://purl.org/heritagedata/schemes/571"/>
        <dc:identifier>http://purl.org/heritagedata/schemes/571/concepts/151164</dc:identifier>
        <dc:issued rdf:datatype="http://www.w3.org/2001/XMLSchema#dateTime">2024-07-01T17:17:33</dc:issued>
        <cc:license rdf:resource="https://www.nationalarchives.gov.uk/doc/open-government-licence/version/3/"/>
        <cc:attributionURL rdf:resource="https://historicengland.org.uk/"/>
        <cc:attributionName xml:lang="en">Historic England</cc:attributionName>
        <dc:publisher rdf:resource="https://historicengland.org.uk/"/>
        <dc:spatial rdf:resource="http://vocab.getty.edu/tgn/7002445"/>
        <dc:spatial rdf:resource="http://dbpedia.org/resource/England"/>
        <skos:prefLabel xml:lang="en">Service Station</skos:prefLabel>
        <skos:scopeNote xml:lang="en">A commercial complex, usually sited along motorways or trunk roads, providing facilities such as car parking, restaurants, shop and fuel stations.</skos:scopeNote>
      </skos:Concept>
    </skos:narrower>

    <skos:narrower>
      <skos:Concept rdf:about="http://purl.org/heritagedata/schemes/571/concepts/151168">
        <skos:broader rdf:resource="http://purl.org/heritagedata/schemes/571/concepts/151651"/>
        <skos:inScheme rdf:resource="http://purl.org/heritagedata/schemes/571"/>
        <dc:identifier>http://purl.org/heritagedata/schemes/571/concepts/151168</dc:identifier>
        <dc:issued rdf:datatype="http://www.w3.org/2001/XMLSchema#dateTime">2024-07-01T17:17:33</dc:issued>
        <cc:license rdf:resource="https://www.nationalarchives.gov.uk/doc/open-government-licence/version/3/"/>
        <cc:attributionURL rdf:resource="https://historicengland.org.uk/"/>
        <cc:attributionName xml:lang="en">Historic England</cc:attributionName>
        <dc:publisher rdf:resource="https://historicengland.org.uk/"/>
        <dc:spatial rdf:resource="http://vocab.getty.edu/tgn/7002445"/>
        <dc:spatial rdf:resource="http://dbpedia.org/resource/England"/>
        <skos:prefLabel xml:lang="en">Road Junction Complex</skos:prefLabel>
        <skos:scopeNote xml:lang="en">A place where several roads meet, often negotiated using roundabouts.</skos:scopeNote>
      </skos:Concept>
    </skos:narrower>

    <skos:narrower>
      <skos:Concept rdf:about="http://purl.org/heritagedata/schemes/571/concepts/151403">
        <skos:broader rdf:resource="http://purl.org/heritagedata/schemes/571/concepts/151651"/>
        <skos:inScheme rdf:resource="http://purl.org/heritagedata/schemes/571"/>
        <dc:identifier>http://purl.org/heritagedata/schemes/571/concepts/151403</dc:identifier>
        <dc:issued rdf:datatype="http://www.w3.org/2001/XMLSchema#dateTime">2024-07-01T17:17:33</dc:issued>
        <cc:license rdf:resource="https://www.nationalarchives.gov.uk/doc/open-government-licence/version/3/"/>
        <cc:attributionURL rdf:resource="https://historicengland.org.uk/"/>
        <cc:attributionName xml:lang="en">Historic England</cc:attributionName>
        <dc:publisher rdf:resource="https://historicengland.org.uk/"/>
        <dc:spatial rdf:resource="http://vocab.getty.edu/tgn/7002445"/>
        <dc:spatial rdf:resource="http://dbpedia.org/resource/England"/>
        <skos:prefLabel xml:lang="en">Park And Ride</skos:prefLabel>
        <skos:scopeNote xml:lang="en">Car parks with connections to public transport that allow people wishing to travel into busy areas to leave their vehicles and transfer to public transport for the remainder of their trip. Usually on the outskirts of towns and cities.</skos:scopeNote>
      </skos:Concept>
    </skos:narrower>

    <skos:narrower>
      <skos:Concept rdf:about="http://purl.org/heritagedata/schemes/571/concepts/151657">
        <skos:broader rdf:resource="http://purl.org/heritagedata/schemes/571/concepts/151651"/>
        <skos:inScheme rdf:resource="http://purl.org/heritagedata/schemes/571"/>
        <dc:identifier>http://purl.org/heritagedata/schemes/571/concepts/151657</dc:identifier>
        <dc:issued rdf:datatype="http://www.w3.org/2001/XMLSchema#dateTime">2024-07-01T17:17:33</dc:issued>
        <cc:license rdf:resource="https://www.nationalarchives.gov.uk/doc/open-government-licence/version/3/"/>
        <cc:attributionURL rdf:resource="https://historicengland.org.uk/"/>
        <cc:attributionName xml:lang="en">Historic England</cc:attributionName>
        <dc:publisher rdf:resource="https://historicengland.org.uk/"/>
        <dc:spatial rdf:resource="http://vocab.getty.edu/tgn/7002445"/>
        <dc:spatial rdf:resource="http://dbpedia.org/resource/England"/>
        <skos:prefLabel xml:lang="en">Road Bridge</skos:prefLabel>
        <skos:scopeNote xml:lang="en">A bridge carrying a road.</skos:scopeNote>
      </skos:Concept>
    </skos:narrower>

    <skos:narrower>
      <skos:Concept rdf:about="http://purl.org/heritagedata/schemes/571/concepts/160134">
        <skos:broader rdf:resource="http://purl.org/heritagedata/schemes/571/concepts/151651"/>
        <skos:inScheme rdf:resource="http://purl.org/heritagedata/schemes/571"/>
        <dc:identifier>http://purl.org/heritagedata/schemes/571/concepts/160134</dc:identifier>
        <dc:issued rdf:datatype="http://www.w3.org/2001/XMLSchema#dateTime">2024-07-01T17:17:33</dc:issued>
        <cc:license rdf:resource="https://www.nationalarchives.gov.uk/doc/open-government-licence/version/3/"/>
        <cc:attributionURL rdf:resource="https://historicengland.org.uk/"/>
        <cc:attributionName xml:lang="en">Historic England</cc:attributionName>
        <dc:publisher rdf:resource="https://historicengland.org.uk/"/>
        <dc:spatial rdf:resource="http://vocab.getty.edu/tgn/7002445"/>
        <dc:spatial rdf:resource="http://dbpedia.org/resource/England"/>
        <skos:prefLabel xml:lang="en">Road Tunnel</skos:prefLabel>
        <skos:scopeNote xml:lang="en">A tunnel through which a road runs.</skos:scopeNote>
      </skos:Concept>
    </skos:narrower>

    <skos:broader rdf:resource="http://purl.org/heritagedata/schemes/571/concepts/151449"/>
    <skos:inScheme rdf:resource="http://purl.org/heritagedata/schemes/571"/>
    <dc:identifier>http://purl.org/heritagedata/schemes/571/concepts/151651</dc:identifier>
    <dc:issued rdf:datatype="http://www.w3.org/2001/XMLSchema#dateTime">2024-07-01T17:17:33</dc:issued>
    <cc:license rdf:resource="https://www.nationalarchives.gov.uk/doc/open-government-licence/version/3/"/>
    <cc:attributionURL rdf:resource="https://historicengland.org.uk/"/>
    <cc:attributionName xml:lang="en">Historic England</cc:attributionName>
    <dc:publisher rdf:resource="https://historicengland.org.uk/"/>
    <dc:spatial rdf:resource="http://vocab.getty.edu/tgn/7002445"/>
    <dc:spatial rdf:resource="http://dbpedia.org/resource/England"/>
    <skos:prefLabel xml:lang="en">Road Transport</skos:prefLabel>
    <skos:scopeNote xml:lang="en">Buildings and structures associated with road transport.</skos:scopeNote>
  </skos:Concept>

  <skos:Concept rdf:about="http://purl.org/heritagedata/schemes/571/concepts/151114">
    <skos:broader rdf:resource="http://purl.org/heritagedata/schemes/571/concepts/151650"/>
    <skos:inScheme rdf:resource="http://purl.org/heritagedata/schemes/571"/>
    <dc:identifier>http://purl.org/heritagedata/schemes/571/concepts/151114</dc:identifier>
    <dc:issued rdf:datatype="http://www.w3.org/2001/XMLSchema#dateTime">2024-07-01T17:17:33</dc:issued>
    <cc:license rdf:resource="https://www.nationalarchives.gov.uk/doc/open-government-licence/version/3/"/>
    <cc:attributionURL rdf:resource="https://historicengland.org.uk/"/>
    <cc:attributionName xml:lang="en">Historic England</cc:attributionName>
    <dc:publisher rdf:resource="https://historicengland.org.uk/"/>
    <dc:spatial rdf:resource="http://vocab.getty.edu/tgn/7002445"/>
    <dc:spatial rdf:resource="http://dbpedia.org/resource/England"/>
    <skos:prefLabel xml:lang="en">Railway</skos:prefLabel>
    <skos:scopeNote xml:lang="en">System of rail tracks along which passenger carriages or goods wagons are moved, usually by locomotive engines. Usually includes beds, cuttings, embankments, tunnels etc.</skos:scopeNote>
  </skos:Concept>

  <skos:Concept rdf:about="http://purl.org/heritagedata/schemes/571/concepts/151650">
    <skos:narrower rdf:resource="http://purl.org/heritagedata/schemes/571/concepts/151114"/>
    <skos:narrower>
      <skos:Concept rdf:about="http://purl.org/heritagedata/schemes/571/concepts/151115">
        <skos:broader rdf:resource="http://purl.org/heritagedata/schemes/571/concepts/151650"/>
        <skos:inScheme rdf:resource="http://purl.org/heritagedata/schemes/571"/>
        <dc:identifier>http://purl.org/heritagedata/schemes/571/concepts/151115</dc:identifier>
        <dc:issued rdf:datatype="http://www.w3.org/2001/XMLSchema#dateTime">2024-07-01T17:17:33</dc:issued>
        <cc:license rdf:resource="https://www.nationalarchives.gov.uk/doc/open-government-licence/version/3/"/>
        <cc:attributionURL rdf:resource="https://historicengland.org.uk/"/>
        <cc:attributionName xml:lang="en">Historic England</cc:attributionName>
        <dc:publisher rdf:resource="https://historicengland.org.uk/"/>
        <dc:spatial rdf:resource="http://vocab.getty.edu/tgn/7002445"/>
        <dc:spatial rdf:resource="http://dbpedia.org/resource/England"/>
        <skos:prefLabel xml:lang="en">Railway Station</skos:prefLabel>
        <skos:scopeNote xml:lang="en">Where railway trains stop to load and unload passengers or freight. Includes buildings and directly related grounds.</skos:scopeNote>
      </skos:Concept>
    </skos:narrower>

    <skos:narrower>
      <skos:Concept rdf:about="http://purl.org/heritagedata/schemes/571/concepts/151116">
        <skos:broader rdf:resource="http://purl.org/heritagedata/schemes/571/concepts/151650"/>
        <skos:inScheme rdf:resource="http://purl.org/heritagedata/schemes/571"/>
        <dc:identifier>http://purl.org/heritagedata/schemes/571/concepts/151116</dc:identifier>
        <dc:issued rdf:datatype="http://www.w3.org/2001/XMLSchema#dateTime">2024-07-01T17:17:33</dc:issued>
        <cc:license rdf:resource="https://www.nationalarchives.gov.uk/doc/open-government-licence/version/3/"/>
        <cc:attributionURL rdf:resource="https://historicengland.org.uk/"/>
        <cc:attributionName xml:lang="en">Historic England</cc:attributionName>
        <dc:publisher rdf:resource="https://historicengland.org.uk/"/>
        <dc:spatial rdf:resource="http://vocab.getty.edu/tgn/7002445"/>
        <dc:spatial rdf:resource="http://dbpedia.org/resource/England"/>
        <skos:prefLabel xml:lang="en">Railyard</skos:prefLabel>
        <skos:scopeNote xml:lang="en">Complex, often attached to a railway station where engines, coaches and wagons are laid up and maintained.</skos:scopeNote>
      </skos:Concept>
    </skos:narrower>

    <skos:narrower>
      <skos:Concept rdf:about="http://purl.org/heritagedata/schemes/571/concepts/151165">
        <skos:broader rdf:resource="http://purl.org/heritagedata/schemes/571/concepts/151650"/>
        <skos:inScheme rdf:resource="http://purl.org/heritagedata/schemes/571"/>
        <dc:identifier>http://purl.org/heritagedata/schemes/571/concepts/151165</dc:identifier>
        <dc:issued rdf:datatype="http://www.w3.org/2001/XMLSchema#dateTime">2024-07-01T17:17:33</dc:issued>
        <cc:license rdf:resource="https://www.nationalarchives.gov.uk/doc/open-government-licence/version/3/"/>
        <cc:attributionURL rdf:resource="https://historicengland.org.uk/"/>
        <cc:attributionName xml:lang="en">Historic England</cc:attributionName>
        <dc:publisher rdf:resource="https://historicengland.org.uk/"/>
        <dc:spatial rdf:resource="http://vocab.getty.edu/tgn/7002445"/>
        <dc:spatial rdf:resource="http://dbpedia.org/resource/England"/>
        <skos:prefLabel xml:lang="en">Engine Shed</skos:prefLabel>
        <skos:scopeNote xml:lang="en">Long sheds, into which railway lines run, used to house railway engines.</skos:scopeNote>
      </skos:Concept>
    </skos:narrower>

    <skos:narrower>
      <skos:Concept rdf:about="http://purl.org/heritagedata/schemes/571/concepts/151166">
        <skos:broader rdf:resource="http://purl.org/heritagedata/schemes/571/concepts/151650"/>
        <skos:inScheme rdf:resource="http://purl.org/heritagedata/schemes/571"/>
        <dc:identifier>http://purl.org/heritagedata/schemes/571/concepts/151166</dc:identifier>
        <dc:issued rdf:datatype="http://www.w3.org/2001/XMLSchema#dateTime">2024-07-01T17:17:33</dc:issued>
        <cc:license rdf:resource="https://www.nationalarchives.gov.uk/doc/open-government-licence/version/3/"/>
        <cc:attributionURL rdf:resource="https://historicengland.org.uk/"/>
        <cc:attributionName xml:lang="en">Historic England</cc:attributionName>
        <dc:publisher rdf:resource="https://historicengland.org.uk/"/>
        <dc:spatial rdf:resource="http://vocab.getty.edu/tgn/7002445"/>
        <dc:spatial rdf:resource="http://dbpedia.org/resource/England"/>
        <skos:prefLabel xml:lang="en">Railway Siding</skos:prefLabel>
        <skos:scopeNote xml:lang="en">A short piece of track lying parallel to the main railway line enabling trains and trucks to either pass one another or be parked when not in use.</skos:scopeNote>
      </skos:Concept>
    </skos:narrower>

    <skos:narrower>
      <skos:Concept rdf:about="http://purl.org/heritagedata/schemes/571/concepts/151654">
        <skos:broader rdf:resource="http://purl.org/heritagedata/schemes/571/concepts/151650"/>
        <skos:inScheme rdf:resource="http://purl.org/heritagedata/schemes/571"/>
        <dc:identifier>http://purl.org/heritagedata/schemes/571/concepts/151654</dc:identifier>
        <dc:issued rdf:datatype="http://www.w3.org/2001/XMLSchema#dateTime">2024-07-01T17:17:33</dc:issued>
        <cc:license rdf:resource="https://www.nationalarchives.gov.uk/doc/open-government-licence/version/3/"/>
        <cc:attributionURL rdf:resource="https://historicengland.org.uk/"/>
        <cc:attributionName xml:lang="en">Historic England</cc:attributionName>
        <dc:publisher rdf:resource="https://historicengland.org.uk/"/>
        <dc:spatial rdf:resource="http://vocab.getty.edu/tgn/7002445"/>
        <dc:spatial rdf:resource="http://dbpedia.org/resource/England"/>
        <skos:prefLabel xml:lang="en">Railway Tunnel</skos:prefLabel>
        <skos:scopeNote xml:lang="en">A tunnel through which a railway line runs.</skos:scopeNote>
      </skos:Concept>
    </skos:narrower>

    <skos:narrower>
      <skos:Concept rdf:about="http://purl.org/heritagedata/schemes/571/concepts/151658">
        <skos:broader rdf:resource="http://purl.org/heritagedata/schemes/571/concepts/151650"/>
        <skos:inScheme rdf:resource="http://purl.org/heritagedata/schemes/571"/>
        <dc:identifier>http://purl.org/heritagedata/schemes/571/concepts/151658</dc:identifier>
        <dc:issued rdf:datatype="http://www.w3.org/2001/XMLSchema#dateTime">2024-07-01T17:17:33</dc:issued>
        <cc:license rdf:resource="https://www.nationalarchives.gov.uk/doc/open-government-licence/version/3/"/>
        <cc:attributionURL rdf:resource="https://historicengland.org.uk/"/>
        <cc:attributionName xml:lang="en">Historic England</cc:attributionName>
        <dc:publisher rdf:resource="https://historicengland.org.uk/"/>
        <dc:spatial rdf:resource="http://vocab.getty.edu/tgn/7002445"/>
        <dc:spatial rdf:resource="http://dbpedia.org/resource/England"/>
        <skos:prefLabel xml:lang="en">Railway Bridge</skos:prefLabel>
        <skos:scopeNote xml:lang="en">A bridge carrying a railway track.</skos:scopeNote>
      </skos:Concept>
    </skos:narrower>

    <skos:narrower>
      <skos:Concept rdf:about="http://purl.org/heritagedata/schemes/571/concepts/152562">
        <skos:broader rdf:resource="http://purl.org/heritagedata/schemes/571/concepts/151650"/>
        <skos:inScheme rdf:resource="http://purl.org/heritagedata/schemes/571"/>
        <dc:identifier>http://purl.org/heritagedata/schemes/571/concepts/152562</dc:identifier>
        <dc:issued rdf:datatype="http://www.w3.org/2001/XMLSchema#dateTime">2024-07-01T17:17:33</dc:issued>
        <cc:license rdf:resource="https://www.nationalarchives.gov.uk/doc/open-government-licence/version/3/"/>
        <cc:attributionURL rdf:resource="https://historicengland.org.uk/"/>
        <cc:attributionName xml:lang="en">Historic England</cc:attributionName>
        <dc:publisher rdf:resource="https://historicengland.org.uk/"/>
        <dc:spatial rdf:resource="http://vocab.getty.edu/tgn/7002445"/>
        <dc:spatial rdf:resource="http://dbpedia.org/resource/England"/>
        <skos:prefLabel xml:lang="en">Tramway</skos:prefLabel>
        <skos:scopeNote xml:lang="en">A light railway. Early usage tended to be in industrial contexts with animal drawn stock; later usage tended to be for the conveyance of passengers, often in urban areas, with vehicles run along sunken rails.</skos:scopeNote>
      </skos:Concept>
    </skos:narrower>

    <skos:broader rdf:resource="http://purl.org/heritagedata/schemes/571/concepts/151449"/>
    <skos:inScheme rdf:resource="http://purl.org/heritagedata/schemes/571"/>
    <dc:identifier>http://purl.org/heritagedata/schemes/571/concepts/151650</dc:identifier>
    <dc:issued rdf:datatype="http://www.w3.org/2001/XMLSchema#dateTime">2024-07-01T17:17:33</dc:issued>
    <cc:license rdf:resource="https://www.nationalarchives.gov.uk/doc/open-government-licence/version/3/"/>
    <cc:attributionURL rdf:resource="https://historicengland.org.uk/"/>
    <cc:attributionName xml:lang="en">Historic England</cc:attributionName>
    <dc:publisher rdf:resource="https://historicengland.org.uk/"/>
    <dc:spatial rdf:resource="http://vocab.getty.edu/tgn/7002445"/>
    <dc:spatial rdf:resource="http://dbpedia.org/resource/England"/>
    <skos:prefLabel xml:lang="en">Railway Transport</skos:prefLabel>
    <skos:scopeNote xml:lang="en">Buildings and structures associated with railway transport.</skos:scopeNote>
  </skos:Concept>

  <skos:Concept rdf:about="http://purl.org/heritagedata/schemes/571/concepts/151122">
    <skos:broader rdf:resource="http://purl.org/heritagedata/schemes/571/concepts/151444"/>
    <skos:inScheme rdf:resource="http://purl.org/heritagedata/schemes/571"/>
    <dc:identifier>http://purl.org/heritagedata/schemes/571/concepts/151122</dc:identifier>
    <dc:issued rdf:datatype="http://www.w3.org/2001/XMLSchema#dateTime">2024-07-01T17:17:33</dc:issued>
    <cc:license rdf:resource="https://www.nationalarchives.gov.uk/doc/open-government-licence/version/3/"/>
    <cc:attributionURL rdf:resource="https://historicengland.org.uk/"/>
    <cc:attributionName xml:lang="en">Historic England</cc:attributionName>
    <dc:publisher rdf:resource="https://historicengland.org.uk/"/>
    <dc:spatial rdf:resource="http://vocab.getty.edu/tgn/7002445"/>
    <dc:spatial rdf:resource="http://dbpedia.org/resource/England"/>
    <skos:prefLabel xml:lang="en">Lake</skos:prefLabel>
    <skos:scopeNote xml:lang="en">An inland body of fresh water. Lakes generally refer to larger examples, ponds to smaller, but there is no clear break along the gradation between the two.</skos:scopeNote>
  </skos:Concept>

  <skos:Concept rdf:about="http://purl.org/heritagedata/schemes/571/concepts/151444">
    <skos:narrower rdf:resource="http://purl.org/heritagedata/schemes/571/concepts/151122"/>
    <skos:narrower rdf:resource="http://purl.org/heritagedata/schemes/571/concepts/151123"/>
    <skos:narrower>
      <skos:Concept rdf:about="http://purl.org/heritagedata/schemes/571/concepts/151124">
        <skos:broader rdf:resource="http://purl.org/heritagedata/schemes/571/concepts/151444"/>
        <skos:inScheme rdf:resource="http://purl.org/heritagedata/schemes/571"/>
        <dc:identifier>http://purl.org/heritagedata/schemes/571/concepts/151124</dc:identifier>
        <dc:issued rdf:datatype="http://www.w3.org/2001/XMLSchema#dateTime">2024-07-01T17:17:33</dc:issued>
        <cc:license rdf:resource="https://www.nationalarchives.gov.uk/doc/open-government-licence/version/3/"/>
        <cc:attributionURL rdf:resource="https://historicengland.org.uk/"/>
        <cc:attributionName xml:lang="en">Historic England</cc:attributionName>
        <dc:publisher rdf:resource="https://historicengland.org.uk/"/>
        <dc:spatial rdf:resource="http://vocab.getty.edu/tgn/7002445"/>
        <dc:spatial rdf:resource="http://dbpedia.org/resource/England"/>
        <skos:prefLabel xml:lang="en">Pond</skos:prefLabel>
        <skos:scopeNote xml:lang="en">An inland body of fresh water. Ponds generally refer to smaller examples, lakes to larger, but there is no clear break along the gradation between the two. Ponds are often artificial and made for a specific purpose.</skos:scopeNote>
      </skos:Concept>
    </skos:narrower>

    <skos:narrower>
      <skos:Concept rdf:about="http://purl.org/heritagedata/schemes/571/concepts/151125">
        <skos:broader rdf:resource="http://purl.org/heritagedata/schemes/571/concepts/151444"/>
        <skos:inScheme rdf:resource="http://purl.org/heritagedata/schemes/571"/>
        <dc:identifier>http://purl.org/heritagedata/schemes/571/concepts/151125</dc:identifier>
        <dc:issued rdf:datatype="http://www.w3.org/2001/XMLSchema#dateTime">2024-07-01T17:17:33</dc:issued>
        <cc:license rdf:resource="https://www.nationalarchives.gov.uk/doc/open-government-licence/version/3/"/>
        <cc:attributionURL rdf:resource="https://historicengland.org.uk/"/>
        <cc:attributionName xml:lang="en">Historic England</cc:attributionName>
        <dc:publisher rdf:resource="https://historicengland.org.uk/"/>
        <dc:spatial rdf:resource="http://vocab.getty.edu/tgn/7002445"/>
        <dc:spatial rdf:resource="http://dbpedia.org/resource/England"/>
        <skos:prefLabel xml:lang="en">Mere</skos:prefLabel>
        <skos:scopeNote xml:lang="en">A shallow lake that is broad in relation to its depth</skos:scopeNote>
      </skos:Concept>
    </skos:narrower>

    <skos:narrower rdf:resource="http://purl.org/heritagedata/schemes/571/concepts/152594"/>
    <skos:broader rdf:resource="http://purl.org/heritagedata/schemes/571/concepts/151456"/>
    <skos:inScheme rdf:resource="http://purl.org/heritagedata/schemes/571"/>
    <dc:identifier>http://purl.org/heritagedata/schemes/571/concepts/151444</dc:identifier>
    <dc:issued rdf:datatype="http://www.w3.org/2001/XMLSchema#dateTime">2024-07-01T17:17:33</dc:issued>
    <cc:license rdf:resource="https://www.nationalarchives.gov.uk/doc/open-government-licence/version/3/"/>
    <cc:attributionURL rdf:resource="https://historicengland.org.uk/"/>
    <cc:attributionName xml:lang="en">Historic England</cc:attributionName>
    <dc:publisher rdf:resource="https://historicengland.org.uk/"/>
    <dc:spatial rdf:resource="http://vocab.getty.edu/tgn/7002445"/>
    <dc:spatial rdf:resource="http://dbpedia.org/resource/England"/>
    <skos:prefLabel xml:lang="en">Freshwater Body</skos:prefLabel>
    <skos:scopeNote xml:lang="en">An area of freshwater found inland.</skos:scopeNote>
  </skos:Concept>

  <skos:Concept rdf:about="http://purl.org/heritagedata/schemes/571/concepts/151123">
    <skos:broader rdf:resource="http://purl.org/heritagedata/schemes/571/concepts/151444"/>
    <skos:broader rdf:resource="http://purl.org/heritagedata/schemes/571/concepts/151443"/>
    <skos:inScheme rdf:resource="http://purl.org/heritagedata/schemes/571"/>
    <dc:identifier>http://purl.org/heritagedata/schemes/571/concepts/151123</dc:identifier>
    <dc:issued rdf:datatype="http://www.w3.org/2001/XMLSchema#dateTime">2024-07-01T17:17:33</dc:issued>
    <cc:license rdf:resource="https://www.nationalarchives.gov.uk/doc/open-government-licence/version/3/"/>
    <cc:attributionURL rdf:resource="https://historicengland.org.uk/"/>
    <cc:attributionName xml:lang="en">Historic England</cc:attributionName>
    <dc:publisher rdf:resource="https://historicengland.org.uk/"/>
    <dc:spatial rdf:resource="http://vocab.getty.edu/tgn/7002445"/>
    <dc:spatial rdf:resource="http://dbpedia.org/resource/England"/>
    <skos:prefLabel xml:lang="en">Lagoon</skos:prefLabel>
    <skos:scopeNote xml:lang="en">A body of shallow salt, brackish or fresh water totally or partially enclosed from the sea by a sand bar, spit or reef running across the entrance.</skos:scopeNote>
  </skos:Concept>

  <skos:Concept rdf:about="http://purl.org/heritagedata/schemes/571/concepts/151443">
    <skos:narrower rdf:resource="http://purl.org/heritagedata/schemes/571/concepts/151123"/>
    <skos:narrower>
      <skos:Concept rdf:about="http://purl.org/heritagedata/schemes/571/concepts/151126">
        <skos:broader rdf:resource="http://purl.org/heritagedata/schemes/571/concepts/151443"/>
        <skos:inScheme rdf:resource="http://purl.org/heritagedata/schemes/571"/>
        <dc:identifier>http://purl.org/heritagedata/schemes/571/concepts/151126</dc:identifier>
        <dc:issued rdf:datatype="http://www.w3.org/2001/XMLSchema#dateTime">2024-07-01T17:17:33</dc:issued>
        <cc:license rdf:resource="https://www.nationalarchives.gov.uk/doc/open-government-licence/version/3/"/>
        <cc:attributionURL rdf:resource="https://historicengland.org.uk/"/>
        <cc:attributionName xml:lang="en">Historic England</cc:attributionName>
        <dc:publisher rdf:resource="https://historicengland.org.uk/"/>
        <dc:spatial rdf:resource="http://vocab.getty.edu/tgn/7002445"/>
        <dc:spatial rdf:resource="http://dbpedia.org/resource/England"/>
        <skos:prefLabel xml:lang="en">Creek</skos:prefLabel>
        <skos:scopeNote xml:lang="en">A small inlet on a sea coast or estuary, its sediments often exposed at low tide. Sometimes applied to a river tributary or stream.</skos:scopeNote>
      </skos:Concept>
    </skos:narrower>

    <skos:narrower rdf:resource="http://purl.org/heritagedata/schemes/571/concepts/151129"/>
    <skos:narrower rdf:resource="http://purl.org/heritagedata/schemes/571/concepts/151416"/>
    <skos:narrower rdf:resource="http://purl.org/heritagedata/schemes/571/concepts/151614"/>
    <skos:narrower>
      <skos:Concept rdf:about="http://purl.org/heritagedata/schemes/571/concepts/151617">
        <skos:broader rdf:resource="http://purl.org/heritagedata/schemes/571/concepts/151443"/>
        <skos:inScheme rdf:resource="http://purl.org/heritagedata/schemes/571"/>
        <dc:identifier>http://purl.org/heritagedata/schemes/571/concepts/151617</dc:identifier>
        <dc:issued rdf:datatype="http://www.w3.org/2001/XMLSchema#dateTime">2024-07-01T17:17:33</dc:issued>
        <cc:license rdf:resource="https://www.nationalarchives.gov.uk/doc/open-government-licence/version/3/"/>
        <cc:attributionURL rdf:resource="https://historicengland.org.uk/"/>
        <cc:attributionName xml:lang="en">Historic England</cc:attributionName>
        <dc:publisher rdf:resource="https://historicengland.org.uk/"/>
        <dc:spatial rdf:resource="http://vocab.getty.edu/tgn/7002445"/>
        <dc:spatial rdf:resource="http://dbpedia.org/resource/England"/>
        <skos:prefLabel xml:lang="en">Spit</skos:prefLabel>
        <skos:scopeNote xml:lang="en">A deposition landform that develops by the process of longshore drift forming a narrow strip of land that juts out into the sea.</skos:scopeNote>
      </skos:Concept>
    </skos:narrower>

    <skos:narrower rdf:resource="http://purl.org/heritagedata/schemes/571/concepts/152317"/>
    <skos:narrower rdf:resource="http://purl.org/heritagedata/schemes/571/concepts/152534"/>
    <skos:broader rdf:resource="http://purl.org/heritagedata/schemes/571/concepts/151456"/>
    <skos:inScheme rdf:resource="http://purl.org/heritagedata/schemes/571"/>
    <dc:identifier>http://purl.org/heritagedata/schemes/571/concepts/151443</dc:identifier>
    <dc:issued rdf:datatype="http://www.w3.org/2001/XMLSchema#dateTime">2024-07-01T17:17:33</dc:issued>
    <cc:license rdf:resource="https://www.nationalarchives.gov.uk/doc/open-government-licence/version/3/"/>
    <cc:attributionURL rdf:resource="https://historicengland.org.uk/"/>
    <cc:attributionName xml:lang="en">Historic England</cc:attributionName>
    <dc:publisher rdf:resource="https://historicengland.org.uk/"/>
    <dc:spatial rdf:resource="http://vocab.getty.edu/tgn/7002445"/>
    <dc:spatial rdf:resource="http://dbpedia.org/resource/England"/>
    <skos:prefLabel xml:lang="en">Coastal And Intertidal</skos:prefLabel>
    <skos:scopeNote xml:lang="en">The topography at the interface of sea and land, subject to the constant changes in form and perception associated with the tides, the erosive forces of sea and issuing rivers.</skos:scopeNote>
  </skos:Concept>

  <skos:Concept rdf:about="http://purl.org/heritagedata/schemes/571/concepts/151128">
    <skos:broader rdf:resource="http://purl.org/heritagedata/schemes/571/concepts/152591"/>
    <skos:inScheme rdf:resource="http://purl.org/heritagedata/schemes/571"/>
    <dc:identifier>http://purl.org/heritagedata/schemes/571/concepts/151128</dc:identifier>
    <dc:issued rdf:datatype="http://www.w3.org/2001/XMLSchema#dateTime">2024-07-01T17:17:33</dc:issued>
    <cc:license rdf:resource="https://www.nationalarchives.gov.uk/doc/open-government-licence/version/3/"/>
    <cc:attributionURL rdf:resource="https://historicengland.org.uk/"/>
    <cc:attributionName xml:lang="en">Historic England</cc:attributionName>
    <dc:publisher rdf:resource="https://historicengland.org.uk/"/>
    <dc:spatial rdf:resource="http://vocab.getty.edu/tgn/7002445"/>
    <dc:spatial rdf:resource="http://dbpedia.org/resource/England"/>
    <skos:prefLabel xml:lang="en">Submerged Forest</skos:prefLabel>
    <skos:scopeNote xml:lang="en">Tracts of submerged land retaining macrofossil evidence, often in situ, for former woodland and other woody vegetation cover.</skos:scopeNote>
  </skos:Concept>

  <skos:Concept rdf:about="http://purl.org/heritagedata/schemes/571/concepts/152591">
    <skos:narrower rdf:resource="http://purl.org/heritagedata/schemes/571/concepts/151128"/>
    <skos:narrower>
      <skos:Concept rdf:about="http://purl.org/heritagedata/schemes/571/concepts/152592">
        <skos:broader rdf:resource="http://purl.org/heritagedata/schemes/571/concepts/152591"/>
        <skos:inScheme rdf:resource="http://purl.org/heritagedata/schemes/571"/>
        <dc:identifier>http://purl.org/heritagedata/schemes/571/concepts/152592</dc:identifier>
        <dc:issued rdf:datatype="http://www.w3.org/2001/XMLSchema#dateTime">2024-07-01T17:17:33</dc:issued>
        <cc:license rdf:resource="https://www.nationalarchives.gov.uk/doc/open-government-licence/version/3/"/>
        <cc:attributionURL rdf:resource="https://historicengland.org.uk/"/>
        <cc:attributionName xml:lang="en">Historic England</cc:attributionName>
        <dc:publisher rdf:resource="https://historicengland.org.uk/"/>
        <dc:spatial rdf:resource="http://vocab.getty.edu/tgn/7002445"/>
        <dc:spatial rdf:resource="http://dbpedia.org/resource/England"/>
        <skos:prefLabel xml:lang="en">Palaeochannel</skos:prefLabel>
        <skos:scopeNote xml:lang="en">The course or channel of a river or stream preserved as a geological or geomorphological feature. Use for areas containing individual examples or an individual system. For areas of inter-fluvial ridges &amp; other features, use 'Palaeolandscape component'.</skos:scopeNote>
      </skos:Concept>
    </skos:narrower>

    <skos:narrower rdf:resource="http://purl.org/heritagedata/schemes/571/concepts/152593"/>
    <skos:broader rdf:resource="http://purl.org/heritagedata/schemes/571/concepts/151456"/>
    <skos:inScheme rdf:resource="http://purl.org/heritagedata/schemes/571"/>
    <dc:identifier>http://purl.org/heritagedata/schemes/571/concepts/152591</dc:identifier>
    <dc:issued rdf:datatype="http://www.w3.org/2001/XMLSchema#dateTime">2024-07-01T17:17:33</dc:issued>
    <cc:license rdf:resource="https://www.nationalarchives.gov.uk/doc/open-government-licence/version/3/"/>
    <cc:attributionURL rdf:resource="https://historicengland.org.uk/"/>
    <cc:attributionName xml:lang="en">Historic England</cc:attributionName>
    <dc:publisher rdf:resource="https://historicengland.org.uk/"/>
    <dc:spatial rdf:resource="http://vocab.getty.edu/tgn/7002445"/>
    <dc:spatial rdf:resource="http://dbpedia.org/resource/England"/>
    <skos:prefLabel xml:lang="en">Palaeolandscape Component</skos:prefLabel>
    <skos:scopeNote xml:lang="en">Relates to surviving areas of ancient topographic features of former exposed land with evidence or strong potential for associated palaeo-environmental deposits and/or old land surfaces.</skos:scopeNote>
  </skos:Concept>

  <skos:Concept rdf:about="http://purl.org/heritagedata/schemes/571/concepts/151129">
    <skos:broader rdf:resource="http://purl.org/heritagedata/schemes/571/concepts/151443"/>
    <skos:inScheme rdf:resource="http://purl.org/heritagedata/schemes/571"/>
    <dc:identifier>http://purl.org/heritagedata/schemes/571/concepts/151129</dc:identifier>
    <dc:issued rdf:datatype="http://www.w3.org/2001/XMLSchema#dateTime">2024-07-01T17:17:33</dc:issued>
    <cc:license rdf:resource="https://www.nationalarchives.gov.uk/doc/open-government-licence/version/3/"/>
    <cc:attributionURL rdf:resource="https://historicengland.org.uk/"/>
    <cc:attributionName xml:lang="en">Historic England</cc:attributionName>
    <dc:publisher rdf:resource="https://historicengland.org.uk/"/>
    <dc:spatial rdf:resource="http://vocab.getty.edu/tgn/7002445"/>
    <dc:spatial rdf:resource="http://dbpedia.org/resource/England"/>
    <skos:prefLabel xml:lang="en">Cliff</skos:prefLabel>
    <skos:related rdf:resource="http://purl.org/heritagedata/schemes/571/concepts/152322"/>
    <skos:scopeNote xml:lang="en">A tall, steep and largely exposed face of the local geological formation, usually of rock though in some areas cliffs may form from erosion of softer materials such as boulder clay.</skos:scopeNote>
  </skos:Concept>

  <skos:Concept rdf:about="http://purl.org/heritagedata/schemes/571/concepts/151131">
    <skos:broader rdf:resource="http://purl.org/heritagedata/schemes/571/concepts/152320"/>
    <skos:inScheme rdf:resource="http://purl.org/heritagedata/schemes/571"/>
    <dc:identifier>http://purl.org/heritagedata/schemes/571/concepts/151131</dc:identifier>
    <dc:issued rdf:datatype="http://www.w3.org/2001/XMLSchema#dateTime">2024-07-01T17:17:33</dc:issued>
    <cc:license rdf:resource="https://www.nationalarchives.gov.uk/doc/open-government-licence/version/3/"/>
    <cc:attributionURL rdf:resource="https://historicengland.org.uk/"/>
    <cc:attributionName xml:lang="en">Historic England</cc:attributionName>
    <dc:publisher rdf:resource="https://historicengland.org.uk/"/>
    <dc:spatial rdf:resource="http://vocab.getty.edu/tgn/7002445"/>
    <dc:spatial rdf:resource="http://dbpedia.org/resource/England"/>
    <skos:prefLabel xml:lang="en">Mountain</skos:prefLabel>
    <skos:related rdf:resource="http://purl.org/heritagedata/schemes/571/concepts/152322"/>
    <skos:scopeNote xml:lang="en">A large, steep elevation in the earth's surface with a relatively small surface area on its summit.</skos:scopeNote>
  </skos:Concept>

  <skos:Concept rdf:about="http://purl.org/heritagedata/schemes/571/concepts/152320">
    <skos:narrower rdf:resource="http://purl.org/heritagedata/schemes/571/concepts/151131"/>
    <skos:narrower rdf:resource="http://purl.org/heritagedata/schemes/571/concepts/151132"/>
    <skos:narrower rdf:resource="http://purl.org/heritagedata/schemes/571/concepts/151265"/>
    <skos:narrower>
      <skos:Concept rdf:about="http://purl.org/heritagedata/schemes/571/concepts/151414">
        <skos:broader rdf:resource="http://purl.org/heritagedata/schemes/571/concepts/152320"/>
        <skos:inScheme rdf:resource="http://purl.org/heritagedata/schemes/571"/>
        <dc:identifier>http://purl.org/heritagedata/schemes/571/concepts/151414</dc:identifier>
        <dc:issued rdf:datatype="http://www.w3.org/2001/XMLSchema#dateTime">2024-07-01T17:17:33</dc:issued>
        <cc:license rdf:resource="https://www.nationalarchives.gov.uk/doc/open-government-licence/version/3/"/>
        <cc:attributionURL rdf:resource="https://historicengland.org.uk/"/>
        <cc:attributionName xml:lang="en">Historic England</cc:attributionName>
        <dc:publisher rdf:resource="https://historicengland.org.uk/"/>
        <dc:spatial rdf:resource="http://vocab.getty.edu/tgn/7002445"/>
        <dc:spatial rdf:resource="http://dbpedia.org/resource/England"/>
        <skos:prefLabel xml:lang="en">Tor</skos:prefLabel>
        <skos:scopeNote xml:lang="en">A rock outcrop exposed and shaped by weathering, usually found at or near the summit of a hill.</skos:scopeNote>
      </skos:Concept>
    </skos:narrower>

    <skos:narrower rdf:resource="http://purl.org/heritagedata/schemes/571/concepts/152601"/>
    <skos:broader rdf:resource="http://purl.org/heritagedata/schemes/571/concepts/151456"/>
    <skos:inScheme rdf:resource="http://purl.org/heritagedata/schemes/571"/>
    <dc:identifier>http://purl.org/heritagedata/schemes/571/concepts/152320</dc:identifier>
    <dc:issued rdf:datatype="http://www.w3.org/2001/XMLSchema#dateTime">2024-07-01T17:17:33</dc:issued>
    <cc:license rdf:resource="https://www.nationalarchives.gov.uk/doc/open-government-licence/version/3/"/>
    <cc:attributionURL rdf:resource="https://historicengland.org.uk/"/>
    <cc:attributionName xml:lang="en">Historic England</cc:attributionName>
    <dc:publisher rdf:resource="https://historicengland.org.uk/"/>
    <dc:spatial rdf:resource="http://vocab.getty.edu/tgn/7002445"/>
    <dc:spatial rdf:resource="http://dbpedia.org/resource/England"/>
    <skos:prefLabel xml:lang="en">Upland</skos:prefLabel>
    <skos:scopeNote xml:lang="en">An area of elevated ground. As it is a relative term, the altitude of uplands can vary greatly.</skos:scopeNote>
  </skos:Concept>

  <skos:Concept rdf:about="http://purl.org/heritagedata/schemes/571/concepts/151132">
    <skos:broader rdf:resource="http://purl.org/heritagedata/schemes/571/concepts/152326"/>
    <skos:broader rdf:resource="http://purl.org/heritagedata/schemes/571/concepts/152320"/>
    <skos:broader rdf:resource="http://purl.org/heritagedata/schemes/571/concepts/151250"/>
    <skos:narrower>
      <skos:Concept rdf:about="http://purl.org/heritagedata/schemes/571/concepts/160153">
        <skos:broader rdf:resource="http://purl.org/heritagedata/schemes/571/concepts/151132"/>
        <skos:inScheme rdf:resource="http://purl.org/heritagedata/schemes/571"/>
        <dc:identifier>http://purl.org/heritagedata/schemes/571/concepts/160153</dc:identifier>
        <dc:issued rdf:datatype="http://www.w3.org/2001/XMLSchema#dateTime">2024-07-01T17:17:33</dc:issued>
        <cc:license rdf:resource="https://www.nationalarchives.gov.uk/doc/open-government-licence/version/3/"/>
        <cc:attributionURL rdf:resource="https://historicengland.org.uk/"/>
        <cc:attributionName xml:lang="en">Historic England</cc:attributionName>
        <dc:publisher rdf:resource="https://historicengland.org.uk/"/>
        <dc:spatial rdf:resource="http://vocab.getty.edu/tgn/7002445"/>
        <dc:spatial rdf:resource="http://dbpedia.org/resource/England"/>
        <skos:prefLabel xml:lang="en">Moorland (Divided)</skos:prefLabel>
        <skos:scopeNote xml:lang="en">Moorland divided by stock-proof boundaries.</skos:scopeNote>
      </skos:Concept>
    </skos:narrower>

    <skos:narrower>
      <skos:Concept rdf:about="http://purl.org/heritagedata/schemes/571/concepts/160154">
        <skos:broader rdf:resource="http://purl.org/heritagedata/schemes/571/concepts/151132"/>
        <skos:inScheme rdf:resource="http://purl.org/heritagedata/schemes/571"/>
        <dc:identifier>http://purl.org/heritagedata/schemes/571/concepts/160154</dc:identifier>
        <dc:issued rdf:datatype="http://www.w3.org/2001/XMLSchema#dateTime">2024-07-01T17:17:33</dc:issued>
        <cc:license rdf:resource="https://www.nationalarchives.gov.uk/doc/open-government-licence/version/3/"/>
        <cc:attributionURL rdf:resource="https://historicengland.org.uk/"/>
        <cc:attributionName xml:lang="en">Historic England</cc:attributionName>
        <dc:publisher rdf:resource="https://historicengland.org.uk/"/>
        <dc:spatial rdf:resource="http://vocab.getty.edu/tgn/7002445"/>
        <dc:spatial rdf:resource="http://dbpedia.org/resource/England"/>
        <skos:prefLabel xml:lang="en">Moorland (Undivided)</skos:prefLabel>
        <skos:scopeNote xml:lang="en">Moorland left open, not divided by stock-proof boundaries.</skos:scopeNote>
      </skos:Concept>
    </skos:narrower>

    <skos:inScheme rdf:resource="http://purl.org/heritagedata/schemes/571"/>
    <dc:identifier>http://purl.org/heritagedata/schemes/571/concepts/151132</dc:identifier>
    <dc:issued rdf:datatype="http://www.w3.org/2001/XMLSchema#dateTime">2024-07-01T17:17:33</dc:issued>
    <cc:license rdf:resource="https://www.nationalarchives.gov.uk/doc/open-government-licence/version/3/"/>
    <cc:attributionURL rdf:resource="https://historicengland.org.uk/"/>
    <cc:attributionName xml:lang="en">Historic England</cc:attributionName>
    <dc:publisher rdf:resource="https://historicengland.org.uk/"/>
    <dc:spatial rdf:resource="http://vocab.getty.edu/tgn/7002445"/>
    <dc:spatial rdf:resource="http://dbpedia.org/resource/England"/>
    <skos:prefLabel xml:lang="en">Moorland</skos:prefLabel>
    <skos:scopeNote xml:lang="en">Poorly drained land, can include uplands with extensive blanket bog or low-lying damp unimproved ground. Used for rough grazing, occasionally for hay-making, and where peat was cut as a source of turf for domestic fuel.</skos:scopeNote>
  </skos:Concept>

  <skos:Concept rdf:about="http://purl.org/heritagedata/schemes/571/concepts/152326">
    <skos:narrower rdf:resource="http://purl.org/heritagedata/schemes/571/concepts/151132"/>
    <skos:narrower rdf:resource="http://purl.org/heritagedata/schemes/571/concepts/151133"/>
    <skos:narrower rdf:resource="http://purl.org/heritagedata/schemes/571/concepts/151264"/>
    <skos:narrower rdf:resource="http://purl.org/heritagedata/schemes/571/concepts/151416"/>
    <skos:narrower rdf:resource="http://purl.org/heritagedata/schemes/571/concepts/151609"/>
    <skos:narrower rdf:resource="http://purl.org/heritagedata/schemes/571/concepts/152327"/>
    <skos:narrower rdf:resource="http://purl.org/heritagedata/schemes/571/concepts/152330"/>
    <skos:narrower rdf:resource="http://purl.org/heritagedata/schemes/571/concepts/152379"/>
    <skos:narrower rdf:resource="http://purl.org/heritagedata/schemes/571/concepts/152382"/>
    <skos:narrower rdf:resource="http://purl.org/heritagedata/schemes/571/concepts/160476"/>
    <skos:inScheme rdf:resource="http://purl.org/heritagedata/schemes/571"/>
    <dc:identifier>http://purl.org/heritagedata/schemes/571/concepts/152326</dc:identifier>
    <dc:issued rdf:datatype="http://www.w3.org/2001/XMLSchema#dateTime">2024-07-01T17:17:33</dc:issued>
    <cc:license rdf:resource="https://www.nationalarchives.gov.uk/doc/open-government-licence/version/3/"/>
    <cc:attributionURL rdf:resource="https://historicengland.org.uk/"/>
    <cc:attributionName xml:lang="en">Historic England</cc:attributionName>
    <dc:publisher rdf:resource="https://historicengland.org.uk/"/>
    <dc:spatial rdf:resource="http://vocab.getty.edu/tgn/7002445"/>
    <dc:spatial rdf:resource="http://dbpedia.org/resource/England"/>
    <skos:prefLabel xml:lang="en">Unimproved Land</skos:prefLabel>
    <skos:scopeNote xml:lang="en">-</skos:scopeNote>
    <skos:topConceptOf rdf:resource="http://purl.org/heritagedata/schemes/571"/>
  </skos:Concept>

  <skos:Concept rdf:about="http://purl.org/heritagedata/schemes/571/concepts/151250">
    <skos:narrower rdf:resource="http://purl.org/heritagedata/schemes/571/concepts/151132"/>
    <skos:narrower rdf:resource="http://purl.org/heritagedata/schemes/571/concepts/151134"/>
    <skos:narrower rdf:resource="http://purl.org/heritagedata/schemes/571/concepts/151611"/>
    <skos:narrower rdf:resource="http://purl.org/heritagedata/schemes/571/concepts/152317"/>
    <skos:narrower rdf:resource="http://purl.org/heritagedata/schemes/571/concepts/152593"/>
    <skos:broader rdf:resource="http://purl.org/heritagedata/schemes/571/concepts/151456"/>
    <skos:inScheme rdf:resource="http://purl.org/heritagedata/schemes/571"/>
    <dc:identifier>http://purl.org/heritagedata/schemes/571/concepts/151250</dc:identifier>
    <dc:issued rdf:datatype="http://www.w3.org/2001/XMLSchema#dateTime">2024-07-01T17:17:33</dc:issued>
    <cc:license rdf:resource="https://www.nationalarchives.gov.uk/doc/open-government-licence/version/3/"/>
    <cc:attributionURL rdf:resource="https://historicengland.org.uk/"/>
    <cc:attributionName xml:lang="en">Historic England</cc:attributionName>
    <dc:publisher rdf:resource="https://historicengland.org.uk/"/>
    <dc:spatial rdf:resource="http://vocab.getty.edu/tgn/7002445"/>
    <dc:spatial rdf:resource="http://dbpedia.org/resource/England"/>
    <skos:prefLabel xml:lang="en">Wetland</skos:prefLabel>
    <skos:scopeNote xml:lang="en">An area whose soil is saturated with moisture either permanently or on an intermittent cycle eg. fens, marshes and peat bogs. The dominant vegetation of wetlands varies enormously and the vegetation cover may be broken by areas of open water.</skos:scopeNote>
  </skos:Concept>

  <skos:Concept rdf:about="http://purl.org/heritagedata/schemes/571/concepts/151133">
    <skos:broader rdf:resource="http://purl.org/heritagedata/schemes/571/concepts/152326"/>
    <skos:broader rdf:resource="http://purl.org/heritagedata/schemes/571/concepts/152317"/>
    <skos:narrower>
      <skos:Concept rdf:about="http://purl.org/heritagedata/schemes/571/concepts/151415">
        <skos:broader rdf:resource="http://purl.org/heritagedata/schemes/571/concepts/151133"/>
        <skos:inScheme rdf:resource="http://purl.org/heritagedata/schemes/571"/>
        <dc:identifier>http://purl.org/heritagedata/schemes/571/concepts/151415</dc:identifier>
        <dc:issued rdf:datatype="http://www.w3.org/2001/XMLSchema#dateTime">2024-07-01T17:17:33</dc:issued>
        <cc:license rdf:resource="https://www.nationalarchives.gov.uk/doc/open-government-licence/version/3/"/>
        <cc:attributionURL rdf:resource="https://historicengland.org.uk/"/>
        <cc:attributionName xml:lang="en">Historic England</cc:attributionName>
        <dc:publisher rdf:resource="https://historicengland.org.uk/"/>
        <dc:spatial rdf:resource="http://vocab.getty.edu/tgn/7002445"/>
        <dc:spatial rdf:resource="http://dbpedia.org/resource/England"/>
        <skos:prefLabel xml:lang="en">Saltmarsh</skos:prefLabel>
        <skos:scopeNote xml:lang="en">An area in the upper inter tidal zone that is sometimes overflowed by the sea and whose vegetation is dominated by salt tolerant herbaceous plants. Saltmarshes are often used for pasture or for collecting water for the production of salt.</skos:scopeNote>
      </skos:Concept>
    </skos:narrower>

    <skos:narrower>
      <skos:Concept rdf:about="http://purl.org/heritagedata/schemes/571/concepts/160481">
        <skos:broader rdf:resource="http://purl.org/heritagedata/schemes/571/concepts/151133"/>
        <skos:inScheme rdf:resource="http://purl.org/heritagedata/schemes/571"/>
        <dc:identifier>http://purl.org/heritagedata/schemes/571/concepts/160481</dc:identifier>
        <dc:issued rdf:datatype="http://www.w3.org/2001/XMLSchema#dateTime">2024-07-01T17:17:33</dc:issued>
        <cc:license rdf:resource="https://www.nationalarchives.gov.uk/doc/open-government-licence/version/3/"/>
        <cc:attributionURL rdf:resource="https://historicengland.org.uk/"/>
        <cc:attributionName xml:lang="en">Historic England</cc:attributionName>
        <dc:publisher rdf:resource="https://historicengland.org.uk/"/>
        <dc:spatial rdf:resource="http://vocab.getty.edu/tgn/7002445"/>
        <dc:spatial rdf:resource="http://dbpedia.org/resource/England"/>
        <skos:prefLabel xml:lang="en">Marsh (Divided)</skos:prefLabel>
        <skos:scopeNote xml:lang="en">Marshland divided by stock-proof boundaries.</skos:scopeNote>
      </skos:Concept>
    </skos:narrower>

    <skos:narrower>
      <skos:Concept rdf:about="http://purl.org/heritagedata/schemes/571/concepts/160482">
        <skos:broader rdf:resource="http://purl.org/heritagedata/schemes/571/concepts/151133"/>
        <skos:inScheme rdf:resource="http://purl.org/heritagedata/schemes/571"/>
        <dc:identifier>http://purl.org/heritagedata/schemes/571/concepts/160482</dc:identifier>
        <dc:issued rdf:datatype="http://www.w3.org/2001/XMLSchema#dateTime">2024-07-01T17:17:33</dc:issued>
        <cc:license rdf:resource="https://www.nationalarchives.gov.uk/doc/open-government-licence/version/3/"/>
        <cc:attributionURL rdf:resource="https://historicengland.org.uk/"/>
        <cc:attributionName xml:lang="en">Historic England</cc:attributionName>
        <dc:publisher rdf:resource="https://historicengland.org.uk/"/>
        <dc:spatial rdf:resource="http://vocab.getty.edu/tgn/7002445"/>
        <dc:spatial rdf:resource="http://dbpedia.org/resource/England"/>
        <skos:prefLabel xml:lang="en">Marsh (Undivided)</skos:prefLabel>
        <skos:scopeNote xml:lang="en">Marshland left open, not divided by stock-proof boundaries.</skos:scopeNote>
      </skos:Concept>
    </skos:narrower>

    <skos:inScheme rdf:resource="http://purl.org/heritagedata/schemes/571"/>
    <dc:identifier>http://purl.org/heritagedata/schemes/571/concepts/151133</dc:identifier>
    <dc:issued rdf:datatype="http://www.w3.org/2001/XMLSchema#dateTime">2024-07-01T17:17:33</dc:issued>
    <cc:license rdf:resource="https://www.nationalarchives.gov.uk/doc/open-government-licence/version/3/"/>
    <cc:attributionURL rdf:resource="https://historicengland.org.uk/"/>
    <cc:attributionName xml:lang="en">Historic England</cc:attributionName>
    <dc:publisher rdf:resource="https://historicengland.org.uk/"/>
    <dc:spatial rdf:resource="http://vocab.getty.edu/tgn/7002445"/>
    <dc:spatial rdf:resource="http://dbpedia.org/resource/England"/>
    <skos:prefLabel xml:lang="en">Marsh</skos:prefLabel>
    <skos:scopeNote xml:lang="en">Low-lying land often covered by water and usually with peaty vegetation. Used seasonally for grazing. Historically, peat was sometimes cut as domestic fuel and the area also used for trapping wildfowl.</skos:scopeNote>
  </skos:Concept>

  <skos:Concept rdf:about="http://purl.org/heritagedata/schemes/571/concepts/152317">
    <skos:narrower rdf:resource="http://purl.org/heritagedata/schemes/571/concepts/151133"/>
    <skos:narrower>
      <skos:Concept rdf:about="http://purl.org/heritagedata/schemes/571/concepts/151187">
        <skos:broader rdf:resource="http://purl.org/heritagedata/schemes/571/concepts/152317"/>
        <skos:inScheme rdf:resource="http://purl.org/heritagedata/schemes/571"/>
        <dc:identifier>http://purl.org/heritagedata/schemes/571/concepts/151187</dc:identifier>
        <dc:issued rdf:datatype="http://www.w3.org/2001/XMLSchema#dateTime">2024-07-01T17:17:33</dc:issued>
        <cc:license rdf:resource="https://www.nationalarchives.gov.uk/doc/open-government-licence/version/3/"/>
        <cc:attributionURL rdf:resource="https://historicengland.org.uk/"/>
        <cc:attributionName xml:lang="en">Historic England</cc:attributionName>
        <dc:publisher rdf:resource="https://historicengland.org.uk/"/>
        <dc:spatial rdf:resource="http://vocab.getty.edu/tgn/7002445"/>
        <dc:spatial rdf:resource="http://dbpedia.org/resource/England"/>
        <skos:prefLabel xml:lang="en">Mudflat</skos:prefLabel>
        <skos:scopeNote xml:lang="en">Areas of relatively mobile, thick deposits of clays, silts, organic detritus and some very fine sand content, submerged at high tide and exposed at low tide, and often expressed as areas of muddy banks in sheltered areas along estuary sides.</skos:scopeNote>
      </skos:Concept>
    </skos:narrower>

    <skos:narrower>
      <skos:Concept rdf:about="http://purl.org/heritagedata/schemes/571/concepts/151442">
        <skos:broader rdf:resource="http://purl.org/heritagedata/schemes/571/concepts/152317"/>
        <skos:inScheme rdf:resource="http://purl.org/heritagedata/schemes/571"/>
        <dc:identifier>http://purl.org/heritagedata/schemes/571/concepts/151442</dc:identifier>
        <dc:issued rdf:datatype="http://www.w3.org/2001/XMLSchema#dateTime">2024-07-01T17:17:33</dc:issued>
        <cc:license rdf:resource="https://www.nationalarchives.gov.uk/doc/open-government-licence/version/3/"/>
        <cc:attributionURL rdf:resource="https://historicengland.org.uk/"/>
        <cc:attributionName xml:lang="en">Historic England</cc:attributionName>
        <dc:publisher rdf:resource="https://historicengland.org.uk/"/>
        <dc:spatial rdf:resource="http://vocab.getty.edu/tgn/7002445"/>
        <dc:spatial rdf:resource="http://dbpedia.org/resource/England"/>
        <skos:prefLabel xml:lang="en">Sandflats</skos:prefLabel>
        <skos:scopeNote xml:lang="en">Areas of relatively mobile, thick sand deposits, submerged at high tide and exposed at low tide, and often expressed as areas of sandbanks detached from the shore by tidal channels.</skos:scopeNote>
      </skos:Concept>
    </skos:narrower>

    <skos:broader rdf:resource="http://purl.org/heritagedata/schemes/571/concepts/151443"/>
    <skos:broader rdf:resource="http://purl.org/heritagedata/schemes/571/concepts/151250"/>
    <skos:inScheme rdf:resource="http://purl.org/heritagedata/schemes/571"/>
    <dc:identifier>http://purl.org/heritagedata/schemes/571/concepts/152317</dc:identifier>
    <dc:issued rdf:datatype="http://www.w3.org/2001/XMLSchema#dateTime">2024-07-01T17:17:33</dc:issued>
    <cc:license rdf:resource="https://www.nationalarchives.gov.uk/doc/open-government-licence/version/3/"/>
    <cc:attributionURL rdf:resource="https://historicengland.org.uk/"/>
    <cc:attributionName xml:lang="en">Historic England</cc:attributionName>
    <dc:publisher rdf:resource="https://historicengland.org.uk/"/>
    <dc:spatial rdf:resource="http://vocab.getty.edu/tgn/7002445"/>
    <dc:spatial rdf:resource="http://dbpedia.org/resource/England"/>
    <skos:prefLabel xml:lang="en">Coastal Wetland</skos:prefLabel>
    <skos:scopeNote xml:lang="en">Coastally situated or inter-tidal areas of permanently saturated land such as saltmarsh whose vegetation and extents of open water may be dominated by its slope and elevation relative to the tidal cycle.</skos:scopeNote>
  </skos:Concept>

  <skos:Concept rdf:about="http://purl.org/heritagedata/schemes/571/concepts/151134">
    <skos:broader rdf:resource="http://purl.org/heritagedata/schemes/571/concepts/151273"/>
    <skos:broader rdf:resource="http://purl.org/heritagedata/schemes/571/concepts/151250"/>
    <skos:inScheme rdf:resource="http://purl.org/heritagedata/schemes/571"/>
    <dc:identifier>http://purl.org/heritagedata/schemes/571/concepts/151134</dc:identifier>
    <dc:issued rdf:datatype="http://www.w3.org/2001/XMLSchema#dateTime">2024-07-01T17:17:33</dc:issued>
    <cc:license rdf:resource="https://www.nationalarchives.gov.uk/doc/open-government-licence/version/3/"/>
    <cc:attributionURL rdf:resource="https://historicengland.org.uk/"/>
    <cc:attributionName xml:lang="en">Historic England</cc:attributionName>
    <dc:publisher rdf:resource="https://historicengland.org.uk/"/>
    <dc:spatial rdf:resource="http://vocab.getty.edu/tgn/7002445"/>
    <dc:spatial rdf:resource="http://dbpedia.org/resource/England"/>
    <skos:prefLabel xml:lang="en">Carr</skos:prefLabel>
    <skos:scopeNote xml:lang="en">An area of fenland that has become overgrown with trees or shrubs. Normally the result of natural succession, and thus regarded as a form of ancient woodland.</skos:scopeNote>
  </skos:Concept>

  <skos:Concept rdf:about="http://purl.org/heritagedata/schemes/571/concepts/151273">
    <skos:narrower rdf:resource="http://purl.org/heritagedata/schemes/571/concepts/151134"/>
    <skos:narrower rdf:resource="http://purl.org/heritagedata/schemes/571/concepts/151272"/>
    <skos:narrower>
      <skos:Concept rdf:about="http://purl.org/heritagedata/schemes/571/concepts/151584">
        <skos:broader rdf:resource="http://purl.org/heritagedata/schemes/571/concepts/151273"/>
        <skos:inScheme rdf:resource="http://purl.org/heritagedata/schemes/571"/>
        <dc:identifier>http://purl.org/heritagedata/schemes/571/concepts/151584</dc:identifier>
        <dc:issued rdf:datatype="http://www.w3.org/2001/XMLSchema#dateTime">2024-07-01T17:17:33</dc:issued>
        <cc:license rdf:resource="https://www.nationalarchives.gov.uk/doc/open-government-licence/version/3/"/>
        <cc:attributionURL rdf:resource="https://historicengland.org.uk/"/>
        <cc:attributionName xml:lang="en">Historic England</cc:attributionName>
        <dc:publisher rdf:resource="https://historicengland.org.uk/"/>
        <dc:spatial rdf:resource="http://vocab.getty.edu/tgn/7002445"/>
        <dc:spatial rdf:resource="http://dbpedia.org/resource/England"/>
        <skos:prefLabel xml:lang="en">Ancient Woodland (Broadleaved)</skos:prefLabel>
        <skos:scopeNote xml:lang="en">Ancient woodland that predominantly consists of broadleaved trees, often the progeny of ancient trees.</skos:scopeNote>
      </skos:Concept>
    </skos:narrower>

    <skos:narrower>
      <skos:Concept rdf:about="http://purl.org/heritagedata/schemes/571/concepts/151585">
        <skos:broader rdf:resource="http://purl.org/heritagedata/schemes/571/concepts/151273"/>
        <skos:inScheme rdf:resource="http://purl.org/heritagedata/schemes/571"/>
        <dc:identifier>http://purl.org/heritagedata/schemes/571/concepts/151585</dc:identifier>
        <dc:issued rdf:datatype="http://www.w3.org/2001/XMLSchema#dateTime">2024-07-01T17:17:33</dc:issued>
        <cc:license rdf:resource="https://www.nationalarchives.gov.uk/doc/open-government-licence/version/3/"/>
        <cc:attributionURL rdf:resource="https://historicengland.org.uk/"/>
        <cc:attributionName xml:lang="en">Historic England</cc:attributionName>
        <dc:publisher rdf:resource="https://historicengland.org.uk/"/>
        <dc:spatial rdf:resource="http://vocab.getty.edu/tgn/7002445"/>
        <dc:spatial rdf:resource="http://dbpedia.org/resource/England"/>
        <skos:prefLabel xml:lang="en">Ancient Woodland (Coniferous)</skos:prefLabel>
        <skos:scopeNote xml:lang="en">Ancient woodland that predominantly consists of coniferous trees, often the products of modern replanting.</skos:scopeNote>
      </skos:Concept>
    </skos:narrower>

    <skos:narrower>
      <skos:Concept rdf:about="http://purl.org/heritagedata/schemes/571/concepts/151586">
        <skos:broader rdf:resource="http://purl.org/heritagedata/schemes/571/concepts/151273"/>
        <skos:inScheme rdf:resource="http://purl.org/heritagedata/schemes/571"/>
        <dc:identifier>http://purl.org/heritagedata/schemes/571/concepts/151586</dc:identifier>
        <dc:issued rdf:datatype="http://www.w3.org/2001/XMLSchema#dateTime">2024-07-01T17:17:33</dc:issued>
        <cc:license rdf:resource="https://www.nationalarchives.gov.uk/doc/open-government-licence/version/3/"/>
        <cc:attributionURL rdf:resource="https://historicengland.org.uk/"/>
        <cc:attributionName xml:lang="en">Historic England</cc:attributionName>
        <dc:publisher rdf:resource="https://historicengland.org.uk/"/>
        <dc:spatial rdf:resource="http://vocab.getty.edu/tgn/7002445"/>
        <dc:spatial rdf:resource="http://dbpedia.org/resource/England"/>
        <skos:prefLabel xml:lang="en">Ancient Woodland (Mixed)</skos:prefLabel>
        <skos:scopeNote xml:lang="en">Ancient woodland that consists of broadleaved and coniferous trees, often the product of modern replanting.</skos:scopeNote>
      </skos:Concept>
    </skos:narrower>

    <skos:narrower>
      <skos:Concept rdf:about="http://purl.org/heritagedata/schemes/571/concepts/164071">
        <skos:broader rdf:resource="http://purl.org/heritagedata/schemes/571/concepts/151273"/>
        <skos:inScheme rdf:resource="http://purl.org/heritagedata/schemes/571"/>
        <dc:identifier>http://purl.org/heritagedata/schemes/571/concepts/164071</dc:identifier>
        <dc:issued rdf:datatype="http://www.w3.org/2001/XMLSchema#dateTime">2024-07-01T17:17:33</dc:issued>
        <cc:license rdf:resource="https://www.nationalarchives.gov.uk/doc/open-government-licence/version/3/"/>
        <cc:attributionURL rdf:resource="https://historicengland.org.uk/"/>
        <cc:attributionName xml:lang="en">Historic England</cc:attributionName>
        <dc:publisher rdf:resource="https://historicengland.org.uk/"/>
        <dc:spatial rdf:resource="http://vocab.getty.edu/tgn/7002445"/>
        <dc:spatial rdf:resource="http://dbpedia.org/resource/England"/>
        <skos:prefLabel xml:lang="en">Ancient Woodland (Replanted)</skos:prefLabel>
        <skos:scopeNote xml:lang="en">Ancient woodland where original natural tree coverage has been clear-felled (often during the 20th century world wars) and the area replanted with other trees, often coniferous.</skos:scopeNote>
      </skos:Concept>
    </skos:narrower>

    <skos:broader rdf:resource="http://purl.org/heritagedata/schemes/571/concepts/151448"/>
    <skos:inScheme rdf:resource="http://purl.org/heritagedata/schemes/571"/>
    <dc:identifier>http://purl.org/heritagedata/schemes/571/concepts/151273</dc:identifier>
    <dc:issued rdf:datatype="http://www.w3.org/2001/XMLSchema#dateTime">2024-07-01T17:17:33</dc:issued>
    <cc:license rdf:resource="https://www.nationalarchives.gov.uk/doc/open-government-licence/version/3/"/>
    <cc:attributionURL rdf:resource="https://historicengland.org.uk/"/>
    <cc:attributionName xml:lang="en">Historic England</cc:attributionName>
    <dc:publisher rdf:resource="https://historicengland.org.uk/"/>
    <dc:spatial rdf:resource="http://vocab.getty.edu/tgn/7002445"/>
    <dc:spatial rdf:resource="http://dbpedia.org/resource/England"/>
    <skos:prefLabel xml:lang="en">Ancient Woodland</skos:prefLabel>
    <skos:scopeNote xml:lang="en">Woodland believed to have existed since at least 1600 in England and in England defined as such by Natural England. Usually managed for timber, coppice etc and often contains dividing banks, trackways, charcoal burning platforms etc.</skos:scopeNote>
  </skos:Concept>

  <skos:Concept rdf:about="http://purl.org/heritagedata/schemes/571/concepts/151136">
    <skos:broader rdf:resource="http://purl.org/heritagedata/schemes/571/concepts/151461"/>
    <skos:inScheme rdf:resource="http://purl.org/heritagedata/schemes/571"/>
    <dc:identifier>http://purl.org/heritagedata/schemes/571/concepts/151136</dc:identifier>
    <dc:issued rdf:datatype="http://www.w3.org/2001/XMLSchema#dateTime">2024-07-01T17:17:33</dc:issued>
    <cc:license rdf:resource="https://www.nationalarchives.gov.uk/doc/open-government-licence/version/3/"/>
    <cc:attributionURL rdf:resource="https://historicengland.org.uk/"/>
    <cc:attributionName xml:lang="en">Historic England</cc:attributionName>
    <dc:publisher rdf:resource="https://historicengland.org.uk/"/>
    <dc:spatial rdf:resource="http://vocab.getty.edu/tgn/7002445"/>
    <dc:spatial rdf:resource="http://dbpedia.org/resource/England"/>
    <skos:prefLabel xml:lang="en">Natural Gas Field</skos:prefLabel>
    <skos:related rdf:resource="http://purl.org/heritagedata/schemes/571/concepts/151738"/>
    <skos:scopeNote xml:lang="en">A site where natural gas produced by geological processes is extracted from deep beneath the earth's surface.</skos:scopeNote>
  </skos:Concept>

  <skos:Concept rdf:about="http://purl.org/heritagedata/schemes/571/concepts/151461">
    <skos:narrower rdf:resource="http://purl.org/heritagedata/schemes/571/concepts/151136"/>
    <skos:narrower rdf:resource="http://purl.org/heritagedata/schemes/571/concepts/151137"/>
    <skos:narrower rdf:resource="http://purl.org/heritagedata/schemes/571/concepts/151422"/>
    <skos:narrower rdf:resource="http://purl.org/heritagedata/schemes/571/concepts/151436"/>
    <skos:narrower rdf:resource="http://purl.org/heritagedata/schemes/571/concepts/151462"/>
    <skos:narrower rdf:resource="http://purl.org/heritagedata/schemes/571/concepts/151569"/>
    <skos:narrower rdf:resource="http://purl.org/heritagedata/schemes/571/concepts/151735"/>
    <skos:narrower rdf:resource="http://purl.org/heritagedata/schemes/571/concepts/151737"/>
    <skos:narrower rdf:resource="http://purl.org/heritagedata/schemes/571/concepts/151738"/>
    <skos:narrower rdf:resource="http://purl.org/heritagedata/schemes/571/concepts/151743"/>
    <skos:narrower rdf:resource="http://purl.org/heritagedata/schemes/571/concepts/151744"/>
    <skos:narrower rdf:resource="http://purl.org/heritagedata/schemes/571/concepts/152521"/>
    <skos:narrower rdf:resource="http://purl.org/heritagedata/schemes/571/concepts/160169"/>
    <skos:broader rdf:resource="http://purl.org/heritagedata/schemes/571/concepts/151457"/>
    <skos:inScheme rdf:resource="http://purl.org/heritagedata/schemes/571"/>
    <dc:identifier>http://purl.org/heritagedata/schemes/571/concepts/151461</dc:identifier>
    <dc:issued rdf:datatype="http://www.w3.org/2001/XMLSchema#dateTime">2024-07-01T17:17:33</dc:issued>
    <cc:license rdf:resource="https://www.nationalarchives.gov.uk/doc/open-government-licence/version/3/"/>
    <cc:attributionURL rdf:resource="https://historicengland.org.uk/"/>
    <cc:attributionName xml:lang="en">Historic England</cc:attributionName>
    <dc:publisher rdf:resource="https://historicengland.org.uk/"/>
    <dc:spatial rdf:resource="http://vocab.getty.edu/tgn/7002445"/>
    <dc:spatial rdf:resource="http://dbpedia.org/resource/England"/>
    <skos:prefLabel xml:lang="en">Extractive Industry</skos:prefLabel>
    <skos:scopeNote xml:lang="en">-</skos:scopeNote>
  </skos:Concept>

  <skos:Concept rdf:about="http://purl.org/heritagedata/schemes/571/concepts/151137">
    <skos:broader rdf:resource="http://purl.org/heritagedata/schemes/571/concepts/151461"/>
    <skos:inScheme rdf:resource="http://purl.org/heritagedata/schemes/571"/>
    <dc:identifier>http://purl.org/heritagedata/schemes/571/concepts/151137</dc:identifier>
    <dc:issued rdf:datatype="http://www.w3.org/2001/XMLSchema#dateTime">2024-07-01T17:17:33</dc:issued>
    <cc:license rdf:resource="https://www.nationalarchives.gov.uk/doc/open-government-licence/version/3/"/>
    <cc:attributionURL rdf:resource="https://historicengland.org.uk/"/>
    <cc:attributionName xml:lang="en">Historic England</cc:attributionName>
    <dc:publisher rdf:resource="https://historicengland.org.uk/"/>
    <dc:spatial rdf:resource="http://vocab.getty.edu/tgn/7002445"/>
    <dc:spatial rdf:resource="http://dbpedia.org/resource/England"/>
    <skos:prefLabel xml:lang="en">Oil Field</skos:prefLabel>
    <skos:related rdf:resource="http://purl.org/heritagedata/schemes/571/concepts/151737"/>
    <skos:scopeNote xml:lang="en">An area from which oil produced by geological processes is extracted from deep beneath the earth's surface.</skos:scopeNote>
  </skos:Concept>

  <skos:Concept rdf:about="http://purl.org/heritagedata/schemes/571/concepts/151138">
    <skos:broader rdf:resource="http://purl.org/heritagedata/schemes/571/concepts/151734"/>
    <skos:inScheme rdf:resource="http://purl.org/heritagedata/schemes/571"/>
    <dc:identifier>http://purl.org/heritagedata/schemes/571/concepts/151138</dc:identifier>
    <dc:issued rdf:datatype="http://www.w3.org/2001/XMLSchema#dateTime">2024-07-01T17:17:33</dc:issued>
    <cc:license rdf:resource="https://www.nationalarchives.gov.uk/doc/open-government-licence/version/3/"/>
    <cc:attributionURL rdf:resource="https://historicengland.org.uk/"/>
    <cc:attributionName xml:lang="en">Historic England</cc:attributionName>
    <dc:publisher rdf:resource="https://historicengland.org.uk/"/>
    <dc:spatial rdf:resource="http://vocab.getty.edu/tgn/7002445"/>
    <dc:spatial rdf:resource="http://dbpedia.org/resource/England"/>
    <skos:prefLabel xml:lang="en">Salt Works</skos:prefLabel>
    <skos:scopeNote xml:lang="en">A site, building or factory used for the production of salt.</skos:scopeNote>
  </skos:Concept>

  <skos:Concept rdf:about="http://purl.org/heritagedata/schemes/571/concepts/151734">
    <skos:narrower rdf:resource="http://purl.org/heritagedata/schemes/571/concepts/151138"/>
    <skos:broader rdf:resource="http://purl.org/heritagedata/schemes/571/concepts/152624"/>
    <skos:inScheme rdf:resource="http://purl.org/heritagedata/schemes/571"/>
    <dc:identifier>http://purl.org/heritagedata/schemes/571/concepts/151734</dc:identifier>
    <dc:issued rdf:datatype="http://www.w3.org/2001/XMLSchema#dateTime">2024-07-01T17:17:33</dc:issued>
    <cc:license rdf:resource="https://www.nationalarchives.gov.uk/doc/open-government-licence/version/3/"/>
    <cc:attributionURL rdf:resource="https://historicengland.org.uk/"/>
    <cc:attributionName xml:lang="en">Historic England</cc:attributionName>
    <dc:publisher rdf:resource="https://historicengland.org.uk/"/>
    <dc:spatial rdf:resource="http://vocab.getty.edu/tgn/7002445"/>
    <dc:spatial rdf:resource="http://dbpedia.org/resource/England"/>
    <skos:prefLabel xml:lang="en">Salt Production</skos:prefLabel>
    <skos:scopeNote xml:lang="en">Sites, buildings or structures associated with the entire process of salt production by various means.</skos:scopeNote>
  </skos:Concept>

  <skos:Concept rdf:about="http://purl.org/heritagedata/schemes/571/concepts/151139">
    <skos:broader rdf:resource="http://purl.org/heritagedata/schemes/571/concepts/151642"/>
    <skos:inScheme rdf:resource="http://purl.org/heritagedata/schemes/571"/>
    <dc:identifier>http://purl.org/heritagedata/schemes/571/concepts/151139</dc:identifier>
    <dc:issued rdf:datatype="http://www.w3.org/2001/XMLSchema#dateTime">2024-07-01T17:17:33</dc:issued>
    <cc:license rdf:resource="https://www.nationalarchives.gov.uk/doc/open-government-licence/version/3/"/>
    <cc:attributionURL rdf:resource="https://historicengland.org.uk/"/>
    <cc:attributionName xml:lang="en">Historic England</cc:attributionName>
    <dc:publisher rdf:resource="https://historicengland.org.uk/"/>
    <dc:spatial rdf:resource="http://vocab.getty.edu/tgn/7002445"/>
    <dc:spatial rdf:resource="http://dbpedia.org/resource/England"/>
    <skos:prefLabel xml:lang="en">Naval Dockyard</skos:prefLabel>
    <skos:scopeNote xml:lang="en">A naval base that builds, repairs, docks or converts warships and is manned by civilian engineers and workers and administered by engineer duty officers.</skos:scopeNote>
  </skos:Concept>

  <skos:Concept rdf:about="http://purl.org/heritagedata/schemes/571/concepts/151642">
    <skos:narrower rdf:resource="http://purl.org/heritagedata/schemes/571/concepts/151139"/>
    <skos:narrower>
      <skos:Concept rdf:about="http://purl.org/heritagedata/schemes/571/concepts/151228">
        <skos:broader rdf:resource="http://purl.org/heritagedata/schemes/571/concepts/151642"/>
        <skos:inScheme rdf:resource="http://purl.org/heritagedata/schemes/571"/>
        <dc:identifier>http://purl.org/heritagedata/schemes/571/concepts/151228</dc:identifier>
        <dc:issued rdf:datatype="http://www.w3.org/2001/XMLSchema#dateTime">2024-07-01T17:17:33</dc:issued>
        <cc:license rdf:resource="https://www.nationalarchives.gov.uk/doc/open-government-licence/version/3/"/>
        <cc:attributionURL rdf:resource="https://historicengland.org.uk/"/>
        <cc:attributionName xml:lang="en">Historic England</cc:attributionName>
        <dc:publisher rdf:resource="https://historicengland.org.uk/"/>
        <dc:spatial rdf:resource="http://vocab.getty.edu/tgn/7002445"/>
        <dc:spatial rdf:resource="http://dbpedia.org/resource/England"/>
        <skos:prefLabel xml:lang="en">Submarine Base</skos:prefLabel>
        <skos:scopeNote xml:lang="en">Coastal base for the docking, launch and maintenance of submarines.</skos:scopeNote>
      </skos:Concept>
    </skos:narrower>

    <skos:narrower rdf:resource="http://purl.org/heritagedata/schemes/571/concepts/151233"/>
    <skos:broader rdf:resource="http://purl.org/heritagedata/schemes/571/concepts/151447"/>
    <skos:inScheme rdf:resource="http://purl.org/heritagedata/schemes/571"/>
    <dc:identifier>http://purl.org/heritagedata/schemes/571/concepts/151642</dc:identifier>
    <dc:issued rdf:datatype="http://www.w3.org/2001/XMLSchema#dateTime">2024-07-01T17:17:33</dc:issued>
    <cc:license rdf:resource="https://www.nationalarchives.gov.uk/doc/open-government-licence/version/3/"/>
    <cc:attributionURL rdf:resource="https://historicengland.org.uk/"/>
    <cc:attributionName xml:lang="en">Historic England</cc:attributionName>
    <dc:publisher rdf:resource="https://historicengland.org.uk/"/>
    <dc:spatial rdf:resource="http://vocab.getty.edu/tgn/7002445"/>
    <dc:spatial rdf:resource="http://dbpedia.org/resource/England"/>
    <skos:prefLabel xml:lang="en">Military Transport</skos:prefLabel>
    <skos:scopeNote xml:lang="en">Complexes for transport, storage and deployment of military vehicles, vessels, aircraft etc and their associated armaments. Can also, as in the case of airfields, cover complexes actively employed in defence and aggression.</skos:scopeNote>
  </skos:Concept>

  <skos:Concept rdf:about="http://purl.org/heritagedata/schemes/571/concepts/151140">
    <skos:broader rdf:resource="http://purl.org/heritagedata/schemes/571/concepts/151451"/>
    <skos:inScheme rdf:resource="http://purl.org/heritagedata/schemes/571"/>
    <dc:identifier>http://purl.org/heritagedata/schemes/571/concepts/151140</dc:identifier>
    <dc:issued rdf:datatype="http://www.w3.org/2001/XMLSchema#dateTime">2024-07-01T17:17:33</dc:issued>
    <cc:license rdf:resource="https://www.nationalarchives.gov.uk/doc/open-government-licence/version/3/"/>
    <cc:attributionURL rdf:resource="https://historicengland.org.uk/"/>
    <cc:attributionName xml:lang="en">Historic England</cc:attributionName>
    <dc:publisher rdf:resource="https://historicengland.org.uk/"/>
    <dc:spatial rdf:resource="http://vocab.getty.edu/tgn/7002445"/>
    <dc:spatial rdf:resource="http://dbpedia.org/resource/England"/>
    <skos:prefLabel xml:lang="en">Orchard</skos:prefLabel>
    <skos:scopeNote xml:lang="en">An enclosed area of land or garden for the growing of fruit-bearing trees.</skos:scopeNote>
  </skos:Concept>

  <skos:Concept rdf:about="http://purl.org/heritagedata/schemes/571/concepts/151451">
    <skos:narrower rdf:resource="http://purl.org/heritagedata/schemes/571/concepts/151140"/>
    <skos:narrower>
      <skos:Concept rdf:about="http://purl.org/heritagedata/schemes/571/concepts/151141">
        <skos:broader rdf:resource="http://purl.org/heritagedata/schemes/571/concepts/151451"/>
        <skos:inScheme rdf:resource="http://purl.org/heritagedata/schemes/571"/>
        <dc:identifier>http://purl.org/heritagedata/schemes/571/concepts/151141</dc:identifier>
        <dc:issued rdf:datatype="http://www.w3.org/2001/XMLSchema#dateTime">2024-07-01T17:17:33</dc:issued>
        <cc:license rdf:resource="https://www.nationalarchives.gov.uk/doc/open-government-licence/version/3/"/>
        <cc:attributionURL rdf:resource="https://historicengland.org.uk/"/>
        <cc:attributionName xml:lang="en">Historic England</cc:attributionName>
        <dc:publisher rdf:resource="https://historicengland.org.uk/"/>
        <dc:spatial rdf:resource="http://vocab.getty.edu/tgn/7002445"/>
        <dc:spatial rdf:resource="http://dbpedia.org/resource/England"/>
        <skos:prefLabel xml:lang="en">Vineyard</skos:prefLabel>
        <skos:scopeNote xml:lang="en">An area of land and associated buildings where grapevines are cultivated.</skos:scopeNote>
      </skos:Concept>
    </skos:narrower>

    <skos:narrower rdf:resource="http://purl.org/heritagedata/schemes/571/concepts/151285"/>
    <skos:narrower rdf:resource="http://purl.org/heritagedata/schemes/571/concepts/151751"/>
    <skos:narrower>
      <skos:Concept rdf:about="http://purl.org/heritagedata/schemes/571/concepts/151753">
        <skos:broader rdf:resource="http://purl.org/heritagedata/schemes/571/concepts/151451"/>
        <skos:inScheme rdf:resource="http://purl.org/heritagedata/schemes/571"/>
        <dc:identifier>http://purl.org/heritagedata/schemes/571/concepts/151753</dc:identifier>
        <dc:issued rdf:datatype="http://www.w3.org/2001/XMLSchema#dateTime">2024-07-01T17:17:33</dc:issued>
        <cc:license rdf:resource="https://www.nationalarchives.gov.uk/doc/open-government-licence/version/3/"/>
        <cc:attributionURL rdf:resource="https://historicengland.org.uk/"/>
        <cc:attributionName xml:lang="en">Historic England</cc:attributionName>
        <dc:publisher rdf:resource="https://historicengland.org.uk/"/>
        <dc:spatial rdf:resource="http://vocab.getty.edu/tgn/7002445"/>
        <dc:spatial rdf:resource="http://dbpedia.org/resource/England"/>
        <skos:prefLabel xml:lang="en">Flower Farm</skos:prefLabel>
        <skos:scopeNote xml:lang="en">A farm concerned with the cultivation of flowering and ornamental plants for gardens and for floristry.</skos:scopeNote>
      </skos:Concept>
    </skos:narrower>

    <skos:inScheme rdf:resource="http://purl.org/heritagedata/schemes/571"/>
    <dc:identifier>http://purl.org/heritagedata/schemes/571/concepts/151451</dc:identifier>
    <dc:issued rdf:datatype="http://www.w3.org/2001/XMLSchema#dateTime">2024-07-01T17:17:33</dc:issued>
    <cc:license rdf:resource="https://www.nationalarchives.gov.uk/doc/open-government-licence/version/3/"/>
    <cc:attributionURL rdf:resource="https://historicengland.org.uk/"/>
    <cc:attributionName xml:lang="en">Historic England</cc:attributionName>
    <dc:publisher rdf:resource="https://historicengland.org.uk/"/>
    <dc:spatial rdf:resource="http://vocab.getty.edu/tgn/7002445"/>
    <dc:spatial rdf:resource="http://dbpedia.org/resource/England"/>
    <skos:prefLabel xml:lang="en">Orchards And Horticulture</skos:prefLabel>
    <skos:scopeNote xml:lang="en">-</skos:scopeNote>
    <skos:topConceptOf rdf:resource="http://purl.org/heritagedata/schemes/571"/>
  </skos:Concept>

  <skos:Concept rdf:about="http://purl.org/heritagedata/schemes/571/concepts/151142">
    <skos:broader rdf:resource="http://purl.org/heritagedata/schemes/571/concepts/160197"/>
    <skos:narrower>
      <skos:Concept rdf:about="http://purl.org/heritagedata/schemes/571/concepts/151143">
        <skos:broader rdf:resource="http://purl.org/heritagedata/schemes/571/concepts/151142"/>
        <skos:inScheme rdf:resource="http://purl.org/heritagedata/schemes/571"/>
        <dc:identifier>http://purl.org/heritagedata/schemes/571/concepts/151143</dc:identifier>
        <dc:issued rdf:datatype="http://www.w3.org/2001/XMLSchema#dateTime">2024-07-01T17:17:33</dc:issued>
        <cc:license rdf:resource="https://www.nationalarchives.gov.uk/doc/open-government-licence/version/3/"/>
        <cc:attributionURL rdf:resource="https://historicengland.org.uk/"/>
        <cc:attributionName xml:lang="en">Historic England</cc:attributionName>
        <dc:publisher rdf:resource="https://historicengland.org.uk/"/>
        <dc:spatial rdf:resource="http://vocab.getty.edu/tgn/7002445"/>
        <dc:spatial rdf:resource="http://dbpedia.org/resource/England"/>
        <skos:prefLabel xml:lang="en">Formal Garden</skos:prefLabel>
        <skos:scopeNote xml:lang="en">A garden of regular, linear or geometrical design, often associated with the traditional Italian, French and Dutch styles. Usually either adjacent to the house or within the pleasure grounds.</skos:scopeNote>
      </skos:Concept>
    </skos:narrower>

    <skos:inScheme rdf:resource="http://purl.org/heritagedata/schemes/571"/>
    <dc:identifier>http://purl.org/heritagedata/schemes/571/concepts/151142</dc:identifier>
    <dc:issued rdf:datatype="http://www.w3.org/2001/XMLSchema#dateTime">2024-07-01T17:17:33</dc:issued>
    <cc:license rdf:resource="https://www.nationalarchives.gov.uk/doc/open-government-licence/version/3/"/>
    <cc:attributionURL rdf:resource="https://historicengland.org.uk/"/>
    <cc:attributionName xml:lang="en">Historic England</cc:attributionName>
    <dc:publisher rdf:resource="https://historicengland.org.uk/"/>
    <dc:spatial rdf:resource="http://vocab.getty.edu/tgn/7002445"/>
    <dc:spatial rdf:resource="http://dbpedia.org/resource/England"/>
    <skos:prefLabel xml:lang="en">Ornamental Garden</skos:prefLabel>
    <skos:scopeNote xml:lang="en">A garden that has been designed for the purpose of aesthetic pleasure, rather than the production of crops and usually an element of ornamentally designed landscapes.</skos:scopeNote>
  </skos:Concept>

  <skos:Concept rdf:about="http://purl.org/heritagedata/schemes/571/concepts/160197">
    <skos:narrower rdf:resource="http://purl.org/heritagedata/schemes/571/concepts/151142"/>
    <skos:narrower>
      <skos:Concept rdf:about="http://purl.org/heritagedata/schemes/571/concepts/151144">
        <skos:broader rdf:resource="http://purl.org/heritagedata/schemes/571/concepts/160197"/>
        <skos:inScheme rdf:resource="http://purl.org/heritagedata/schemes/571"/>
        <dc:identifier>http://purl.org/heritagedata/schemes/571/concepts/151144</dc:identifier>
        <dc:issued rdf:datatype="http://www.w3.org/2001/XMLSchema#dateTime">2024-07-01T17:17:33</dc:issued>
        <cc:license rdf:resource="https://www.nationalarchives.gov.uk/doc/open-government-licence/version/3/"/>
        <cc:attributionURL rdf:resource="https://historicengland.org.uk/"/>
        <cc:attributionName xml:lang="en">Historic England</cc:attributionName>
        <dc:publisher rdf:resource="https://historicengland.org.uk/"/>
        <dc:spatial rdf:resource="http://vocab.getty.edu/tgn/7002445"/>
        <dc:spatial rdf:resource="http://dbpedia.org/resource/England"/>
        <skos:prefLabel xml:lang="en">Arboretum</skos:prefLabel>
        <skos:scopeNote xml:lang="en">A botanical garden, as an element of a designed or ornamental landscape, designed specifically for the cultivation and display of, often rare, trees.</skos:scopeNote>
      </skos:Concept>
    </skos:narrower>

    <skos:narrower>
      <skos:Concept rdf:about="http://purl.org/heritagedata/schemes/571/concepts/151601">
        <skos:broader rdf:resource="http://purl.org/heritagedata/schemes/571/concepts/160197"/>
        <skos:inScheme rdf:resource="http://purl.org/heritagedata/schemes/571"/>
        <dc:identifier>http://purl.org/heritagedata/schemes/571/concepts/151601</dc:identifier>
        <dc:issued rdf:datatype="http://www.w3.org/2001/XMLSchema#dateTime">2024-07-01T17:17:33</dc:issued>
        <cc:license rdf:resource="https://www.nationalarchives.gov.uk/doc/open-government-licence/version/3/"/>
        <cc:attributionURL rdf:resource="https://historicengland.org.uk/"/>
        <cc:attributionName xml:lang="en">Historic England</cc:attributionName>
        <dc:publisher rdf:resource="https://historicengland.org.uk/"/>
        <dc:spatial rdf:resource="http://vocab.getty.edu/tgn/7002445"/>
        <dc:spatial rdf:resource="http://dbpedia.org/resource/England"/>
        <skos:prefLabel xml:lang="en">Wilderness</skos:prefLabel>
        <skos:scopeNote xml:lang="en">Part of a landscape garden or park planted to give an uncultivated appearance, often using exotic or unusual trees and shrubs. Usually provided with networks of pathways, often more formally arranged than the term might suggest.</skos:scopeNote>
      </skos:Concept>
    </skos:narrower>

    <skos:broader rdf:resource="http://purl.org/heritagedata/schemes/571/concepts/151452"/>
    <skos:inScheme rdf:resource="http://purl.org/heritagedata/schemes/571"/>
    <dc:identifier>http://purl.org/heritagedata/schemes/571/concepts/160197</dc:identifier>
    <dc:issued rdf:datatype="http://www.w3.org/2001/XMLSchema#dateTime">2024-07-01T17:17:33</dc:issued>
    <cc:license rdf:resource="https://www.nationalarchives.gov.uk/doc/open-government-licence/version/3/"/>
    <cc:attributionURL rdf:resource="https://historicengland.org.uk/"/>
    <cc:attributionName xml:lang="en">Historic England</cc:attributionName>
    <dc:publisher rdf:resource="https://historicengland.org.uk/"/>
    <dc:spatial rdf:resource="http://vocab.getty.edu/tgn/7002445"/>
    <dc:spatial rdf:resource="http://dbpedia.org/resource/England"/>
    <skos:prefLabel xml:lang="en">Pleasure Grounds</skos:prefLabel>
    <skos:scopeNote xml:lang="en">An area within an ornamentally designed landscape where owners and guests walked about for pleasure. Typically complex mixes of plantings, ornamental gardens and play areas (bowling, croquet, etc).</skos:scopeNote>
  </skos:Concept>

  <skos:Concept rdf:about="http://purl.org/heritagedata/schemes/571/concepts/151146">
    <skos:broader rdf:resource="http://purl.org/heritagedata/schemes/571/concepts/160213"/>
    <skos:inScheme rdf:resource="http://purl.org/heritagedata/schemes/571"/>
    <dc:identifier>http://purl.org/heritagedata/schemes/571/concepts/151146</dc:identifier>
    <dc:issued rdf:datatype="http://www.w3.org/2001/XMLSchema#dateTime">2024-07-01T17:17:33</dc:issued>
    <cc:license rdf:resource="https://www.nationalarchives.gov.uk/doc/open-government-licence/version/3/"/>
    <cc:attributionURL rdf:resource="https://historicengland.org.uk/"/>
    <cc:attributionName xml:lang="en">Historic England</cc:attributionName>
    <dc:publisher rdf:resource="https://historicengland.org.uk/"/>
    <dc:spatial rdf:resource="http://vocab.getty.edu/tgn/7002445"/>
    <dc:spatial rdf:resource="http://dbpedia.org/resource/England"/>
    <skos:prefLabel xml:lang="en">Promenade</skos:prefLabel>
    <skos:scopeNote xml:lang="en">A designed open space within or extending from a settlement area, usually linear and specifically intended for strolling and public walks with good coastal views; they commonly form part of the planned complex of facilities of a coastal resort.</skos:scopeNote>
  </skos:Concept>

  <skos:Concept rdf:about="http://purl.org/heritagedata/schemes/571/concepts/160213">
    <skos:narrower rdf:resource="http://purl.org/heritagedata/schemes/571/concepts/151146"/>
    <skos:narrower>
      <skos:Concept rdf:about="http://purl.org/heritagedata/schemes/571/concepts/151290">
        <skos:broader rdf:resource="http://purl.org/heritagedata/schemes/571/concepts/160213"/>
        <skos:inScheme rdf:resource="http://purl.org/heritagedata/schemes/571"/>
        <dc:identifier>http://purl.org/heritagedata/schemes/571/concepts/151290</dc:identifier>
        <dc:issued rdf:datatype="http://www.w3.org/2001/XMLSchema#dateTime">2024-07-01T17:17:33</dc:issued>
        <cc:license rdf:resource="https://www.nationalarchives.gov.uk/doc/open-government-licence/version/3/"/>
        <cc:attributionURL rdf:resource="https://historicengland.org.uk/"/>
        <cc:attributionName xml:lang="en">Historic England</cc:attributionName>
        <dc:publisher rdf:resource="https://historicengland.org.uk/"/>
        <dc:spatial rdf:resource="http://vocab.getty.edu/tgn/7002445"/>
        <dc:spatial rdf:resource="http://dbpedia.org/resource/England"/>
        <skos:prefLabel xml:lang="en">Beach Huts</skos:prefLabel>
        <skos:scopeNote xml:lang="en">An area, usually immediately adjacent to a beach with numerous small timber one-roomed dwellings or shelters where holiday makers could rest after a day spent sunbathing, swimming and playing on the beach.</skos:scopeNote>
      </skos:Concept>
    </skos:narrower>

    <skos:narrower>
      <skos:Concept rdf:about="http://purl.org/heritagedata/schemes/571/concepts/152611">
        <skos:broader rdf:resource="http://purl.org/heritagedata/schemes/571/concepts/160213"/>
        <skos:inScheme rdf:resource="http://purl.org/heritagedata/schemes/571"/>
        <dc:identifier>http://purl.org/heritagedata/schemes/571/concepts/152611</dc:identifier>
        <dc:issued rdf:datatype="http://www.w3.org/2001/XMLSchema#dateTime">2024-07-01T17:17:33</dc:issued>
        <cc:license rdf:resource="https://www.nationalarchives.gov.uk/doc/open-government-licence/version/3/"/>
        <cc:attributionURL rdf:resource="https://historicengland.org.uk/"/>
        <cc:attributionName xml:lang="en">Historic England</cc:attributionName>
        <dc:publisher rdf:resource="https://historicengland.org.uk/"/>
        <dc:spatial rdf:resource="http://vocab.getty.edu/tgn/7002445"/>
        <dc:spatial rdf:resource="http://dbpedia.org/resource/England"/>
        <skos:prefLabel xml:lang="en">Pleasure Pier</skos:prefLabel>
        <skos:scopeNote xml:lang="en">A raised platform, generally of iron and/or wood, supported on spaced pillars or props and projecting out into the sea and designed to provide primarily recreational access over the sea from the shore to an adjacent position near or below MLW.</skos:scopeNote>
      </skos:Concept>
    </skos:narrower>

    <skos:narrower>
      <skos:Concept rdf:about="http://purl.org/heritagedata/schemes/571/concepts/152612">
        <skos:broader rdf:resource="http://purl.org/heritagedata/schemes/571/concepts/160213"/>
        <skos:inScheme rdf:resource="http://purl.org/heritagedata/schemes/571"/>
        <dc:identifier>http://purl.org/heritagedata/schemes/571/concepts/152612</dc:identifier>
        <dc:issued rdf:datatype="http://www.w3.org/2001/XMLSchema#dateTime">2024-07-01T17:17:33</dc:issued>
        <cc:license rdf:resource="https://www.nationalarchives.gov.uk/doc/open-government-licence/version/3/"/>
        <cc:attributionURL rdf:resource="https://historicengland.org.uk/"/>
        <cc:attributionName xml:lang="en">Historic England</cc:attributionName>
        <dc:publisher rdf:resource="https://historicengland.org.uk/"/>
        <dc:spatial rdf:resource="http://vocab.getty.edu/tgn/7002445"/>
        <dc:spatial rdf:resource="http://dbpedia.org/resource/England"/>
        <skos:prefLabel xml:lang="en">Leisure Beach</skos:prefLabel>
        <skos:scopeNote xml:lang="en">Largely inter-tidal areas, predominantly of sand, used mostly for leisure and relaxation by coastal visitors. May be managed actively, eg by periodic scraping or beach replenishment, or passively, eg by groynes, to retain the sand cover.</skos:scopeNote>
      </skos:Concept>
    </skos:narrower>

    <skos:narrower>
      <skos:Concept rdf:about="http://purl.org/heritagedata/schemes/571/concepts/152614">
        <skos:broader rdf:resource="http://purl.org/heritagedata/schemes/571/concepts/160213"/>
        <skos:inScheme rdf:resource="http://purl.org/heritagedata/schemes/571"/>
        <dc:identifier>http://purl.org/heritagedata/schemes/571/concepts/152614</dc:identifier>
        <dc:issued rdf:datatype="http://www.w3.org/2001/XMLSchema#dateTime">2024-07-01T17:17:33</dc:issued>
        <cc:license rdf:resource="https://www.nationalarchives.gov.uk/doc/open-government-licence/version/3/"/>
        <cc:attributionURL rdf:resource="https://historicengland.org.uk/"/>
        <cc:attributionName xml:lang="en">Historic England</cc:attributionName>
        <dc:publisher rdf:resource="https://historicengland.org.uk/"/>
        <dc:spatial rdf:resource="http://vocab.getty.edu/tgn/7002445"/>
        <dc:spatial rdf:resource="http://dbpedia.org/resource/England"/>
        <skos:prefLabel xml:lang="en">Bathing/Swimming Area</skos:prefLabel>
        <skos:scopeNote xml:lang="en">An outdoor area, commonly on the coast, used by people predominantly for bathing and/or swimming.</skos:scopeNote>
      </skos:Concept>
    </skos:narrower>

    <skos:narrower>
      <skos:Concept rdf:about="http://purl.org/heritagedata/schemes/571/concepts/160212">
        <skos:broader rdf:resource="http://purl.org/heritagedata/schemes/571/concepts/160213"/>
        <skos:inScheme rdf:resource="http://purl.org/heritagedata/schemes/571"/>
        <dc:identifier>http://purl.org/heritagedata/schemes/571/concepts/160212</dc:identifier>
        <dc:issued rdf:datatype="http://www.w3.org/2001/XMLSchema#dateTime">2024-07-01T17:17:33</dc:issued>
        <cc:license rdf:resource="https://www.nationalarchives.gov.uk/doc/open-government-licence/version/3/"/>
        <cc:attributionURL rdf:resource="https://historicengland.org.uk/"/>
        <cc:attributionName xml:lang="en">Historic England</cc:attributionName>
        <dc:publisher rdf:resource="https://historicengland.org.uk/"/>
        <dc:spatial rdf:resource="http://vocab.getty.edu/tgn/7002445"/>
        <dc:spatial rdf:resource="http://dbpedia.org/resource/England"/>
        <skos:prefLabel xml:lang="en">Cliff Gardens</skos:prefLabel>
        <skos:scopeNote xml:lang="en">Ornamental gardens, usually open to the public, that take advantage of the peculiar topography and climate found on cliffs.</skos:scopeNote>
      </skos:Concept>
    </skos:narrower>

    <skos:broader rdf:resource="http://purl.org/heritagedata/schemes/571/concepts/160285"/>
    <skos:inScheme rdf:resource="http://purl.org/heritagedata/schemes/571"/>
    <dc:identifier>http://purl.org/heritagedata/schemes/571/concepts/160213</dc:identifier>
    <dc:issued rdf:datatype="http://www.w3.org/2001/XMLSchema#dateTime">2024-07-01T17:17:33</dc:issued>
    <cc:license rdf:resource="https://www.nationalarchives.gov.uk/doc/open-government-licence/version/3/"/>
    <cc:attributionURL rdf:resource="https://historicengland.org.uk/"/>
    <cc:attributionName xml:lang="en">Historic England</cc:attributionName>
    <dc:publisher rdf:resource="https://historicengland.org.uk/"/>
    <dc:spatial rdf:resource="http://vocab.getty.edu/tgn/7002445"/>
    <dc:spatial rdf:resource="http://dbpedia.org/resource/England"/>
    <skos:prefLabel xml:lang="en">Coastal Recreation</skos:prefLabel>
    <skos:scopeNote xml:lang="en">Taking pleasure from the particular qualities and facilities afforded by or established at the sea and coast.</skos:scopeNote>
  </skos:Concept>

  <skos:Concept rdf:about="http://purl.org/heritagedata/schemes/571/concepts/151147">
    <skos:broader rdf:resource="http://purl.org/heritagedata/schemes/571/concepts/160288"/>
    <skos:inScheme rdf:resource="http://purl.org/heritagedata/schemes/571"/>
    <dc:identifier>http://purl.org/heritagedata/schemes/571/concepts/151147</dc:identifier>
    <dc:issued rdf:datatype="http://www.w3.org/2001/XMLSchema#dateTime">2024-07-01T17:17:33</dc:issued>
    <cc:license rdf:resource="https://www.nationalarchives.gov.uk/doc/open-government-licence/version/3/"/>
    <cc:attributionURL rdf:resource="https://historicengland.org.uk/"/>
    <cc:attributionName xml:lang="en">Historic England</cc:attributionName>
    <dc:publisher rdf:resource="https://historicengland.org.uk/"/>
    <dc:spatial rdf:resource="http://vocab.getty.edu/tgn/7002445"/>
    <dc:spatial rdf:resource="http://dbpedia.org/resource/England"/>
    <skos:prefLabel xml:lang="en">Holiday Park</skos:prefLabel>
    <skos:scopeNote xml:lang="en">Areas dominated by commercial complex(es) encompassing lightly-built holidaymaker's accommodation and associated facilities, sometimes including entertainment areas.</skos:scopeNote>
  </skos:Concept>

  <skos:Concept rdf:about="http://purl.org/heritagedata/schemes/571/concepts/160288">
    <skos:narrower rdf:resource="http://purl.org/heritagedata/schemes/571/concepts/151147"/>
    <skos:narrower>
      <skos:Concept rdf:about="http://purl.org/heritagedata/schemes/571/concepts/151149">
        <skos:broader rdf:resource="http://purl.org/heritagedata/schemes/571/concepts/160288"/>
        <skos:inScheme rdf:resource="http://purl.org/heritagedata/schemes/571"/>
        <dc:identifier>http://purl.org/heritagedata/schemes/571/concepts/151149</dc:identifier>
        <dc:issued rdf:datatype="http://www.w3.org/2001/XMLSchema#dateTime">2024-07-01T17:17:33</dc:issued>
        <cc:license rdf:resource="https://www.nationalarchives.gov.uk/doc/open-government-licence/version/3/"/>
        <cc:attributionURL rdf:resource="https://historicengland.org.uk/"/>
        <cc:attributionName xml:lang="en">Historic England</cc:attributionName>
        <dc:publisher rdf:resource="https://historicengland.org.uk/"/>
        <dc:spatial rdf:resource="http://vocab.getty.edu/tgn/7002445"/>
        <dc:spatial rdf:resource="http://dbpedia.org/resource/England"/>
        <skos:prefLabel xml:lang="en">Caravan Site</skos:prefLabel>
        <skos:scopeNote xml:lang="en">An area providing space for those with caravans or similar recreational vehicles to park. Sometimes with associated facilities such as power points, toilet blocks etc.</skos:scopeNote>
      </skos:Concept>
    </skos:narrower>

    <skos:narrower>
      <skos:Concept rdf:about="http://purl.org/heritagedata/schemes/571/concepts/151150">
        <skos:broader rdf:resource="http://purl.org/heritagedata/schemes/571/concepts/160288"/>
        <skos:inScheme rdf:resource="http://purl.org/heritagedata/schemes/571"/>
        <dc:identifier>http://purl.org/heritagedata/schemes/571/concepts/151150</dc:identifier>
        <dc:issued rdf:datatype="http://www.w3.org/2001/XMLSchema#dateTime">2024-07-01T17:17:33</dc:issued>
        <cc:license rdf:resource="https://www.nationalarchives.gov.uk/doc/open-government-licence/version/3/"/>
        <cc:attributionURL rdf:resource="https://historicengland.org.uk/"/>
        <cc:attributionName xml:lang="en">Historic England</cc:attributionName>
        <dc:publisher rdf:resource="https://historicengland.org.uk/"/>
        <dc:spatial rdf:resource="http://vocab.getty.edu/tgn/7002445"/>
        <dc:spatial rdf:resource="http://dbpedia.org/resource/England"/>
        <skos:prefLabel xml:lang="en">Camp Site</skos:prefLabel>
        <skos:scopeNote xml:lang="en">An area dedicated to camping, providing space for individuals to park vehicles and pitch tents often with associated facilities such as toilets and shower blocks.</skos:scopeNote>
      </skos:Concept>
    </skos:narrower>

    <skos:narrower rdf:resource="http://purl.org/heritagedata/schemes/571/concepts/151610"/>
    <skos:broader rdf:resource="http://purl.org/heritagedata/schemes/571/concepts/151450"/>
    <skos:inScheme rdf:resource="http://purl.org/heritagedata/schemes/571"/>
    <dc:identifier>http://purl.org/heritagedata/schemes/571/concepts/160288</dc:identifier>
    <dc:issued rdf:datatype="http://www.w3.org/2001/XMLSchema#dateTime">2024-07-01T17:17:33</dc:issued>
    <cc:license rdf:resource="https://www.nationalarchives.gov.uk/doc/open-government-licence/version/3/"/>
    <cc:attributionURL rdf:resource="https://historicengland.org.uk/"/>
    <cc:attributionName xml:lang="en">Historic England</cc:attributionName>
    <dc:publisher rdf:resource="https://historicengland.org.uk/"/>
    <dc:spatial rdf:resource="http://vocab.getty.edu/tgn/7002445"/>
    <dc:spatial rdf:resource="http://dbpedia.org/resource/England"/>
    <skos:prefLabel xml:lang="en">Recreational Accommodation</skos:prefLabel>
    <skos:scopeNote xml:lang="en">Provision for occasional accommodation for those who have travelled from home for enjoyment, amusement or pleasure.</skos:scopeNote>
  </skos:Concept>

  <skos:Concept rdf:about="http://purl.org/heritagedata/schemes/571/concepts/151148">
    <skos:broader rdf:resource="http://purl.org/heritagedata/schemes/571/concepts/160292"/>
    <skos:inScheme rdf:resource="http://purl.org/heritagedata/schemes/571"/>
    <dc:identifier>http://purl.org/heritagedata/schemes/571/concepts/151148</dc:identifier>
    <dc:issued rdf:datatype="http://www.w3.org/2001/XMLSchema#dateTime">2024-07-01T17:17:33</dc:issued>
    <cc:license rdf:resource="https://www.nationalarchives.gov.uk/doc/open-government-licence/version/3/"/>
    <cc:attributionURL rdf:resource="https://historicengland.org.uk/"/>
    <cc:attributionName xml:lang="en">Historic England</cc:attributionName>
    <dc:publisher rdf:resource="https://historicengland.org.uk/"/>
    <dc:spatial rdf:resource="http://vocab.getty.edu/tgn/7002445"/>
    <dc:spatial rdf:resource="http://dbpedia.org/resource/England"/>
    <skos:prefLabel xml:lang="en">Zoo</skos:prefLabel>
    <skos:scopeNote xml:lang="en">An enclosed area where wild animals are bred, studied and exhibited to the public.</skos:scopeNote>
  </skos:Concept>

  <skos:Concept rdf:about="http://purl.org/heritagedata/schemes/571/concepts/160292">
    <skos:narrower rdf:resource="http://purl.org/heritagedata/schemes/571/concepts/151148"/>
    <skos:narrower>
      <skos:Concept rdf:about="http://purl.org/heritagedata/schemes/571/concepts/151789">
        <skos:broader rdf:resource="http://purl.org/heritagedata/schemes/571/concepts/160292"/>
        <skos:inScheme rdf:resource="http://purl.org/heritagedata/schemes/571"/>
        <dc:identifier>http://purl.org/heritagedata/schemes/571/concepts/151789</dc:identifier>
        <dc:issued rdf:datatype="http://www.w3.org/2001/XMLSchema#dateTime">2024-07-01T17:17:33</dc:issued>
        <cc:license rdf:resource="https://www.nationalarchives.gov.uk/doc/open-government-licence/version/3/"/>
        <cc:attributionURL rdf:resource="https://historicengland.org.uk/"/>
        <cc:attributionName xml:lang="en">Historic England</cc:attributionName>
        <dc:publisher rdf:resource="https://historicengland.org.uk/"/>
        <dc:spatial rdf:resource="http://vocab.getty.edu/tgn/7002445"/>
        <dc:spatial rdf:resource="http://dbpedia.org/resource/England"/>
        <skos:prefLabel xml:lang="en">Lido</skos:prefLabel>
        <skos:scopeNote xml:lang="en">A public recreational complex centred around an open-air swimming pool.</skos:scopeNote>
      </skos:Concept>
    </skos:narrower>

    <skos:narrower rdf:resource="http://purl.org/heritagedata/schemes/571/concepts/160264"/>
    <skos:narrower rdf:resource="http://purl.org/heritagedata/schemes/571/concepts/160274"/>
    <skos:broader rdf:resource="http://purl.org/heritagedata/schemes/571/concepts/160285"/>
    <skos:inScheme rdf:resource="http://purl.org/heritagedata/schemes/571"/>
    <dc:identifier>http://purl.org/heritagedata/schemes/571/concepts/160292</dc:identifier>
    <dc:issued rdf:datatype="http://www.w3.org/2001/XMLSchema#dateTime">2024-07-01T17:17:33</dc:issued>
    <cc:license rdf:resource="https://www.nationalarchives.gov.uk/doc/open-government-licence/version/3/"/>
    <cc:attributionURL rdf:resource="https://historicengland.org.uk/"/>
    <cc:attributionName xml:lang="en">Historic England</cc:attributionName>
    <dc:publisher rdf:resource="https://historicengland.org.uk/"/>
    <dc:spatial rdf:resource="http://vocab.getty.edu/tgn/7002445"/>
    <dc:spatial rdf:resource="http://dbpedia.org/resource/England"/>
    <skos:prefLabel xml:lang="en">Recreation Ground</skos:prefLabel>
    <skos:scopeNote xml:lang="en">Area of open ground with permanent or semi-permanent facilities established to enable people to enjoy, amuse or please themselves.</skos:scopeNote>
  </skos:Concept>

  <skos:Concept rdf:about="http://purl.org/heritagedata/schemes/571/concepts/151151">
    <skos:broader rdf:resource="http://purl.org/heritagedata/schemes/571/concepts/160382"/>
    <skos:inScheme rdf:resource="http://purl.org/heritagedata/schemes/571"/>
    <dc:identifier>http://purl.org/heritagedata/schemes/571/concepts/151151</dc:identifier>
    <dc:issued rdf:datatype="http://www.w3.org/2001/XMLSchema#dateTime">2024-07-01T17:17:33</dc:issued>
    <cc:license rdf:resource="https://www.nationalarchives.gov.uk/doc/open-government-licence/version/3/"/>
    <cc:attributionURL rdf:resource="https://historicengland.org.uk/"/>
    <cc:attributionName xml:lang="en">Historic England</cc:attributionName>
    <dc:publisher rdf:resource="https://historicengland.org.uk/"/>
    <dc:spatial rdf:resource="http://vocab.getty.edu/tgn/7002445"/>
    <dc:spatial rdf:resource="http://dbpedia.org/resource/England"/>
    <skos:prefLabel xml:lang="en">Golf Course</skos:prefLabel>
    <skos:scopeNote xml:lang="en">A landscaped area of ground, encompassing different types of terrain and features, such as ponds, sand-filled bunkers etc, on which the game of golf is played.</skos:scopeNote>
  </skos:Concept>

  <skos:Concept rdf:about="http://purl.org/heritagedata/schemes/571/concepts/160382">
    <skos:narrower rdf:resource="http://purl.org/heritagedata/schemes/571/concepts/151151"/>
    <skos:narrower>
      <skos:Concept rdf:about="http://purl.org/heritagedata/schemes/571/concepts/151152">
        <skos:broader rdf:resource="http://purl.org/heritagedata/schemes/571/concepts/160382"/>
        <skos:inScheme rdf:resource="http://purl.org/heritagedata/schemes/571"/>
        <dc:identifier>http://purl.org/heritagedata/schemes/571/concepts/151152</dc:identifier>
        <dc:issued rdf:datatype="http://www.w3.org/2001/XMLSchema#dateTime">2024-07-01T17:17:33</dc:issued>
        <cc:license rdf:resource="https://www.nationalarchives.gov.uk/doc/open-government-licence/version/3/"/>
        <cc:attributionURL rdf:resource="https://historicengland.org.uk/"/>
        <cc:attributionName xml:lang="en">Historic England</cc:attributionName>
        <dc:publisher rdf:resource="https://historicengland.org.uk/"/>
        <dc:spatial rdf:resource="http://vocab.getty.edu/tgn/7002445"/>
        <dc:spatial rdf:resource="http://dbpedia.org/resource/England"/>
        <skos:prefLabel xml:lang="en">Bowling Green</skos:prefLabel>
        <skos:scopeNote xml:lang="en">An area of closely mown lawn measured out and appropriately marked for use in the game of flat or crown green bowling.</skos:scopeNote>
      </skos:Concept>
    </skos:narrower>

    <skos:narrower>
      <skos:Concept rdf:about="http://purl.org/heritagedata/schemes/571/concepts/151154">
        <skos:broader rdf:resource="http://purl.org/heritagedata/schemes/571/concepts/160382"/>
        <skos:inScheme rdf:resource="http://purl.org/heritagedata/schemes/571"/>
        <dc:identifier>http://purl.org/heritagedata/schemes/571/concepts/151154</dc:identifier>
        <dc:issued rdf:datatype="http://www.w3.org/2001/XMLSchema#dateTime">2024-07-01T17:17:33</dc:issued>
        <cc:license rdf:resource="https://www.nationalarchives.gov.uk/doc/open-government-licence/version/3/"/>
        <cc:attributionURL rdf:resource="https://historicengland.org.uk/"/>
        <cc:attributionName xml:lang="en">Historic England</cc:attributionName>
        <dc:publisher rdf:resource="https://historicengland.org.uk/"/>
        <dc:spatial rdf:resource="http://vocab.getty.edu/tgn/7002445"/>
        <dc:spatial rdf:resource="http://dbpedia.org/resource/England"/>
        <skos:prefLabel xml:lang="en">Cricket Pitch</skos:prefLabel>
        <skos:scopeNote xml:lang="en">An area of grass, marked out for use in the game of cricket.</skos:scopeNote>
      </skos:Concept>
    </skos:narrower>

    <skos:broader rdf:resource="http://purl.org/heritagedata/schemes/571/concepts/152615"/>
    <skos:inScheme rdf:resource="http://purl.org/heritagedata/schemes/571"/>
    <dc:identifier>http://purl.org/heritagedata/schemes/571/concepts/160382</dc:identifier>
    <dc:issued rdf:datatype="http://www.w3.org/2001/XMLSchema#dateTime">2024-07-01T17:17:33</dc:issued>
    <cc:license rdf:resource="https://www.nationalarchives.gov.uk/doc/open-government-licence/version/3/"/>
    <cc:attributionURL rdf:resource="https://historicengland.org.uk/"/>
    <cc:attributionName xml:lang="en">Historic England</cc:attributionName>
    <dc:publisher rdf:resource="https://historicengland.org.uk/"/>
    <dc:spatial rdf:resource="http://vocab.getty.edu/tgn/7002445"/>
    <dc:spatial rdf:resource="http://dbpedia.org/resource/England"/>
    <skos:prefLabel xml:lang="en">Sports Field</skos:prefLabel>
    <skos:scopeNote xml:lang="en">An area of ground, often publically owned, where outdoor sports are played, usually with the necessary marking out and structures (goal posts etc). Distinguished from sports grounds where spectators pay to watch.</skos:scopeNote>
  </skos:Concept>

  <skos:Concept rdf:about="http://purl.org/heritagedata/schemes/571/concepts/151155">
    <skos:broader rdf:resource="http://purl.org/heritagedata/schemes/571/concepts/160294"/>
    <skos:inScheme rdf:resource="http://purl.org/heritagedata/schemes/571"/>
    <dc:identifier>http://purl.org/heritagedata/schemes/571/concepts/151155</dc:identifier>
    <dc:issued rdf:datatype="http://www.w3.org/2001/XMLSchema#dateTime">2024-07-01T17:17:33</dc:issued>
    <cc:license rdf:resource="https://www.nationalarchives.gov.uk/doc/open-government-licence/version/3/"/>
    <cc:attributionURL rdf:resource="https://historicengland.org.uk/"/>
    <cc:attributionName xml:lang="en">Historic England</cc:attributionName>
    <dc:publisher rdf:resource="https://historicengland.org.uk/"/>
    <dc:spatial rdf:resource="http://vocab.getty.edu/tgn/7002445"/>
    <dc:spatial rdf:resource="http://dbpedia.org/resource/England"/>
    <skos:prefLabel xml:lang="en">Safari Park</skos:prefLabel>
    <skos:scopeNote xml:lang="en">An area of parkland where animals are exhibited to the public but, unlike a zoo where they would occupy cages or small enclosures, are allowed to roam a large open environment.</skos:scopeNote>
  </skos:Concept>

  <skos:Concept rdf:about="http://purl.org/heritagedata/schemes/571/concepts/160294">
    <skos:narrower rdf:resource="http://purl.org/heritagedata/schemes/571/concepts/151155"/>
    <skos:narrower rdf:resource="http://purl.org/heritagedata/schemes/571/concepts/151159"/>
    <skos:broader rdf:resource="http://purl.org/heritagedata/schemes/571/concepts/151450"/>
    <skos:inScheme rdf:resource="http://purl.org/heritagedata/schemes/571"/>
    <dc:identifier>http://purl.org/heritagedata/schemes/571/concepts/160294</dc:identifier>
    <dc:issued rdf:datatype="http://www.w3.org/2001/XMLSchema#dateTime">2024-07-01T17:17:33</dc:issued>
    <cc:license rdf:resource="https://www.nationalarchives.gov.uk/doc/open-government-licence/version/3/"/>
    <cc:attributionURL rdf:resource="https://historicengland.org.uk/"/>
    <cc:attributionName xml:lang="en">Historic England</cc:attributionName>
    <dc:publisher rdf:resource="https://historicengland.org.uk/"/>
    <dc:spatial rdf:resource="http://vocab.getty.edu/tgn/7002445"/>
    <dc:spatial rdf:resource="http://dbpedia.org/resource/England"/>
    <skos:prefLabel xml:lang="en">Open Space</skos:prefLabel>
    <skos:scopeNote xml:lang="en">Public outdoor areas often with facilities for games and other activities.</skos:scopeNote>
  </skos:Concept>

  <skos:Concept rdf:about="http://purl.org/heritagedata/schemes/571/concepts/151158">
    <skos:broader rdf:resource="http://purl.org/heritagedata/schemes/571/concepts/160215"/>
    <skos:inScheme rdf:resource="http://purl.org/heritagedata/schemes/571"/>
    <dc:identifier>http://purl.org/heritagedata/schemes/571/concepts/151158</dc:identifier>
    <dc:issued rdf:datatype="http://www.w3.org/2001/XMLSchema#dateTime">2024-07-01T17:17:33</dc:issued>
    <cc:license rdf:resource="https://www.nationalarchives.gov.uk/doc/open-government-licence/version/3/"/>
    <cc:attributionURL rdf:resource="https://historicengland.org.uk/"/>
    <cc:attributionName xml:lang="en">Historic England</cc:attributionName>
    <dc:publisher rdf:resource="https://historicengland.org.uk/"/>
    <dc:spatial rdf:resource="http://vocab.getty.edu/tgn/7002445"/>
    <dc:spatial rdf:resource="http://dbpedia.org/resource/England"/>
    <skos:prefLabel xml:lang="en">Exhibition Centre</skos:prefLabel>
    <skos:scopeNote xml:lang="en">A complex, including large covered areas, used for housing public displays.</skos:scopeNote>
  </skos:Concept>

  <skos:Concept rdf:about="http://purl.org/heritagedata/schemes/571/concepts/160215">
    <skos:narrower rdf:resource="http://purl.org/heritagedata/schemes/571/concepts/151158"/>
    <skos:narrower>
      <skos:Concept rdf:about="http://purl.org/heritagedata/schemes/571/concepts/151291">
        <skos:broader rdf:resource="http://purl.org/heritagedata/schemes/571/concepts/160215"/>
        <skos:inScheme rdf:resource="http://purl.org/heritagedata/schemes/571"/>
        <dc:identifier>http://purl.org/heritagedata/schemes/571/concepts/151291</dc:identifier>
        <dc:issued rdf:datatype="http://www.w3.org/2001/XMLSchema#dateTime">2024-07-01T17:17:33</dc:issued>
        <cc:license rdf:resource="https://www.nationalarchives.gov.uk/doc/open-government-licence/version/3/"/>
        <cc:attributionURL rdf:resource="https://historicengland.org.uk/"/>
        <cc:attributionName xml:lang="en">Historic England</cc:attributionName>
        <dc:publisher rdf:resource="https://historicengland.org.uk/"/>
        <dc:spatial rdf:resource="http://vocab.getty.edu/tgn/7002445"/>
        <dc:spatial rdf:resource="http://dbpedia.org/resource/England"/>
        <skos:prefLabel xml:lang="en">Showground</skos:prefLabel>
        <skos:scopeNote xml:lang="en">A large area, usually open-air, used for permanent, seasonal or regular shows, events or exhibitions.</skos:scopeNote>
      </skos:Concept>
    </skos:narrower>

    <skos:broader rdf:resource="http://purl.org/heritagedata/schemes/571/concepts/151450"/>
    <skos:inScheme rdf:resource="http://purl.org/heritagedata/schemes/571"/>
    <dc:identifier>http://purl.org/heritagedata/schemes/571/concepts/160215</dc:identifier>
    <dc:issued rdf:datatype="http://www.w3.org/2001/XMLSchema#dateTime">2024-07-01T17:17:33</dc:issued>
    <cc:license rdf:resource="https://www.nationalarchives.gov.uk/doc/open-government-licence/version/3/"/>
    <cc:attributionURL rdf:resource="https://historicengland.org.uk/"/>
    <cc:attributionName xml:lang="en">Historic England</cc:attributionName>
    <dc:publisher rdf:resource="https://historicengland.org.uk/"/>
    <dc:spatial rdf:resource="http://vocab.getty.edu/tgn/7002445"/>
    <dc:spatial rdf:resource="http://dbpedia.org/resource/England"/>
    <skos:prefLabel xml:lang="en">Events</skos:prefLabel>
    <skos:scopeNote xml:lang="en">Complex designed to accomodate major gatherings.</skos:scopeNote>
  </skos:Concept>

  <skos:Concept rdf:about="http://purl.org/heritagedata/schemes/571/concepts/151159">
    <skos:broader rdf:resource="http://purl.org/heritagedata/schemes/571/concepts/160294"/>
    <skos:inScheme rdf:resource="http://purl.org/heritagedata/schemes/571"/>
    <dc:identifier>http://purl.org/heritagedata/schemes/571/concepts/151159</dc:identifier>
    <dc:issued rdf:datatype="http://www.w3.org/2001/XMLSchema#dateTime">2024-07-01T17:17:33</dc:issued>
    <cc:license rdf:resource="https://www.nationalarchives.gov.uk/doc/open-government-licence/version/3/"/>
    <cc:attributionURL rdf:resource="https://historicengland.org.uk/"/>
    <cc:attributionName xml:lang="en">Historic England</cc:attributionName>
    <dc:publisher rdf:resource="https://historicengland.org.uk/"/>
    <dc:spatial rdf:resource="http://vocab.getty.edu/tgn/7002445"/>
    <dc:spatial rdf:resource="http://dbpedia.org/resource/England"/>
    <skos:prefLabel xml:lang="en">Country Park</skos:prefLabel>
    <skos:related rdf:resource="http://purl.org/heritagedata/schemes/571/concepts/151756"/>
    <skos:scopeNote xml:lang="en">An area of managed countryside designated for visitors to enjoy recreations, such as walking specified parks and trails, in a rural environment. Often provides public facilities such as car parking, toilets, cafes and visitor information.</skos:scopeNote>
  </skos:Concept>

  <skos:Concept rdf:about="http://purl.org/heritagedata/schemes/571/concepts/151161">
    <skos:broader rdf:resource="http://purl.org/heritagedata/schemes/571/concepts/152301"/>
    <skos:inScheme rdf:resource="http://purl.org/heritagedata/schemes/571"/>
    <dc:identifier>http://purl.org/heritagedata/schemes/571/concepts/151161</dc:identifier>
    <dc:issued rdf:datatype="http://www.w3.org/2001/XMLSchema#dateTime">2024-07-01T17:17:33</dc:issued>
    <cc:license rdf:resource="https://www.nationalarchives.gov.uk/doc/open-government-licence/version/3/"/>
    <cc:attributionURL rdf:resource="https://historicengland.org.uk/"/>
    <cc:attributionName xml:lang="en">Historic England</cc:attributionName>
    <dc:publisher rdf:resource="https://historicengland.org.uk/"/>
    <dc:spatial rdf:resource="http://vocab.getty.edu/tgn/7002445"/>
    <dc:spatial rdf:resource="http://dbpedia.org/resource/England"/>
    <skos:prefLabel xml:lang="en">Stadium</skos:prefLabel>
    <skos:scopeNote xml:lang="en">A large, usually unroofed, sports ground surrounded by spectator seating arranged in tiers or terraces.</skos:scopeNote>
  </skos:Concept>

  <skos:Concept rdf:about="http://purl.org/heritagedata/schemes/571/concepts/152301">
    <skos:narrower rdf:resource="http://purl.org/heritagedata/schemes/571/concepts/151161"/>
    <skos:narrower>
      <skos:Concept rdf:about="http://purl.org/heritagedata/schemes/571/concepts/151288">
        <skos:broader rdf:resource="http://purl.org/heritagedata/schemes/571/concepts/152301"/>
        <skos:inScheme rdf:resource="http://purl.org/heritagedata/schemes/571"/>
        <dc:identifier>http://purl.org/heritagedata/schemes/571/concepts/151288</dc:identifier>
        <dc:issued rdf:datatype="http://www.w3.org/2001/XMLSchema#dateTime">2024-07-01T17:17:33</dc:issued>
        <cc:license rdf:resource="https://www.nationalarchives.gov.uk/doc/open-government-licence/version/3/"/>
        <cc:attributionURL rdf:resource="https://historicengland.org.uk/"/>
        <cc:attributionName xml:lang="en">Historic England</cc:attributionName>
        <dc:publisher rdf:resource="https://historicengland.org.uk/"/>
        <dc:spatial rdf:resource="http://vocab.getty.edu/tgn/7002445"/>
        <dc:spatial rdf:resource="http://dbpedia.org/resource/England"/>
        <skos:prefLabel xml:lang="en">Cricket Ground</skos:prefLabel>
        <skos:scopeNote xml:lang="en">The entire playing area and associated buildings upon which the game of cricket is played and where spectators pay to watch.</skos:scopeNote>
      </skos:Concept>
    </skos:narrower>

    <skos:narrower>
      <skos:Concept rdf:about="http://purl.org/heritagedata/schemes/571/concepts/151797">
        <skos:broader rdf:resource="http://purl.org/heritagedata/schemes/571/concepts/152301"/>
        <skos:inScheme rdf:resource="http://purl.org/heritagedata/schemes/571"/>
        <dc:identifier>http://purl.org/heritagedata/schemes/571/concepts/151797</dc:identifier>
        <dc:issued rdf:datatype="http://www.w3.org/2001/XMLSchema#dateTime">2024-07-01T17:17:33</dc:issued>
        <cc:license rdf:resource="https://www.nationalarchives.gov.uk/doc/open-government-licence/version/3/"/>
        <cc:attributionURL rdf:resource="https://historicengland.org.uk/"/>
        <cc:attributionName xml:lang="en">Historic England</cc:attributionName>
        <dc:publisher rdf:resource="https://historicengland.org.uk/"/>
        <dc:spatial rdf:resource="http://vocab.getty.edu/tgn/7002445"/>
        <dc:spatial rdf:resource="http://dbpedia.org/resource/England"/>
        <skos:prefLabel xml:lang="en">Motor Sports Track</skos:prefLabel>
        <skos:scopeNote xml:lang="en">A purpose-built facility for racing motor cars and/or motor cycles which may also include grandstands or concourses.</skos:scopeNote>
      </skos:Concept>
    </skos:narrower>

    <skos:narrower>
      <skos:Concept rdf:about="http://purl.org/heritagedata/schemes/571/concepts/152302">
        <skos:broader rdf:resource="http://purl.org/heritagedata/schemes/571/concepts/152301"/>
        <skos:inScheme rdf:resource="http://purl.org/heritagedata/schemes/571"/>
        <dc:identifier>http://purl.org/heritagedata/schemes/571/concepts/152302</dc:identifier>
        <dc:issued rdf:datatype="http://www.w3.org/2001/XMLSchema#dateTime">2024-07-01T17:17:33</dc:issued>
        <cc:license rdf:resource="https://www.nationalarchives.gov.uk/doc/open-government-licence/version/3/"/>
        <cc:attributionURL rdf:resource="https://historicengland.org.uk/"/>
        <cc:attributionName xml:lang="en">Historic England</cc:attributionName>
        <dc:publisher rdf:resource="https://historicengland.org.uk/"/>
        <dc:spatial rdf:resource="http://vocab.getty.edu/tgn/7002445"/>
        <dc:spatial rdf:resource="http://dbpedia.org/resource/England"/>
        <skos:prefLabel xml:lang="en">Football Ground</skos:prefLabel>
        <skos:scopeNote xml:lang="en">A site including a pitch, stands and other ancillary buildings and areas associated with playing and paying to watch the game of football.</skos:scopeNote>
      </skos:Concept>
    </skos:narrower>

    <skos:broader rdf:resource="http://purl.org/heritagedata/schemes/571/concepts/152615"/>
    <skos:inScheme rdf:resource="http://purl.org/heritagedata/schemes/571"/>
    <dc:identifier>http://purl.org/heritagedata/schemes/571/concepts/152301</dc:identifier>
    <dc:issued rdf:datatype="http://www.w3.org/2001/XMLSchema#dateTime">2024-07-01T17:17:33</dc:issued>
    <cc:license rdf:resource="https://www.nationalarchives.gov.uk/doc/open-government-licence/version/3/"/>
    <cc:attributionURL rdf:resource="https://historicengland.org.uk/"/>
    <cc:attributionName xml:lang="en">Historic England</cc:attributionName>
    <dc:publisher rdf:resource="https://historicengland.org.uk/"/>
    <dc:spatial rdf:resource="http://vocab.getty.edu/tgn/7002445"/>
    <dc:spatial rdf:resource="http://dbpedia.org/resource/England"/>
    <skos:prefLabel xml:lang="en">Sports Ground</skos:prefLabel>
    <skos:scopeNote xml:lang="en">An area of prepared ground on which a sport is played and where paying spectators watch. Use more specific type where known.</skos:scopeNote>
  </skos:Concept>

  <skos:Concept rdf:about="http://purl.org/heritagedata/schemes/571/concepts/151163">
    <skos:broader rdf:resource="http://purl.org/heritagedata/schemes/571/concepts/151646"/>
    <skos:inScheme rdf:resource="http://purl.org/heritagedata/schemes/571"/>
    <dc:identifier>http://purl.org/heritagedata/schemes/571/concepts/151163</dc:identifier>
    <dc:issued rdf:datatype="http://www.w3.org/2001/XMLSchema#dateTime">2024-07-01T17:17:33</dc:issued>
    <cc:license rdf:resource="https://www.nationalarchives.gov.uk/doc/open-government-licence/version/3/"/>
    <cc:attributionURL rdf:resource="https://historicengland.org.uk/"/>
    <cc:attributionName xml:lang="en">Historic England</cc:attributionName>
    <dc:publisher rdf:resource="https://historicengland.org.uk/"/>
    <dc:spatial rdf:resource="http://vocab.getty.edu/tgn/7002445"/>
    <dc:spatial rdf:resource="http://dbpedia.org/resource/England"/>
    <skos:prefLabel xml:lang="en">Hangars</skos:prefLabel>
    <skos:related rdf:resource="http://purl.org/heritagedata/schemes/571/concepts/151081"/>
    <skos:related rdf:resource="http://purl.org/heritagedata/schemes/571/concepts/151089"/>
    <skos:related rdf:resource="http://purl.org/heritagedata/schemes/571/concepts/151233"/>
    <skos:scopeNote xml:lang="en">Large sheds for the housing and maintainence of aircraft, etc.</skos:scopeNote>
  </skos:Concept>

  <skos:Concept rdf:about="http://purl.org/heritagedata/schemes/571/concepts/151646">
    <skos:narrower rdf:resource="http://purl.org/heritagedata/schemes/571/concepts/151163"/>
    <skos:broader rdf:resource="http://purl.org/heritagedata/schemes/571/concepts/151576"/>
    <skos:inScheme rdf:resource="http://purl.org/heritagedata/schemes/571"/>
    <dc:identifier>http://purl.org/heritagedata/schemes/571/concepts/151646</dc:identifier>
    <dc:issued rdf:datatype="http://www.w3.org/2001/XMLSchema#dateTime">2024-07-01T17:17:33</dc:issued>
    <cc:license rdf:resource="https://www.nationalarchives.gov.uk/doc/open-government-licence/version/3/"/>
    <cc:attributionURL rdf:resource="https://historicengland.org.uk/"/>
    <cc:attributionName xml:lang="en">Historic England</cc:attributionName>
    <dc:publisher rdf:resource="https://historicengland.org.uk/"/>
    <dc:spatial rdf:resource="http://vocab.getty.edu/tgn/7002445"/>
    <dc:spatial rdf:resource="http://dbpedia.org/resource/England"/>
    <skos:prefLabel xml:lang="en">Aircraft Storage Facility</skos:prefLabel>
    <skos:scopeNote xml:lang="en">A building or place where aircraft can be stored and maintained.</skos:scopeNote>
  </skos:Concept>

  <skos:Concept rdf:about="http://purl.org/heritagedata/schemes/571/concepts/151169">
    <skos:broader rdf:resource="http://purl.org/heritagedata/schemes/571/concepts/151727"/>
    <skos:inScheme rdf:resource="http://purl.org/heritagedata/schemes/571"/>
    <dc:identifier>http://purl.org/heritagedata/schemes/571/concepts/151169</dc:identifier>
    <dc:issued rdf:datatype="http://www.w3.org/2001/XMLSchema#dateTime">2024-07-01T17:17:33</dc:issued>
    <cc:license rdf:resource="https://www.nationalarchives.gov.uk/doc/open-government-licence/version/3/"/>
    <cc:attributionURL rdf:resource="https://historicengland.org.uk/"/>
    <cc:attributionName xml:lang="en">Historic England</cc:attributionName>
    <dc:publisher rdf:resource="https://historicengland.org.uk/"/>
    <dc:spatial rdf:resource="http://vocab.getty.edu/tgn/7002445"/>
    <dc:spatial rdf:resource="http://dbpedia.org/resource/England"/>
    <skos:prefLabel xml:lang="en">Paddocks</skos:prefLabel>
    <skos:scopeNote xml:lang="en">An enclosed field for horses. Usually a modern adaptation of part of an early field system.</skos:scopeNote>
  </skos:Concept>

  <skos:Concept rdf:about="http://purl.org/heritagedata/schemes/571/concepts/151727">
    <skos:narrower rdf:resource="http://purl.org/heritagedata/schemes/571/concepts/151169"/>
    <skos:narrower rdf:resource="http://purl.org/heritagedata/schemes/571/concepts/151173"/>
    <skos:narrower rdf:resource="http://purl.org/heritagedata/schemes/571/concepts/151281"/>
    <skos:narrower rdf:resource="http://purl.org/heritagedata/schemes/571/concepts/151728"/>
    <skos:narrower>
      <skos:Concept rdf:about="http://purl.org/heritagedata/schemes/571/concepts/151733">
        <skos:broader rdf:resource="http://purl.org/heritagedata/schemes/571/concepts/151727"/>
        <skos:inScheme rdf:resource="http://purl.org/heritagedata/schemes/571"/>
        <dc:identifier>http://purl.org/heritagedata/schemes/571/concepts/151733</dc:identifier>
        <dc:issued rdf:datatype="http://www.w3.org/2001/XMLSchema#dateTime">2024-07-01T17:17:33</dc:issued>
        <cc:license rdf:resource="https://www.nationalarchives.gov.uk/doc/open-government-licence/version/3/"/>
        <cc:attributionURL rdf:resource="https://historicengland.org.uk/"/>
        <cc:attributionName xml:lang="en">Historic England</cc:attributionName>
        <dc:publisher rdf:resource="https://historicengland.org.uk/"/>
        <dc:spatial rdf:resource="http://vocab.getty.edu/tgn/7002445"/>
        <dc:spatial rdf:resource="http://dbpedia.org/resource/England"/>
        <skos:prefLabel xml:lang="en">Prairie Fields</skos:prefLabel>
        <skos:scopeNote xml:lang="en">Patterns of very large fields, some with boundaries over 1km long. Usually resulting from post WW2 combination of holdings &amp; the removal of earlier boundaries creating land units convenient for highly mechanised arable, or for extensive livestock raising</skos:scopeNote>
      </skos:Concept>
    </skos:narrower>

    <skos:narrower rdf:resource="http://purl.org/heritagedata/schemes/571/concepts/151780"/>
    <skos:narrower>
      <skos:Concept rdf:about="http://purl.org/heritagedata/schemes/571/concepts/151785">
        <skos:broader rdf:resource="http://purl.org/heritagedata/schemes/571/concepts/151727"/>
        <skos:inScheme rdf:resource="http://purl.org/heritagedata/schemes/571"/>
        <dc:identifier>http://purl.org/heritagedata/schemes/571/concepts/151785</dc:identifier>
        <dc:issued rdf:datatype="http://www.w3.org/2001/XMLSchema#dateTime">2024-07-01T17:17:33</dc:issued>
        <cc:license rdf:resource="https://www.nationalarchives.gov.uk/doc/open-government-licence/version/3/"/>
        <cc:attributionURL rdf:resource="https://historicengland.org.uk/"/>
        <cc:attributionName xml:lang="en">Historic England</cc:attributionName>
        <dc:publisher rdf:resource="https://historicengland.org.uk/"/>
        <dc:spatial rdf:resource="http://vocab.getty.edu/tgn/7002445"/>
        <dc:spatial rdf:resource="http://dbpedia.org/resource/England"/>
        <skos:prefLabel xml:lang="en">Reorganised Field System</skos:prefLabel>
        <skos:scopeNote xml:lang="en">Field pattern of any type or date that has been subject to revision, through either insertion or removal of boundaries, but where the original form is still legible.</skos:scopeNote>
      </skos:Concept>
    </skos:narrower>

    <skos:narrower rdf:resource="http://purl.org/heritagedata/schemes/571/concepts/151787"/>
    <skos:narrower rdf:resource="http://purl.org/heritagedata/schemes/571/concepts/160157"/>
    <skos:narrower rdf:resource="http://purl.org/heritagedata/schemes/571/concepts/160160"/>
    <skos:narrower>
      <skos:Concept rdf:about="http://purl.org/heritagedata/schemes/571/concepts/160161">
        <skos:broader rdf:resource="http://purl.org/heritagedata/schemes/571/concepts/151727"/>
        <skos:inScheme rdf:resource="http://purl.org/heritagedata/schemes/571"/>
        <dc:identifier>http://purl.org/heritagedata/schemes/571/concepts/160161</dc:identifier>
        <dc:issued rdf:datatype="http://www.w3.org/2001/XMLSchema#dateTime">2024-07-01T17:17:33</dc:issued>
        <cc:license rdf:resource="https://www.nationalarchives.gov.uk/doc/open-government-licence/version/3/"/>
        <cc:attributionURL rdf:resource="https://historicengland.org.uk/"/>
        <cc:attributionName xml:lang="en">Historic England</cc:attributionName>
        <dc:publisher rdf:resource="https://historicengland.org.uk/"/>
        <dc:spatial rdf:resource="http://vocab.getty.edu/tgn/7002445"/>
        <dc:spatial rdf:resource="http://dbpedia.org/resource/England"/>
        <skos:prefLabel xml:lang="en">Infields</skos:prefLabel>
        <skos:scopeNote xml:lang="en">The more closely assessed and more intensively worked fields of an infield-outfield system, usually of open field type.</skos:scopeNote>
      </skos:Concept>
    </skos:narrower>

    <skos:narrower>
      <skos:Concept rdf:about="http://purl.org/heritagedata/schemes/571/concepts/160164">
        <skos:broader rdf:resource="http://purl.org/heritagedata/schemes/571/concepts/151727"/>
        <skos:inScheme rdf:resource="http://purl.org/heritagedata/schemes/571"/>
        <dc:identifier>http://purl.org/heritagedata/schemes/571/concepts/160164</dc:identifier>
        <dc:issued rdf:datatype="http://www.w3.org/2001/XMLSchema#dateTime">2024-07-01T17:17:33</dc:issued>
        <cc:license rdf:resource="https://www.nationalarchives.gov.uk/doc/open-government-licence/version/3/"/>
        <cc:attributionURL rdf:resource="https://historicengland.org.uk/"/>
        <cc:attributionName xml:lang="en">Historic England</cc:attributionName>
        <dc:publisher rdf:resource="https://historicengland.org.uk/"/>
        <dc:spatial rdf:resource="http://vocab.getty.edu/tgn/7002445"/>
        <dc:spatial rdf:resource="http://dbpedia.org/resource/England"/>
        <skos:prefLabel xml:lang="en">Outfields</skos:prefLabel>
        <skos:scopeNote xml:lang="en">Marginal fields, often part of open field systems, beyond the more closely assessed and more intensively worked infields. In places left uncultivated for many decades. Often worked in common and divided into strips.</skos:scopeNote>
      </skos:Concept>
    </skos:narrower>

    <skos:narrower rdf:resource="http://purl.org/heritagedata/schemes/571/concepts/160165"/>
    <skos:broader rdf:resource="http://purl.org/heritagedata/schemes/571/concepts/151453"/>
    <skos:inScheme rdf:resource="http://purl.org/heritagedata/schemes/571"/>
    <dc:identifier>http://purl.org/heritagedata/schemes/571/concepts/151727</dc:identifier>
    <dc:issued rdf:datatype="http://www.w3.org/2001/XMLSchema#dateTime">2024-07-01T17:17:33</dc:issued>
    <cc:license rdf:resource="https://www.nationalarchives.gov.uk/doc/open-government-licence/version/3/"/>
    <cc:attributionURL rdf:resource="https://historicengland.org.uk/"/>
    <cc:attributionName xml:lang="en">Historic England</cc:attributionName>
    <dc:publisher rdf:resource="https://historicengland.org.uk/"/>
    <dc:spatial rdf:resource="http://vocab.getty.edu/tgn/7002445"/>
    <dc:spatial rdf:resource="http://dbpedia.org/resource/England"/>
    <skos:prefLabel xml:lang="en">Field System</skos:prefLabel>
    <skos:scopeNote xml:lang="en">A group or complex of fields which appear to form a coherent whole, usually on the basis of another system, normally that of tenure. Includes rearrangements of earlier systems.</skos:scopeNote>
  </skos:Concept>

  <skos:Concept rdf:about="http://purl.org/heritagedata/schemes/571/concepts/151170">
    <skos:broader rdf:resource="http://purl.org/heritagedata/schemes/571/concepts/151453"/>
    <skos:inScheme rdf:resource="http://purl.org/heritagedata/schemes/571"/>
    <dc:identifier>http://purl.org/heritagedata/schemes/571/concepts/151170</dc:identifier>
    <dc:issued rdf:datatype="http://www.w3.org/2001/XMLSchema#dateTime">2024-07-01T17:17:33</dc:issued>
    <cc:license rdf:resource="https://www.nationalarchives.gov.uk/doc/open-government-licence/version/3/"/>
    <cc:attributionURL rdf:resource="https://historicengland.org.uk/"/>
    <cc:attributionName xml:lang="en">Historic England</cc:attributionName>
    <dc:publisher rdf:resource="https://historicengland.org.uk/"/>
    <dc:spatial rdf:resource="http://vocab.getty.edu/tgn/7002445"/>
    <dc:spatial rdf:resource="http://dbpedia.org/resource/England"/>
    <skos:prefLabel xml:lang="en">Meadow</skos:prefLabel>
    <skos:scopeNote xml:lang="en">Permanent grassland, usually enclosed with stock-proof boundaries. Low-lying and damp or hard by farmstead, receiving yard dung. Ideally lush, and mown for hay. Also secure convenient grazing for young or sickly livestock. Common or individually held.</skos:scopeNote>
  </skos:Concept>

  <skos:Concept rdf:about="http://purl.org/heritagedata/schemes/571/concepts/151453">
    <skos:narrower rdf:resource="http://purl.org/heritagedata/schemes/571/concepts/151170"/>
    <skos:narrower rdf:resource="http://purl.org/heritagedata/schemes/571/concepts/151176"/>
    <skos:narrower>
      <skos:Concept rdf:about="http://purl.org/heritagedata/schemes/571/concepts/151182">
        <skos:broader rdf:resource="http://purl.org/heritagedata/schemes/571/concepts/151453"/>
        <skos:inScheme rdf:resource="http://purl.org/heritagedata/schemes/571"/>
        <dc:identifier>http://purl.org/heritagedata/schemes/571/concepts/151182</dc:identifier>
        <dc:issued rdf:datatype="http://www.w3.org/2001/XMLSchema#dateTime">2024-07-01T17:17:33</dc:issued>
        <cc:license rdf:resource="https://www.nationalarchives.gov.uk/doc/open-government-licence/version/3/"/>
        <cc:attributionURL rdf:resource="https://historicengland.org.uk/"/>
        <cc:attributionName xml:lang="en">Historic England</cc:attributionName>
        <dc:publisher rdf:resource="https://historicengland.org.uk/"/>
        <dc:spatial rdf:resource="http://vocab.getty.edu/tgn/7002445"/>
        <dc:spatial rdf:resource="http://dbpedia.org/resource/England"/>
        <skos:prefLabel xml:lang="en">Squatter Enclosure</skos:prefLabel>
        <skos:scopeNote xml:lang="en">A small, irregular enclosure taken from formerly open land, usually common land. Sometimes associated with industrial activity and/or routes of access. Normally later medieval or early post-medieval.</skos:scopeNote>
      </skos:Concept>
    </skos:narrower>

    <skos:narrower rdf:resource="http://purl.org/heritagedata/schemes/571/concepts/151297"/>
    <skos:narrower rdf:resource="http://purl.org/heritagedata/schemes/571/concepts/151417"/>
    <skos:narrower rdf:resource="http://purl.org/heritagedata/schemes/571/concepts/151727"/>
    <skos:narrower rdf:resource="http://purl.org/heritagedata/schemes/571/concepts/151730"/>
    <skos:narrower rdf:resource="http://purl.org/heritagedata/schemes/571/concepts/151732"/>
    <skos:narrower>
      <skos:Concept rdf:about="http://purl.org/heritagedata/schemes/571/concepts/151786">
        <skos:broader rdf:resource="http://purl.org/heritagedata/schemes/571/concepts/151453"/>
        <skos:inScheme rdf:resource="http://purl.org/heritagedata/schemes/571"/>
        <dc:identifier>http://purl.org/heritagedata/schemes/571/concepts/151786</dc:identifier>
        <dc:issued rdf:datatype="http://www.w3.org/2001/XMLSchema#dateTime">2024-07-01T17:17:33</dc:issued>
        <cc:license rdf:resource="https://www.nationalarchives.gov.uk/doc/open-government-licence/version/3/"/>
        <cc:attributionURL rdf:resource="https://historicengland.org.uk/"/>
        <cc:attributionName xml:lang="en">Historic England</cc:attributionName>
        <dc:publisher rdf:resource="https://historicengland.org.uk/"/>
        <dc:spatial rdf:resource="http://vocab.getty.edu/tgn/7002445"/>
        <dc:spatial rdf:resource="http://dbpedia.org/resource/England"/>
        <skos:prefLabel xml:lang="en">Restored Fields</skos:prefLabel>
        <skos:scopeNote xml:lang="en">Fields created on the surface of restored land, such as that landscaped from the former dumps of coal mines. Modern and often regular.</skos:scopeNote>
      </skos:Concept>
    </skos:narrower>

    <skos:narrower rdf:resource="http://purl.org/heritagedata/schemes/571/concepts/160155"/>
    <skos:narrower rdf:resource="http://purl.org/heritagedata/schemes/571/concepts/160156"/>
    <skos:narrower>
      <skos:Concept rdf:about="http://purl.org/heritagedata/schemes/571/concepts/160159">
        <skos:broader rdf:resource="http://purl.org/heritagedata/schemes/571/concepts/151453"/>
        <skos:inScheme rdf:resource="http://purl.org/heritagedata/schemes/571"/>
        <dc:identifier>http://purl.org/heritagedata/schemes/571/concepts/160159</dc:identifier>
        <dc:issued rdf:datatype="http://www.w3.org/2001/XMLSchema#dateTime">2024-07-01T17:17:33</dc:issued>
        <cc:license rdf:resource="https://www.nationalarchives.gov.uk/doc/open-government-licence/version/3/"/>
        <cc:attributionURL rdf:resource="https://historicengland.org.uk/"/>
        <cc:attributionName xml:lang="en">Historic England</cc:attributionName>
        <dc:publisher rdf:resource="https://historicengland.org.uk/"/>
        <dc:spatial rdf:resource="http://vocab.getty.edu/tgn/7002445"/>
        <dc:spatial rdf:resource="http://dbpedia.org/resource/England"/>
        <skos:prefLabel xml:lang="en">Enclosure Of Parkland</skos:prefLabel>
        <skos:scopeNote xml:lang="en">Fields established within former parkland, either medieval deer park or post-medieval landscaped park. Tend to be large and regular fields and land often retains some parkland features, notably standard trees.</skos:scopeNote>
      </skos:Concept>
    </skos:narrower>

    <skos:narrower>
      <skos:Concept rdf:about="http://purl.org/heritagedata/schemes/571/concepts/160162">
        <skos:broader rdf:resource="http://purl.org/heritagedata/schemes/571/concepts/151453"/>
        <skos:inScheme rdf:resource="http://purl.org/heritagedata/schemes/571"/>
        <dc:identifier>http://purl.org/heritagedata/schemes/571/concepts/160162</dc:identifier>
        <dc:issued rdf:datatype="http://www.w3.org/2001/XMLSchema#dateTime">2024-07-01T17:17:33</dc:issued>
        <cc:license rdf:resource="https://www.nationalarchives.gov.uk/doc/open-government-licence/version/3/"/>
        <cc:attributionURL rdf:resource="https://historicengland.org.uk/"/>
        <cc:attributionName xml:lang="en">Historic England</cc:attributionName>
        <dc:publisher rdf:resource="https://historicengland.org.uk/"/>
        <dc:spatial rdf:resource="http://vocab.getty.edu/tgn/7002445"/>
        <dc:spatial rdf:resource="http://dbpedia.org/resource/England"/>
        <skos:prefLabel xml:lang="en">Intake From Rough Ground</skos:prefLabel>
        <skos:scopeNote xml:lang="en">Fields established on former rough ground. Mostly post-medieval.</skos:scopeNote>
      </skos:Concept>
    </skos:narrower>

    <skos:narrower rdf:resource="http://purl.org/heritagedata/schemes/571/concepts/160163"/>
    <skos:narrower rdf:resource="http://purl.org/heritagedata/schemes/571/concepts/160166"/>
    <skos:inScheme rdf:resource="http://purl.org/heritagedata/schemes/571"/>
    <dc:identifier>http://purl.org/heritagedata/schemes/571/concepts/151453</dc:identifier>
    <dc:issued rdf:datatype="http://www.w3.org/2001/XMLSchema#dateTime">2024-07-01T17:17:33</dc:issued>
    <cc:license rdf:resource="https://www.nationalarchives.gov.uk/doc/open-government-licence/version/3/"/>
    <cc:attributionURL rdf:resource="https://historicengland.org.uk/"/>
    <cc:attributionName xml:lang="en">Historic England</cc:attributionName>
    <dc:publisher rdf:resource="https://historicengland.org.uk/"/>
    <dc:spatial rdf:resource="http://vocab.getty.edu/tgn/7002445"/>
    <dc:spatial rdf:resource="http://dbpedia.org/resource/England"/>
    <skos:prefLabel xml:lang="en">Enclosure</skos:prefLabel>
    <skos:scopeNote xml:lang="en">Patterns of fields that took in farmland (either cultivated or improved grassland) from other land uses.</skos:scopeNote>
    <skos:topConceptOf rdf:resource="http://purl.org/heritagedata/schemes/571"/>
  </skos:Concept>

  <skos:Concept rdf:about="http://purl.org/heritagedata/schemes/571/concepts/151171">
    <skos:broader rdf:resource="http://purl.org/heritagedata/schemes/571/concepts/152403"/>
    <skos:inScheme rdf:resource="http://purl.org/heritagedata/schemes/571"/>
    <dc:identifier>http://purl.org/heritagedata/schemes/571/concepts/151171</dc:identifier>
    <dc:issued rdf:datatype="http://www.w3.org/2001/XMLSchema#dateTime">2024-07-01T17:17:33</dc:issued>
    <cc:license rdf:resource="https://www.nationalarchives.gov.uk/doc/open-government-licence/version/3/"/>
    <cc:attributionURL rdf:resource="https://historicengland.org.uk/"/>
    <cc:attributionName xml:lang="en">Historic England</cc:attributionName>
    <dc:publisher rdf:resource="https://historicengland.org.uk/"/>
    <dc:spatial rdf:resource="http://vocab.getty.edu/tgn/7002445"/>
    <dc:spatial rdf:resource="http://dbpedia.org/resource/England"/>
    <skos:prefLabel xml:lang="en">Stud Farm</skos:prefLabel>
    <skos:scopeNote xml:lang="en">A farm where racehorses are bred and stabled.</skos:scopeNote>
  </skos:Concept>

  <skos:Concept rdf:about="http://purl.org/heritagedata/schemes/571/concepts/152403">
    <skos:narrower rdf:resource="http://purl.org/heritagedata/schemes/571/concepts/151171"/>
    <skos:narrower>
      <skos:Concept rdf:about="http://purl.org/heritagedata/schemes/571/concepts/152299">
        <skos:broader rdf:resource="http://purl.org/heritagedata/schemes/571/concepts/152403"/>
        <skos:inScheme rdf:resource="http://purl.org/heritagedata/schemes/571"/>
        <dc:identifier>http://purl.org/heritagedata/schemes/571/concepts/152299</dc:identifier>
        <dc:issued rdf:datatype="http://www.w3.org/2001/XMLSchema#dateTime">2024-07-01T17:17:33</dc:issued>
        <cc:license rdf:resource="https://www.nationalarchives.gov.uk/doc/open-government-licence/version/3/"/>
        <cc:attributionURL rdf:resource="https://historicengland.org.uk/"/>
        <cc:attributionName xml:lang="en">Historic England</cc:attributionName>
        <dc:publisher rdf:resource="https://historicengland.org.uk/"/>
        <dc:spatial rdf:resource="http://vocab.getty.edu/tgn/7002445"/>
        <dc:spatial rdf:resource="http://dbpedia.org/resource/England"/>
        <skos:prefLabel xml:lang="en">Stables</skos:prefLabel>
        <skos:scopeNote xml:lang="en">Building complex with yards etc, where horses are bred, raised and securely kept.</skos:scopeNote>
      </skos:Concept>
    </skos:narrower>

    <skos:narrower rdf:resource="http://purl.org/heritagedata/schemes/571/concepts/152305"/>
    <skos:narrower>
      <skos:Concept rdf:about="http://purl.org/heritagedata/schemes/571/concepts/160275">
        <skos:broader rdf:resource="http://purl.org/heritagedata/schemes/571/concepts/152403"/>
        <skos:inScheme rdf:resource="http://purl.org/heritagedata/schemes/571"/>
        <dc:identifier>http://purl.org/heritagedata/schemes/571/concepts/160275</dc:identifier>
        <dc:issued rdf:datatype="http://www.w3.org/2001/XMLSchema#dateTime">2024-07-01T17:17:33</dc:issued>
        <cc:license rdf:resource="https://www.nationalarchives.gov.uk/doc/open-government-licence/version/3/"/>
        <cc:attributionURL rdf:resource="https://historicengland.org.uk/"/>
        <cc:attributionName xml:lang="en">Historic England</cc:attributionName>
        <dc:publisher rdf:resource="https://historicengland.org.uk/"/>
        <dc:spatial rdf:resource="http://vocab.getty.edu/tgn/7002445"/>
        <dc:spatial rdf:resource="http://dbpedia.org/resource/England"/>
        <skos:prefLabel xml:lang="en">Race Course</skos:prefLabel>
        <skos:scopeNote xml:lang="en">A purpose-built facility for the racing of horses; may also include grandstands or concourses.</skos:scopeNote>
      </skos:Concept>
    </skos:narrower>

    <skos:broader rdf:resource="http://purl.org/heritagedata/schemes/571/concepts/152615"/>
    <skos:inScheme rdf:resource="http://purl.org/heritagedata/schemes/571"/>
    <dc:identifier>http://purl.org/heritagedata/schemes/571/concepts/152403</dc:identifier>
    <dc:issued rdf:datatype="http://www.w3.org/2001/XMLSchema#dateTime">2024-07-01T17:17:33</dc:issued>
    <cc:license rdf:resource="https://www.nationalarchives.gov.uk/doc/open-government-licence/version/3/"/>
    <cc:attributionURL rdf:resource="https://historicengland.org.uk/"/>
    <cc:attributionName xml:lang="en">Historic England</cc:attributionName>
    <dc:publisher rdf:resource="https://historicengland.org.uk/"/>
    <dc:spatial rdf:resource="http://vocab.getty.edu/tgn/7002445"/>
    <dc:spatial rdf:resource="http://dbpedia.org/resource/England"/>
    <skos:prefLabel xml:lang="en">Horse Racing</skos:prefLabel>
    <skos:scopeNote xml:lang="en">Areas relating to the sport that involves breeding and training thoroughbred horses and racing them against each other on large courses.</skos:scopeNote>
  </skos:Concept>

  <skos:Concept rdf:about="http://purl.org/heritagedata/schemes/571/concepts/151173">
    <skos:broader rdf:resource="http://purl.org/heritagedata/schemes/571/concepts/151727"/>
    <skos:narrower rdf:resource="http://purl.org/heritagedata/schemes/571/concepts/151781"/>
    <skos:inScheme rdf:resource="http://purl.org/heritagedata/schemes/571"/>
    <dc:identifier>http://purl.org/heritagedata/schemes/571/concepts/151173</dc:identifier>
    <dc:issued rdf:datatype="http://www.w3.org/2001/XMLSchema#dateTime">2024-07-01T17:17:33</dc:issued>
    <cc:license rdf:resource="https://www.nationalarchives.gov.uk/doc/open-government-licence/version/3/"/>
    <cc:attributionURL rdf:resource="https://historicengland.org.uk/"/>
    <cc:attributionName xml:lang="en">Historic England</cc:attributionName>
    <dc:publisher rdf:resource="https://historicengland.org.uk/"/>
    <dc:spatial rdf:resource="http://vocab.getty.edu/tgn/7002445"/>
    <dc:spatial rdf:resource="http://dbpedia.org/resource/England"/>
    <skos:prefLabel xml:lang="en">Open Field System</skos:prefLabel>
    <skos:related rdf:resource="http://purl.org/heritagedata/schemes/571/concepts/160155"/>
    <skos:scopeNote xml:lang="en">System of fields in which several farmers held land in common, intermixed in narrow strips assessable via length and width, with low or no separating boundaries. Mostly medieval. Few survive. Lost to piecemeal or planned enclosure, 13th - 20th century.</skos:scopeNote>
  </skos:Concept>

  <skos:Concept rdf:about="http://purl.org/heritagedata/schemes/571/concepts/151176">
    <skos:broader rdf:resource="http://purl.org/heritagedata/schemes/571/concepts/151453"/>
    <skos:inScheme rdf:resource="http://purl.org/heritagedata/schemes/571"/>
    <dc:identifier>http://purl.org/heritagedata/schemes/571/concepts/151176</dc:identifier>
    <dc:issued rdf:datatype="http://www.w3.org/2001/XMLSchema#dateTime">2024-07-01T17:17:33</dc:issued>
    <cc:license rdf:resource="https://www.nationalarchives.gov.uk/doc/open-government-licence/version/3/"/>
    <cc:attributionURL rdf:resource="https://historicengland.org.uk/"/>
    <cc:attributionName xml:lang="en">Historic England</cc:attributionName>
    <dc:publisher rdf:resource="https://historicengland.org.uk/"/>
    <dc:spatial rdf:resource="http://vocab.getty.edu/tgn/7002445"/>
    <dc:spatial rdf:resource="http://dbpedia.org/resource/England"/>
    <skos:prefLabel xml:lang="en">Croft</skos:prefLabel>
    <skos:related rdf:resource="http://purl.org/heritagedata/schemes/571/concepts/160155"/>
    <skos:related rdf:resource="http://purl.org/heritagedata/schemes/571/concepts/160166"/>
    <skos:scopeNote xml:lang="en">Meaning varies: In Scotland a holding of enclosed farmland, in Cornwall later medieval and post-medieval enclosure containing rough ground used for grazing and furze. In central England a strip of garden attached to a messuage in a medieval village.</skos:scopeNote>
  </skos:Concept>

  <skos:Concept rdf:about="http://purl.org/heritagedata/schemes/571/concepts/151177">
    <skos:broader rdf:resource="http://purl.org/heritagedata/schemes/571/concepts/151732"/>
    <skos:inScheme rdf:resource="http://purl.org/heritagedata/schemes/571"/>
    <dc:identifier>http://purl.org/heritagedata/schemes/571/concepts/151177</dc:identifier>
    <dc:issued rdf:datatype="http://www.w3.org/2001/XMLSchema#dateTime">2024-07-01T17:17:33</dc:issued>
    <cc:license rdf:resource="https://www.nationalarchives.gov.uk/doc/open-government-licence/version/3/"/>
    <cc:attributionURL rdf:resource="https://historicengland.org.uk/"/>
    <cc:attributionName xml:lang="en">Historic England</cc:attributionName>
    <dc:publisher rdf:resource="https://historicengland.org.uk/"/>
    <dc:spatial rdf:resource="http://vocab.getty.edu/tgn/7002445"/>
    <dc:spatial rdf:resource="http://dbpedia.org/resource/England"/>
    <skos:prefLabel xml:lang="en">Parliamentary Enclosure</skos:prefLabel>
    <skos:scopeNote xml:lang="en">Field patterns usually rectilinear and regular with straight boundaries and access lanes, fixed by surveyors, resulting from Parliamentary Enclosure of large areas of common arable (open fields) and rough ground. Mainly 18th and 19th centuries.</skos:scopeNote>
  </skos:Concept>

  <skos:Concept rdf:about="http://purl.org/heritagedata/schemes/571/concepts/151732">
    <skos:narrower rdf:resource="http://purl.org/heritagedata/schemes/571/concepts/151177"/>
    <skos:broader rdf:resource="http://purl.org/heritagedata/schemes/571/concepts/151453"/>
    <skos:inScheme rdf:resource="http://purl.org/heritagedata/schemes/571"/>
    <dc:identifier>http://purl.org/heritagedata/schemes/571/concepts/151732</dc:identifier>
    <dc:issued rdf:datatype="http://www.w3.org/2001/XMLSchema#dateTime">2024-07-01T17:17:33</dc:issued>
    <cc:license rdf:resource="https://www.nationalarchives.gov.uk/doc/open-government-licence/version/3/"/>
    <cc:attributionURL rdf:resource="https://historicengland.org.uk/"/>
    <cc:attributionName xml:lang="en">Historic England</cc:attributionName>
    <dc:publisher rdf:resource="https://historicengland.org.uk/"/>
    <dc:spatial rdf:resource="http://vocab.getty.edu/tgn/7002445"/>
    <dc:spatial rdf:resource="http://dbpedia.org/resource/England"/>
    <skos:prefLabel xml:lang="en">Planned Enclosure</skos:prefLabel>
    <skos:scopeNote xml:lang="en">Field patterns with perfectly straight stock-proof boundaries, usually rectilinear and regular. Normally produced by planned enclosure by several landholders of formerly open or common land. Usually post medieval or modern.</skos:scopeNote>
  </skos:Concept>

  <skos:Concept rdf:about="http://purl.org/heritagedata/schemes/571/concepts/151178">
    <skos:broader rdf:resource="http://purl.org/heritagedata/schemes/571/concepts/160165"/>
    <skos:inScheme rdf:resource="http://purl.org/heritagedata/schemes/571"/>
    <dc:identifier>http://purl.org/heritagedata/schemes/571/concepts/151178</dc:identifier>
    <dc:issued rdf:datatype="http://www.w3.org/2001/XMLSchema#dateTime">2024-07-01T17:17:33</dc:issued>
    <cc:license rdf:resource="https://www.nationalarchives.gov.uk/doc/open-government-licence/version/3/"/>
    <cc:attributionURL rdf:resource="https://historicengland.org.uk/"/>
    <cc:attributionName xml:lang="en">Historic England</cc:attributionName>
    <dc:publisher rdf:resource="https://historicengland.org.uk/"/>
    <dc:spatial rdf:resource="http://vocab.getty.edu/tgn/7002445"/>
    <dc:spatial rdf:resource="http://dbpedia.org/resource/England"/>
    <skos:prefLabel xml:lang="en">Ladder Field System</skos:prefLabel>
    <skos:scopeNote xml:lang="en">A holding's fields contained within two long, usually perfectly straight boundaries extending outwards from a farmstead; often parallel, but sometimes splayed. Divided by cross boundaries into fields. Usually post-medieval or modern.</skos:scopeNote>
  </skos:Concept>

  <skos:Concept rdf:about="http://purl.org/heritagedata/schemes/571/concepts/160165">
    <skos:narrower rdf:resource="http://purl.org/heritagedata/schemes/571/concepts/151178"/>
    <skos:broader rdf:resource="http://purl.org/heritagedata/schemes/571/concepts/151727"/>
    <skos:inScheme rdf:resource="http://purl.org/heritagedata/schemes/571"/>
    <dc:identifier>http://purl.org/heritagedata/schemes/571/concepts/160165</dc:identifier>
    <dc:issued rdf:datatype="http://www.w3.org/2001/XMLSchema#dateTime">2024-07-01T17:17:33</dc:issued>
    <cc:license rdf:resource="https://www.nationalarchives.gov.uk/doc/open-government-licence/version/3/"/>
    <cc:attributionURL rdf:resource="https://historicengland.org.uk/"/>
    <cc:attributionName xml:lang="en">Historic England</cc:attributionName>
    <dc:publisher rdf:resource="https://historicengland.org.uk/"/>
    <dc:spatial rdf:resource="http://vocab.getty.edu/tgn/7002445"/>
    <dc:spatial rdf:resource="http://dbpedia.org/resource/England"/>
    <skos:prefLabel xml:lang="en">Planned Field System</skos:prefLabel>
    <skos:scopeNote xml:lang="en">Field system, usually with perfectly straight boundaries, usually rectilinear and regular, developed by reorganisation by several landowners of an earlier system. Term often used for post-medieval non-Parliamentary Enclosure of open fields.</skos:scopeNote>
  </skos:Concept>

  <skos:Concept rdf:about="http://purl.org/heritagedata/schemes/571/concepts/151179">
    <skos:broader rdf:resource="http://purl.org/heritagedata/schemes/571/concepts/151728"/>
    <skos:inScheme rdf:resource="http://purl.org/heritagedata/schemes/571"/>
    <dc:identifier>http://purl.org/heritagedata/schemes/571/concepts/151179</dc:identifier>
    <dc:issued rdf:datatype="http://www.w3.org/2001/XMLSchema#dateTime">2024-07-01T17:17:33</dc:issued>
    <cc:license rdf:resource="https://www.nationalarchives.gov.uk/doc/open-government-licence/version/3/"/>
    <cc:attributionURL rdf:resource="https://historicengland.org.uk/"/>
    <cc:attributionName xml:lang="en">Historic England</cc:attributionName>
    <dc:publisher rdf:resource="https://historicengland.org.uk/"/>
    <dc:spatial rdf:resource="http://vocab.getty.edu/tgn/7002445"/>
    <dc:spatial rdf:resource="http://dbpedia.org/resource/England"/>
    <skos:prefLabel xml:lang="en">Regular Coaxial Field System</skos:prefLabel>
    <skos:scopeNote xml:lang="en">Coaxial field system in which boundaries tend towards the straight (rather than the sinuous) and so form patterns dominated by quite rectangular fields.</skos:scopeNote>
  </skos:Concept>

  <skos:Concept rdf:about="http://purl.org/heritagedata/schemes/571/concepts/151728">
    <skos:narrower rdf:resource="http://purl.org/heritagedata/schemes/571/concepts/151179"/>
    <skos:narrower>
      <skos:Concept rdf:about="http://purl.org/heritagedata/schemes/571/concepts/151180">
        <skos:broader rdf:resource="http://purl.org/heritagedata/schemes/571/concepts/151728"/>
        <skos:inScheme rdf:resource="http://purl.org/heritagedata/schemes/571"/>
        <dc:identifier>http://purl.org/heritagedata/schemes/571/concepts/151180</dc:identifier>
        <dc:issued rdf:datatype="http://www.w3.org/2001/XMLSchema#dateTime">2024-07-01T17:17:33</dc:issued>
        <cc:license rdf:resource="https://www.nationalarchives.gov.uk/doc/open-government-licence/version/3/"/>
        <cc:attributionURL rdf:resource="https://historicengland.org.uk/"/>
        <cc:attributionName xml:lang="en">Historic England</cc:attributionName>
        <dc:publisher rdf:resource="https://historicengland.org.uk/"/>
        <dc:spatial rdf:resource="http://vocab.getty.edu/tgn/7002445"/>
        <dc:spatial rdf:resource="http://dbpedia.org/resource/England"/>
        <skos:prefLabel xml:lang="en">Irregular Coaxial Field System</skos:prefLabel>
        <skos:scopeNote xml:lang="en">A coaxial field system characterised by primary boundaries that are slightly sinuous.</skos:scopeNote>
      </skos:Concept>
    </skos:narrower>

    <skos:narrower rdf:resource="http://purl.org/heritagedata/schemes/571/concepts/151181"/>
    <skos:broader rdf:resource="http://purl.org/heritagedata/schemes/571/concepts/151727"/>
    <skos:broader rdf:resource="http://purl.org/heritagedata/schemes/571/concepts/151730"/>
    <skos:inScheme rdf:resource="http://purl.org/heritagedata/schemes/571"/>
    <dc:identifier>http://purl.org/heritagedata/schemes/571/concepts/151728</dc:identifier>
    <dc:issued rdf:datatype="http://www.w3.org/2001/XMLSchema#dateTime">2024-07-01T17:17:33</dc:issued>
    <cc:license rdf:resource="https://www.nationalarchives.gov.uk/doc/open-government-licence/version/3/"/>
    <cc:attributionURL rdf:resource="https://historicengland.org.uk/"/>
    <cc:attributionName xml:lang="en">Historic England</cc:attributionName>
    <dc:publisher rdf:resource="https://historicengland.org.uk/"/>
    <dc:spatial rdf:resource="http://vocab.getty.edu/tgn/7002445"/>
    <dc:spatial rdf:resource="http://dbpedia.org/resource/England"/>
    <skos:prefLabel xml:lang="en">Coaxial Field System</skos:prefLabel>
    <skos:related rdf:resource="http://purl.org/heritagedata/schemes/571/concepts/160155"/>
    <skos:scopeNote xml:lang="en">Field system with prevailing orientation.Most boundaries are straight or nearly so and closely align with main axis or run perpendicular to it. Usually prehistoric or early medieval. Suggestive of early planned land allotment.</skos:scopeNote>
  </skos:Concept>

  <skos:Concept rdf:about="http://purl.org/heritagedata/schemes/571/concepts/151181">
    <skos:broader rdf:resource="http://purl.org/heritagedata/schemes/571/concepts/151728"/>
    <skos:inScheme rdf:resource="http://purl.org/heritagedata/schemes/571"/>
    <dc:identifier>http://purl.org/heritagedata/schemes/571/concepts/151181</dc:identifier>
    <dc:issued rdf:datatype="http://www.w3.org/2001/XMLSchema#dateTime">2024-07-01T17:17:33</dc:issued>
    <cc:license rdf:resource="https://www.nationalarchives.gov.uk/doc/open-government-licence/version/3/"/>
    <cc:attributionURL rdf:resource="https://historicengland.org.uk/"/>
    <cc:attributionName xml:lang="en">Historic England</cc:attributionName>
    <dc:publisher rdf:resource="https://historicengland.org.uk/"/>
    <dc:spatial rdf:resource="http://vocab.getty.edu/tgn/7002445"/>
    <dc:spatial rdf:resource="http://dbpedia.org/resource/England"/>
    <skos:prefLabel xml:lang="en">Dual Axis Coaxial Field System</skos:prefLabel>
    <skos:related rdf:resource="http://purl.org/heritagedata/schemes/571/concepts/160155"/>
    <skos:scopeNote xml:lang="en">A coaxial field system with two perpendicular lines of axis, forming a grid-like field pattern. Often possible to establish a more dominant axis.</skos:scopeNote>
  </skos:Concept>

  <skos:Concept rdf:about="http://purl.org/heritagedata/schemes/571/concepts/151186">
    <skos:broader rdf:resource="http://purl.org/heritagedata/schemes/571/concepts/151611"/>
    <skos:inScheme rdf:resource="http://purl.org/heritagedata/schemes/571"/>
    <dc:identifier>http://purl.org/heritagedata/schemes/571/concepts/151186</dc:identifier>
    <dc:issued rdf:datatype="http://www.w3.org/2001/XMLSchema#dateTime">2024-07-01T17:17:33</dc:issued>
    <cc:license rdf:resource="https://www.nationalarchives.gov.uk/doc/open-government-licence/version/3/"/>
    <cc:attributionURL rdf:resource="https://historicengland.org.uk/"/>
    <cc:attributionName xml:lang="en">Historic England</cc:attributionName>
    <dc:publisher rdf:resource="https://historicengland.org.uk/"/>
    <dc:spatial rdf:resource="http://vocab.getty.edu/tgn/7002445"/>
    <dc:spatial rdf:resource="http://dbpedia.org/resource/England"/>
    <skos:prefLabel xml:lang="en">Raised Bog</skos:prefLabel>
    <skos:scopeNote xml:lang="en">A bog which has developed from a lake or flat marshy area where the silt and/or peat has built up to such an extent that a shallow dome of raised peat is formed. The dome is often surrounded by strips of fen or other wetland vegetation at the edges.</skos:scopeNote>
  </skos:Concept>

  <skos:Concept rdf:about="http://purl.org/heritagedata/schemes/571/concepts/151611">
    <skos:narrower rdf:resource="http://purl.org/heritagedata/schemes/571/concepts/151186"/>
    <skos:narrower>
      <skos:Concept rdf:about="http://purl.org/heritagedata/schemes/571/concepts/151612">
        <skos:broader rdf:resource="http://purl.org/heritagedata/schemes/571/concepts/151611"/>
        <skos:inScheme rdf:resource="http://purl.org/heritagedata/schemes/571"/>
        <dc:identifier>http://purl.org/heritagedata/schemes/571/concepts/151612</dc:identifier>
        <dc:issued rdf:datatype="http://www.w3.org/2001/XMLSchema#dateTime">2024-07-01T17:17:33</dc:issued>
        <cc:license rdf:resource="https://www.nationalarchives.gov.uk/doc/open-government-licence/version/3/"/>
        <cc:attributionURL rdf:resource="https://historicengland.org.uk/"/>
        <cc:attributionName xml:lang="en">Historic England</cc:attributionName>
        <dc:publisher rdf:resource="https://historicengland.org.uk/"/>
        <dc:spatial rdf:resource="http://vocab.getty.edu/tgn/7002445"/>
        <dc:spatial rdf:resource="http://dbpedia.org/resource/England"/>
        <skos:prefLabel xml:lang="en">Blanket Bog</skos:prefLabel>
        <skos:scopeNote xml:lang="en">A bog which has developed as the result of consistent high rainfall providing conditions for the development of bog vegetation over large tracts of land, blanketing even hilltops and slopes.</skos:scopeNote>
      </skos:Concept>
    </skos:narrower>

    <skos:narrower>
      <skos:Concept rdf:about="http://purl.org/heritagedata/schemes/571/concepts/152316">
        <skos:broader rdf:resource="http://purl.org/heritagedata/schemes/571/concepts/151611"/>
        <skos:inScheme rdf:resource="http://purl.org/heritagedata/schemes/571"/>
        <dc:identifier>http://purl.org/heritagedata/schemes/571/concepts/152316</dc:identifier>
        <dc:issued rdf:datatype="http://www.w3.org/2001/XMLSchema#dateTime">2024-07-01T17:17:33</dc:issued>
        <cc:license rdf:resource="https://www.nationalarchives.gov.uk/doc/open-government-licence/version/3/"/>
        <cc:attributionURL rdf:resource="https://historicengland.org.uk/"/>
        <cc:attributionName xml:lang="en">Historic England</cc:attributionName>
        <dc:publisher rdf:resource="https://historicengland.org.uk/"/>
        <dc:spatial rdf:resource="http://vocab.getty.edu/tgn/7002445"/>
        <dc:spatial rdf:resource="http://dbpedia.org/resource/England"/>
        <skos:prefLabel xml:lang="en">Valley Bog</skos:prefLabel>
        <skos:scopeNote xml:lang="en">A bog that develops in gently sloping valleys upon a peat layer. Valley bogs may develop in relatively dry and warm climates, but because they rely on ground or surface water, they only occur on acidic substrates.</skos:scopeNote>
      </skos:Concept>
    </skos:narrower>

    <skos:broader rdf:resource="http://purl.org/heritagedata/schemes/571/concepts/151250"/>
    <skos:inScheme rdf:resource="http://purl.org/heritagedata/schemes/571"/>
    <dc:identifier>http://purl.org/heritagedata/schemes/571/concepts/151611</dc:identifier>
    <dc:issued rdf:datatype="http://www.w3.org/2001/XMLSchema#dateTime">2024-07-01T17:17:33</dc:issued>
    <cc:license rdf:resource="https://www.nationalarchives.gov.uk/doc/open-government-licence/version/3/"/>
    <cc:attributionURL rdf:resource="https://historicengland.org.uk/"/>
    <cc:attributionName xml:lang="en">Historic England</cc:attributionName>
    <dc:publisher rdf:resource="https://historicengland.org.uk/"/>
    <dc:spatial rdf:resource="http://vocab.getty.edu/tgn/7002445"/>
    <dc:spatial rdf:resource="http://dbpedia.org/resource/England"/>
    <skos:prefLabel xml:lang="en">Bog</skos:prefLabel>
    <skos:related rdf:resource="http://purl.org/heritagedata/schemes/571/concepts/152593"/>
    <skos:scopeNote xml:lang="en">A wetland type that accumulates acidic peat. Sometimes named 'moss'.</skos:scopeNote>
  </skos:Concept>

  <skos:Concept rdf:about="http://purl.org/heritagedata/schemes/571/concepts/151189">
    <skos:broader rdf:resource="http://purl.org/heritagedata/schemes/571/concepts/151462"/>
    <skos:narrower>
      <skos:Concept rdf:about="http://purl.org/heritagedata/schemes/571/concepts/151190">
        <skos:broader rdf:resource="http://purl.org/heritagedata/schemes/571/concepts/151189"/>
        <skos:inScheme rdf:resource="http://purl.org/heritagedata/schemes/571"/>
        <dc:identifier>http://purl.org/heritagedata/schemes/571/concepts/151190</dc:identifier>
        <dc:issued rdf:datatype="http://www.w3.org/2001/XMLSchema#dateTime">2024-07-01T17:17:33</dc:issued>
        <cc:license rdf:resource="https://www.nationalarchives.gov.uk/doc/open-government-licence/version/3/"/>
        <cc:attributionURL rdf:resource="https://historicengland.org.uk/"/>
        <cc:attributionName xml:lang="en">Historic England</cc:attributionName>
        <dc:publisher rdf:resource="https://historicengland.org.uk/"/>
        <dc:spatial rdf:resource="http://vocab.getty.edu/tgn/7002445"/>
        <dc:spatial rdf:resource="http://dbpedia.org/resource/England"/>
        <skos:prefLabel xml:lang="en">Cementstone Quarry</skos:prefLabel>
        <skos:scopeNote xml:lang="en">A site where cementstone nodules are extracted.</skos:scopeNote>
      </skos:Concept>
    </skos:narrower>

    <skos:narrower>
      <skos:Concept rdf:about="http://purl.org/heritagedata/schemes/571/concepts/151191">
        <skos:broader rdf:resource="http://purl.org/heritagedata/schemes/571/concepts/151189"/>
        <skos:inScheme rdf:resource="http://purl.org/heritagedata/schemes/571"/>
        <dc:identifier>http://purl.org/heritagedata/schemes/571/concepts/151191</dc:identifier>
        <dc:issued rdf:datatype="http://www.w3.org/2001/XMLSchema#dateTime">2024-07-01T17:17:33</dc:issued>
        <cc:license rdf:resource="https://www.nationalarchives.gov.uk/doc/open-government-licence/version/3/"/>
        <cc:attributionURL rdf:resource="https://historicengland.org.uk/"/>
        <cc:attributionName xml:lang="en">Historic England</cc:attributionName>
        <dc:publisher rdf:resource="https://historicengland.org.uk/"/>
        <dc:spatial rdf:resource="http://vocab.getty.edu/tgn/7002445"/>
        <dc:spatial rdf:resource="http://dbpedia.org/resource/England"/>
        <skos:prefLabel xml:lang="en">Granite Quarry</skos:prefLabel>
        <skos:scopeNote xml:lang="en">A place from which granite is excavated.</skos:scopeNote>
      </skos:Concept>
    </skos:narrower>

    <skos:narrower>
      <skos:Concept rdf:about="http://purl.org/heritagedata/schemes/571/concepts/151192">
        <skos:broader rdf:resource="http://purl.org/heritagedata/schemes/571/concepts/151189"/>
        <skos:inScheme rdf:resource="http://purl.org/heritagedata/schemes/571"/>
        <dc:identifier>http://purl.org/heritagedata/schemes/571/concepts/151192</dc:identifier>
        <dc:issued rdf:datatype="http://www.w3.org/2001/XMLSchema#dateTime">2024-07-01T17:17:33</dc:issued>
        <cc:license rdf:resource="https://www.nationalarchives.gov.uk/doc/open-government-licence/version/3/"/>
        <cc:attributionURL rdf:resource="https://historicengland.org.uk/"/>
        <cc:attributionName xml:lang="en">Historic England</cc:attributionName>
        <dc:publisher rdf:resource="https://historicengland.org.uk/"/>
        <dc:spatial rdf:resource="http://vocab.getty.edu/tgn/7002445"/>
        <dc:spatial rdf:resource="http://dbpedia.org/resource/England"/>
        <skos:prefLabel xml:lang="en">Gypsum Quarry</skos:prefLabel>
        <skos:scopeNote xml:lang="en">A place from which gypsum is excavated.</skos:scopeNote>
      </skos:Concept>
    </skos:narrower>

    <skos:narrower>
      <skos:Concept rdf:about="http://purl.org/heritagedata/schemes/571/concepts/151193">
        <skos:broader rdf:resource="http://purl.org/heritagedata/schemes/571/concepts/151189"/>
        <skos:inScheme rdf:resource="http://purl.org/heritagedata/schemes/571"/>
        <dc:identifier>http://purl.org/heritagedata/schemes/571/concepts/151193</dc:identifier>
        <dc:issued rdf:datatype="http://www.w3.org/2001/XMLSchema#dateTime">2024-07-01T17:17:33</dc:issued>
        <cc:license rdf:resource="https://www.nationalarchives.gov.uk/doc/open-government-licence/version/3/"/>
        <cc:attributionURL rdf:resource="https://historicengland.org.uk/"/>
        <cc:attributionName xml:lang="en">Historic England</cc:attributionName>
        <dc:publisher rdf:resource="https://historicengland.org.uk/"/>
        <dc:spatial rdf:resource="http://vocab.getty.edu/tgn/7002445"/>
        <dc:spatial rdf:resource="http://dbpedia.org/resource/England"/>
        <skos:prefLabel xml:lang="en">Limestone Quarry</skos:prefLabel>
        <skos:scopeNote xml:lang="en">A place from which limestone is extracted. Includes closely associated spoil, processing, and transport facilities.</skos:scopeNote>
      </skos:Concept>
    </skos:narrower>

    <skos:narrower>
      <skos:Concept rdf:about="http://purl.org/heritagedata/schemes/571/concepts/151194">
        <skos:broader rdf:resource="http://purl.org/heritagedata/schemes/571/concepts/151189"/>
        <skos:inScheme rdf:resource="http://purl.org/heritagedata/schemes/571"/>
        <dc:identifier>http://purl.org/heritagedata/schemes/571/concepts/151194</dc:identifier>
        <dc:issued rdf:datatype="http://www.w3.org/2001/XMLSchema#dateTime">2024-07-01T17:17:33</dc:issued>
        <cc:license rdf:resource="https://www.nationalarchives.gov.uk/doc/open-government-licence/version/3/"/>
        <cc:attributionURL rdf:resource="https://historicengland.org.uk/"/>
        <cc:attributionName xml:lang="en">Historic England</cc:attributionName>
        <dc:publisher rdf:resource="https://historicengland.org.uk/"/>
        <dc:spatial rdf:resource="http://vocab.getty.edu/tgn/7002445"/>
        <dc:spatial rdf:resource="http://dbpedia.org/resource/England"/>
        <skos:prefLabel xml:lang="en">Marble Quarry</skos:prefLabel>
        <skos:scopeNote xml:lang="en">A site where marble is extracted from the ground.</skos:scopeNote>
      </skos:Concept>
    </skos:narrower>

    <skos:narrower>
      <skos:Concept rdf:about="http://purl.org/heritagedata/schemes/571/concepts/151196">
        <skos:broader rdf:resource="http://purl.org/heritagedata/schemes/571/concepts/151189"/>
        <skos:inScheme rdf:resource="http://purl.org/heritagedata/schemes/571"/>
        <dc:identifier>http://purl.org/heritagedata/schemes/571/concepts/151196</dc:identifier>
        <dc:issued rdf:datatype="http://www.w3.org/2001/XMLSchema#dateTime">2024-07-01T17:17:33</dc:issued>
        <cc:license rdf:resource="https://www.nationalarchives.gov.uk/doc/open-government-licence/version/3/"/>
        <cc:attributionURL rdf:resource="https://historicengland.org.uk/"/>
        <cc:attributionName xml:lang="en">Historic England</cc:attributionName>
        <dc:publisher rdf:resource="https://historicengland.org.uk/"/>
        <dc:spatial rdf:resource="http://vocab.getty.edu/tgn/7002445"/>
        <dc:spatial rdf:resource="http://dbpedia.org/resource/England"/>
        <skos:prefLabel xml:lang="en">Sandstone Quarry</skos:prefLabel>
        <skos:scopeNote xml:lang="en">A place from which sandstone is excavated.</skos:scopeNote>
      </skos:Concept>
    </skos:narrower>

    <skos:narrower>
      <skos:Concept rdf:about="http://purl.org/heritagedata/schemes/571/concepts/151197">
        <skos:broader rdf:resource="http://purl.org/heritagedata/schemes/571/concepts/151189"/>
        <skos:inScheme rdf:resource="http://purl.org/heritagedata/schemes/571"/>
        <dc:identifier>http://purl.org/heritagedata/schemes/571/concepts/151197</dc:identifier>
        <dc:issued rdf:datatype="http://www.w3.org/2001/XMLSchema#dateTime">2024-07-01T17:17:33</dc:issued>
        <cc:license rdf:resource="https://www.nationalarchives.gov.uk/doc/open-government-licence/version/3/"/>
        <cc:attributionURL rdf:resource="https://historicengland.org.uk/"/>
        <cc:attributionName xml:lang="en">Historic England</cc:attributionName>
        <dc:publisher rdf:resource="https://historicengland.org.uk/"/>
        <dc:spatial rdf:resource="http://vocab.getty.edu/tgn/7002445"/>
        <dc:spatial rdf:resource="http://dbpedia.org/resource/England"/>
        <skos:prefLabel xml:lang="en">Shale Quarry</skos:prefLabel>
        <skos:scopeNote xml:lang="en">A place from which shale, a laminated clay or silt which has been compressed by the weight of the rocks over it, is extracted from the ground.</skos:scopeNote>
      </skos:Concept>
    </skos:narrower>

    <skos:narrower>
      <skos:Concept rdf:about="http://purl.org/heritagedata/schemes/571/concepts/151198">
        <skos:broader rdf:resource="http://purl.org/heritagedata/schemes/571/concepts/151189"/>
        <skos:inScheme rdf:resource="http://purl.org/heritagedata/schemes/571"/>
        <dc:identifier>http://purl.org/heritagedata/schemes/571/concepts/151198</dc:identifier>
        <dc:issued rdf:datatype="http://www.w3.org/2001/XMLSchema#dateTime">2024-07-01T17:17:33</dc:issued>
        <cc:license rdf:resource="https://www.nationalarchives.gov.uk/doc/open-government-licence/version/3/"/>
        <cc:attributionURL rdf:resource="https://historicengland.org.uk/"/>
        <cc:attributionName xml:lang="en">Historic England</cc:attributionName>
        <dc:publisher rdf:resource="https://historicengland.org.uk/"/>
        <dc:spatial rdf:resource="http://vocab.getty.edu/tgn/7002445"/>
        <dc:spatial rdf:resource="http://dbpedia.org/resource/England"/>
        <skos:prefLabel xml:lang="en">Slate Quarry</skos:prefLabel>
        <skos:scopeNote xml:lang="en">A place from which slate is quarried from the ground.</skos:scopeNote>
      </skos:Concept>
    </skos:narrower>

    <skos:inScheme rdf:resource="http://purl.org/heritagedata/schemes/571"/>
    <dc:identifier>http://purl.org/heritagedata/schemes/571/concepts/151189</dc:identifier>
    <dc:issued rdf:datatype="http://www.w3.org/2001/XMLSchema#dateTime">2024-07-01T17:17:33</dc:issued>
    <cc:license rdf:resource="https://www.nationalarchives.gov.uk/doc/open-government-licence/version/3/"/>
    <cc:attributionURL rdf:resource="https://historicengland.org.uk/"/>
    <cc:attributionName xml:lang="en">Historic England</cc:attributionName>
    <dc:publisher rdf:resource="https://historicengland.org.uk/"/>
    <dc:spatial rdf:resource="http://vocab.getty.edu/tgn/7002445"/>
    <dc:spatial rdf:resource="http://dbpedia.org/resource/England"/>
    <skos:prefLabel xml:lang="en">Stone Quarry</skos:prefLabel>
    <skos:scopeNote xml:lang="en">An excavation from which stone for building, hardcore, hedging etc is obtained by cutting, blasting, hoisting, crushing, dressing etc.</skos:scopeNote>
  </skos:Concept>

  <skos:Concept rdf:about="http://purl.org/heritagedata/schemes/571/concepts/151462">
    <skos:narrower rdf:resource="http://purl.org/heritagedata/schemes/571/concepts/151189"/>
    <skos:narrower rdf:resource="http://purl.org/heritagedata/schemes/571/concepts/151419"/>
    <skos:broader rdf:resource="http://purl.org/heritagedata/schemes/571/concepts/151461"/>
    <skos:inScheme rdf:resource="http://purl.org/heritagedata/schemes/571"/>
    <dc:identifier>http://purl.org/heritagedata/schemes/571/concepts/151462</dc:identifier>
    <dc:issued rdf:datatype="http://www.w3.org/2001/XMLSchema#dateTime">2024-07-01T17:17:33</dc:issued>
    <cc:license rdf:resource="https://www.nationalarchives.gov.uk/doc/open-government-licence/version/3/"/>
    <cc:attributionURL rdf:resource="https://historicengland.org.uk/"/>
    <cc:attributionName xml:lang="en">Historic England</cc:attributionName>
    <dc:publisher rdf:resource="https://historicengland.org.uk/"/>
    <dc:spatial rdf:resource="http://vocab.getty.edu/tgn/7002445"/>
    <dc:spatial rdf:resource="http://dbpedia.org/resource/England"/>
    <skos:prefLabel xml:lang="en">Quarry</skos:prefLabel>
    <skos:related rdf:resource="http://purl.org/heritagedata/schemes/571/concepts/151743"/>
    <skos:scopeNote xml:lang="en">An excavation on land from which stone or aggregates are extracted for use primarily building and civil engineering.</skos:scopeNote>
  </skos:Concept>

  <skos:Concept rdf:about="http://purl.org/heritagedata/schemes/571/concepts/151199">
    <skos:broader rdf:resource="http://purl.org/heritagedata/schemes/571/concepts/151422"/>
    <skos:inScheme rdf:resource="http://purl.org/heritagedata/schemes/571"/>
    <dc:identifier>http://purl.org/heritagedata/schemes/571/concepts/151199</dc:identifier>
    <dc:issued rdf:datatype="http://www.w3.org/2001/XMLSchema#dateTime">2024-07-01T17:17:33</dc:issued>
    <cc:license rdf:resource="https://www.nationalarchives.gov.uk/doc/open-government-licence/version/3/"/>
    <cc:attributionURL rdf:resource="https://historicengland.org.uk/"/>
    <cc:attributionName xml:lang="en">Historic England</cc:attributionName>
    <dc:publisher rdf:resource="https://historicengland.org.uk/"/>
    <dc:spatial rdf:resource="http://vocab.getty.edu/tgn/7002445"/>
    <dc:spatial rdf:resource="http://dbpedia.org/resource/England"/>
    <skos:prefLabel xml:lang="en">Colliery</skos:prefLabel>
    <skos:related rdf:resource="http://purl.org/heritagedata/schemes/571/concepts/151436"/>
    <skos:scopeNote xml:lang="en">A place where coal is mined. Includes closely associated spoil, processing and transport facilities.</skos:scopeNote>
  </skos:Concept>

  <skos:Concept rdf:about="http://purl.org/heritagedata/schemes/571/concepts/151422">
    <skos:narrower rdf:resource="http://purl.org/heritagedata/schemes/571/concepts/151199"/>
    <skos:narrower rdf:resource="http://purl.org/heritagedata/schemes/571/concepts/151202"/>
    <skos:narrower>
      <skos:Concept rdf:about="http://purl.org/heritagedata/schemes/571/concepts/151423">
        <skos:broader rdf:resource="http://purl.org/heritagedata/schemes/571/concepts/151422"/>
        <skos:inScheme rdf:resource="http://purl.org/heritagedata/schemes/571"/>
        <dc:identifier>http://purl.org/heritagedata/schemes/571/concepts/151423</dc:identifier>
        <dc:issued rdf:datatype="http://www.w3.org/2001/XMLSchema#dateTime">2024-07-01T17:17:33</dc:issued>
        <cc:license rdf:resource="https://www.nationalarchives.gov.uk/doc/open-government-licence/version/3/"/>
        <cc:attributionURL rdf:resource="https://historicengland.org.uk/"/>
        <cc:attributionName xml:lang="en">Historic England</cc:attributionName>
        <dc:publisher rdf:resource="https://historicengland.org.uk/"/>
        <dc:spatial rdf:resource="http://vocab.getty.edu/tgn/7002445"/>
        <dc:spatial rdf:resource="http://dbpedia.org/resource/England"/>
        <skos:prefLabel xml:lang="en">Cobalt Mine</skos:prefLabel>
        <skos:scopeNote xml:lang="en">A site where cobalt is mined. Includes closely associated spoil, processing and transport facilities.</skos:scopeNote>
      </skos:Concept>
    </skos:narrower>

    <skos:narrower>
      <skos:Concept rdf:about="http://purl.org/heritagedata/schemes/571/concepts/151424">
        <skos:broader rdf:resource="http://purl.org/heritagedata/schemes/571/concepts/151422"/>
        <skos:inScheme rdf:resource="http://purl.org/heritagedata/schemes/571"/>
        <dc:identifier>http://purl.org/heritagedata/schemes/571/concepts/151424</dc:identifier>
        <dc:issued rdf:datatype="http://www.w3.org/2001/XMLSchema#dateTime">2024-07-01T17:17:33</dc:issued>
        <cc:license rdf:resource="https://www.nationalarchives.gov.uk/doc/open-government-licence/version/3/"/>
        <cc:attributionURL rdf:resource="https://historicengland.org.uk/"/>
        <cc:attributionName xml:lang="en">Historic England</cc:attributionName>
        <dc:publisher rdf:resource="https://historicengland.org.uk/"/>
        <dc:spatial rdf:resource="http://vocab.getty.edu/tgn/7002445"/>
        <dc:spatial rdf:resource="http://dbpedia.org/resource/England"/>
        <skos:prefLabel xml:lang="en">Copper Mine</skos:prefLabel>
        <skos:scopeNote xml:lang="en">A site where copper is mined. Includes closely associated spoil, processing and transport facilities. Also use MINE plus other relevant ore name as appropriate.</skos:scopeNote>
      </skos:Concept>
    </skos:narrower>

    <skos:narrower>
      <skos:Concept rdf:about="http://purl.org/heritagedata/schemes/571/concepts/151425">
        <skos:broader rdf:resource="http://purl.org/heritagedata/schemes/571/concepts/151422"/>
        <skos:inScheme rdf:resource="http://purl.org/heritagedata/schemes/571"/>
        <dc:identifier>http://purl.org/heritagedata/schemes/571/concepts/151425</dc:identifier>
        <dc:issued rdf:datatype="http://www.w3.org/2001/XMLSchema#dateTime">2024-07-01T17:17:33</dc:issued>
        <cc:license rdf:resource="https://www.nationalarchives.gov.uk/doc/open-government-licence/version/3/"/>
        <cc:attributionURL rdf:resource="https://historicengland.org.uk/"/>
        <cc:attributionName xml:lang="en">Historic England</cc:attributionName>
        <dc:publisher rdf:resource="https://historicengland.org.uk/"/>
        <dc:spatial rdf:resource="http://vocab.getty.edu/tgn/7002445"/>
        <dc:spatial rdf:resource="http://dbpedia.org/resource/England"/>
        <skos:prefLabel xml:lang="en">Ironstone Mine</skos:prefLabel>
        <skos:scopeNote xml:lang="en">A place from which iron ore is mined. Includes closely associated spoil, processing, and transport facilities.</skos:scopeNote>
      </skos:Concept>
    </skos:narrower>

    <skos:narrower>
      <skos:Concept rdf:about="http://purl.org/heritagedata/schemes/571/concepts/151426">
        <skos:broader rdf:resource="http://purl.org/heritagedata/schemes/571/concepts/151422"/>
        <skos:inScheme rdf:resource="http://purl.org/heritagedata/schemes/571"/>
        <dc:identifier>http://purl.org/heritagedata/schemes/571/concepts/151426</dc:identifier>
        <dc:issued rdf:datatype="http://www.w3.org/2001/XMLSchema#dateTime">2024-07-01T17:17:33</dc:issued>
        <cc:license rdf:resource="https://www.nationalarchives.gov.uk/doc/open-government-licence/version/3/"/>
        <cc:attributionURL rdf:resource="https://historicengland.org.uk/"/>
        <cc:attributionName xml:lang="en">Historic England</cc:attributionName>
        <dc:publisher rdf:resource="https://historicengland.org.uk/"/>
        <dc:spatial rdf:resource="http://vocab.getty.edu/tgn/7002445"/>
        <dc:spatial rdf:resource="http://dbpedia.org/resource/England"/>
        <skos:prefLabel xml:lang="en">Lead Mine</skos:prefLabel>
        <skos:scopeNote xml:lang="en">A place from which lead ore is mined. Includes closely associated spoil, processing, and transport facilities. Also use MINE and other ores extracted where relevant, eg. SILVER MINE.</skos:scopeNote>
      </skos:Concept>
    </skos:narrower>

    <skos:narrower>
      <skos:Concept rdf:about="http://purl.org/heritagedata/schemes/571/concepts/151427">
        <skos:broader rdf:resource="http://purl.org/heritagedata/schemes/571/concepts/151422"/>
        <skos:inScheme rdf:resource="http://purl.org/heritagedata/schemes/571"/>
        <dc:identifier>http://purl.org/heritagedata/schemes/571/concepts/151427</dc:identifier>
        <dc:issued rdf:datatype="http://www.w3.org/2001/XMLSchema#dateTime">2024-07-01T17:17:33</dc:issued>
        <cc:license rdf:resource="https://www.nationalarchives.gov.uk/doc/open-government-licence/version/3/"/>
        <cc:attributionURL rdf:resource="https://historicengland.org.uk/"/>
        <cc:attributionName xml:lang="en">Historic England</cc:attributionName>
        <dc:publisher rdf:resource="https://historicengland.org.uk/"/>
        <dc:spatial rdf:resource="http://vocab.getty.edu/tgn/7002445"/>
        <dc:spatial rdf:resource="http://dbpedia.org/resource/England"/>
        <skos:prefLabel xml:lang="en">Manganese Mine</skos:prefLabel>
        <skos:scopeNote xml:lang="en">A place from which manganese ore is extracted. Includes closely associated spoil, processing, and transport facilities. Use with other ores extracted and MINE where relevant.</skos:scopeNote>
      </skos:Concept>
    </skos:narrower>

    <skos:narrower>
      <skos:Concept rdf:about="http://purl.org/heritagedata/schemes/571/concepts/151429">
        <skos:broader rdf:resource="http://purl.org/heritagedata/schemes/571/concepts/151422"/>
        <skos:inScheme rdf:resource="http://purl.org/heritagedata/schemes/571"/>
        <dc:identifier>http://purl.org/heritagedata/schemes/571/concepts/151429</dc:identifier>
        <dc:issued rdf:datatype="http://www.w3.org/2001/XMLSchema#dateTime">2024-07-01T17:17:33</dc:issued>
        <cc:license rdf:resource="https://www.nationalarchives.gov.uk/doc/open-government-licence/version/3/"/>
        <cc:attributionURL rdf:resource="https://historicengland.org.uk/"/>
        <cc:attributionName xml:lang="en">Historic England</cc:attributionName>
        <dc:publisher rdf:resource="https://historicengland.org.uk/"/>
        <dc:spatial rdf:resource="http://vocab.getty.edu/tgn/7002445"/>
        <dc:spatial rdf:resource="http://dbpedia.org/resource/England"/>
        <skos:prefLabel xml:lang="en">Nickel Mine</skos:prefLabel>
        <skos:scopeNote xml:lang="en">A place where nickel ore is extracted. Also use with other metal ores extracted and MINE where relevant.</skos:scopeNote>
      </skos:Concept>
    </skos:narrower>

    <skos:narrower>
      <skos:Concept rdf:about="http://purl.org/heritagedata/schemes/571/concepts/151430">
        <skos:broader rdf:resource="http://purl.org/heritagedata/schemes/571/concepts/151422"/>
        <skos:inScheme rdf:resource="http://purl.org/heritagedata/schemes/571"/>
        <dc:identifier>http://purl.org/heritagedata/schemes/571/concepts/151430</dc:identifier>
        <dc:issued rdf:datatype="http://www.w3.org/2001/XMLSchema#dateTime">2024-07-01T17:17:33</dc:issued>
        <cc:license rdf:resource="https://www.nationalarchives.gov.uk/doc/open-government-licence/version/3/"/>
        <cc:attributionURL rdf:resource="https://historicengland.org.uk/"/>
        <cc:attributionName xml:lang="en">Historic England</cc:attributionName>
        <dc:publisher rdf:resource="https://historicengland.org.uk/"/>
        <dc:spatial rdf:resource="http://vocab.getty.edu/tgn/7002445"/>
        <dc:spatial rdf:resource="http://dbpedia.org/resource/England"/>
        <skos:prefLabel xml:lang="en">Silver Mine</skos:prefLabel>
        <skos:scopeNote xml:lang="en">A place where silver is extracted. Use with other minerals extracted and MINE where relevant, eg. LEAD MINE.</skos:scopeNote>
      </skos:Concept>
    </skos:narrower>

    <skos:narrower>
      <skos:Concept rdf:about="http://purl.org/heritagedata/schemes/571/concepts/151431">
        <skos:broader rdf:resource="http://purl.org/heritagedata/schemes/571/concepts/151422"/>
        <skos:inScheme rdf:resource="http://purl.org/heritagedata/schemes/571"/>
        <dc:identifier>http://purl.org/heritagedata/schemes/571/concepts/151431</dc:identifier>
        <dc:issued rdf:datatype="http://www.w3.org/2001/XMLSchema#dateTime">2024-07-01T17:17:33</dc:issued>
        <cc:license rdf:resource="https://www.nationalarchives.gov.uk/doc/open-government-licence/version/3/"/>
        <cc:attributionURL rdf:resource="https://historicengland.org.uk/"/>
        <cc:attributionName xml:lang="en">Historic England</cc:attributionName>
        <dc:publisher rdf:resource="https://historicengland.org.uk/"/>
        <dc:spatial rdf:resource="http://vocab.getty.edu/tgn/7002445"/>
        <dc:spatial rdf:resource="http://dbpedia.org/resource/England"/>
        <skos:prefLabel xml:lang="en">Gold Mine</skos:prefLabel>
        <skos:scopeNote xml:lang="en">A place from which gold is extracted. Includes closely associated spoil, processing, and transport facilities.</skos:scopeNote>
      </skos:Concept>
    </skos:narrower>

    <skos:narrower>
      <skos:Concept rdf:about="http://purl.org/heritagedata/schemes/571/concepts/151432">
        <skos:broader rdf:resource="http://purl.org/heritagedata/schemes/571/concepts/151422"/>
        <skos:inScheme rdf:resource="http://purl.org/heritagedata/schemes/571"/>
        <dc:identifier>http://purl.org/heritagedata/schemes/571/concepts/151432</dc:identifier>
        <dc:issued rdf:datatype="http://www.w3.org/2001/XMLSchema#dateTime">2024-07-01T17:17:33</dc:issued>
        <cc:license rdf:resource="https://www.nationalarchives.gov.uk/doc/open-government-licence/version/3/"/>
        <cc:attributionURL rdf:resource="https://historicengland.org.uk/"/>
        <cc:attributionName xml:lang="en">Historic England</cc:attributionName>
        <dc:publisher rdf:resource="https://historicengland.org.uk/"/>
        <dc:spatial rdf:resource="http://vocab.getty.edu/tgn/7002445"/>
        <dc:spatial rdf:resource="http://dbpedia.org/resource/England"/>
        <skos:prefLabel xml:lang="en">Tin Mine</skos:prefLabel>
        <skos:scopeNote xml:lang="en">A mine used for the extraction of tin bearing ore.</skos:scopeNote>
      </skos:Concept>
    </skos:narrower>

    <skos:narrower>
      <skos:Concept rdf:about="http://purl.org/heritagedata/schemes/571/concepts/151433">
        <skos:broader rdf:resource="http://purl.org/heritagedata/schemes/571/concepts/151422"/>
        <skos:inScheme rdf:resource="http://purl.org/heritagedata/schemes/571"/>
        <dc:identifier>http://purl.org/heritagedata/schemes/571/concepts/151433</dc:identifier>
        <dc:issued rdf:datatype="http://www.w3.org/2001/XMLSchema#dateTime">2024-07-01T17:17:33</dc:issued>
        <cc:license rdf:resource="https://www.nationalarchives.gov.uk/doc/open-government-licence/version/3/"/>
        <cc:attributionURL rdf:resource="https://historicengland.org.uk/"/>
        <cc:attributionName xml:lang="en">Historic England</cc:attributionName>
        <dc:publisher rdf:resource="https://historicengland.org.uk/"/>
        <dc:spatial rdf:resource="http://vocab.getty.edu/tgn/7002445"/>
        <dc:spatial rdf:resource="http://dbpedia.org/resource/England"/>
        <skos:prefLabel xml:lang="en">Tungsten Mine</skos:prefLabel>
        <skos:scopeNote xml:lang="en">A mine used for the extraction of tungsten-bearing ore. Use with other mineral ores extracted and MINE, eg. TIN MINE.</skos:scopeNote>
      </skos:Concept>
    </skos:narrower>

    <skos:narrower>
      <skos:Concept rdf:about="http://purl.org/heritagedata/schemes/571/concepts/151435">
        <skos:broader rdf:resource="http://purl.org/heritagedata/schemes/571/concepts/151422"/>
        <skos:inScheme rdf:resource="http://purl.org/heritagedata/schemes/571"/>
        <dc:identifier>http://purl.org/heritagedata/schemes/571/concepts/151435</dc:identifier>
        <dc:issued rdf:datatype="http://www.w3.org/2001/XMLSchema#dateTime">2024-07-01T17:17:33</dc:issued>
        <cc:license rdf:resource="https://www.nationalarchives.gov.uk/doc/open-government-licence/version/3/"/>
        <cc:attributionURL rdf:resource="https://historicengland.org.uk/"/>
        <cc:attributionName xml:lang="en">Historic England</cc:attributionName>
        <dc:publisher rdf:resource="https://historicengland.org.uk/"/>
        <dc:spatial rdf:resource="http://vocab.getty.edu/tgn/7002445"/>
        <dc:spatial rdf:resource="http://dbpedia.org/resource/England"/>
        <skos:prefLabel xml:lang="en">Zinc Mine</skos:prefLabel>
        <skos:scopeNote xml:lang="en">A mine used for the extraction of zinc-bearing ore. Use with other metal ores extracted and MINE where necessary, eg. LEAD MINE.</skos:scopeNote>
      </skos:Concept>
    </skos:narrower>

    <skos:narrower rdf:resource="http://purl.org/heritagedata/schemes/571/concepts/151736"/>
    <skos:broader rdf:resource="http://purl.org/heritagedata/schemes/571/concepts/151461"/>
    <skos:inScheme rdf:resource="http://purl.org/heritagedata/schemes/571"/>
    <dc:identifier>http://purl.org/heritagedata/schemes/571/concepts/151422</dc:identifier>
    <dc:issued rdf:datatype="http://www.w3.org/2001/XMLSchema#dateTime">2024-07-01T17:17:33</dc:issued>
    <cc:license rdf:resource="https://www.nationalarchives.gov.uk/doc/open-government-licence/version/3/"/>
    <cc:attributionURL rdf:resource="https://historicengland.org.uk/"/>
    <cc:attributionName xml:lang="en">Historic England</cc:attributionName>
    <dc:publisher rdf:resource="https://historicengland.org.uk/"/>
    <dc:spatial rdf:resource="http://vocab.getty.edu/tgn/7002445"/>
    <dc:spatial rdf:resource="http://dbpedia.org/resource/England"/>
    <skos:prefLabel xml:lang="en">Mine</skos:prefLabel>
    <skos:related rdf:resource="http://purl.org/heritagedata/schemes/571/concepts/151436"/>
    <skos:related rdf:resource="http://purl.org/heritagedata/schemes/571/concepts/151744"/>
    <skos:scopeNote xml:lang="en">An excavation made in the earth for the purpose of digging out metallic ores, coal, salt, or precious stones etc. Use specific type where known.</skos:scopeNote>
  </skos:Concept>

  <skos:Concept rdf:about="http://purl.org/heritagedata/schemes/571/concepts/151200">
    <skos:broader rdf:resource="http://purl.org/heritagedata/schemes/571/concepts/160170"/>
    <skos:inScheme rdf:resource="http://purl.org/heritagedata/schemes/571"/>
    <dc:identifier>http://purl.org/heritagedata/schemes/571/concepts/151200</dc:identifier>
    <dc:issued rdf:datatype="http://www.w3.org/2001/XMLSchema#dateTime">2024-07-01T17:17:33</dc:issued>
    <cc:license rdf:resource="https://www.nationalarchives.gov.uk/doc/open-government-licence/version/3/"/>
    <cc:attributionURL rdf:resource="https://historicengland.org.uk/"/>
    <cc:attributionName xml:lang="en">Historic England</cc:attributionName>
    <dc:publisher rdf:resource="https://historicengland.org.uk/"/>
    <dc:spatial rdf:resource="http://vocab.getty.edu/tgn/7002445"/>
    <dc:spatial rdf:resource="http://dbpedia.org/resource/England"/>
    <skos:prefLabel xml:lang="en">Brickworks</skos:prefLabel>
    <skos:scopeNote xml:lang="en">An industrial manufacturing complex producing bricks.</skos:scopeNote>
  </skos:Concept>

  <skos:Concept rdf:about="http://purl.org/heritagedata/schemes/571/concepts/160170">
    <skos:narrower rdf:resource="http://purl.org/heritagedata/schemes/571/concepts/151200"/>
    <skos:narrower rdf:resource="http://purl.org/heritagedata/schemes/571/concepts/151226"/>
    <skos:narrower>
      <skos:Concept rdf:about="http://purl.org/heritagedata/schemes/571/concepts/151626">
        <skos:broader rdf:resource="http://purl.org/heritagedata/schemes/571/concepts/160170"/>
        <skos:inScheme rdf:resource="http://purl.org/heritagedata/schemes/571"/>
        <dc:identifier>http://purl.org/heritagedata/schemes/571/concepts/151626</dc:identifier>
        <dc:issued rdf:datatype="http://www.w3.org/2001/XMLSchema#dateTime">2024-07-01T17:17:33</dc:issued>
        <cc:license rdf:resource="https://www.nationalarchives.gov.uk/doc/open-government-licence/version/3/"/>
        <cc:attributionURL rdf:resource="https://historicengland.org.uk/"/>
        <cc:attributionName xml:lang="en">Historic England</cc:attributionName>
        <dc:publisher rdf:resource="https://historicengland.org.uk/"/>
        <dc:spatial rdf:resource="http://vocab.getty.edu/tgn/7002445"/>
        <dc:spatial rdf:resource="http://dbpedia.org/resource/England"/>
        <skos:prefLabel xml:lang="en">Ice Works</skos:prefLabel>
        <skos:scopeNote xml:lang="en">A factory or plant for the manufacture of ice using mechanised refrigeration techniques.</skos:scopeNote>
      </skos:Concept>
    </skos:narrower>

    <skos:narrower>
      <skos:Concept rdf:about="http://purl.org/heritagedata/schemes/571/concepts/152627">
        <skos:broader rdf:resource="http://purl.org/heritagedata/schemes/571/concepts/160170"/>
        <skos:inScheme rdf:resource="http://purl.org/heritagedata/schemes/571"/>
        <dc:identifier>http://purl.org/heritagedata/schemes/571/concepts/152627</dc:identifier>
        <dc:issued rdf:datatype="http://www.w3.org/2001/XMLSchema#dateTime">2024-07-01T17:17:33</dc:issued>
        <cc:license rdf:resource="https://www.nationalarchives.gov.uk/doc/open-government-licence/version/3/"/>
        <cc:attributionURL rdf:resource="https://historicengland.org.uk/"/>
        <cc:attributionName xml:lang="en">Historic England</cc:attributionName>
        <dc:publisher rdf:resource="https://historicengland.org.uk/"/>
        <dc:spatial rdf:resource="http://vocab.getty.edu/tgn/7002445"/>
        <dc:spatial rdf:resource="http://dbpedia.org/resource/England"/>
        <skos:prefLabel xml:lang="en">Steel Works</skos:prefLabel>
        <skos:scopeNote xml:lang="en">An industrial complex for large-scale production of steel in the 19th and 20th centuries.</skos:scopeNote>
      </skos:Concept>
    </skos:narrower>

    <skos:broader rdf:resource="http://purl.org/heritagedata/schemes/571/concepts/151457"/>
    <skos:inScheme rdf:resource="http://purl.org/heritagedata/schemes/571"/>
    <dc:identifier>http://purl.org/heritagedata/schemes/571/concepts/160170</dc:identifier>
    <dc:issued rdf:datatype="http://www.w3.org/2001/XMLSchema#dateTime">2024-07-01T17:17:33</dc:issued>
    <cc:license rdf:resource="https://www.nationalarchives.gov.uk/doc/open-government-licence/version/3/"/>
    <cc:attributionURL rdf:resource="https://historicengland.org.uk/"/>
    <cc:attributionName xml:lang="en">Historic England</cc:attributionName>
    <dc:publisher rdf:resource="https://historicengland.org.uk/"/>
    <dc:spatial rdf:resource="http://vocab.getty.edu/tgn/7002445"/>
    <dc:spatial rdf:resource="http://dbpedia.org/resource/England"/>
    <skos:prefLabel xml:lang="en">Manufacturing Industry</skos:prefLabel>
    <skos:scopeNote xml:lang="en">Production of secondary materials through various processes; distinguished from PROCESSING INDUSTRYs preparation of primary materials.</skos:scopeNote>
  </skos:Concept>

  <skos:Concept rdf:about="http://purl.org/heritagedata/schemes/571/concepts/151201">
    <skos:broader rdf:resource="http://purl.org/heritagedata/schemes/571/concepts/151743"/>
    <skos:inScheme rdf:resource="http://purl.org/heritagedata/schemes/571"/>
    <dc:identifier>http://purl.org/heritagedata/schemes/571/concepts/151201</dc:identifier>
    <dc:issued rdf:datatype="http://www.w3.org/2001/XMLSchema#dateTime">2024-07-01T17:17:33</dc:issued>
    <cc:license rdf:resource="https://www.nationalarchives.gov.uk/doc/open-government-licence/version/3/"/>
    <cc:attributionURL rdf:resource="https://historicengland.org.uk/"/>
    <cc:attributionName xml:lang="en">Historic England</cc:attributionName>
    <dc:publisher rdf:resource="https://historicengland.org.uk/"/>
    <dc:spatial rdf:resource="http://vocab.getty.edu/tgn/7002445"/>
    <dc:spatial rdf:resource="http://dbpedia.org/resource/England"/>
    <skos:prefLabel xml:lang="en">Marl Pit</skos:prefLabel>
    <skos:scopeNote xml:lang="en">A pit from which marl, a mixture of clay and carbonate of lime, is excavated. Marl is used as a fertilizer.</skos:scopeNote>
  </skos:Concept>

  <skos:Concept rdf:about="http://purl.org/heritagedata/schemes/571/concepts/151743">
    <skos:narrower rdf:resource="http://purl.org/heritagedata/schemes/571/concepts/151201"/>
    <skos:narrower>
      <skos:Concept rdf:about="http://purl.org/heritagedata/schemes/571/concepts/151745">
        <skos:broader rdf:resource="http://purl.org/heritagedata/schemes/571/concepts/151743"/>
        <skos:inScheme rdf:resource="http://purl.org/heritagedata/schemes/571"/>
        <dc:identifier>http://purl.org/heritagedata/schemes/571/concepts/151745</dc:identifier>
        <dc:issued rdf:datatype="http://www.w3.org/2001/XMLSchema#dateTime">2024-07-01T17:17:33</dc:issued>
        <cc:license rdf:resource="https://www.nationalarchives.gov.uk/doc/open-government-licence/version/3/"/>
        <cc:attributionURL rdf:resource="https://historicengland.org.uk/"/>
        <cc:attributionName xml:lang="en">Historic England</cc:attributionName>
        <dc:publisher rdf:resource="https://historicengland.org.uk/"/>
        <dc:spatial rdf:resource="http://vocab.getty.edu/tgn/7002445"/>
        <dc:spatial rdf:resource="http://dbpedia.org/resource/England"/>
        <skos:prefLabel xml:lang="en">Flooded Pit</skos:prefLabel>
        <skos:scopeNote xml:lang="en">Abandoned and/or derelict surface workings such as shallow shafts, lode workings, open-pit methods and quarrying that have subsequently become flooded with water.</skos:scopeNote>
      </skos:Concept>
    </skos:narrower>

    <skos:broader rdf:resource="http://purl.org/heritagedata/schemes/571/concepts/151461"/>
    <skos:inScheme rdf:resource="http://purl.org/heritagedata/schemes/571"/>
    <dc:identifier>http://purl.org/heritagedata/schemes/571/concepts/151743</dc:identifier>
    <dc:issued rdf:datatype="http://www.w3.org/2001/XMLSchema#dateTime">2024-07-01T17:17:33</dc:issued>
    <cc:license rdf:resource="https://www.nationalarchives.gov.uk/doc/open-government-licence/version/3/"/>
    <cc:attributionURL rdf:resource="https://historicengland.org.uk/"/>
    <cc:attributionName xml:lang="en">Historic England</cc:attributionName>
    <dc:publisher rdf:resource="https://historicengland.org.uk/"/>
    <dc:spatial rdf:resource="http://vocab.getty.edu/tgn/7002445"/>
    <dc:spatial rdf:resource="http://dbpedia.org/resource/England"/>
    <skos:prefLabel xml:lang="en">Extractive Pit</skos:prefLabel>
    <skos:related rdf:resource="http://purl.org/heritagedata/schemes/571/concepts/151202"/>
    <skos:related rdf:resource="http://purl.org/heritagedata/schemes/571/concepts/151205"/>
    <skos:related rdf:resource="http://purl.org/heritagedata/schemes/571/concepts/151462"/>
    <skos:scopeNote xml:lang="en">Surface workings including shallow shafts, lode workings, open-pit methods and quarrying including some mines of stone, clays, compounds, etc.</skos:scopeNote>
  </skos:Concept>

  <skos:Concept rdf:about="http://purl.org/heritagedata/schemes/571/concepts/151202">
    <skos:broader rdf:resource="http://purl.org/heritagedata/schemes/571/concepts/151422"/>
    <skos:inScheme rdf:resource="http://purl.org/heritagedata/schemes/571"/>
    <dc:identifier>http://purl.org/heritagedata/schemes/571/concepts/151202</dc:identifier>
    <dc:issued rdf:datatype="http://www.w3.org/2001/XMLSchema#dateTime">2024-07-01T17:17:33</dc:issued>
    <cc:license rdf:resource="https://www.nationalarchives.gov.uk/doc/open-government-licence/version/3/"/>
    <cc:attributionURL rdf:resource="https://historicengland.org.uk/"/>
    <cc:attributionName xml:lang="en">Historic England</cc:attributionName>
    <dc:publisher rdf:resource="https://historicengland.org.uk/"/>
    <dc:spatial rdf:resource="http://vocab.getty.edu/tgn/7002445"/>
    <dc:spatial rdf:resource="http://dbpedia.org/resource/England"/>
    <skos:prefLabel xml:lang="en">Open Cast Mine</skos:prefLabel>
    <skos:related rdf:resource="http://purl.org/heritagedata/schemes/571/concepts/151743"/>
    <skos:scopeNote xml:lang="en">An excavation open to the sky, caused by the extraction of coal, stone or similar. Use with product type where known.</skos:scopeNote>
  </skos:Concept>

  <skos:Concept rdf:about="http://purl.org/heritagedata/schemes/571/concepts/151203">
    <skos:broader rdf:resource="http://purl.org/heritagedata/schemes/571/concepts/151737"/>
    <skos:inScheme rdf:resource="http://purl.org/heritagedata/schemes/571"/>
    <dc:identifier>http://purl.org/heritagedata/schemes/571/concepts/151203</dc:identifier>
    <dc:issued rdf:datatype="http://www.w3.org/2001/XMLSchema#dateTime">2024-07-01T17:17:33</dc:issued>
    <cc:license rdf:resource="https://www.nationalarchives.gov.uk/doc/open-government-licence/version/3/"/>
    <cc:attributionURL rdf:resource="https://historicengland.org.uk/"/>
    <cc:attributionName xml:lang="en">Historic England</cc:attributionName>
    <dc:publisher rdf:resource="https://historicengland.org.uk/"/>
    <dc:spatial rdf:resource="http://vocab.getty.edu/tgn/7002445"/>
    <dc:spatial rdf:resource="http://dbpedia.org/resource/England"/>
    <skos:prefLabel xml:lang="en">Oil Refinery</skos:prefLabel>
    <skos:scopeNote xml:lang="en">A works where crude oil is distilled into its fractions or cuts.</skos:scopeNote>
  </skos:Concept>

  <skos:Concept rdf:about="http://purl.org/heritagedata/schemes/571/concepts/151737">
    <skos:narrower rdf:resource="http://purl.org/heritagedata/schemes/571/concepts/151203"/>
    <skos:narrower>
      <skos:Concept rdf:about="http://purl.org/heritagedata/schemes/571/concepts/151437">
        <skos:broader rdf:resource="http://purl.org/heritagedata/schemes/571/concepts/151737"/>
        <skos:inScheme rdf:resource="http://purl.org/heritagedata/schemes/571"/>
        <dc:identifier>http://purl.org/heritagedata/schemes/571/concepts/151437</dc:identifier>
        <dc:issued rdf:datatype="http://www.w3.org/2001/XMLSchema#dateTime">2024-07-01T17:17:33</dc:issued>
        <cc:license rdf:resource="https://www.nationalarchives.gov.uk/doc/open-government-licence/version/3/"/>
        <cc:attributionURL rdf:resource="https://historicengland.org.uk/"/>
        <cc:attributionName xml:lang="en">Historic England</cc:attributionName>
        <dc:publisher rdf:resource="https://historicengland.org.uk/"/>
        <dc:spatial rdf:resource="http://vocab.getty.edu/tgn/7002445"/>
        <dc:spatial rdf:resource="http://dbpedia.org/resource/England"/>
        <skos:prefLabel xml:lang="en">Oil Rig</skos:prefLabel>
        <skos:scopeNote xml:lang="en">A supporting structure for drilling machinery used in the extraction of, or prospecting for, mineral oils.</skos:scopeNote>
      </skos:Concept>
    </skos:narrower>

    <skos:broader rdf:resource="http://purl.org/heritagedata/schemes/571/concepts/151461"/>
    <skos:broader rdf:resource="http://purl.org/heritagedata/schemes/571/concepts/152605"/>
    <skos:inScheme rdf:resource="http://purl.org/heritagedata/schemes/571"/>
    <dc:identifier>http://purl.org/heritagedata/schemes/571/concepts/151737</dc:identifier>
    <dc:issued rdf:datatype="http://www.w3.org/2001/XMLSchema#dateTime">2024-07-01T17:17:33</dc:issued>
    <cc:license rdf:resource="https://www.nationalarchives.gov.uk/doc/open-government-licence/version/3/"/>
    <cc:attributionURL rdf:resource="https://historicengland.org.uk/"/>
    <cc:attributionName xml:lang="en">Historic England</cc:attributionName>
    <dc:publisher rdf:resource="https://historicengland.org.uk/"/>
    <dc:spatial rdf:resource="http://vocab.getty.edu/tgn/7002445"/>
    <dc:spatial rdf:resource="http://dbpedia.org/resource/England"/>
    <skos:prefLabel xml:lang="en">Oil Works</skos:prefLabel>
    <skos:related rdf:resource="http://purl.org/heritagedata/schemes/571/concepts/151137"/>
    <skos:scopeNote xml:lang="en">Buildings, sites and structures associated with the retrieval, refining, processing and storage of petroleum oil.</skos:scopeNote>
  </skos:Concept>

  <skos:Concept rdf:about="http://purl.org/heritagedata/schemes/571/concepts/151204">
    <skos:broader rdf:resource="http://purl.org/heritagedata/schemes/571/concepts/152605"/>
    <skos:narrower rdf:resource="http://purl.org/heritagedata/schemes/571/concepts/152628"/>
    <skos:inScheme rdf:resource="http://purl.org/heritagedata/schemes/571"/>
    <dc:identifier>http://purl.org/heritagedata/schemes/571/concepts/151204</dc:identifier>
    <dc:issued rdf:datatype="http://www.w3.org/2001/XMLSchema#dateTime">2024-07-01T17:17:33</dc:issued>
    <cc:license rdf:resource="https://www.nationalarchives.gov.uk/doc/open-government-licence/version/3/"/>
    <cc:attributionURL rdf:resource="https://historicengland.org.uk/"/>
    <cc:attributionName xml:lang="en">Historic England</cc:attributionName>
    <dc:publisher rdf:resource="https://historicengland.org.uk/"/>
    <dc:spatial rdf:resource="http://vocab.getty.edu/tgn/7002445"/>
    <dc:spatial rdf:resource="http://dbpedia.org/resource/England"/>
    <skos:prefLabel xml:lang="en">Pipeline</skos:prefLabel>
    <skos:scopeNote xml:lang="en">A conduit or pipes, used primarily for conveying liquid or gas such as petroleum from oil wells to a refinery, or for supplying water to a town or district, etc.</skos:scopeNote>
  </skos:Concept>

  <skos:Concept rdf:about="http://purl.org/heritagedata/schemes/571/concepts/152605">
    <skos:narrower rdf:resource="http://purl.org/heritagedata/schemes/571/concepts/151204"/>
    <skos:narrower rdf:resource="http://purl.org/heritagedata/schemes/571/concepts/151572"/>
    <skos:narrower rdf:resource="http://purl.org/heritagedata/schemes/571/concepts/151737"/>
    <skos:narrower rdf:resource="http://purl.org/heritagedata/schemes/571/concepts/151746"/>
    <skos:narrower rdf:resource="http://purl.org/heritagedata/schemes/571/concepts/152620"/>
    <skos:narrower rdf:resource="http://purl.org/heritagedata/schemes/571/concepts/152621"/>
    <skos:narrower>
      <skos:Concept rdf:about="http://purl.org/heritagedata/schemes/571/concepts/152625">
        <skos:broader rdf:resource="http://purl.org/heritagedata/schemes/571/concepts/152605"/>
        <skos:inScheme rdf:resource="http://purl.org/heritagedata/schemes/571"/>
        <dc:identifier>http://purl.org/heritagedata/schemes/571/concepts/152625</dc:identifier>
        <dc:issued rdf:datatype="http://www.w3.org/2001/XMLSchema#dateTime">2024-07-01T17:17:33</dc:issued>
        <cc:license rdf:resource="https://www.nationalarchives.gov.uk/doc/open-government-licence/version/3/"/>
        <cc:attributionURL rdf:resource="https://historicengland.org.uk/"/>
        <cc:attributionName xml:lang="en">Historic England</cc:attributionName>
        <dc:publisher rdf:resource="https://historicengland.org.uk/"/>
        <dc:spatial rdf:resource="http://vocab.getty.edu/tgn/7002445"/>
        <dc:spatial rdf:resource="http://dbpedia.org/resource/England"/>
        <skos:prefLabel xml:lang="en">Nuclear Reprocessing</skos:prefLabel>
        <skos:scopeNote xml:lang="en">Industrial area for the decommissioning of structures associated with the nuclear industry, reprocessing of nuclear materials, nuclear waste management and/or nuclear fuel manufacturing activities take place.</skos:scopeNote>
      </skos:Concept>
    </skos:narrower>

    <skos:broader rdf:resource="http://purl.org/heritagedata/schemes/571/concepts/151457"/>
    <skos:inScheme rdf:resource="http://purl.org/heritagedata/schemes/571"/>
    <dc:identifier>http://purl.org/heritagedata/schemes/571/concepts/152605</dc:identifier>
    <dc:issued rdf:datatype="http://www.w3.org/2001/XMLSchema#dateTime">2024-07-01T17:17:33</dc:issued>
    <cc:license rdf:resource="https://www.nationalarchives.gov.uk/doc/open-government-licence/version/3/"/>
    <cc:attributionURL rdf:resource="https://historicengland.org.uk/"/>
    <cc:attributionName xml:lang="en">Historic England</cc:attributionName>
    <dc:publisher rdf:resource="https://historicengland.org.uk/"/>
    <dc:spatial rdf:resource="http://vocab.getty.edu/tgn/7002445"/>
    <dc:spatial rdf:resource="http://dbpedia.org/resource/England"/>
    <skos:prefLabel xml:lang="en">Energy Industry</skos:prefLabel>
    <skos:scopeNote xml:lang="en">-</skos:scopeNote>
  </skos:Concept>

  <skos:Concept rdf:about="http://purl.org/heritagedata/schemes/571/concepts/151205">
    <skos:broader rdf:resource="http://purl.org/heritagedata/schemes/571/concepts/151569"/>
    <skos:narrower>
      <skos:Concept rdf:about="http://purl.org/heritagedata/schemes/571/concepts/151206">
        <skos:broader rdf:resource="http://purl.org/heritagedata/schemes/571/concepts/151205"/>
        <skos:inScheme rdf:resource="http://purl.org/heritagedata/schemes/571"/>
        <dc:identifier>http://purl.org/heritagedata/schemes/571/concepts/151206</dc:identifier>
        <dc:issued rdf:datatype="http://www.w3.org/2001/XMLSchema#dateTime">2024-07-01T17:17:33</dc:issued>
        <cc:license rdf:resource="https://www.nationalarchives.gov.uk/doc/open-government-licence/version/3/"/>
        <cc:attributionURL rdf:resource="https://historicengland.org.uk/"/>
        <cc:attributionName xml:lang="en">Historic England</cc:attributionName>
        <dc:publisher rdf:resource="https://historicengland.org.uk/"/>
        <dc:spatial rdf:resource="http://vocab.getty.edu/tgn/7002445"/>
        <dc:spatial rdf:resource="http://dbpedia.org/resource/England"/>
        <skos:prefLabel xml:lang="en">Brickearth Pit</skos:prefLabel>
        <skos:scopeNote xml:lang="en">A pit and its associated features used for the excavation of clay suitable for making bricks.</skos:scopeNote>
      </skos:Concept>
    </skos:narrower>

    <skos:inScheme rdf:resource="http://purl.org/heritagedata/schemes/571"/>
    <dc:identifier>http://purl.org/heritagedata/schemes/571/concepts/151205</dc:identifier>
    <dc:issued rdf:datatype="http://www.w3.org/2001/XMLSchema#dateTime">2024-07-01T17:17:33</dc:issued>
    <cc:license rdf:resource="https://www.nationalarchives.gov.uk/doc/open-government-licence/version/3/"/>
    <cc:attributionURL rdf:resource="https://historicengland.org.uk/"/>
    <cc:attributionName xml:lang="en">Historic England</cc:attributionName>
    <dc:publisher rdf:resource="https://historicengland.org.uk/"/>
    <dc:spatial rdf:resource="http://vocab.getty.edu/tgn/7002445"/>
    <dc:spatial rdf:resource="http://dbpedia.org/resource/England"/>
    <skos:prefLabel xml:lang="en">Clay Pit</skos:prefLabel>
    <skos:related rdf:resource="http://purl.org/heritagedata/schemes/571/concepts/151743"/>
    <skos:scopeNote xml:lang="en">A place from which clay is extracted.</skos:scopeNote>
  </skos:Concept>

  <skos:Concept rdf:about="http://purl.org/heritagedata/schemes/571/concepts/151569">
    <skos:narrower rdf:resource="http://purl.org/heritagedata/schemes/571/concepts/151205"/>
    <skos:narrower rdf:resource="http://purl.org/heritagedata/schemes/571/concepts/151571"/>
    <skos:broader rdf:resource="http://purl.org/heritagedata/schemes/571/concepts/151461"/>
    <skos:inScheme rdf:resource="http://purl.org/heritagedata/schemes/571"/>
    <dc:identifier>http://purl.org/heritagedata/schemes/571/concepts/151569</dc:identifier>
    <dc:issued rdf:datatype="http://www.w3.org/2001/XMLSchema#dateTime">2024-07-01T17:17:33</dc:issued>
    <cc:license rdf:resource="https://www.nationalarchives.gov.uk/doc/open-government-licence/version/3/"/>
    <cc:attributionURL rdf:resource="https://historicengland.org.uk/"/>
    <cc:attributionName xml:lang="en">Historic England</cc:attributionName>
    <dc:publisher rdf:resource="https://historicengland.org.uk/"/>
    <dc:spatial rdf:resource="http://vocab.getty.edu/tgn/7002445"/>
    <dc:spatial rdf:resource="http://dbpedia.org/resource/England"/>
    <skos:prefLabel xml:lang="en">Clay Extraction Site</skos:prefLabel>
    <skos:scopeNote xml:lang="en">Buildings, sites and structures associated with the extraction of clay.</skos:scopeNote>
  </skos:Concept>

  <skos:Concept rdf:about="http://purl.org/heritagedata/schemes/571/concepts/151207">
    <skos:broader rdf:resource="http://purl.org/heritagedata/schemes/571/concepts/151572"/>
    <skos:narrower>
      <skos:Concept rdf:about="http://purl.org/heritagedata/schemes/571/concepts/151208">
        <skos:broader rdf:resource="http://purl.org/heritagedata/schemes/571/concepts/151207"/>
        <skos:inScheme rdf:resource="http://purl.org/heritagedata/schemes/571"/>
        <dc:identifier>http://purl.org/heritagedata/schemes/571/concepts/151208</dc:identifier>
        <dc:issued rdf:datatype="http://www.w3.org/2001/XMLSchema#dateTime">2024-07-01T17:17:33</dc:issued>
        <cc:license rdf:resource="https://www.nationalarchives.gov.uk/doc/open-government-licence/version/3/"/>
        <cc:attributionURL rdf:resource="https://historicengland.org.uk/"/>
        <cc:attributionName xml:lang="en">Historic England</cc:attributionName>
        <dc:publisher rdf:resource="https://historicengland.org.uk/"/>
        <dc:spatial rdf:resource="http://vocab.getty.edu/tgn/7002445"/>
        <dc:spatial rdf:resource="http://dbpedia.org/resource/England"/>
        <skos:prefLabel xml:lang="en">Coal Fired Power Station</skos:prefLabel>
        <skos:scopeNote xml:lang="en">A coal-burning power station where domestic electricity for an area is produced, eg. Drax Power Station near the Humber Estuary.</skos:scopeNote>
      </skos:Concept>
    </skos:narrower>

    <skos:narrower>
      <skos:Concept rdf:about="http://purl.org/heritagedata/schemes/571/concepts/151209">
        <skos:broader rdf:resource="http://purl.org/heritagedata/schemes/571/concepts/151207"/>
        <skos:inScheme rdf:resource="http://purl.org/heritagedata/schemes/571"/>
        <dc:identifier>http://purl.org/heritagedata/schemes/571/concepts/151209</dc:identifier>
        <dc:issued rdf:datatype="http://www.w3.org/2001/XMLSchema#dateTime">2024-07-01T17:17:33</dc:issued>
        <cc:license rdf:resource="https://www.nationalarchives.gov.uk/doc/open-government-licence/version/3/"/>
        <cc:attributionURL rdf:resource="https://historicengland.org.uk/"/>
        <cc:attributionName xml:lang="en">Historic England</cc:attributionName>
        <dc:publisher rdf:resource="https://historicengland.org.uk/"/>
        <dc:spatial rdf:resource="http://vocab.getty.edu/tgn/7002445"/>
        <dc:spatial rdf:resource="http://dbpedia.org/resource/England"/>
        <skos:prefLabel xml:lang="en">Gas Fired Power Station</skos:prefLabel>
        <skos:scopeNote xml:lang="en">A power station used to produce electricity, fired by coal gas.</skos:scopeNote>
      </skos:Concept>
    </skos:narrower>

    <skos:narrower>
      <skos:Concept rdf:about="http://purl.org/heritagedata/schemes/571/concepts/151211">
        <skos:broader rdf:resource="http://purl.org/heritagedata/schemes/571/concepts/151207"/>
        <skos:inScheme rdf:resource="http://purl.org/heritagedata/schemes/571"/>
        <dc:identifier>http://purl.org/heritagedata/schemes/571/concepts/151211</dc:identifier>
        <dc:issued rdf:datatype="http://www.w3.org/2001/XMLSchema#dateTime">2024-07-01T17:17:33</dc:issued>
        <cc:license rdf:resource="https://www.nationalarchives.gov.uk/doc/open-government-licence/version/3/"/>
        <cc:attributionURL rdf:resource="https://historicengland.org.uk/"/>
        <cc:attributionName xml:lang="en">Historic England</cc:attributionName>
        <dc:publisher rdf:resource="https://historicengland.org.uk/"/>
        <dc:spatial rdf:resource="http://vocab.getty.edu/tgn/7002445"/>
        <dc:spatial rdf:resource="http://dbpedia.org/resource/England"/>
        <skos:prefLabel xml:lang="en">Nuclear Power Station</skos:prefLabel>
        <skos:scopeNote xml:lang="en">A complex of buildings producing power derived from nuclear energy.</skos:scopeNote>
      </skos:Concept>
    </skos:narrower>

    <skos:narrower>
      <skos:Concept rdf:about="http://purl.org/heritagedata/schemes/571/concepts/151212">
        <skos:broader rdf:resource="http://purl.org/heritagedata/schemes/571/concepts/151207"/>
        <skos:inScheme rdf:resource="http://purl.org/heritagedata/schemes/571"/>
        <dc:identifier>http://purl.org/heritagedata/schemes/571/concepts/151212</dc:identifier>
        <dc:issued rdf:datatype="http://www.w3.org/2001/XMLSchema#dateTime">2024-07-01T17:17:33</dc:issued>
        <cc:license rdf:resource="https://www.nationalarchives.gov.uk/doc/open-government-licence/version/3/"/>
        <cc:attributionURL rdf:resource="https://historicengland.org.uk/"/>
        <cc:attributionName xml:lang="en">Historic England</cc:attributionName>
        <dc:publisher rdf:resource="https://historicengland.org.uk/"/>
        <dc:spatial rdf:resource="http://vocab.getty.edu/tgn/7002445"/>
        <dc:spatial rdf:resource="http://dbpedia.org/resource/England"/>
        <skos:prefLabel xml:lang="en">Oil Fired Power Station</skos:prefLabel>
        <skos:scopeNote xml:lang="en">An electricity-producing power station fired by oil.</skos:scopeNote>
      </skos:Concept>
    </skos:narrower>

    <skos:narrower rdf:resource="http://purl.org/heritagedata/schemes/571/concepts/151573"/>
    <skos:inScheme rdf:resource="http://purl.org/heritagedata/schemes/571"/>
    <dc:identifier>http://purl.org/heritagedata/schemes/571/concepts/151207</dc:identifier>
    <dc:issued rdf:datatype="http://www.w3.org/2001/XMLSchema#dateTime">2024-07-01T17:17:33</dc:issued>
    <cc:license rdf:resource="https://www.nationalarchives.gov.uk/doc/open-government-licence/version/3/"/>
    <cc:attributionURL rdf:resource="https://historicengland.org.uk/"/>
    <cc:attributionName xml:lang="en">Historic England</cc:attributionName>
    <dc:publisher rdf:resource="https://historicengland.org.uk/"/>
    <dc:spatial rdf:resource="http://vocab.getty.edu/tgn/7002445"/>
    <dc:spatial rdf:resource="http://dbpedia.org/resource/England"/>
    <skos:prefLabel xml:lang="en">Power Station</skos:prefLabel>
    <skos:scopeNote xml:lang="en">A building or set of buildings and structures where power, especially electrical or mechanical, is generated. Use more specific type where known.</skos:scopeNote>
  </skos:Concept>

  <skos:Concept rdf:about="http://purl.org/heritagedata/schemes/571/concepts/151572">
    <skos:narrower rdf:resource="http://purl.org/heritagedata/schemes/571/concepts/151207"/>
    <skos:broader rdf:resource="http://purl.org/heritagedata/schemes/571/concepts/152605"/>
    <skos:inScheme rdf:resource="http://purl.org/heritagedata/schemes/571"/>
    <dc:identifier>http://purl.org/heritagedata/schemes/571/concepts/151572</dc:identifier>
    <dc:issued rdf:datatype="http://www.w3.org/2001/XMLSchema#dateTime">2024-07-01T17:17:33</dc:issued>
    <cc:license rdf:resource="https://www.nationalarchives.gov.uk/doc/open-government-licence/version/3/"/>
    <cc:attributionURL rdf:resource="https://historicengland.org.uk/"/>
    <cc:attributionName xml:lang="en">Historic England</cc:attributionName>
    <dc:publisher rdf:resource="https://historicengland.org.uk/"/>
    <dc:spatial rdf:resource="http://vocab.getty.edu/tgn/7002445"/>
    <dc:spatial rdf:resource="http://dbpedia.org/resource/England"/>
    <skos:prefLabel xml:lang="en">Electricity Generation</skos:prefLabel>
    <skos:scopeNote xml:lang="en">Buildings, sites and structures associated with the generation of electricity.</skos:scopeNote>
  </skos:Concept>

  <skos:Concept rdf:about="http://purl.org/heritagedata/schemes/571/concepts/151210">
    <skos:broader rdf:resource="http://purl.org/heritagedata/schemes/571/concepts/151573"/>
    <skos:inScheme rdf:resource="http://purl.org/heritagedata/schemes/571"/>
    <dc:identifier>http://purl.org/heritagedata/schemes/571/concepts/151210</dc:identifier>
    <dc:issued rdf:datatype="http://www.w3.org/2001/XMLSchema#dateTime">2024-07-01T17:17:33</dc:issued>
    <cc:license rdf:resource="https://www.nationalarchives.gov.uk/doc/open-government-licence/version/3/"/>
    <cc:attributionURL rdf:resource="https://historicengland.org.uk/"/>
    <cc:attributionName xml:lang="en">Historic England</cc:attributionName>
    <dc:publisher rdf:resource="https://historicengland.org.uk/"/>
    <dc:spatial rdf:resource="http://vocab.getty.edu/tgn/7002445"/>
    <dc:spatial rdf:resource="http://dbpedia.org/resource/England"/>
    <skos:prefLabel xml:lang="en">Hydroelectric Power Station</skos:prefLabel>
    <skos:scopeNote xml:lang="en">Power generation by releasing stored water through a turbine driving a generator.</skos:scopeNote>
  </skos:Concept>

  <skos:Concept rdf:about="http://purl.org/heritagedata/schemes/571/concepts/151573">
    <skos:narrower rdf:resource="http://purl.org/heritagedata/schemes/571/concepts/151210"/>
    <skos:narrower>
      <skos:Concept rdf:about="http://purl.org/heritagedata/schemes/571/concepts/151213">
        <skos:broader rdf:resource="http://purl.org/heritagedata/schemes/571/concepts/151573"/>
        <skos:inScheme rdf:resource="http://purl.org/heritagedata/schemes/571"/>
        <dc:identifier>http://purl.org/heritagedata/schemes/571/concepts/151213</dc:identifier>
        <dc:issued rdf:datatype="http://www.w3.org/2001/XMLSchema#dateTime">2024-07-01T17:17:33</dc:issued>
        <cc:license rdf:resource="https://www.nationalarchives.gov.uk/doc/open-government-licence/version/3/"/>
        <cc:attributionURL rdf:resource="https://historicengland.org.uk/"/>
        <cc:attributionName xml:lang="en">Historic England</cc:attributionName>
        <dc:publisher rdf:resource="https://historicengland.org.uk/"/>
        <dc:spatial rdf:resource="http://vocab.getty.edu/tgn/7002445"/>
        <dc:spatial rdf:resource="http://dbpedia.org/resource/England"/>
        <skos:prefLabel xml:lang="en">Wind Power</skos:prefLabel>
        <skos:scopeNote xml:lang="en">Buildings, sites and structures associated with the generation of electricity by harnessing the energy of the wind.</skos:scopeNote>
      </skos:Concept>
    </skos:narrower>

    <skos:narrower>
      <skos:Concept rdf:about="http://purl.org/heritagedata/schemes/571/concepts/151418">
        <skos:broader rdf:resource="http://purl.org/heritagedata/schemes/571/concepts/151573"/>
        <skos:inScheme rdf:resource="http://purl.org/heritagedata/schemes/571"/>
        <dc:identifier>http://purl.org/heritagedata/schemes/571/concepts/151418</dc:identifier>
        <dc:issued rdf:datatype="http://www.w3.org/2001/XMLSchema#dateTime">2024-07-01T17:17:33</dc:issued>
        <cc:license rdf:resource="https://www.nationalarchives.gov.uk/doc/open-government-licence/version/3/"/>
        <cc:attributionURL rdf:resource="https://historicengland.org.uk/"/>
        <cc:attributionName xml:lang="en">Historic England</cc:attributionName>
        <dc:publisher rdf:resource="https://historicengland.org.uk/"/>
        <dc:spatial rdf:resource="http://vocab.getty.edu/tgn/7002445"/>
        <dc:spatial rdf:resource="http://dbpedia.org/resource/England"/>
        <skos:prefLabel xml:lang="en">Tidal Power</skos:prefLabel>
        <skos:scopeNote xml:lang="en">Buildings, sites and structures associated with the generation of electricity by utilising the power of the tide.</skos:scopeNote>
      </skos:Concept>
    </skos:narrower>

    <skos:narrower>
      <skos:Concept rdf:about="http://purl.org/heritagedata/schemes/571/concepts/152543">
        <skos:broader rdf:resource="http://purl.org/heritagedata/schemes/571/concepts/151573"/>
        <skos:inScheme rdf:resource="http://purl.org/heritagedata/schemes/571"/>
        <dc:identifier>http://purl.org/heritagedata/schemes/571/concepts/152543</dc:identifier>
        <dc:issued rdf:datatype="http://www.w3.org/2001/XMLSchema#dateTime">2024-07-01T17:17:33</dc:issued>
        <cc:license rdf:resource="https://www.nationalarchives.gov.uk/doc/open-government-licence/version/3/"/>
        <cc:attributionURL rdf:resource="https://historicengland.org.uk/"/>
        <cc:attributionName xml:lang="en">Historic England</cc:attributionName>
        <dc:publisher rdf:resource="https://historicengland.org.uk/"/>
        <dc:spatial rdf:resource="http://vocab.getty.edu/tgn/7002445"/>
        <dc:spatial rdf:resource="http://dbpedia.org/resource/England"/>
        <skos:prefLabel xml:lang="en">Wave Power</skos:prefLabel>
        <skos:scopeNote xml:lang="en">Buildings, sites and structures associated with the harnessing the energy of wave power for electrical power generation.</skos:scopeNote>
      </skos:Concept>
    </skos:narrower>

    <skos:broader rdf:resource="http://purl.org/heritagedata/schemes/571/concepts/151207"/>
    <skos:inScheme rdf:resource="http://purl.org/heritagedata/schemes/571"/>
    <dc:identifier>http://purl.org/heritagedata/schemes/571/concepts/151573</dc:identifier>
    <dc:issued rdf:datatype="http://www.w3.org/2001/XMLSchema#dateTime">2024-07-01T17:17:33</dc:issued>
    <cc:license rdf:resource="https://www.nationalarchives.gov.uk/doc/open-government-licence/version/3/"/>
    <cc:attributionURL rdf:resource="https://historicengland.org.uk/"/>
    <cc:attributionName xml:lang="en">Historic England</cc:attributionName>
    <dc:publisher rdf:resource="https://historicengland.org.uk/"/>
    <dc:spatial rdf:resource="http://vocab.getty.edu/tgn/7002445"/>
    <dc:spatial rdf:resource="http://dbpedia.org/resource/England"/>
    <skos:prefLabel xml:lang="en">Renewable Energy Installation</skos:prefLabel>
    <skos:scopeNote xml:lang="en">Structures where electrical energy is generated by conversion from continually replenished energy flows in the natural environment, such as sunlight, wind, rain, tides, waves, etc.</skos:scopeNote>
  </skos:Concept>

  <skos:Concept rdf:about="http://purl.org/heritagedata/schemes/571/concepts/151224">
    <skos:broader rdf:resource="http://purl.org/heritagedata/schemes/571/concepts/151749"/>
    <skos:inScheme rdf:resource="http://purl.org/heritagedata/schemes/571"/>
    <dc:identifier>http://purl.org/heritagedata/schemes/571/concepts/151224</dc:identifier>
    <dc:issued rdf:datatype="http://www.w3.org/2001/XMLSchema#dateTime">2024-07-01T17:17:33</dc:issued>
    <cc:license rdf:resource="https://www.nationalarchives.gov.uk/doc/open-government-licence/version/3/"/>
    <cc:attributionURL rdf:resource="https://historicengland.org.uk/"/>
    <cc:attributionName xml:lang="en">Historic England</cc:attributionName>
    <dc:publisher rdf:resource="https://historicengland.org.uk/"/>
    <dc:spatial rdf:resource="http://vocab.getty.edu/tgn/7002445"/>
    <dc:spatial rdf:resource="http://dbpedia.org/resource/England"/>
    <skos:prefLabel xml:lang="en">Timber Yard</skos:prefLabel>
    <skos:scopeNote xml:lang="en">An open yard or place where timber is stacked or stored.</skos:scopeNote>
  </skos:Concept>

  <skos:Concept rdf:about="http://purl.org/heritagedata/schemes/571/concepts/151749">
    <skos:narrower rdf:resource="http://purl.org/heritagedata/schemes/571/concepts/151224"/>
    <skos:broader rdf:resource="http://purl.org/heritagedata/schemes/571/concepts/152624"/>
    <skos:inScheme rdf:resource="http://purl.org/heritagedata/schemes/571"/>
    <dc:identifier>http://purl.org/heritagedata/schemes/571/concepts/151749</dc:identifier>
    <dc:issued rdf:datatype="http://www.w3.org/2001/XMLSchema#dateTime">2024-07-01T17:17:33</dc:issued>
    <cc:license rdf:resource="https://www.nationalarchives.gov.uk/doc/open-government-licence/version/3/"/>
    <cc:attributionURL rdf:resource="https://historicengland.org.uk/"/>
    <cc:attributionName xml:lang="en">Historic England</cc:attributionName>
    <dc:publisher rdf:resource="https://historicengland.org.uk/"/>
    <dc:spatial rdf:resource="http://vocab.getty.edu/tgn/7002445"/>
    <dc:spatial rdf:resource="http://dbpedia.org/resource/England"/>
    <skos:prefLabel xml:lang="en">Timber Processing</skos:prefLabel>
    <skos:scopeNote xml:lang="en">Buildings, sites and structures associated with the processing of timber.</skos:scopeNote>
  </skos:Concept>

  <skos:Concept rdf:about="http://purl.org/heritagedata/schemes/571/concepts/151225">
    <skos:broader rdf:resource="http://purl.org/heritagedata/schemes/571/concepts/151457"/>
    <skos:inScheme rdf:resource="http://purl.org/heritagedata/schemes/571"/>
    <dc:identifier>http://purl.org/heritagedata/schemes/571/concepts/151225</dc:identifier>
    <dc:issued rdf:datatype="http://www.w3.org/2001/XMLSchema#dateTime">2024-07-01T17:17:33</dc:issued>
    <cc:license rdf:resource="https://www.nationalarchives.gov.uk/doc/open-government-licence/version/3/"/>
    <cc:attributionURL rdf:resource="https://historicengland.org.uk/"/>
    <cc:attributionName xml:lang="en">Historic England</cc:attributionName>
    <dc:publisher rdf:resource="https://historicengland.org.uk/"/>
    <dc:spatial rdf:resource="http://vocab.getty.edu/tgn/7002445"/>
    <dc:spatial rdf:resource="http://dbpedia.org/resource/England"/>
    <skos:prefLabel xml:lang="en">Industrial Estate</skos:prefLabel>
    <skos:scopeNote xml:lang="en">An area of land owned by a developer, whether a private entrepreneur or a public authority, and divided into plots for leasing or sale to manufacturing or commercial concerns which may share some common services.</skos:scopeNote>
  </skos:Concept>

  <skos:Concept rdf:about="http://purl.org/heritagedata/schemes/571/concepts/151457">
    <skos:narrower rdf:resource="http://purl.org/heritagedata/schemes/571/concepts/151225"/>
    <skos:narrower rdf:resource="http://purl.org/heritagedata/schemes/571/concepts/151461"/>
    <skos:narrower rdf:resource="http://purl.org/heritagedata/schemes/571/concepts/152605"/>
    <skos:narrower rdf:resource="http://purl.org/heritagedata/schemes/571/concepts/152624"/>
    <skos:narrower rdf:resource="http://purl.org/heritagedata/schemes/571/concepts/152638"/>
    <skos:narrower rdf:resource="http://purl.org/heritagedata/schemes/571/concepts/160170"/>
    <skos:inScheme rdf:resource="http://purl.org/heritagedata/schemes/571"/>
    <dc:identifier>http://purl.org/heritagedata/schemes/571/concepts/151457</dc:identifier>
    <dc:issued rdf:datatype="http://www.w3.org/2001/XMLSchema#dateTime">2024-07-01T17:17:33</dc:issued>
    <cc:license rdf:resource="https://www.nationalarchives.gov.uk/doc/open-government-licence/version/3/"/>
    <cc:attributionURL rdf:resource="https://historicengland.org.uk/"/>
    <cc:attributionName xml:lang="en">Historic England</cc:attributionName>
    <dc:publisher rdf:resource="https://historicengland.org.uk/"/>
    <dc:spatial rdf:resource="http://vocab.getty.edu/tgn/7002445"/>
    <dc:spatial rdf:resource="http://dbpedia.org/resource/England"/>
    <skos:prefLabel xml:lang="en">Industry</skos:prefLabel>
    <skos:scopeNote xml:lang="en">-</skos:scopeNote>
    <skos:topConceptOf rdf:resource="http://purl.org/heritagedata/schemes/571"/>
  </skos:Concept>

  <skos:Concept rdf:about="http://purl.org/heritagedata/schemes/571/concepts/151226">
    <skos:broader rdf:resource="http://purl.org/heritagedata/schemes/571/concepts/160170"/>
    <skos:narrower>
      <skos:Concept rdf:about="http://purl.org/heritagedata/schemes/571/concepts/151575">
        <skos:broader rdf:resource="http://purl.org/heritagedata/schemes/571/concepts/151226"/>
        <skos:inScheme rdf:resource="http://purl.org/heritagedata/schemes/571"/>
        <dc:identifier>http://purl.org/heritagedata/schemes/571/concepts/151575</dc:identifier>
        <dc:issued rdf:datatype="http://www.w3.org/2001/XMLSchema#dateTime">2024-07-01T17:17:33</dc:issued>
        <cc:license rdf:resource="https://www.nationalarchives.gov.uk/doc/open-government-licence/version/3/"/>
        <cc:attributionURL rdf:resource="https://historicengland.org.uk/"/>
        <cc:attributionName xml:lang="en">Historic England</cc:attributionName>
        <dc:publisher rdf:resource="https://historicengland.org.uk/"/>
        <dc:spatial rdf:resource="http://vocab.getty.edu/tgn/7002445"/>
        <dc:spatial rdf:resource="http://dbpedia.org/resource/England"/>
        <skos:prefLabel xml:lang="en">Textile Mill</skos:prefLabel>
        <skos:scopeNote xml:lang="en">A factory used for the manufacture of textiles.</skos:scopeNote>
      </skos:Concept>
    </skos:narrower>

    <skos:inScheme rdf:resource="http://purl.org/heritagedata/schemes/571"/>
    <dc:identifier>http://purl.org/heritagedata/schemes/571/concepts/151226</dc:identifier>
    <dc:issued rdf:datatype="http://www.w3.org/2001/XMLSchema#dateTime">2024-07-01T17:17:33</dc:issued>
    <cc:license rdf:resource="https://www.nationalarchives.gov.uk/doc/open-government-licence/version/3/"/>
    <cc:attributionURL rdf:resource="https://historicengland.org.uk/"/>
    <cc:attributionName xml:lang="en">Historic England</cc:attributionName>
    <dc:publisher rdf:resource="https://historicengland.org.uk/"/>
    <dc:spatial rdf:resource="http://vocab.getty.edu/tgn/7002445"/>
    <dc:spatial rdf:resource="http://dbpedia.org/resource/England"/>
    <skos:prefLabel xml:lang="en">Mill</skos:prefLabel>
    <skos:scopeNote xml:lang="en">A factory used for processing raw materials. Use more specific mill type where known.</skos:scopeNote>
  </skos:Concept>

  <skos:Concept rdf:about="http://purl.org/heritagedata/schemes/571/concepts/151227">
    <skos:broader rdf:resource="http://purl.org/heritagedata/schemes/571/concepts/152624"/>
    <skos:inScheme rdf:resource="http://purl.org/heritagedata/schemes/571"/>
    <dc:identifier>http://purl.org/heritagedata/schemes/571/concepts/151227</dc:identifier>
    <dc:issued rdf:datatype="http://www.w3.org/2001/XMLSchema#dateTime">2024-07-01T17:17:33</dc:issued>
    <cc:license rdf:resource="https://www.nationalarchives.gov.uk/doc/open-government-licence/version/3/"/>
    <cc:attributionURL rdf:resource="https://historicengland.org.uk/"/>
    <cc:attributionName xml:lang="en">Historic England</cc:attributionName>
    <dc:publisher rdf:resource="https://historicengland.org.uk/"/>
    <dc:spatial rdf:resource="http://vocab.getty.edu/tgn/7002445"/>
    <dc:spatial rdf:resource="http://dbpedia.org/resource/England"/>
    <skos:prefLabel xml:lang="en">Chemical Works</skos:prefLabel>
    <skos:scopeNote xml:lang="en">An industrial complex involved in the production of chemicals.</skos:scopeNote>
  </skos:Concept>

  <skos:Concept rdf:about="http://purl.org/heritagedata/schemes/571/concepts/152624">
    <skos:narrower rdf:resource="http://purl.org/heritagedata/schemes/571/concepts/151227"/>
    <skos:narrower rdf:resource="http://purl.org/heritagedata/schemes/571/concepts/151734"/>
    <skos:narrower rdf:resource="http://purl.org/heritagedata/schemes/571/concepts/151749"/>
    <skos:narrower>
      <skos:Concept rdf:about="http://purl.org/heritagedata/schemes/571/concepts/152622">
        <skos:broader rdf:resource="http://purl.org/heritagedata/schemes/571/concepts/152624"/>
        <skos:inScheme rdf:resource="http://purl.org/heritagedata/schemes/571"/>
        <dc:identifier>http://purl.org/heritagedata/schemes/571/concepts/152622</dc:identifier>
        <dc:issued rdf:datatype="http://www.w3.org/2001/XMLSchema#dateTime">2024-07-01T17:17:33</dc:issued>
        <cc:license rdf:resource="https://www.nationalarchives.gov.uk/doc/open-government-licence/version/3/"/>
        <cc:attributionURL rdf:resource="https://historicengland.org.uk/"/>
        <cc:attributionName xml:lang="en">Historic England</cc:attributionName>
        <dc:publisher rdf:resource="https://historicengland.org.uk/"/>
        <dc:spatial rdf:resource="http://vocab.getty.edu/tgn/7002445"/>
        <dc:spatial rdf:resource="http://dbpedia.org/resource/England"/>
        <skos:prefLabel xml:lang="en">Lime Production</skos:prefLabel>
        <skos:scopeNote xml:lang="en">Areas associated primarily with the transport and production of burnt lime from limestone, largely for agricultural use but also for lime mortar.</skos:scopeNote>
      </skos:Concept>
    </skos:narrower>

    <skos:narrower rdf:resource="http://purl.org/heritagedata/schemes/571/concepts/152623"/>
    <skos:narrower>
      <skos:Concept rdf:about="http://purl.org/heritagedata/schemes/571/concepts/152626">
        <skos:broader rdf:resource="http://purl.org/heritagedata/schemes/571/concepts/152624"/>
        <skos:inScheme rdf:resource="http://purl.org/heritagedata/schemes/571"/>
        <dc:identifier>http://purl.org/heritagedata/schemes/571/concepts/152626</dc:identifier>
        <dc:issued rdf:datatype="http://www.w3.org/2001/XMLSchema#dateTime">2024-07-01T17:17:33</dc:issued>
        <cc:license rdf:resource="https://www.nationalarchives.gov.uk/doc/open-government-licence/version/3/"/>
        <cc:attributionURL rdf:resource="https://historicengland.org.uk/"/>
        <cc:attributionName xml:lang="en">Historic England</cc:attributionName>
        <dc:publisher rdf:resource="https://historicengland.org.uk/"/>
        <dc:spatial rdf:resource="http://vocab.getty.edu/tgn/7002445"/>
        <dc:spatial rdf:resource="http://dbpedia.org/resource/England"/>
        <skos:prefLabel xml:lang="en">Iron Works</skos:prefLabel>
        <skos:scopeNote xml:lang="en">An industrial complex for large-scale production of iron.</skos:scopeNote>
      </skos:Concept>
    </skos:narrower>

    <skos:narrower>
      <skos:Concept rdf:about="http://purl.org/heritagedata/schemes/571/concepts/160171">
        <skos:broader rdf:resource="http://purl.org/heritagedata/schemes/571/concepts/152624"/>
        <skos:inScheme rdf:resource="http://purl.org/heritagedata/schemes/571"/>
        <dc:identifier>http://purl.org/heritagedata/schemes/571/concepts/160171</dc:identifier>
        <dc:issued rdf:datatype="http://www.w3.org/2001/XMLSchema#dateTime">2024-07-01T17:17:33</dc:issued>
        <cc:license rdf:resource="https://www.nationalarchives.gov.uk/doc/open-government-licence/version/3/"/>
        <cc:attributionURL rdf:resource="https://historicengland.org.uk/"/>
        <cc:attributionName xml:lang="en">Historic England</cc:attributionName>
        <dc:publisher rdf:resource="https://historicengland.org.uk/"/>
        <dc:spatial rdf:resource="http://vocab.getty.edu/tgn/7002445"/>
        <dc:spatial rdf:resource="http://dbpedia.org/resource/England"/>
        <skos:prefLabel xml:lang="en">Metal Works</skos:prefLabel>
        <skos:scopeNote xml:lang="en">A place where metal ores are dressed, smelted and transformed into utilitarian material.</skos:scopeNote>
      </skos:Concept>
    </skos:narrower>

    <skos:broader rdf:resource="http://purl.org/heritagedata/schemes/571/concepts/151457"/>
    <skos:inScheme rdf:resource="http://purl.org/heritagedata/schemes/571"/>
    <dc:identifier>http://purl.org/heritagedata/schemes/571/concepts/152624</dc:identifier>
    <dc:issued rdf:datatype="http://www.w3.org/2001/XMLSchema#dateTime">2024-07-01T17:17:33</dc:issued>
    <cc:license rdf:resource="https://www.nationalarchives.gov.uk/doc/open-government-licence/version/3/"/>
    <cc:attributionURL rdf:resource="https://historicengland.org.uk/"/>
    <cc:attributionName xml:lang="en">Historic England</cc:attributionName>
    <dc:publisher rdf:resource="https://historicengland.org.uk/"/>
    <dc:spatial rdf:resource="http://vocab.getty.edu/tgn/7002445"/>
    <dc:spatial rdf:resource="http://dbpedia.org/resource/England"/>
    <skos:prefLabel xml:lang="en">Processing Industry</skos:prefLabel>
    <skos:scopeNote xml:lang="en">Covers industries applying various processes to primary materials to prepare them for use either directly or in manufacturing industry. Use specific type where known.</skos:scopeNote>
  </skos:Concept>

  <skos:Concept rdf:about="http://purl.org/heritagedata/schemes/571/concepts/151229">
    <skos:broader rdf:resource="http://purl.org/heritagedata/schemes/571/concepts/151235"/>
    <skos:inScheme rdf:resource="http://purl.org/heritagedata/schemes/571"/>
    <dc:identifier>http://purl.org/heritagedata/schemes/571/concepts/151229</dc:identifier>
    <dc:issued rdf:datatype="http://www.w3.org/2001/XMLSchema#dateTime">2024-07-01T17:17:33</dc:issued>
    <cc:license rdf:resource="https://www.nationalarchives.gov.uk/doc/open-government-licence/version/3/"/>
    <cc:attributionURL rdf:resource="https://historicengland.org.uk/"/>
    <cc:attributionName xml:lang="en">Historic England</cc:attributionName>
    <dc:publisher rdf:resource="https://historicengland.org.uk/"/>
    <dc:spatial rdf:resource="http://vocab.getty.edu/tgn/7002445"/>
    <dc:spatial rdf:resource="http://dbpedia.org/resource/England"/>
    <skos:prefLabel xml:lang="en">Artillery Fort</skos:prefLabel>
    <skos:scopeNote xml:lang="en">A fortified building or site with purpose-built emplacements for artillery pieces.</skos:scopeNote>
  </skos:Concept>

  <skos:Concept rdf:about="http://purl.org/heritagedata/schemes/571/concepts/151235">
    <skos:narrower rdf:resource="http://purl.org/heritagedata/schemes/571/concepts/151229"/>
    <skos:narrower rdf:resource="http://purl.org/heritagedata/schemes/571/concepts/151231"/>
    <skos:narrower>
      <skos:Concept rdf:about="http://purl.org/heritagedata/schemes/571/concepts/151232">
        <skos:broader rdf:resource="http://purl.org/heritagedata/schemes/571/concepts/151235"/>
        <skos:inScheme rdf:resource="http://purl.org/heritagedata/schemes/571"/>
        <dc:identifier>http://purl.org/heritagedata/schemes/571/concepts/151232</dc:identifier>
        <dc:issued rdf:datatype="http://www.w3.org/2001/XMLSchema#dateTime">2024-07-01T17:17:33</dc:issued>
        <cc:license rdf:resource="https://www.nationalarchives.gov.uk/doc/open-government-licence/version/3/"/>
        <cc:attributionURL rdf:resource="https://historicengland.org.uk/"/>
        <cc:attributionName xml:lang="en">Historic England</cc:attributionName>
        <dc:publisher rdf:resource="https://historicengland.org.uk/"/>
        <dc:spatial rdf:resource="http://vocab.getty.edu/tgn/7002445"/>
        <dc:spatial rdf:resource="http://dbpedia.org/resource/England"/>
        <skos:prefLabel xml:lang="en">Town Wall</skos:prefLabel>
        <skos:scopeNote xml:lang="en">A fortified wall surrounding a town or city.</skos:scopeNote>
      </skos:Concept>
    </skos:narrower>

    <skos:narrower rdf:resource="http://purl.org/heritagedata/schemes/571/concepts/151928"/>
    <skos:narrower rdf:resource="http://purl.org/heritagedata/schemes/571/concepts/160194"/>
    <skos:broader rdf:resource="http://purl.org/heritagedata/schemes/571/concepts/151447"/>
    <skos:inScheme rdf:resource="http://purl.org/heritagedata/schemes/571"/>
    <dc:identifier>http://purl.org/heritagedata/schemes/571/concepts/151235</dc:identifier>
    <dc:issued rdf:datatype="http://www.w3.org/2001/XMLSchema#dateTime">2024-07-01T17:17:33</dc:issued>
    <cc:license rdf:resource="https://www.nationalarchives.gov.uk/doc/open-government-licence/version/3/"/>
    <cc:attributionURL rdf:resource="https://historicengland.org.uk/"/>
    <cc:attributionName xml:lang="en">Historic England</cc:attributionName>
    <dc:publisher rdf:resource="https://historicengland.org.uk/"/>
    <dc:spatial rdf:resource="http://vocab.getty.edu/tgn/7002445"/>
    <dc:spatial rdf:resource="http://dbpedia.org/resource/England"/>
    <skos:prefLabel xml:lang="en">Fortification</skos:prefLabel>
    <skos:scopeNote xml:lang="en">A defensive work, usually permanent. Use specific type where known.</skos:scopeNote>
  </skos:Concept>

  <skos:Concept rdf:about="http://purl.org/heritagedata/schemes/571/concepts/151230">
    <skos:broader rdf:resource="http://purl.org/heritagedata/schemes/571/concepts/151630"/>
    <skos:inScheme rdf:resource="http://purl.org/heritagedata/schemes/571"/>
    <dc:identifier>http://purl.org/heritagedata/schemes/571/concepts/151230</dc:identifier>
    <dc:issued rdf:datatype="http://www.w3.org/2001/XMLSchema#dateTime">2024-07-01T17:17:33</dc:issued>
    <cc:license rdf:resource="https://www.nationalarchives.gov.uk/doc/open-government-licence/version/3/"/>
    <cc:attributionURL rdf:resource="https://historicengland.org.uk/"/>
    <cc:attributionName xml:lang="en">Historic England</cc:attributionName>
    <dc:publisher rdf:resource="https://historicengland.org.uk/"/>
    <dc:spatial rdf:resource="http://vocab.getty.edu/tgn/7002445"/>
    <dc:spatial rdf:resource="http://dbpedia.org/resource/England"/>
    <skos:prefLabel xml:lang="en">Coastal Battery</skos:prefLabel>
    <skos:scopeNote xml:lang="en">A site including artillery pieces and associated structures directed out to sea to engage enemy shipping and defend the coastline.</skos:scopeNote>
  </skos:Concept>

  <skos:Concept rdf:about="http://purl.org/heritagedata/schemes/571/concepts/151630">
    <skos:narrower rdf:resource="http://purl.org/heritagedata/schemes/571/concepts/151230"/>
    <skos:broader rdf:resource="http://purl.org/heritagedata/schemes/571/concepts/151631"/>
    <skos:inScheme rdf:resource="http://purl.org/heritagedata/schemes/571"/>
    <dc:identifier>http://purl.org/heritagedata/schemes/571/concepts/151630</dc:identifier>
    <dc:issued rdf:datatype="http://www.w3.org/2001/XMLSchema#dateTime">2024-07-01T17:17:33</dc:issued>
    <cc:license rdf:resource="https://www.nationalarchives.gov.uk/doc/open-government-licence/version/3/"/>
    <cc:attributionURL rdf:resource="https://historicengland.org.uk/"/>
    <cc:attributionName xml:lang="en">Historic England</cc:attributionName>
    <dc:publisher rdf:resource="https://historicengland.org.uk/"/>
    <dc:spatial rdf:resource="http://vocab.getty.edu/tgn/7002445"/>
    <dc:spatial rdf:resource="http://dbpedia.org/resource/England"/>
    <skos:prefLabel xml:lang="en">Coastal Defences</skos:prefLabel>
    <skos:scopeNote xml:lang="en">An area of defensive installations on the coast designed for use against emeny attacks or invasion on the coast by sea or air.</skos:scopeNote>
  </skos:Concept>

  <skos:Concept rdf:about="http://purl.org/heritagedata/schemes/571/concepts/151231">
    <skos:broader rdf:resource="http://purl.org/heritagedata/schemes/571/concepts/151900"/>
    <skos:broader rdf:resource="http://purl.org/heritagedata/schemes/571/concepts/151235"/>
    <skos:inScheme rdf:resource="http://purl.org/heritagedata/schemes/571"/>
    <dc:identifier>http://purl.org/heritagedata/schemes/571/concepts/151231</dc:identifier>
    <dc:issued rdf:datatype="http://www.w3.org/2001/XMLSchema#dateTime">2024-07-01T17:17:33</dc:issued>
    <cc:license rdf:resource="https://www.nationalarchives.gov.uk/doc/open-government-licence/version/3/"/>
    <cc:attributionURL rdf:resource="https://historicengland.org.uk/"/>
    <cc:attributionName xml:lang="en">Historic England</cc:attributionName>
    <dc:publisher rdf:resource="https://historicengland.org.uk/"/>
    <dc:spatial rdf:resource="http://vocab.getty.edu/tgn/7002445"/>
    <dc:spatial rdf:resource="http://dbpedia.org/resource/England"/>
    <skos:prefLabel xml:lang="en">Castle</skos:prefLabel>
    <skos:scopeNote xml:lang="en">Fortified residence, usually of a noble and usually medieval or early post-medieval in date. Castle forms developed through time although some features, such as curtain walls and gatehouses, were common throughout.</skos:scopeNote>
  </skos:Concept>

  <skos:Concept rdf:about="http://purl.org/heritagedata/schemes/571/concepts/151900">
    <skos:narrower rdf:resource="http://purl.org/heritagedata/schemes/571/concepts/151231"/>
    <skos:narrower rdf:resource="http://purl.org/heritagedata/schemes/571/concepts/151928"/>
    <skos:narrower rdf:resource="http://purl.org/heritagedata/schemes/571/concepts/160194"/>
    <skos:broader rdf:resource="http://purl.org/heritagedata/schemes/571/concepts/151450"/>
    <skos:inScheme rdf:resource="http://purl.org/heritagedata/schemes/571"/>
    <dc:identifier>http://purl.org/heritagedata/schemes/571/concepts/151900</dc:identifier>
    <dc:issued rdf:datatype="http://www.w3.org/2001/XMLSchema#dateTime">2024-07-01T17:17:33</dc:issued>
    <cc:license rdf:resource="https://www.nationalarchives.gov.uk/doc/open-government-licence/version/3/"/>
    <cc:attributionURL rdf:resource="https://historicengland.org.uk/"/>
    <cc:attributionName xml:lang="en">Historic England</cc:attributionName>
    <dc:publisher rdf:resource="https://historicengland.org.uk/"/>
    <dc:spatial rdf:resource="http://vocab.getty.edu/tgn/7002445"/>
    <dc:spatial rdf:resource="http://dbpedia.org/resource/England"/>
    <skos:prefLabel xml:lang="en">Managed Heritage Asset</skos:prefLabel>
    <skos:scopeNote xml:lang="en">Large archaeological site presented to the public.</skos:scopeNote>
  </skos:Concept>

  <skos:Concept rdf:about="http://purl.org/heritagedata/schemes/571/concepts/151233">
    <skos:broader rdf:resource="http://purl.org/heritagedata/schemes/571/concepts/151642"/>
    <skos:inScheme rdf:resource="http://purl.org/heritagedata/schemes/571"/>
    <dc:identifier>http://purl.org/heritagedata/schemes/571/concepts/151233</dc:identifier>
    <dc:issued rdf:datatype="http://www.w3.org/2001/XMLSchema#dateTime">2024-07-01T17:17:33</dc:issued>
    <cc:license rdf:resource="https://www.nationalarchives.gov.uk/doc/open-government-licence/version/3/"/>
    <cc:attributionURL rdf:resource="https://historicengland.org.uk/"/>
    <cc:attributionName xml:lang="en">Historic England</cc:attributionName>
    <dc:publisher rdf:resource="https://historicengland.org.uk/"/>
    <dc:spatial rdf:resource="http://vocab.getty.edu/tgn/7002445"/>
    <dc:spatial rdf:resource="http://dbpedia.org/resource/England"/>
    <skos:prefLabel xml:lang="en">Military Airfield</skos:prefLabel>
    <skos:related rdf:resource="http://purl.org/heritagedata/schemes/571/concepts/151082"/>
    <skos:related rdf:resource="http://purl.org/heritagedata/schemes/571/concepts/151163"/>
    <skos:scopeNote xml:lang="en">A landing and taking-off area for military aircraft. Often includes ancilliary structures and buildings for the maintenance and storage of aircraft, defence of the site, accommodation of staff, controlling airspace etc.</skos:scopeNote>
  </skos:Concept>

  <skos:Concept rdf:about="http://purl.org/heritagedata/schemes/571/concepts/151234">
    <skos:broader rdf:resource="http://purl.org/heritagedata/schemes/571/concepts/151644"/>
    <skos:inScheme rdf:resource="http://purl.org/heritagedata/schemes/571"/>
    <dc:identifier>http://purl.org/heritagedata/schemes/571/concepts/151234</dc:identifier>
    <dc:issued rdf:datatype="http://www.w3.org/2001/XMLSchema#dateTime">2024-07-01T17:17:33</dc:issued>
    <cc:license rdf:resource="https://www.nationalarchives.gov.uk/doc/open-government-licence/version/3/"/>
    <cc:attributionURL rdf:resource="https://historicengland.org.uk/"/>
    <cc:attributionName xml:lang="en">Historic England</cc:attributionName>
    <dc:publisher rdf:resource="https://historicengland.org.uk/"/>
    <dc:spatial rdf:resource="http://vocab.getty.edu/tgn/7002445"/>
    <dc:spatial rdf:resource="http://dbpedia.org/resource/England"/>
    <skos:prefLabel xml:lang="en">Prisoner Of War Camp</skos:prefLabel>
    <skos:scopeNote xml:lang="en">A prison for the containment of servicemen captured in war.</skos:scopeNote>
  </skos:Concept>

  <skos:Concept rdf:about="http://purl.org/heritagedata/schemes/571/concepts/151644">
    <skos:narrower rdf:resource="http://purl.org/heritagedata/schemes/571/concepts/151234"/>
    <skos:narrower>
      <skos:Concept rdf:about="http://purl.org/heritagedata/schemes/571/concepts/151242">
        <skos:broader rdf:resource="http://purl.org/heritagedata/schemes/571/concepts/151644"/>
        <skos:inScheme rdf:resource="http://purl.org/heritagedata/schemes/571"/>
        <dc:identifier>http://purl.org/heritagedata/schemes/571/concepts/151242</dc:identifier>
        <dc:issued rdf:datatype="http://www.w3.org/2001/XMLSchema#dateTime">2024-07-01T17:17:33</dc:issued>
        <cc:license rdf:resource="https://www.nationalarchives.gov.uk/doc/open-government-licence/version/3/"/>
        <cc:attributionURL rdf:resource="https://historicengland.org.uk/"/>
        <cc:attributionName xml:lang="en">Historic England</cc:attributionName>
        <dc:publisher rdf:resource="https://historicengland.org.uk/"/>
        <dc:spatial rdf:resource="http://vocab.getty.edu/tgn/7002445"/>
        <dc:spatial rdf:resource="http://dbpedia.org/resource/England"/>
        <skos:prefLabel xml:lang="en">Barracks</skos:prefLabel>
        <skos:scopeNote xml:lang="en">Areas of buildings used to house members of the armed forces. Such areas may also include closely related buildings such as refectories, mess rooms, hospitals, schools and gymnasia.</skos:scopeNote>
      </skos:Concept>
    </skos:narrower>

    <skos:broader rdf:resource="http://purl.org/heritagedata/schemes/571/concepts/151447"/>
    <skos:inScheme rdf:resource="http://purl.org/heritagedata/schemes/571"/>
    <dc:identifier>http://purl.org/heritagedata/schemes/571/concepts/151644</dc:identifier>
    <dc:issued rdf:datatype="http://www.w3.org/2001/XMLSchema#dateTime">2024-07-01T17:17:33</dc:issued>
    <cc:license rdf:resource="https://www.nationalarchives.gov.uk/doc/open-government-licence/version/3/"/>
    <cc:attributionURL rdf:resource="https://historicengland.org.uk/"/>
    <cc:attributionName xml:lang="en">Historic England</cc:attributionName>
    <dc:publisher rdf:resource="https://historicengland.org.uk/"/>
    <dc:spatial rdf:resource="http://vocab.getty.edu/tgn/7002445"/>
    <dc:spatial rdf:resource="http://dbpedia.org/resource/England"/>
    <skos:prefLabel xml:lang="en">Military Residence</skos:prefLabel>
    <skos:scopeNote xml:lang="en">A residence for military personnel.</skos:scopeNote>
  </skos:Concept>

  <skos:Concept rdf:about="http://purl.org/heritagedata/schemes/571/concepts/151447">
    <skos:narrower rdf:resource="http://purl.org/heritagedata/schemes/571/concepts/151235"/>
    <skos:narrower>
      <skos:Concept rdf:about="http://purl.org/heritagedata/schemes/571/concepts/151408">
        <skos:broader rdf:resource="http://purl.org/heritagedata/schemes/571/concepts/151447"/>
        <skos:inScheme rdf:resource="http://purl.org/heritagedata/schemes/571"/>
        <dc:identifier>http://purl.org/heritagedata/schemes/571/concepts/151408</dc:identifier>
        <dc:issued rdf:datatype="http://www.w3.org/2001/XMLSchema#dateTime">2024-07-01T17:17:33</dc:issued>
        <cc:license rdf:resource="https://www.nationalarchives.gov.uk/doc/open-government-licence/version/3/"/>
        <cc:attributionURL rdf:resource="https://historicengland.org.uk/"/>
        <cc:attributionName xml:lang="en">Historic England</cc:attributionName>
        <dc:publisher rdf:resource="https://historicengland.org.uk/"/>
        <dc:spatial rdf:resource="http://vocab.getty.edu/tgn/7002445"/>
        <dc:spatial rdf:resource="http://dbpedia.org/resource/England"/>
        <skos:prefLabel xml:lang="en">Defence Research Establishment</skos:prefLabel>
        <skos:scopeNote xml:lang="en">A complex of buildings and areas in which a range of weaponry and techniques are developed and trialled.</skos:scopeNote>
      </skos:Concept>
    </skos:narrower>

    <skos:narrower rdf:resource="http://purl.org/heritagedata/schemes/571/concepts/151631"/>
    <skos:narrower rdf:resource="http://purl.org/heritagedata/schemes/571/concepts/151634"/>
    <skos:narrower rdf:resource="http://purl.org/heritagedata/schemes/571/concepts/151636"/>
    <skos:narrower rdf:resource="http://purl.org/heritagedata/schemes/571/concepts/151642"/>
    <skos:narrower rdf:resource="http://purl.org/heritagedata/schemes/571/concepts/151644"/>
    <skos:narrower rdf:resource="http://purl.org/heritagedata/schemes/571/concepts/152570"/>
    <skos:narrower rdf:resource="http://purl.org/heritagedata/schemes/571/concepts/152571"/>
    <skos:inScheme rdf:resource="http://purl.org/heritagedata/schemes/571"/>
    <dc:identifier>http://purl.org/heritagedata/schemes/571/concepts/151447</dc:identifier>
    <dc:issued rdf:datatype="http://www.w3.org/2001/XMLSchema#dateTime">2024-07-01T17:17:33</dc:issued>
    <cc:license rdf:resource="https://www.nationalarchives.gov.uk/doc/open-government-licence/version/3/"/>
    <cc:attributionURL rdf:resource="https://historicengland.org.uk/"/>
    <cc:attributionName xml:lang="en">Historic England</cc:attributionName>
    <dc:publisher rdf:resource="https://historicengland.org.uk/"/>
    <dc:spatial rdf:resource="http://vocab.getty.edu/tgn/7002445"/>
    <dc:spatial rdf:resource="http://dbpedia.org/resource/England"/>
    <skos:prefLabel xml:lang="en">Military</skos:prefLabel>
    <skos:scopeNote xml:lang="en">-</skos:scopeNote>
    <skos:topConceptOf rdf:resource="http://purl.org/heritagedata/schemes/571"/>
  </skos:Concept>

  <skos:Concept rdf:about="http://purl.org/heritagedata/schemes/571/concepts/151236">
    <skos:broader rdf:resource="http://purl.org/heritagedata/schemes/571/concepts/152577"/>
    <skos:inScheme rdf:resource="http://purl.org/heritagedata/schemes/571"/>
    <dc:identifier>http://purl.org/heritagedata/schemes/571/concepts/151236</dc:identifier>
    <dc:issued rdf:datatype="http://www.w3.org/2001/XMLSchema#dateTime">2024-07-01T17:17:33</dc:issued>
    <cc:license rdf:resource="https://www.nationalarchives.gov.uk/doc/open-government-licence/version/3/"/>
    <cc:attributionURL rdf:resource="https://historicengland.org.uk/"/>
    <cc:attributionName xml:lang="en">Historic England</cc:attributionName>
    <dc:publisher rdf:resource="https://historicengland.org.uk/"/>
    <dc:spatial rdf:resource="http://vocab.getty.edu/tgn/7002445"/>
    <dc:spatial rdf:resource="http://dbpedia.org/resource/England"/>
    <skos:prefLabel xml:lang="en">Minefield</skos:prefLabel>
    <skos:scopeNote xml:lang="en">An area of ground or water containing explosive mines. In controlled minefields, also includes areas containing the controlling sites.</skos:scopeNote>
  </skos:Concept>

  <skos:Concept rdf:about="http://purl.org/heritagedata/schemes/571/concepts/152577">
    <skos:narrower rdf:resource="http://purl.org/heritagedata/schemes/571/concepts/151236"/>
    <skos:narrower>
      <skos:Concept rdf:about="http://purl.org/heritagedata/schemes/571/concepts/151628">
        <skos:broader rdf:resource="http://purl.org/heritagedata/schemes/571/concepts/152577"/>
        <skos:inScheme rdf:resource="http://purl.org/heritagedata/schemes/571"/>
        <dc:identifier>http://purl.org/heritagedata/schemes/571/concepts/151628</dc:identifier>
        <dc:issued rdf:datatype="http://www.w3.org/2001/XMLSchema#dateTime">2024-07-01T17:17:33</dc:issued>
        <cc:license rdf:resource="https://www.nationalarchives.gov.uk/doc/open-government-licence/version/3/"/>
        <cc:attributionURL rdf:resource="https://historicengland.org.uk/"/>
        <cc:attributionName xml:lang="en">Historic England</cc:attributionName>
        <dc:publisher rdf:resource="https://historicengland.org.uk/"/>
        <dc:spatial rdf:resource="http://vocab.getty.edu/tgn/7002445"/>
        <dc:spatial rdf:resource="http://dbpedia.org/resource/England"/>
        <skos:prefLabel xml:lang="en">Anti Tank Defence</skos:prefLabel>
        <skos:scopeNote xml:lang="en">Defensive structures, obstacles like concrete cubes, cylinders or pimples against invading tanks that were erected in the defence of Britain during the Second World War.</skos:scopeNote>
      </skos:Concept>
    </skos:narrower>

    <skos:narrower>
      <skos:Concept rdf:about="http://purl.org/heritagedata/schemes/571/concepts/151629">
        <skos:broader rdf:resource="http://purl.org/heritagedata/schemes/571/concepts/152577"/>
        <skos:inScheme rdf:resource="http://purl.org/heritagedata/schemes/571"/>
        <dc:identifier>http://purl.org/heritagedata/schemes/571/concepts/151629</dc:identifier>
        <dc:issued rdf:datatype="http://www.w3.org/2001/XMLSchema#dateTime">2024-07-01T17:17:33</dc:issued>
        <cc:license rdf:resource="https://www.nationalarchives.gov.uk/doc/open-government-licence/version/3/"/>
        <cc:attributionURL rdf:resource="https://historicengland.org.uk/"/>
        <cc:attributionName xml:lang="en">Historic England</cc:attributionName>
        <dc:publisher rdf:resource="https://historicengland.org.uk/"/>
        <dc:spatial rdf:resource="http://vocab.getty.edu/tgn/7002445"/>
        <dc:spatial rdf:resource="http://dbpedia.org/resource/England"/>
        <skos:prefLabel xml:lang="en">Anti Landing Obstacle</skos:prefLabel>
        <skos:scopeNote xml:lang="en">Obstacles placed in open spaces and alongside roads designed to prevent the successful landing of enemy airborne forces; usually of Second World War date.</skos:scopeNote>
      </skos:Concept>
    </skos:narrower>

    <skos:broader rdf:resource="http://purl.org/heritagedata/schemes/571/concepts/151631"/>
    <skos:inScheme rdf:resource="http://purl.org/heritagedata/schemes/571"/>
    <dc:identifier>http://purl.org/heritagedata/schemes/571/concepts/152577</dc:identifier>
    <dc:issued rdf:datatype="http://www.w3.org/2001/XMLSchema#dateTime">2024-07-01T17:17:33</dc:issued>
    <cc:license rdf:resource="https://www.nationalarchives.gov.uk/doc/open-government-licence/version/3/"/>
    <cc:attributionURL rdf:resource="https://historicengland.org.uk/"/>
    <cc:attributionName xml:lang="en">Historic England</cc:attributionName>
    <dc:publisher rdf:resource="https://historicengland.org.uk/"/>
    <dc:spatial rdf:resource="http://vocab.getty.edu/tgn/7002445"/>
    <dc:spatial rdf:resource="http://dbpedia.org/resource/England"/>
    <skos:prefLabel xml:lang="en">Anti Invasion Defence</skos:prefLabel>
    <skos:scopeNote xml:lang="en">Sites, buildings and structures associated with the defence of the British Isles against invasion from seaborne or airborne forces.</skos:scopeNote>
  </skos:Concept>

  <skos:Concept rdf:about="http://purl.org/heritagedata/schemes/571/concepts/151237">
    <skos:broader rdf:resource="http://purl.org/heritagedata/schemes/571/concepts/151243"/>
    <skos:inScheme rdf:resource="http://purl.org/heritagedata/schemes/571"/>
    <dc:identifier>http://purl.org/heritagedata/schemes/571/concepts/151237</dc:identifier>
    <dc:issued rdf:datatype="http://www.w3.org/2001/XMLSchema#dateTime">2024-07-01T17:17:33</dc:issued>
    <cc:license rdf:resource="https://www.nationalarchives.gov.uk/doc/open-government-licence/version/3/"/>
    <cc:attributionURL rdf:resource="https://historicengland.org.uk/"/>
    <cc:attributionName xml:lang="en">Historic England</cc:attributionName>
    <dc:publisher rdf:resource="https://historicengland.org.uk/"/>
    <dc:spatial rdf:resource="http://vocab.getty.edu/tgn/7002445"/>
    <dc:spatial rdf:resource="http://dbpedia.org/resource/England"/>
    <skos:prefLabel xml:lang="en">Ordnance Dump</skos:prefLabel>
    <skos:scopeNote xml:lang="en">An area used by the armed forces for the storage and issuing of military stores and materials.</skos:scopeNote>
  </skos:Concept>

  <skos:Concept rdf:about="http://purl.org/heritagedata/schemes/571/concepts/151243">
    <skos:narrower rdf:resource="http://purl.org/heritagedata/schemes/571/concepts/151237"/>
    <skos:narrower>
      <skos:Concept rdf:about="http://purl.org/heritagedata/schemes/571/concepts/151241">
        <skos:broader rdf:resource="http://purl.org/heritagedata/schemes/571/concepts/151243"/>
        <skos:inScheme rdf:resource="http://purl.org/heritagedata/schemes/571"/>
        <dc:identifier>http://purl.org/heritagedata/schemes/571/concepts/151241</dc:identifier>
        <dc:issued rdf:datatype="http://www.w3.org/2001/XMLSchema#dateTime">2024-07-01T17:17:33</dc:issued>
        <cc:license rdf:resource="https://www.nationalarchives.gov.uk/doc/open-government-licence/version/3/"/>
        <cc:attributionURL rdf:resource="https://historicengland.org.uk/"/>
        <cc:attributionName xml:lang="en">Historic England</cc:attributionName>
        <dc:publisher rdf:resource="https://historicengland.org.uk/"/>
        <dc:spatial rdf:resource="http://vocab.getty.edu/tgn/7002445"/>
        <dc:spatial rdf:resource="http://dbpedia.org/resource/England"/>
        <skos:prefLabel xml:lang="en">Fuel Depot</skos:prefLabel>
        <skos:scopeNote xml:lang="en">A building or site used for the storage and distribution of fuel for military purposes.</skos:scopeNote>
      </skos:Concept>
    </skos:narrower>

    <skos:broader rdf:resource="http://purl.org/heritagedata/schemes/571/concepts/152570"/>
    <skos:inScheme rdf:resource="http://purl.org/heritagedata/schemes/571"/>
    <dc:identifier>http://purl.org/heritagedata/schemes/571/concepts/151243</dc:identifier>
    <dc:issued rdf:datatype="http://www.w3.org/2001/XMLSchema#dateTime">2024-07-01T17:17:33</dc:issued>
    <cc:license rdf:resource="https://www.nationalarchives.gov.uk/doc/open-government-licence/version/3/"/>
    <cc:attributionURL rdf:resource="https://historicengland.org.uk/"/>
    <cc:attributionName xml:lang="en">Historic England</cc:attributionName>
    <dc:publisher rdf:resource="https://historicengland.org.uk/"/>
    <dc:spatial rdf:resource="http://vocab.getty.edu/tgn/7002445"/>
    <dc:spatial rdf:resource="http://dbpedia.org/resource/England"/>
    <skos:prefLabel xml:lang="en">Military Depot</skos:prefLabel>
    <skos:scopeNote xml:lang="en">An area usually with a building or group of buildings, often enclosed by a system of fortifications, used by an armed force for the storage and distribution of military equipment.</skos:scopeNote>
  </skos:Concept>

  <skos:Concept rdf:about="http://purl.org/heritagedata/schemes/571/concepts/151238">
    <skos:broader rdf:resource="http://purl.org/heritagedata/schemes/571/concepts/152607"/>
    <skos:inScheme rdf:resource="http://purl.org/heritagedata/schemes/571"/>
    <dc:identifier>http://purl.org/heritagedata/schemes/571/concepts/151238</dc:identifier>
    <dc:issued rdf:datatype="http://www.w3.org/2001/XMLSchema#dateTime">2024-07-01T17:17:33</dc:issued>
    <cc:license rdf:resource="https://www.nationalarchives.gov.uk/doc/open-government-licence/version/3/"/>
    <cc:attributionURL rdf:resource="https://historicengland.org.uk/"/>
    <cc:attributionName xml:lang="en">Historic England</cc:attributionName>
    <dc:publisher rdf:resource="https://historicengland.org.uk/"/>
    <dc:spatial rdf:resource="http://vocab.getty.edu/tgn/7002445"/>
    <dc:spatial rdf:resource="http://dbpedia.org/resource/England"/>
    <skos:prefLabel xml:lang="en">Rifle Range</skos:prefLabel>
    <skos:scopeNote xml:lang="en">A target range used for rifle and small arms practice.</skos:scopeNote>
  </skos:Concept>

  <skos:Concept rdf:about="http://purl.org/heritagedata/schemes/571/concepts/152607">
    <skos:narrower rdf:resource="http://purl.org/heritagedata/schemes/571/concepts/151238"/>
    <skos:narrower>
      <skos:Concept rdf:about="http://purl.org/heritagedata/schemes/571/concepts/151627">
        <skos:broader rdf:resource="http://purl.org/heritagedata/schemes/571/concepts/152607"/>
        <skos:inScheme rdf:resource="http://purl.org/heritagedata/schemes/571"/>
        <dc:identifier>http://purl.org/heritagedata/schemes/571/concepts/151627</dc:identifier>
        <dc:issued rdf:datatype="http://www.w3.org/2001/XMLSchema#dateTime">2024-07-01T17:17:33</dc:issued>
        <cc:license rdf:resource="https://www.nationalarchives.gov.uk/doc/open-government-licence/version/3/"/>
        <cc:attributionURL rdf:resource="https://historicengland.org.uk/"/>
        <cc:attributionName xml:lang="en">Historic England</cc:attributionName>
        <dc:publisher rdf:resource="https://historicengland.org.uk/"/>
        <dc:spatial rdf:resource="http://vocab.getty.edu/tgn/7002445"/>
        <dc:spatial rdf:resource="http://dbpedia.org/resource/England"/>
        <skos:prefLabel xml:lang="en">Artillery Firing Range</skos:prefLabel>
        <skos:scopeNote xml:lang="en">A piece of ground, or a building, on which artillery may be fired at targets during training or exercises..</skos:scopeNote>
      </skos:Concept>
    </skos:narrower>

    <skos:narrower>
      <skos:Concept rdf:about="http://purl.org/heritagedata/schemes/571/concepts/151632">
        <skos:broader rdf:resource="http://purl.org/heritagedata/schemes/571/concepts/152607"/>
        <skos:inScheme rdf:resource="http://purl.org/heritagedata/schemes/571"/>
        <dc:identifier>http://purl.org/heritagedata/schemes/571/concepts/151632</dc:identifier>
        <dc:issued rdf:datatype="http://www.w3.org/2001/XMLSchema#dateTime">2024-07-01T17:17:33</dc:issued>
        <cc:license rdf:resource="https://www.nationalarchives.gov.uk/doc/open-government-licence/version/3/"/>
        <cc:attributionURL rdf:resource="https://historicengland.org.uk/"/>
        <cc:attributionName xml:lang="en">Historic England</cc:attributionName>
        <dc:publisher rdf:resource="https://historicengland.org.uk/"/>
        <dc:spatial rdf:resource="http://vocab.getty.edu/tgn/7002445"/>
        <dc:spatial rdf:resource="http://dbpedia.org/resource/England"/>
        <skos:prefLabel xml:lang="en">Naval Firing Range</skos:prefLabel>
        <skos:scopeNote xml:lang="en">An area of sea across which naval ships fire artillery at target sites or areas. In some cases accompanied by land-based observation facilities housing equipment to record accuracy and damage.</skos:scopeNote>
      </skos:Concept>
    </skos:narrower>

    <skos:broader rdf:resource="http://purl.org/heritagedata/schemes/571/concepts/151634"/>
    <skos:inScheme rdf:resource="http://purl.org/heritagedata/schemes/571"/>
    <dc:identifier>http://purl.org/heritagedata/schemes/571/concepts/152607</dc:identifier>
    <dc:issued rdf:datatype="http://www.w3.org/2001/XMLSchema#dateTime">2024-07-01T17:17:33</dc:issued>
    <cc:license rdf:resource="https://www.nationalarchives.gov.uk/doc/open-government-licence/version/3/"/>
    <cc:attributionURL rdf:resource="https://historicengland.org.uk/"/>
    <cc:attributionName xml:lang="en">Historic England</cc:attributionName>
    <dc:publisher rdf:resource="https://historicengland.org.uk/"/>
    <dc:spatial rdf:resource="http://vocab.getty.edu/tgn/7002445"/>
    <dc:spatial rdf:resource="http://dbpedia.org/resource/England"/>
    <skos:prefLabel xml:lang="en">Firing Range</skos:prefLabel>
    <skos:scopeNote xml:lang="en">A piece of ground over which small arms or large artillery may be fired at targets during training or exercises. Firing ranges regularly form components of much larger military practice areas.</skos:scopeNote>
  </skos:Concept>

  <skos:Concept rdf:about="http://purl.org/heritagedata/schemes/571/concepts/151239">
    <skos:broader rdf:resource="http://purl.org/heritagedata/schemes/571/concepts/151634"/>
    <skos:inScheme rdf:resource="http://purl.org/heritagedata/schemes/571"/>
    <dc:identifier>http://purl.org/heritagedata/schemes/571/concepts/151239</dc:identifier>
    <dc:issued rdf:datatype="http://www.w3.org/2001/XMLSchema#dateTime">2024-07-01T17:17:33</dc:issued>
    <cc:license rdf:resource="https://www.nationalarchives.gov.uk/doc/open-government-licence/version/3/"/>
    <cc:attributionURL rdf:resource="https://historicengland.org.uk/"/>
    <cc:attributionName xml:lang="en">Historic England</cc:attributionName>
    <dc:publisher rdf:resource="https://historicengland.org.uk/"/>
    <dc:spatial rdf:resource="http://vocab.getty.edu/tgn/7002445"/>
    <dc:spatial rdf:resource="http://dbpedia.org/resource/England"/>
    <skos:prefLabel xml:lang="en">Bombing Range</skos:prefLabel>
    <skos:scopeNote xml:lang="en">An area of land, with associated buildings and targets, used for practicing the dropping of bombs and other aspects of aerial warfare.</skos:scopeNote>
  </skos:Concept>

  <skos:Concept rdf:about="http://purl.org/heritagedata/schemes/571/concepts/151634">
    <skos:narrower rdf:resource="http://purl.org/heritagedata/schemes/571/concepts/151239"/>
    <skos:narrower>
      <skos:Concept rdf:about="http://purl.org/heritagedata/schemes/571/concepts/151637">
        <skos:broader rdf:resource="http://purl.org/heritagedata/schemes/571/concepts/151634"/>
        <skos:inScheme rdf:resource="http://purl.org/heritagedata/schemes/571"/>
        <dc:identifier>http://purl.org/heritagedata/schemes/571/concepts/151637</dc:identifier>
        <dc:issued rdf:datatype="http://www.w3.org/2001/XMLSchema#dateTime">2024-07-01T17:17:33</dc:issued>
        <cc:license rdf:resource="https://www.nationalarchives.gov.uk/doc/open-government-licence/version/3/"/>
        <cc:attributionURL rdf:resource="https://historicengland.org.uk/"/>
        <cc:attributionName xml:lang="en">Historic England</cc:attributionName>
        <dc:publisher rdf:resource="https://historicengland.org.uk/"/>
        <dc:spatial rdf:resource="http://vocab.getty.edu/tgn/7002445"/>
        <dc:spatial rdf:resource="http://dbpedia.org/resource/England"/>
        <skos:prefLabel xml:lang="en">Submarine Training Area</skos:prefLabel>
        <skos:scopeNote xml:lang="en">A designated area of water in which the performance of submarines can be evaluated and where crews can practice.</skos:scopeNote>
      </skos:Concept>
    </skos:narrower>

    <skos:narrower>
      <skos:Concept rdf:about="http://purl.org/heritagedata/schemes/571/concepts/151852">
        <skos:broader rdf:resource="http://purl.org/heritagedata/schemes/571/concepts/151634"/>
        <skos:inScheme rdf:resource="http://purl.org/heritagedata/schemes/571"/>
        <dc:identifier>http://purl.org/heritagedata/schemes/571/concepts/151852</dc:identifier>
        <dc:issued rdf:datatype="http://www.w3.org/2001/XMLSchema#dateTime">2024-07-01T17:17:33</dc:issued>
        <cc:license rdf:resource="https://www.nationalarchives.gov.uk/doc/open-government-licence/version/3/"/>
        <cc:attributionURL rdf:resource="https://historicengland.org.uk/"/>
        <cc:attributionName xml:lang="en">Historic England</cc:attributionName>
        <dc:publisher rdf:resource="https://historicengland.org.uk/"/>
        <dc:spatial rdf:resource="http://vocab.getty.edu/tgn/7002445"/>
        <dc:spatial rdf:resource="http://dbpedia.org/resource/England"/>
        <skos:prefLabel xml:lang="en">Tank Range</skos:prefLabel>
        <skos:scopeNote xml:lang="en">An area of ground used for the testing of, and practicing with armoured tanks.</skos:scopeNote>
      </skos:Concept>
    </skos:narrower>

    <skos:narrower rdf:resource="http://purl.org/heritagedata/schemes/571/concepts/152607"/>
    <skos:broader rdf:resource="http://purl.org/heritagedata/schemes/571/concepts/151447"/>
    <skos:inScheme rdf:resource="http://purl.org/heritagedata/schemes/571"/>
    <dc:identifier>http://purl.org/heritagedata/schemes/571/concepts/151634</dc:identifier>
    <dc:issued rdf:datatype="http://www.w3.org/2001/XMLSchema#dateTime">2024-07-01T17:17:33</dc:issued>
    <cc:license rdf:resource="https://www.nationalarchives.gov.uk/doc/open-government-licence/version/3/"/>
    <cc:attributionURL rdf:resource="https://historicengland.org.uk/"/>
    <cc:attributionName xml:lang="en">Historic England</cc:attributionName>
    <dc:publisher rdf:resource="https://historicengland.org.uk/"/>
    <dc:spatial rdf:resource="http://vocab.getty.edu/tgn/7002445"/>
    <dc:spatial rdf:resource="http://dbpedia.org/resource/England"/>
    <skos:prefLabel xml:lang="en">Military Practice Area</skos:prefLabel>
    <skos:scopeNote xml:lang="en">Areas used by armed forces on land or at sea for training and military exercises.</skos:scopeNote>
  </skos:Concept>

  <skos:Concept rdf:about="http://purl.org/heritagedata/schemes/571/concepts/151240">
    <skos:broader rdf:resource="http://purl.org/heritagedata/schemes/571/concepts/151636"/>
    <skos:inScheme rdf:resource="http://purl.org/heritagedata/schemes/571"/>
    <dc:identifier>http://purl.org/heritagedata/schemes/571/concepts/151240</dc:identifier>
    <dc:issued rdf:datatype="http://www.w3.org/2001/XMLSchema#dateTime">2024-07-01T17:17:33</dc:issued>
    <cc:license rdf:resource="https://www.nationalarchives.gov.uk/doc/open-government-licence/version/3/"/>
    <cc:attributionURL rdf:resource="https://historicengland.org.uk/"/>
    <cc:attributionName xml:lang="en">Historic England</cc:attributionName>
    <dc:publisher rdf:resource="https://historicengland.org.uk/"/>
    <dc:spatial rdf:resource="http://vocab.getty.edu/tgn/7002445"/>
    <dc:spatial rdf:resource="http://dbpedia.org/resource/England"/>
    <skos:prefLabel xml:lang="en">Radar Station</skos:prefLabel>
    <skos:scopeNote xml:lang="en">A building or site incorporating radar equipment used for detecting the presence of enemy aircraft or ships.</skos:scopeNote>
  </skos:Concept>

  <skos:Concept rdf:about="http://purl.org/heritagedata/schemes/571/concepts/151636">
    <skos:narrower rdf:resource="http://purl.org/heritagedata/schemes/571/concepts/151240"/>
    <skos:broader rdf:resource="http://purl.org/heritagedata/schemes/571/concepts/151447"/>
    <skos:inScheme rdf:resource="http://purl.org/heritagedata/schemes/571"/>
    <dc:identifier>http://purl.org/heritagedata/schemes/571/concepts/151636</dc:identifier>
    <dc:issued rdf:datatype="http://www.w3.org/2001/XMLSchema#dateTime">2024-07-01T17:17:33</dc:issued>
    <cc:license rdf:resource="https://www.nationalarchives.gov.uk/doc/open-government-licence/version/3/"/>
    <cc:attributionURL rdf:resource="https://historicengland.org.uk/"/>
    <cc:attributionName xml:lang="en">Historic England</cc:attributionName>
    <dc:publisher rdf:resource="https://historicengland.org.uk/"/>
    <dc:spatial rdf:resource="http://vocab.getty.edu/tgn/7002445"/>
    <dc:spatial rdf:resource="http://dbpedia.org/resource/England"/>
    <skos:prefLabel xml:lang="en">Military Signalling</skos:prefLabel>
    <skos:scopeNote xml:lang="en">Buildings and structures used for sending and receiving signals.</skos:scopeNote>
  </skos:Concept>

  <skos:Concept rdf:about="http://purl.org/heritagedata/schemes/571/concepts/152570">
    <skos:narrower rdf:resource="http://purl.org/heritagedata/schemes/571/concepts/151243"/>
    <skos:narrower>
      <skos:Concept rdf:about="http://purl.org/heritagedata/schemes/571/concepts/151643">
        <skos:broader rdf:resource="http://purl.org/heritagedata/schemes/571/concepts/152570"/>
        <skos:inScheme rdf:resource="http://purl.org/heritagedata/schemes/571"/>
        <dc:identifier>http://purl.org/heritagedata/schemes/571/concepts/151643</dc:identifier>
        <dc:issued rdf:datatype="http://www.w3.org/2001/XMLSchema#dateTime">2024-07-01T17:17:33</dc:issued>
        <cc:license rdf:resource="https://www.nationalarchives.gov.uk/doc/open-government-licence/version/3/"/>
        <cc:attributionURL rdf:resource="https://historicengland.org.uk/"/>
        <cc:attributionName xml:lang="en">Historic England</cc:attributionName>
        <dc:publisher rdf:resource="https://historicengland.org.uk/"/>
        <dc:spatial rdf:resource="http://vocab.getty.edu/tgn/7002445"/>
        <dc:spatial rdf:resource="http://dbpedia.org/resource/England"/>
        <skos:prefLabel xml:lang="en">Military Base</skos:prefLabel>
        <skos:scopeNote xml:lang="en">A building or group of buildings, often surrounded by a system of fortifications, used as a residential and training site by members of an armed force.</skos:scopeNote>
      </skos:Concept>
    </skos:narrower>

    <skos:broader rdf:resource="http://purl.org/heritagedata/schemes/571/concepts/151447"/>
    <skos:inScheme rdf:resource="http://purl.org/heritagedata/schemes/571"/>
    <dc:identifier>http://purl.org/heritagedata/schemes/571/concepts/152570</dc:identifier>
    <dc:issued rdf:datatype="http://www.w3.org/2001/XMLSchema#dateTime">2024-07-01T17:17:33</dc:issued>
    <cc:license rdf:resource="https://www.nationalarchives.gov.uk/doc/open-government-licence/version/3/"/>
    <cc:attributionURL rdf:resource="https://historicengland.org.uk/"/>
    <cc:attributionName xml:lang="en">Historic England</cc:attributionName>
    <dc:publisher rdf:resource="https://historicengland.org.uk/"/>
    <dc:spatial rdf:resource="http://vocab.getty.edu/tgn/7002445"/>
    <dc:spatial rdf:resource="http://dbpedia.org/resource/England"/>
    <skos:prefLabel xml:lang="en">Military Installation</skos:prefLabel>
    <skos:scopeNote xml:lang="en">A site and associated buildings used by the military for various purposes, usually defensive.</skos:scopeNote>
  </skos:Concept>

  <skos:Concept rdf:about="http://purl.org/heritagedata/schemes/571/concepts/151244">
    <skos:broader rdf:resource="http://purl.org/heritagedata/schemes/571/concepts/151448"/>
    <skos:narrower>
      <skos:Concept rdf:about="http://purl.org/heritagedata/schemes/571/concepts/151279">
        <skos:broader rdf:resource="http://purl.org/heritagedata/schemes/571/concepts/151244"/>
        <skos:inScheme rdf:resource="http://purl.org/heritagedata/schemes/571"/>
        <dc:identifier>http://purl.org/heritagedata/schemes/571/concepts/151279</dc:identifier>
        <dc:issued rdf:datatype="http://www.w3.org/2001/XMLSchema#dateTime">2024-07-01T17:17:33</dc:issued>
        <cc:license rdf:resource="https://www.nationalarchives.gov.uk/doc/open-government-licence/version/3/"/>
        <cc:attributionURL rdf:resource="https://historicengland.org.uk/"/>
        <cc:attributionName xml:lang="en">Historic England</cc:attributionName>
        <dc:publisher rdf:resource="https://historicengland.org.uk/"/>
        <dc:spatial rdf:resource="http://vocab.getty.edu/tgn/7002445"/>
        <dc:spatial rdf:resource="http://dbpedia.org/resource/England"/>
        <skos:prefLabel xml:lang="en">Short Rotation Coppice</skos:prefLabel>
        <skos:scopeNote xml:lang="en">A coppice, often of willow or poplar, that is grown as an energy crop.Usually for biomass power stations and usually harvested by machine when the trees are just two to five years old.</skos:scopeNote>
      </skos:Concept>
    </skos:narrower>

    <skos:inScheme rdf:resource="http://purl.org/heritagedata/schemes/571"/>
    <dc:identifier>http://purl.org/heritagedata/schemes/571/concepts/151244</dc:identifier>
    <dc:issued rdf:datatype="http://www.w3.org/2001/XMLSchema#dateTime">2024-07-01T17:17:33</dc:issued>
    <cc:license rdf:resource="https://www.nationalarchives.gov.uk/doc/open-government-licence/version/3/"/>
    <cc:attributionURL rdf:resource="https://historicengland.org.uk/"/>
    <cc:attributionName xml:lang="en">Historic England</cc:attributionName>
    <dc:publisher rdf:resource="https://historicengland.org.uk/"/>
    <dc:spatial rdf:resource="http://vocab.getty.edu/tgn/7002445"/>
    <dc:spatial rdf:resource="http://dbpedia.org/resource/England"/>
    <skos:prefLabel xml:lang="en">Coppice</skos:prefLabel>
    <skos:scopeNote xml:lang="en">Area of managed woodland, usually oak, ash, hornbeam, hazel, alder, willow or beech, periodically cut to encourage new growth providing a source of smaller timber; for rods, fuel, charcoal etc. Larger coppies often divided into cropping areas or coups.</skos:scopeNote>
  </skos:Concept>

  <skos:Concept rdf:about="http://purl.org/heritagedata/schemes/571/concepts/151448">
    <skos:narrower rdf:resource="http://purl.org/heritagedata/schemes/571/concepts/151244"/>
    <skos:narrower rdf:resource="http://purl.org/heritagedata/schemes/571/concepts/151245"/>
    <skos:narrower>
      <skos:Concept rdf:about="http://purl.org/heritagedata/schemes/571/concepts/151247">
        <skos:broader rdf:resource="http://purl.org/heritagedata/schemes/571/concepts/151448"/>
        <skos:inScheme rdf:resource="http://purl.org/heritagedata/schemes/571"/>
        <dc:identifier>http://purl.org/heritagedata/schemes/571/concepts/151247</dc:identifier>
        <dc:issued rdf:datatype="http://www.w3.org/2001/XMLSchema#dateTime">2024-07-01T17:17:33</dc:issued>
        <cc:license rdf:resource="https://www.nationalarchives.gov.uk/doc/open-government-licence/version/3/"/>
        <cc:attributionURL rdf:resource="https://historicengland.org.uk/"/>
        <cc:attributionName xml:lang="en">Historic England</cc:attributionName>
        <dc:publisher rdf:resource="https://historicengland.org.uk/"/>
        <dc:spatial rdf:resource="http://vocab.getty.edu/tgn/7002445"/>
        <dc:spatial rdf:resource="http://dbpedia.org/resource/England"/>
        <skos:prefLabel xml:lang="en">Wood Pasture</skos:prefLabel>
        <skos:scopeNote xml:lang="en">Scattered trees within grassland, the trees providing shelter for forage as well as being harvested for timber and fuel. Now most often found within deer parks, but more widespread, especially on steep slopes, in the medieval period.</skos:scopeNote>
      </skos:Concept>
    </skos:narrower>

    <skos:narrower rdf:resource="http://purl.org/heritagedata/schemes/571/concepts/151273"/>
    <skos:narrower>
      <skos:Concept rdf:about="http://purl.org/heritagedata/schemes/571/concepts/151274">
        <skos:broader rdf:resource="http://purl.org/heritagedata/schemes/571/concepts/151448"/>
        <skos:inScheme rdf:resource="http://purl.org/heritagedata/schemes/571"/>
        <dc:identifier>http://purl.org/heritagedata/schemes/571/concepts/151274</dc:identifier>
        <dc:issued rdf:datatype="http://www.w3.org/2001/XMLSchema#dateTime">2024-07-01T17:17:33</dc:issued>
        <cc:license rdf:resource="https://www.nationalarchives.gov.uk/doc/open-government-licence/version/3/"/>
        <cc:attributionURL rdf:resource="https://historicengland.org.uk/"/>
        <cc:attributionName xml:lang="en">Historic England</cc:attributionName>
        <dc:publisher rdf:resource="https://historicengland.org.uk/"/>
        <dc:spatial rdf:resource="http://vocab.getty.edu/tgn/7002445"/>
        <dc:spatial rdf:resource="http://dbpedia.org/resource/England"/>
        <skos:prefLabel xml:lang="en">Woodland (Broadleaved)</skos:prefLabel>
        <skos:scopeNote xml:lang="en">Areas of woodland dominated by broadleaved trees.</skos:scopeNote>
      </skos:Concept>
    </skos:narrower>

    <skos:narrower>
      <skos:Concept rdf:about="http://purl.org/heritagedata/schemes/571/concepts/151275">
        <skos:broader rdf:resource="http://purl.org/heritagedata/schemes/571/concepts/151448"/>
        <skos:inScheme rdf:resource="http://purl.org/heritagedata/schemes/571"/>
        <dc:identifier>http://purl.org/heritagedata/schemes/571/concepts/151275</dc:identifier>
        <dc:issued rdf:datatype="http://www.w3.org/2001/XMLSchema#dateTime">2024-07-01T17:17:33</dc:issued>
        <cc:license rdf:resource="https://www.nationalarchives.gov.uk/doc/open-government-licence/version/3/"/>
        <cc:attributionURL rdf:resource="https://historicengland.org.uk/"/>
        <cc:attributionName xml:lang="en">Historic England</cc:attributionName>
        <dc:publisher rdf:resource="https://historicengland.org.uk/"/>
        <dc:spatial rdf:resource="http://vocab.getty.edu/tgn/7002445"/>
        <dc:spatial rdf:resource="http://dbpedia.org/resource/England"/>
        <skos:prefLabel xml:lang="en">Woodland (Coniferous)</skos:prefLabel>
        <skos:scopeNote xml:lang="en">Areas of woodland dominated by coniferous trees.</skos:scopeNote>
      </skos:Concept>
    </skos:narrower>

    <skos:narrower>
      <skos:Concept rdf:about="http://purl.org/heritagedata/schemes/571/concepts/151276">
        <skos:broader rdf:resource="http://purl.org/heritagedata/schemes/571/concepts/151448"/>
        <skos:inScheme rdf:resource="http://purl.org/heritagedata/schemes/571"/>
        <dc:identifier>http://purl.org/heritagedata/schemes/571/concepts/151276</dc:identifier>
        <dc:issued rdf:datatype="http://www.w3.org/2001/XMLSchema#dateTime">2024-07-01T17:17:33</dc:issued>
        <cc:license rdf:resource="https://www.nationalarchives.gov.uk/doc/open-government-licence/version/3/"/>
        <cc:attributionURL rdf:resource="https://historicengland.org.uk/"/>
        <cc:attributionName xml:lang="en">Historic England</cc:attributionName>
        <dc:publisher rdf:resource="https://historicengland.org.uk/"/>
        <dc:spatial rdf:resource="http://vocab.getty.edu/tgn/7002445"/>
        <dc:spatial rdf:resource="http://dbpedia.org/resource/England"/>
        <skos:prefLabel xml:lang="en">Woodland (Mixed)</skos:prefLabel>
        <skos:scopeNote xml:lang="en">Areas of woodland consisting of both broadleaved and coniferous trees.</skos:scopeNote>
      </skos:Concept>
    </skos:narrower>

    <skos:narrower rdf:resource="http://purl.org/heritagedata/schemes/571/concepts/151280"/>
    <skos:narrower rdf:resource="http://purl.org/heritagedata/schemes/571/concepts/151594"/>
    <skos:inScheme rdf:resource="http://purl.org/heritagedata/schemes/571"/>
    <dc:identifier>http://purl.org/heritagedata/schemes/571/concepts/151448</dc:identifier>
    <dc:issued rdf:datatype="http://www.w3.org/2001/XMLSchema#dateTime">2024-07-01T17:17:33</dc:issued>
    <cc:license rdf:resource="https://www.nationalarchives.gov.uk/doc/open-government-licence/version/3/"/>
    <cc:attributionURL rdf:resource="https://historicengland.org.uk/"/>
    <cc:attributionName xml:lang="en">Historic England</cc:attributionName>
    <dc:publisher rdf:resource="https://historicengland.org.uk/"/>
    <dc:spatial rdf:resource="http://vocab.getty.edu/tgn/7002445"/>
    <dc:spatial rdf:resource="http://dbpedia.org/resource/England"/>
    <skos:prefLabel xml:lang="en">Woodland</skos:prefLabel>
    <skos:scopeNote xml:lang="en">In HLC used for woodland that has not been classified as ancient, plantation or secondary.</skos:scopeNote>
    <skos:topConceptOf rdf:resource="http://purl.org/heritagedata/schemes/571"/>
  </skos:Concept>

  <skos:Concept rdf:about="http://purl.org/heritagedata/schemes/571/concepts/151245">
    <skos:broader rdf:resource="http://purl.org/heritagedata/schemes/571/concepts/151448"/>
    <skos:narrower>
      <skos:Concept rdf:about="http://purl.org/heritagedata/schemes/571/concepts/151590">
        <skos:broader rdf:resource="http://purl.org/heritagedata/schemes/571/concepts/151245"/>
        <skos:inScheme rdf:resource="http://purl.org/heritagedata/schemes/571"/>
        <dc:identifier>http://purl.org/heritagedata/schemes/571/concepts/151590</dc:identifier>
        <dc:issued rdf:datatype="http://www.w3.org/2001/XMLSchema#dateTime">2024-07-01T17:17:33</dc:issued>
        <cc:license rdf:resource="https://www.nationalarchives.gov.uk/doc/open-government-licence/version/3/"/>
        <cc:attributionURL rdf:resource="https://historicengland.org.uk/"/>
        <cc:attributionName xml:lang="en">Historic England</cc:attributionName>
        <dc:publisher rdf:resource="https://historicengland.org.uk/"/>
        <dc:spatial rdf:resource="http://vocab.getty.edu/tgn/7002445"/>
        <dc:spatial rdf:resource="http://dbpedia.org/resource/England"/>
        <skos:prefLabel xml:lang="en">Plantation (Broadleaved)</skos:prefLabel>
        <skos:scopeNote xml:lang="en">Plantations dominated by broadleaved trees, including areas of planting, ground ripping, immature or mature stands, felled areas.</skos:scopeNote>
      </skos:Concept>
    </skos:narrower>

    <skos:narrower>
      <skos:Concept rdf:about="http://purl.org/heritagedata/schemes/571/concepts/151591">
        <skos:broader rdf:resource="http://purl.org/heritagedata/schemes/571/concepts/151245"/>
        <skos:inScheme rdf:resource="http://purl.org/heritagedata/schemes/571"/>
        <dc:identifier>http://purl.org/heritagedata/schemes/571/concepts/151591</dc:identifier>
        <dc:issued rdf:datatype="http://www.w3.org/2001/XMLSchema#dateTime">2024-07-01T17:17:33</dc:issued>
        <cc:license rdf:resource="https://www.nationalarchives.gov.uk/doc/open-government-licence/version/3/"/>
        <cc:attributionURL rdf:resource="https://historicengland.org.uk/"/>
        <cc:attributionName xml:lang="en">Historic England</cc:attributionName>
        <dc:publisher rdf:resource="https://historicengland.org.uk/"/>
        <dc:spatial rdf:resource="http://vocab.getty.edu/tgn/7002445"/>
        <dc:spatial rdf:resource="http://dbpedia.org/resource/England"/>
        <skos:prefLabel xml:lang="en">Plantation (Coniferous)</skos:prefLabel>
        <skos:scopeNote xml:lang="en">Plantations dominated by coniferous trees, including areas of planting, ground ripping, immature or mature stands, felled areas.</skos:scopeNote>
      </skos:Concept>
    </skos:narrower>

    <skos:narrower>
      <skos:Concept rdf:about="http://purl.org/heritagedata/schemes/571/concepts/151592">
        <skos:broader rdf:resource="http://purl.org/heritagedata/schemes/571/concepts/151245"/>
        <skos:inScheme rdf:resource="http://purl.org/heritagedata/schemes/571"/>
        <dc:identifier>http://purl.org/heritagedata/schemes/571/concepts/151592</dc:identifier>
        <dc:issued rdf:datatype="http://www.w3.org/2001/XMLSchema#dateTime">2024-07-01T17:17:33</dc:issued>
        <cc:license rdf:resource="https://www.nationalarchives.gov.uk/doc/open-government-licence/version/3/"/>
        <cc:attributionURL rdf:resource="https://historicengland.org.uk/"/>
        <cc:attributionName xml:lang="en">Historic England</cc:attributionName>
        <dc:publisher rdf:resource="https://historicengland.org.uk/"/>
        <dc:spatial rdf:resource="http://vocab.getty.edu/tgn/7002445"/>
        <dc:spatial rdf:resource="http://dbpedia.org/resource/England"/>
        <skos:prefLabel xml:lang="en">Plantation (Mixed)</skos:prefLabel>
        <skos:scopeNote xml:lang="en">Plantations containing both broadleaved and coniferous trees, including areas of planting, ground ripping, immature or mature stands, felled areas.</skos:scopeNote>
      </skos:Concept>
    </skos:narrower>

    <skos:inScheme rdf:resource="http://purl.org/heritagedata/schemes/571"/>
    <dc:identifier>http://purl.org/heritagedata/schemes/571/concepts/151245</dc:identifier>
    <dc:issued rdf:datatype="http://www.w3.org/2001/XMLSchema#dateTime">2024-07-01T17:17:33</dc:issued>
    <cc:license rdf:resource="https://www.nationalarchives.gov.uk/doc/open-government-licence/version/3/"/>
    <cc:attributionURL rdf:resource="https://historicengland.org.uk/"/>
    <cc:attributionName xml:lang="en">Historic England</cc:attributionName>
    <dc:publisher rdf:resource="https://historicengland.org.uk/"/>
    <dc:spatial rdf:resource="http://vocab.getty.edu/tgn/7002445"/>
    <dc:spatial rdf:resource="http://dbpedia.org/resource/England"/>
    <skos:prefLabel xml:lang="en">Plantation</skos:prefLabel>
    <skos:related rdf:resource="http://purl.org/heritagedata/schemes/571/concepts/151272"/>
    <skos:related rdf:resource="http://purl.org/heritagedata/schemes/571/concepts/151594"/>
    <skos:scopeNote xml:lang="en">Woodland planted deliberately, either for landscaping or to produce a crop of timber. Mid 20th century plantations usually single spicies conifers often plated in rows. Earlier plantations and those of the late 20th century onwards are often more mixed.</skos:scopeNote>
  </skos:Concept>

  <skos:Concept rdf:about="http://purl.org/heritagedata/schemes/571/concepts/151456">
    <skos:narrower rdf:resource="http://purl.org/heritagedata/schemes/571/concepts/151250"/>
    <skos:narrower rdf:resource="http://purl.org/heritagedata/schemes/571/concepts/151443"/>
    <skos:narrower rdf:resource="http://purl.org/heritagedata/schemes/571/concepts/151444"/>
    <skos:narrower rdf:resource="http://purl.org/heritagedata/schemes/571/concepts/152320"/>
    <skos:narrower rdf:resource="http://purl.org/heritagedata/schemes/571/concepts/152322"/>
    <skos:narrower rdf:resource="http://purl.org/heritagedata/schemes/571/concepts/152591"/>
    <skos:narrower rdf:resource="http://purl.org/heritagedata/schemes/571/concepts/152595"/>
    <skos:inScheme rdf:resource="http://purl.org/heritagedata/schemes/571"/>
    <dc:identifier>http://purl.org/heritagedata/schemes/571/concepts/151456</dc:identifier>
    <dc:issued rdf:datatype="http://www.w3.org/2001/XMLSchema#dateTime">2024-07-01T17:17:33</dc:issued>
    <cc:license rdf:resource="https://www.nationalarchives.gov.uk/doc/open-government-licence/version/3/"/>
    <cc:attributionURL rdf:resource="https://historicengland.org.uk/"/>
    <cc:attributionName xml:lang="en">Historic England</cc:attributionName>
    <dc:publisher rdf:resource="https://historicengland.org.uk/"/>
    <dc:spatial rdf:resource="http://vocab.getty.edu/tgn/7002445"/>
    <dc:spatial rdf:resource="http://dbpedia.org/resource/England"/>
    <skos:prefLabel xml:lang="en">Cultural Topography</skos:prefLabel>
    <skos:scopeNote xml:lang="en">-</skos:scopeNote>
    <skos:topConceptOf rdf:resource="http://purl.org/heritagedata/schemes/571"/>
  </skos:Concept>

  <skos:Concept rdf:about="http://purl.org/heritagedata/schemes/571/concepts/151251">
    <skos:broader rdf:resource="http://purl.org/heritagedata/schemes/571/concepts/164070"/>
    <skos:inScheme rdf:resource="http://purl.org/heritagedata/schemes/571"/>
    <dc:identifier>http://purl.org/heritagedata/schemes/571/concepts/151251</dc:identifier>
    <dc:issued rdf:datatype="http://www.w3.org/2001/XMLSchema#dateTime">2024-07-01T17:17:33</dc:issued>
    <cc:license rdf:resource="https://www.nationalarchives.gov.uk/doc/open-government-licence/version/3/"/>
    <cc:attributionURL rdf:resource="https://historicengland.org.uk/"/>
    <cc:attributionName xml:lang="en">Historic England</cc:attributionName>
    <dc:publisher rdf:resource="https://historicengland.org.uk/"/>
    <dc:spatial rdf:resource="http://vocab.getty.edu/tgn/7002445"/>
    <dc:spatial rdf:resource="http://dbpedia.org/resource/England"/>
    <skos:prefLabel xml:lang="en">Osier Beds</skos:prefLabel>
    <skos:scopeNote xml:lang="en">An area where osiers (types of willows, producing long straight stems) are cultivated for use in basketry.</skos:scopeNote>
  </skos:Concept>

  <skos:Concept rdf:about="http://purl.org/heritagedata/schemes/571/concepts/164070">
    <skos:narrower rdf:resource="http://purl.org/heritagedata/schemes/571/concepts/151251"/>
    <skos:broader rdf:resource="http://purl.org/heritagedata/schemes/571/concepts/152394"/>
    <skos:inScheme rdf:resource="http://purl.org/heritagedata/schemes/571"/>
    <dc:identifier>http://purl.org/heritagedata/schemes/571/concepts/164070</dc:identifier>
    <dc:issued rdf:datatype="http://www.w3.org/2001/XMLSchema#dateTime">2024-07-01T17:17:33</dc:issued>
    <cc:license rdf:resource="https://www.nationalarchives.gov.uk/doc/open-government-licence/version/3/"/>
    <cc:attributionURL rdf:resource="https://historicengland.org.uk/"/>
    <cc:attributionName xml:lang="en">Historic England</cc:attributionName>
    <dc:publisher rdf:resource="https://historicengland.org.uk/"/>
    <dc:spatial rdf:resource="http://vocab.getty.edu/tgn/7002445"/>
    <dc:spatial rdf:resource="http://dbpedia.org/resource/England"/>
    <skos:prefLabel xml:lang="en">Willow Gardens</skos:prefLabel>
    <skos:scopeNote xml:lang="en">Areas, often enclosed by stock-proof boundaries, where willows are cultivated for various purposes, including basketry, but also for fuel.</skos:scopeNote>
  </skos:Concept>

  <skos:Concept rdf:about="http://purl.org/heritagedata/schemes/571/concepts/151252">
    <skos:broader rdf:resource="http://purl.org/heritagedata/schemes/571/concepts/152394"/>
    <skos:inScheme rdf:resource="http://purl.org/heritagedata/schemes/571"/>
    <dc:identifier>http://purl.org/heritagedata/schemes/571/concepts/151252</dc:identifier>
    <dc:issued rdf:datatype="http://www.w3.org/2001/XMLSchema#dateTime">2024-07-01T17:17:33</dc:issued>
    <cc:license rdf:resource="https://www.nationalarchives.gov.uk/doc/open-government-licence/version/3/"/>
    <cc:attributionURL rdf:resource="https://historicengland.org.uk/"/>
    <cc:attributionName xml:lang="en">Historic England</cc:attributionName>
    <dc:publisher rdf:resource="https://historicengland.org.uk/"/>
    <dc:spatial rdf:resource="http://vocab.getty.edu/tgn/7002445"/>
    <dc:spatial rdf:resource="http://dbpedia.org/resource/England"/>
    <skos:prefLabel xml:lang="en">Watercress Beds</skos:prefLabel>
    <skos:scopeNote xml:lang="en">An area set aside for growing watercress. As the watercress requires large quantities of slightly alkaline water the beds are usually sited around the headwaters of chalk streams.</skos:scopeNote>
  </skos:Concept>

  <skos:Concept rdf:about="http://purl.org/heritagedata/schemes/571/concepts/152394">
    <skos:narrower rdf:resource="http://purl.org/heritagedata/schemes/571/concepts/151252"/>
    <skos:narrower>
      <skos:Concept rdf:about="http://purl.org/heritagedata/schemes/571/concepts/164065">
        <skos:broader rdf:resource="http://purl.org/heritagedata/schemes/571/concepts/152394"/>
        <skos:inScheme rdf:resource="http://purl.org/heritagedata/schemes/571"/>
        <dc:identifier>http://purl.org/heritagedata/schemes/571/concepts/164065</dc:identifier>
        <dc:issued rdf:datatype="http://www.w3.org/2001/XMLSchema#dateTime">2024-07-01T17:17:33</dc:issued>
        <cc:license rdf:resource="https://www.nationalarchives.gov.uk/doc/open-government-licence/version/3/"/>
        <cc:attributionURL rdf:resource="https://historicengland.org.uk/"/>
        <cc:attributionName xml:lang="en">Historic England</cc:attributionName>
        <dc:publisher rdf:resource="https://historicengland.org.uk/"/>
        <dc:spatial rdf:resource="http://vocab.getty.edu/tgn/7002445"/>
        <dc:spatial rdf:resource="http://dbpedia.org/resource/England"/>
        <skos:prefLabel xml:lang="en">Mill Water System</skos:prefLabel>
        <skos:scopeNote xml:lang="en">Water management system typically with weir, leat, mill pool, mill and its associated structures, spaces and tailrace.</skos:scopeNote>
      </skos:Concept>
    </skos:narrower>

    <skos:narrower>
      <skos:Concept rdf:about="http://purl.org/heritagedata/schemes/571/concepts/164066">
        <skos:broader rdf:resource="http://purl.org/heritagedata/schemes/571/concepts/152394"/>
        <skos:inScheme rdf:resource="http://purl.org/heritagedata/schemes/571"/>
        <dc:identifier>http://purl.org/heritagedata/schemes/571/concepts/164066</dc:identifier>
        <dc:issued rdf:datatype="http://www.w3.org/2001/XMLSchema#dateTime">2024-07-01T17:17:33</dc:issued>
        <cc:license rdf:resource="https://www.nationalarchives.gov.uk/doc/open-government-licence/version/3/"/>
        <cc:attributionURL rdf:resource="https://historicengland.org.uk/"/>
        <cc:attributionName xml:lang="en">Historic England</cc:attributionName>
        <dc:publisher rdf:resource="https://historicengland.org.uk/"/>
        <dc:spatial rdf:resource="http://vocab.getty.edu/tgn/7002445"/>
        <dc:spatial rdf:resource="http://dbpedia.org/resource/England"/>
        <skos:prefLabel xml:lang="en">Valley Bottom Meadow</skos:prefLabel>
        <skos:scopeNote xml:lang="en">Permanent grassland on poorly drained valley floors, exploited for the lush grass it supports. Often enclosed, sometimes held in common and used for hay-making and best summer pasture.</skos:scopeNote>
      </skos:Concept>
    </skos:narrower>

    <skos:narrower rdf:resource="http://purl.org/heritagedata/schemes/571/concepts/164067"/>
    <skos:narrower rdf:resource="http://purl.org/heritagedata/schemes/571/concepts/164070"/>
    <skos:inScheme rdf:resource="http://purl.org/heritagedata/schemes/571"/>
    <dc:identifier>http://purl.org/heritagedata/schemes/571/concepts/152394</dc:identifier>
    <dc:issued rdf:datatype="http://www.w3.org/2001/XMLSchema#dateTime">2024-07-01T17:17:33</dc:issued>
    <cc:license rdf:resource="https://www.nationalarchives.gov.uk/doc/open-government-licence/version/3/"/>
    <cc:attributionURL rdf:resource="https://historicengland.org.uk/"/>
    <cc:attributionName xml:lang="en">Historic England</cc:attributionName>
    <dc:publisher rdf:resource="https://historicengland.org.uk/"/>
    <dc:spatial rdf:resource="http://vocab.getty.edu/tgn/7002445"/>
    <dc:spatial rdf:resource="http://dbpedia.org/resource/England"/>
    <skos:prefLabel xml:lang="en">Valley Floor And Wetland Exploitation</skos:prefLabel>
    <skos:scopeNote xml:lang="en">-</skos:scopeNote>
    <skos:topConceptOf rdf:resource="http://purl.org/heritagedata/schemes/571"/>
  </skos:Concept>

  <skos:Concept rdf:about="http://purl.org/heritagedata/schemes/571/concepts/151253">
    <skos:broader rdf:resource="http://purl.org/heritagedata/schemes/571/concepts/151254"/>
    <skos:inScheme rdf:resource="http://purl.org/heritagedata/schemes/571"/>
    <dc:identifier>http://purl.org/heritagedata/schemes/571/concepts/151253</dc:identifier>
    <dc:issued rdf:datatype="http://www.w3.org/2001/XMLSchema#dateTime">2024-07-01T17:17:33</dc:issued>
    <cc:license rdf:resource="https://www.nationalarchives.gov.uk/doc/open-government-licence/version/3/"/>
    <cc:attributionURL rdf:resource="https://historicengland.org.uk/"/>
    <cc:attributionName xml:lang="en">Historic England</cc:attributionName>
    <dc:publisher rdf:resource="https://historicengland.org.uk/"/>
    <dc:spatial rdf:resource="http://vocab.getty.edu/tgn/7002445"/>
    <dc:spatial rdf:resource="http://dbpedia.org/resource/England"/>
    <skos:prefLabel xml:lang="en">Market Town</skos:prefLabel>
    <skos:scopeNote xml:lang="en">A town notable for hosting on a regular basis a market, usually for agricultural products, including livestock.</skos:scopeNote>
  </skos:Concept>

  <skos:Concept rdf:about="http://purl.org/heritagedata/schemes/571/concepts/151254">
    <skos:narrower rdf:resource="http://purl.org/heritagedata/schemes/571/concepts/151253"/>
    <skos:narrower>
      <skos:Concept rdf:about="http://purl.org/heritagedata/schemes/571/concepts/151255">
        <skos:broader rdf:resource="http://purl.org/heritagedata/schemes/571/concepts/151254"/>
        <skos:inScheme rdf:resource="http://purl.org/heritagedata/schemes/571"/>
        <dc:identifier>http://purl.org/heritagedata/schemes/571/concepts/151255</dc:identifier>
        <dc:issued rdf:datatype="http://www.w3.org/2001/XMLSchema#dateTime">2024-07-01T17:17:33</dc:issued>
        <cc:license rdf:resource="https://www.nationalarchives.gov.uk/doc/open-government-licence/version/3/"/>
        <cc:attributionURL rdf:resource="https://historicengland.org.uk/"/>
        <cc:attributionName xml:lang="en">Historic England</cc:attributionName>
        <dc:publisher rdf:resource="https://historicengland.org.uk/"/>
        <dc:spatial rdf:resource="http://vocab.getty.edu/tgn/7002445"/>
        <dc:spatial rdf:resource="http://dbpedia.org/resource/England"/>
        <skos:prefLabel xml:lang="en">New Town</skos:prefLabel>
        <skos:scopeNote xml:lang="en">A planned town built to disperse population following the Second World War, largely under the powers of the New Towns Act 1946. Normally not actually new, but developed around existing settlements that form historic urban cores.</skos:scopeNote>
      </skos:Concept>
    </skos:narrower>

    <skos:narrower>
      <skos:Concept rdf:about="http://purl.org/heritagedata/schemes/571/concepts/151256">
        <skos:broader rdf:resource="http://purl.org/heritagedata/schemes/571/concepts/151254"/>
        <skos:inScheme rdf:resource="http://purl.org/heritagedata/schemes/571"/>
        <dc:identifier>http://purl.org/heritagedata/schemes/571/concepts/151256</dc:identifier>
        <dc:issued rdf:datatype="http://www.w3.org/2001/XMLSchema#dateTime">2024-07-01T17:17:33</dc:issued>
        <cc:license rdf:resource="https://www.nationalarchives.gov.uk/doc/open-government-licence/version/3/"/>
        <cc:attributionURL rdf:resource="https://historicengland.org.uk/"/>
        <cc:attributionName xml:lang="en">Historic England</cc:attributionName>
        <dc:publisher rdf:resource="https://historicengland.org.uk/"/>
        <dc:spatial rdf:resource="http://vocab.getty.edu/tgn/7002445"/>
        <dc:spatial rdf:resource="http://dbpedia.org/resource/England"/>
        <skos:prefLabel xml:lang="en">Garden City</skos:prefLabel>
        <skos:scopeNote xml:lang="en">A planned town that developed from the Garden City Movement of the early 20th century, founded by Ebenezer Howard, and promoting the idea of separating residential and industrial/commercial areas with bands of parkland.</skos:scopeNote>
      </skos:Concept>
    </skos:narrower>

    <skos:broader rdf:resource="http://purl.org/heritagedata/schemes/571/concepts/151445"/>
    <skos:inScheme rdf:resource="http://purl.org/heritagedata/schemes/571"/>
    <dc:identifier>http://purl.org/heritagedata/schemes/571/concepts/151254</dc:identifier>
    <dc:issued rdf:datatype="http://www.w3.org/2001/XMLSchema#dateTime">2024-07-01T17:17:33</dc:issued>
    <cc:license rdf:resource="https://www.nationalarchives.gov.uk/doc/open-government-licence/version/3/"/>
    <cc:attributionURL rdf:resource="https://historicengland.org.uk/"/>
    <cc:attributionName xml:lang="en">Historic England</cc:attributionName>
    <dc:publisher rdf:resource="https://historicengland.org.uk/"/>
    <dc:spatial rdf:resource="http://vocab.getty.edu/tgn/7002445"/>
    <dc:spatial rdf:resource="http://dbpedia.org/resource/England"/>
    <skos:prefLabel xml:lang="en">Town</skos:prefLabel>
    <skos:related rdf:resource="http://purl.org/heritagedata/schemes/571/concepts/151077"/>
    <skos:related rdf:resource="http://purl.org/heritagedata/schemes/571/concepts/151078"/>
    <skos:related rdf:resource="http://purl.org/heritagedata/schemes/571/concepts/151079"/>
    <skos:related rdf:resource="http://purl.org/heritagedata/schemes/571/concepts/151762"/>
    <skos:scopeNote xml:lang="en">Settlement normally larger than a village, smaller than a city, usually with some administrative autonomy. Early towns often walled. Mixes of public and private buildings and spaces, and residential, civic, commercial and industrial areas.</skos:scopeNote>
  </skos:Concept>

  <skos:Concept rdf:about="http://purl.org/heritagedata/schemes/571/concepts/151445">
    <skos:narrower rdf:resource="http://purl.org/heritagedata/schemes/571/concepts/151254"/>
    <skos:narrower rdf:resource="http://purl.org/heritagedata/schemes/571/concepts/151577"/>
    <skos:narrower rdf:resource="http://purl.org/heritagedata/schemes/571/concepts/151581"/>
    <skos:narrower rdf:resource="http://purl.org/heritagedata/schemes/571/concepts/151762"/>
    <skos:narrower rdf:resource="http://purl.org/heritagedata/schemes/571/concepts/151763"/>
    <skos:narrower rdf:resource="http://purl.org/heritagedata/schemes/571/concepts/163214"/>
    <skos:inScheme rdf:resource="http://purl.org/heritagedata/schemes/571"/>
    <dc:identifier>http://purl.org/heritagedata/schemes/571/concepts/151445</dc:identifier>
    <dc:issued rdf:datatype="http://www.w3.org/2001/XMLSchema#dateTime">2024-07-01T17:17:33</dc:issued>
    <cc:license rdf:resource="https://www.nationalarchives.gov.uk/doc/open-government-licence/version/3/"/>
    <cc:attributionURL rdf:resource="https://historicengland.org.uk/"/>
    <cc:attributionName xml:lang="en">Historic England</cc:attributionName>
    <dc:publisher rdf:resource="https://historicengland.org.uk/"/>
    <dc:spatial rdf:resource="http://vocab.getty.edu/tgn/7002445"/>
    <dc:spatial rdf:resource="http://dbpedia.org/resource/England"/>
    <skos:prefLabel xml:lang="en">Urban Settlement</skos:prefLabel>
    <skos:scopeNote xml:lang="en">-</skos:scopeNote>
    <skos:topConceptOf rdf:resource="http://purl.org/heritagedata/schemes/571"/>
  </skos:Concept>

  <skos:Concept rdf:about="http://purl.org/heritagedata/schemes/571/concepts/151257">
    <skos:broader rdf:resource="http://purl.org/heritagedata/schemes/571/concepts/151446"/>
    <skos:broader rdf:resource="http://purl.org/heritagedata/schemes/571/concepts/163214"/>
    <skos:narrower>
      <skos:Concept rdf:about="http://purl.org/heritagedata/schemes/571/concepts/160424">
        <skos:broader rdf:resource="http://purl.org/heritagedata/schemes/571/concepts/151257"/>
        <skos:inScheme rdf:resource="http://purl.org/heritagedata/schemes/571"/>
        <dc:identifier>http://purl.org/heritagedata/schemes/571/concepts/160424</dc:identifier>
        <dc:issued rdf:datatype="http://www.w3.org/2001/XMLSchema#dateTime">2024-07-01T17:17:33</dc:issued>
        <cc:license rdf:resource="https://www.nationalarchives.gov.uk/doc/open-government-licence/version/3/"/>
        <cc:attributionURL rdf:resource="https://historicengland.org.uk/"/>
        <cc:attributionName xml:lang="en">Historic England</cc:attributionName>
        <dc:publisher rdf:resource="https://historicengland.org.uk/"/>
        <dc:spatial rdf:resource="http://vocab.getty.edu/tgn/7002445"/>
        <dc:spatial rdf:resource="http://dbpedia.org/resource/England"/>
        <skos:prefLabel xml:lang="en">Council Housing</skos:prefLabel>
        <skos:scopeNote xml:lang="en">Set of local authority provided dwellings for rent. Usually of uniform design, with gardens, and often located either at the edges of villages or at the roadside in open country.</skos:scopeNote>
      </skos:Concept>
    </skos:narrower>

    <skos:inScheme rdf:resource="http://purl.org/heritagedata/schemes/571"/>
    <dc:identifier>http://purl.org/heritagedata/schemes/571/concepts/151257</dc:identifier>
    <dc:issued rdf:datatype="http://www.w3.org/2001/XMLSchema#dateTime">2024-07-01T17:17:33</dc:issued>
    <cc:license rdf:resource="https://www.nationalarchives.gov.uk/doc/open-government-licence/version/3/"/>
    <cc:attributionURL rdf:resource="https://historicengland.org.uk/"/>
    <cc:attributionName xml:lang="en">Historic England</cc:attributionName>
    <dc:publisher rdf:resource="https://historicengland.org.uk/"/>
    <dc:spatial rdf:resource="http://vocab.getty.edu/tgn/7002445"/>
    <dc:spatial rdf:resource="http://dbpedia.org/resource/England"/>
    <skos:prefLabel xml:lang="en">Housing Estate</skos:prefLabel>
    <skos:related rdf:resource="http://purl.org/heritagedata/schemes/571/concepts/151582"/>
    <skos:scopeNote xml:lang="en">A planned residential area, usually with its own self-contained street system including cul-de-sacs, sometimes with its own amenities, such as shops, a public house etc.</skos:scopeNote>
  </skos:Concept>

  <skos:Concept rdf:about="http://purl.org/heritagedata/schemes/571/concepts/151446">
    <skos:narrower rdf:resource="http://purl.org/heritagedata/schemes/571/concepts/151257"/>
    <skos:narrower rdf:resource="http://purl.org/heritagedata/schemes/571/concepts/151295"/>
    <skos:narrower rdf:resource="http://purl.org/heritagedata/schemes/571/concepts/160426"/>
    <skos:narrower rdf:resource="http://purl.org/heritagedata/schemes/571/concepts/160427"/>
    <skos:inScheme rdf:resource="http://purl.org/heritagedata/schemes/571"/>
    <dc:identifier>http://purl.org/heritagedata/schemes/571/concepts/151446</dc:identifier>
    <dc:issued rdf:datatype="http://www.w3.org/2001/XMLSchema#dateTime">2024-07-01T17:17:33</dc:issued>
    <cc:license rdf:resource="https://www.nationalarchives.gov.uk/doc/open-government-licence/version/3/"/>
    <cc:attributionURL rdf:resource="https://historicengland.org.uk/"/>
    <cc:attributionName xml:lang="en">Historic England</cc:attributionName>
    <dc:publisher rdf:resource="https://historicengland.org.uk/"/>
    <dc:spatial rdf:resource="http://vocab.getty.edu/tgn/7002445"/>
    <dc:spatial rdf:resource="http://dbpedia.org/resource/England"/>
    <skos:prefLabel xml:lang="en">Rural Settlement</skos:prefLabel>
    <skos:scopeNote xml:lang="en">-</skos:scopeNote>
    <skos:topConceptOf rdf:resource="http://purl.org/heritagedata/schemes/571"/>
  </skos:Concept>

  <skos:Concept rdf:about="http://purl.org/heritagedata/schemes/571/concepts/163214">
    <skos:narrower rdf:resource="http://purl.org/heritagedata/schemes/571/concepts/151257"/>
    <skos:narrower rdf:resource="http://purl.org/heritagedata/schemes/571/concepts/151582"/>
    <skos:broader rdf:resource="http://purl.org/heritagedata/schemes/571/concepts/151445"/>
    <skos:inScheme rdf:resource="http://purl.org/heritagedata/schemes/571"/>
    <dc:identifier>http://purl.org/heritagedata/schemes/571/concepts/163214</dc:identifier>
    <dc:issued rdf:datatype="http://www.w3.org/2001/XMLSchema#dateTime">2024-07-01T17:17:33</dc:issued>
    <cc:license rdf:resource="https://www.nationalarchives.gov.uk/doc/open-government-licence/version/3/"/>
    <cc:attributionURL rdf:resource="https://historicengland.org.uk/"/>
    <cc:attributionName xml:lang="en">Historic England</cc:attributionName>
    <dc:publisher rdf:resource="https://historicengland.org.uk/"/>
    <dc:spatial rdf:resource="http://vocab.getty.edu/tgn/7002445"/>
    <dc:spatial rdf:resource="http://dbpedia.org/resource/England"/>
    <skos:prefLabel xml:lang="en">Residential Area</skos:prefLabel>
    <skos:related rdf:resource="http://purl.org/heritagedata/schemes/571/concepts/151298"/>
    <skos:related rdf:resource="http://purl.org/heritagedata/schemes/571/concepts/151299"/>
    <skos:related rdf:resource="http://purl.org/heritagedata/schemes/571/concepts/151300"/>
    <skos:related rdf:resource="http://purl.org/heritagedata/schemes/571/concepts/151301"/>
    <skos:scopeNote xml:lang="en">Urban area dominated by housing.</skos:scopeNote>
  </skos:Concept>

  <skos:Concept rdf:about="http://purl.org/heritagedata/schemes/571/concepts/151258">
    <skos:broader rdf:resource="http://purl.org/heritagedata/schemes/571/concepts/151762"/>
    <skos:broader rdf:resource="http://purl.org/heritagedata/schemes/571/concepts/151766"/>
    <skos:inScheme rdf:resource="http://purl.org/heritagedata/schemes/571"/>
    <dc:identifier>http://purl.org/heritagedata/schemes/571/concepts/151258</dc:identifier>
    <dc:issued rdf:datatype="http://www.w3.org/2001/XMLSchema#dateTime">2024-07-01T17:17:33</dc:issued>
    <cc:license rdf:resource="https://www.nationalarchives.gov.uk/doc/open-government-licence/version/3/"/>
    <cc:attributionURL rdf:resource="https://historicengland.org.uk/"/>
    <cc:attributionName xml:lang="en">Historic England</cc:attributionName>
    <dc:publisher rdf:resource="https://historicengland.org.uk/"/>
    <dc:spatial rdf:resource="http://vocab.getty.edu/tgn/7002445"/>
    <dc:spatial rdf:resource="http://dbpedia.org/resource/England"/>
    <skos:prefLabel xml:lang="en">Market Place</skos:prefLabel>
    <skos:scopeNote xml:lang="en">An area, often consisting of widened streets or a town square used for regular or occasional markets.</skos:scopeNote>
  </skos:Concept>

  <skos:Concept rdf:about="http://purl.org/heritagedata/schemes/571/concepts/151762">
    <skos:narrower rdf:resource="http://purl.org/heritagedata/schemes/571/concepts/151258"/>
    <skos:narrower>
      <skos:Concept rdf:about="http://purl.org/heritagedata/schemes/571/concepts/151765">
        <skos:broader rdf:resource="http://purl.org/heritagedata/schemes/571/concepts/151762"/>
        <skos:inScheme rdf:resource="http://purl.org/heritagedata/schemes/571"/>
        <dc:identifier>http://purl.org/heritagedata/schemes/571/concepts/151765</dc:identifier>
        <dc:issued rdf:datatype="http://www.w3.org/2001/XMLSchema#dateTime">2024-07-01T17:17:33</dc:issued>
        <cc:license rdf:resource="https://www.nationalarchives.gov.uk/doc/open-government-licence/version/3/"/>
        <cc:attributionURL rdf:resource="https://historicengland.org.uk/"/>
        <cc:attributionName xml:lang="en">Historic England</cc:attributionName>
        <dc:publisher rdf:resource="https://historicengland.org.uk/"/>
        <dc:spatial rdf:resource="http://vocab.getty.edu/tgn/7002445"/>
        <dc:spatial rdf:resource="http://dbpedia.org/resource/England"/>
        <skos:prefLabel xml:lang="en">Burgage Plot</skos:prefLabel>
        <skos:scopeNote xml:lang="en">A plot of land longer than it is wide, usually running perpendicularly from street with dwelling on street front. The holding of a burgess, and thus typical of medieval towns.</skos:scopeNote>
      </skos:Concept>
    </skos:narrower>

    <skos:broader rdf:resource="http://purl.org/heritagedata/schemes/571/concepts/151445"/>
    <skos:inScheme rdf:resource="http://purl.org/heritagedata/schemes/571"/>
    <dc:identifier>http://purl.org/heritagedata/schemes/571/concepts/151762</dc:identifier>
    <dc:issued rdf:datatype="http://www.w3.org/2001/XMLSchema#dateTime">2024-07-01T17:17:33</dc:issued>
    <cc:license rdf:resource="https://www.nationalarchives.gov.uk/doc/open-government-licence/version/3/"/>
    <cc:attributionURL rdf:resource="https://historicengland.org.uk/"/>
    <cc:attributionName xml:lang="en">Historic England</cc:attributionName>
    <dc:publisher rdf:resource="https://historicengland.org.uk/"/>
    <dc:spatial rdf:resource="http://vocab.getty.edu/tgn/7002445"/>
    <dc:spatial rdf:resource="http://dbpedia.org/resource/England"/>
    <skos:prefLabel xml:lang="en">Historic Urban Core</skos:prefLabel>
    <skos:related rdf:resource="http://purl.org/heritagedata/schemes/571/concepts/151254"/>
    <skos:related rdf:resource="http://purl.org/heritagedata/schemes/571/concepts/151577"/>
    <skos:scopeNote xml:lang="en">The long-established historic centre of a town or city, typically delineated in historic characterisation as extent shown on an early epoch of OS mapping.</skos:scopeNote>
  </skos:Concept>

  <skos:Concept rdf:about="http://purl.org/heritagedata/schemes/571/concepts/151766">
    <skos:narrower rdf:resource="http://purl.org/heritagedata/schemes/571/concepts/151258"/>
    <skos:narrower rdf:resource="http://purl.org/heritagedata/schemes/571/concepts/151619"/>
    <skos:broader rdf:resource="http://purl.org/heritagedata/schemes/571/concepts/151458"/>
    <skos:inScheme rdf:resource="http://purl.org/heritagedata/schemes/571"/>
    <dc:identifier>http://purl.org/heritagedata/schemes/571/concepts/151766</dc:identifier>
    <dc:issued rdf:datatype="http://www.w3.org/2001/XMLSchema#dateTime">2024-07-01T17:17:33</dc:issued>
    <cc:license rdf:resource="https://www.nationalarchives.gov.uk/doc/open-government-licence/version/3/"/>
    <cc:attributionURL rdf:resource="https://historicengland.org.uk/"/>
    <cc:attributionName xml:lang="en">Historic England</cc:attributionName>
    <dc:publisher rdf:resource="https://historicengland.org.uk/"/>
    <dc:spatial rdf:resource="http://vocab.getty.edu/tgn/7002445"/>
    <dc:spatial rdf:resource="http://dbpedia.org/resource/England"/>
    <skos:prefLabel xml:lang="en">Market</skos:prefLabel>
    <skos:scopeNote xml:lang="en">An open space or covered building(s) to which livestock, goods, etc, are brought and displayed for sale.</skos:scopeNote>
  </skos:Concept>

  <skos:Concept rdf:about="http://purl.org/heritagedata/schemes/571/concepts/151263">
    <skos:broader rdf:resource="http://purl.org/heritagedata/schemes/571/concepts/151264"/>
    <skos:inScheme rdf:resource="http://purl.org/heritagedata/schemes/571"/>
    <dc:identifier>http://purl.org/heritagedata/schemes/571/concepts/151263</dc:identifier>
    <dc:issued rdf:datatype="http://www.w3.org/2001/XMLSchema#dateTime">2024-07-01T17:17:33</dc:issued>
    <cc:license rdf:resource="https://www.nationalarchives.gov.uk/doc/open-government-licence/version/3/"/>
    <cc:attributionURL rdf:resource="https://historicengland.org.uk/"/>
    <cc:attributionName xml:lang="en">Historic England</cc:attributionName>
    <dc:publisher rdf:resource="https://historicengland.org.uk/"/>
    <dc:spatial rdf:resource="http://vocab.getty.edu/tgn/7002445"/>
    <dc:spatial rdf:resource="http://dbpedia.org/resource/England"/>
    <skos:prefLabel xml:lang="en">Green</skos:prefLabel>
    <skos:scopeNote xml:lang="en">Area of often grassy ground, usually common, normally situated at the centre of a village or hamlet, sometimes within or near a town. Usually maintained by grazing.</skos:scopeNote>
  </skos:Concept>

  <skos:Concept rdf:about="http://purl.org/heritagedata/schemes/571/concepts/151264">
    <skos:narrower rdf:resource="http://purl.org/heritagedata/schemes/571/concepts/151263"/>
    <skos:narrower>
      <skos:Concept rdf:about="http://purl.org/heritagedata/schemes/571/concepts/152329">
        <skos:broader rdf:resource="http://purl.org/heritagedata/schemes/571/concepts/151264"/>
        <skos:inScheme rdf:resource="http://purl.org/heritagedata/schemes/571"/>
        <dc:identifier>http://purl.org/heritagedata/schemes/571/concepts/152329</dc:identifier>
        <dc:issued rdf:datatype="http://www.w3.org/2001/XMLSchema#dateTime">2024-07-01T17:17:33</dc:issued>
        <cc:license rdf:resource="https://www.nationalarchives.gov.uk/doc/open-government-licence/version/3/"/>
        <cc:attributionURL rdf:resource="https://historicengland.org.uk/"/>
        <cc:attributionName xml:lang="en">Historic England</cc:attributionName>
        <dc:publisher rdf:resource="https://historicengland.org.uk/"/>
        <dc:spatial rdf:resource="http://vocab.getty.edu/tgn/7002445"/>
        <dc:spatial rdf:resource="http://dbpedia.org/resource/England"/>
        <skos:prefLabel xml:lang="en">Drove Common</skos:prefLabel>
        <skos:scopeNote xml:lang="en">A common used for the resting and grazing of herds cattle being 'driven' to and from market.</skos:scopeNote>
      </skos:Concept>
    </skos:narrower>

    <skos:broader rdf:resource="http://purl.org/heritagedata/schemes/571/concepts/152326"/>
    <skos:inScheme rdf:resource="http://purl.org/heritagedata/schemes/571"/>
    <dc:identifier>http://purl.org/heritagedata/schemes/571/concepts/151264</dc:identifier>
    <dc:issued rdf:datatype="http://www.w3.org/2001/XMLSchema#dateTime">2024-07-01T17:17:33</dc:issued>
    <cc:license rdf:resource="https://www.nationalarchives.gov.uk/doc/open-government-licence/version/3/"/>
    <cc:attributionURL rdf:resource="https://historicengland.org.uk/"/>
    <cc:attributionName xml:lang="en">Historic England</cc:attributionName>
    <dc:publisher rdf:resource="https://historicengland.org.uk/"/>
    <dc:spatial rdf:resource="http://vocab.getty.edu/tgn/7002445"/>
    <dc:spatial rdf:resource="http://dbpedia.org/resource/England"/>
    <skos:prefLabel xml:lang="en">Common</skos:prefLabel>
    <skos:related rdf:resource="http://purl.org/heritagedata/schemes/571/concepts/151767"/>
    <skos:scopeNote xml:lang="en">Unenclosed land, such as wasteland, forest or pasture, owned by an estate, but over which tenants and sometimes certain others have rights (pasture, turbary, estovers, pannage, etc).</skos:scopeNote>
  </skos:Concept>

  <skos:Concept rdf:about="http://purl.org/heritagedata/schemes/571/concepts/151265">
    <skos:broader rdf:resource="http://purl.org/heritagedata/schemes/571/concepts/152320"/>
    <skos:inScheme rdf:resource="http://purl.org/heritagedata/schemes/571"/>
    <dc:identifier>http://purl.org/heritagedata/schemes/571/concepts/151265</dc:identifier>
    <dc:issued rdf:datatype="http://www.w3.org/2001/XMLSchema#dateTime">2024-07-01T17:17:33</dc:issued>
    <cc:license rdf:resource="https://www.nationalarchives.gov.uk/doc/open-government-licence/version/3/"/>
    <cc:attributionURL rdf:resource="https://historicengland.org.uk/"/>
    <cc:attributionName xml:lang="en">Historic England</cc:attributionName>
    <dc:publisher rdf:resource="https://historicengland.org.uk/"/>
    <dc:spatial rdf:resource="http://vocab.getty.edu/tgn/7002445"/>
    <dc:spatial rdf:resource="http://dbpedia.org/resource/England"/>
    <skos:prefLabel xml:lang="en">Downland</skos:prefLabel>
    <skos:related rdf:resource="http://purl.org/heritagedata/schemes/571/concepts/152380"/>
    <skos:scopeNote xml:lang="en">An area of rolling upland terrain characterised by chalk escarpments separated by vales of softer earth.</skos:scopeNote>
  </skos:Concept>

  <skos:Concept rdf:about="http://purl.org/heritagedata/schemes/571/concepts/151266">
    <skos:broader rdf:resource="http://purl.org/heritagedata/schemes/571/concepts/160214"/>
    <skos:narrower>
      <skos:Concept rdf:about="http://purl.org/heritagedata/schemes/571/concepts/151293">
        <skos:broader rdf:resource="http://purl.org/heritagedata/schemes/571/concepts/151266"/>
        <skos:inScheme rdf:resource="http://purl.org/heritagedata/schemes/571"/>
        <dc:identifier>http://purl.org/heritagedata/schemes/571/concepts/151293</dc:identifier>
        <dc:issued rdf:datatype="http://www.w3.org/2001/XMLSchema#dateTime">2024-07-01T17:17:33</dc:issued>
        <cc:license rdf:resource="https://www.nationalarchives.gov.uk/doc/open-government-licence/version/3/"/>
        <cc:attributionURL rdf:resource="https://historicengland.org.uk/"/>
        <cc:attributionName xml:lang="en">Historic England</cc:attributionName>
        <dc:publisher rdf:resource="https://historicengland.org.uk/"/>
        <dc:spatial rdf:resource="http://vocab.getty.edu/tgn/7002445"/>
        <dc:spatial rdf:resource="http://dbpedia.org/resource/England"/>
        <skos:prefLabel xml:lang="en">Deer Course</skos:prefLabel>
        <skos:scopeNote xml:lang="en">Area in a deer park where a single deer was chased by dogs over a set distance, with bets made on the outcome. It usually includes a stand (for viewing) and can also include three distance markers, a finishing post and a ditch behind the last post.</skos:scopeNote>
      </skos:Concept>
    </skos:narrower>

    <skos:inScheme rdf:resource="http://purl.org/heritagedata/schemes/571"/>
    <dc:identifier>http://purl.org/heritagedata/schemes/571/concepts/151266</dc:identifier>
    <dc:issued rdf:datatype="http://www.w3.org/2001/XMLSchema#dateTime">2024-07-01T17:17:33</dc:issued>
    <cc:license rdf:resource="https://www.nationalarchives.gov.uk/doc/open-government-licence/version/3/"/>
    <cc:attributionURL rdf:resource="https://historicengland.org.uk/"/>
    <cc:attributionName xml:lang="en">Historic England</cc:attributionName>
    <dc:publisher rdf:resource="https://historicengland.org.uk/"/>
    <dc:spatial rdf:resource="http://vocab.getty.edu/tgn/7002445"/>
    <dc:spatial rdf:resource="http://dbpedia.org/resource/England"/>
    <skos:prefLabel xml:lang="en">Deer Park</skos:prefLabel>
    <skos:scopeNote xml:lang="en">A large, enclosed park, often containing some woodland and divided to provide a variety of habitats for shelter, grazing etc for deer, usually fallow, for hunting and for aesthetic appreciation..</skos:scopeNote>
  </skos:Concept>

  <skos:Concept rdf:about="http://purl.org/heritagedata/schemes/571/concepts/160214">
    <skos:narrower rdf:resource="http://purl.org/heritagedata/schemes/571/concepts/151266"/>
    <skos:narrower>
      <skos:Concept rdf:about="http://purl.org/heritagedata/schemes/571/concepts/151294">
        <skos:broader rdf:resource="http://purl.org/heritagedata/schemes/571/concepts/160214"/>
        <skos:inScheme rdf:resource="http://purl.org/heritagedata/schemes/571"/>
        <dc:identifier>http://purl.org/heritagedata/schemes/571/concepts/151294</dc:identifier>
        <dc:issued rdf:datatype="http://www.w3.org/2001/XMLSchema#dateTime">2024-07-01T17:17:33</dc:issued>
        <cc:license rdf:resource="https://www.nationalarchives.gov.uk/doc/open-government-licence/version/3/"/>
        <cc:attributionURL rdf:resource="https://historicengland.org.uk/"/>
        <cc:attributionName xml:lang="en">Historic England</cc:attributionName>
        <dc:publisher rdf:resource="https://historicengland.org.uk/"/>
        <dc:spatial rdf:resource="http://vocab.getty.edu/tgn/7002445"/>
        <dc:spatial rdf:resource="http://dbpedia.org/resource/England"/>
        <skos:prefLabel xml:lang="en">Kennels</skos:prefLabel>
        <skos:scopeNote xml:lang="en">Buildings and yards in which dogs and hunting hounds are kept and exercised.</skos:scopeNote>
      </skos:Concept>
    </skos:narrower>

    <skos:narrower>
      <skos:Concept rdf:about="http://purl.org/heritagedata/schemes/571/concepts/151607">
        <skos:broader rdf:resource="http://purl.org/heritagedata/schemes/571/concepts/160214"/>
        <skos:inScheme rdf:resource="http://purl.org/heritagedata/schemes/571"/>
        <dc:identifier>http://purl.org/heritagedata/schemes/571/concepts/151607</dc:identifier>
        <dc:issued rdf:datatype="http://www.w3.org/2001/XMLSchema#dateTime">2024-07-01T17:17:33</dc:issued>
        <cc:license rdf:resource="https://www.nationalarchives.gov.uk/doc/open-government-licence/version/3/"/>
        <cc:attributionURL rdf:resource="https://historicengland.org.uk/"/>
        <cc:attributionName xml:lang="en">Historic England</cc:attributionName>
        <dc:publisher rdf:resource="https://historicengland.org.uk/"/>
        <dc:spatial rdf:resource="http://vocab.getty.edu/tgn/7002445"/>
        <dc:spatial rdf:resource="http://dbpedia.org/resource/England"/>
        <skos:prefLabel xml:lang="en">Duck Decoy Pond</skos:prefLabel>
        <skos:scopeNote xml:lang="en">A pond or pool with arms covered with nets into which wild birds, are allured and then caught or shot.</skos:scopeNote>
      </skos:Concept>
    </skos:narrower>

    <skos:narrower>
      <skos:Concept rdf:about="http://purl.org/heritagedata/schemes/571/concepts/151794">
        <skos:broader rdf:resource="http://purl.org/heritagedata/schemes/571/concepts/160214"/>
        <skos:inScheme rdf:resource="http://purl.org/heritagedata/schemes/571"/>
        <dc:identifier>http://purl.org/heritagedata/schemes/571/concepts/151794</dc:identifier>
        <dc:issued rdf:datatype="http://www.w3.org/2001/XMLSchema#dateTime">2024-07-01T17:17:33</dc:issued>
        <cc:license rdf:resource="https://www.nationalarchives.gov.uk/doc/open-government-licence/version/3/"/>
        <cc:attributionURL rdf:resource="https://historicengland.org.uk/"/>
        <cc:attributionName xml:lang="en">Historic England</cc:attributionName>
        <dc:publisher rdf:resource="https://historicengland.org.uk/"/>
        <dc:spatial rdf:resource="http://vocab.getty.edu/tgn/7002445"/>
        <dc:spatial rdf:resource="http://dbpedia.org/resource/England"/>
        <skos:prefLabel xml:lang="en">Grouse Moor</skos:prefLabel>
        <skos:scopeNote xml:lang="en">Heathland used for the shooting of Red Grouse. Managed, by the controlled burning of areas of heather, to create a habitat that is favourable to grouse. Lines of butts used by the shooters are a common feature.</skos:scopeNote>
      </skos:Concept>
    </skos:narrower>

    <skos:narrower>
      <skos:Concept rdf:about="http://purl.org/heritagedata/schemes/571/concepts/151795">
        <skos:broader rdf:resource="http://purl.org/heritagedata/schemes/571/concepts/160214"/>
        <skos:inScheme rdf:resource="http://purl.org/heritagedata/schemes/571"/>
        <dc:identifier>http://purl.org/heritagedata/schemes/571/concepts/151795</dc:identifier>
        <dc:issued rdf:datatype="http://www.w3.org/2001/XMLSchema#dateTime">2024-07-01T17:17:33</dc:issued>
        <cc:license rdf:resource="https://www.nationalarchives.gov.uk/doc/open-government-licence/version/3/"/>
        <cc:attributionURL rdf:resource="https://historicengland.org.uk/"/>
        <cc:attributionName xml:lang="en">Historic England</cc:attributionName>
        <dc:publisher rdf:resource="https://historicengland.org.uk/"/>
        <dc:spatial rdf:resource="http://vocab.getty.edu/tgn/7002445"/>
        <dc:spatial rdf:resource="http://dbpedia.org/resource/England"/>
        <skos:prefLabel xml:lang="en">Royal Forest</skos:prefLabel>
        <skos:scopeNote xml:lang="en">Land including hunting areas for a monarch or (by invitation) the aristocracy; they usually included large areas of heath, grassland and wetland, that is habitats that supported deer and other game, but also farmland.</skos:scopeNote>
      </skos:Concept>
    </skos:narrower>

    <skos:broader rdf:resource="http://purl.org/heritagedata/schemes/571/concepts/151450"/>
    <skos:inScheme rdf:resource="http://purl.org/heritagedata/schemes/571"/>
    <dc:identifier>http://purl.org/heritagedata/schemes/571/concepts/160214</dc:identifier>
    <dc:issued rdf:datatype="http://www.w3.org/2001/XMLSchema#dateTime">2024-07-01T17:17:33</dc:issued>
    <cc:license rdf:resource="https://www.nationalarchives.gov.uk/doc/open-government-licence/version/3/"/>
    <cc:attributionURL rdf:resource="https://historicengland.org.uk/"/>
    <cc:attributionName xml:lang="en">Historic England</cc:attributionName>
    <dc:publisher rdf:resource="https://historicengland.org.uk/"/>
    <dc:spatial rdf:resource="http://vocab.getty.edu/tgn/7002445"/>
    <dc:spatial rdf:resource="http://dbpedia.org/resource/England"/>
    <skos:prefLabel xml:lang="en">Country Sport</skos:prefLabel>
    <skos:scopeNote xml:lang="en">Land primarily devoted to the persuit, trapping, shooting and hunting of wild or purposefully raised animals.</skos:scopeNote>
  </skos:Concept>

  <skos:Concept rdf:about="http://purl.org/heritagedata/schemes/571/concepts/151272">
    <skos:broader rdf:resource="http://purl.org/heritagedata/schemes/571/concepts/151273"/>
    <skos:broader rdf:resource="http://purl.org/heritagedata/schemes/571/concepts/151594"/>
    <skos:inScheme rdf:resource="http://purl.org/heritagedata/schemes/571"/>
    <dc:identifier>http://purl.org/heritagedata/schemes/571/concepts/151272</dc:identifier>
    <dc:issued rdf:datatype="http://www.w3.org/2001/XMLSchema#dateTime">2024-07-01T17:17:33</dc:issued>
    <cc:license rdf:resource="https://www.nationalarchives.gov.uk/doc/open-government-licence/version/3/"/>
    <cc:attributionURL rdf:resource="https://historicengland.org.uk/"/>
    <cc:attributionName xml:lang="en">Historic England</cc:attributionName>
    <dc:publisher rdf:resource="https://historicengland.org.uk/"/>
    <dc:spatial rdf:resource="http://vocab.getty.edu/tgn/7002445"/>
    <dc:spatial rdf:resource="http://dbpedia.org/resource/England"/>
    <skos:prefLabel xml:lang="en">Ancient Replanted Woodland</skos:prefLabel>
    <skos:related rdf:resource="http://purl.org/heritagedata/schemes/571/concepts/151245"/>
    <skos:scopeNote xml:lang="en">Ancient woodland where original natural tree coverage has been replanted with other trees, often coniferous.</skos:scopeNote>
  </skos:Concept>

  <skos:Concept rdf:about="http://purl.org/heritagedata/schemes/571/concepts/151594">
    <skos:narrower rdf:resource="http://purl.org/heritagedata/schemes/571/concepts/151272"/>
    <skos:broader rdf:resource="http://purl.org/heritagedata/schemes/571/concepts/151448"/>
    <skos:inScheme rdf:resource="http://purl.org/heritagedata/schemes/571"/>
    <dc:identifier>http://purl.org/heritagedata/schemes/571/concepts/151594</dc:identifier>
    <dc:issued rdf:datatype="http://www.w3.org/2001/XMLSchema#dateTime">2024-07-01T17:17:33</dc:issued>
    <cc:license rdf:resource="https://www.nationalarchives.gov.uk/doc/open-government-licence/version/3/"/>
    <cc:attributionURL rdf:resource="https://historicengland.org.uk/"/>
    <cc:attributionName xml:lang="en">Historic England</cc:attributionName>
    <dc:publisher rdf:resource="https://historicengland.org.uk/"/>
    <dc:spatial rdf:resource="http://vocab.getty.edu/tgn/7002445"/>
    <dc:spatial rdf:resource="http://dbpedia.org/resource/England"/>
    <skos:prefLabel xml:lang="en">Replanted Woodland</skos:prefLabel>
    <skos:related rdf:resource="http://purl.org/heritagedata/schemes/571/concepts/151245"/>
    <skos:scopeNote xml:lang="en">A woodland that has had its original tree coverage felled and replaced with new trees, often coniferous.</skos:scopeNote>
  </skos:Concept>

  <skos:Concept rdf:about="http://purl.org/heritagedata/schemes/571/concepts/151280">
    <skos:broader rdf:resource="http://purl.org/heritagedata/schemes/571/concepts/151448"/>
    <skos:narrower>
      <skos:Concept rdf:about="http://purl.org/heritagedata/schemes/571/concepts/151587">
        <skos:broader rdf:resource="http://purl.org/heritagedata/schemes/571/concepts/151280"/>
        <skos:inScheme rdf:resource="http://purl.org/heritagedata/schemes/571"/>
        <dc:identifier>http://purl.org/heritagedata/schemes/571/concepts/151587</dc:identifier>
        <dc:issued rdf:datatype="http://www.w3.org/2001/XMLSchema#dateTime">2024-07-01T17:17:33</dc:issued>
        <cc:license rdf:resource="https://www.nationalarchives.gov.uk/doc/open-government-licence/version/3/"/>
        <cc:attributionURL rdf:resource="https://historicengland.org.uk/"/>
        <cc:attributionName xml:lang="en">Historic England</cc:attributionName>
        <dc:publisher rdf:resource="https://historicengland.org.uk/"/>
        <dc:spatial rdf:resource="http://vocab.getty.edu/tgn/7002445"/>
        <dc:spatial rdf:resource="http://dbpedia.org/resource/England"/>
        <skos:prefLabel xml:lang="en">Secondary Woodland (Broadleaved)</skos:prefLabel>
        <skos:scopeNote xml:lang="en">Secondary woodland whose species are largely broadleaved.</skos:scopeNote>
      </skos:Concept>
    </skos:narrower>

    <skos:narrower>
      <skos:Concept rdf:about="http://purl.org/heritagedata/schemes/571/concepts/151588">
        <skos:broader rdf:resource="http://purl.org/heritagedata/schemes/571/concepts/151280"/>
        <skos:inScheme rdf:resource="http://purl.org/heritagedata/schemes/571"/>
        <dc:identifier>http://purl.org/heritagedata/schemes/571/concepts/151588</dc:identifier>
        <dc:issued rdf:datatype="http://www.w3.org/2001/XMLSchema#dateTime">2024-07-01T17:17:33</dc:issued>
        <cc:license rdf:resource="https://www.nationalarchives.gov.uk/doc/open-government-licence/version/3/"/>
        <cc:attributionURL rdf:resource="https://historicengland.org.uk/"/>
        <cc:attributionName xml:lang="en">Historic England</cc:attributionName>
        <dc:publisher rdf:resource="https://historicengland.org.uk/"/>
        <dc:spatial rdf:resource="http://vocab.getty.edu/tgn/7002445"/>
        <dc:spatial rdf:resource="http://dbpedia.org/resource/England"/>
        <skos:prefLabel xml:lang="en">Secondary Woodland (Coniferous)</skos:prefLabel>
        <skos:scopeNote xml:lang="en">Secondary woodland whose species are largely conifers.</skos:scopeNote>
      </skos:Concept>
    </skos:narrower>

    <skos:narrower>
      <skos:Concept rdf:about="http://purl.org/heritagedata/schemes/571/concepts/151589">
        <skos:broader rdf:resource="http://purl.org/heritagedata/schemes/571/concepts/151280"/>
        <skos:inScheme rdf:resource="http://purl.org/heritagedata/schemes/571"/>
        <dc:identifier>http://purl.org/heritagedata/schemes/571/concepts/151589</dc:identifier>
        <dc:issued rdf:datatype="http://www.w3.org/2001/XMLSchema#dateTime">2024-07-01T17:17:33</dc:issued>
        <cc:license rdf:resource="https://www.nationalarchives.gov.uk/doc/open-government-licence/version/3/"/>
        <cc:attributionURL rdf:resource="https://historicengland.org.uk/"/>
        <cc:attributionName xml:lang="en">Historic England</cc:attributionName>
        <dc:publisher rdf:resource="https://historicengland.org.uk/"/>
        <dc:spatial rdf:resource="http://vocab.getty.edu/tgn/7002445"/>
        <dc:spatial rdf:resource="http://dbpedia.org/resource/England"/>
        <skos:prefLabel xml:lang="en">Secondary Woodland (Mixed)</skos:prefLabel>
        <skos:scopeNote xml:lang="en">Secondary woodland whose species are a mix of broadleaved and coniferous trees.</skos:scopeNote>
      </skos:Concept>
    </skos:narrower>

    <skos:inScheme rdf:resource="http://purl.org/heritagedata/schemes/571"/>
    <dc:identifier>http://purl.org/heritagedata/schemes/571/concepts/151280</dc:identifier>
    <dc:issued rdf:datatype="http://www.w3.org/2001/XMLSchema#dateTime">2024-07-01T17:17:33</dc:issued>
    <cc:license rdf:resource="https://www.nationalarchives.gov.uk/doc/open-government-licence/version/3/"/>
    <cc:attributionURL rdf:resource="https://historicengland.org.uk/"/>
    <cc:attributionName xml:lang="en">Historic England</cc:attributionName>
    <dc:publisher rdf:resource="https://historicengland.org.uk/"/>
    <dc:spatial rdf:resource="http://vocab.getty.edu/tgn/7002445"/>
    <dc:spatial rdf:resource="http://dbpedia.org/resource/England"/>
    <skos:prefLabel xml:lang="en">Secondary Woodland</skos:prefLabel>
    <skos:scopeNote xml:lang="en">Woodland that has developed, usually by natural colonization, on land formerly used for other purposes (agriculture, settlement, industry etc). If this process pre-dated 1600, secondary woodland can be classified as ancient woodland.</skos:scopeNote>
  </skos:Concept>

  <skos:Concept rdf:about="http://purl.org/heritagedata/schemes/571/concepts/151281">
    <skos:broader rdf:resource="http://purl.org/heritagedata/schemes/571/concepts/151282"/>
    <skos:broader rdf:resource="http://purl.org/heritagedata/schemes/571/concepts/151727"/>
    <skos:inScheme rdf:resource="http://purl.org/heritagedata/schemes/571"/>
    <dc:identifier>http://purl.org/heritagedata/schemes/571/concepts/151281</dc:identifier>
    <dc:issued rdf:datatype="http://www.w3.org/2001/XMLSchema#dateTime">2024-07-01T17:17:33</dc:issued>
    <cc:license rdf:resource="https://www.nationalarchives.gov.uk/doc/open-government-licence/version/3/"/>
    <cc:attributionURL rdf:resource="https://historicengland.org.uk/"/>
    <cc:attributionName xml:lang="en">Historic England</cc:attributionName>
    <dc:publisher rdf:resource="https://historicengland.org.uk/"/>
    <dc:spatial rdf:resource="http://vocab.getty.edu/tgn/7002445"/>
    <dc:spatial rdf:resource="http://dbpedia.org/resource/England"/>
    <skos:prefLabel xml:lang="en">Allotments</skos:prefLabel>
    <skos:related rdf:resource="http://purl.org/heritagedata/schemes/571/concepts/160163"/>
    <skos:related rdf:resource="http://purl.org/heritagedata/schemes/571/concepts/160166"/>
    <skos:scopeNote xml:lang="en">Land, often public, let out to individuals or an individual for the purposes of cultivation or other land use. Often in numerous small parcels, sometimes individually fenced.</skos:scopeNote>
  </skos:Concept>

  <skos:Concept rdf:about="http://purl.org/heritagedata/schemes/571/concepts/151282">
    <skos:narrower rdf:resource="http://purl.org/heritagedata/schemes/571/concepts/151281"/>
    <skos:narrower>
      <skos:Concept rdf:about="http://purl.org/heritagedata/schemes/571/concepts/151284">
        <skos:broader rdf:resource="http://purl.org/heritagedata/schemes/571/concepts/151282"/>
        <skos:inScheme rdf:resource="http://purl.org/heritagedata/schemes/571"/>
        <dc:identifier>http://purl.org/heritagedata/schemes/571/concepts/151284</dc:identifier>
        <dc:issued rdf:datatype="http://www.w3.org/2001/XMLSchema#dateTime">2024-07-01T17:17:33</dc:issued>
        <cc:license rdf:resource="https://www.nationalarchives.gov.uk/doc/open-government-licence/version/3/"/>
        <cc:attributionURL rdf:resource="https://historicengland.org.uk/"/>
        <cc:attributionName xml:lang="en">Historic England</cc:attributionName>
        <dc:publisher rdf:resource="https://historicengland.org.uk/"/>
        <dc:spatial rdf:resource="http://vocab.getty.edu/tgn/7002445"/>
        <dc:spatial rdf:resource="http://dbpedia.org/resource/England"/>
        <skos:prefLabel xml:lang="en">Vegetable Garden</skos:prefLabel>
        <skos:scopeNote xml:lang="en">A garden devoted to the growth of vegetables, for either domestic use or sale.</skos:scopeNote>
      </skos:Concept>
    </skos:narrower>

    <skos:broader rdf:resource="http://purl.org/heritagedata/schemes/571/concepts/151751"/>
    <skos:inScheme rdf:resource="http://purl.org/heritagedata/schemes/571"/>
    <dc:identifier>http://purl.org/heritagedata/schemes/571/concepts/151282</dc:identifier>
    <dc:issued rdf:datatype="http://www.w3.org/2001/XMLSchema#dateTime">2024-07-01T17:17:33</dc:issued>
    <cc:license rdf:resource="https://www.nationalarchives.gov.uk/doc/open-government-licence/version/3/"/>
    <cc:attributionURL rdf:resource="https://historicengland.org.uk/"/>
    <cc:attributionName xml:lang="en">Historic England</cc:attributionName>
    <dc:publisher rdf:resource="https://historicengland.org.uk/"/>
    <dc:spatial rdf:resource="http://vocab.getty.edu/tgn/7002445"/>
    <dc:spatial rdf:resource="http://dbpedia.org/resource/England"/>
    <skos:prefLabel xml:lang="en">Market Garden</skos:prefLabel>
    <skos:related rdf:resource="http://purl.org/heritagedata/schemes/571/concepts/151285"/>
    <skos:scopeNote xml:lang="en">An area of land used to grow vegetables, fruit and flowers to be sold at markets.</skos:scopeNote>
  </skos:Concept>

  <skos:Concept rdf:about="http://purl.org/heritagedata/schemes/571/concepts/151751">
    <skos:narrower rdf:resource="http://purl.org/heritagedata/schemes/571/concepts/151282"/>
    <skos:narrower>
      <skos:Concept rdf:about="http://purl.org/heritagedata/schemes/571/concepts/151283">
        <skos:broader rdf:resource="http://purl.org/heritagedata/schemes/571/concepts/151751"/>
        <skos:inScheme rdf:resource="http://purl.org/heritagedata/schemes/571"/>
        <dc:identifier>http://purl.org/heritagedata/schemes/571/concepts/151283</dc:identifier>
        <dc:issued rdf:datatype="http://www.w3.org/2001/XMLSchema#dateTime">2024-07-01T17:17:33</dc:issued>
        <cc:license rdf:resource="https://www.nationalarchives.gov.uk/doc/open-government-licence/version/3/"/>
        <cc:attributionURL rdf:resource="https://historicengland.org.uk/"/>
        <cc:attributionName xml:lang="en">Historic England</cc:attributionName>
        <dc:publisher rdf:resource="https://historicengland.org.uk/"/>
        <dc:spatial rdf:resource="http://vocab.getty.edu/tgn/7002445"/>
        <dc:spatial rdf:resource="http://dbpedia.org/resource/England"/>
        <skos:prefLabel xml:lang="en">Nursery</skos:prefLabel>
        <skos:scopeNote xml:lang="en">An area such as a commercial garden where plants and trees are grown and nurtured for the purpose of transportation or sale.</skos:scopeNote>
      </skos:Concept>
    </skos:narrower>

    <skos:narrower>
      <skos:Concept rdf:about="http://purl.org/heritagedata/schemes/571/concepts/151286">
        <skos:broader rdf:resource="http://purl.org/heritagedata/schemes/571/concepts/151751"/>
        <skos:inScheme rdf:resource="http://purl.org/heritagedata/schemes/571"/>
        <dc:identifier>http://purl.org/heritagedata/schemes/571/concepts/151286</dc:identifier>
        <dc:issued rdf:datatype="http://www.w3.org/2001/XMLSchema#dateTime">2024-07-01T17:17:33</dc:issued>
        <cc:license rdf:resource="https://www.nationalarchives.gov.uk/doc/open-government-licence/version/3/"/>
        <cc:attributionURL rdf:resource="https://historicengland.org.uk/"/>
        <cc:attributionName xml:lang="en">Historic England</cc:attributionName>
        <dc:publisher rdf:resource="https://historicengland.org.uk/"/>
        <dc:spatial rdf:resource="http://vocab.getty.edu/tgn/7002445"/>
        <dc:spatial rdf:resource="http://dbpedia.org/resource/England"/>
        <skos:prefLabel xml:lang="en">Kitchen Garden</skos:prefLabel>
        <skos:scopeNote xml:lang="en">A private garden established primarily for growing vegetables and soft and bush fruit for domestic consumption.</skos:scopeNote>
      </skos:Concept>
    </skos:narrower>

    <skos:narrower>
      <skos:Concept rdf:about="http://purl.org/heritagedata/schemes/571/concepts/151754">
        <skos:broader rdf:resource="http://purl.org/heritagedata/schemes/571/concepts/151751"/>
        <skos:inScheme rdf:resource="http://purl.org/heritagedata/schemes/571"/>
        <dc:identifier>http://purl.org/heritagedata/schemes/571/concepts/151754</dc:identifier>
        <dc:issued rdf:datatype="http://www.w3.org/2001/XMLSchema#dateTime">2024-07-01T17:17:33</dc:issued>
        <cc:license rdf:resource="https://www.nationalarchives.gov.uk/doc/open-government-licence/version/3/"/>
        <cc:attributionURL rdf:resource="https://historicengland.org.uk/"/>
        <cc:attributionName xml:lang="en">Historic England</cc:attributionName>
        <dc:publisher rdf:resource="https://historicengland.org.uk/"/>
        <dc:spatial rdf:resource="http://vocab.getty.edu/tgn/7002445"/>
        <dc:spatial rdf:resource="http://dbpedia.org/resource/England"/>
        <skos:prefLabel xml:lang="en">Hop Garden</skos:prefLabel>
        <skos:scopeNote xml:lang="en">A piece of land used for the cultivation of hops.</skos:scopeNote>
      </skos:Concept>
    </skos:narrower>

    <skos:narrower>
      <skos:Concept rdf:about="http://purl.org/heritagedata/schemes/571/concepts/151755">
        <skos:broader rdf:resource="http://purl.org/heritagedata/schemes/571/concepts/151751"/>
        <skos:inScheme rdf:resource="http://purl.org/heritagedata/schemes/571"/>
        <dc:identifier>http://purl.org/heritagedata/schemes/571/concepts/151755</dc:identifier>
        <dc:issued rdf:datatype="http://www.w3.org/2001/XMLSchema#dateTime">2024-07-01T17:17:33</dc:issued>
        <cc:license rdf:resource="https://www.nationalarchives.gov.uk/doc/open-government-licence/version/3/"/>
        <cc:attributionURL rdf:resource="https://historicengland.org.uk/"/>
        <cc:attributionName xml:lang="en">Historic England</cc:attributionName>
        <dc:publisher rdf:resource="https://historicengland.org.uk/"/>
        <dc:spatial rdf:resource="http://vocab.getty.edu/tgn/7002445"/>
        <dc:spatial rdf:resource="http://dbpedia.org/resource/England"/>
        <skos:prefLabel xml:lang="en">Garden (Recreational)</skos:prefLabel>
        <skos:scopeNote xml:lang="en">An enclosed piece of ground devoted to recreational purposes.</skos:scopeNote>
      </skos:Concept>
    </skos:narrower>

    <skos:broader rdf:resource="http://purl.org/heritagedata/schemes/571/concepts/151451"/>
    <skos:inScheme rdf:resource="http://purl.org/heritagedata/schemes/571"/>
    <dc:identifier>http://purl.org/heritagedata/schemes/571/concepts/151751</dc:identifier>
    <dc:issued rdf:datatype="http://www.w3.org/2001/XMLSchema#dateTime">2024-07-01T17:17:33</dc:issued>
    <cc:license rdf:resource="https://www.nationalarchives.gov.uk/doc/open-government-licence/version/3/"/>
    <cc:attributionURL rdf:resource="https://historicengland.org.uk/"/>
    <cc:attributionName xml:lang="en">Historic England</cc:attributionName>
    <dc:publisher rdf:resource="https://historicengland.org.uk/"/>
    <dc:spatial rdf:resource="http://vocab.getty.edu/tgn/7002445"/>
    <dc:spatial rdf:resource="http://dbpedia.org/resource/England"/>
    <skos:prefLabel xml:lang="en">Garden</skos:prefLabel>
    <skos:scopeNote xml:lang="en">An enclosed piece of ground devoted to the cultivation of flowers, fruit or vegetables for domestic use.</skos:scopeNote>
  </skos:Concept>

  <skos:Concept rdf:about="http://purl.org/heritagedata/schemes/571/concepts/151285">
    <skos:broader rdf:resource="http://purl.org/heritagedata/schemes/571/concepts/151451"/>
    <skos:inScheme rdf:resource="http://purl.org/heritagedata/schemes/571"/>
    <dc:identifier>http://purl.org/heritagedata/schemes/571/concepts/151285</dc:identifier>
    <dc:issued rdf:datatype="http://www.w3.org/2001/XMLSchema#dateTime">2024-07-01T17:17:33</dc:issued>
    <cc:license rdf:resource="https://www.nationalarchives.gov.uk/doc/open-government-licence/version/3/"/>
    <cc:attributionURL rdf:resource="https://historicengland.org.uk/"/>
    <cc:attributionName xml:lang="en">Historic England</cc:attributionName>
    <dc:publisher rdf:resource="https://historicengland.org.uk/"/>
    <dc:spatial rdf:resource="http://vocab.getty.edu/tgn/7002445"/>
    <dc:spatial rdf:resource="http://dbpedia.org/resource/England"/>
    <skos:prefLabel xml:lang="en">Glasshouses</skos:prefLabel>
    <skos:related rdf:resource="http://purl.org/heritagedata/schemes/571/concepts/151282"/>
    <skos:scopeNote xml:lang="en">Buildings made chiefly of glass, in which plants and fruit are germinated, brought on and sometimes grown to maturity. Often grouped on land with a favourable aspect.</skos:scopeNote>
  </skos:Concept>

  <skos:Concept rdf:about="http://purl.org/heritagedata/schemes/571/concepts/151287">
    <skos:broader rdf:resource="http://purl.org/heritagedata/schemes/571/concepts/151452"/>
    <skos:inScheme rdf:resource="http://purl.org/heritagedata/schemes/571"/>
    <dc:identifier>http://purl.org/heritagedata/schemes/571/concepts/151287</dc:identifier>
    <dc:issued rdf:datatype="http://www.w3.org/2001/XMLSchema#dateTime">2024-07-01T17:17:33</dc:issued>
    <cc:license rdf:resource="https://www.nationalarchives.gov.uk/doc/open-government-licence/version/3/"/>
    <cc:attributionURL rdf:resource="https://historicengland.org.uk/"/>
    <cc:attributionName xml:lang="en">Historic England</cc:attributionName>
    <dc:publisher rdf:resource="https://historicengland.org.uk/"/>
    <dc:spatial rdf:resource="http://vocab.getty.edu/tgn/7002445"/>
    <dc:spatial rdf:resource="http://dbpedia.org/resource/England"/>
    <skos:prefLabel xml:lang="en">Ornamental Waterbody</skos:prefLabel>
    <skos:related rdf:resource="http://purl.org/heritagedata/schemes/571/concepts/151600"/>
    <skos:scopeNote xml:lang="en">An artificial lake or pond, often made by damming a stream, whose main function is to catch the eye and to contribute to ornamentally designed landscapes. As such a common feature of landscape parks.</skos:scopeNote>
  </skos:Concept>

  <skos:Concept rdf:about="http://purl.org/heritagedata/schemes/571/concepts/151452">
    <skos:narrower rdf:resource="http://purl.org/heritagedata/schemes/571/concepts/151287"/>
    <skos:narrower rdf:resource="http://purl.org/heritagedata/schemes/571/concepts/151409"/>
    <skos:narrower rdf:resource="http://purl.org/heritagedata/schemes/571/concepts/151598"/>
    <skos:narrower rdf:resource="http://purl.org/heritagedata/schemes/571/concepts/151599"/>
    <skos:narrower rdf:resource="http://purl.org/heritagedata/schemes/571/concepts/151756"/>
    <skos:narrower rdf:resource="http://purl.org/heritagedata/schemes/571/concepts/160197"/>
    <skos:inScheme rdf:resource="http://purl.org/heritagedata/schemes/571"/>
    <dc:identifier>http://purl.org/heritagedata/schemes/571/concepts/151452</dc:identifier>
    <dc:issued rdf:datatype="http://www.w3.org/2001/XMLSchema#dateTime">2024-07-01T17:17:33</dc:issued>
    <cc:license rdf:resource="https://www.nationalarchives.gov.uk/doc/open-government-licence/version/3/"/>
    <cc:attributionURL rdf:resource="https://historicengland.org.uk/"/>
    <cc:attributionName xml:lang="en">Historic England</cc:attributionName>
    <dc:publisher rdf:resource="https://historicengland.org.uk/"/>
    <dc:spatial rdf:resource="http://vocab.getty.edu/tgn/7002445"/>
    <dc:spatial rdf:resource="http://dbpedia.org/resource/England"/>
    <skos:prefLabel xml:lang="en">Ornamentation</skos:prefLabel>
    <skos:scopeNote xml:lang="en">-</skos:scopeNote>
    <skos:topConceptOf rdf:resource="http://purl.org/heritagedata/schemes/571"/>
  </skos:Concept>

  <skos:Concept rdf:about="http://purl.org/heritagedata/schemes/571/concepts/151295">
    <skos:broader rdf:resource="http://purl.org/heritagedata/schemes/571/concepts/151446"/>
    <skos:narrower rdf:resource="http://purl.org/heritagedata/schemes/571/concepts/151421"/>
    <skos:narrower rdf:resource="http://purl.org/heritagedata/schemes/571/concepts/151596"/>
    <skos:narrower rdf:resource="http://purl.org/heritagedata/schemes/571/concepts/151597"/>
    <skos:inScheme rdf:resource="http://purl.org/heritagedata/schemes/571"/>
    <dc:identifier>http://purl.org/heritagedata/schemes/571/concepts/151295</dc:identifier>
    <dc:issued rdf:datatype="http://www.w3.org/2001/XMLSchema#dateTime">2024-07-01T17:17:33</dc:issued>
    <cc:license rdf:resource="https://www.nationalarchives.gov.uk/doc/open-government-licence/version/3/"/>
    <cc:attributionURL rdf:resource="https://historicengland.org.uk/"/>
    <cc:attributionName xml:lang="en">Historic England</cc:attributionName>
    <dc:publisher rdf:resource="https://historicengland.org.uk/"/>
    <dc:spatial rdf:resource="http://vocab.getty.edu/tgn/7002445"/>
    <dc:spatial rdf:resource="http://dbpedia.org/resource/England"/>
    <skos:prefLabel xml:lang="en">Nucleated Settlement</skos:prefLabel>
    <skos:scopeNote xml:lang="en">Rural settlement in which  farmsteads are typically clustered together, normally as villages (and especially in the central province), but also as hamlets. Can also refer to a single nucleated settlement.</skos:scopeNote>
  </skos:Concept>

  <skos:Concept rdf:about="http://purl.org/heritagedata/schemes/571/concepts/151296">
    <skos:broader rdf:resource="http://purl.org/heritagedata/schemes/571/concepts/160427"/>
    <skos:inScheme rdf:resource="http://purl.org/heritagedata/schemes/571"/>
    <dc:identifier>http://purl.org/heritagedata/schemes/571/concepts/151296</dc:identifier>
    <dc:issued rdf:datatype="http://www.w3.org/2001/XMLSchema#dateTime">2024-07-01T17:17:33</dc:issued>
    <cc:license rdf:resource="https://www.nationalarchives.gov.uk/doc/open-government-licence/version/3/"/>
    <cc:attributionURL rdf:resource="https://historicengland.org.uk/"/>
    <cc:attributionName xml:lang="en">Historic England</cc:attributionName>
    <dc:publisher rdf:resource="https://historicengland.org.uk/"/>
    <dc:spatial rdf:resource="http://vocab.getty.edu/tgn/7002445"/>
    <dc:spatial rdf:resource="http://dbpedia.org/resource/England"/>
    <skos:prefLabel xml:lang="en">Farmstead</skos:prefLabel>
    <skos:scopeNote xml:lang="en">A farmhouse and ancillary farm buildings forming the operational centre for the surrounding farmland.</skos:scopeNote>
  </skos:Concept>

  <skos:Concept rdf:about="http://purl.org/heritagedata/schemes/571/concepts/160427">
    <skos:narrower rdf:resource="http://purl.org/heritagedata/schemes/571/concepts/151296"/>
    <skos:narrower rdf:resource="http://purl.org/heritagedata/schemes/571/concepts/151297"/>
    <skos:narrower>
      <skos:Concept rdf:about="http://purl.org/heritagedata/schemes/571/concepts/151413">
        <skos:broader rdf:resource="http://purl.org/heritagedata/schemes/571/concepts/160427"/>
        <skos:inScheme rdf:resource="http://purl.org/heritagedata/schemes/571"/>
        <dc:identifier>http://purl.org/heritagedata/schemes/571/concepts/151413</dc:identifier>
        <dc:issued rdf:datatype="http://www.w3.org/2001/XMLSchema#dateTime">2024-07-01T17:17:33</dc:issued>
        <cc:license rdf:resource="https://www.nationalarchives.gov.uk/doc/open-government-licence/version/3/"/>
        <cc:attributionURL rdf:resource="https://historicengland.org.uk/"/>
        <cc:attributionName xml:lang="en">Historic England</cc:attributionName>
        <dc:publisher rdf:resource="https://historicengland.org.uk/"/>
        <dc:spatial rdf:resource="http://vocab.getty.edu/tgn/7002445"/>
        <dc:spatial rdf:resource="http://dbpedia.org/resource/England"/>
        <skos:prefLabel xml:lang="en">Manor Farm</skos:prefLabel>
        <skos:scopeNote xml:lang="en">The home farm of a manor.</skos:scopeNote>
      </skos:Concept>
    </skos:narrower>

    <skos:broader rdf:resource="http://purl.org/heritagedata/schemes/571/concepts/151446"/>
    <skos:inScheme rdf:resource="http://purl.org/heritagedata/schemes/571"/>
    <dc:identifier>http://purl.org/heritagedata/schemes/571/concepts/160427</dc:identifier>
    <dc:issued rdf:datatype="http://www.w3.org/2001/XMLSchema#dateTime">2024-07-01T17:17:33</dc:issued>
    <cc:license rdf:resource="https://www.nationalarchives.gov.uk/doc/open-government-licence/version/3/"/>
    <cc:attributionURL rdf:resource="https://historicengland.org.uk/"/>
    <cc:attributionName xml:lang="en">Historic England</cc:attributionName>
    <dc:publisher rdf:resource="https://historicengland.org.uk/"/>
    <dc:spatial rdf:resource="http://vocab.getty.edu/tgn/7002445"/>
    <dc:spatial rdf:resource="http://dbpedia.org/resource/England"/>
    <skos:prefLabel xml:lang="en">Isolated Farm</skos:prefLabel>
    <skos:scopeNote xml:lang="en">Farmstead with no near neighbours, usually an element of a dispersed settlement pattern.</skos:scopeNote>
  </skos:Concept>

  <skos:Concept rdf:about="http://purl.org/heritagedata/schemes/571/concepts/151297">
    <skos:broader rdf:resource="http://purl.org/heritagedata/schemes/571/concepts/151453"/>
    <skos:broader rdf:resource="http://purl.org/heritagedata/schemes/571/concepts/160427"/>
    <skos:inScheme rdf:resource="http://purl.org/heritagedata/schemes/571"/>
    <dc:identifier>http://purl.org/heritagedata/schemes/571/concepts/151297</dc:identifier>
    <dc:issued rdf:datatype="http://www.w3.org/2001/XMLSchema#dateTime">2024-07-01T17:17:33</dc:issued>
    <cc:license rdf:resource="https://www.nationalarchives.gov.uk/doc/open-government-licence/version/3/"/>
    <cc:attributionURL rdf:resource="https://historicengland.org.uk/"/>
    <cc:attributionName xml:lang="en">Historic England</cc:attributionName>
    <dc:publisher rdf:resource="https://historicengland.org.uk/"/>
    <dc:spatial rdf:resource="http://vocab.getty.edu/tgn/7002445"/>
    <dc:spatial rdf:resource="http://dbpedia.org/resource/England"/>
    <skos:prefLabel xml:lang="en">Smallholding</skos:prefLabel>
    <skos:scopeNote xml:lang="en">Group of small fields associated with a single small-scale agricultural concern, typically c5 acres in total. Often associated with part-time famring undertaken by families of industrial workers and thus typically post-medieval and modern.</skos:scopeNote>
  </skos:Concept>

  <skos:Concept rdf:about="http://purl.org/heritagedata/schemes/571/concepts/151298">
    <skos:broader rdf:resource="http://purl.org/heritagedata/schemes/571/concepts/151763"/>
    <skos:inScheme rdf:resource="http://purl.org/heritagedata/schemes/571"/>
    <dc:identifier>http://purl.org/heritagedata/schemes/571/concepts/151298</dc:identifier>
    <dc:issued rdf:datatype="http://www.w3.org/2001/XMLSchema#dateTime">2024-07-01T17:17:33</dc:issued>
    <cc:license rdf:resource="https://www.nationalarchives.gov.uk/doc/open-government-licence/version/3/"/>
    <cc:attributionURL rdf:resource="https://historicengland.org.uk/"/>
    <cc:attributionName xml:lang="en">Historic England</cc:attributionName>
    <dc:publisher rdf:resource="https://historicengland.org.uk/"/>
    <dc:spatial rdf:resource="http://vocab.getty.edu/tgn/7002445"/>
    <dc:spatial rdf:resource="http://dbpedia.org/resource/England"/>
    <skos:prefLabel xml:lang="en">Terraced Housing</skos:prefLabel>
    <skos:related rdf:resource="http://purl.org/heritagedata/schemes/571/concepts/163214"/>
    <skos:scopeNote xml:lang="en">Residential area dominated by lines of attached houses, usually planned and built as one unit. Often associated with industrial towns. Sometimes follow earlier patterns, such as those of the fields they overlay.</skos:scopeNote>
  </skos:Concept>

  <skos:Concept rdf:about="http://purl.org/heritagedata/schemes/571/concepts/151763">
    <skos:narrower rdf:resource="http://purl.org/heritagedata/schemes/571/concepts/151298"/>
    <skos:narrower rdf:resource="http://purl.org/heritagedata/schemes/571/concepts/151299"/>
    <skos:narrower rdf:resource="http://purl.org/heritagedata/schemes/571/concepts/151300"/>
    <skos:narrower rdf:resource="http://purl.org/heritagedata/schemes/571/concepts/151301"/>
    <skos:broader rdf:resource="http://purl.org/heritagedata/schemes/571/concepts/151445"/>
    <skos:inScheme rdf:resource="http://purl.org/heritagedata/schemes/571"/>
    <dc:identifier>http://purl.org/heritagedata/schemes/571/concepts/151763</dc:identifier>
    <dc:issued rdf:datatype="http://www.w3.org/2001/XMLSchema#dateTime">2024-07-01T17:17:33</dc:issued>
    <cc:license rdf:resource="https://www.nationalarchives.gov.uk/doc/open-government-licence/version/3/"/>
    <cc:attributionURL rdf:resource="https://historicengland.org.uk/"/>
    <cc:attributionName xml:lang="en">Historic England</cc:attributionName>
    <dc:publisher rdf:resource="https://historicengland.org.uk/"/>
    <dc:spatial rdf:resource="http://vocab.getty.edu/tgn/7002445"/>
    <dc:spatial rdf:resource="http://dbpedia.org/resource/England"/>
    <skos:prefLabel xml:lang="en">Dwelling</skos:prefLabel>
    <skos:scopeNote xml:lang="en">Places of permanent or temporary residence.</skos:scopeNote>
  </skos:Concept>

  <skos:Concept rdf:about="http://purl.org/heritagedata/schemes/571/concepts/151299">
    <skos:broader rdf:resource="http://purl.org/heritagedata/schemes/571/concepts/151763"/>
    <skos:inScheme rdf:resource="http://purl.org/heritagedata/schemes/571"/>
    <dc:identifier>http://purl.org/heritagedata/schemes/571/concepts/151299</dc:identifier>
    <dc:issued rdf:datatype="http://www.w3.org/2001/XMLSchema#dateTime">2024-07-01T17:17:33</dc:issued>
    <cc:license rdf:resource="https://www.nationalarchives.gov.uk/doc/open-government-licence/version/3/"/>
    <cc:attributionURL rdf:resource="https://historicengland.org.uk/"/>
    <cc:attributionName xml:lang="en">Historic England</cc:attributionName>
    <dc:publisher rdf:resource="https://historicengland.org.uk/"/>
    <dc:spatial rdf:resource="http://vocab.getty.edu/tgn/7002445"/>
    <dc:spatial rdf:resource="http://dbpedia.org/resource/England"/>
    <skos:prefLabel xml:lang="en">Semi Detached Housing</skos:prefLabel>
    <skos:related rdf:resource="http://purl.org/heritagedata/schemes/571/concepts/163214"/>
    <skos:scopeNote xml:lang="en">Residential area dominated by houses joined to just one other to form one building.</skos:scopeNote>
  </skos:Concept>

  <skos:Concept rdf:about="http://purl.org/heritagedata/schemes/571/concepts/151300">
    <skos:broader rdf:resource="http://purl.org/heritagedata/schemes/571/concepts/151763"/>
    <skos:inScheme rdf:resource="http://purl.org/heritagedata/schemes/571"/>
    <dc:identifier>http://purl.org/heritagedata/schemes/571/concepts/151300</dc:identifier>
    <dc:issued rdf:datatype="http://www.w3.org/2001/XMLSchema#dateTime">2024-07-01T17:17:33</dc:issued>
    <cc:license rdf:resource="https://www.nationalarchives.gov.uk/doc/open-government-licence/version/3/"/>
    <cc:attributionURL rdf:resource="https://historicengland.org.uk/"/>
    <cc:attributionName xml:lang="en">Historic England</cc:attributionName>
    <dc:publisher rdf:resource="https://historicengland.org.uk/"/>
    <dc:spatial rdf:resource="http://vocab.getty.edu/tgn/7002445"/>
    <dc:spatial rdf:resource="http://dbpedia.org/resource/England"/>
    <skos:prefLabel xml:lang="en">Detached Housing</skos:prefLabel>
    <skos:related rdf:resource="http://purl.org/heritagedata/schemes/571/concepts/163214"/>
    <skos:scopeNote xml:lang="en">Residential area dominated by free-standing houses that are not joined to others on any side.</skos:scopeNote>
  </skos:Concept>

  <skos:Concept rdf:about="http://purl.org/heritagedata/schemes/571/concepts/151301">
    <skos:broader rdf:resource="http://purl.org/heritagedata/schemes/571/concepts/151763"/>
    <skos:inScheme rdf:resource="http://purl.org/heritagedata/schemes/571"/>
    <dc:identifier>http://purl.org/heritagedata/schemes/571/concepts/151301</dc:identifier>
    <dc:issued rdf:datatype="http://www.w3.org/2001/XMLSchema#dateTime">2024-07-01T17:17:33</dc:issued>
    <cc:license rdf:resource="https://www.nationalarchives.gov.uk/doc/open-government-licence/version/3/"/>
    <cc:attributionURL rdf:resource="https://historicengland.org.uk/"/>
    <cc:attributionName xml:lang="en">Historic England</cc:attributionName>
    <dc:publisher rdf:resource="https://historicengland.org.uk/"/>
    <dc:spatial rdf:resource="http://vocab.getty.edu/tgn/7002445"/>
    <dc:spatial rdf:resource="http://dbpedia.org/resource/England"/>
    <skos:prefLabel xml:lang="en">Flats And Apartments</skos:prefLabel>
    <skos:related rdf:resource="http://purl.org/heritagedata/schemes/571/concepts/163214"/>
    <skos:scopeNote xml:lang="en">Residential area dominated by purpose-built tenement buildings, each containing several flats or apartments.</skos:scopeNote>
  </skos:Concept>

  <skos:Concept rdf:about="http://purl.org/heritagedata/schemes/571/concepts/151404">
    <skos:broader rdf:resource="http://purl.org/heritagedata/schemes/571/concepts/151667"/>
    <skos:inScheme rdf:resource="http://purl.org/heritagedata/schemes/571"/>
    <dc:identifier>http://purl.org/heritagedata/schemes/571/concepts/151404</dc:identifier>
    <dc:issued rdf:datatype="http://www.w3.org/2001/XMLSchema#dateTime">2024-07-01T17:17:33</dc:issued>
    <cc:license rdf:resource="https://www.nationalarchives.gov.uk/doc/open-government-licence/version/3/"/>
    <cc:attributionURL rdf:resource="https://historicengland.org.uk/"/>
    <cc:attributionName xml:lang="en">Historic England</cc:attributionName>
    <dc:publisher rdf:resource="https://historicengland.org.uk/"/>
    <dc:spatial rdf:resource="http://vocab.getty.edu/tgn/7002445"/>
    <dc:spatial rdf:resource="http://dbpedia.org/resource/England"/>
    <skos:prefLabel xml:lang="en">Harbour</skos:prefLabel>
    <skos:related rdf:resource="http://purl.org/heritagedata/schemes/571/concepts/152587"/>
    <skos:scopeNote xml:lang="en">An area of the coast where ships can find shelter or safe anchorage. Harbours require features, natural or artificial that provide shelter and a pool area large and deep enough to accommodate vessels at anchor.</skos:scopeNote>
  </skos:Concept>

  <skos:Concept rdf:about="http://purl.org/heritagedata/schemes/571/concepts/151405">
    <skos:broader rdf:resource="http://purl.org/heritagedata/schemes/571/concepts/151667"/>
    <skos:inScheme rdf:resource="http://purl.org/heritagedata/schemes/571"/>
    <dc:identifier>http://purl.org/heritagedata/schemes/571/concepts/151405</dc:identifier>
    <dc:issued rdf:datatype="http://www.w3.org/2001/XMLSchema#dateTime">2024-07-01T17:17:33</dc:issued>
    <cc:license rdf:resource="https://www.nationalarchives.gov.uk/doc/open-government-licence/version/3/"/>
    <cc:attributionURL rdf:resource="https://historicengland.org.uk/"/>
    <cc:attributionName xml:lang="en">Historic England</cc:attributionName>
    <dc:publisher rdf:resource="https://historicengland.org.uk/"/>
    <dc:spatial rdf:resource="http://vocab.getty.edu/tgn/7002445"/>
    <dc:spatial rdf:resource="http://dbpedia.org/resource/England"/>
    <skos:prefLabel xml:lang="en">Wharves</skos:prefLabel>
    <skos:related rdf:resource="http://purl.org/heritagedata/schemes/571/concepts/151096"/>
    <skos:scopeNote xml:lang="en">Large structures built alongside the water's edge where ships may lie for unloading.</skos:scopeNote>
  </skos:Concept>

  <skos:Concept rdf:about="http://purl.org/heritagedata/schemes/571/concepts/151406">
    <skos:broader rdf:resource="http://purl.org/heritagedata/schemes/571/concepts/151656"/>
    <skos:inScheme rdf:resource="http://purl.org/heritagedata/schemes/571"/>
    <dc:identifier>http://purl.org/heritagedata/schemes/571/concepts/151406</dc:identifier>
    <dc:issued rdf:datatype="http://www.w3.org/2001/XMLSchema#dateTime">2024-07-01T17:17:33</dc:issued>
    <cc:license rdf:resource="https://www.nationalarchives.gov.uk/doc/open-government-licence/version/3/"/>
    <cc:attributionURL rdf:resource="https://historicengland.org.uk/"/>
    <cc:attributionName xml:lang="en">Historic England</cc:attributionName>
    <dc:publisher rdf:resource="https://historicengland.org.uk/"/>
    <dc:spatial rdf:resource="http://vocab.getty.edu/tgn/7002445"/>
    <dc:spatial rdf:resource="http://dbpedia.org/resource/England"/>
    <skos:prefLabel xml:lang="en">Telecommunication Complex</skos:prefLabel>
    <skos:scopeNote xml:lang="en">A complex of buildings and other structures (and directly related grounds) used to transmit information via telecommunication systems.</skos:scopeNote>
  </skos:Concept>

  <skos:Concept rdf:about="http://purl.org/heritagedata/schemes/571/concepts/151656">
    <skos:narrower rdf:resource="http://purl.org/heritagedata/schemes/571/concepts/151406"/>
    <skos:narrower rdf:resource="http://purl.org/heritagedata/schemes/571/concepts/151407"/>
    <skos:broader rdf:resource="http://purl.org/heritagedata/schemes/571/concepts/151449"/>
    <skos:inScheme rdf:resource="http://purl.org/heritagedata/schemes/571"/>
    <dc:identifier>http://purl.org/heritagedata/schemes/571/concepts/151656</dc:identifier>
    <dc:issued rdf:datatype="http://www.w3.org/2001/XMLSchema#dateTime">2024-07-01T17:17:33</dc:issued>
    <cc:license rdf:resource="https://www.nationalarchives.gov.uk/doc/open-government-licence/version/3/"/>
    <cc:attributionURL rdf:resource="https://historicengland.org.uk/"/>
    <cc:attributionName xml:lang="en">Historic England</cc:attributionName>
    <dc:publisher rdf:resource="https://historicengland.org.uk/"/>
    <dc:spatial rdf:resource="http://vocab.getty.edu/tgn/7002445"/>
    <dc:spatial rdf:resource="http://dbpedia.org/resource/England"/>
    <skos:prefLabel xml:lang="en">Telecommunication</skos:prefLabel>
    <skos:scopeNote xml:lang="en">Communication of information by wire, radio, electrical and digital means.</skos:scopeNote>
  </skos:Concept>

  <skos:Concept rdf:about="http://purl.org/heritagedata/schemes/571/concepts/151407">
    <skos:broader rdf:resource="http://purl.org/heritagedata/schemes/571/concepts/151656"/>
    <skos:narrower>
      <skos:Concept rdf:about="http://purl.org/heritagedata/schemes/571/concepts/152633">
        <skos:broader rdf:resource="http://purl.org/heritagedata/schemes/571/concepts/151407"/>
        <skos:inScheme rdf:resource="http://purl.org/heritagedata/schemes/571"/>
        <dc:identifier>http://purl.org/heritagedata/schemes/571/concepts/152633</dc:identifier>
        <dc:issued rdf:datatype="http://www.w3.org/2001/XMLSchema#dateTime">2024-07-01T17:17:33</dc:issued>
        <cc:license rdf:resource="https://www.nationalarchives.gov.uk/doc/open-government-licence/version/3/"/>
        <cc:attributionURL rdf:resource="https://historicengland.org.uk/"/>
        <cc:attributionName xml:lang="en">Historic England</cc:attributionName>
        <dc:publisher rdf:resource="https://historicengland.org.uk/"/>
        <dc:spatial rdf:resource="http://vocab.getty.edu/tgn/7002445"/>
        <dc:spatial rdf:resource="http://dbpedia.org/resource/England"/>
        <skos:prefLabel xml:lang="en">Submarine Telecommunication Cable</skos:prefLabel>
        <skos:scopeNote xml:lang="en">Cables laid beneath the sea to carry telecommunications including telephone and internet communications, also historic telegraph systems. The most frequent function of submarine cabling, especially that covering long distances.</skos:scopeNote>
      </skos:Concept>
    </skos:narrower>

    <skos:inScheme rdf:resource="http://purl.org/heritagedata/schemes/571"/>
    <dc:identifier>http://purl.org/heritagedata/schemes/571/concepts/151407</dc:identifier>
    <dc:issued rdf:datatype="http://www.w3.org/2001/XMLSchema#dateTime">2024-07-01T17:17:33</dc:issued>
    <cc:license rdf:resource="https://www.nationalarchives.gov.uk/doc/open-government-licence/version/3/"/>
    <cc:attributionURL rdf:resource="https://historicengland.org.uk/"/>
    <cc:attributionName xml:lang="en">Historic England</cc:attributionName>
    <dc:publisher rdf:resource="https://historicengland.org.uk/"/>
    <dc:spatial rdf:resource="http://vocab.getty.edu/tgn/7002445"/>
    <dc:spatial rdf:resource="http://dbpedia.org/resource/England"/>
    <skos:prefLabel xml:lang="en">Telecommunication Cable</skos:prefLabel>
    <skos:scopeNote xml:lang="en">A terrestrial or submarine insulated cable or pipe along which telecommunication data is passed.</skos:scopeNote>
  </skos:Concept>

  <skos:Concept rdf:about="http://purl.org/heritagedata/schemes/571/concepts/151409">
    <skos:broader rdf:resource="http://purl.org/heritagedata/schemes/571/concepts/151452"/>
    <skos:narrower>
      <skos:Concept rdf:about="http://purl.org/heritagedata/schemes/571/concepts/151757">
        <skos:broader rdf:resource="http://purl.org/heritagedata/schemes/571/concepts/151409"/>
        <skos:inScheme rdf:resource="http://purl.org/heritagedata/schemes/571"/>
        <dc:identifier>http://purl.org/heritagedata/schemes/571/concepts/151757</dc:identifier>
        <dc:issued rdf:datatype="http://www.w3.org/2001/XMLSchema#dateTime">2024-07-01T17:17:33</dc:issued>
        <cc:license rdf:resource="https://www.nationalarchives.gov.uk/doc/open-government-licence/version/3/"/>
        <cc:attributionURL rdf:resource="https://historicengland.org.uk/"/>
        <cc:attributionName xml:lang="en">Historic England</cc:attributionName>
        <dc:publisher rdf:resource="https://historicengland.org.uk/"/>
        <dc:spatial rdf:resource="http://vocab.getty.edu/tgn/7002445"/>
        <dc:spatial rdf:resource="http://dbpedia.org/resource/England"/>
        <skos:prefLabel xml:lang="en">Tree Avenue</skos:prefLabel>
        <skos:scopeNote xml:lang="en">A straight road lined with trees along either side, also straight lines of trees found in parkland usually leading to a landscape feature.</skos:scopeNote>
      </skos:Concept>
    </skos:narrower>

    <skos:inScheme rdf:resource="http://purl.org/heritagedata/schemes/571"/>
    <dc:identifier>http://purl.org/heritagedata/schemes/571/concepts/151409</dc:identifier>
    <dc:issued rdf:datatype="http://www.w3.org/2001/XMLSchema#dateTime">2024-07-01T17:17:33</dc:issued>
    <cc:license rdf:resource="https://www.nationalarchives.gov.uk/doc/open-government-licence/version/3/"/>
    <cc:attributionURL rdf:resource="https://historicengland.org.uk/"/>
    <cc:attributionName xml:lang="en">Historic England</cc:attributionName>
    <dc:publisher rdf:resource="https://historicengland.org.uk/"/>
    <dc:spatial rdf:resource="http://vocab.getty.edu/tgn/7002445"/>
    <dc:spatial rdf:resource="http://dbpedia.org/resource/England"/>
    <skos:prefLabel xml:lang="en">Avenue</skos:prefLabel>
    <skos:related rdf:resource="http://purl.org/heritagedata/schemes/571/concepts/151600"/>
    <skos:scopeNote xml:lang="en">Approach or drive within an aornamentally designed landscape marked by carefully planted trees, sometimes also by banks or walls. Often comprises one or more straight lines with a house or other feature displayed at one end.</skos:scopeNote>
  </skos:Concept>

  <skos:Concept rdf:about="http://purl.org/heritagedata/schemes/571/concepts/151410">
    <skos:broader rdf:resource="http://purl.org/heritagedata/schemes/571/concepts/160252"/>
    <skos:inScheme rdf:resource="http://purl.org/heritagedata/schemes/571"/>
    <dc:identifier>http://purl.org/heritagedata/schemes/571/concepts/151410</dc:identifier>
    <dc:issued rdf:datatype="http://www.w3.org/2001/XMLSchema#dateTime">2024-07-01T17:17:33</dc:issued>
    <cc:license rdf:resource="https://www.nationalarchives.gov.uk/doc/open-government-licence/version/3/"/>
    <cc:attributionURL rdf:resource="https://historicengland.org.uk/"/>
    <cc:attributionName xml:lang="en">Historic England</cc:attributionName>
    <dc:publisher rdf:resource="https://historicengland.org.uk/"/>
    <dc:spatial rdf:resource="http://vocab.getty.edu/tgn/7002445"/>
    <dc:spatial rdf:resource="http://dbpedia.org/resource/England"/>
    <skos:prefLabel xml:lang="en">Aquarium</skos:prefLabel>
    <skos:scopeNote xml:lang="en">An area of buildings, artificial ponds and/or tanks in which aquatic plants and animals are kept for observaton and study as recreation.</skos:scopeNote>
  </skos:Concept>

  <skos:Concept rdf:about="http://purl.org/heritagedata/schemes/571/concepts/160252">
    <skos:narrower rdf:resource="http://purl.org/heritagedata/schemes/571/concepts/151410"/>
    <skos:narrower rdf:resource="http://purl.org/heritagedata/schemes/571/concepts/151604"/>
    <skos:narrower>
      <skos:Concept rdf:about="http://purl.org/heritagedata/schemes/571/concepts/151792">
        <skos:broader rdf:resource="http://purl.org/heritagedata/schemes/571/concepts/160252"/>
        <skos:inScheme rdf:resource="http://purl.org/heritagedata/schemes/571"/>
        <dc:identifier>http://purl.org/heritagedata/schemes/571/concepts/151792</dc:identifier>
        <dc:issued rdf:datatype="http://www.w3.org/2001/XMLSchema#dateTime">2024-07-01T17:17:33</dc:issued>
        <cc:license rdf:resource="https://www.nationalarchives.gov.uk/doc/open-government-licence/version/3/"/>
        <cc:attributionURL rdf:resource="https://historicengland.org.uk/"/>
        <cc:attributionName xml:lang="en">Historic England</cc:attributionName>
        <dc:publisher rdf:resource="https://historicengland.org.uk/"/>
        <dc:spatial rdf:resource="http://vocab.getty.edu/tgn/7002445"/>
        <dc:spatial rdf:resource="http://dbpedia.org/resource/England"/>
        <skos:prefLabel xml:lang="en">Cinema</skos:prefLabel>
        <skos:scopeNote xml:lang="en">A building where people pay to see films and 'moving pictures'.</skos:scopeNote>
      </skos:Concept>
    </skos:narrower>

    <skos:narrower>
      <skos:Concept rdf:about="http://purl.org/heritagedata/schemes/571/concepts/152303">
        <skos:broader rdf:resource="http://purl.org/heritagedata/schemes/571/concepts/160252"/>
        <skos:inScheme rdf:resource="http://purl.org/heritagedata/schemes/571"/>
        <dc:identifier>http://purl.org/heritagedata/schemes/571/concepts/152303</dc:identifier>
        <dc:issued rdf:datatype="http://www.w3.org/2001/XMLSchema#dateTime">2024-07-01T17:17:33</dc:issued>
        <cc:license rdf:resource="https://www.nationalarchives.gov.uk/doc/open-government-licence/version/3/"/>
        <cc:attributionURL rdf:resource="https://historicengland.org.uk/"/>
        <cc:attributionName xml:lang="en">Historic England</cc:attributionName>
        <dc:publisher rdf:resource="https://historicengland.org.uk/"/>
        <dc:spatial rdf:resource="http://vocab.getty.edu/tgn/7002445"/>
        <dc:spatial rdf:resource="http://dbpedia.org/resource/England"/>
        <skos:prefLabel xml:lang="en">Leisure Centre</skos:prefLabel>
        <skos:scopeNote xml:lang="en">A purpose built building and associated grounds, usually owned and operated by a local authority, where people go to keep fit or relax through using the facilities.</skos:scopeNote>
      </skos:Concept>
    </skos:narrower>

    <skos:narrower>
      <skos:Concept rdf:about="http://purl.org/heritagedata/schemes/571/concepts/152311">
        <skos:broader rdf:resource="http://purl.org/heritagedata/schemes/571/concepts/160252"/>
        <skos:inScheme rdf:resource="http://purl.org/heritagedata/schemes/571"/>
        <dc:identifier>http://purl.org/heritagedata/schemes/571/concepts/152311</dc:identifier>
        <dc:issued rdf:datatype="http://www.w3.org/2001/XMLSchema#dateTime">2024-07-01T17:17:33</dc:issued>
        <cc:license rdf:resource="https://www.nationalarchives.gov.uk/doc/open-government-licence/version/3/"/>
        <cc:attributionURL rdf:resource="https://historicengland.org.uk/"/>
        <cc:attributionName xml:lang="en">Historic England</cc:attributionName>
        <dc:publisher rdf:resource="https://historicengland.org.uk/"/>
        <dc:spatial rdf:resource="http://vocab.getty.edu/tgn/7002445"/>
        <dc:spatial rdf:resource="http://dbpedia.org/resource/England"/>
        <skos:prefLabel xml:lang="en">Amusements</skos:prefLabel>
        <skos:scopeNote xml:lang="en">An area or place for recreation, typically with electronic game machines and gambling machines.</skos:scopeNote>
      </skos:Concept>
    </skos:narrower>

    <skos:broader rdf:resource="http://purl.org/heritagedata/schemes/571/concepts/160285"/>
    <skos:inScheme rdf:resource="http://purl.org/heritagedata/schemes/571"/>
    <dc:identifier>http://purl.org/heritagedata/schemes/571/concepts/160252</dc:identifier>
    <dc:issued rdf:datatype="http://www.w3.org/2001/XMLSchema#dateTime">2024-07-01T17:17:33</dc:issued>
    <cc:license rdf:resource="https://www.nationalarchives.gov.uk/doc/open-government-licence/version/3/"/>
    <cc:attributionURL rdf:resource="https://historicengland.org.uk/"/>
    <cc:attributionName xml:lang="en">Historic England</cc:attributionName>
    <dc:publisher rdf:resource="https://historicengland.org.uk/"/>
    <dc:spatial rdf:resource="http://vocab.getty.edu/tgn/7002445"/>
    <dc:spatial rdf:resource="http://dbpedia.org/resource/England"/>
    <skos:prefLabel xml:lang="en">Indoor Recreation</skos:prefLabel>
    <skos:scopeNote xml:lang="en">Facilities provided for indoor recreation, often with external grounds associated (car parks etc).</skos:scopeNote>
  </skos:Concept>

  <skos:Concept rdf:about="http://purl.org/heritagedata/schemes/571/concepts/151411">
    <skos:broader rdf:resource="http://purl.org/heritagedata/schemes/571/concepts/151775"/>
    <skos:inScheme rdf:resource="http://purl.org/heritagedata/schemes/571"/>
    <dc:identifier>http://purl.org/heritagedata/schemes/571/concepts/151411</dc:identifier>
    <dc:issued rdf:datatype="http://www.w3.org/2001/XMLSchema#dateTime">2024-07-01T17:17:33</dc:issued>
    <cc:license rdf:resource="https://www.nationalarchives.gov.uk/doc/open-government-licence/version/3/"/>
    <cc:attributionURL rdf:resource="https://historicengland.org.uk/"/>
    <cc:attributionName xml:lang="en">Historic England</cc:attributionName>
    <dc:publisher rdf:resource="https://historicengland.org.uk/"/>
    <dc:spatial rdf:resource="http://vocab.getty.edu/tgn/7002445"/>
    <dc:spatial rdf:resource="http://dbpedia.org/resource/England"/>
    <skos:prefLabel xml:lang="en">Country House</skos:prefLabel>
    <skos:related rdf:resource="http://purl.org/heritagedata/schemes/571/concepts/151420"/>
    <skos:scopeNote xml:lang="en">Gentry house in a rural setting, normally within a landscape park, and usually accompanied by a range of attached and detached offices, yards, etc.</skos:scopeNote>
  </skos:Concept>

  <skos:Concept rdf:about="http://purl.org/heritagedata/schemes/571/concepts/151775">
    <skos:narrower rdf:resource="http://purl.org/heritagedata/schemes/571/concepts/151411"/>
    <skos:broader rdf:resource="http://purl.org/heritagedata/schemes/571/concepts/160426"/>
    <skos:inScheme rdf:resource="http://purl.org/heritagedata/schemes/571"/>
    <dc:identifier>http://purl.org/heritagedata/schemes/571/concepts/151775</dc:identifier>
    <dc:issued rdf:datatype="http://www.w3.org/2001/XMLSchema#dateTime">2024-07-01T17:17:33</dc:issued>
    <cc:license rdf:resource="https://www.nationalarchives.gov.uk/doc/open-government-licence/version/3/"/>
    <cc:attributionURL rdf:resource="https://historicengland.org.uk/"/>
    <cc:attributionName xml:lang="en">Historic England</cc:attributionName>
    <dc:publisher rdf:resource="https://historicengland.org.uk/"/>
    <dc:spatial rdf:resource="http://vocab.getty.edu/tgn/7002445"/>
    <dc:spatial rdf:resource="http://dbpedia.org/resource/England"/>
    <skos:prefLabel xml:lang="en">House</skos:prefLabel>
    <skos:scopeNote xml:lang="en">A dwelling with its immediately associated enclosures (yards, etc).</skos:scopeNote>
  </skos:Concept>

  <skos:Concept rdf:about="http://purl.org/heritagedata/schemes/571/concepts/151412">
    <skos:broader rdf:resource="http://purl.org/heritagedata/schemes/571/concepts/160426"/>
    <skos:inScheme rdf:resource="http://purl.org/heritagedata/schemes/571"/>
    <dc:identifier>http://purl.org/heritagedata/schemes/571/concepts/151412</dc:identifier>
    <dc:issued rdf:datatype="http://www.w3.org/2001/XMLSchema#dateTime">2024-07-01T17:17:33</dc:issued>
    <cc:license rdf:resource="https://www.nationalarchives.gov.uk/doc/open-government-licence/version/3/"/>
    <cc:attributionURL rdf:resource="https://historicengland.org.uk/"/>
    <cc:attributionName xml:lang="en">Historic England</cc:attributionName>
    <dc:publisher rdf:resource="https://historicengland.org.uk/"/>
    <dc:spatial rdf:resource="http://vocab.getty.edu/tgn/7002445"/>
    <dc:spatial rdf:resource="http://dbpedia.org/resource/England"/>
    <skos:prefLabel xml:lang="en">Hunting Lodge</skos:prefLabel>
    <skos:scopeNote xml:lang="en">A weekend retreat for parties and others, when hunting in the deer park or forests, or as a viewing station for the chase.</skos:scopeNote>
  </skos:Concept>

  <skos:Concept rdf:about="http://purl.org/heritagedata/schemes/571/concepts/160426">
    <skos:narrower rdf:resource="http://purl.org/heritagedata/schemes/571/concepts/151412"/>
    <skos:narrower rdf:resource="http://purl.org/heritagedata/schemes/571/concepts/151420"/>
    <skos:narrower rdf:resource="http://purl.org/heritagedata/schemes/571/concepts/151775"/>
    <skos:broader rdf:resource="http://purl.org/heritagedata/schemes/571/concepts/151446"/>
    <skos:inScheme rdf:resource="http://purl.org/heritagedata/schemes/571"/>
    <dc:identifier>http://purl.org/heritagedata/schemes/571/concepts/160426</dc:identifier>
    <dc:issued rdf:datatype="http://www.w3.org/2001/XMLSchema#dateTime">2024-07-01T17:17:33</dc:issued>
    <cc:license rdf:resource="https://www.nationalarchives.gov.uk/doc/open-government-licence/version/3/"/>
    <cc:attributionURL rdf:resource="https://historicengland.org.uk/"/>
    <cc:attributionName xml:lang="en">Historic England</cc:attributionName>
    <dc:publisher rdf:resource="https://historicengland.org.uk/"/>
    <dc:spatial rdf:resource="http://vocab.getty.edu/tgn/7002445"/>
    <dc:spatial rdf:resource="http://dbpedia.org/resource/England"/>
    <skos:prefLabel xml:lang="en">Isolated Dwelling</skos:prefLabel>
    <skos:scopeNote xml:lang="en">Rural residence with no immediate neighbours.</skos:scopeNote>
  </skos:Concept>

  <skos:Concept rdf:about="http://purl.org/heritagedata/schemes/571/concepts/151416">
    <skos:broader rdf:resource="http://purl.org/heritagedata/schemes/571/concepts/151443"/>
    <skos:broader rdf:resource="http://purl.org/heritagedata/schemes/571/concepts/152326"/>
    <skos:inScheme rdf:resource="http://purl.org/heritagedata/schemes/571"/>
    <dc:identifier>http://purl.org/heritagedata/schemes/571/concepts/151416</dc:identifier>
    <dc:issued rdf:datatype="http://www.w3.org/2001/XMLSchema#dateTime">2024-07-01T17:17:33</dc:issued>
    <cc:license rdf:resource="https://www.nationalarchives.gov.uk/doc/open-government-licence/version/3/"/>
    <cc:attributionURL rdf:resource="https://historicengland.org.uk/"/>
    <cc:attributionName xml:lang="en">Historic England</cc:attributionName>
    <dc:publisher rdf:resource="https://historicengland.org.uk/"/>
    <dc:spatial rdf:resource="http://vocab.getty.edu/tgn/7002445"/>
    <dc:spatial rdf:resource="http://dbpedia.org/resource/England"/>
    <skos:prefLabel xml:lang="en">Dunes</skos:prefLabel>
    <skos:scopeNote xml:lang="en">Coastal areas containing hills or ridges of unconsolidated wind-blown sand. Surfaces of ridges and intervening slacks may be stabilised by surface vegetation. Used for rough grazing.</skos:scopeNote>
  </skos:Concept>

  <skos:Concept rdf:about="http://purl.org/heritagedata/schemes/571/concepts/151417">
    <skos:broader rdf:resource="http://purl.org/heritagedata/schemes/571/concepts/151453"/>
    <skos:narrower>
      <skos:Concept rdf:about="http://purl.org/heritagedata/schemes/571/concepts/152602">
        <skos:broader rdf:resource="http://purl.org/heritagedata/schemes/571/concepts/151417"/>
        <skos:inScheme rdf:resource="http://purl.org/heritagedata/schemes/571"/>
        <dc:identifier>http://purl.org/heritagedata/schemes/571/concepts/152602</dc:identifier>
        <dc:issued rdf:datatype="http://www.w3.org/2001/XMLSchema#dateTime">2024-07-01T17:17:33</dc:issued>
        <cc:license rdf:resource="https://www.nationalarchives.gov.uk/doc/open-government-licence/version/3/"/>
        <cc:attributionURL rdf:resource="https://historicengland.org.uk/"/>
        <cc:attributionName xml:lang="en">Historic England</cc:attributionName>
        <dc:publisher rdf:resource="https://historicengland.org.uk/"/>
        <dc:spatial rdf:resource="http://vocab.getty.edu/tgn/7002445"/>
        <dc:spatial rdf:resource="http://dbpedia.org/resource/England"/>
        <skos:prefLabel xml:lang="en">Reclamation From Sea</skos:prefLabel>
        <skos:scopeNote xml:lang="en">Land reclaimed directly from the sea by enclosure and drainage.</skos:scopeNote>
      </skos:Concept>
    </skos:narrower>

    <skos:narrower>
      <skos:Concept rdf:about="http://purl.org/heritagedata/schemes/571/concepts/152603">
        <skos:broader rdf:resource="http://purl.org/heritagedata/schemes/571/concepts/151417"/>
        <skos:inScheme rdf:resource="http://purl.org/heritagedata/schemes/571"/>
        <dc:identifier>http://purl.org/heritagedata/schemes/571/concepts/152603</dc:identifier>
        <dc:issued rdf:datatype="http://www.w3.org/2001/XMLSchema#dateTime">2024-07-01T17:17:33</dc:issued>
        <cc:license rdf:resource="https://www.nationalarchives.gov.uk/doc/open-government-licence/version/3/"/>
        <cc:attributionURL rdf:resource="https://historicengland.org.uk/"/>
        <cc:attributionName xml:lang="en">Historic England</cc:attributionName>
        <dc:publisher rdf:resource="https://historicengland.org.uk/"/>
        <dc:spatial rdf:resource="http://vocab.getty.edu/tgn/7002445"/>
        <dc:spatial rdf:resource="http://dbpedia.org/resource/England"/>
        <skos:prefLabel xml:lang="en">Reclamation From Tidal Marsh</skos:prefLabel>
        <skos:scopeNote xml:lang="en">Land reclaimed directly from tidal marsh, usually salt marsh, by enclosure and drainage.</skos:scopeNote>
      </skos:Concept>
    </skos:narrower>

    <skos:narrower>
      <skos:Concept rdf:about="http://purl.org/heritagedata/schemes/571/concepts/152604">
        <skos:broader rdf:resource="http://purl.org/heritagedata/schemes/571/concepts/151417"/>
        <skos:inScheme rdf:resource="http://purl.org/heritagedata/schemes/571"/>
        <dc:identifier>http://purl.org/heritagedata/schemes/571/concepts/152604</dc:identifier>
        <dc:issued rdf:datatype="http://www.w3.org/2001/XMLSchema#dateTime">2024-07-01T17:17:33</dc:issued>
        <cc:license rdf:resource="https://www.nationalarchives.gov.uk/doc/open-government-licence/version/3/"/>
        <cc:attributionURL rdf:resource="https://historicengland.org.uk/"/>
        <cc:attributionName xml:lang="en">Historic England</cc:attributionName>
        <dc:publisher rdf:resource="https://historicengland.org.uk/"/>
        <dc:spatial rdf:resource="http://vocab.getty.edu/tgn/7002445"/>
        <dc:spatial rdf:resource="http://dbpedia.org/resource/England"/>
        <skos:prefLabel xml:lang="en">Reclamation From Wetland</skos:prefLabel>
        <skos:scopeNote xml:lang="en">Land reclaimed directly from wetland.</skos:scopeNote>
      </skos:Concept>
    </skos:narrower>

    <skos:inScheme rdf:resource="http://purl.org/heritagedata/schemes/571"/>
    <dc:identifier>http://purl.org/heritagedata/schemes/571/concepts/151417</dc:identifier>
    <dc:issued rdf:datatype="http://www.w3.org/2001/XMLSchema#dateTime">2024-07-01T17:17:33</dc:issued>
    <cc:license rdf:resource="https://www.nationalarchives.gov.uk/doc/open-government-licence/version/3/"/>
    <cc:attributionURL rdf:resource="https://historicengland.org.uk/"/>
    <cc:attributionName xml:lang="en">Historic England</cc:attributionName>
    <dc:publisher rdf:resource="https://historicengland.org.uk/"/>
    <dc:spatial rdf:resource="http://vocab.getty.edu/tgn/7002445"/>
    <dc:spatial rdf:resource="http://dbpedia.org/resource/England"/>
    <skos:prefLabel xml:lang="en">Reclaimed Land</skos:prefLabel>
    <skos:scopeNote xml:lang="en">Coastal or other low-lying ground taken in for agriculture, usually by dyking and draining. Some medieval (usually smaller more irregular patterns), but mainly post-medieval and modern (larger, rectilinear, and more regular).</skos:scopeNote>
  </skos:Concept>

  <skos:Concept rdf:about="http://purl.org/heritagedata/schemes/571/concepts/151419">
    <skos:broader rdf:resource="http://purl.org/heritagedata/schemes/571/concepts/151462"/>
    <skos:inScheme rdf:resource="http://purl.org/heritagedata/schemes/571"/>
    <dc:identifier>http://purl.org/heritagedata/schemes/571/concepts/151419</dc:identifier>
    <dc:issued rdf:datatype="http://www.w3.org/2001/XMLSchema#dateTime">2024-07-01T17:17:33</dc:issued>
    <cc:license rdf:resource="https://www.nationalarchives.gov.uk/doc/open-government-licence/version/3/"/>
    <cc:attributionURL rdf:resource="https://historicengland.org.uk/"/>
    <cc:attributionName xml:lang="en">Historic England</cc:attributionName>
    <dc:publisher rdf:resource="https://historicengland.org.uk/"/>
    <dc:spatial rdf:resource="http://vocab.getty.edu/tgn/7002445"/>
    <dc:spatial rdf:resource="http://dbpedia.org/resource/England"/>
    <skos:prefLabel xml:lang="en">Aggregates Quarry</skos:prefLabel>
    <skos:related rdf:resource="http://purl.org/heritagedata/schemes/571/concepts/152521"/>
    <skos:scopeNote xml:lang="en">Areas of excavation from which sand and gravel are obtained for use principally in construction and civil engineering. Includes directly associated facilities for aggregates processing.</skos:scopeNote>
  </skos:Concept>

  <skos:Concept rdf:about="http://purl.org/heritagedata/schemes/571/concepts/151420">
    <skos:broader rdf:resource="http://purl.org/heritagedata/schemes/571/concepts/160426"/>
    <skos:inScheme rdf:resource="http://purl.org/heritagedata/schemes/571"/>
    <dc:identifier>http://purl.org/heritagedata/schemes/571/concepts/151420</dc:identifier>
    <dc:issued rdf:datatype="http://www.w3.org/2001/XMLSchema#dateTime">2024-07-01T17:17:33</dc:issued>
    <cc:license rdf:resource="https://www.nationalarchives.gov.uk/doc/open-government-licence/version/3/"/>
    <cc:attributionURL rdf:resource="https://historicengland.org.uk/"/>
    <cc:attributionName xml:lang="en">Historic England</cc:attributionName>
    <dc:publisher rdf:resource="https://historicengland.org.uk/"/>
    <dc:spatial rdf:resource="http://vocab.getty.edu/tgn/7002445"/>
    <dc:spatial rdf:resource="http://dbpedia.org/resource/England"/>
    <skos:prefLabel xml:lang="en">Palace</skos:prefLabel>
    <skos:related rdf:resource="http://purl.org/heritagedata/schemes/571/concepts/151411"/>
    <skos:scopeNote xml:lang="en">A grand residence, royal, aristocratic or ecclesiastical, rural or urban, with immediately associated yards and offices.</skos:scopeNote>
  </skos:Concept>

  <skos:Concept rdf:about="http://purl.org/heritagedata/schemes/571/concepts/151421">
    <skos:broader rdf:resource="http://purl.org/heritagedata/schemes/571/concepts/151295"/>
    <skos:narrower>
      <skos:Concept rdf:about="http://purl.org/heritagedata/schemes/571/concepts/151779">
        <skos:broader rdf:resource="http://purl.org/heritagedata/schemes/571/concepts/151421"/>
        <skos:inScheme rdf:resource="http://purl.org/heritagedata/schemes/571"/>
        <dc:identifier>http://purl.org/heritagedata/schemes/571/concepts/151779</dc:identifier>
        <dc:issued rdf:datatype="http://www.w3.org/2001/XMLSchema#dateTime">2024-07-01T17:17:33</dc:issued>
        <cc:license rdf:resource="https://www.nationalarchives.gov.uk/doc/open-government-licence/version/3/"/>
        <cc:attributionURL rdf:resource="https://historicengland.org.uk/"/>
        <cc:attributionName xml:lang="en">Historic England</cc:attributionName>
        <dc:publisher rdf:resource="https://historicengland.org.uk/"/>
        <dc:spatial rdf:resource="http://vocab.getty.edu/tgn/7002445"/>
        <dc:spatial rdf:resource="http://dbpedia.org/resource/England"/>
        <skos:prefLabel xml:lang="en">Interrupted Row</skos:prefLabel>
        <skos:scopeNote xml:lang="en">A row settlement (linear arrangement of dwellings along a road) with numerous substantial gaps between buildings.</skos:scopeNote>
      </skos:Concept>
    </skos:narrower>

    <skos:inScheme rdf:resource="http://purl.org/heritagedata/schemes/571"/>
    <dc:identifier>http://purl.org/heritagedata/schemes/571/concepts/151421</dc:identifier>
    <dc:issued rdf:datatype="http://www.w3.org/2001/XMLSchema#dateTime">2024-07-01T17:17:33</dc:issued>
    <cc:license rdf:resource="https://www.nationalarchives.gov.uk/doc/open-government-licence/version/3/"/>
    <cc:attributionURL rdf:resource="https://historicengland.org.uk/"/>
    <cc:attributionName xml:lang="en">Historic England</cc:attributionName>
    <dc:publisher rdf:resource="https://historicengland.org.uk/"/>
    <dc:spatial rdf:resource="http://vocab.getty.edu/tgn/7002445"/>
    <dc:spatial rdf:resource="http://dbpedia.org/resource/England"/>
    <skos:prefLabel xml:lang="en">Rural Row</skos:prefLabel>
    <skos:scopeNote xml:lang="en">Linear arrangement of farmsteads and dwellings, usually built along a road.</skos:scopeNote>
  </skos:Concept>

  <skos:Concept rdf:about="http://purl.org/heritagedata/schemes/571/concepts/151436">
    <skos:broader rdf:resource="http://purl.org/heritagedata/schemes/571/concepts/151461"/>
    <skos:inScheme rdf:resource="http://purl.org/heritagedata/schemes/571"/>
    <dc:identifier>http://purl.org/heritagedata/schemes/571/concepts/151436</dc:identifier>
    <dc:issued rdf:datatype="http://www.w3.org/2001/XMLSchema#dateTime">2024-07-01T17:17:33</dc:issued>
    <cc:license rdf:resource="https://www.nationalarchives.gov.uk/doc/open-government-licence/version/3/"/>
    <cc:attributionURL rdf:resource="https://historicengland.org.uk/"/>
    <cc:attributionName xml:lang="en">Historic England</cc:attributionName>
    <dc:publisher rdf:resource="https://historicengland.org.uk/"/>
    <dc:spatial rdf:resource="http://vocab.getty.edu/tgn/7002445"/>
    <dc:spatial rdf:resource="http://dbpedia.org/resource/England"/>
    <skos:prefLabel xml:lang="en">Spoil Heap</skos:prefLabel>
    <skos:related rdf:resource="http://purl.org/heritagedata/schemes/571/concepts/151199"/>
    <skos:related rdf:resource="http://purl.org/heritagedata/schemes/571/concepts/151422"/>
    <skos:related rdf:resource="http://purl.org/heritagedata/schemes/571/concepts/152623"/>
    <skos:scopeNote xml:lang="en">A conical, ramped or flat-topped tip of waste discarded from a mine, quarry, clayworks or similar site.</skos:scopeNote>
  </skos:Concept>

  <skos:Concept rdf:about="http://purl.org/heritagedata/schemes/571/concepts/151571">
    <skos:broader rdf:resource="http://purl.org/heritagedata/schemes/571/concepts/151569"/>
    <skos:narrower>
      <skos:Concept rdf:about="http://purl.org/heritagedata/schemes/571/concepts/160168">
        <skos:broader rdf:resource="http://purl.org/heritagedata/schemes/571/concepts/151571"/>
        <skos:inScheme rdf:resource="http://purl.org/heritagedata/schemes/571"/>
        <dc:identifier>http://purl.org/heritagedata/schemes/571/concepts/160168</dc:identifier>
        <dc:issued rdf:datatype="http://www.w3.org/2001/XMLSchema#dateTime">2024-07-01T17:17:33</dc:issued>
        <cc:license rdf:resource="https://www.nationalarchives.gov.uk/doc/open-government-licence/version/3/"/>
        <cc:attributionURL rdf:resource="https://historicengland.org.uk/"/>
        <cc:attributionName xml:lang="en">Historic England</cc:attributionName>
        <dc:publisher rdf:resource="https://historicengland.org.uk/"/>
        <dc:spatial rdf:resource="http://vocab.getty.edu/tgn/7002445"/>
        <dc:spatial rdf:resource="http://dbpedia.org/resource/England"/>
        <skos:prefLabel xml:lang="en">China Clay Works</skos:prefLabel>
        <skos:scopeNote xml:lang="en">A place where china-clay (kaolin) is extracted and purified.</skos:scopeNote>
      </skos:Concept>
    </skos:narrower>

    <skos:inScheme rdf:resource="http://purl.org/heritagedata/schemes/571"/>
    <dc:identifier>http://purl.org/heritagedata/schemes/571/concepts/151571</dc:identifier>
    <dc:issued rdf:datatype="http://www.w3.org/2001/XMLSchema#dateTime">2024-07-01T17:17:33</dc:issued>
    <cc:license rdf:resource="https://www.nationalarchives.gov.uk/doc/open-government-licence/version/3/"/>
    <cc:attributionURL rdf:resource="https://historicengland.org.uk/"/>
    <cc:attributionName xml:lang="en">Historic England</cc:attributionName>
    <dc:publisher rdf:resource="https://historicengland.org.uk/"/>
    <dc:spatial rdf:resource="http://vocab.getty.edu/tgn/7002445"/>
    <dc:spatial rdf:resource="http://dbpedia.org/resource/England"/>
    <skos:prefLabel xml:lang="en">Clayworks</skos:prefLabel>
    <skos:scopeNote xml:lang="en">A site where clay is extracted from the surface of the ground.</skos:scopeNote>
  </skos:Concept>

  <skos:Concept rdf:about="http://purl.org/heritagedata/schemes/571/concepts/151449">
    <skos:narrower rdf:resource="http://purl.org/heritagedata/schemes/571/concepts/151576"/>
    <skos:narrower rdf:resource="http://purl.org/heritagedata/schemes/571/concepts/151648"/>
    <skos:narrower rdf:resource="http://purl.org/heritagedata/schemes/571/concepts/151650"/>
    <skos:narrower rdf:resource="http://purl.org/heritagedata/schemes/571/concepts/151651"/>
    <skos:narrower rdf:resource="http://purl.org/heritagedata/schemes/571/concepts/151656"/>
    <skos:inScheme rdf:resource="http://purl.org/heritagedata/schemes/571"/>
    <dc:identifier>http://purl.org/heritagedata/schemes/571/concepts/151449</dc:identifier>
    <dc:issued rdf:datatype="http://www.w3.org/2001/XMLSchema#dateTime">2024-07-01T17:17:33</dc:issued>
    <cc:license rdf:resource="https://www.nationalarchives.gov.uk/doc/open-government-licence/version/3/"/>
    <cc:attributionURL rdf:resource="https://historicengland.org.uk/"/>
    <cc:attributionName xml:lang="en">Historic England</cc:attributionName>
    <dc:publisher rdf:resource="https://historicengland.org.uk/"/>
    <dc:spatial rdf:resource="http://vocab.getty.edu/tgn/7002445"/>
    <dc:spatial rdf:resource="http://dbpedia.org/resource/England"/>
    <skos:prefLabel xml:lang="en">Communications And Movement</skos:prefLabel>
    <skos:scopeNote xml:lang="en">-</skos:scopeNote>
    <skos:topConceptOf rdf:resource="http://purl.org/heritagedata/schemes/571"/>
  </skos:Concept>

  <skos:Concept rdf:about="http://purl.org/heritagedata/schemes/571/concepts/151577">
    <skos:broader rdf:resource="http://purl.org/heritagedata/schemes/571/concepts/151445"/>
    <skos:inScheme rdf:resource="http://purl.org/heritagedata/schemes/571"/>
    <dc:identifier>http://purl.org/heritagedata/schemes/571/concepts/151577</dc:identifier>
    <dc:issued rdf:datatype="http://www.w3.org/2001/XMLSchema#dateTime">2024-07-01T17:17:33</dc:issued>
    <cc:license rdf:resource="https://www.nationalarchives.gov.uk/doc/open-government-licence/version/3/"/>
    <cc:attributionURL rdf:resource="https://historicengland.org.uk/"/>
    <cc:attributionName xml:lang="en">Historic England</cc:attributionName>
    <dc:publisher rdf:resource="https://historicengland.org.uk/"/>
    <dc:spatial rdf:resource="http://vocab.getty.edu/tgn/7002445"/>
    <dc:spatial rdf:resource="http://dbpedia.org/resource/England"/>
    <skos:prefLabel xml:lang="en">City</skos:prefLabel>
    <skos:related rdf:resource="http://purl.org/heritagedata/schemes/571/concepts/151062"/>
    <skos:related rdf:resource="http://purl.org/heritagedata/schemes/571/concepts/151077"/>
    <skos:related rdf:resource="http://purl.org/heritagedata/schemes/571/concepts/151078"/>
    <skos:related rdf:resource="http://purl.org/heritagedata/schemes/571/concepts/151079"/>
    <skos:related rdf:resource="http://purl.org/heritagedata/schemes/571/concepts/151762"/>
    <skos:related rdf:resource="http://purl.org/heritagedata/schemes/571/concepts/151708"/>
    <skos:scopeNote xml:lang="en">Large urban settlement, including residential, industrial, civic, commercial and business areas. Usually having a cathedral within its bounds. Often a central place within a region, with subsidiary towns etc.</skos:scopeNote>
  </skos:Concept>

  <skos:Concept rdf:about="http://purl.org/heritagedata/schemes/571/concepts/151581">
    <skos:broader rdf:resource="http://purl.org/heritagedata/schemes/571/concepts/151445"/>
    <skos:narrower rdf:resource="http://purl.org/heritagedata/schemes/571/concepts/151582"/>
    <skos:narrower>
      <skos:Concept rdf:about="http://purl.org/heritagedata/schemes/571/concepts/151583">
        <skos:broader rdf:resource="http://purl.org/heritagedata/schemes/571/concepts/151581"/>
        <skos:inScheme rdf:resource="http://purl.org/heritagedata/schemes/571"/>
        <dc:identifier>http://purl.org/heritagedata/schemes/571/concepts/151583</dc:identifier>
        <dc:issued rdf:datatype="http://www.w3.org/2001/XMLSchema#dateTime">2024-07-01T17:17:33</dc:issued>
        <cc:license rdf:resource="https://www.nationalarchives.gov.uk/doc/open-government-licence/version/3/"/>
        <cc:attributionURL rdf:resource="https://historicengland.org.uk/"/>
        <cc:attributionName xml:lang="en">Historic England</cc:attributionName>
        <dc:publisher rdf:resource="https://historicengland.org.uk/"/>
        <dc:spatial rdf:resource="http://vocab.getty.edu/tgn/7002445"/>
        <dc:spatial rdf:resource="http://dbpedia.org/resource/England"/>
        <skos:prefLabel xml:lang="en">Infill</skos:prefLabel>
        <skos:scopeNote xml:lang="en">Land within a generally built-up area, previously either open or used differently, that has been used for further construction.</skos:scopeNote>
      </skos:Concept>
    </skos:narrower>

    <skos:narrower>
      <skos:Concept rdf:about="http://purl.org/heritagedata/schemes/571/concepts/151764">
        <skos:broader rdf:resource="http://purl.org/heritagedata/schemes/571/concepts/151581"/>
        <skos:inScheme rdf:resource="http://purl.org/heritagedata/schemes/571"/>
        <dc:identifier>http://purl.org/heritagedata/schemes/571/concepts/151764</dc:identifier>
        <dc:issued rdf:datatype="http://www.w3.org/2001/XMLSchema#dateTime">2024-07-01T17:17:33</dc:issued>
        <cc:license rdf:resource="https://www.nationalarchives.gov.uk/doc/open-government-licence/version/3/"/>
        <cc:attributionURL rdf:resource="https://historicengland.org.uk/"/>
        <cc:attributionName xml:lang="en">Historic England</cc:attributionName>
        <dc:publisher rdf:resource="https://historicengland.org.uk/"/>
        <dc:spatial rdf:resource="http://vocab.getty.edu/tgn/7002445"/>
        <dc:spatial rdf:resource="http://dbpedia.org/resource/England"/>
        <skos:prefLabel xml:lang="en">Linear Urban Development</skos:prefLabel>
        <skos:scopeNote xml:lang="en">Urban extension, usually along a major thoroughfare (canal, road or railway).</skos:scopeNote>
      </skos:Concept>
    </skos:narrower>

    <skos:inScheme rdf:resource="http://purl.org/heritagedata/schemes/571"/>
    <dc:identifier>http://purl.org/heritagedata/schemes/571/concepts/151581</dc:identifier>
    <dc:issued rdf:datatype="http://www.w3.org/2001/XMLSchema#dateTime">2024-07-01T17:17:33</dc:issued>
    <cc:license rdf:resource="https://www.nationalarchives.gov.uk/doc/open-government-licence/version/3/"/>
    <cc:attributionURL rdf:resource="https://historicengland.org.uk/"/>
    <cc:attributionName xml:lang="en">Historic England</cc:attributionName>
    <dc:publisher rdf:resource="https://historicengland.org.uk/"/>
    <dc:spatial rdf:resource="http://vocab.getty.edu/tgn/7002445"/>
    <dc:spatial rdf:resource="http://dbpedia.org/resource/England"/>
    <skos:prefLabel xml:lang="en">Urban Extension</skos:prefLabel>
    <skos:scopeNote xml:lang="en">Extension of town or city beyond the Historic Urban Core, usually as defined by extents shown on early epoch OS mapping.</skos:scopeNote>
  </skos:Concept>

  <skos:Concept rdf:about="http://purl.org/heritagedata/schemes/571/concepts/151582">
    <skos:broader rdf:resource="http://purl.org/heritagedata/schemes/571/concepts/151581"/>
    <skos:broader rdf:resource="http://purl.org/heritagedata/schemes/571/concepts/163214"/>
    <skos:inScheme rdf:resource="http://purl.org/heritagedata/schemes/571"/>
    <dc:identifier>http://purl.org/heritagedata/schemes/571/concepts/151582</dc:identifier>
    <dc:issued rdf:datatype="http://www.w3.org/2001/XMLSchema#dateTime">2024-07-01T17:17:33</dc:issued>
    <cc:license rdf:resource="https://www.nationalarchives.gov.uk/doc/open-government-licence/version/3/"/>
    <cc:attributionURL rdf:resource="https://historicengland.org.uk/"/>
    <cc:attributionName xml:lang="en">Historic England</cc:attributionName>
    <dc:publisher rdf:resource="https://historicengland.org.uk/"/>
    <dc:spatial rdf:resource="http://vocab.getty.edu/tgn/7002445"/>
    <dc:spatial rdf:resource="http://dbpedia.org/resource/England"/>
    <skos:prefLabel xml:lang="en">Suburb</skos:prefLabel>
    <skos:related rdf:resource="http://purl.org/heritagedata/schemes/571/concepts/151257"/>
    <skos:scopeNote xml:lang="en">A largely residential area within a town or city usually situated away from its centre, often in medieval towns outwith any town walls. Modern suburbs often develop through urban growths absorption of a pre-existing smaller town or village.</skos:scopeNote>
  </skos:Concept>

  <skos:Concept rdf:about="http://purl.org/heritagedata/schemes/571/concepts/151596">
    <skos:broader rdf:resource="http://purl.org/heritagedata/schemes/571/concepts/151295"/>
    <skos:narrower rdf:resource="http://purl.org/heritagedata/schemes/571/concepts/151767"/>
    <skos:narrower>
      <skos:Concept rdf:about="http://purl.org/heritagedata/schemes/571/concepts/151770">
        <skos:broader rdf:resource="http://purl.org/heritagedata/schemes/571/concepts/151596"/>
        <skos:inScheme rdf:resource="http://purl.org/heritagedata/schemes/571"/>
        <dc:identifier>http://purl.org/heritagedata/schemes/571/concepts/151770</dc:identifier>
        <dc:issued rdf:datatype="http://www.w3.org/2001/XMLSchema#dateTime">2024-07-01T17:17:33</dc:issued>
        <cc:license rdf:resource="https://www.nationalarchives.gov.uk/doc/open-government-licence/version/3/"/>
        <cc:attributionURL rdf:resource="https://historicengland.org.uk/"/>
        <cc:attributionName xml:lang="en">Historic England</cc:attributionName>
        <dc:publisher rdf:resource="https://historicengland.org.uk/"/>
        <dc:spatial rdf:resource="http://vocab.getty.edu/tgn/7002445"/>
        <dc:spatial rdf:resource="http://dbpedia.org/resource/England"/>
        <skos:prefLabel xml:lang="en">Planned Village</skos:prefLabel>
        <skos:scopeNote xml:lang="en">Village whose regularity of spacing and shape of plots, and also often of form of dwellings, suggests a degree of external planning, usually by a landlord.</skos:scopeNote>
      </skos:Concept>
    </skos:narrower>

    <skos:narrower>
      <skos:Concept rdf:about="http://purl.org/heritagedata/schemes/571/concepts/151771">
        <skos:broader rdf:resource="http://purl.org/heritagedata/schemes/571/concepts/151596"/>
        <skos:inScheme rdf:resource="http://purl.org/heritagedata/schemes/571"/>
        <dc:identifier>http://purl.org/heritagedata/schemes/571/concepts/151771</dc:identifier>
        <dc:issued rdf:datatype="http://www.w3.org/2001/XMLSchema#dateTime">2024-07-01T17:17:33</dc:issued>
        <cc:license rdf:resource="https://www.nationalarchives.gov.uk/doc/open-government-licence/version/3/"/>
        <cc:attributionURL rdf:resource="https://historicengland.org.uk/"/>
        <cc:attributionName xml:lang="en">Historic England</cc:attributionName>
        <dc:publisher rdf:resource="https://historicengland.org.uk/"/>
        <dc:spatial rdf:resource="http://vocab.getty.edu/tgn/7002445"/>
        <dc:spatial rdf:resource="http://dbpedia.org/resource/England"/>
        <skos:prefLabel xml:lang="en">Industrial Village</skos:prefLabel>
        <skos:scopeNote xml:lang="en">Village for accommodation of industrial workers, usually close to either extractive industry or milling.</skos:scopeNote>
      </skos:Concept>
    </skos:narrower>

    <skos:narrower>
      <skos:Concept rdf:about="http://purl.org/heritagedata/schemes/571/concepts/160425">
        <skos:broader rdf:resource="http://purl.org/heritagedata/schemes/571/concepts/151596"/>
        <skos:inScheme rdf:resource="http://purl.org/heritagedata/schemes/571"/>
        <dc:identifier>http://purl.org/heritagedata/schemes/571/concepts/160425</dc:identifier>
        <dc:issued rdf:datatype="http://www.w3.org/2001/XMLSchema#dateTime">2024-07-01T17:17:33</dc:issued>
        <cc:license rdf:resource="https://www.nationalarchives.gov.uk/doc/open-government-licence/version/3/"/>
        <cc:attributionURL rdf:resource="https://historicengland.org.uk/"/>
        <cc:attributionName xml:lang="en">Historic England</cc:attributionName>
        <dc:publisher rdf:resource="https://historicengland.org.uk/"/>
        <dc:spatial rdf:resource="http://vocab.getty.edu/tgn/7002445"/>
        <dc:spatial rdf:resource="http://dbpedia.org/resource/England"/>
        <skos:prefLabel xml:lang="en">Green Edge Village</skos:prefLabel>
        <skos:scopeNote xml:lang="en">Agricultural village with farmsteads and cottages wholly or mainly arranged around the edges of a green.</skos:scopeNote>
      </skos:Concept>
    </skos:narrower>

    <skos:inScheme rdf:resource="http://purl.org/heritagedata/schemes/571"/>
    <dc:identifier>http://purl.org/heritagedata/schemes/571/concepts/151596</dc:identifier>
    <dc:issued rdf:datatype="http://www.w3.org/2001/XMLSchema#dateTime">2024-07-01T17:17:33</dc:issued>
    <cc:license rdf:resource="https://www.nationalarchives.gov.uk/doc/open-government-licence/version/3/"/>
    <cc:attributionURL rdf:resource="https://historicengland.org.uk/"/>
    <cc:attributionName xml:lang="en">Historic England</cc:attributionName>
    <dc:publisher rdf:resource="https://historicengland.org.uk/"/>
    <dc:spatial rdf:resource="http://vocab.getty.edu/tgn/7002445"/>
    <dc:spatial rdf:resource="http://dbpedia.org/resource/England"/>
    <skos:prefLabel xml:lang="en">Village</skos:prefLabel>
    <skos:scopeNote xml:lang="en">Collection of farmsteads, dwellings, yards, gardens etc. Larger than hamlet, smaller than town. Often includes church, inn, shops, workshops, manor house. Main rural settlement form in central province; rarer elsewhere. Also industrial villages.</skos:scopeNote>
  </skos:Concept>

  <skos:Concept rdf:about="http://purl.org/heritagedata/schemes/571/concepts/151597">
    <skos:broader rdf:resource="http://purl.org/heritagedata/schemes/571/concepts/151295"/>
    <skos:narrower>
      <skos:Concept rdf:about="http://purl.org/heritagedata/schemes/571/concepts/151773">
        <skos:broader rdf:resource="http://purl.org/heritagedata/schemes/571/concepts/151597"/>
        <skos:inScheme rdf:resource="http://purl.org/heritagedata/schemes/571"/>
        <dc:identifier>http://purl.org/heritagedata/schemes/571/concepts/151773</dc:identifier>
        <dc:issued rdf:datatype="http://www.w3.org/2001/XMLSchema#dateTime">2024-07-01T17:17:33</dc:issued>
        <cc:license rdf:resource="https://www.nationalarchives.gov.uk/doc/open-government-licence/version/3/"/>
        <cc:attributionURL rdf:resource="https://historicengland.org.uk/"/>
        <cc:attributionName xml:lang="en">Historic England</cc:attributionName>
        <dc:publisher rdf:resource="https://historicengland.org.uk/"/>
        <dc:spatial rdf:resource="http://vocab.getty.edu/tgn/7002445"/>
        <dc:spatial rdf:resource="http://dbpedia.org/resource/England"/>
        <skos:prefLabel xml:lang="en">Agricultural Hamlet</skos:prefLabel>
        <skos:scopeNote xml:lang="en">A small settlement containing two or more farmsteads, but few amenities. Typical rural settlement form away from central province.</skos:scopeNote>
      </skos:Concept>
    </skos:narrower>

    <skos:narrower>
      <skos:Concept rdf:about="http://purl.org/heritagedata/schemes/571/concepts/151774">
        <skos:broader rdf:resource="http://purl.org/heritagedata/schemes/571/concepts/151597"/>
        <skos:inScheme rdf:resource="http://purl.org/heritagedata/schemes/571"/>
        <dc:identifier>http://purl.org/heritagedata/schemes/571/concepts/151774</dc:identifier>
        <dc:issued rdf:datatype="http://www.w3.org/2001/XMLSchema#dateTime">2024-07-01T17:17:33</dc:issued>
        <cc:license rdf:resource="https://www.nationalarchives.gov.uk/doc/open-government-licence/version/3/"/>
        <cc:attributionURL rdf:resource="https://historicengland.org.uk/"/>
        <cc:attributionName xml:lang="en">Historic England</cc:attributionName>
        <dc:publisher rdf:resource="https://historicengland.org.uk/"/>
        <dc:spatial rdf:resource="http://vocab.getty.edu/tgn/7002445"/>
        <dc:spatial rdf:resource="http://dbpedia.org/resource/England"/>
        <skos:prefLabel xml:lang="en">Industrial Hamlet</skos:prefLabel>
        <skos:scopeNote xml:lang="en">Hamlet for accommodation of industrial workers, usually close to either extractive industry or milling.</skos:scopeNote>
      </skos:Concept>
    </skos:narrower>

    <skos:inScheme rdf:resource="http://purl.org/heritagedata/schemes/571"/>
    <dc:identifier>http://purl.org/heritagedata/schemes/571/concepts/151597</dc:identifier>
    <dc:issued rdf:datatype="http://www.w3.org/2001/XMLSchema#dateTime">2024-07-01T17:17:33</dc:issued>
    <cc:license rdf:resource="https://www.nationalarchives.gov.uk/doc/open-government-licence/version/3/"/>
    <cc:attributionURL rdf:resource="https://historicengland.org.uk/"/>
    <cc:attributionName xml:lang="en">Historic England</cc:attributionName>
    <dc:publisher rdf:resource="https://historicengland.org.uk/"/>
    <dc:spatial rdf:resource="http://vocab.getty.edu/tgn/7002445"/>
    <dc:spatial rdf:resource="http://dbpedia.org/resource/England"/>
    <skos:prefLabel xml:lang="en">Hamlet</skos:prefLabel>
    <skos:scopeNote xml:lang="en">Small settlement with no ecclesiastical or lay administrative function and usually with no other amenities.</skos:scopeNote>
  </skos:Concept>

  <skos:Concept rdf:about="http://purl.org/heritagedata/schemes/571/concepts/151598">
    <skos:broader rdf:resource="http://purl.org/heritagedata/schemes/571/concepts/151452"/>
    <skos:inScheme rdf:resource="http://purl.org/heritagedata/schemes/571"/>
    <dc:identifier>http://purl.org/heritagedata/schemes/571/concepts/151598</dc:identifier>
    <dc:issued rdf:datatype="http://www.w3.org/2001/XMLSchema#dateTime">2024-07-01T17:17:33</dc:issued>
    <cc:license rdf:resource="https://www.nationalarchives.gov.uk/doc/open-government-licence/version/3/"/>
    <cc:attributionURL rdf:resource="https://historicengland.org.uk/"/>
    <cc:attributionName xml:lang="en">Historic England</cc:attributionName>
    <dc:publisher rdf:resource="https://historicengland.org.uk/"/>
    <dc:spatial rdf:resource="http://vocab.getty.edu/tgn/7002445"/>
    <dc:spatial rdf:resource="http://dbpedia.org/resource/England"/>
    <skos:prefLabel xml:lang="en">Shelterbelt</skos:prefLabel>
    <skos:related rdf:resource="http://purl.org/heritagedata/schemes/571/concepts/151600"/>
    <skos:scopeNote xml:lang="en">A plantation of trees or shrubs usually linear in plan placed to provide shelter from the wind for parks and gardens.</skos:scopeNote>
  </skos:Concept>

  <skos:Concept rdf:about="http://purl.org/heritagedata/schemes/571/concepts/151599">
    <skos:broader rdf:resource="http://purl.org/heritagedata/schemes/571/concepts/151452"/>
    <skos:inScheme rdf:resource="http://purl.org/heritagedata/schemes/571"/>
    <dc:identifier>http://purl.org/heritagedata/schemes/571/concepts/151599</dc:identifier>
    <dc:issued rdf:datatype="http://www.w3.org/2001/XMLSchema#dateTime">2024-07-01T17:17:33</dc:issued>
    <cc:license rdf:resource="https://www.nationalarchives.gov.uk/doc/open-government-licence/version/3/"/>
    <cc:attributionURL rdf:resource="https://historicengland.org.uk/"/>
    <cc:attributionName xml:lang="en">Historic England</cc:attributionName>
    <dc:publisher rdf:resource="https://historicengland.org.uk/"/>
    <dc:spatial rdf:resource="http://vocab.getty.edu/tgn/7002445"/>
    <dc:spatial rdf:resource="http://dbpedia.org/resource/England"/>
    <skos:prefLabel xml:lang="en">Ornamental Plantation</skos:prefLabel>
    <skos:related rdf:resource="http://purl.org/heritagedata/schemes/571/concepts/151600"/>
    <skos:scopeNote xml:lang="en">A group of planted trees or shrubs, designed to enhance the landscape, often by obscuring eyescores or by framing preferred views. A common feature of landscape parks.</skos:scopeNote>
  </skos:Concept>

  <skos:Concept rdf:about="http://purl.org/heritagedata/schemes/571/concepts/151600">
    <skos:broader rdf:resource="http://purl.org/heritagedata/schemes/571/concepts/151756"/>
    <skos:inScheme rdf:resource="http://purl.org/heritagedata/schemes/571"/>
    <dc:identifier>http://purl.org/heritagedata/schemes/571/concepts/151600</dc:identifier>
    <dc:issued rdf:datatype="http://www.w3.org/2001/XMLSchema#dateTime">2024-07-01T17:17:33</dc:issued>
    <cc:license rdf:resource="https://www.nationalarchives.gov.uk/doc/open-government-licence/version/3/"/>
    <cc:attributionURL rdf:resource="https://historicengland.org.uk/"/>
    <cc:attributionName xml:lang="en">Historic England</cc:attributionName>
    <dc:publisher rdf:resource="https://historicengland.org.uk/"/>
    <dc:spatial rdf:resource="http://vocab.getty.edu/tgn/7002445"/>
    <dc:spatial rdf:resource="http://dbpedia.org/resource/England"/>
    <skos:prefLabel xml:lang="en">Landscape Park</skos:prefLabel>
    <skos:related rdf:resource="http://purl.org/heritagedata/schemes/571/concepts/151287"/>
    <skos:related rdf:resource="http://purl.org/heritagedata/schemes/571/concepts/151409"/>
    <skos:related rdf:resource="http://purl.org/heritagedata/schemes/571/concepts/151598"/>
    <skos:related rdf:resource="http://purl.org/heritagedata/schemes/571/concepts/151599"/>
    <skos:scopeNote xml:lang="en">Extensive grounds, usually associated with a country house, laid out (with tree plantations, shrubs and often adjusted with earth movement) so as to produce a perception of broad unmanaged and often unpeopled vistas.</skos:scopeNote>
  </skos:Concept>

  <skos:Concept rdf:about="http://purl.org/heritagedata/schemes/571/concepts/151756">
    <skos:narrower rdf:resource="http://purl.org/heritagedata/schemes/571/concepts/151600"/>
    <skos:narrower rdf:resource="http://purl.org/heritagedata/schemes/571/concepts/160264"/>
    <skos:broader rdf:resource="http://purl.org/heritagedata/schemes/571/concepts/151452"/>
    <skos:inScheme rdf:resource="http://purl.org/heritagedata/schemes/571"/>
    <dc:identifier>http://purl.org/heritagedata/schemes/571/concepts/151756</dc:identifier>
    <dc:issued rdf:datatype="http://www.w3.org/2001/XMLSchema#dateTime">2024-07-01T17:17:33</dc:issued>
    <cc:license rdf:resource="https://www.nationalarchives.gov.uk/doc/open-government-licence/version/3/"/>
    <cc:attributionURL rdf:resource="https://historicengland.org.uk/"/>
    <cc:attributionName xml:lang="en">Historic England</cc:attributionName>
    <dc:publisher rdf:resource="https://historicengland.org.uk/"/>
    <dc:spatial rdf:resource="http://vocab.getty.edu/tgn/7002445"/>
    <dc:spatial rdf:resource="http://dbpedia.org/resource/England"/>
    <skos:prefLabel xml:lang="en">Park</skos:prefLabel>
    <skos:related rdf:resource="http://purl.org/heritagedata/schemes/571/concepts/151159"/>
    <skos:scopeNote xml:lang="en">An enclosed piece of land, generally large in area, usually either surrounding a country house or castle, or conveniently adjacent to it. Used for hunting, the cultivation of trees, pasture and visual enjoyment.</skos:scopeNote>
  </skos:Concept>

  <skos:Concept rdf:about="http://purl.org/heritagedata/schemes/571/concepts/151604">
    <skos:broader rdf:resource="http://purl.org/heritagedata/schemes/571/concepts/151698"/>
    <skos:broader rdf:resource="http://purl.org/heritagedata/schemes/571/concepts/160252"/>
    <skos:inScheme rdf:resource="http://purl.org/heritagedata/schemes/571"/>
    <dc:identifier>http://purl.org/heritagedata/schemes/571/concepts/151604</dc:identifier>
    <dc:issued rdf:datatype="http://www.w3.org/2001/XMLSchema#dateTime">2024-07-01T17:17:33</dc:issued>
    <cc:license rdf:resource="https://www.nationalarchives.gov.uk/doc/open-government-licence/version/3/"/>
    <cc:attributionURL rdf:resource="https://historicengland.org.uk/"/>
    <cc:attributionName xml:lang="en">Historic England</cc:attributionName>
    <dc:publisher rdf:resource="https://historicengland.org.uk/"/>
    <dc:spatial rdf:resource="http://vocab.getty.edu/tgn/7002445"/>
    <dc:spatial rdf:resource="http://dbpedia.org/resource/England"/>
    <skos:prefLabel xml:lang="en">Spa</skos:prefLabel>
    <skos:scopeNote xml:lang="en">A medicinal or mineral spring often with an associated building and directly associated grounds. Often found closely grouped, around which settlements and spa towns have developed.</skos:scopeNote>
  </skos:Concept>

  <skos:Concept rdf:about="http://purl.org/heritagedata/schemes/571/concepts/151609">
    <skos:broader rdf:resource="http://purl.org/heritagedata/schemes/571/concepts/152326"/>
    <skos:narrower>
      <skos:Concept rdf:about="http://purl.org/heritagedata/schemes/571/concepts/160479">
        <skos:broader rdf:resource="http://purl.org/heritagedata/schemes/571/concepts/151609"/>
        <skos:inScheme rdf:resource="http://purl.org/heritagedata/schemes/571"/>
        <dc:identifier>http://purl.org/heritagedata/schemes/571/concepts/160479</dc:identifier>
        <dc:issued rdf:datatype="http://www.w3.org/2001/XMLSchema#dateTime">2024-07-01T17:17:33</dc:issued>
        <cc:license rdf:resource="https://www.nationalarchives.gov.uk/doc/open-government-licence/version/3/"/>
        <cc:attributionURL rdf:resource="https://historicengland.org.uk/"/>
        <cc:attributionName xml:lang="en">Historic England</cc:attributionName>
        <dc:publisher rdf:resource="https://historicengland.org.uk/"/>
        <dc:spatial rdf:resource="http://vocab.getty.edu/tgn/7002445"/>
        <dc:spatial rdf:resource="http://dbpedia.org/resource/England"/>
        <skos:prefLabel xml:lang="en">Heathland (Divided)</skos:prefLabel>
        <skos:scopeNote xml:lang="en">Heathland divided by stock-proof boundaries.</skos:scopeNote>
      </skos:Concept>
    </skos:narrower>

    <skos:narrower>
      <skos:Concept rdf:about="http://purl.org/heritagedata/schemes/571/concepts/160480">
        <skos:broader rdf:resource="http://purl.org/heritagedata/schemes/571/concepts/151609"/>
        <skos:inScheme rdf:resource="http://purl.org/heritagedata/schemes/571"/>
        <dc:identifier>http://purl.org/heritagedata/schemes/571/concepts/160480</dc:identifier>
        <dc:issued rdf:datatype="http://www.w3.org/2001/XMLSchema#dateTime">2024-07-01T17:17:33</dc:issued>
        <cc:license rdf:resource="https://www.nationalarchives.gov.uk/doc/open-government-licence/version/3/"/>
        <cc:attributionURL rdf:resource="https://historicengland.org.uk/"/>
        <cc:attributionName xml:lang="en">Historic England</cc:attributionName>
        <dc:publisher rdf:resource="https://historicengland.org.uk/"/>
        <dc:spatial rdf:resource="http://vocab.getty.edu/tgn/7002445"/>
        <dc:spatial rdf:resource="http://dbpedia.org/resource/England"/>
        <skos:prefLabel xml:lang="en">Heathland (Undivided)</skos:prefLabel>
        <skos:scopeNote xml:lang="en">Heathland left open, not divided by stock-proof boundaries.</skos:scopeNote>
      </skos:Concept>
    </skos:narrower>

    <skos:inScheme rdf:resource="http://purl.org/heritagedata/schemes/571"/>
    <dc:identifier>http://purl.org/heritagedata/schemes/571/concepts/151609</dc:identifier>
    <dc:issued rdf:datatype="http://www.w3.org/2001/XMLSchema#dateTime">2024-07-01T17:17:33</dc:issued>
    <cc:license rdf:resource="https://www.nationalarchives.gov.uk/doc/open-government-licence/version/3/"/>
    <cc:attributionURL rdf:resource="https://historicengland.org.uk/"/>
    <cc:attributionName xml:lang="en">Historic England</cc:attributionName>
    <dc:publisher rdf:resource="https://historicengland.org.uk/"/>
    <dc:spatial rdf:resource="http://vocab.getty.edu/tgn/7002445"/>
    <dc:spatial rdf:resource="http://dbpedia.org/resource/England"/>
    <skos:prefLabel xml:lang="en">Heathland</skos:prefLabel>
    <skos:scopeNote xml:lang="en">Unimproved, but grazed area of low-growing woody shrubby vegetation, including heathers and gorses, sometimes in a mosaic with grassland and damp areas.</skos:scopeNote>
  </skos:Concept>

  <skos:Concept rdf:about="http://purl.org/heritagedata/schemes/571/concepts/151610">
    <skos:broader rdf:resource="http://purl.org/heritagedata/schemes/571/concepts/151458"/>
    <skos:broader rdf:resource="http://purl.org/heritagedata/schemes/571/concepts/160288"/>
    <skos:inScheme rdf:resource="http://purl.org/heritagedata/schemes/571"/>
    <dc:identifier>http://purl.org/heritagedata/schemes/571/concepts/151610</dc:identifier>
    <dc:issued rdf:datatype="http://www.w3.org/2001/XMLSchema#dateTime">2024-07-01T17:17:33</dc:issued>
    <cc:license rdf:resource="https://www.nationalarchives.gov.uk/doc/open-government-licence/version/3/"/>
    <cc:attributionURL rdf:resource="https://historicengland.org.uk/"/>
    <cc:attributionName xml:lang="en">Historic England</cc:attributionName>
    <dc:publisher rdf:resource="https://historicengland.org.uk/"/>
    <dc:spatial rdf:resource="http://vocab.getty.edu/tgn/7002445"/>
    <dc:spatial rdf:resource="http://dbpedia.org/resource/England"/>
    <skos:prefLabel xml:lang="en">Hotel</skos:prefLabel>
    <skos:scopeNote xml:lang="en">A building and its directly associated grounds, used for the accommodation of paying travellers and guests.</skos:scopeNote>
  </skos:Concept>

  <skos:Concept rdf:about="http://purl.org/heritagedata/schemes/571/concepts/151614">
    <skos:broader rdf:resource="http://purl.org/heritagedata/schemes/571/concepts/151443"/>
    <skos:narrower>
      <skos:Concept rdf:about="http://purl.org/heritagedata/schemes/571/concepts/151615">
        <skos:broader rdf:resource="http://purl.org/heritagedata/schemes/571/concepts/151614"/>
        <skos:inScheme rdf:resource="http://purl.org/heritagedata/schemes/571"/>
        <dc:identifier>http://purl.org/heritagedata/schemes/571/concepts/151615</dc:identifier>
        <dc:issued rdf:datatype="http://www.w3.org/2001/XMLSchema#dateTime">2024-07-01T17:17:33</dc:issued>
        <cc:license rdf:resource="https://www.nationalarchives.gov.uk/doc/open-government-licence/version/3/"/>
        <cc:attributionURL rdf:resource="https://historicengland.org.uk/"/>
        <cc:attributionName xml:lang="en">Historic England</cc:attributionName>
        <dc:publisher rdf:resource="https://historicengland.org.uk/"/>
        <dc:spatial rdf:resource="http://vocab.getty.edu/tgn/7002445"/>
        <dc:spatial rdf:resource="http://dbpedia.org/resource/England"/>
        <skos:prefLabel xml:lang="en">Foreshore (Rocky)</skos:prefLabel>
        <skos:scopeNote xml:lang="en">An area of foreshore where the predominant cover is exposed bedrock.</skos:scopeNote>
      </skos:Concept>
    </skos:narrower>

    <skos:narrower>
      <skos:Concept rdf:about="http://purl.org/heritagedata/schemes/571/concepts/151616">
        <skos:broader rdf:resource="http://purl.org/heritagedata/schemes/571/concepts/151614"/>
        <skos:inScheme rdf:resource="http://purl.org/heritagedata/schemes/571"/>
        <dc:identifier>http://purl.org/heritagedata/schemes/571/concepts/151616</dc:identifier>
        <dc:issued rdf:datatype="http://www.w3.org/2001/XMLSchema#dateTime">2024-07-01T17:17:33</dc:issued>
        <cc:license rdf:resource="https://www.nationalarchives.gov.uk/doc/open-government-licence/version/3/"/>
        <cc:attributionURL rdf:resource="https://historicengland.org.uk/"/>
        <cc:attributionName xml:lang="en">Historic England</cc:attributionName>
        <dc:publisher rdf:resource="https://historicengland.org.uk/"/>
        <dc:spatial rdf:resource="http://vocab.getty.edu/tgn/7002445"/>
        <dc:spatial rdf:resource="http://dbpedia.org/resource/England"/>
        <skos:prefLabel xml:lang="en">Foreshore (Sandy)</skos:prefLabel>
        <skos:scopeNote xml:lang="en">An area of foreshore where the predominant cover is exposed fine rock sediments of a grain size generally perceived as 'sand'.</skos:scopeNote>
      </skos:Concept>
    </skos:narrower>

    <skos:narrower>
      <skos:Concept rdf:about="http://purl.org/heritagedata/schemes/571/concepts/152508">
        <skos:broader rdf:resource="http://purl.org/heritagedata/schemes/571/concepts/151614"/>
        <skos:inScheme rdf:resource="http://purl.org/heritagedata/schemes/571"/>
        <dc:identifier>http://purl.org/heritagedata/schemes/571/concepts/152508</dc:identifier>
        <dc:issued rdf:datatype="http://www.w3.org/2001/XMLSchema#dateTime">2024-07-01T17:17:33</dc:issued>
        <cc:license rdf:resource="https://www.nationalarchives.gov.uk/doc/open-government-licence/version/3/"/>
        <cc:attributionURL rdf:resource="https://historicengland.org.uk/"/>
        <cc:attributionName xml:lang="en">Historic England</cc:attributionName>
        <dc:publisher rdf:resource="https://historicengland.org.uk/"/>
        <dc:spatial rdf:resource="http://vocab.getty.edu/tgn/7002445"/>
        <dc:spatial rdf:resource="http://dbpedia.org/resource/England"/>
        <skos:prefLabel xml:lang="en">Foreshore (Shingle)</skos:prefLabel>
        <skos:scopeNote xml:lang="en">An area of foreshore where the predominant cover is exposed coarse rock sediments of a grain size generally perceived as 'shingle' or 'pebbles'.</skos:scopeNote>
      </skos:Concept>
    </skos:narrower>

    <skos:inScheme rdf:resource="http://purl.org/heritagedata/schemes/571"/>
    <dc:identifier>http://purl.org/heritagedata/schemes/571/concepts/151614</dc:identifier>
    <dc:issued rdf:datatype="http://www.w3.org/2001/XMLSchema#dateTime">2024-07-01T17:17:33</dc:issued>
    <cc:license rdf:resource="https://www.nationalarchives.gov.uk/doc/open-government-licence/version/3/"/>
    <cc:attributionURL rdf:resource="https://historicengland.org.uk/"/>
    <cc:attributionName xml:lang="en">Historic England</cc:attributionName>
    <dc:publisher rdf:resource="https://historicengland.org.uk/"/>
    <dc:spatial rdf:resource="http://vocab.getty.edu/tgn/7002445"/>
    <dc:spatial rdf:resource="http://dbpedia.org/resource/England"/>
    <skos:prefLabel xml:lang="en">Foreshore</skos:prefLabel>
    <skos:scopeNote xml:lang="en">The foreshore is broadly equated with land sloping down through the inter-tidal zone from the landward coastal margin; Its extent is defined by perception of the inter-tidal rather than by detailed tidal level definitions.</skos:scopeNote>
  </skos:Concept>

  <skos:Concept rdf:about="http://purl.org/heritagedata/schemes/571/concepts/151619">
    <skos:broader rdf:resource="http://purl.org/heritagedata/schemes/571/concepts/151666"/>
    <skos:broader rdf:resource="http://purl.org/heritagedata/schemes/571/concepts/151766"/>
    <skos:inScheme rdf:resource="http://purl.org/heritagedata/schemes/571"/>
    <dc:identifier>http://purl.org/heritagedata/schemes/571/concepts/151619</dc:identifier>
    <dc:issued rdf:datatype="http://www.w3.org/2001/XMLSchema#dateTime">2024-07-01T17:17:33</dc:issued>
    <cc:license rdf:resource="https://www.nationalarchives.gov.uk/doc/open-government-licence/version/3/"/>
    <cc:attributionURL rdf:resource="https://historicengland.org.uk/"/>
    <cc:attributionName xml:lang="en">Historic England</cc:attributionName>
    <dc:publisher rdf:resource="https://historicengland.org.uk/"/>
    <dc:spatial rdf:resource="http://vocab.getty.edu/tgn/7002445"/>
    <dc:spatial rdf:resource="http://dbpedia.org/resource/England"/>
    <skos:prefLabel xml:lang="en">Fish Market</skos:prefLabel>
    <skos:scopeNote xml:lang="en">A market where fish is sold. Includes closely and functionally associated open areas, built structures, wharves, quays and distribution facilities.</skos:scopeNote>
  </skos:Concept>

  <skos:Concept rdf:about="http://purl.org/heritagedata/schemes/571/concepts/151666">
    <skos:narrower rdf:resource="http://purl.org/heritagedata/schemes/571/concepts/151619"/>
    <skos:narrower rdf:resource="http://purl.org/heritagedata/schemes/571/concepts/151683"/>
    <skos:narrower>
      <skos:Concept rdf:about="http://purl.org/heritagedata/schemes/571/concepts/151691">
        <skos:broader rdf:resource="http://purl.org/heritagedata/schemes/571/concepts/151666"/>
        <skos:inScheme rdf:resource="http://purl.org/heritagedata/schemes/571"/>
        <dc:identifier>http://purl.org/heritagedata/schemes/571/concepts/151691</dc:identifier>
        <dc:issued rdf:datatype="http://www.w3.org/2001/XMLSchema#dateTime">2024-07-01T17:17:33</dc:issued>
        <cc:license rdf:resource="https://www.nationalarchives.gov.uk/doc/open-government-licence/version/3/"/>
        <cc:attributionURL rdf:resource="https://historicengland.org.uk/"/>
        <cc:attributionName xml:lang="en">Historic England</cc:attributionName>
        <dc:publisher rdf:resource="https://historicengland.org.uk/"/>
        <dc:spatial rdf:resource="http://vocab.getty.edu/tgn/7002445"/>
        <dc:spatial rdf:resource="http://dbpedia.org/resource/England"/>
        <skos:prefLabel xml:lang="en">Bait Digging</skos:prefLabel>
        <skos:scopeNote xml:lang="en">Areas whose character is dominated by regular digging to acquire bait for fishing by various methods. Generally found in estuaries, sandy and rocky foreshores.</skos:scopeNote>
      </skos:Concept>
    </skos:narrower>

    <skos:narrower rdf:resource="http://purl.org/heritagedata/schemes/571/concepts/152549"/>
    <skos:inScheme rdf:resource="http://purl.org/heritagedata/schemes/571"/>
    <dc:identifier>http://purl.org/heritagedata/schemes/571/concepts/151666</dc:identifier>
    <dc:issued rdf:datatype="http://www.w3.org/2001/XMLSchema#dateTime">2024-07-01T17:17:33</dc:issued>
    <cc:license rdf:resource="https://www.nationalarchives.gov.uk/doc/open-government-licence/version/3/"/>
    <cc:attributionURL rdf:resource="https://historicengland.org.uk/"/>
    <cc:attributionName xml:lang="en">Historic England</cc:attributionName>
    <dc:publisher rdf:resource="https://historicengland.org.uk/"/>
    <dc:spatial rdf:resource="http://vocab.getty.edu/tgn/7002445"/>
    <dc:spatial rdf:resource="http://dbpedia.org/resource/England"/>
    <skos:prefLabel xml:lang="en">Fisheries And Aquaculture</skos:prefLabel>
    <skos:scopeNote xml:lang="en">-</skos:scopeNote>
    <skos:topConceptOf rdf:resource="http://purl.org/heritagedata/schemes/571"/>
  </skos:Concept>

  <skos:Concept rdf:about="http://purl.org/heritagedata/schemes/571/concepts/151620">
    <skos:broader rdf:resource="http://purl.org/heritagedata/schemes/571/concepts/151683"/>
    <skos:inScheme rdf:resource="http://purl.org/heritagedata/schemes/571"/>
    <dc:identifier>http://purl.org/heritagedata/schemes/571/concepts/151620</dc:identifier>
    <dc:issued rdf:datatype="http://www.w3.org/2001/XMLSchema#dateTime">2024-07-01T17:17:33</dc:issued>
    <cc:license rdf:resource="https://www.nationalarchives.gov.uk/doc/open-government-licence/version/3/"/>
    <cc:attributionURL rdf:resource="https://historicengland.org.uk/"/>
    <cc:attributionName xml:lang="en">Historic England</cc:attributionName>
    <dc:publisher rdf:resource="https://historicengland.org.uk/"/>
    <dc:spatial rdf:resource="http://vocab.getty.edu/tgn/7002445"/>
    <dc:spatial rdf:resource="http://dbpedia.org/resource/England"/>
    <skos:prefLabel xml:lang="en">Fishing Ground</skos:prefLabel>
    <skos:scopeNote xml:lang="en">An area regularly exploited for commercial fish and/or shellfish extraction; within which the locations of actual fishing activity may vary at any given time, seasonally, according to the species concerned and regulations govening their exploitation.</skos:scopeNote>
  </skos:Concept>

  <skos:Concept rdf:about="http://purl.org/heritagedata/schemes/571/concepts/151683">
    <skos:narrower rdf:resource="http://purl.org/heritagedata/schemes/571/concepts/151620"/>
    <skos:narrower>
      <skos:Concept rdf:about="http://purl.org/heritagedata/schemes/571/concepts/151687">
        <skos:broader rdf:resource="http://purl.org/heritagedata/schemes/571/concepts/151683"/>
        <skos:inScheme rdf:resource="http://purl.org/heritagedata/schemes/571"/>
        <dc:identifier>http://purl.org/heritagedata/schemes/571/concepts/151687</dc:identifier>
        <dc:issued rdf:datatype="http://www.w3.org/2001/XMLSchema#dateTime">2024-07-01T17:17:33</dc:issued>
        <cc:license rdf:resource="https://www.nationalarchives.gov.uk/doc/open-government-licence/version/3/"/>
        <cc:attributionURL rdf:resource="https://historicengland.org.uk/"/>
        <cc:attributionName xml:lang="en">Historic England</cc:attributionName>
        <dc:publisher rdf:resource="https://historicengland.org.uk/"/>
        <dc:spatial rdf:resource="http://vocab.getty.edu/tgn/7002445"/>
        <dc:spatial rdf:resource="http://dbpedia.org/resource/England"/>
        <skos:prefLabel xml:lang="en">Pelagic Trawling</skos:prefLabel>
        <skos:scopeNote xml:lang="en">Commercial fishing that involves trawling midwater levels of the water column targeting the pelagic fish species using large funnel shaped nets, held open at the mouth by floats and weights which are towed by one or two (pair trawling) vessels.</skos:scopeNote>
      </skos:Concept>
    </skos:narrower>

    <skos:narrower>
      <skos:Concept rdf:about="http://purl.org/heritagedata/schemes/571/concepts/151688">
        <skos:broader rdf:resource="http://purl.org/heritagedata/schemes/571/concepts/151683"/>
        <skos:inScheme rdf:resource="http://purl.org/heritagedata/schemes/571"/>
        <dc:identifier>http://purl.org/heritagedata/schemes/571/concepts/151688</dc:identifier>
        <dc:issued rdf:datatype="http://www.w3.org/2001/XMLSchema#dateTime">2024-07-01T17:17:33</dc:issued>
        <cc:license rdf:resource="https://www.nationalarchives.gov.uk/doc/open-government-licence/version/3/"/>
        <cc:attributionURL rdf:resource="https://historicengland.org.uk/"/>
        <cc:attributionName xml:lang="en">Historic England</cc:attributionName>
        <dc:publisher rdf:resource="https://historicengland.org.uk/"/>
        <dc:spatial rdf:resource="http://vocab.getty.edu/tgn/7002445"/>
        <dc:spatial rdf:resource="http://dbpedia.org/resource/England"/>
        <skos:prefLabel xml:lang="en">Drift Netting</skos:prefLabel>
        <skos:scopeNote xml:lang="en">Areas characterised by commercial fishing using large nets that drift in the water, moved by currents and lacking any fixtures to keep them in place. They are rigged in a straight line and are generally used to catch pelagic or migratory species.</skos:scopeNote>
      </skos:Concept>
    </skos:narrower>

    <skos:narrower>
      <skos:Concept rdf:about="http://purl.org/heritagedata/schemes/571/concepts/151690">
        <skos:broader rdf:resource="http://purl.org/heritagedata/schemes/571/concepts/151683"/>
        <skos:inScheme rdf:resource="http://purl.org/heritagedata/schemes/571"/>
        <dc:identifier>http://purl.org/heritagedata/schemes/571/concepts/151690</dc:identifier>
        <dc:issued rdf:datatype="http://www.w3.org/2001/XMLSchema#dateTime">2024-07-01T17:17:33</dc:issued>
        <cc:license rdf:resource="https://www.nationalarchives.gov.uk/doc/open-government-licence/version/3/"/>
        <cc:attributionURL rdf:resource="https://historicengland.org.uk/"/>
        <cc:attributionName xml:lang="en">Historic England</cc:attributionName>
        <dc:publisher rdf:resource="https://historicengland.org.uk/"/>
        <dc:spatial rdf:resource="http://vocab.getty.edu/tgn/7002445"/>
        <dc:spatial rdf:resource="http://dbpedia.org/resource/England"/>
        <skos:prefLabel xml:lang="en">Potting Area</skos:prefLabel>
        <skos:scopeNote xml:lang="en">Areas characterised by commercial fishing using pots or creels which are small portable traps set on the sea floor in coastal waters to catch a variety of crustacea and molluscs. Potting grounds, rarely more than a mile offshore usually on a rocky bottom.</skos:scopeNote>
      </skos:Concept>
    </skos:narrower>

    <skos:narrower>
      <skos:Concept rdf:about="http://purl.org/heritagedata/schemes/571/concepts/151692">
        <skos:broader rdf:resource="http://purl.org/heritagedata/schemes/571/concepts/151683"/>
        <skos:inScheme rdf:resource="http://purl.org/heritagedata/schemes/571"/>
        <dc:identifier>http://purl.org/heritagedata/schemes/571/concepts/151692</dc:identifier>
        <dc:issued rdf:datatype="http://www.w3.org/2001/XMLSchema#dateTime">2024-07-01T17:17:33</dc:issued>
        <cc:license rdf:resource="https://www.nationalarchives.gov.uk/doc/open-government-licence/version/3/"/>
        <cc:attributionURL rdf:resource="https://historicengland.org.uk/"/>
        <cc:attributionName xml:lang="en">Historic England</cc:attributionName>
        <dc:publisher rdf:resource="https://historicengland.org.uk/"/>
        <dc:spatial rdf:resource="http://vocab.getty.edu/tgn/7002445"/>
        <dc:spatial rdf:resource="http://dbpedia.org/resource/England"/>
        <skos:prefLabel xml:lang="en">Shellfish Dredging</skos:prefLabel>
        <skos:scopeNote xml:lang="en">Areas characterised by the regular commercial collection of naturally occurring shellfish stocks for food, bait or other products using a dredge towed behind a fishing vessel. In UK waters the target is usually scallops.</skos:scopeNote>
      </skos:Concept>
    </skos:narrower>

    <skos:narrower>
      <skos:Concept rdf:about="http://purl.org/heritagedata/schemes/571/concepts/151695">
        <skos:broader rdf:resource="http://purl.org/heritagedata/schemes/571/concepts/151683"/>
        <skos:inScheme rdf:resource="http://purl.org/heritagedata/schemes/571"/>
        <dc:identifier>http://purl.org/heritagedata/schemes/571/concepts/151695</dc:identifier>
        <dc:issued rdf:datatype="http://www.w3.org/2001/XMLSchema#dateTime">2024-07-01T17:17:33</dc:issued>
        <cc:license rdf:resource="https://www.nationalarchives.gov.uk/doc/open-government-licence/version/3/"/>
        <cc:attributionURL rdf:resource="https://historicengland.org.uk/"/>
        <cc:attributionName xml:lang="en">Historic England</cc:attributionName>
        <dc:publisher rdf:resource="https://historicengland.org.uk/"/>
        <dc:spatial rdf:resource="http://vocab.getty.edu/tgn/7002445"/>
        <dc:spatial rdf:resource="http://dbpedia.org/resource/England"/>
        <skos:prefLabel xml:lang="en">Bottom Trawling</skos:prefLabel>
        <skos:scopeNote xml:lang="en">Commercial fishing that involves trawling the lowest levels of the water column and/or the surface of the sea floor. These methods often result in disturbance to the sea floor itself.</skos:scopeNote>
      </skos:Concept>
    </skos:narrower>

    <skos:narrower>
      <skos:Concept rdf:about="http://purl.org/heritagedata/schemes/571/concepts/152544">
        <skos:broader rdf:resource="http://purl.org/heritagedata/schemes/571/concepts/151683"/>
        <skos:inScheme rdf:resource="http://purl.org/heritagedata/schemes/571"/>
        <dc:identifier>http://purl.org/heritagedata/schemes/571/concepts/152544</dc:identifier>
        <dc:issued rdf:datatype="http://www.w3.org/2001/XMLSchema#dateTime">2024-07-01T17:17:33</dc:issued>
        <cc:license rdf:resource="https://www.nationalarchives.gov.uk/doc/open-government-licence/version/3/"/>
        <cc:attributionURL rdf:resource="https://historicengland.org.uk/"/>
        <cc:attributionName xml:lang="en">Historic England</cc:attributionName>
        <dc:publisher rdf:resource="https://historicengland.org.uk/"/>
        <dc:spatial rdf:resource="http://vocab.getty.edu/tgn/7002445"/>
        <dc:spatial rdf:resource="http://dbpedia.org/resource/England"/>
        <skos:prefLabel xml:lang="en">Longlining</skos:prefLabel>
        <skos:scopeNote xml:lang="en">Areas characterised by commercial fishing using long line methods; this involves setting out a fishing line, often several kilometers long, from which shorter lines (snoods) are spaced at intervals with baited hooks.</skos:scopeNote>
      </skos:Concept>
    </skos:narrower>

    <skos:narrower>
      <skos:Concept rdf:about="http://purl.org/heritagedata/schemes/571/concepts/152545">
        <skos:broader rdf:resource="http://purl.org/heritagedata/schemes/571/concepts/151683"/>
        <skos:inScheme rdf:resource="http://purl.org/heritagedata/schemes/571"/>
        <dc:identifier>http://purl.org/heritagedata/schemes/571/concepts/152545</dc:identifier>
        <dc:issued rdf:datatype="http://www.w3.org/2001/XMLSchema#dateTime">2024-07-01T17:17:33</dc:issued>
        <cc:license rdf:resource="https://www.nationalarchives.gov.uk/doc/open-government-licence/version/3/"/>
        <cc:attributionURL rdf:resource="https://historicengland.org.uk/"/>
        <cc:attributionName xml:lang="en">Historic England</cc:attributionName>
        <dc:publisher rdf:resource="https://historicengland.org.uk/"/>
        <dc:spatial rdf:resource="http://vocab.getty.edu/tgn/7002445"/>
        <dc:spatial rdf:resource="http://dbpedia.org/resource/England"/>
        <skos:prefLabel xml:lang="en">Seine Netting</skos:prefLabel>
        <skos:scopeNote xml:lang="en">Areas characterised by commercial fishing using seine nets; which is a long net that hangs in the water column with floats along the upper edge and weights along the bottom. The ends of the net can be drawn together to encircle and herd a school of fish.</skos:scopeNote>
      </skos:Concept>
    </skos:narrower>

    <skos:narrower>
      <skos:Concept rdf:about="http://purl.org/heritagedata/schemes/571/concepts/152551">
        <skos:broader rdf:resource="http://purl.org/heritagedata/schemes/571/concepts/151683"/>
        <skos:inScheme rdf:resource="http://purl.org/heritagedata/schemes/571"/>
        <dc:identifier>http://purl.org/heritagedata/schemes/571/concepts/152551</dc:identifier>
        <dc:issued rdf:datatype="http://www.w3.org/2001/XMLSchema#dateTime">2024-07-01T17:17:33</dc:issued>
        <cc:license rdf:resource="https://www.nationalarchives.gov.uk/doc/open-government-licence/version/3/"/>
        <cc:attributionURL rdf:resource="https://historicengland.org.uk/"/>
        <cc:attributionName xml:lang="en">Historic England</cc:attributionName>
        <dc:publisher rdf:resource="https://historicengland.org.uk/"/>
        <dc:spatial rdf:resource="http://vocab.getty.edu/tgn/7002445"/>
        <dc:spatial rdf:resource="http://dbpedia.org/resource/England"/>
        <skos:prefLabel xml:lang="en">Fish Trapping</skos:prefLabel>
        <skos:scopeNote xml:lang="en">Areas characterised by the use of semi permanent/permanent fish traps for the capture of naturally occurring fish stocks. Does not include temporary portable pots and creels which are covered by POTTING AREA.</skos:scopeNote>
      </skos:Concept>
    </skos:narrower>

    <skos:narrower>
      <skos:Concept rdf:about="http://purl.org/heritagedata/schemes/571/concepts/152552">
        <skos:broader rdf:resource="http://purl.org/heritagedata/schemes/571/concepts/151683"/>
        <skos:inScheme rdf:resource="http://purl.org/heritagedata/schemes/571"/>
        <dc:identifier>http://purl.org/heritagedata/schemes/571/concepts/152552</dc:identifier>
        <dc:issued rdf:datatype="http://www.w3.org/2001/XMLSchema#dateTime">2024-07-01T17:17:33</dc:issued>
        <cc:license rdf:resource="https://www.nationalarchives.gov.uk/doc/open-government-licence/version/3/"/>
        <cc:attributionURL rdf:resource="https://historicengland.org.uk/"/>
        <cc:attributionName xml:lang="en">Historic England</cc:attributionName>
        <dc:publisher rdf:resource="https://historicengland.org.uk/"/>
        <dc:spatial rdf:resource="http://vocab.getty.edu/tgn/7002445"/>
        <dc:spatial rdf:resource="http://dbpedia.org/resource/England"/>
        <skos:prefLabel xml:lang="en">Shellfish Collection</skos:prefLabel>
        <skos:scopeNote xml:lang="en">Areas characterised by the regular commercial collection by hand or hand held tools, of naturally occurring shellfish stocks for food. If collected for bait use BAIT DIGGING AREA and for commercial farming from artificial structures use SHELLFISH FARMING.</skos:scopeNote>
      </skos:Concept>
    </skos:narrower>

    <skos:narrower>
      <skos:Concept rdf:about="http://purl.org/heritagedata/schemes/571/concepts/152553">
        <skos:broader rdf:resource="http://purl.org/heritagedata/schemes/571/concepts/151683"/>
        <skos:inScheme rdf:resource="http://purl.org/heritagedata/schemes/571"/>
        <dc:identifier>http://purl.org/heritagedata/schemes/571/concepts/152553</dc:identifier>
        <dc:issued rdf:datatype="http://www.w3.org/2001/XMLSchema#dateTime">2024-07-01T17:17:33</dc:issued>
        <cc:license rdf:resource="https://www.nationalarchives.gov.uk/doc/open-government-licence/version/3/"/>
        <cc:attributionURL rdf:resource="https://historicengland.org.uk/"/>
        <cc:attributionName xml:lang="en">Historic England</cc:attributionName>
        <dc:publisher rdf:resource="https://historicengland.org.uk/"/>
        <dc:spatial rdf:resource="http://vocab.getty.edu/tgn/7002445"/>
        <dc:spatial rdf:resource="http://dbpedia.org/resource/England"/>
        <skos:prefLabel xml:lang="en">Fixed Netting</skos:prefLabel>
        <skos:scopeNote xml:lang="en">Areas characterised by commercial fishing using fixed netting or set netting as it is sometimes known. It refers to netting held vertically and stationery in the water column, rather than being towed by a vessel or allowed to drift in the current.</skos:scopeNote>
      </skos:Concept>
    </skos:narrower>

    <skos:narrower>
      <skos:Concept rdf:about="http://purl.org/heritagedata/schemes/571/concepts/152555">
        <skos:broader rdf:resource="http://purl.org/heritagedata/schemes/571/concepts/151683"/>
        <skos:inScheme rdf:resource="http://purl.org/heritagedata/schemes/571"/>
        <dc:identifier>http://purl.org/heritagedata/schemes/571/concepts/152555</dc:identifier>
        <dc:issued rdf:datatype="http://www.w3.org/2001/XMLSchema#dateTime">2024-07-01T17:17:33</dc:issued>
        <cc:license rdf:resource="https://www.nationalarchives.gov.uk/doc/open-government-licence/version/3/"/>
        <cc:attributionURL rdf:resource="https://historicengland.org.uk/"/>
        <cc:attributionName xml:lang="en">Historic England</cc:attributionName>
        <dc:publisher rdf:resource="https://historicengland.org.uk/"/>
        <dc:spatial rdf:resource="http://vocab.getty.edu/tgn/7002445"/>
        <dc:spatial rdf:resource="http://dbpedia.org/resource/England"/>
        <skos:prefLabel xml:lang="en">Hand Netting</skos:prefLabel>
        <skos:scopeNote xml:lang="en">Areas characterised by commercial fishing using hand nets worked by an individual fisherman. This consists of a rectangular frame from which a net is suspended. Regional variations include haaf netting, lave netting and dip netting.</skos:scopeNote>
      </skos:Concept>
    </skos:narrower>

    <skos:broader rdf:resource="http://purl.org/heritagedata/schemes/571/concepts/151666"/>
    <skos:inScheme rdf:resource="http://purl.org/heritagedata/schemes/571"/>
    <dc:identifier>http://purl.org/heritagedata/schemes/571/concepts/151683</dc:identifier>
    <dc:issued rdf:datatype="http://www.w3.org/2001/XMLSchema#dateTime">2024-07-01T17:17:33</dc:issued>
    <cc:license rdf:resource="https://www.nationalarchives.gov.uk/doc/open-government-licence/version/3/"/>
    <cc:attributionURL rdf:resource="https://historicengland.org.uk/"/>
    <cc:attributionName xml:lang="en">Historic England</cc:attributionName>
    <dc:publisher rdf:resource="https://historicengland.org.uk/"/>
    <dc:spatial rdf:resource="http://vocab.getty.edu/tgn/7002445"/>
    <dc:spatial rdf:resource="http://dbpedia.org/resource/England"/>
    <skos:prefLabel xml:lang="en">Fishing</skos:prefLabel>
    <skos:scopeNote xml:lang="en">Activities concerned with the capture or gathering of wild fish and shellfish stocks by various methods such as trawling, netting, trapping, potting, dredging and collection by hand.</skos:scopeNote>
  </skos:Concept>

  <skos:Concept rdf:about="http://purl.org/heritagedata/schemes/571/concepts/151622">
    <skos:broader rdf:resource="http://purl.org/heritagedata/schemes/571/concepts/152549"/>
    <skos:inScheme rdf:resource="http://purl.org/heritagedata/schemes/571"/>
    <dc:identifier>http://purl.org/heritagedata/schemes/571/concepts/151622</dc:identifier>
    <dc:issued rdf:datatype="http://www.w3.org/2001/XMLSchema#dateTime">2024-07-01T17:17:33</dc:issued>
    <cc:license rdf:resource="https://www.nationalarchives.gov.uk/doc/open-government-licence/version/3/"/>
    <cc:attributionURL rdf:resource="https://historicengland.org.uk/"/>
    <cc:attributionName xml:lang="en">Historic England</cc:attributionName>
    <dc:publisher rdf:resource="https://historicengland.org.uk/"/>
    <dc:spatial rdf:resource="http://vocab.getty.edu/tgn/7002445"/>
    <dc:spatial rdf:resource="http://dbpedia.org/resource/England"/>
    <skos:prefLabel xml:lang="en">Fish Farming</skos:prefLabel>
    <skos:scopeNote xml:lang="en">Areas characterised by the commercial cultivation of fish populations under controlled conditions. These areas may be sited in inland or be coastally located artificial ponds, or in rivers, estuaries and the open sea and enclosed in tanks, cages or nets.</skos:scopeNote>
  </skos:Concept>

  <skos:Concept rdf:about="http://purl.org/heritagedata/schemes/571/concepts/152549">
    <skos:narrower rdf:resource="http://purl.org/heritagedata/schemes/571/concepts/151622"/>
    <skos:narrower>
      <skos:Concept rdf:about="http://purl.org/heritagedata/schemes/571/concepts/152550">
        <skos:broader rdf:resource="http://purl.org/heritagedata/schemes/571/concepts/152549"/>
        <skos:inScheme rdf:resource="http://purl.org/heritagedata/schemes/571"/>
        <dc:identifier>http://purl.org/heritagedata/schemes/571/concepts/152550</dc:identifier>
        <dc:issued rdf:datatype="http://www.w3.org/2001/XMLSchema#dateTime">2024-07-01T17:17:33</dc:issued>
        <cc:license rdf:resource="https://www.nationalarchives.gov.uk/doc/open-government-licence/version/3/"/>
        <cc:attributionURL rdf:resource="https://historicengland.org.uk/"/>
        <cc:attributionName xml:lang="en">Historic England</cc:attributionName>
        <dc:publisher rdf:resource="https://historicengland.org.uk/"/>
        <dc:spatial rdf:resource="http://vocab.getty.edu/tgn/7002445"/>
        <dc:spatial rdf:resource="http://dbpedia.org/resource/England"/>
        <skos:prefLabel xml:lang="en">Shellfish Farming</skos:prefLabel>
        <skos:scopeNote xml:lang="en">Areas chacterised by the commercial cultivation of shellfish populations under controlled conditions, sometimes enclosed from wild stocks. Shellfish farming includes oyster, mussel and cockle beds which are seeded and managed over several seasons.</skos:scopeNote>
      </skos:Concept>
    </skos:narrower>

    <skos:broader rdf:resource="http://purl.org/heritagedata/schemes/571/concepts/151666"/>
    <skos:inScheme rdf:resource="http://purl.org/heritagedata/schemes/571"/>
    <dc:identifier>http://purl.org/heritagedata/schemes/571/concepts/152549</dc:identifier>
    <dc:issued rdf:datatype="http://www.w3.org/2001/XMLSchema#dateTime">2024-07-01T17:17:33</dc:issued>
    <cc:license rdf:resource="https://www.nationalarchives.gov.uk/doc/open-government-licence/version/3/"/>
    <cc:attributionURL rdf:resource="https://historicengland.org.uk/"/>
    <cc:attributionName xml:lang="en">Historic England</cc:attributionName>
    <dc:publisher rdf:resource="https://historicengland.org.uk/"/>
    <dc:spatial rdf:resource="http://vocab.getty.edu/tgn/7002445"/>
    <dc:spatial rdf:resource="http://dbpedia.org/resource/England"/>
    <skos:prefLabel xml:lang="en">Aquaculture</skos:prefLabel>
    <skos:scopeNote xml:lang="en">The commercial cultivation of fish and shellfish populations under controlled conditions, often enclosed from wild stocks. It includes the raising of saltwater and/or freshwater species and may occur both inland or in fully marine situations.</skos:scopeNote>
  </skos:Concept>

  <skos:Concept rdf:about="http://purl.org/heritagedata/schemes/571/concepts/151631">
    <skos:narrower rdf:resource="http://purl.org/heritagedata/schemes/571/concepts/151630"/>
    <skos:narrower rdf:resource="http://purl.org/heritagedata/schemes/571/concepts/152577"/>
    <skos:broader rdf:resource="http://purl.org/heritagedata/schemes/571/concepts/151447"/>
    <skos:inScheme rdf:resource="http://purl.org/heritagedata/schemes/571"/>
    <dc:identifier>http://purl.org/heritagedata/schemes/571/concepts/151631</dc:identifier>
    <dc:issued rdf:datatype="http://www.w3.org/2001/XMLSchema#dateTime">2024-07-01T17:17:33</dc:issued>
    <cc:license rdf:resource="https://www.nationalarchives.gov.uk/doc/open-government-licence/version/3/"/>
    <cc:attributionURL rdf:resource="https://historicengland.org.uk/"/>
    <cc:attributionName xml:lang="en">Historic England</cc:attributionName>
    <dc:publisher rdf:resource="https://historicengland.org.uk/"/>
    <dc:spatial rdf:resource="http://vocab.getty.edu/tgn/7002445"/>
    <dc:spatial rdf:resource="http://dbpedia.org/resource/England"/>
    <skos:prefLabel xml:lang="en">Defence</skos:prefLabel>
    <skos:scopeNote xml:lang="en">Areas, sites and linked systems of such involved in the passive or active defence of the country against hostile forces on land, sea and in the air.</skos:scopeNote>
  </skos:Concept>

  <skos:Concept rdf:about="http://purl.org/heritagedata/schemes/571/concepts/151655">
    <skos:broader rdf:resource="http://purl.org/heritagedata/schemes/571/concepts/151090"/>
    <skos:inScheme rdf:resource="http://purl.org/heritagedata/schemes/571"/>
    <dc:identifier>http://purl.org/heritagedata/schemes/571/concepts/151655</dc:identifier>
    <dc:issued rdf:datatype="http://www.w3.org/2001/XMLSchema#dateTime">2024-07-01T17:17:33</dc:issued>
    <cc:license rdf:resource="https://www.nationalarchives.gov.uk/doc/open-government-licence/version/3/"/>
    <cc:attributionURL rdf:resource="https://historicengland.org.uk/"/>
    <cc:attributionName xml:lang="en">Historic England</cc:attributionName>
    <dc:publisher rdf:resource="https://historicengland.org.uk/"/>
    <dc:spatial rdf:resource="http://vocab.getty.edu/tgn/7002445"/>
    <dc:spatial rdf:resource="http://dbpedia.org/resource/England"/>
    <skos:prefLabel xml:lang="en">Canal Tunnel</skos:prefLabel>
    <skos:related rdf:resource="http://purl.org/heritagedata/schemes/571/concepts/151087"/>
    <skos:scopeNote xml:lang="en">A tunnel through which a canal runs.</skos:scopeNote>
  </skos:Concept>

  <skos:Concept rdf:about="http://purl.org/heritagedata/schemes/571/concepts/151679">
    <skos:broader rdf:resource="http://purl.org/heritagedata/schemes/571/concepts/152539"/>
    <skos:inScheme rdf:resource="http://purl.org/heritagedata/schemes/571"/>
    <dc:identifier>http://purl.org/heritagedata/schemes/571/concepts/151679</dc:identifier>
    <dc:issued rdf:datatype="http://www.w3.org/2001/XMLSchema#dateTime">2024-07-01T17:17:33</dc:issued>
    <cc:license rdf:resource="https://www.nationalarchives.gov.uk/doc/open-government-licence/version/3/"/>
    <cc:attributionURL rdf:resource="https://historicengland.org.uk/"/>
    <cc:attributionName xml:lang="en">Historic England</cc:attributionName>
    <dc:publisher rdf:resource="https://historicengland.org.uk/"/>
    <dc:spatial rdf:resource="http://vocab.getty.edu/tgn/7002445"/>
    <dc:spatial rdf:resource="http://dbpedia.org/resource/England"/>
    <skos:prefLabel xml:lang="en">Landmark Tower</skos:prefLabel>
    <skos:related rdf:resource="http://purl.org/heritagedata/schemes/571/concepts/152523"/>
    <skos:scopeNote xml:lang="en">A prominent structure situated on land specifically as a guide to navigation or warning to sailors.</skos:scopeNote>
  </skos:Concept>

  <skos:Concept rdf:about="http://purl.org/heritagedata/schemes/571/concepts/151700">
    <skos:broader rdf:resource="http://purl.org/heritagedata/schemes/571/concepts/151696"/>
    <skos:narrower>
      <skos:Concept rdf:about="http://purl.org/heritagedata/schemes/571/concepts/151701">
        <skos:broader rdf:resource="http://purl.org/heritagedata/schemes/571/concepts/151700"/>
        <skos:inScheme rdf:resource="http://purl.org/heritagedata/schemes/571"/>
        <dc:identifier>http://purl.org/heritagedata/schemes/571/concepts/151701</dc:identifier>
        <dc:issued rdf:datatype="http://www.w3.org/2001/XMLSchema#dateTime">2024-07-01T17:17:33</dc:issued>
        <cc:license rdf:resource="https://www.nationalarchives.gov.uk/doc/open-government-licence/version/3/"/>
        <cc:attributionURL rdf:resource="https://historicengland.org.uk/"/>
        <cc:attributionName xml:lang="en">Historic England</cc:attributionName>
        <dc:publisher rdf:resource="https://historicengland.org.uk/"/>
        <dc:spatial rdf:resource="http://vocab.getty.edu/tgn/7002445"/>
        <dc:spatial rdf:resource="http://dbpedia.org/resource/England"/>
        <skos:prefLabel xml:lang="en">National Government Office</skos:prefLabel>
        <skos:scopeNote xml:lang="en">A building which houses administrative functions relating to central government and its agencies. Includes directly associated and usually defined grounds.</skos:scopeNote>
      </skos:Concept>
    </skos:narrower>

    <skos:narrower>
      <skos:Concept rdf:about="http://purl.org/heritagedata/schemes/571/concepts/151702">
        <skos:broader rdf:resource="http://purl.org/heritagedata/schemes/571/concepts/151700"/>
        <skos:inScheme rdf:resource="http://purl.org/heritagedata/schemes/571"/>
        <dc:identifier>http://purl.org/heritagedata/schemes/571/concepts/151702</dc:identifier>
        <dc:issued rdf:datatype="http://www.w3.org/2001/XMLSchema#dateTime">2024-07-01T17:17:33</dc:issued>
        <cc:license rdf:resource="https://www.nationalarchives.gov.uk/doc/open-government-licence/version/3/"/>
        <cc:attributionURL rdf:resource="https://historicengland.org.uk/"/>
        <cc:attributionName xml:lang="en">Historic England</cc:attributionName>
        <dc:publisher rdf:resource="https://historicengland.org.uk/"/>
        <dc:spatial rdf:resource="http://vocab.getty.edu/tgn/7002445"/>
        <dc:spatial rdf:resource="http://dbpedia.org/resource/England"/>
        <skos:prefLabel xml:lang="en">Local Government Office</skos:prefLabel>
        <skos:scopeNote xml:lang="en">A building which houses administrative functions relating to local government. Includes directly associated and usually defined grounds.</skos:scopeNote>
      </skos:Concept>
    </skos:narrower>

    <skos:inScheme rdf:resource="http://purl.org/heritagedata/schemes/571"/>
    <dc:identifier>http://purl.org/heritagedata/schemes/571/concepts/151700</dc:identifier>
    <dc:issued rdf:datatype="http://www.w3.org/2001/XMLSchema#dateTime">2024-07-01T17:17:33</dc:issued>
    <cc:license rdf:resource="https://www.nationalarchives.gov.uk/doc/open-government-licence/version/3/"/>
    <cc:attributionURL rdf:resource="https://historicengland.org.uk/"/>
    <cc:attributionName xml:lang="en">Historic England</cc:attributionName>
    <dc:publisher rdf:resource="https://historicengland.org.uk/"/>
    <dc:spatial rdf:resource="http://vocab.getty.edu/tgn/7002445"/>
    <dc:spatial rdf:resource="http://dbpedia.org/resource/England"/>
    <skos:prefLabel xml:lang="en">Government Office</skos:prefLabel>
    <skos:scopeNote xml:lang="en">The offices and directly associated grounds of a Government Department responsible for the administration of the country or a part of it.</skos:scopeNote>
  </skos:Concept>

  <skos:Concept rdf:about="http://purl.org/heritagedata/schemes/571/concepts/151704">
    <skos:broader rdf:resource="http://purl.org/heritagedata/schemes/571/concepts/151697"/>
    <skos:narrower rdf:resource="http://purl.org/heritagedata/schemes/571/concepts/160274"/>
    <skos:inScheme rdf:resource="http://purl.org/heritagedata/schemes/571"/>
    <dc:identifier>http://purl.org/heritagedata/schemes/571/concepts/151704</dc:identifier>
    <dc:issued rdf:datatype="http://www.w3.org/2001/XMLSchema#dateTime">2024-07-01T17:17:33</dc:issued>
    <cc:license rdf:resource="https://www.nationalarchives.gov.uk/doc/open-government-licence/version/3/"/>
    <cc:attributionURL rdf:resource="https://historicengland.org.uk/"/>
    <cc:attributionName xml:lang="en">Historic England</cc:attributionName>
    <dc:publisher rdf:resource="https://historicengland.org.uk/"/>
    <dc:spatial rdf:resource="http://vocab.getty.edu/tgn/7002445"/>
    <dc:spatial rdf:resource="http://dbpedia.org/resource/England"/>
    <skos:prefLabel xml:lang="en">Museum Complex</skos:prefLabel>
    <skos:related rdf:resource="http://purl.org/heritagedata/schemes/571/concepts/151705"/>
    <skos:scopeNote xml:lang="en">A building, group of buildings or space within a building, where objects of value such as works of art, antiquities, scientific specimens, or other artefacts are housed, conserved and displayed. Includes directly associated and usually defined grounds.</skos:scopeNote>
  </skos:Concept>

  <skos:Concept rdf:about="http://purl.org/heritagedata/schemes/571/concepts/151705">
    <skos:broader rdf:resource="http://purl.org/heritagedata/schemes/571/concepts/151697"/>
    <skos:inScheme rdf:resource="http://purl.org/heritagedata/schemes/571"/>
    <dc:identifier>http://purl.org/heritagedata/schemes/571/concepts/151705</dc:identifier>
    <dc:issued rdf:datatype="http://www.w3.org/2001/XMLSchema#dateTime">2024-07-01T17:17:33</dc:issued>
    <cc:license rdf:resource="https://www.nationalarchives.gov.uk/doc/open-government-licence/version/3/"/>
    <cc:attributionURL rdf:resource="https://historicengland.org.uk/"/>
    <cc:attributionName xml:lang="en">Historic England</cc:attributionName>
    <dc:publisher rdf:resource="https://historicengland.org.uk/"/>
    <dc:spatial rdf:resource="http://vocab.getty.edu/tgn/7002445"/>
    <dc:spatial rdf:resource="http://dbpedia.org/resource/England"/>
    <skos:prefLabel xml:lang="en">Gallery Complex</skos:prefLabel>
    <skos:related rdf:resource="http://purl.org/heritagedata/schemes/571/concepts/151704"/>
    <skos:scopeNote xml:lang="en">A building in which works of art are displayed, permanently or temporarily.</skos:scopeNote>
  </skos:Concept>

  <skos:Concept rdf:about="http://purl.org/heritagedata/schemes/571/concepts/160130">
    <skos:narrower rdf:resource="http://purl.org/heritagedata/schemes/571/concepts/151707"/>
    <skos:narrower>
      <skos:Concept rdf:about="http://purl.org/heritagedata/schemes/571/concepts/160131">
        <skos:broader rdf:resource="http://purl.org/heritagedata/schemes/571/concepts/160130"/>
        <skos:inScheme rdf:resource="http://purl.org/heritagedata/schemes/571"/>
        <dc:identifier>http://purl.org/heritagedata/schemes/571/concepts/160131</dc:identifier>
        <dc:issued rdf:datatype="http://www.w3.org/2001/XMLSchema#dateTime">2024-07-01T17:17:33</dc:issued>
        <cc:license rdf:resource="https://www.nationalarchives.gov.uk/doc/open-government-licence/version/3/"/>
        <cc:attributionURL rdf:resource="https://historicengland.org.uk/"/>
        <cc:attributionName xml:lang="en">Historic England</cc:attributionName>
        <dc:publisher rdf:resource="https://historicengland.org.uk/"/>
        <dc:spatial rdf:resource="http://vocab.getty.edu/tgn/7002445"/>
        <dc:spatial rdf:resource="http://dbpedia.org/resource/England"/>
        <skos:prefLabel xml:lang="en">Religious Community</skos:prefLabel>
        <skos:scopeNote xml:lang="en">Buildings and grounds where a group of devotees to a religion live and worship. Subdivide by form of religion, sect, etc.</skos:scopeNote>
      </skos:Concept>
    </skos:narrower>

    <skos:broader rdf:resource="http://purl.org/heritagedata/schemes/571/concepts/151459"/>
    <skos:inScheme rdf:resource="http://purl.org/heritagedata/schemes/571"/>
    <dc:identifier>http://purl.org/heritagedata/schemes/571/concepts/160130</dc:identifier>
    <dc:issued rdf:datatype="http://www.w3.org/2001/XMLSchema#dateTime">2024-07-01T17:17:33</dc:issued>
    <cc:license rdf:resource="https://www.nationalarchives.gov.uk/doc/open-government-licence/version/3/"/>
    <cc:attributionURL rdf:resource="https://historicengland.org.uk/"/>
    <cc:attributionName xml:lang="en">Historic England</cc:attributionName>
    <dc:publisher rdf:resource="https://historicengland.org.uk/"/>
    <dc:spatial rdf:resource="http://vocab.getty.edu/tgn/7002445"/>
    <dc:spatial rdf:resource="http://dbpedia.org/resource/England"/>
    <skos:prefLabel xml:lang="en">Religion</skos:prefLabel>
    <skos:scopeNote xml:lang="en">Organised public system, often involving agreed symbols and behaviours, relating humanity to particular beliefs and values. Often links explanatory schemes (for example of the origin and meaning of life) to morality and ethics.</skos:scopeNote>
  </skos:Concept>

  <skos:Concept rdf:about="http://purl.org/heritagedata/schemes/571/concepts/151708">
    <skos:broader rdf:resource="http://purl.org/heritagedata/schemes/571/concepts/151707"/>
    <skos:inScheme rdf:resource="http://purl.org/heritagedata/schemes/571"/>
    <dc:identifier>http://purl.org/heritagedata/schemes/571/concepts/151708</dc:identifier>
    <dc:issued rdf:datatype="http://www.w3.org/2001/XMLSchema#dateTime">2024-07-01T17:17:33</dc:issued>
    <cc:license rdf:resource="https://www.nationalarchives.gov.uk/doc/open-government-licence/version/3/"/>
    <cc:attributionURL rdf:resource="https://historicengland.org.uk/"/>
    <cc:attributionName xml:lang="en">Historic England</cc:attributionName>
    <dc:publisher rdf:resource="https://historicengland.org.uk/"/>
    <dc:spatial rdf:resource="http://vocab.getty.edu/tgn/7002445"/>
    <dc:spatial rdf:resource="http://dbpedia.org/resource/England"/>
    <skos:prefLabel xml:lang="en">Cathedral</skos:prefLabel>
    <skos:related rdf:resource="http://purl.org/heritagedata/schemes/571/concepts/151577"/>
    <skos:scopeNote xml:lang="en">The principal church of a diocese in which the cathedra or bishop's throne is to be found. Includes precinct and immediately related features.</skos:scopeNote>
  </skos:Concept>

  <skos:Concept rdf:about="http://purl.org/heritagedata/schemes/571/concepts/151710">
    <skos:broader rdf:resource="http://purl.org/heritagedata/schemes/571/concepts/160133"/>
    <skos:broader rdf:resource="http://purl.org/heritagedata/schemes/571/concepts/151667"/>
    <skos:narrower>
      <skos:Concept rdf:about="http://purl.org/heritagedata/schemes/571/concepts/152548">
        <skos:broader rdf:resource="http://purl.org/heritagedata/schemes/571/concepts/151710"/>
        <skos:inScheme rdf:resource="http://purl.org/heritagedata/schemes/571"/>
        <dc:identifier>http://purl.org/heritagedata/schemes/571/concepts/152548</dc:identifier>
        <dc:issued rdf:datatype="http://www.w3.org/2001/XMLSchema#dateTime">2024-07-01T17:17:33</dc:issued>
        <cc:license rdf:resource="https://www.nationalarchives.gov.uk/doc/open-government-licence/version/3/"/>
        <cc:attributionURL rdf:resource="https://historicengland.org.uk/"/>
        <cc:attributionName xml:lang="en">Historic England</cc:attributionName>
        <dc:publisher rdf:resource="https://historicengland.org.uk/"/>
        <dc:spatial rdf:resource="http://vocab.getty.edu/tgn/7002445"/>
        <dc:spatial rdf:resource="http://dbpedia.org/resource/England"/>
        <skos:prefLabel xml:lang="en">Fish Warehouse</skos:prefLabel>
        <skos:scopeNote xml:lang="en">Buildings &amp; grounds used specifically for storage of fish or fish products. Such storage may relate to several aspects of the fishing industry, for example the storage of fish after landing &amp; before auction or sale, or the cold storage of fish after sale.</skos:scopeNote>
      </skos:Concept>
    </skos:narrower>

    <skos:inScheme rdf:resource="http://purl.org/heritagedata/schemes/571"/>
    <dc:identifier>http://purl.org/heritagedata/schemes/571/concepts/151710</dc:identifier>
    <dc:issued rdf:datatype="http://www.w3.org/2001/XMLSchema#dateTime">2024-07-01T17:17:33</dc:issued>
    <cc:license rdf:resource="https://www.nationalarchives.gov.uk/doc/open-government-licence/version/3/"/>
    <cc:attributionURL rdf:resource="https://historicengland.org.uk/"/>
    <cc:attributionName xml:lang="en">Historic England</cc:attributionName>
    <dc:publisher rdf:resource="https://historicengland.org.uk/"/>
    <dc:spatial rdf:resource="http://vocab.getty.edu/tgn/7002445"/>
    <dc:spatial rdf:resource="http://dbpedia.org/resource/England"/>
    <skos:prefLabel xml:lang="en">Warehousing</skos:prefLabel>
    <skos:scopeNote xml:lang="en">A building or part of a building and directly associated grounds, used for the storage of goods or merchandise.</skos:scopeNote>
  </skos:Concept>

  <skos:Concept rdf:about="http://purl.org/heritagedata/schemes/571/concepts/160133">
    <skos:narrower rdf:resource="http://purl.org/heritagedata/schemes/571/concepts/151710"/>
    <skos:narrower>
      <skos:Concept rdf:about="http://purl.org/heritagedata/schemes/571/concepts/151711">
        <skos:broader rdf:resource="http://purl.org/heritagedata/schemes/571/concepts/160133"/>
        <skos:inScheme rdf:resource="http://purl.org/heritagedata/schemes/571"/>
        <dc:identifier>http://purl.org/heritagedata/schemes/571/concepts/151711</dc:identifier>
        <dc:issued rdf:datatype="http://www.w3.org/2001/XMLSchema#dateTime">2024-07-01T17:17:33</dc:issued>
        <cc:license rdf:resource="https://www.nationalarchives.gov.uk/doc/open-government-licence/version/3/"/>
        <cc:attributionURL rdf:resource="https://historicengland.org.uk/"/>
        <cc:attributionName xml:lang="en">Historic England</cc:attributionName>
        <dc:publisher rdf:resource="https://historicengland.org.uk/"/>
        <dc:spatial rdf:resource="http://vocab.getty.edu/tgn/7002445"/>
        <dc:spatial rdf:resource="http://dbpedia.org/resource/England"/>
        <skos:prefLabel xml:lang="en">Motor Vehicle Storage</skos:prefLabel>
        <skos:scopeNote xml:lang="en">An area where motor vehicles are stored, often associated with commerce.</skos:scopeNote>
      </skos:Concept>
    </skos:narrower>

    <skos:narrower>
      <skos:Concept rdf:about="http://purl.org/heritagedata/schemes/571/concepts/151713">
        <skos:broader rdf:resource="http://purl.org/heritagedata/schemes/571/concepts/160133"/>
        <skos:inScheme rdf:resource="http://purl.org/heritagedata/schemes/571"/>
        <dc:identifier>http://purl.org/heritagedata/schemes/571/concepts/151713</dc:identifier>
        <dc:issued rdf:datatype="http://www.w3.org/2001/XMLSchema#dateTime">2024-07-01T17:17:33</dc:issued>
        <cc:license rdf:resource="https://www.nationalarchives.gov.uk/doc/open-government-licence/version/3/"/>
        <cc:attributionURL rdf:resource="https://historicengland.org.uk/"/>
        <cc:attributionName xml:lang="en">Historic England</cc:attributionName>
        <dc:publisher rdf:resource="https://historicengland.org.uk/"/>
        <dc:spatial rdf:resource="http://vocab.getty.edu/tgn/7002445"/>
        <dc:spatial rdf:resource="http://dbpedia.org/resource/England"/>
        <skos:prefLabel xml:lang="en">Freight Handling</skos:prefLabel>
        <skos:scopeNote xml:lang="en">Sites and structures associated with the handling of commercial cargo.</skos:scopeNote>
      </skos:Concept>
    </skos:narrower>

    <skos:broader rdf:resource="http://purl.org/heritagedata/schemes/571/concepts/151458"/>
    <skos:inScheme rdf:resource="http://purl.org/heritagedata/schemes/571"/>
    <dc:identifier>http://purl.org/heritagedata/schemes/571/concepts/160133</dc:identifier>
    <dc:issued rdf:datatype="http://www.w3.org/2001/XMLSchema#dateTime">2024-07-01T17:17:33</dc:issued>
    <cc:license rdf:resource="https://www.nationalarchives.gov.uk/doc/open-government-licence/version/3/"/>
    <cc:attributionURL rdf:resource="https://historicengland.org.uk/"/>
    <cc:attributionName xml:lang="en">Historic England</cc:attributionName>
    <dc:publisher rdf:resource="https://historicengland.org.uk/"/>
    <dc:spatial rdf:resource="http://vocab.getty.edu/tgn/7002445"/>
    <dc:spatial rdf:resource="http://dbpedia.org/resource/England"/>
    <skos:prefLabel xml:lang="en">Storage And Handling</skos:prefLabel>
    <skos:scopeNote xml:lang="en">Facilities (buildings and directly associated grounds) for the storage of goods.</skos:scopeNote>
  </skos:Concept>

  <skos:Concept rdf:about="http://purl.org/heritagedata/schemes/571/concepts/151460">
    <skos:narrower rdf:resource="http://purl.org/heritagedata/schemes/571/concepts/151715"/>
    <skos:narrower rdf:resource="http://purl.org/heritagedata/schemes/571/concepts/151717"/>
    <skos:narrower rdf:resource="http://purl.org/heritagedata/schemes/571/concepts/152561"/>
    <skos:inScheme rdf:resource="http://purl.org/heritagedata/schemes/571"/>
    <dc:identifier>http://purl.org/heritagedata/schemes/571/concepts/151460</dc:identifier>
    <dc:issued rdf:datatype="http://www.w3.org/2001/XMLSchema#dateTime">2024-07-01T17:17:33</dc:issued>
    <cc:license rdf:resource="https://www.nationalarchives.gov.uk/doc/open-government-licence/version/3/"/>
    <cc:attributionURL rdf:resource="https://historicengland.org.uk/"/>
    <cc:attributionName xml:lang="en">Historic England</cc:attributionName>
    <dc:publisher rdf:resource="https://historicengland.org.uk/"/>
    <dc:spatial rdf:resource="http://vocab.getty.edu/tgn/7002445"/>
    <dc:spatial rdf:resource="http://dbpedia.org/resource/England"/>
    <skos:prefLabel xml:lang="en">Civic Amenities</skos:prefLabel>
    <skos:scopeNote xml:lang="en">-</skos:scopeNote>
    <skos:topConceptOf rdf:resource="http://purl.org/heritagedata/schemes/571"/>
  </skos:Concept>

  <skos:Concept rdf:about="http://purl.org/heritagedata/schemes/571/concepts/151730">
    <skos:narrower rdf:resource="http://purl.org/heritagedata/schemes/571/concepts/151728"/>
    <skos:narrower>
      <skos:Concept rdf:about="http://purl.org/heritagedata/schemes/571/concepts/151731">
        <skos:broader rdf:resource="http://purl.org/heritagedata/schemes/571/concepts/151730"/>
        <skos:inScheme rdf:resource="http://purl.org/heritagedata/schemes/571"/>
        <dc:identifier>http://purl.org/heritagedata/schemes/571/concepts/151731</dc:identifier>
        <dc:issued rdf:datatype="http://www.w3.org/2001/XMLSchema#dateTime">2024-07-01T17:17:33</dc:issued>
        <cc:license rdf:resource="https://www.nationalarchives.gov.uk/doc/open-government-licence/version/3/"/>
        <cc:attributionURL rdf:resource="https://historicengland.org.uk/"/>
        <cc:attributionName xml:lang="en">Historic England</cc:attributionName>
        <dc:publisher rdf:resource="https://historicengland.org.uk/"/>
        <dc:spatial rdf:resource="http://vocab.getty.edu/tgn/7002445"/>
        <dc:spatial rdf:resource="http://dbpedia.org/resource/England"/>
        <skos:prefLabel xml:lang="en">Irregular Ancient Enclosure</skos:prefLabel>
        <skos:scopeNote xml:lang="en">Area of ancient fields whose boundaries are either curving or sinuous and whose shapes do not conform to a regular pattern. Often seen to have developed by sequential accretion of individual enclosures and by ad hoc subdivision.</skos:scopeNote>
      </skos:Concept>
    </skos:narrower>

    <skos:narrower rdf:resource="http://purl.org/heritagedata/schemes/571/concepts/160158"/>
    <skos:broader rdf:resource="http://purl.org/heritagedata/schemes/571/concepts/151453"/>
    <skos:inScheme rdf:resource="http://purl.org/heritagedata/schemes/571"/>
    <dc:identifier>http://purl.org/heritagedata/schemes/571/concepts/151730</dc:identifier>
    <dc:issued rdf:datatype="http://www.w3.org/2001/XMLSchema#dateTime">2024-07-01T17:17:33</dc:issued>
    <cc:license rdf:resource="https://www.nationalarchives.gov.uk/doc/open-government-licence/version/3/"/>
    <cc:attributionURL rdf:resource="https://historicengland.org.uk/"/>
    <cc:attributionName xml:lang="en">Historic England</cc:attributionName>
    <dc:publisher rdf:resource="https://historicengland.org.uk/"/>
    <dc:spatial rdf:resource="http://vocab.getty.edu/tgn/7002445"/>
    <dc:spatial rdf:resource="http://dbpedia.org/resource/England"/>
    <skos:prefLabel xml:lang="en">Ancient Enclosure</skos:prefLabel>
    <skos:related rdf:resource="http://purl.org/heritagedata/schemes/571/concepts/160155"/>
    <skos:scopeNote xml:lang="en">Fields that can be demonstrated by to be either prehistoric or early medieval in origin by virtue of either form or direct association with early farming settlement.</skos:scopeNote>
  </skos:Concept>

  <skos:Concept rdf:about="http://purl.org/heritagedata/schemes/571/concepts/151735">
    <skos:broader rdf:resource="http://purl.org/heritagedata/schemes/571/concepts/151461"/>
    <skos:inScheme rdf:resource="http://purl.org/heritagedata/schemes/571"/>
    <dc:identifier>http://purl.org/heritagedata/schemes/571/concepts/151735</dc:identifier>
    <dc:issued rdf:datatype="http://www.w3.org/2001/XMLSchema#dateTime">2024-07-01T17:17:33</dc:issued>
    <cc:license rdf:resource="https://www.nationalarchives.gov.uk/doc/open-government-licence/version/3/"/>
    <cc:attributionURL rdf:resource="https://historicengland.org.uk/"/>
    <cc:attributionName xml:lang="en">Historic England</cc:attributionName>
    <dc:publisher rdf:resource="https://historicengland.org.uk/"/>
    <dc:spatial rdf:resource="http://vocab.getty.edu/tgn/7002445"/>
    <dc:spatial rdf:resource="http://dbpedia.org/resource/England"/>
    <skos:prefLabel xml:lang="en">Flash</skos:prefLabel>
    <skos:related rdf:resource="http://purl.org/heritagedata/schemes/571/concepts/151736"/>
    <skos:scopeNote xml:lang="en">A water filled hollow caused by subsidence resulting from subterranean industrial extraction, for example coal mining and salt extraction.</skos:scopeNote>
  </skos:Concept>

  <skos:Concept rdf:about="http://purl.org/heritagedata/schemes/571/concepts/151736">
    <skos:broader rdf:resource="http://purl.org/heritagedata/schemes/571/concepts/151422"/>
    <skos:inScheme rdf:resource="http://purl.org/heritagedata/schemes/571"/>
    <dc:identifier>http://purl.org/heritagedata/schemes/571/concepts/151736</dc:identifier>
    <dc:issued rdf:datatype="http://www.w3.org/2001/XMLSchema#dateTime">2024-07-01T17:17:33</dc:issued>
    <cc:license rdf:resource="https://www.nationalarchives.gov.uk/doc/open-government-licence/version/3/"/>
    <cc:attributionURL rdf:resource="https://historicengland.org.uk/"/>
    <cc:attributionName xml:lang="en">Historic England</cc:attributionName>
    <dc:publisher rdf:resource="https://historicengland.org.uk/"/>
    <dc:spatial rdf:resource="http://vocab.getty.edu/tgn/7002445"/>
    <dc:spatial rdf:resource="http://dbpedia.org/resource/England"/>
    <skos:prefLabel xml:lang="en">Salt Mine</skos:prefLabel>
    <skos:related rdf:resource="http://purl.org/heritagedata/schemes/571/concepts/151735"/>
    <skos:scopeNote xml:lang="en">A mine yielding rock salt extracted either as rock salt or pumped out as brine.</skos:scopeNote>
  </skos:Concept>

  <skos:Concept rdf:about="http://purl.org/heritagedata/schemes/571/concepts/151738">
    <skos:broader rdf:resource="http://purl.org/heritagedata/schemes/571/concepts/151461"/>
    <skos:narrower>
      <skos:Concept rdf:about="http://purl.org/heritagedata/schemes/571/concepts/151739">
        <skos:broader rdf:resource="http://purl.org/heritagedata/schemes/571/concepts/151738"/>
        <skos:inScheme rdf:resource="http://purl.org/heritagedata/schemes/571"/>
        <dc:identifier>http://purl.org/heritagedata/schemes/571/concepts/151739</dc:identifier>
        <dc:issued rdf:datatype="http://www.w3.org/2001/XMLSchema#dateTime">2024-07-01T17:17:33</dc:issued>
        <cc:license rdf:resource="https://www.nationalarchives.gov.uk/doc/open-government-licence/version/3/"/>
        <cc:attributionURL rdf:resource="https://historicengland.org.uk/"/>
        <cc:attributionName xml:lang="en">Historic England</cc:attributionName>
        <dc:publisher rdf:resource="https://historicengland.org.uk/"/>
        <dc:spatial rdf:resource="http://vocab.getty.edu/tgn/7002445"/>
        <dc:spatial rdf:resource="http://dbpedia.org/resource/England"/>
        <skos:prefLabel xml:lang="en">Natural Gas Rig</skos:prefLabel>
        <skos:scopeNote xml:lang="en">A supporting structure for drilling machinery used in the extraction of, or prospecting for, natural gas.</skos:scopeNote>
      </skos:Concept>
    </skos:narrower>

    <skos:narrower>
      <skos:Concept rdf:about="http://purl.org/heritagedata/schemes/571/concepts/151740">
        <skos:broader rdf:resource="http://purl.org/heritagedata/schemes/571/concepts/151738"/>
        <skos:inScheme rdf:resource="http://purl.org/heritagedata/schemes/571"/>
        <dc:identifier>http://purl.org/heritagedata/schemes/571/concepts/151740</dc:identifier>
        <dc:issued rdf:datatype="http://www.w3.org/2001/XMLSchema#dateTime">2024-07-01T17:17:33</dc:issued>
        <cc:license rdf:resource="https://www.nationalarchives.gov.uk/doc/open-government-licence/version/3/"/>
        <cc:attributionURL rdf:resource="https://historicengland.org.uk/"/>
        <cc:attributionName xml:lang="en">Historic England</cc:attributionName>
        <dc:publisher rdf:resource="https://historicengland.org.uk/"/>
        <dc:spatial rdf:resource="http://vocab.getty.edu/tgn/7002445"/>
        <dc:spatial rdf:resource="http://dbpedia.org/resource/England"/>
        <skos:prefLabel xml:lang="en">Natural Gas Refinery</skos:prefLabel>
        <skos:scopeNote xml:lang="en">A plant used to purify the raw natural gas produced from underground gas fields to deliver pipeline-quality natural gas that can be used as a domestic and/or industrial fuel.</skos:scopeNote>
      </skos:Concept>
    </skos:narrower>

    <skos:inScheme rdf:resource="http://purl.org/heritagedata/schemes/571"/>
    <dc:identifier>http://purl.org/heritagedata/schemes/571/concepts/151738</dc:identifier>
    <dc:issued rdf:datatype="http://www.w3.org/2001/XMLSchema#dateTime">2024-07-01T17:17:33</dc:issued>
    <cc:license rdf:resource="https://www.nationalarchives.gov.uk/doc/open-government-licence/version/3/"/>
    <cc:attributionURL rdf:resource="https://historicengland.org.uk/"/>
    <cc:attributionName xml:lang="en">Historic England</cc:attributionName>
    <dc:publisher rdf:resource="https://historicengland.org.uk/"/>
    <dc:spatial rdf:resource="http://vocab.getty.edu/tgn/7002445"/>
    <dc:spatial rdf:resource="http://dbpedia.org/resource/England"/>
    <skos:prefLabel xml:lang="en">Natural Gas Production</skos:prefLabel>
    <skos:related rdf:resource="http://purl.org/heritagedata/schemes/571/concepts/151136"/>
    <skos:scopeNote xml:lang="en">Buildings, sites and structures associated with the retrieval, refining, processing and storage of natural gas.</skos:scopeNote>
  </skos:Concept>

  <skos:Concept rdf:about="http://purl.org/heritagedata/schemes/571/concepts/151744">
    <skos:broader rdf:resource="http://purl.org/heritagedata/schemes/571/concepts/151461"/>
    <skos:inScheme rdf:resource="http://purl.org/heritagedata/schemes/571"/>
    <dc:identifier>http://purl.org/heritagedata/schemes/571/concepts/151744</dc:identifier>
    <dc:issued rdf:datatype="http://www.w3.org/2001/XMLSchema#dateTime">2024-07-01T17:17:33</dc:issued>
    <cc:license rdf:resource="https://www.nationalarchives.gov.uk/doc/open-government-licence/version/3/"/>
    <cc:attributionURL rdf:resource="https://historicengland.org.uk/"/>
    <cc:attributionName xml:lang="en">Historic England</cc:attributionName>
    <dc:publisher rdf:resource="https://historicengland.org.uk/"/>
    <dc:spatial rdf:resource="http://vocab.getty.edu/tgn/7002445"/>
    <dc:spatial rdf:resource="http://dbpedia.org/resource/England"/>
    <skos:prefLabel xml:lang="en">Shafthead Complex</skos:prefLabel>
    <skos:related rdf:resource="http://purl.org/heritagedata/schemes/571/concepts/151422"/>
    <skos:scopeNote xml:lang="en">Buildings found at the site of a mine at the point where underground workings meet the surface.</skos:scopeNote>
  </skos:Concept>

  <skos:Concept rdf:about="http://purl.org/heritagedata/schemes/571/concepts/151746">
    <skos:broader rdf:resource="http://purl.org/heritagedata/schemes/571/concepts/152605"/>
    <skos:inScheme rdf:resource="http://purl.org/heritagedata/schemes/571"/>
    <dc:identifier>http://purl.org/heritagedata/schemes/571/concepts/151746</dc:identifier>
    <dc:issued rdf:datatype="http://www.w3.org/2001/XMLSchema#dateTime">2024-07-01T17:17:33</dc:issued>
    <cc:license rdf:resource="https://www.nationalarchives.gov.uk/doc/open-government-licence/version/3/"/>
    <cc:attributionURL rdf:resource="https://historicengland.org.uk/"/>
    <cc:attributionName xml:lang="en">Historic England</cc:attributionName>
    <dc:publisher rdf:resource="https://historicengland.org.uk/"/>
    <dc:spatial rdf:resource="http://vocab.getty.edu/tgn/7002445"/>
    <dc:spatial rdf:resource="http://dbpedia.org/resource/England"/>
    <skos:prefLabel xml:lang="en">Electricity Distribution</skos:prefLabel>
    <skos:related rdf:resource="http://purl.org/heritagedata/schemes/571/concepts/152620"/>
    <skos:related rdf:resource="http://purl.org/heritagedata/schemes/571/concepts/152621"/>
    <skos:scopeNote xml:lang="en">Buildings, sites and structures associated with the distribution of electricity.</skos:scopeNote>
  </skos:Concept>

  <skos:Concept rdf:about="http://purl.org/heritagedata/schemes/571/concepts/151767">
    <skos:broader rdf:resource="http://purl.org/heritagedata/schemes/571/concepts/151596"/>
    <skos:inScheme rdf:resource="http://purl.org/heritagedata/schemes/571"/>
    <dc:identifier>http://purl.org/heritagedata/schemes/571/concepts/151767</dc:identifier>
    <dc:issued rdf:datatype="http://www.w3.org/2001/XMLSchema#dateTime">2024-07-01T17:17:33</dc:issued>
    <cc:license rdf:resource="https://www.nationalarchives.gov.uk/doc/open-government-licence/version/3/"/>
    <cc:attributionURL rdf:resource="https://historicengland.org.uk/"/>
    <cc:attributionName xml:lang="en">Historic England</cc:attributionName>
    <dc:publisher rdf:resource="https://historicengland.org.uk/"/>
    <dc:spatial rdf:resource="http://vocab.getty.edu/tgn/7002445"/>
    <dc:spatial rdf:resource="http://dbpedia.org/resource/England"/>
    <skos:prefLabel xml:lang="en">Common Edge Village</skos:prefLabel>
    <skos:related rdf:resource="http://purl.org/heritagedata/schemes/571/concepts/151264"/>
    <skos:scopeNote xml:lang="en">Agricultural village with farmsteads and cottages wholly or mainly arranged along the edge of a common.</skos:scopeNote>
  </skos:Concept>

  <skos:Concept rdf:about="http://purl.org/heritagedata/schemes/571/concepts/151780">
    <skos:broader rdf:resource="http://purl.org/heritagedata/schemes/571/concepts/151727"/>
    <skos:narrower rdf:resource="http://purl.org/heritagedata/schemes/571/concepts/151781"/>
    <skos:narrower>
      <skos:Concept rdf:about="http://purl.org/heritagedata/schemes/571/concepts/160167">
        <skos:broader rdf:resource="http://purl.org/heritagedata/schemes/571/concepts/151780"/>
        <skos:inScheme rdf:resource="http://purl.org/heritagedata/schemes/571"/>
        <dc:identifier>http://purl.org/heritagedata/schemes/571/concepts/160167</dc:identifier>
        <dc:issued rdf:datatype="http://www.w3.org/2001/XMLSchema#dateTime">2024-07-01T17:17:33</dc:issued>
        <cc:license rdf:resource="https://www.nationalarchives.gov.uk/doc/open-government-licence/version/3/"/>
        <cc:attributionURL rdf:resource="https://historicengland.org.uk/"/>
        <cc:attributionName xml:lang="en">Historic England</cc:attributionName>
        <dc:publisher rdf:resource="https://historicengland.org.uk/"/>
        <dc:spatial rdf:resource="http://vocab.getty.edu/tgn/7002445"/>
        <dc:spatial rdf:resource="http://dbpedia.org/resource/England"/>
        <skos:prefLabel xml:lang="en">Strip Fields</skos:prefLabel>
        <skos:scopeNote xml:lang="en">Long narrow plots of land within an open field. Also used for those plots once enclosed and held in severalty, the form in which most now survive.</skos:scopeNote>
      </skos:Concept>
    </skos:narrower>

    <skos:inScheme rdf:resource="http://purl.org/heritagedata/schemes/571"/>
    <dc:identifier>http://purl.org/heritagedata/schemes/571/concepts/151780</dc:identifier>
    <dc:issued rdf:datatype="http://www.w3.org/2001/XMLSchema#dateTime">2024-07-01T17:17:33</dc:issued>
    <cc:license rdf:resource="https://www.nationalarchives.gov.uk/doc/open-government-licence/version/3/"/>
    <cc:attributionURL rdf:resource="https://historicengland.org.uk/"/>
    <cc:attributionName xml:lang="en">Historic England</cc:attributionName>
    <dc:publisher rdf:resource="https://historicengland.org.uk/"/>
    <dc:spatial rdf:resource="http://vocab.getty.edu/tgn/7002445"/>
    <dc:spatial rdf:resource="http://dbpedia.org/resource/England"/>
    <skos:prefLabel xml:lang="en">Piecemeal Enclosure</skos:prefLabel>
    <skos:related rdf:resource="http://purl.org/heritagedata/schemes/571/concepts/160155"/>
    <skos:scopeNote xml:lang="en">Field systems derived from gradual enclosure of open fields, usually from 13C to 17 &amp; 18C when Parliamentary Enclosure dominated. Individual strips or groups enclosed by landholders, leaving elements of the former open field pattern visible.</skos:scopeNote>
  </skos:Concept>

  <skos:Concept rdf:about="http://purl.org/heritagedata/schemes/571/concepts/151781">
    <skos:broader rdf:resource="http://purl.org/heritagedata/schemes/571/concepts/151173"/>
    <skos:broader rdf:resource="http://purl.org/heritagedata/schemes/571/concepts/151780"/>
    <skos:inScheme rdf:resource="http://purl.org/heritagedata/schemes/571"/>
    <dc:identifier>http://purl.org/heritagedata/schemes/571/concepts/151781</dc:identifier>
    <dc:issued rdf:datatype="http://www.w3.org/2001/XMLSchema#dateTime">2024-07-01T17:17:33</dc:issued>
    <cc:license rdf:resource="https://www.nationalarchives.gov.uk/doc/open-government-licence/version/3/"/>
    <cc:attributionURL rdf:resource="https://historicengland.org.uk/"/>
    <cc:attributionName xml:lang="en">Historic England</cc:attributionName>
    <dc:publisher rdf:resource="https://historicengland.org.uk/"/>
    <dc:spatial rdf:resource="http://vocab.getty.edu/tgn/7002445"/>
    <dc:spatial rdf:resource="http://dbpedia.org/resource/England"/>
    <skos:prefLabel xml:lang="en">Furlong</skos:prefLabel>
    <skos:scopeNote xml:lang="en">Block of land within an open field system containing a number of individual strips and usually managed as a single cropping or farming unit. In places such blocks were associated with fixed lengths, hence also name for a customary length of 220 yards.</skos:scopeNote>
  </skos:Concept>

  <skos:Concept rdf:about="http://purl.org/heritagedata/schemes/571/concepts/151787">
    <skos:broader rdf:resource="http://purl.org/heritagedata/schemes/571/concepts/151727"/>
    <skos:inScheme rdf:resource="http://purl.org/heritagedata/schemes/571"/>
    <dc:identifier>http://purl.org/heritagedata/schemes/571/concepts/151787</dc:identifier>
    <dc:issued rdf:datatype="http://www.w3.org/2001/XMLSchema#dateTime">2024-07-01T17:17:33</dc:issued>
    <cc:license rdf:resource="https://www.nationalarchives.gov.uk/doc/open-government-licence/version/3/"/>
    <cc:attributionURL rdf:resource="https://historicengland.org.uk/"/>
    <cc:attributionName xml:lang="en">Historic England</cc:attributionName>
    <dc:publisher rdf:resource="https://historicengland.org.uk/"/>
    <dc:spatial rdf:resource="http://vocab.getty.edu/tgn/7002445"/>
    <dc:spatial rdf:resource="http://dbpedia.org/resource/England"/>
    <skos:prefLabel xml:lang="en">Amalgamated Fields</skos:prefLabel>
    <skos:related rdf:resource="http://purl.org/heritagedata/schemes/571/concepts/160163"/>
    <skos:scopeNote xml:lang="en">Enlarged fields, created by the amalgamation by boundary removal of smaller fields, mainly since the 19th century and usually since the Second World War. Usually to ease mechanised working and increase productivity.</skos:scopeNote>
  </skos:Concept>

  <skos:Concept rdf:about="http://purl.org/heritagedata/schemes/571/concepts/151793">
    <skos:broader rdf:resource="http://purl.org/heritagedata/schemes/571/concepts/151450"/>
    <skos:inScheme rdf:resource="http://purl.org/heritagedata/schemes/571"/>
    <dc:identifier>http://purl.org/heritagedata/schemes/571/concepts/151793</dc:identifier>
    <dc:issued rdf:datatype="http://www.w3.org/2001/XMLSchema#dateTime">2024-07-01T17:17:33</dc:issued>
    <cc:license rdf:resource="https://www.nationalarchives.gov.uk/doc/open-government-licence/version/3/"/>
    <cc:attributionURL rdf:resource="https://historicengland.org.uk/"/>
    <cc:attributionName xml:lang="en">Historic England</cc:attributionName>
    <dc:publisher rdf:resource="https://historicengland.org.uk/"/>
    <dc:spatial rdf:resource="http://vocab.getty.edu/tgn/7002445"/>
    <dc:spatial rdf:resource="http://dbpedia.org/resource/England"/>
    <skos:prefLabel xml:lang="en">Hunting Site</skos:prefLabel>
    <skos:scopeNote xml:lang="en">An area, building, site or structure associated with the hunting of animals.</skos:scopeNote>
  </skos:Concept>

  <skos:Concept rdf:about="http://purl.org/heritagedata/schemes/571/concepts/151450">
    <skos:narrower rdf:resource="http://purl.org/heritagedata/schemes/571/concepts/151793"/>
    <skos:narrower rdf:resource="http://purl.org/heritagedata/schemes/571/concepts/151900"/>
    <skos:narrower>
      <skos:Concept rdf:about="http://purl.org/heritagedata/schemes/571/concepts/152314">
        <skos:broader rdf:resource="http://purl.org/heritagedata/schemes/571/concepts/151450"/>
        <skos:inScheme rdf:resource="http://purl.org/heritagedata/schemes/571"/>
        <dc:identifier>http://purl.org/heritagedata/schemes/571/concepts/152314</dc:identifier>
        <dc:issued rdf:datatype="http://www.w3.org/2001/XMLSchema#dateTime">2024-07-01T17:17:33</dc:issued>
        <cc:license rdf:resource="https://www.nationalarchives.gov.uk/doc/open-government-licence/version/3/"/>
        <cc:attributionURL rdf:resource="https://historicengland.org.uk/"/>
        <cc:attributionName xml:lang="en">Historic England</cc:attributionName>
        <dc:publisher rdf:resource="https://historicengland.org.uk/"/>
        <dc:spatial rdf:resource="http://vocab.getty.edu/tgn/7002445"/>
        <dc:spatial rdf:resource="http://dbpedia.org/resource/England"/>
        <skos:prefLabel xml:lang="en">Leisure Sailing Area</skos:prefLabel>
        <skos:scopeNote xml:lang="en">Area used for recreational sailing, yachting, and other small craft pursuits.</skos:scopeNote>
      </skos:Concept>
    </skos:narrower>

    <skos:narrower rdf:resource="http://purl.org/heritagedata/schemes/571/concepts/152615"/>
    <skos:narrower rdf:resource="http://purl.org/heritagedata/schemes/571/concepts/160214"/>
    <skos:narrower rdf:resource="http://purl.org/heritagedata/schemes/571/concepts/160215"/>
    <skos:narrower rdf:resource="http://purl.org/heritagedata/schemes/571/concepts/160285"/>
    <skos:narrower rdf:resource="http://purl.org/heritagedata/schemes/571/concepts/160288"/>
    <skos:narrower rdf:resource="http://purl.org/heritagedata/schemes/571/concepts/160294"/>
    <skos:narrower>
      <skos:Concept rdf:about="http://purl.org/heritagedata/schemes/571/concepts/171101">
        <skos:broader rdf:resource="http://purl.org/heritagedata/schemes/571/concepts/151450"/>
        <skos:inScheme rdf:resource="http://purl.org/heritagedata/schemes/571"/>
        <dc:identifier>http://purl.org/heritagedata/schemes/571/concepts/171101</dc:identifier>
        <dc:issued rdf:datatype="http://www.w3.org/2001/XMLSchema#dateTime">2024-07-01T17:17:33</dc:issued>
        <cc:license rdf:resource="https://www.nationalarchives.gov.uk/doc/open-government-licence/version/3/"/>
        <cc:attributionURL rdf:resource="https://historicengland.org.uk/"/>
        <cc:attributionName xml:lang="en">Historic England</cc:attributionName>
        <dc:publisher rdf:resource="https://historicengland.org.uk/"/>
        <dc:spatial rdf:resource="http://vocab.getty.edu/tgn/7002445"/>
        <dc:spatial rdf:resource="http://dbpedia.org/resource/England"/>
        <skos:prefLabel xml:lang="en">Leisure Fishing Area</skos:prefLabel>
        <skos:scopeNote xml:lang="en">An area used for recreational fishing and angling.</skos:scopeNote>
      </skos:Concept>
    </skos:narrower>

    <skos:inScheme rdf:resource="http://purl.org/heritagedata/schemes/571"/>
    <dc:identifier>http://purl.org/heritagedata/schemes/571/concepts/151450</dc:identifier>
    <dc:issued rdf:datatype="http://www.w3.org/2001/XMLSchema#dateTime">2024-07-01T17:17:33</dc:issued>
    <cc:license rdf:resource="https://www.nationalarchives.gov.uk/doc/open-government-licence/version/3/"/>
    <cc:attributionURL rdf:resource="https://historicengland.org.uk/"/>
    <cc:attributionName xml:lang="en">Historic England</cc:attributionName>
    <dc:publisher rdf:resource="https://historicengland.org.uk/"/>
    <dc:spatial rdf:resource="http://vocab.getty.edu/tgn/7002445"/>
    <dc:spatial rdf:resource="http://dbpedia.org/resource/England"/>
    <skos:prefLabel xml:lang="en">Recreation And Leisure</skos:prefLabel>
    <skos:scopeNote xml:lang="en">-</skos:scopeNote>
    <skos:topConceptOf rdf:resource="http://purl.org/heritagedata/schemes/571"/>
  </skos:Concept>

  <skos:Concept rdf:about="http://purl.org/heritagedata/schemes/571/concepts/151928">
    <skos:broader rdf:resource="http://purl.org/heritagedata/schemes/571/concepts/151900"/>
    <skos:broader rdf:resource="http://purl.org/heritagedata/schemes/571/concepts/151235"/>
    <skos:inScheme rdf:resource="http://purl.org/heritagedata/schemes/571"/>
    <dc:identifier>http://purl.org/heritagedata/schemes/571/concepts/151928</dc:identifier>
    <dc:issued rdf:datatype="http://www.w3.org/2001/XMLSchema#dateTime">2024-07-01T17:17:33</dc:issued>
    <cc:license rdf:resource="https://www.nationalarchives.gov.uk/doc/open-government-licence/version/3/"/>
    <cc:attributionURL rdf:resource="https://historicengland.org.uk/"/>
    <cc:attributionName xml:lang="en">Historic England</cc:attributionName>
    <dc:publisher rdf:resource="https://historicengland.org.uk/"/>
    <dc:spatial rdf:resource="http://vocab.getty.edu/tgn/7002445"/>
    <dc:spatial rdf:resource="http://dbpedia.org/resource/England"/>
    <skos:prefLabel xml:lang="en">Hillfort</skos:prefLabel>
    <skos:scopeNote xml:lang="en">A hilltop enclosure bounded by one or more substantial banks, ramparts and ditches. Now forming a feature within other landscape character types such as recreation, rough ground or enclosed land.</skos:scopeNote>
  </skos:Concept>

  <skos:Concept rdf:about="http://purl.org/heritagedata/schemes/571/concepts/151975">
    <skos:broader rdf:resource="http://purl.org/heritagedata/schemes/571/concepts/152309"/>
    <skos:inScheme rdf:resource="http://purl.org/heritagedata/schemes/571"/>
    <dc:identifier>http://purl.org/heritagedata/schemes/571/concepts/151975</dc:identifier>
    <dc:issued rdf:datatype="http://www.w3.org/2001/XMLSchema#dateTime">2024-07-01T17:17:33</dc:issued>
    <cc:license rdf:resource="https://www.nationalarchives.gov.uk/doc/open-government-licence/version/3/"/>
    <cc:attributionURL rdf:resource="https://historicengland.org.uk/"/>
    <cc:attributionName xml:lang="en">Historic England</cc:attributionName>
    <dc:publisher rdf:resource="https://historicengland.org.uk/"/>
    <dc:spatial rdf:resource="http://vocab.getty.edu/tgn/7002445"/>
    <dc:spatial rdf:resource="http://dbpedia.org/resource/England"/>
    <skos:prefLabel xml:lang="en">Rowing Lake</skos:prefLabel>
    <skos:scopeNote xml:lang="en">A lake, sometimes purpose built, for use in the sport of rowing.</skos:scopeNote>
  </skos:Concept>

  <skos:Concept rdf:about="http://purl.org/heritagedata/schemes/571/concepts/152309">
    <skos:narrower rdf:resource="http://purl.org/heritagedata/schemes/571/concepts/151975"/>
    <skos:narrower>
      <skos:Concept rdf:about="http://purl.org/heritagedata/schemes/571/concepts/152312">
        <skos:broader rdf:resource="http://purl.org/heritagedata/schemes/571/concepts/152309"/>
        <skos:inScheme rdf:resource="http://purl.org/heritagedata/schemes/571"/>
        <dc:identifier>http://purl.org/heritagedata/schemes/571/concepts/152312</dc:identifier>
        <dc:issued rdf:datatype="http://www.w3.org/2001/XMLSchema#dateTime">2024-07-01T17:17:33</dc:issued>
        <cc:license rdf:resource="https://www.nationalarchives.gov.uk/doc/open-government-licence/version/3/"/>
        <cc:attributionURL rdf:resource="https://historicengland.org.uk/"/>
        <cc:attributionName xml:lang="en">Historic England</cc:attributionName>
        <dc:publisher rdf:resource="https://historicengland.org.uk/"/>
        <dc:spatial rdf:resource="http://vocab.getty.edu/tgn/7002445"/>
        <dc:spatial rdf:resource="http://dbpedia.org/resource/England"/>
        <skos:prefLabel xml:lang="en">Recreational Dive Area</skos:prefLabel>
        <skos:scopeNote xml:lang="en">An area used by recreational divers, sometimes concentrated on wreck sites and other areas of semi-natural or historic environment interest.</skos:scopeNote>
      </skos:Concept>
    </skos:narrower>

    <skos:narrower>
      <skos:Concept rdf:about="http://purl.org/heritagedata/schemes/571/concepts/160216">
        <skos:broader rdf:resource="http://purl.org/heritagedata/schemes/571/concepts/152309"/>
        <skos:inScheme rdf:resource="http://purl.org/heritagedata/schemes/571"/>
        <dc:identifier>http://purl.org/heritagedata/schemes/571/concepts/160216</dc:identifier>
        <dc:issued rdf:datatype="http://www.w3.org/2001/XMLSchema#dateTime">2024-07-01T17:17:33</dc:issued>
        <cc:license rdf:resource="https://www.nationalarchives.gov.uk/doc/open-government-licence/version/3/"/>
        <cc:attributionURL rdf:resource="https://historicengland.org.uk/"/>
        <cc:attributionName xml:lang="en">Historic England</cc:attributionName>
        <dc:publisher rdf:resource="https://historicengland.org.uk/"/>
        <dc:spatial rdf:resource="http://vocab.getty.edu/tgn/7002445"/>
        <dc:spatial rdf:resource="http://dbpedia.org/resource/England"/>
        <skos:prefLabel xml:lang="en">Fishing Area</skos:prefLabel>
        <skos:scopeNote xml:lang="en">Areas dominated by use for recreational fishing and angling.</skos:scopeNote>
      </skos:Concept>
    </skos:narrower>

    <skos:narrower>
      <skos:Concept rdf:about="http://purl.org/heritagedata/schemes/571/concepts/160297">
        <skos:broader rdf:resource="http://purl.org/heritagedata/schemes/571/concepts/152309"/>
        <skos:inScheme rdf:resource="http://purl.org/heritagedata/schemes/571"/>
        <dc:identifier>http://purl.org/heritagedata/schemes/571/concepts/160297</dc:identifier>
        <dc:issued rdf:datatype="http://www.w3.org/2001/XMLSchema#dateTime">2024-07-01T17:17:33</dc:issued>
        <cc:license rdf:resource="https://www.nationalarchives.gov.uk/doc/open-government-licence/version/3/"/>
        <cc:attributionURL rdf:resource="https://historicengland.org.uk/"/>
        <cc:attributionName xml:lang="en">Historic England</cc:attributionName>
        <dc:publisher rdf:resource="https://historicengland.org.uk/"/>
        <dc:spatial rdf:resource="http://vocab.getty.edu/tgn/7002445"/>
        <dc:spatial rdf:resource="http://dbpedia.org/resource/England"/>
        <skos:prefLabel xml:lang="en">Sailing Area</skos:prefLabel>
        <skos:scopeNote xml:lang="en">Area used for recreational sailing, yachting and other small craft persuits.</skos:scopeNote>
      </skos:Concept>
    </skos:narrower>

    <skos:narrower>
      <skos:Concept rdf:about="http://purl.org/heritagedata/schemes/571/concepts/160383">
        <skos:broader rdf:resource="http://purl.org/heritagedata/schemes/571/concepts/152309"/>
        <skos:inScheme rdf:resource="http://purl.org/heritagedata/schemes/571"/>
        <dc:identifier>http://purl.org/heritagedata/schemes/571/concepts/160383</dc:identifier>
        <dc:issued rdf:datatype="http://www.w3.org/2001/XMLSchema#dateTime">2024-07-01T17:17:33</dc:issued>
        <cc:license rdf:resource="https://www.nationalarchives.gov.uk/doc/open-government-licence/version/3/"/>
        <cc:attributionURL rdf:resource="https://historicengland.org.uk/"/>
        <cc:attributionName xml:lang="en">Historic England</cc:attributionName>
        <dc:publisher rdf:resource="https://historicengland.org.uk/"/>
        <dc:spatial rdf:resource="http://vocab.getty.edu/tgn/7002445"/>
        <dc:spatial rdf:resource="http://dbpedia.org/resource/England"/>
        <skos:prefLabel xml:lang="en">Swimming Pool</skos:prefLabel>
        <skos:scopeNote xml:lang="en">Indoor pool for sports such as swimming and diving. Includes any directly associated grounds.</skos:scopeNote>
      </skos:Concept>
    </skos:narrower>

    <skos:broader rdf:resource="http://purl.org/heritagedata/schemes/571/concepts/152615"/>
    <skos:inScheme rdf:resource="http://purl.org/heritagedata/schemes/571"/>
    <dc:identifier>http://purl.org/heritagedata/schemes/571/concepts/152309</dc:identifier>
    <dc:issued rdf:datatype="http://www.w3.org/2001/XMLSchema#dateTime">2024-07-01T17:17:33</dc:issued>
    <cc:license rdf:resource="https://www.nationalarchives.gov.uk/doc/open-government-licence/version/3/"/>
    <cc:attributionURL rdf:resource="https://historicengland.org.uk/"/>
    <cc:attributionName xml:lang="en">Historic England</cc:attributionName>
    <dc:publisher rdf:resource="https://historicengland.org.uk/"/>
    <dc:spatial rdf:resource="http://vocab.getty.edu/tgn/7002445"/>
    <dc:spatial rdf:resource="http://dbpedia.org/resource/England"/>
    <skos:prefLabel xml:lang="en">Water Sports</skos:prefLabel>
    <skos:scopeNote xml:lang="en">Buildings, sites and structures associated with water sporting activities. Use more specific type where known.</skos:scopeNote>
  </skos:Concept>

  <skos:Concept rdf:about="http://purl.org/heritagedata/schemes/571/concepts/152298">
    <skos:broader rdf:resource="http://purl.org/heritagedata/schemes/571/concepts/152615"/>
    <skos:inScheme rdf:resource="http://purl.org/heritagedata/schemes/571"/>
    <dc:identifier>http://purl.org/heritagedata/schemes/571/concepts/152298</dc:identifier>
    <dc:issued rdf:datatype="http://www.w3.org/2001/XMLSchema#dateTime">2024-07-01T17:17:33</dc:issued>
    <cc:license rdf:resource="https://www.nationalarchives.gov.uk/doc/open-government-licence/version/3/"/>
    <cc:attributionURL rdf:resource="https://historicengland.org.uk/"/>
    <cc:attributionName xml:lang="en">Historic England</cc:attributionName>
    <dc:publisher rdf:resource="https://historicengland.org.uk/"/>
    <dc:spatial rdf:resource="http://vocab.getty.edu/tgn/7002445"/>
    <dc:spatial rdf:resource="http://dbpedia.org/resource/England"/>
    <skos:prefLabel xml:lang="en">Equestrian Centre</skos:prefLabel>
    <skos:related rdf:resource="http://purl.org/heritagedata/schemes/571/concepts/152305"/>
    <skos:scopeNote xml:lang="en">A complex including buildings providing accomadation and activity areas for those involved in equestrian sports/activities and their horses.</skos:scopeNote>
  </skos:Concept>

  <skos:Concept rdf:about="http://purl.org/heritagedata/schemes/571/concepts/152615">
    <skos:narrower rdf:resource="http://purl.org/heritagedata/schemes/571/concepts/152298"/>
    <skos:narrower rdf:resource="http://purl.org/heritagedata/schemes/571/concepts/152301"/>
    <skos:narrower rdf:resource="http://purl.org/heritagedata/schemes/571/concepts/152309"/>
    <skos:narrower rdf:resource="http://purl.org/heritagedata/schemes/571/concepts/152403"/>
    <skos:narrower rdf:resource="http://purl.org/heritagedata/schemes/571/concepts/160382"/>
    <skos:broader rdf:resource="http://purl.org/heritagedata/schemes/571/concepts/151450"/>
    <skos:inScheme rdf:resource="http://purl.org/heritagedata/schemes/571"/>
    <dc:identifier>http://purl.org/heritagedata/schemes/571/concepts/152615</dc:identifier>
    <dc:issued rdf:datatype="http://www.w3.org/2001/XMLSchema#dateTime">2024-07-01T17:17:33</dc:issued>
    <cc:license rdf:resource="https://www.nationalarchives.gov.uk/doc/open-government-licence/version/3/"/>
    <cc:attributionURL rdf:resource="https://historicengland.org.uk/"/>
    <cc:attributionName xml:lang="en">Historic England</cc:attributionName>
    <dc:publisher rdf:resource="https://historicengland.org.uk/"/>
    <dc:spatial rdf:resource="http://vocab.getty.edu/tgn/7002445"/>
    <dc:spatial rdf:resource="http://dbpedia.org/resource/England"/>
    <skos:prefLabel xml:lang="en">Sports Facility</skos:prefLabel>
    <skos:scopeNote xml:lang="en">Areas whose dominant character is provision for sporting activity, whether or not commercially provided, and whether or not in areas of purpose-built structures.</skos:scopeNote>
  </skos:Concept>

  <skos:Concept rdf:about="http://purl.org/heritagedata/schemes/571/concepts/152305">
    <skos:broader rdf:resource="http://purl.org/heritagedata/schemes/571/concepts/152403"/>
    <skos:inScheme rdf:resource="http://purl.org/heritagedata/schemes/571"/>
    <dc:identifier>http://purl.org/heritagedata/schemes/571/concepts/152305</dc:identifier>
    <dc:issued rdf:datatype="http://www.w3.org/2001/XMLSchema#dateTime">2024-07-01T17:17:33</dc:issued>
    <cc:license rdf:resource="https://www.nationalarchives.gov.uk/doc/open-government-licence/version/3/"/>
    <cc:attributionURL rdf:resource="https://historicengland.org.uk/"/>
    <cc:attributionName xml:lang="en">Historic England</cc:attributionName>
    <dc:publisher rdf:resource="https://historicengland.org.uk/"/>
    <dc:spatial rdf:resource="http://vocab.getty.edu/tgn/7002445"/>
    <dc:spatial rdf:resource="http://dbpedia.org/resource/England"/>
    <skos:prefLabel xml:lang="en">Gallops</skos:prefLabel>
    <skos:related rdf:resource="http://purl.org/heritagedata/schemes/571/concepts/152298"/>
    <skos:scopeNote xml:lang="en">A track or area where horses are exercised at a gallop.</skos:scopeNote>
  </skos:Concept>

  <skos:Concept rdf:about="http://purl.org/heritagedata/schemes/571/concepts/152322">
    <skos:broader rdf:resource="http://purl.org/heritagedata/schemes/571/concepts/151456"/>
    <skos:inScheme rdf:resource="http://purl.org/heritagedata/schemes/571"/>
    <dc:identifier>http://purl.org/heritagedata/schemes/571/concepts/152322</dc:identifier>
    <dc:issued rdf:datatype="http://www.w3.org/2001/XMLSchema#dateTime">2024-07-01T17:17:33</dc:issued>
    <cc:license rdf:resource="https://www.nationalarchives.gov.uk/doc/open-government-licence/version/3/"/>
    <cc:attributionURL rdf:resource="https://historicengland.org.uk/"/>
    <cc:attributionName xml:lang="en">Historic England</cc:attributionName>
    <dc:publisher rdf:resource="https://historicengland.org.uk/"/>
    <dc:spatial rdf:resource="http://vocab.getty.edu/tgn/7002445"/>
    <dc:spatial rdf:resource="http://dbpedia.org/resource/England"/>
    <skos:prefLabel xml:lang="en">Scree</skos:prefLabel>
    <skos:related rdf:resource="http://purl.org/heritagedata/schemes/571/concepts/151129"/>
    <skos:related rdf:resource="http://purl.org/heritagedata/schemes/571/concepts/151131"/>
    <skos:scopeNote xml:lang="en">An accumulation of broken rock debris found on the slopes and at the base of crags, mountain cliffs, or valley shoulders.</skos:scopeNote>
  </skos:Concept>

  <skos:Concept rdf:about="http://purl.org/heritagedata/schemes/571/concepts/152324">
    <skos:broader rdf:resource="http://purl.org/heritagedata/schemes/571/concepts/152594"/>
    <skos:inScheme rdf:resource="http://purl.org/heritagedata/schemes/571"/>
    <dc:identifier>http://purl.org/heritagedata/schemes/571/concepts/152324</dc:identifier>
    <dc:issued rdf:datatype="http://www.w3.org/2001/XMLSchema#dateTime">2024-07-01T17:17:33</dc:issued>
    <cc:license rdf:resource="https://www.nationalarchives.gov.uk/doc/open-government-licence/version/3/"/>
    <cc:attributionURL rdf:resource="https://historicengland.org.uk/"/>
    <cc:attributionName xml:lang="en">Historic England</cc:attributionName>
    <dc:publisher rdf:resource="https://historicengland.org.uk/"/>
    <dc:spatial rdf:resource="http://vocab.getty.edu/tgn/7002445"/>
    <dc:spatial rdf:resource="http://dbpedia.org/resource/England"/>
    <skos:prefLabel xml:lang="en">River</skos:prefLabel>
    <skos:scopeNote xml:lang="en">A significant watercourse largely following the natural drainage pattern and flowing towards another river, a lake or the sea.</skos:scopeNote>
  </skos:Concept>

  <skos:Concept rdf:about="http://purl.org/heritagedata/schemes/571/concepts/152594">
    <skos:narrower rdf:resource="http://purl.org/heritagedata/schemes/571/concepts/152324"/>
    <skos:broader rdf:resource="http://purl.org/heritagedata/schemes/571/concepts/151444"/>
    <skos:inScheme rdf:resource="http://purl.org/heritagedata/schemes/571"/>
    <dc:identifier>http://purl.org/heritagedata/schemes/571/concepts/152594</dc:identifier>
    <dc:issued rdf:datatype="http://www.w3.org/2001/XMLSchema#dateTime">2024-07-01T17:17:33</dc:issued>
    <cc:license rdf:resource="https://www.nationalarchives.gov.uk/doc/open-government-licence/version/3/"/>
    <cc:attributionURL rdf:resource="https://historicengland.org.uk/"/>
    <cc:attributionName xml:lang="en">Historic England</cc:attributionName>
    <dc:publisher rdf:resource="https://historicengland.org.uk/"/>
    <dc:spatial rdf:resource="http://vocab.getty.edu/tgn/7002445"/>
    <dc:spatial rdf:resource="http://dbpedia.org/resource/England"/>
    <skos:prefLabel xml:lang="en">Watercourse</skos:prefLabel>
    <skos:scopeNote xml:lang="en">A channel used for or formed by the conveyance of water.</skos:scopeNote>
  </skos:Concept>

  <skos:Concept rdf:about="http://purl.org/heritagedata/schemes/571/concepts/152327">
    <skos:broader rdf:resource="http://purl.org/heritagedata/schemes/571/concepts/152326"/>
    <skos:narrower>
      <skos:Concept rdf:about="http://purl.org/heritagedata/schemes/571/concepts/160487">
        <skos:broader rdf:resource="http://purl.org/heritagedata/schemes/571/concepts/152327"/>
        <skos:inScheme rdf:resource="http://purl.org/heritagedata/schemes/571"/>
        <dc:identifier>http://purl.org/heritagedata/schemes/571/concepts/160487</dc:identifier>
        <dc:issued rdf:datatype="http://www.w3.org/2001/XMLSchema#dateTime">2024-07-01T17:17:33</dc:issued>
        <cc:license rdf:resource="https://www.nationalarchives.gov.uk/doc/open-government-licence/version/3/"/>
        <cc:attributionURL rdf:resource="https://historicengland.org.uk/"/>
        <cc:attributionName xml:lang="en">Historic England</cc:attributionName>
        <dc:publisher rdf:resource="https://historicengland.org.uk/"/>
        <dc:spatial rdf:resource="http://vocab.getty.edu/tgn/7002445"/>
        <dc:spatial rdf:resource="http://dbpedia.org/resource/England"/>
        <skos:prefLabel xml:lang="en">Scrub (Divided)</skos:prefLabel>
        <skos:scopeNote xml:lang="en">Scrub divided by stock-proof boundaries.</skos:scopeNote>
      </skos:Concept>
    </skos:narrower>

    <skos:narrower>
      <skos:Concept rdf:about="http://purl.org/heritagedata/schemes/571/concepts/160488">
        <skos:broader rdf:resource="http://purl.org/heritagedata/schemes/571/concepts/152327"/>
        <skos:inScheme rdf:resource="http://purl.org/heritagedata/schemes/571"/>
        <dc:identifier>http://purl.org/heritagedata/schemes/571/concepts/160488</dc:identifier>
        <dc:issued rdf:datatype="http://www.w3.org/2001/XMLSchema#dateTime">2024-07-01T17:17:33</dc:issued>
        <cc:license rdf:resource="https://www.nationalarchives.gov.uk/doc/open-government-licence/version/3/"/>
        <cc:attributionURL rdf:resource="https://historicengland.org.uk/"/>
        <cc:attributionName xml:lang="en">Historic England</cc:attributionName>
        <dc:publisher rdf:resource="https://historicengland.org.uk/"/>
        <dc:spatial rdf:resource="http://vocab.getty.edu/tgn/7002445"/>
        <dc:spatial rdf:resource="http://dbpedia.org/resource/England"/>
        <skos:prefLabel xml:lang="en">Scrub (Undivided)</skos:prefLabel>
        <skos:scopeNote xml:lang="en">Scrub left open, not divided by stock-proof boundaries.</skos:scopeNote>
      </skos:Concept>
    </skos:narrower>

    <skos:inScheme rdf:resource="http://purl.org/heritagedata/schemes/571"/>
    <dc:identifier>http://purl.org/heritagedata/schemes/571/concepts/152327</dc:identifier>
    <dc:issued rdf:datatype="http://www.w3.org/2001/XMLSchema#dateTime">2024-07-01T17:17:33</dc:issued>
    <cc:license rdf:resource="https://www.nationalarchives.gov.uk/doc/open-government-licence/version/3/"/>
    <cc:attributionURL rdf:resource="https://historicengland.org.uk/"/>
    <cc:attributionName xml:lang="en">Historic England</cc:attributionName>
    <dc:publisher rdf:resource="https://historicengland.org.uk/"/>
    <dc:spatial rdf:resource="http://vocab.getty.edu/tgn/7002445"/>
    <dc:spatial rdf:resource="http://dbpedia.org/resource/England"/>
    <skos:prefLabel xml:lang="en">Scrub</skos:prefLabel>
    <skos:scopeNote xml:lang="en">Uncultivated land characterised by vegetation dominated by shrubs or bushes of woody plants, sometimes including small trees.</skos:scopeNote>
  </skos:Concept>

  <skos:Concept rdf:about="http://purl.org/heritagedata/schemes/571/concepts/152330">
    <skos:broader rdf:resource="http://purl.org/heritagedata/schemes/571/concepts/152326"/>
    <skos:narrower>
      <skos:Concept rdf:about="http://purl.org/heritagedata/schemes/571/concepts/152331">
        <skos:broader rdf:resource="http://purl.org/heritagedata/schemes/571/concepts/152330"/>
        <skos:inScheme rdf:resource="http://purl.org/heritagedata/schemes/571"/>
        <dc:identifier>http://purl.org/heritagedata/schemes/571/concepts/152331</dc:identifier>
        <dc:issued rdf:datatype="http://www.w3.org/2001/XMLSchema#dateTime">2024-07-01T17:17:33</dc:issued>
        <cc:license rdf:resource="https://www.nationalarchives.gov.uk/doc/open-government-licence/version/3/"/>
        <cc:attributionURL rdf:resource="https://historicengland.org.uk/"/>
        <cc:attributionName xml:lang="en">Historic England</cc:attributionName>
        <dc:publisher rdf:resource="https://historicengland.org.uk/"/>
        <dc:spatial rdf:resource="http://vocab.getty.edu/tgn/7002445"/>
        <dc:spatial rdf:resource="http://dbpedia.org/resource/England"/>
        <skos:prefLabel xml:lang="en">Open Rough Ground</skos:prefLabel>
        <skos:scopeNote xml:lang="en">-</skos:scopeNote>
      </skos:Concept>
    </skos:narrower>

    <skos:narrower rdf:resource="http://purl.org/heritagedata/schemes/571/concepts/152332"/>
    <skos:narrower rdf:resource="http://purl.org/heritagedata/schemes/571/concepts/152333"/>
    <skos:narrower rdf:resource="http://purl.org/heritagedata/schemes/571/concepts/152334"/>
    <skos:narrower>
      <skos:Concept rdf:about="http://purl.org/heritagedata/schemes/571/concepts/152337">
        <skos:broader rdf:resource="http://purl.org/heritagedata/schemes/571/concepts/152330"/>
        <skos:inScheme rdf:resource="http://purl.org/heritagedata/schemes/571"/>
        <dc:identifier>http://purl.org/heritagedata/schemes/571/concepts/152337</dc:identifier>
        <dc:issued rdf:datatype="http://www.w3.org/2001/XMLSchema#dateTime">2024-07-01T17:17:33</dc:issued>
        <cc:license rdf:resource="https://www.nationalarchives.gov.uk/doc/open-government-licence/version/3/"/>
        <cc:attributionURL rdf:resource="https://historicengland.org.uk/"/>
        <cc:attributionName xml:lang="en">Historic England</cc:attributionName>
        <dc:publisher rdf:resource="https://historicengland.org.uk/"/>
        <dc:spatial rdf:resource="http://vocab.getty.edu/tgn/7002445"/>
        <dc:spatial rdf:resource="http://dbpedia.org/resource/England"/>
        <skos:prefLabel xml:lang="en">Secondary Rough Ground</skos:prefLabel>
        <skos:scopeNote xml:lang="en">Rough ground that has developed recently, usually as a result of the suspension of other land uses and management . Not normally subjected to grazing, fuel collection etc.</skos:scopeNote>
      </skos:Concept>
    </skos:narrower>

    <skos:inScheme rdf:resource="http://purl.org/heritagedata/schemes/571"/>
    <dc:identifier>http://purl.org/heritagedata/schemes/571/concepts/152330</dc:identifier>
    <dc:issued rdf:datatype="http://www.w3.org/2001/XMLSchema#dateTime">2024-07-01T17:17:33</dc:issued>
    <cc:license rdf:resource="https://www.nationalarchives.gov.uk/doc/open-government-licence/version/3/"/>
    <cc:attributionURL rdf:resource="https://historicengland.org.uk/"/>
    <cc:attributionName xml:lang="en">Historic England</cc:attributionName>
    <dc:publisher rdf:resource="https://historicengland.org.uk/"/>
    <dc:spatial rdf:resource="http://vocab.getty.edu/tgn/7002445"/>
    <dc:spatial rdf:resource="http://dbpedia.org/resource/England"/>
    <skos:prefLabel xml:lang="en">Rough Ground</skos:prefLabel>
    <skos:scopeNote xml:lang="en">Area dominated by rough vegetation, with no visible evidence of recent agricultural improvement. Used primarily for grazing and, historically, fuel gathering, often in common.</skos:scopeNote>
  </skos:Concept>

  <skos:Concept rdf:about="http://purl.org/heritagedata/schemes/571/concepts/152332">
    <skos:broader rdf:resource="http://purl.org/heritagedata/schemes/571/concepts/152330"/>
    <skos:narrower rdf:resource="http://purl.org/heritagedata/schemes/571/concepts/160474"/>
    <skos:narrower rdf:resource="http://purl.org/heritagedata/schemes/571/concepts/160475"/>
    <skos:inScheme rdf:resource="http://purl.org/heritagedata/schemes/571"/>
    <dc:identifier>http://purl.org/heritagedata/schemes/571/concepts/152332</dc:identifier>
    <dc:issued rdf:datatype="http://www.w3.org/2001/XMLSchema#dateTime">2024-07-01T17:17:33</dc:issued>
    <cc:license rdf:resource="https://www.nationalarchives.gov.uk/doc/open-government-licence/version/3/"/>
    <cc:attributionURL rdf:resource="https://historicengland.org.uk/"/>
    <cc:attributionName xml:lang="en">Historic England</cc:attributionName>
    <dc:publisher rdf:resource="https://historicengland.org.uk/"/>
    <dc:spatial rdf:resource="http://vocab.getty.edu/tgn/7002445"/>
    <dc:spatial rdf:resource="http://dbpedia.org/resource/England"/>
    <skos:prefLabel xml:lang="en">Coastal Rough Ground</skos:prefLabel>
    <skos:scopeNote xml:lang="en">Coastal area with rough vegetation created and maintained by grazing, often seasonal, and by fuel collection. Much is now neglected and reverting to scrub.</skos:scopeNote>
  </skos:Concept>

  <skos:Concept rdf:about="http://purl.org/heritagedata/schemes/571/concepts/152333">
    <skos:broader rdf:resource="http://purl.org/heritagedata/schemes/571/concepts/152330"/>
    <skos:narrower>
      <skos:Concept rdf:about="http://purl.org/heritagedata/schemes/571/concepts/160489">
        <skos:broader rdf:resource="http://purl.org/heritagedata/schemes/571/concepts/152333"/>
        <skos:inScheme rdf:resource="http://purl.org/heritagedata/schemes/571"/>
        <dc:identifier>http://purl.org/heritagedata/schemes/571/concepts/160489</dc:identifier>
        <dc:issued rdf:datatype="http://www.w3.org/2001/XMLSchema#dateTime">2024-07-01T17:17:33</dc:issued>
        <cc:license rdf:resource="https://www.nationalarchives.gov.uk/doc/open-government-licence/version/3/"/>
        <cc:attributionURL rdf:resource="https://historicengland.org.uk/"/>
        <cc:attributionName xml:lang="en">Historic England</cc:attributionName>
        <dc:publisher rdf:resource="https://historicengland.org.uk/"/>
        <dc:spatial rdf:resource="http://vocab.getty.edu/tgn/7002445"/>
        <dc:spatial rdf:resource="http://dbpedia.org/resource/England"/>
        <skos:prefLabel xml:lang="en">Upland Rough Ground (Divided)</skos:prefLabel>
        <skos:scopeNote xml:lang="en">Upland rough ground divided by stock-proof boundaries.</skos:scopeNote>
      </skos:Concept>
    </skos:narrower>

    <skos:narrower>
      <skos:Concept rdf:about="http://purl.org/heritagedata/schemes/571/concepts/160490">
        <skos:broader rdf:resource="http://purl.org/heritagedata/schemes/571/concepts/152333"/>
        <skos:inScheme rdf:resource="http://purl.org/heritagedata/schemes/571"/>
        <dc:identifier>http://purl.org/heritagedata/schemes/571/concepts/160490</dc:identifier>
        <dc:issued rdf:datatype="http://www.w3.org/2001/XMLSchema#dateTime">2024-07-01T17:17:33</dc:issued>
        <cc:license rdf:resource="https://www.nationalarchives.gov.uk/doc/open-government-licence/version/3/"/>
        <cc:attributionURL rdf:resource="https://historicengland.org.uk/"/>
        <cc:attributionName xml:lang="en">Historic England</cc:attributionName>
        <dc:publisher rdf:resource="https://historicengland.org.uk/"/>
        <dc:spatial rdf:resource="http://vocab.getty.edu/tgn/7002445"/>
        <dc:spatial rdf:resource="http://dbpedia.org/resource/England"/>
        <skos:prefLabel xml:lang="en">Upland Rough Ground (Undivided)</skos:prefLabel>
        <skos:scopeNote xml:lang="en">Upland rough ground left open, not divided by stock-proof boundaries.</skos:scopeNote>
      </skos:Concept>
    </skos:narrower>

    <skos:inScheme rdf:resource="http://purl.org/heritagedata/schemes/571"/>
    <dc:identifier>http://purl.org/heritagedata/schemes/571/concepts/152333</dc:identifier>
    <dc:issued rdf:datatype="http://www.w3.org/2001/XMLSchema#dateTime">2024-07-01T17:17:33</dc:issued>
    <cc:license rdf:resource="https://www.nationalarchives.gov.uk/doc/open-government-licence/version/3/"/>
    <cc:attributionURL rdf:resource="https://historicengland.org.uk/"/>
    <cc:attributionName xml:lang="en">Historic England</cc:attributionName>
    <dc:publisher rdf:resource="https://historicengland.org.uk/"/>
    <dc:spatial rdf:resource="http://vocab.getty.edu/tgn/7002445"/>
    <dc:spatial rdf:resource="http://dbpedia.org/resource/England"/>
    <skos:prefLabel xml:lang="en">Upland Rough Ground</skos:prefLabel>
    <skos:scopeNote xml:lang="en">Upland area with rough vegetation created and maintained by grazing, often seasonal, and historically by fuel collection.</skos:scopeNote>
  </skos:Concept>

  <skos:Concept rdf:about="http://purl.org/heritagedata/schemes/571/concepts/152334">
    <skos:broader rdf:resource="http://purl.org/heritagedata/schemes/571/concepts/152330"/>
    <skos:narrower>
      <skos:Concept rdf:about="http://purl.org/heritagedata/schemes/571/concepts/160491">
        <skos:broader rdf:resource="http://purl.org/heritagedata/schemes/571/concepts/152334"/>
        <skos:inScheme rdf:resource="http://purl.org/heritagedata/schemes/571"/>
        <dc:identifier>http://purl.org/heritagedata/schemes/571/concepts/160491</dc:identifier>
        <dc:issued rdf:datatype="http://www.w3.org/2001/XMLSchema#dateTime">2024-07-01T17:17:33</dc:issued>
        <cc:license rdf:resource="https://www.nationalarchives.gov.uk/doc/open-government-licence/version/3/"/>
        <cc:attributionURL rdf:resource="https://historicengland.org.uk/"/>
        <cc:attributionName xml:lang="en">Historic England</cc:attributionName>
        <dc:publisher rdf:resource="https://historicengland.org.uk/"/>
        <dc:spatial rdf:resource="http://vocab.getty.edu/tgn/7002445"/>
        <dc:spatial rdf:resource="http://dbpedia.org/resource/England"/>
        <skos:prefLabel xml:lang="en">Valley Side Rough Ground (Divided)</skos:prefLabel>
        <skos:scopeNote xml:lang="en">Valley side rough ground divided by stock-proof boundaries.</skos:scopeNote>
      </skos:Concept>
    </skos:narrower>

    <skos:narrower>
      <skos:Concept rdf:about="http://purl.org/heritagedata/schemes/571/concepts/160492">
        <skos:broader rdf:resource="http://purl.org/heritagedata/schemes/571/concepts/152334"/>
        <skos:inScheme rdf:resource="http://purl.org/heritagedata/schemes/571"/>
        <dc:identifier>http://purl.org/heritagedata/schemes/571/concepts/160492</dc:identifier>
        <dc:issued rdf:datatype="http://www.w3.org/2001/XMLSchema#dateTime">2024-07-01T17:17:33</dc:issued>
        <cc:license rdf:resource="https://www.nationalarchives.gov.uk/doc/open-government-licence/version/3/"/>
        <cc:attributionURL rdf:resource="https://historicengland.org.uk/"/>
        <cc:attributionName xml:lang="en">Historic England</cc:attributionName>
        <dc:publisher rdf:resource="https://historicengland.org.uk/"/>
        <dc:spatial rdf:resource="http://vocab.getty.edu/tgn/7002445"/>
        <dc:spatial rdf:resource="http://dbpedia.org/resource/England"/>
        <skos:prefLabel xml:lang="en">Valley Side Rough Ground (Undivided)</skos:prefLabel>
        <skos:scopeNote xml:lang="en">Valley side rough ground left open, not divided by stock-proof boundaries.</skos:scopeNote>
      </skos:Concept>
    </skos:narrower>

    <skos:inScheme rdf:resource="http://purl.org/heritagedata/schemes/571"/>
    <dc:identifier>http://purl.org/heritagedata/schemes/571/concepts/152334</dc:identifier>
    <dc:issued rdf:datatype="http://www.w3.org/2001/XMLSchema#dateTime">2024-07-01T17:17:33</dc:issued>
    <cc:license rdf:resource="https://www.nationalarchives.gov.uk/doc/open-government-licence/version/3/"/>
    <cc:attributionURL rdf:resource="https://historicengland.org.uk/"/>
    <cc:attributionName xml:lang="en">Historic England</cc:attributionName>
    <dc:publisher rdf:resource="https://historicengland.org.uk/"/>
    <dc:spatial rdf:resource="http://vocab.getty.edu/tgn/7002445"/>
    <dc:spatial rdf:resource="http://dbpedia.org/resource/England"/>
    <skos:prefLabel xml:lang="en">Valley Side Rough Ground</skos:prefLabel>
    <skos:scopeNote xml:lang="en">Valley side area with rough vegetation created and maintained by grazing, often seasonal, and historically by fuel collection.</skos:scopeNote>
  </skos:Concept>

  <skos:Concept rdf:about="http://purl.org/heritagedata/schemes/571/concepts/152335">
    <skos:broader rdf:resource="http://purl.org/heritagedata/schemes/571/concepts/160474"/>
    <skos:broader rdf:resource="http://purl.org/heritagedata/schemes/571/concepts/160475"/>
    <skos:inScheme rdf:resource="http://purl.org/heritagedata/schemes/571"/>
    <dc:identifier>http://purl.org/heritagedata/schemes/571/concepts/152335</dc:identifier>
    <dc:issued rdf:datatype="http://www.w3.org/2001/XMLSchema#dateTime">2024-07-01T17:17:33</dc:issued>
    <cc:license rdf:resource="https://www.nationalarchives.gov.uk/doc/open-government-licence/version/3/"/>
    <cc:attributionURL rdf:resource="https://historicengland.org.uk/"/>
    <cc:attributionName xml:lang="en">Historic England</cc:attributionName>
    <dc:publisher rdf:resource="https://historicengland.org.uk/"/>
    <dc:spatial rdf:resource="http://vocab.getty.edu/tgn/7002445"/>
    <dc:spatial rdf:resource="http://dbpedia.org/resource/England"/>
    <skos:prefLabel xml:lang="en">Cliff Top Rough Ground</skos:prefLabel>
    <skos:scopeNote xml:lang="en">Coastal rough ground on the flatter land on cliff tops; grazed by cattle as well as sheep and goats.</skos:scopeNote>
  </skos:Concept>

  <skos:Concept rdf:about="http://purl.org/heritagedata/schemes/571/concepts/160474">
    <skos:narrower rdf:resource="http://purl.org/heritagedata/schemes/571/concepts/152335"/>
    <skos:narrower rdf:resource="http://purl.org/heritagedata/schemes/571/concepts/152336"/>
    <skos:broader rdf:resource="http://purl.org/heritagedata/schemes/571/concepts/152332"/>
    <skos:inScheme rdf:resource="http://purl.org/heritagedata/schemes/571"/>
    <dc:identifier>http://purl.org/heritagedata/schemes/571/concepts/160474</dc:identifier>
    <dc:issued rdf:datatype="http://www.w3.org/2001/XMLSchema#dateTime">2024-07-01T17:17:33</dc:issued>
    <cc:license rdf:resource="https://www.nationalarchives.gov.uk/doc/open-government-licence/version/3/"/>
    <cc:attributionURL rdf:resource="https://historicengland.org.uk/"/>
    <cc:attributionName xml:lang="en">Historic England</cc:attributionName>
    <dc:publisher rdf:resource="https://historicengland.org.uk/"/>
    <dc:spatial rdf:resource="http://vocab.getty.edu/tgn/7002445"/>
    <dc:spatial rdf:resource="http://dbpedia.org/resource/England"/>
    <skos:prefLabel xml:lang="en">Coastal Rough Ground (Divided)</skos:prefLabel>
    <skos:scopeNote xml:lang="en">Coastal rough ground divided by stock-proof boundaries.</skos:scopeNote>
  </skos:Concept>

  <skos:Concept rdf:about="http://purl.org/heritagedata/schemes/571/concepts/160475">
    <skos:narrower rdf:resource="http://purl.org/heritagedata/schemes/571/concepts/152335"/>
    <skos:narrower rdf:resource="http://purl.org/heritagedata/schemes/571/concepts/152336"/>
    <skos:broader rdf:resource="http://purl.org/heritagedata/schemes/571/concepts/152332"/>
    <skos:inScheme rdf:resource="http://purl.org/heritagedata/schemes/571"/>
    <dc:identifier>http://purl.org/heritagedata/schemes/571/concepts/160475</dc:identifier>
    <dc:issued rdf:datatype="http://www.w3.org/2001/XMLSchema#dateTime">2024-07-01T17:17:33</dc:issued>
    <cc:license rdf:resource="https://www.nationalarchives.gov.uk/doc/open-government-licence/version/3/"/>
    <cc:attributionURL rdf:resource="https://historicengland.org.uk/"/>
    <cc:attributionName xml:lang="en">Historic England</cc:attributionName>
    <dc:publisher rdf:resource="https://historicengland.org.uk/"/>
    <dc:spatial rdf:resource="http://vocab.getty.edu/tgn/7002445"/>
    <dc:spatial rdf:resource="http://dbpedia.org/resource/England"/>
    <skos:prefLabel xml:lang="en">Coastal Rough Ground (Undivided)</skos:prefLabel>
    <skos:scopeNote xml:lang="en">Coastal rough ground left open, undivided by stock-proof boundaries.</skos:scopeNote>
  </skos:Concept>

  <skos:Concept rdf:about="http://purl.org/heritagedata/schemes/571/concepts/152336">
    <skos:broader rdf:resource="http://purl.org/heritagedata/schemes/571/concepts/160474"/>
    <skos:broader rdf:resource="http://purl.org/heritagedata/schemes/571/concepts/160475"/>
    <skos:inScheme rdf:resource="http://purl.org/heritagedata/schemes/571"/>
    <dc:identifier>http://purl.org/heritagedata/schemes/571/concepts/152336</dc:identifier>
    <dc:issued rdf:datatype="http://www.w3.org/2001/XMLSchema#dateTime">2024-07-01T17:17:33</dc:issued>
    <cc:license rdf:resource="https://www.nationalarchives.gov.uk/doc/open-government-licence/version/3/"/>
    <cc:attributionURL rdf:resource="https://historicengland.org.uk/"/>
    <cc:attributionName xml:lang="en">Historic England</cc:attributionName>
    <dc:publisher rdf:resource="https://historicengland.org.uk/"/>
    <dc:spatial rdf:resource="http://vocab.getty.edu/tgn/7002445"/>
    <dc:spatial rdf:resource="http://dbpedia.org/resource/England"/>
    <skos:prefLabel xml:lang="en">Cliff Slope Rough Ground</skos:prefLabel>
    <skos:scopeNote xml:lang="en">Coastal rough ground on steep slopes; only able to be grazed by sheep, goats etc.</skos:scopeNote>
  </skos:Concept>

  <skos:Concept rdf:about="http://purl.org/heritagedata/schemes/571/concepts/152379">
    <skos:broader rdf:resource="http://purl.org/heritagedata/schemes/571/concepts/152326"/>
    <skos:narrower rdf:resource="http://purl.org/heritagedata/schemes/571/concepts/152380"/>
    <skos:narrower rdf:resource="http://purl.org/heritagedata/schemes/571/concepts/152608"/>
    <skos:inScheme rdf:resource="http://purl.org/heritagedata/schemes/571"/>
    <dc:identifier>http://purl.org/heritagedata/schemes/571/concepts/152379</dc:identifier>
    <dc:issued rdf:datatype="http://www.w3.org/2001/XMLSchema#dateTime">2024-07-01T17:17:33</dc:issued>
    <cc:license rdf:resource="https://www.nationalarchives.gov.uk/doc/open-government-licence/version/3/"/>
    <cc:attributionURL rdf:resource="https://historicengland.org.uk/"/>
    <cc:attributionName xml:lang="en">Historic England</cc:attributionName>
    <dc:publisher rdf:resource="https://historicengland.org.uk/"/>
    <dc:spatial rdf:resource="http://vocab.getty.edu/tgn/7002445"/>
    <dc:spatial rdf:resource="http://dbpedia.org/resource/England"/>
    <skos:prefLabel xml:lang="en">Grassland</skos:prefLabel>
    <skos:scopeNote xml:lang="en">Unimproved farmland, used primarily for grazing, where the vegetation is dominated by grasses and other herbaceous plants.</skos:scopeNote>
  </skos:Concept>

  <skos:Concept rdf:about="http://purl.org/heritagedata/schemes/571/concepts/152380">
    <skos:broader rdf:resource="http://purl.org/heritagedata/schemes/571/concepts/152379"/>
    <skos:narrower>
      <skos:Concept rdf:about="http://purl.org/heritagedata/schemes/571/concepts/160472">
        <skos:broader rdf:resource="http://purl.org/heritagedata/schemes/571/concepts/152380"/>
        <skos:inScheme rdf:resource="http://purl.org/heritagedata/schemes/571"/>
        <dc:identifier>http://purl.org/heritagedata/schemes/571/concepts/160472</dc:identifier>
        <dc:issued rdf:datatype="http://www.w3.org/2001/XMLSchema#dateTime">2024-07-01T17:17:33</dc:issued>
        <cc:license rdf:resource="https://www.nationalarchives.gov.uk/doc/open-government-licence/version/3/"/>
        <cc:attributionURL rdf:resource="https://historicengland.org.uk/"/>
        <cc:attributionName xml:lang="en">Historic England</cc:attributionName>
        <dc:publisher rdf:resource="https://historicengland.org.uk/"/>
        <dc:spatial rdf:resource="http://vocab.getty.edu/tgn/7002445"/>
        <dc:spatial rdf:resource="http://dbpedia.org/resource/England"/>
        <skos:prefLabel xml:lang="en">Chalk Grassland (Divided)</skos:prefLabel>
        <skos:scopeNote xml:lang="en">Chalk grassland, divided by stock-proof boundaries.</skos:scopeNote>
      </skos:Concept>
    </skos:narrower>

    <skos:narrower>
      <skos:Concept rdf:about="http://purl.org/heritagedata/schemes/571/concepts/160473">
        <skos:broader rdf:resource="http://purl.org/heritagedata/schemes/571/concepts/152380"/>
        <skos:inScheme rdf:resource="http://purl.org/heritagedata/schemes/571"/>
        <dc:identifier>http://purl.org/heritagedata/schemes/571/concepts/160473</dc:identifier>
        <dc:issued rdf:datatype="http://www.w3.org/2001/XMLSchema#dateTime">2024-07-01T17:17:33</dc:issued>
        <cc:license rdf:resource="https://www.nationalarchives.gov.uk/doc/open-government-licence/version/3/"/>
        <cc:attributionURL rdf:resource="https://historicengland.org.uk/"/>
        <cc:attributionName xml:lang="en">Historic England</cc:attributionName>
        <dc:publisher rdf:resource="https://historicengland.org.uk/"/>
        <dc:spatial rdf:resource="http://vocab.getty.edu/tgn/7002445"/>
        <dc:spatial rdf:resource="http://dbpedia.org/resource/England"/>
        <skos:prefLabel xml:lang="en">Chalk Grassland (Undivided)</skos:prefLabel>
        <skos:scopeNote xml:lang="en">Chalk grassland left open, undivided by stock-proof boundaries.</skos:scopeNote>
      </skos:Concept>
    </skos:narrower>

    <skos:inScheme rdf:resource="http://purl.org/heritagedata/schemes/571"/>
    <dc:identifier>http://purl.org/heritagedata/schemes/571/concepts/152380</dc:identifier>
    <dc:issued rdf:datatype="http://www.w3.org/2001/XMLSchema#dateTime">2024-07-01T17:17:33</dc:issued>
    <cc:license rdf:resource="https://www.nationalarchives.gov.uk/doc/open-government-licence/version/3/"/>
    <cc:attributionURL rdf:resource="https://historicengland.org.uk/"/>
    <cc:attributionName xml:lang="en">Historic England</cc:attributionName>
    <dc:publisher rdf:resource="https://historicengland.org.uk/"/>
    <dc:spatial rdf:resource="http://vocab.getty.edu/tgn/7002445"/>
    <dc:spatial rdf:resource="http://dbpedia.org/resource/England"/>
    <skos:prefLabel xml:lang="en">Chalk Grassland</skos:prefLabel>
    <skos:related rdf:resource="http://purl.org/heritagedata/schemes/571/concepts/151265"/>
    <skos:scopeNote xml:lang="en">Spieces-rich grazed land on chalk geology.</skos:scopeNote>
  </skos:Concept>

  <skos:Concept rdf:about="http://purl.org/heritagedata/schemes/571/concepts/152382">
    <skos:broader rdf:resource="http://purl.org/heritagedata/schemes/571/concepts/152326"/>
    <skos:narrower>
      <skos:Concept rdf:about="http://purl.org/heritagedata/schemes/571/concepts/160483">
        <skos:broader rdf:resource="http://purl.org/heritagedata/schemes/571/concepts/152382"/>
        <skos:inScheme rdf:resource="http://purl.org/heritagedata/schemes/571"/>
        <dc:identifier>http://purl.org/heritagedata/schemes/571/concepts/160483</dc:identifier>
        <dc:issued rdf:datatype="http://www.w3.org/2001/XMLSchema#dateTime">2024-07-01T17:17:33</dc:issued>
        <cc:license rdf:resource="https://www.nationalarchives.gov.uk/doc/open-government-licence/version/3/"/>
        <cc:attributionURL rdf:resource="https://historicengland.org.uk/"/>
        <cc:attributionName xml:lang="en">Historic England</cc:attributionName>
        <dc:publisher rdf:resource="https://historicengland.org.uk/"/>
        <dc:spatial rdf:resource="http://vocab.getty.edu/tgn/7002445"/>
        <dc:spatial rdf:resource="http://dbpedia.org/resource/England"/>
        <skos:prefLabel xml:lang="en">Peatland (Divided)</skos:prefLabel>
        <skos:scopeNote xml:lang="en">Peatland divided by stock-proof boundaries.</skos:scopeNote>
      </skos:Concept>
    </skos:narrower>

    <skos:narrower>
      <skos:Concept rdf:about="http://purl.org/heritagedata/schemes/571/concepts/160484">
        <skos:broader rdf:resource="http://purl.org/heritagedata/schemes/571/concepts/152382"/>
        <skos:inScheme rdf:resource="http://purl.org/heritagedata/schemes/571"/>
        <dc:identifier>http://purl.org/heritagedata/schemes/571/concepts/160484</dc:identifier>
        <dc:issued rdf:datatype="http://www.w3.org/2001/XMLSchema#dateTime">2024-07-01T17:17:33</dc:issued>
        <cc:license rdf:resource="https://www.nationalarchives.gov.uk/doc/open-government-licence/version/3/"/>
        <cc:attributionURL rdf:resource="https://historicengland.org.uk/"/>
        <cc:attributionName xml:lang="en">Historic England</cc:attributionName>
        <dc:publisher rdf:resource="https://historicengland.org.uk/"/>
        <dc:spatial rdf:resource="http://vocab.getty.edu/tgn/7002445"/>
        <dc:spatial rdf:resource="http://dbpedia.org/resource/England"/>
        <skos:prefLabel xml:lang="en">Peatland (Undivided)</skos:prefLabel>
        <skos:scopeNote xml:lang="en">Peatland left open, not divided by stock-proof boundaries.</skos:scopeNote>
      </skos:Concept>
    </skos:narrower>

    <skos:inScheme rdf:resource="http://purl.org/heritagedata/schemes/571"/>
    <dc:identifier>http://purl.org/heritagedata/schemes/571/concepts/152382</dc:identifier>
    <dc:issued rdf:datatype="http://www.w3.org/2001/XMLSchema#dateTime">2024-07-01T17:17:33</dc:issued>
    <cc:license rdf:resource="https://www.nationalarchives.gov.uk/doc/open-government-licence/version/3/"/>
    <cc:attributionURL rdf:resource="https://historicengland.org.uk/"/>
    <cc:attributionName xml:lang="en">Historic England</cc:attributionName>
    <dc:publisher rdf:resource="https://historicengland.org.uk/"/>
    <dc:spatial rdf:resource="http://vocab.getty.edu/tgn/7002445"/>
    <dc:spatial rdf:resource="http://dbpedia.org/resource/England"/>
    <skos:prefLabel xml:lang="en">Peatland</skos:prefLabel>
    <skos:scopeNote xml:lang="en">Land with peat soil, such as an active or former bog, the peat often cut for domestic fuel, the land often seasonally grazed. Often known as a 'moss'.</skos:scopeNote>
  </skos:Concept>

  <skos:Concept rdf:about="http://purl.org/heritagedata/schemes/571/concepts/152521">
    <skos:broader rdf:resource="http://purl.org/heritagedata/schemes/571/concepts/151461"/>
    <skos:inScheme rdf:resource="http://purl.org/heritagedata/schemes/571"/>
    <dc:identifier>http://purl.org/heritagedata/schemes/571/concepts/152521</dc:identifier>
    <dc:issued rdf:datatype="http://www.w3.org/2001/XMLSchema#dateTime">2024-07-01T17:17:33</dc:issued>
    <cc:license rdf:resource="https://www.nationalarchives.gov.uk/doc/open-government-licence/version/3/"/>
    <cc:attributionURL rdf:resource="https://historicengland.org.uk/"/>
    <cc:attributionName xml:lang="en">Historic England</cc:attributionName>
    <dc:publisher rdf:resource="https://historicengland.org.uk/"/>
    <dc:spatial rdf:resource="http://vocab.getty.edu/tgn/7002445"/>
    <dc:spatial rdf:resource="http://dbpedia.org/resource/England"/>
    <skos:prefLabel xml:lang="en">Aggregate Dredging</skos:prefLabel>
    <skos:related rdf:resource="http://purl.org/heritagedata/schemes/571/concepts/151419"/>
    <skos:scopeNote xml:lang="en">Areas characterised by the extraction of sand and gravel by dredging from the sea floor, for use principally in construction and civil engineering. Also includes associated onshore facilities such as wharves, and aggregates processing areas.</skos:scopeNote>
  </skos:Concept>

  <skos:Concept rdf:about="http://purl.org/heritagedata/schemes/571/concepts/152523">
    <skos:broader rdf:resource="http://purl.org/heritagedata/schemes/571/concepts/152539"/>
    <skos:inScheme rdf:resource="http://purl.org/heritagedata/schemes/571"/>
    <dc:identifier>http://purl.org/heritagedata/schemes/571/concepts/152523</dc:identifier>
    <dc:issued rdf:datatype="http://www.w3.org/2001/XMLSchema#dateTime">2024-07-01T17:17:33</dc:issued>
    <cc:license rdf:resource="https://www.nationalarchives.gov.uk/doc/open-government-licence/version/3/"/>
    <cc:attributionURL rdf:resource="https://historicengland.org.uk/"/>
    <cc:attributionName xml:lang="en">Historic England</cc:attributionName>
    <dc:publisher rdf:resource="https://historicengland.org.uk/"/>
    <dc:spatial rdf:resource="http://vocab.getty.edu/tgn/7002445"/>
    <dc:spatial rdf:resource="http://dbpedia.org/resource/England"/>
    <skos:prefLabel xml:lang="en">Daymark</skos:prefLabel>
    <skos:related rdf:resource="http://purl.org/heritagedata/schemes/571/concepts/151679"/>
    <skos:scopeNote xml:lang="en">An unlit, highly visible and distinctive feature on the coast that can be used by mariners for navigation during daylight only.</skos:scopeNote>
  </skos:Concept>

  <skos:Concept rdf:about="http://purl.org/heritagedata/schemes/571/concepts/152534">
    <skos:broader rdf:resource="http://purl.org/heritagedata/schemes/571/concepts/151443"/>
    <skos:broader rdf:resource="http://purl.org/heritagedata/schemes/571/concepts/151681"/>
    <skos:inScheme rdf:resource="http://purl.org/heritagedata/schemes/571"/>
    <dc:identifier>http://purl.org/heritagedata/schemes/571/concepts/152534</dc:identifier>
    <dc:issued rdf:datatype="http://www.w3.org/2001/XMLSchema#dateTime">2024-07-01T17:17:33</dc:issued>
    <cc:license rdf:resource="https://www.nationalarchives.gov.uk/doc/open-government-licence/version/3/"/>
    <cc:attributionURL rdf:resource="https://historicengland.org.uk/"/>
    <cc:attributionName xml:lang="en">Historic England</cc:attributionName>
    <dc:publisher rdf:resource="https://historicengland.org.uk/"/>
    <dc:spatial rdf:resource="http://vocab.getty.edu/tgn/7002445"/>
    <dc:spatial rdf:resource="http://dbpedia.org/resource/England"/>
    <skos:prefLabel xml:lang="en">Shoals And Flats</skos:prefLabel>
    <skos:scopeNote xml:lang="en">Shallow areas of sand banks, shoals, bars and spits, highly subject to change and extent of low tide exposure due to mobility of sediments.</skos:scopeNote>
  </skos:Concept>

  <skos:Concept rdf:about="http://purl.org/heritagedata/schemes/571/concepts/152565">
    <skos:broader rdf:resource="http://purl.org/heritagedata/schemes/571/concepts/152571"/>
    <skos:inScheme rdf:resource="http://purl.org/heritagedata/schemes/571"/>
    <dc:identifier>http://purl.org/heritagedata/schemes/571/concepts/152565</dc:identifier>
    <dc:issued rdf:datatype="http://www.w3.org/2001/XMLSchema#dateTime">2024-07-01T17:17:33</dc:issued>
    <cc:license rdf:resource="https://www.nationalarchives.gov.uk/doc/open-government-licence/version/3/"/>
    <cc:attributionURL rdf:resource="https://historicengland.org.uk/"/>
    <cc:attributionName xml:lang="en">Historic England</cc:attributionName>
    <dc:publisher rdf:resource="https://historicengland.org.uk/"/>
    <dc:spatial rdf:resource="http://vocab.getty.edu/tgn/7002445"/>
    <dc:spatial rdf:resource="http://dbpedia.org/resource/England"/>
    <skos:prefLabel xml:lang="en">Naval Battlefield</skos:prefLabel>
    <skos:scopeNote xml:lang="en">Recorded areas of former naval battles, where they form the dominant character of those areas. They may be associated with enhanced material imprints still extant in the form of wrecks and debris.</skos:scopeNote>
  </skos:Concept>

  <skos:Concept rdf:about="http://purl.org/heritagedata/schemes/571/concepts/152571">
    <skos:narrower rdf:resource="http://purl.org/heritagedata/schemes/571/concepts/152565"/>
    <skos:broader rdf:resource="http://purl.org/heritagedata/schemes/571/concepts/151447"/>
    <skos:inScheme rdf:resource="http://purl.org/heritagedata/schemes/571"/>
    <dc:identifier>http://purl.org/heritagedata/schemes/571/concepts/152571</dc:identifier>
    <dc:issued rdf:datatype="http://www.w3.org/2001/XMLSchema#dateTime">2024-07-01T17:17:33</dc:issued>
    <cc:license rdf:resource="https://www.nationalarchives.gov.uk/doc/open-government-licence/version/3/"/>
    <cc:attributionURL rdf:resource="https://historicengland.org.uk/"/>
    <cc:attributionName xml:lang="en">Historic England</cc:attributionName>
    <dc:publisher rdf:resource="https://historicengland.org.uk/"/>
    <dc:spatial rdf:resource="http://vocab.getty.edu/tgn/7002445"/>
    <dc:spatial rdf:resource="http://dbpedia.org/resource/England"/>
    <skos:prefLabel xml:lang="en">Battlefield</skos:prefLabel>
    <skos:scopeNote xml:lang="en">Recorded areas of former battles, where they form the dominant character of, or are the chief historical association attached to those areas.</skos:scopeNote>
  </skos:Concept>

  <skos:Concept rdf:about="http://purl.org/heritagedata/schemes/571/concepts/152583">
    <skos:broader rdf:resource="http://purl.org/heritagedata/schemes/571/concepts/151678"/>
    <skos:narrower>
      <skos:Concept rdf:about="http://purl.org/heritagedata/schemes/571/concepts/152584">
        <skos:broader rdf:resource="http://purl.org/heritagedata/schemes/571/concepts/152583"/>
        <skos:inScheme rdf:resource="http://purl.org/heritagedata/schemes/571"/>
        <dc:identifier>http://purl.org/heritagedata/schemes/571/concepts/152584</dc:identifier>
        <dc:issued rdf:datatype="http://www.w3.org/2001/XMLSchema#dateTime">2024-07-01T17:17:33</dc:issued>
        <cc:license rdf:resource="https://www.nationalarchives.gov.uk/doc/open-government-licence/version/3/"/>
        <cc:attributionURL rdf:resource="https://historicengland.org.uk/"/>
        <cc:attributionName xml:lang="en">Historic England</cc:attributionName>
        <dc:publisher rdf:resource="https://historicengland.org.uk/"/>
        <dc:spatial rdf:resource="http://vocab.getty.edu/tgn/7002445"/>
        <dc:spatial rdf:resource="http://dbpedia.org/resource/England"/>
        <skos:prefLabel xml:lang="en">Active Navigation Channel</skos:prefLabel>
        <skos:scopeNote xml:lang="en">Sea or river channels, charted or otherwise, recorded as in active use by present shipping traffic, whatever the channels' date of origin.</skos:scopeNote>
      </skos:Concept>
    </skos:narrower>

    <skos:narrower rdf:resource="http://purl.org/heritagedata/schemes/571/concepts/152585"/>
    <skos:inScheme rdf:resource="http://purl.org/heritagedata/schemes/571"/>
    <dc:identifier>http://purl.org/heritagedata/schemes/571/concepts/152583</dc:identifier>
    <dc:issued rdf:datatype="http://www.w3.org/2001/XMLSchema#dateTime">2024-07-01T17:17:33</dc:issued>
    <cc:license rdf:resource="https://www.nationalarchives.gov.uk/doc/open-government-licence/version/3/"/>
    <cc:attributionURL rdf:resource="https://historicengland.org.uk/"/>
    <cc:attributionName xml:lang="en">Historic England</cc:attributionName>
    <dc:publisher rdf:resource="https://historicengland.org.uk/"/>
    <dc:spatial rdf:resource="http://vocab.getty.edu/tgn/7002445"/>
    <dc:spatial rdf:resource="http://dbpedia.org/resource/England"/>
    <skos:prefLabel xml:lang="en">Navigation Channel</skos:prefLabel>
    <skos:scopeNote xml:lang="en">Sea and river channels, charted or otherwise, used for shipping traffic. Use more specific type were known.</skos:scopeNote>
  </skos:Concept>

  <skos:Concept rdf:about="http://purl.org/heritagedata/schemes/571/concepts/152585">
    <skos:broader rdf:resource="http://purl.org/heritagedata/schemes/571/concepts/152583"/>
    <skos:narrower>
      <skos:Concept rdf:about="http://purl.org/heritagedata/schemes/571/concepts/152586">
        <skos:broader rdf:resource="http://purl.org/heritagedata/schemes/571/concepts/152585"/>
        <skos:inScheme rdf:resource="http://purl.org/heritagedata/schemes/571"/>
        <dc:identifier>http://purl.org/heritagedata/schemes/571/concepts/152586</dc:identifier>
        <dc:issued rdf:datatype="http://www.w3.org/2001/XMLSchema#dateTime">2024-07-01T17:17:33</dc:issued>
        <cc:license rdf:resource="https://www.nationalarchives.gov.uk/doc/open-government-licence/version/3/"/>
        <cc:attributionURL rdf:resource="https://historicengland.org.uk/"/>
        <cc:attributionName xml:lang="en">Historic England</cc:attributionName>
        <dc:publisher rdf:resource="https://historicengland.org.uk/"/>
        <dc:spatial rdf:resource="http://vocab.getty.edu/tgn/7002445"/>
        <dc:spatial rdf:resource="http://dbpedia.org/resource/England"/>
        <skos:prefLabel xml:lang="en">Buried Navigation Channel</skos:prefLabel>
        <skos:scopeNote xml:lang="en">Sea or river channels no longer charted or recorded as in active navigational use for present shipping traffic and with evidence that the channel is also now a buried feature (if extant at all).</skos:scopeNote>
      </skos:Concept>
    </skos:narrower>

    <skos:inScheme rdf:resource="http://purl.org/heritagedata/schemes/571"/>
    <dc:identifier>http://purl.org/heritagedata/schemes/571/concepts/152585</dc:identifier>
    <dc:issued rdf:datatype="http://www.w3.org/2001/XMLSchema#dateTime">2024-07-01T17:17:33</dc:issued>
    <cc:license rdf:resource="https://www.nationalarchives.gov.uk/doc/open-government-licence/version/3/"/>
    <cc:attributionURL rdf:resource="https://historicengland.org.uk/"/>
    <cc:attributionName xml:lang="en">Historic England</cc:attributionName>
    <dc:publisher rdf:resource="https://historicengland.org.uk/"/>
    <dc:spatial rdf:resource="http://vocab.getty.edu/tgn/7002445"/>
    <dc:spatial rdf:resource="http://dbpedia.org/resource/England"/>
    <skos:prefLabel xml:lang="en">Disused Navigation Channel</skos:prefLabel>
    <skos:scopeNote xml:lang="en">Sea and river channels no longer charted or recorded as in active navigational use for present shipping traffic, whatever the channel's broad date of origin.</skos:scopeNote>
  </skos:Concept>

  <skos:Concept rdf:about="http://purl.org/heritagedata/schemes/571/concepts/152587">
    <skos:broader rdf:resource="http://purl.org/heritagedata/schemes/571/concepts/151667"/>
    <skos:inScheme rdf:resource="http://purl.org/heritagedata/schemes/571"/>
    <dc:identifier>http://purl.org/heritagedata/schemes/571/concepts/152587</dc:identifier>
    <dc:issued rdf:datatype="http://www.w3.org/2001/XMLSchema#dateTime">2024-07-01T17:17:33</dc:issued>
    <cc:license rdf:resource="https://www.nationalarchives.gov.uk/doc/open-government-licence/version/3/"/>
    <cc:attributionURL rdf:resource="https://historicengland.org.uk/"/>
    <cc:attributionName xml:lang="en">Historic England</cc:attributionName>
    <dc:publisher rdf:resource="https://historicengland.org.uk/"/>
    <dc:spatial rdf:resource="http://vocab.getty.edu/tgn/7002445"/>
    <dc:spatial rdf:resource="http://dbpedia.org/resource/England"/>
    <skos:prefLabel xml:lang="en">Harbour Pool</skos:prefLabel>
    <skos:related rdf:resource="http://purl.org/heritagedata/schemes/571/concepts/151404"/>
    <skos:scopeNote xml:lang="en">An area of water adjacent to a port or harbour, falling under the jurisdiction of a port/harbour authority. Includes associated traffic areas and restricted navigation areas.</skos:scopeNote>
  </skos:Concept>

  <skos:Concept rdf:about="http://purl.org/heritagedata/schemes/571/concepts/152593">
    <skos:broader rdf:resource="http://purl.org/heritagedata/schemes/571/concepts/152591"/>
    <skos:broader rdf:resource="http://purl.org/heritagedata/schemes/571/concepts/151250"/>
    <skos:inScheme rdf:resource="http://purl.org/heritagedata/schemes/571"/>
    <dc:identifier>http://purl.org/heritagedata/schemes/571/concepts/152593</dc:identifier>
    <dc:issued rdf:datatype="http://www.w3.org/2001/XMLSchema#dateTime">2024-07-01T17:17:33</dc:issued>
    <cc:license rdf:resource="https://www.nationalarchives.gov.uk/doc/open-government-licence/version/3/"/>
    <cc:attributionURL rdf:resource="https://historicengland.org.uk/"/>
    <cc:attributionName xml:lang="en">Historic England</cc:attributionName>
    <dc:publisher rdf:resource="https://historicengland.org.uk/"/>
    <dc:spatial rdf:resource="http://vocab.getty.edu/tgn/7002445"/>
    <dc:spatial rdf:resource="http://dbpedia.org/resource/England"/>
    <skos:prefLabel xml:lang="en">Peat Deposit</skos:prefLabel>
    <skos:related rdf:resource="http://purl.org/heritagedata/schemes/571/concepts/151611"/>
    <skos:scopeNote xml:lang="en">Peat deposits comprise unconsolidated semi-carbonised plant remains formed in freshwater-saturated environments. The type referred to here are those formed in earlier periods and may be exposed by erosion on the land, inter-tidal or sea-floor surface.</skos:scopeNote>
  </skos:Concept>

  <skos:Concept rdf:about="http://purl.org/heritagedata/schemes/571/concepts/152595">
    <skos:broader rdf:resource="http://purl.org/heritagedata/schemes/571/concepts/151456"/>
    <skos:narrower>
      <skos:Concept rdf:about="http://purl.org/heritagedata/schemes/571/concepts/152596">
        <skos:broader rdf:resource="http://purl.org/heritagedata/schemes/571/concepts/152595"/>
        <skos:inScheme rdf:resource="http://purl.org/heritagedata/schemes/571"/>
        <dc:identifier>http://purl.org/heritagedata/schemes/571/concepts/152596</dc:identifier>
        <dc:issued rdf:datatype="http://www.w3.org/2001/XMLSchema#dateTime">2024-07-01T17:17:33</dc:issued>
        <cc:license rdf:resource="https://www.nationalarchives.gov.uk/doc/open-government-licence/version/3/"/>
        <cc:attributionURL rdf:resource="https://historicengland.org.uk/"/>
        <cc:attributionName xml:lang="en">Historic England</cc:attributionName>
        <dc:publisher rdf:resource="https://historicengland.org.uk/"/>
        <dc:spatial rdf:resource="http://vocab.getty.edu/tgn/7002445"/>
        <dc:spatial rdf:resource="http://dbpedia.org/resource/England"/>
        <skos:prefLabel xml:lang="en">Coarse Sediment Plain</skos:prefLabel>
        <skos:scopeNote xml:lang="en">Extensive areas of seafloor whose surface sediments predominantly comprise different grades of pebbles, rocks, boulders etc with lower sand and very low silt and clay contents.</skos:scopeNote>
      </skos:Concept>
    </skos:narrower>

    <skos:narrower>
      <skos:Concept rdf:about="http://purl.org/heritagedata/schemes/571/concepts/152597">
        <skos:broader rdf:resource="http://purl.org/heritagedata/schemes/571/concepts/152595"/>
        <skos:inScheme rdf:resource="http://purl.org/heritagedata/schemes/571"/>
        <dc:identifier>http://purl.org/heritagedata/schemes/571/concepts/152597</dc:identifier>
        <dc:issued rdf:datatype="http://www.w3.org/2001/XMLSchema#dateTime">2024-07-01T17:17:33</dc:issued>
        <cc:license rdf:resource="https://www.nationalarchives.gov.uk/doc/open-government-licence/version/3/"/>
        <cc:attributionURL rdf:resource="https://historicengland.org.uk/"/>
        <cc:attributionName xml:lang="en">Historic England</cc:attributionName>
        <dc:publisher rdf:resource="https://historicengland.org.uk/"/>
        <dc:spatial rdf:resource="http://vocab.getty.edu/tgn/7002445"/>
        <dc:spatial rdf:resource="http://dbpedia.org/resource/England"/>
        <skos:prefLabel xml:lang="en">Fine Sediment Plain</skos:prefLabel>
        <skos:scopeNote xml:lang="en">Large areas of seafloor whose surface sediments predominantly comprise different grades of sand and very low silt and clay content.</skos:scopeNote>
      </skos:Concept>
    </skos:narrower>

    <skos:narrower>
      <skos:Concept rdf:about="http://purl.org/heritagedata/schemes/571/concepts/152598">
        <skos:broader rdf:resource="http://purl.org/heritagedata/schemes/571/concepts/152595"/>
        <skos:inScheme rdf:resource="http://purl.org/heritagedata/schemes/571"/>
        <dc:identifier>http://purl.org/heritagedata/schemes/571/concepts/152598</dc:identifier>
        <dc:issued rdf:datatype="http://www.w3.org/2001/XMLSchema#dateTime">2024-07-01T17:17:33</dc:issued>
        <cc:license rdf:resource="https://www.nationalarchives.gov.uk/doc/open-government-licence/version/3/"/>
        <cc:attributionURL rdf:resource="https://historicengland.org.uk/"/>
        <cc:attributionName xml:lang="en">Historic England</cc:attributionName>
        <dc:publisher rdf:resource="https://historicengland.org.uk/"/>
        <dc:spatial rdf:resource="http://vocab.getty.edu/tgn/7002445"/>
        <dc:spatial rdf:resource="http://dbpedia.org/resource/England"/>
        <skos:prefLabel xml:lang="en">Mud Plain</skos:prefLabel>
        <skos:scopeNote xml:lang="en">Extensive areas of seafloor whose surface sediments predominantly comprise fine sediment grades with high silt and clay contents.</skos:scopeNote>
      </skos:Concept>
    </skos:narrower>

    <skos:narrower>
      <skos:Concept rdf:about="http://purl.org/heritagedata/schemes/571/concepts/152599">
        <skos:broader rdf:resource="http://purl.org/heritagedata/schemes/571/concepts/152595"/>
        <skos:inScheme rdf:resource="http://purl.org/heritagedata/schemes/571"/>
        <dc:identifier>http://purl.org/heritagedata/schemes/571/concepts/152599</dc:identifier>
        <dc:issued rdf:datatype="http://www.w3.org/2001/XMLSchema#dateTime">2024-07-01T17:17:33</dc:issued>
        <cc:license rdf:resource="https://www.nationalarchives.gov.uk/doc/open-government-licence/version/3/"/>
        <cc:attributionURL rdf:resource="https://historicengland.org.uk/"/>
        <cc:attributionName xml:lang="en">Historic England</cc:attributionName>
        <dc:publisher rdf:resource="https://historicengland.org.uk/"/>
        <dc:spatial rdf:resource="http://vocab.getty.edu/tgn/7002445"/>
        <dc:spatial rdf:resource="http://dbpedia.org/resource/England"/>
        <skos:prefLabel xml:lang="en">Mixed Sediment Plain</skos:prefLabel>
        <skos:scopeNote xml:lang="en">Large areas of seafloor whose surface sediments predominantly comprise heterogeneous sediment grades, from pebbles and gravels to sands, silts and clays. The overall composition can be highly variable, as can the form of their grades' mixing.</skos:scopeNote>
      </skos:Concept>
    </skos:narrower>

    <skos:narrower>
      <skos:Concept rdf:about="http://purl.org/heritagedata/schemes/571/concepts/152600">
        <skos:broader rdf:resource="http://purl.org/heritagedata/schemes/571/concepts/152595"/>
        <skos:inScheme rdf:resource="http://purl.org/heritagedata/schemes/571"/>
        <dc:identifier>http://purl.org/heritagedata/schemes/571/concepts/152600</dc:identifier>
        <dc:issued rdf:datatype="http://www.w3.org/2001/XMLSchema#dateTime">2024-07-01T17:17:33</dc:issued>
        <cc:license rdf:resource="https://www.nationalarchives.gov.uk/doc/open-government-licence/version/3/"/>
        <cc:attributionURL rdf:resource="https://historicengland.org.uk/"/>
        <cc:attributionName xml:lang="en">Historic England</cc:attributionName>
        <dc:publisher rdf:resource="https://historicengland.org.uk/"/>
        <dc:spatial rdf:resource="http://vocab.getty.edu/tgn/7002445"/>
        <dc:spatial rdf:resource="http://dbpedia.org/resource/England"/>
        <skos:prefLabel xml:lang="en">Sandbanks With Sandwaves</skos:prefLabel>
        <skos:scopeNote xml:lang="en">An area of sand banks containing extensive wavelike structures and megaripples formed by rapidly moving currents of water on the sandbanks' surface. May occur around the margins of sandflats or they may occur in deeper water.</skos:scopeNote>
      </skos:Concept>
    </skos:narrower>

    <skos:narrower rdf:resource="http://purl.org/heritagedata/schemes/571/concepts/152601"/>
    <skos:inScheme rdf:resource="http://purl.org/heritagedata/schemes/571"/>
    <dc:identifier>http://purl.org/heritagedata/schemes/571/concepts/152595</dc:identifier>
    <dc:issued rdf:datatype="http://www.w3.org/2001/XMLSchema#dateTime">2024-07-01T17:17:33</dc:issued>
    <cc:license rdf:resource="https://www.nationalarchives.gov.uk/doc/open-government-licence/version/3/"/>
    <cc:attributionURL rdf:resource="https://historicengland.org.uk/"/>
    <cc:attributionName xml:lang="en">Historic England</cc:attributionName>
    <dc:publisher rdf:resource="https://historicengland.org.uk/"/>
    <dc:spatial rdf:resource="http://vocab.getty.edu/tgn/7002445"/>
    <dc:spatial rdf:resource="http://dbpedia.org/resource/England"/>
    <skos:prefLabel xml:lang="en">Marine</skos:prefLabel>
    <skos:scopeNote xml:lang="en">Of the sea, at any or all of its layers: surface, water column, floor and sub-floor.</skos:scopeNote>
  </skos:Concept>

  <skos:Concept rdf:about="http://purl.org/heritagedata/schemes/571/concepts/152601">
    <skos:broader rdf:resource="http://purl.org/heritagedata/schemes/571/concepts/152595"/>
    <skos:broader rdf:resource="http://purl.org/heritagedata/schemes/571/concepts/152320"/>
    <skos:inScheme rdf:resource="http://purl.org/heritagedata/schemes/571"/>
    <dc:identifier>http://purl.org/heritagedata/schemes/571/concepts/152601</dc:identifier>
    <dc:issued rdf:datatype="http://www.w3.org/2001/XMLSchema#dateTime">2024-07-01T17:17:33</dc:issued>
    <cc:license rdf:resource="https://www.nationalarchives.gov.uk/doc/open-government-licence/version/3/"/>
    <cc:attributionURL rdf:resource="https://historicengland.org.uk/"/>
    <cc:attributionName xml:lang="en">Historic England</cc:attributionName>
    <dc:publisher rdf:resource="https://historicengland.org.uk/"/>
    <dc:spatial rdf:resource="http://vocab.getty.edu/tgn/7002445"/>
    <dc:spatial rdf:resource="http://dbpedia.org/resource/England"/>
    <skos:prefLabel xml:lang="en">Exposed Bedrock</skos:prefLabel>
    <skos:scopeNote xml:lang="en">Areas whose surface predominantly comprises bedrock exposures. On the sea-floor can be associated with rocks and boulders but little finer sediment deposition.</skos:scopeNote>
  </skos:Concept>

  <skos:Concept rdf:about="http://purl.org/heritagedata/schemes/571/concepts/152608">
    <skos:broader rdf:resource="http://purl.org/heritagedata/schemes/571/concepts/152379"/>
    <skos:narrower>
      <skos:Concept rdf:about="http://purl.org/heritagedata/schemes/571/concepts/160485">
        <skos:broader rdf:resource="http://purl.org/heritagedata/schemes/571/concepts/152608"/>
        <skos:inScheme rdf:resource="http://purl.org/heritagedata/schemes/571"/>
        <dc:identifier>http://purl.org/heritagedata/schemes/571/concepts/160485</dc:identifier>
        <dc:issued rdf:datatype="http://www.w3.org/2001/XMLSchema#dateTime">2024-07-01T17:17:33</dc:issued>
        <cc:license rdf:resource="https://www.nationalarchives.gov.uk/doc/open-government-licence/version/3/"/>
        <cc:attributionURL rdf:resource="https://historicengland.org.uk/"/>
        <cc:attributionName xml:lang="en">Historic England</cc:attributionName>
        <dc:publisher rdf:resource="https://historicengland.org.uk/"/>
        <dc:spatial rdf:resource="http://vocab.getty.edu/tgn/7002445"/>
        <dc:spatial rdf:resource="http://dbpedia.org/resource/England"/>
        <skos:prefLabel xml:lang="en">Rough Grassland (Divided)</skos:prefLabel>
        <skos:scopeNote xml:lang="en">Rough Grassland divided by stock-proof boundaries.</skos:scopeNote>
      </skos:Concept>
    </skos:narrower>

    <skos:narrower>
      <skos:Concept rdf:about="http://purl.org/heritagedata/schemes/571/concepts/160486">
        <skos:broader rdf:resource="http://purl.org/heritagedata/schemes/571/concepts/152608"/>
        <skos:inScheme rdf:resource="http://purl.org/heritagedata/schemes/571"/>
        <dc:identifier>http://purl.org/heritagedata/schemes/571/concepts/160486</dc:identifier>
        <dc:issued rdf:datatype="http://www.w3.org/2001/XMLSchema#dateTime">2024-07-01T17:17:33</dc:issued>
        <cc:license rdf:resource="https://www.nationalarchives.gov.uk/doc/open-government-licence/version/3/"/>
        <cc:attributionURL rdf:resource="https://historicengland.org.uk/"/>
        <cc:attributionName xml:lang="en">Historic England</cc:attributionName>
        <dc:publisher rdf:resource="https://historicengland.org.uk/"/>
        <dc:spatial rdf:resource="http://vocab.getty.edu/tgn/7002445"/>
        <dc:spatial rdf:resource="http://dbpedia.org/resource/England"/>
        <skos:prefLabel xml:lang="en">Rough Grassland (Undivided)</skos:prefLabel>
        <skos:scopeNote xml:lang="en">Rough grassland left open, not divided by stock-proof boundaries.</skos:scopeNote>
      </skos:Concept>
    </skos:narrower>

    <skos:inScheme rdf:resource="http://purl.org/heritagedata/schemes/571"/>
    <dc:identifier>http://purl.org/heritagedata/schemes/571/concepts/152608</dc:identifier>
    <dc:issued rdf:datatype="http://www.w3.org/2001/XMLSchema#dateTime">2024-07-01T17:17:33</dc:issued>
    <cc:license rdf:resource="https://www.nationalarchives.gov.uk/doc/open-government-licence/version/3/"/>
    <cc:attributionURL rdf:resource="https://historicengland.org.uk/"/>
    <cc:attributionName xml:lang="en">Historic England</cc:attributionName>
    <dc:publisher rdf:resource="https://historicengland.org.uk/"/>
    <dc:spatial rdf:resource="http://vocab.getty.edu/tgn/7002445"/>
    <dc:spatial rdf:resource="http://dbpedia.org/resource/England"/>
    <skos:prefLabel xml:lang="en">Rough Grassland</skos:prefLabel>
    <skos:scopeNote xml:lang="en">Area of rough ground dominated by unintensively managed grassland often the result of long traditions of rough grazing or a conservation measure to prevent land reverting to scrub.</skos:scopeNote>
  </skos:Concept>

  <skos:Concept rdf:about="http://purl.org/heritagedata/schemes/571/concepts/152620">
    <skos:broader rdf:resource="http://purl.org/heritagedata/schemes/571/concepts/152605"/>
    <skos:inScheme rdf:resource="http://purl.org/heritagedata/schemes/571"/>
    <dc:identifier>http://purl.org/heritagedata/schemes/571/concepts/152620</dc:identifier>
    <dc:issued rdf:datatype="http://www.w3.org/2001/XMLSchema#dateTime">2024-07-01T17:17:33</dc:issued>
    <cc:license rdf:resource="https://www.nationalarchives.gov.uk/doc/open-government-licence/version/3/"/>
    <cc:attributionURL rdf:resource="https://historicengland.org.uk/"/>
    <cc:attributionName xml:lang="en">Historic England</cc:attributionName>
    <dc:publisher rdf:resource="https://historicengland.org.uk/"/>
    <dc:spatial rdf:resource="http://vocab.getty.edu/tgn/7002445"/>
    <dc:spatial rdf:resource="http://dbpedia.org/resource/England"/>
    <skos:prefLabel xml:lang="en">Overhead Power Cable</skos:prefLabel>
    <skos:related rdf:resource="http://purl.org/heritagedata/schemes/571/concepts/151746"/>
    <skos:scopeNote xml:lang="en">Raised cable supported on pylons or other structures and used to transmit electricity over long distances.</skos:scopeNote>
  </skos:Concept>

  <skos:Concept rdf:about="http://purl.org/heritagedata/schemes/571/concepts/152621">
    <skos:broader rdf:resource="http://purl.org/heritagedata/schemes/571/concepts/152605"/>
    <skos:inScheme rdf:resource="http://purl.org/heritagedata/schemes/571"/>
    <dc:identifier>http://purl.org/heritagedata/schemes/571/concepts/152621</dc:identifier>
    <dc:issued rdf:datatype="http://www.w3.org/2001/XMLSchema#dateTime">2024-07-01T17:17:33</dc:issued>
    <cc:license rdf:resource="https://www.nationalarchives.gov.uk/doc/open-government-licence/version/3/"/>
    <cc:attributionURL rdf:resource="https://historicengland.org.uk/"/>
    <cc:attributionName xml:lang="en">Historic England</cc:attributionName>
    <dc:publisher rdf:resource="https://historicengland.org.uk/"/>
    <dc:spatial rdf:resource="http://vocab.getty.edu/tgn/7002445"/>
    <dc:spatial rdf:resource="http://dbpedia.org/resource/England"/>
    <skos:prefLabel xml:lang="en">Submarine Power Cable</skos:prefLabel>
    <skos:related rdf:resource="http://purl.org/heritagedata/schemes/571/concepts/151746"/>
    <skos:scopeNote xml:lang="en">Cable laid on or beneath the sea floor and used to transmit electricity from the mainland to islands or to offshore installations, or to link offshore electricity generators to the onshore national electricity grid.</skos:scopeNote>
  </skos:Concept>

  <skos:Concept rdf:about="http://purl.org/heritagedata/schemes/571/concepts/152623">
    <skos:broader rdf:resource="http://purl.org/heritagedata/schemes/571/concepts/152624"/>
    <skos:inScheme rdf:resource="http://purl.org/heritagedata/schemes/571"/>
    <dc:identifier>http://purl.org/heritagedata/schemes/571/concepts/152623</dc:identifier>
    <dc:issued rdf:datatype="http://www.w3.org/2001/XMLSchema#dateTime">2024-07-01T17:17:33</dc:issued>
    <cc:license rdf:resource="https://www.nationalarchives.gov.uk/doc/open-government-licence/version/3/"/>
    <cc:attributionURL rdf:resource="https://historicengland.org.uk/"/>
    <cc:attributionName xml:lang="en">Historic England</cc:attributionName>
    <dc:publisher rdf:resource="https://historicengland.org.uk/"/>
    <dc:spatial rdf:resource="http://vocab.getty.edu/tgn/7002445"/>
    <dc:spatial rdf:resource="http://dbpedia.org/resource/England"/>
    <skos:prefLabel xml:lang="en">Spoil And Waste Dumping</skos:prefLabel>
    <skos:related rdf:resource="http://purl.org/heritagedata/schemes/571/concepts/151436"/>
    <skos:scopeNote xml:lang="en">Areas used for the disposal of domestic and/or industrial waste. Material deposited may include dredging spoil, drilling waste, treated sewage, domestic refuse and other land waste.</skos:scopeNote>
  </skos:Concept>

  <skos:Concept rdf:about="http://purl.org/heritagedata/schemes/571/concepts/152628">
    <skos:broader rdf:resource="http://purl.org/heritagedata/schemes/571/concepts/151204"/>
    <skos:inScheme rdf:resource="http://purl.org/heritagedata/schemes/571"/>
    <dc:identifier>http://purl.org/heritagedata/schemes/571/concepts/152628</dc:identifier>
    <dc:issued rdf:datatype="http://www.w3.org/2001/XMLSchema#dateTime">2024-07-01T17:17:33</dc:issued>
    <cc:license rdf:resource="https://www.nationalarchives.gov.uk/doc/open-government-licence/version/3/"/>
    <cc:attributionURL rdf:resource="https://historicengland.org.uk/"/>
    <cc:attributionName xml:lang="en">Historic England</cc:attributionName>
    <dc:publisher rdf:resource="https://historicengland.org.uk/"/>
    <dc:spatial rdf:resource="http://vocab.getty.edu/tgn/7002445"/>
    <dc:spatial rdf:resource="http://dbpedia.org/resource/England"/>
    <skos:prefLabel xml:lang="en">Hydrocarbon Pipeline</skos:prefLabel>
    <skos:related rdf:resource="http://purl.org/heritagedata/schemes/571/concepts/160169"/>
    <skos:scopeNote xml:lang="en">A pipeline involved in the transmission of oil or natural gas between facilities involved in their extraction, processing, storage or distribution.</skos:scopeNote>
  </skos:Concept>

  <skos:Concept rdf:about="http://purl.org/heritagedata/schemes/571/concepts/152638">
    <skos:broader rdf:resource="http://purl.org/heritagedata/schemes/571/concepts/151457"/>
    <skos:narrower rdf:resource="http://purl.org/heritagedata/schemes/571/concepts/160188"/>
    <skos:inScheme rdf:resource="http://purl.org/heritagedata/schemes/571"/>
    <dc:identifier>http://purl.org/heritagedata/schemes/571/concepts/152638</dc:identifier>
    <dc:issued rdf:datatype="http://www.w3.org/2001/XMLSchema#dateTime">2024-07-01T17:17:33</dc:issued>
    <cc:license rdf:resource="https://www.nationalarchives.gov.uk/doc/open-government-licence/version/3/"/>
    <cc:attributionURL rdf:resource="https://historicengland.org.uk/"/>
    <cc:attributionName xml:lang="en">Historic England</cc:attributionName>
    <dc:publisher rdf:resource="https://historicengland.org.uk/"/>
    <dc:spatial rdf:resource="http://vocab.getty.edu/tgn/7002445"/>
    <dc:spatial rdf:resource="http://dbpedia.org/resource/England"/>
    <skos:prefLabel xml:lang="en">Shipping Industry</skos:prefLabel>
    <skos:scopeNote xml:lang="en">Areas dominated by activity relating directly to the building, use, maintenance, storage and administration of shipping and boats..</skos:scopeNote>
  </skos:Concept>

  <skos:Concept rdf:about="http://purl.org/heritagedata/schemes/571/concepts/160155">
    <skos:broader rdf:resource="http://purl.org/heritagedata/schemes/571/concepts/151453"/>
    <skos:inScheme rdf:resource="http://purl.org/heritagedata/schemes/571"/>
    <dc:identifier>http://purl.org/heritagedata/schemes/571/concepts/160155</dc:identifier>
    <dc:issued rdf:datatype="http://www.w3.org/2001/XMLSchema#dateTime">2024-07-01T17:17:33</dc:issued>
    <cc:license rdf:resource="https://www.nationalarchives.gov.uk/doc/open-government-licence/version/3/"/>
    <cc:attributionURL rdf:resource="https://historicengland.org.uk/"/>
    <cc:attributionName xml:lang="en">Historic England</cc:attributionName>
    <dc:publisher rdf:resource="https://historicengland.org.uk/"/>
    <dc:spatial rdf:resource="http://vocab.getty.edu/tgn/7002445"/>
    <dc:spatial rdf:resource="http://dbpedia.org/resource/England"/>
    <skos:prefLabel xml:lang="en">Anciently Enclosed Land</skos:prefLabel>
    <skos:related rdf:resource="http://purl.org/heritagedata/schemes/571/concepts/151173"/>
    <skos:related rdf:resource="http://purl.org/heritagedata/schemes/571/concepts/151176"/>
    <skos:related rdf:resource="http://purl.org/heritagedata/schemes/571/concepts/151181"/>
    <skos:related rdf:resource="http://purl.org/heritagedata/schemes/571/concepts/151728"/>
    <skos:related rdf:resource="http://purl.org/heritagedata/schemes/571/concepts/151730"/>
    <skos:related rdf:resource="http://purl.org/heritagedata/schemes/571/concepts/151780"/>
    <skos:related rdf:resource="http://purl.org/heritagedata/schemes/571/concepts/160157"/>
    <skos:related rdf:resource="http://purl.org/heritagedata/schemes/571/concepts/160156"/>
    <skos:related rdf:resource="http://purl.org/heritagedata/schemes/571/concepts/160158"/>
    <skos:related rdf:resource="http://purl.org/heritagedata/schemes/571/concepts/160160"/>
    <skos:scopeNote xml:lang="en">Early farmland, whose predominant character developed by the later medieval or earlier. Usually broad-brush characterisation that includes farming settlement and various other land use.</skos:scopeNote>
  </skos:Concept>

  <skos:Concept rdf:about="http://purl.org/heritagedata/schemes/571/concepts/160156">
    <skos:broader rdf:resource="http://purl.org/heritagedata/schemes/571/concepts/151453"/>
    <skos:inScheme rdf:resource="http://purl.org/heritagedata/schemes/571"/>
    <dc:identifier>http://purl.org/heritagedata/schemes/571/concepts/160156</dc:identifier>
    <dc:issued rdf:datatype="http://www.w3.org/2001/XMLSchema#dateTime">2024-07-01T17:17:33</dc:issued>
    <cc:license rdf:resource="https://www.nationalarchives.gov.uk/doc/open-government-licence/version/3/"/>
    <cc:attributionURL rdf:resource="https://historicengland.org.uk/"/>
    <cc:attributionName xml:lang="en">Historic England</cc:attributionName>
    <dc:publisher rdf:resource="https://historicengland.org.uk/"/>
    <dc:spatial rdf:resource="http://vocab.getty.edu/tgn/7002445"/>
    <dc:spatial rdf:resource="http://dbpedia.org/resource/England"/>
    <skos:prefLabel xml:lang="en">Assart</skos:prefLabel>
    <skos:related rdf:resource="http://purl.org/heritagedata/schemes/571/concepts/160155"/>
    <skos:related rdf:resource="http://purl.org/heritagedata/schemes/571/concepts/160166"/>
    <skos:scopeNote xml:lang="en">Land enclosed from woodland. Required licence in medieval period. Term applied more generally in landscape history. Can include planned and regular enclosures and piecemeal irregular ones. Often still with numerous trees on boundaries.</skos:scopeNote>
  </skos:Concept>

  <skos:Concept rdf:about="http://purl.org/heritagedata/schemes/571/concepts/160157">
    <skos:broader rdf:resource="http://purl.org/heritagedata/schemes/571/concepts/151727"/>
    <skos:inScheme rdf:resource="http://purl.org/heritagedata/schemes/571"/>
    <dc:identifier>http://purl.org/heritagedata/schemes/571/concepts/160157</dc:identifier>
    <dc:issued rdf:datatype="http://www.w3.org/2001/XMLSchema#dateTime">2024-07-01T17:17:33</dc:issued>
    <cc:license rdf:resource="https://www.nationalarchives.gov.uk/doc/open-government-licence/version/3/"/>
    <cc:attributionURL rdf:resource="https://historicengland.org.uk/"/>
    <cc:attributionName xml:lang="en">Historic England</cc:attributionName>
    <dc:publisher rdf:resource="https://historicengland.org.uk/"/>
    <dc:spatial rdf:resource="http://vocab.getty.edu/tgn/7002445"/>
    <dc:spatial rdf:resource="http://dbpedia.org/resource/England"/>
    <skos:prefLabel xml:lang="en">Barton Demesne Fields</skos:prefLabel>
    <skos:related rdf:resource="http://purl.org/heritagedata/schemes/571/concepts/160155"/>
    <skos:related rdf:resource="http://purl.org/heritagedata/schemes/571/concepts/160166"/>
    <skos:scopeNote xml:lang="en">Field patterns established by lord of an estate, usually as closes (bounded individual fields), in distinction to the open common fields of tenants. They tend to be relatively large fields.</skos:scopeNote>
  </skos:Concept>

  <skos:Concept rdf:about="http://purl.org/heritagedata/schemes/571/concepts/160158">
    <skos:broader rdf:resource="http://purl.org/heritagedata/schemes/571/concepts/151730"/>
    <skos:inScheme rdf:resource="http://purl.org/heritagedata/schemes/571"/>
    <dc:identifier>http://purl.org/heritagedata/schemes/571/concepts/160158</dc:identifier>
    <dc:issued rdf:datatype="http://www.w3.org/2001/XMLSchema#dateTime">2024-07-01T17:17:33</dc:issued>
    <cc:license rdf:resource="https://www.nationalarchives.gov.uk/doc/open-government-licence/version/3/"/>
    <cc:attributionURL rdf:resource="https://historicengland.org.uk/"/>
    <cc:attributionName xml:lang="en">Historic England</cc:attributionName>
    <dc:publisher rdf:resource="https://historicengland.org.uk/"/>
    <dc:spatial rdf:resource="http://vocab.getty.edu/tgn/7002445"/>
    <dc:spatial rdf:resource="http://dbpedia.org/resource/England"/>
    <skos:prefLabel xml:lang="en">Brick Shaped Fields</skos:prefLabel>
    <skos:related rdf:resource="http://purl.org/heritagedata/schemes/571/concepts/160155"/>
    <skos:scopeNote xml:lang="en">Patterns of early fields, often prehistoric in origin, that are roughly rectilinear with sinuous sides and that share a common general orientation without having the dominant lines of coaxial fields. Sometimes called Celtic Fields.</skos:scopeNote>
  </skos:Concept>

  <skos:Concept rdf:about="http://purl.org/heritagedata/schemes/571/concepts/160160">
    <skos:broader rdf:resource="http://purl.org/heritagedata/schemes/571/concepts/151727"/>
    <skos:inScheme rdf:resource="http://purl.org/heritagedata/schemes/571"/>
    <dc:identifier>http://purl.org/heritagedata/schemes/571/concepts/160160</dc:identifier>
    <dc:issued rdf:datatype="http://www.w3.org/2001/XMLSchema#dateTime">2024-07-01T17:17:33</dc:issued>
    <cc:license rdf:resource="https://www.nationalarchives.gov.uk/doc/open-government-licence/version/3/"/>
    <cc:attributionURL rdf:resource="https://historicengland.org.uk/"/>
    <cc:attributionName xml:lang="en">Historic England</cc:attributionName>
    <dc:publisher rdf:resource="https://historicengland.org.uk/"/>
    <dc:spatial rdf:resource="http://vocab.getty.edu/tgn/7002445"/>
    <dc:spatial rdf:resource="http://dbpedia.org/resource/England"/>
    <skos:prefLabel xml:lang="en">Grange Fields</skos:prefLabel>
    <skos:related rdf:resource="http://purl.org/heritagedata/schemes/571/concepts/160155"/>
    <skos:scopeNote xml:lang="en">Medieval fields, often large and regular, established on the food producing estates of monasteries.</skos:scopeNote>
  </skos:Concept>

  <skos:Concept rdf:about="http://purl.org/heritagedata/schemes/571/concepts/160163">
    <skos:broader rdf:resource="http://purl.org/heritagedata/schemes/571/concepts/151453"/>
    <skos:inScheme rdf:resource="http://purl.org/heritagedata/schemes/571"/>
    <dc:identifier>http://purl.org/heritagedata/schemes/571/concepts/160163</dc:identifier>
    <dc:issued rdf:datatype="http://www.w3.org/2001/XMLSchema#dateTime">2024-07-01T17:17:33</dc:issued>
    <cc:license rdf:resource="https://www.nationalarchives.gov.uk/doc/open-government-licence/version/3/"/>
    <cc:attributionURL rdf:resource="https://historicengland.org.uk/"/>
    <cc:attributionName xml:lang="en">Historic England</cc:attributionName>
    <dc:publisher rdf:resource="https://historicengland.org.uk/"/>
    <dc:spatial rdf:resource="http://vocab.getty.edu/tgn/7002445"/>
    <dc:spatial rdf:resource="http://dbpedia.org/resource/England"/>
    <skos:prefLabel xml:lang="en">Modern Enclosed Land</skos:prefLabel>
    <skos:related rdf:resource="http://purl.org/heritagedata/schemes/571/concepts/151281"/>
    <skos:related rdf:resource="http://purl.org/heritagedata/schemes/571/concepts/151787"/>
    <skos:scopeNote xml:lang="en">Farmland, whose predominant character developed since World War 2. Usually broad-brush characterisation that includes farming settlement and various land use.</skos:scopeNote>
  </skos:Concept>

  <skos:Concept rdf:about="http://purl.org/heritagedata/schemes/571/concepts/160166">
    <skos:broader rdf:resource="http://purl.org/heritagedata/schemes/571/concepts/151453"/>
    <skos:inScheme rdf:resource="http://purl.org/heritagedata/schemes/571"/>
    <dc:identifier>http://purl.org/heritagedata/schemes/571/concepts/160166</dc:identifier>
    <dc:issued rdf:datatype="http://www.w3.org/2001/XMLSchema#dateTime">2024-07-01T17:17:33</dc:issued>
    <cc:license rdf:resource="https://www.nationalarchives.gov.uk/doc/open-government-licence/version/3/"/>
    <cc:attributionURL rdf:resource="https://historicengland.org.uk/"/>
    <cc:attributionName xml:lang="en">Historic England</cc:attributionName>
    <dc:publisher rdf:resource="https://historicengland.org.uk/"/>
    <dc:spatial rdf:resource="http://vocab.getty.edu/tgn/7002445"/>
    <dc:spatial rdf:resource="http://dbpedia.org/resource/England"/>
    <skos:prefLabel xml:lang="en">Recently Enclosed Land</skos:prefLabel>
    <skos:related rdf:resource="http://purl.org/heritagedata/schemes/571/concepts/151176"/>
    <skos:related rdf:resource="http://purl.org/heritagedata/schemes/571/concepts/151281"/>
    <skos:related rdf:resource="http://purl.org/heritagedata/schemes/571/concepts/160156"/>
    <skos:related rdf:resource="http://purl.org/heritagedata/schemes/571/concepts/160157"/>
    <skos:scopeNote xml:lang="en">Farmland, whose predominant character developed between the medieval period and WW2. Usually broad-brush characterisation that includes farming settlement and various land use.</skos:scopeNote>
  </skos:Concept>

  <skos:Concept rdf:about="http://purl.org/heritagedata/schemes/571/concepts/160169">
    <skos:broader rdf:resource="http://purl.org/heritagedata/schemes/571/concepts/151461"/>
    <skos:inScheme rdf:resource="http://purl.org/heritagedata/schemes/571"/>
    <dc:identifier>http://purl.org/heritagedata/schemes/571/concepts/160169</dc:identifier>
    <dc:issued rdf:datatype="http://www.w3.org/2001/XMLSchema#dateTime">2024-07-01T17:17:33</dc:issued>
    <cc:license rdf:resource="https://www.nationalarchives.gov.uk/doc/open-government-licence/version/3/"/>
    <cc:attributionURL rdf:resource="https://historicengland.org.uk/"/>
    <cc:attributionName xml:lang="en">Historic England</cc:attributionName>
    <dc:publisher rdf:resource="https://historicengland.org.uk/"/>
    <dc:spatial rdf:resource="http://vocab.getty.edu/tgn/7002445"/>
    <dc:spatial rdf:resource="http://dbpedia.org/resource/England"/>
    <skos:prefLabel xml:lang="en">Hydrocarbon Extraction</skos:prefLabel>
    <skos:related rdf:resource="http://purl.org/heritagedata/schemes/571/concepts/152628"/>
    <skos:scopeNote xml:lang="en">The removal of oil, oil derivatives or natural gas from naturally occurring reserves.</skos:scopeNote>
  </skos:Concept>

  <skos:Concept rdf:about="http://purl.org/heritagedata/schemes/571/concepts/160194">
    <skos:broader rdf:resource="http://purl.org/heritagedata/schemes/571/concepts/151900"/>
    <skos:broader rdf:resource="http://purl.org/heritagedata/schemes/571/concepts/151235"/>
    <skos:inScheme rdf:resource="http://purl.org/heritagedata/schemes/571"/>
    <dc:identifier>http://purl.org/heritagedata/schemes/571/concepts/160194</dc:identifier>
    <dc:issued rdf:datatype="http://www.w3.org/2001/XMLSchema#dateTime">2024-07-01T17:17:33</dc:issued>
    <cc:license rdf:resource="https://www.nationalarchives.gov.uk/doc/open-government-licence/version/3/"/>
    <cc:attributionURL rdf:resource="https://historicengland.org.uk/"/>
    <cc:attributionName xml:lang="en">Historic England</cc:attributionName>
    <dc:publisher rdf:resource="https://historicengland.org.uk/"/>
    <dc:spatial rdf:resource="http://vocab.getty.edu/tgn/7002445"/>
    <dc:spatial rdf:resource="http://dbpedia.org/resource/England"/>
    <skos:prefLabel xml:lang="en">Roman Fort</skos:prefLabel>
    <skos:scopeNote xml:lang="en">A Roman period, permanently fortified military base incorporating a range of barracks, victualling and command structures. Often built to standardised plans which developed through time.</skos:scopeNote>
  </skos:Concept>

  <skos:Concept rdf:about="http://purl.org/heritagedata/schemes/571/concepts/160285">
    <skos:narrower rdf:resource="http://purl.org/heritagedata/schemes/571/concepts/160213"/>
    <skos:narrower rdf:resource="http://purl.org/heritagedata/schemes/571/concepts/160252"/>
    <skos:narrower rdf:resource="http://purl.org/heritagedata/schemes/571/concepts/160292"/>
    <skos:broader rdf:resource="http://purl.org/heritagedata/schemes/571/concepts/151450"/>
    <skos:inScheme rdf:resource="http://purl.org/heritagedata/schemes/571"/>
    <dc:identifier>http://purl.org/heritagedata/schemes/571/concepts/160285</dc:identifier>
    <dc:issued rdf:datatype="http://www.w3.org/2001/XMLSchema#dateTime">2024-07-01T17:17:33</dc:issued>
    <cc:license rdf:resource="https://www.nationalarchives.gov.uk/doc/open-government-licence/version/3/"/>
    <cc:attributionURL rdf:resource="https://historicengland.org.uk/"/>
    <cc:attributionName xml:lang="en">Historic England</cc:attributionName>
    <dc:publisher rdf:resource="https://historicengland.org.uk/"/>
    <dc:spatial rdf:resource="http://vocab.getty.edu/tgn/7002445"/>
    <dc:spatial rdf:resource="http://dbpedia.org/resource/England"/>
    <skos:prefLabel xml:lang="en">Recreation</skos:prefLabel>
    <skos:scopeNote xml:lang="en">Activities undertaken in leisure (or discretionary) time for the purposes of enjoyment, amusement or pleasure.</skos:scopeNote>
  </skos:Concept>

  <skos:Concept rdf:about="http://purl.org/heritagedata/schemes/571/concepts/160264">
    <skos:broader rdf:resource="http://purl.org/heritagedata/schemes/571/concepts/151756"/>
    <skos:broader rdf:resource="http://purl.org/heritagedata/schemes/571/concepts/160292"/>
    <skos:inScheme rdf:resource="http://purl.org/heritagedata/schemes/571"/>
    <dc:identifier>http://purl.org/heritagedata/schemes/571/concepts/160264</dc:identifier>
    <dc:issued rdf:datatype="http://www.w3.org/2001/XMLSchema#dateTime">2024-07-01T17:17:33</dc:issued>
    <cc:license rdf:resource="https://www.nationalarchives.gov.uk/doc/open-government-licence/version/3/"/>
    <cc:attributionURL rdf:resource="https://historicengland.org.uk/"/>
    <cc:attributionName xml:lang="en">Historic England</cc:attributionName>
    <dc:publisher rdf:resource="https://historicengland.org.uk/"/>
    <dc:spatial rdf:resource="http://vocab.getty.edu/tgn/7002445"/>
    <dc:spatial rdf:resource="http://dbpedia.org/resource/England"/>
    <skos:prefLabel xml:lang="en">Municipal Park</skos:prefLabel>
    <skos:scopeNote xml:lang="en">Land, often in urban areas, dedicated to outdoor public recreation. Usually with ornamental planting of trees and shrubs, with some formal gardens, ornamental ponds etc. Generally more robust than in landscaped parks with public conveniences &amp; playgrounds</skos:scopeNote>
  </skos:Concept>

  <skos:Concept rdf:about="http://purl.org/heritagedata/schemes/571/concepts/160274">
    <skos:broader rdf:resource="http://purl.org/heritagedata/schemes/571/concepts/151704"/>
    <skos:broader rdf:resource="http://purl.org/heritagedata/schemes/571/concepts/160292"/>
    <skos:inScheme rdf:resource="http://purl.org/heritagedata/schemes/571"/>
    <dc:identifier>http://purl.org/heritagedata/schemes/571/concepts/160274</dc:identifier>
    <dc:issued rdf:datatype="http://www.w3.org/2001/XMLSchema#dateTime">2024-07-01T17:17:33</dc:issued>
    <cc:license rdf:resource="https://www.nationalarchives.gov.uk/doc/open-government-licence/version/3/"/>
    <cc:attributionURL rdf:resource="https://historicengland.org.uk/"/>
    <cc:attributionName xml:lang="en">Historic England</cc:attributionName>
    <dc:publisher rdf:resource="https://historicengland.org.uk/"/>
    <dc:spatial rdf:resource="http://vocab.getty.edu/tgn/7002445"/>
    <dc:spatial rdf:resource="http://dbpedia.org/resource/England"/>
    <skos:prefLabel xml:lang="en">Open Air Museum</skos:prefLabel>
    <skos:scopeNote xml:lang="en">A building, group of buildings or space within a building, where objects of value such as works of art, antiquities, scientific specimens, or other artefacts are housed and displayed.</skos:scopeNote>
  </skos:Concept>

  <skos:Concept rdf:about="http://purl.org/heritagedata/schemes/571/concepts/160476">
    <skos:broader rdf:resource="http://purl.org/heritagedata/schemes/571/concepts/152326"/>
    <skos:narrower>
      <skos:Concept rdf:about="http://purl.org/heritagedata/schemes/571/concepts/160477">
        <skos:broader rdf:resource="http://purl.org/heritagedata/schemes/571/concepts/160476"/>
        <skos:inScheme rdf:resource="http://purl.org/heritagedata/schemes/571"/>
        <dc:identifier>http://purl.org/heritagedata/schemes/571/concepts/160477</dc:identifier>
        <dc:issued rdf:datatype="http://www.w3.org/2001/XMLSchema#dateTime">2024-07-01T17:17:33</dc:issued>
        <cc:license rdf:resource="https://www.nationalarchives.gov.uk/doc/open-government-licence/version/3/"/>
        <cc:attributionURL rdf:resource="https://historicengland.org.uk/"/>
        <cc:attributionName xml:lang="en">Historic England</cc:attributionName>
        <dc:publisher rdf:resource="https://historicengland.org.uk/"/>
        <dc:spatial rdf:resource="http://vocab.getty.edu/tgn/7002445"/>
        <dc:spatial rdf:resource="http://dbpedia.org/resource/England"/>
        <skos:prefLabel xml:lang="en">Furze (Divided)</skos:prefLabel>
        <skos:scopeNote xml:lang="en">Areas of furze divided by stock-proof boundaries.</skos:scopeNote>
      </skos:Concept>
    </skos:narrower>

    <skos:narrower>
      <skos:Concept rdf:about="http://purl.org/heritagedata/schemes/571/concepts/160478">
        <skos:broader rdf:resource="http://purl.org/heritagedata/schemes/571/concepts/160476"/>
        <skos:inScheme rdf:resource="http://purl.org/heritagedata/schemes/571"/>
        <dc:identifier>http://purl.org/heritagedata/schemes/571/concepts/160478</dc:identifier>
        <dc:issued rdf:datatype="http://www.w3.org/2001/XMLSchema#dateTime">2024-07-01T17:17:33</dc:issued>
        <cc:license rdf:resource="https://www.nationalarchives.gov.uk/doc/open-government-licence/version/3/"/>
        <cc:attributionURL rdf:resource="https://historicengland.org.uk/"/>
        <cc:attributionName xml:lang="en">Historic England</cc:attributionName>
        <dc:publisher rdf:resource="https://historicengland.org.uk/"/>
        <dc:spatial rdf:resource="http://vocab.getty.edu/tgn/7002445"/>
        <dc:spatial rdf:resource="http://dbpedia.org/resource/England"/>
        <skos:prefLabel xml:lang="en">Furze (Undivided)</skos:prefLabel>
        <skos:scopeNote xml:lang="en">Areas of furze left open, not divided by stock-proof boundaries.</skos:scopeNote>
      </skos:Concept>
    </skos:narrower>

    <skos:inScheme rdf:resource="http://purl.org/heritagedata/schemes/571"/>
    <dc:identifier>http://purl.org/heritagedata/schemes/571/concepts/160476</dc:identifier>
    <dc:issued rdf:datatype="http://www.w3.org/2001/XMLSchema#dateTime">2024-07-01T17:17:33</dc:issued>
    <cc:license rdf:resource="https://www.nationalarchives.gov.uk/doc/open-government-licence/version/3/"/>
    <cc:attributionURL rdf:resource="https://historicengland.org.uk/"/>
    <cc:attributionName xml:lang="en">Historic England</cc:attributionName>
    <dc:publisher rdf:resource="https://historicengland.org.uk/"/>
    <dc:spatial rdf:resource="http://vocab.getty.edu/tgn/7002445"/>
    <dc:spatial rdf:resource="http://dbpedia.org/resource/England"/>
    <skos:prefLabel xml:lang="en">Furze</skos:prefLabel>
    <skos:scopeNote xml:lang="en">Unimproved land dominated by furze (gorse), used for rough grazing and harvested as domestic fuel.</skos:scopeNote>
  </skos:Concept>

  <skos:Concept rdf:about="http://purl.org/heritagedata/schemes/571/concepts/164067">
    <skos:broader rdf:resource="http://purl.org/heritagedata/schemes/571/concepts/152394"/>
    <skos:narrower>
      <skos:Concept rdf:about="http://purl.org/heritagedata/schemes/571/concepts/164068">
        <skos:broader rdf:resource="http://purl.org/heritagedata/schemes/571/concepts/164067"/>
        <skos:inScheme rdf:resource="http://purl.org/heritagedata/schemes/571"/>
        <dc:identifier>http://purl.org/heritagedata/schemes/571/concepts/164068</dc:identifier>
        <dc:issued rdf:datatype="http://www.w3.org/2001/XMLSchema#dateTime">2024-07-01T17:17:33</dc:issued>
        <cc:license rdf:resource="https://www.nationalarchives.gov.uk/doc/open-government-licence/version/3/"/>
        <cc:attributionURL rdf:resource="https://historicengland.org.uk/"/>
        <cc:attributionName xml:lang="en">Historic England</cc:attributionName>
        <dc:publisher rdf:resource="https://historicengland.org.uk/"/>
        <dc:spatial rdf:resource="http://vocab.getty.edu/tgn/7002445"/>
        <dc:spatial rdf:resource="http://dbpedia.org/resource/England"/>
        <skos:prefLabel xml:lang="en">Water Meadow (Regular Pattern)</skos:prefLabel>
        <skos:scopeNote xml:lang="en">Water meadow with relatively rigid patterns of drains, usually perfectly straight and with large numbers parallel with each other.</skos:scopeNote>
      </skos:Concept>
    </skos:narrower>

    <skos:narrower>
      <skos:Concept rdf:about="http://purl.org/heritagedata/schemes/571/concepts/164069">
        <skos:broader rdf:resource="http://purl.org/heritagedata/schemes/571/concepts/164067"/>
        <skos:inScheme rdf:resource="http://purl.org/heritagedata/schemes/571"/>
        <dc:identifier>http://purl.org/heritagedata/schemes/571/concepts/164069</dc:identifier>
        <dc:issued rdf:datatype="http://www.w3.org/2001/XMLSchema#dateTime">2024-07-01T17:17:33</dc:issued>
        <cc:license rdf:resource="https://www.nationalarchives.gov.uk/doc/open-government-licence/version/3/"/>
        <cc:attributionURL rdf:resource="https://historicengland.org.uk/"/>
        <cc:attributionName xml:lang="en">Historic England</cc:attributionName>
        <dc:publisher rdf:resource="https://historicengland.org.uk/"/>
        <dc:spatial rdf:resource="http://vocab.getty.edu/tgn/7002445"/>
        <dc:spatial rdf:resource="http://dbpedia.org/resource/England"/>
        <skos:prefLabel xml:lang="en">Water Meadow (Irregular Pattern)</skos:prefLabel>
        <skos:scopeNote xml:lang="en">Water meadow with a relatively irregular pattern of drains, usually more sinuous and with fewer being parallel with each other.</skos:scopeNote>
      </skos:Concept>
    </skos:narrower>

    <skos:inScheme rdf:resource="http://purl.org/heritagedata/schemes/571"/>
    <dc:identifier>http://purl.org/heritagedata/schemes/571/concepts/164067</dc:identifier>
    <dc:issued rdf:datatype="http://www.w3.org/2001/XMLSchema#dateTime">2024-07-01T17:17:33</dc:issued>
    <cc:license rdf:resource="https://www.nationalarchives.gov.uk/doc/open-government-licence/version/3/"/>
    <cc:attributionURL rdf:resource="https://historicengland.org.uk/"/>
    <cc:attributionName xml:lang="en">Historic England</cc:attributionName>
    <dc:publisher rdf:resource="https://historicengland.org.uk/"/>
    <dc:spatial rdf:resource="http://vocab.getty.edu/tgn/7002445"/>
    <dc:spatial rdf:resource="http://dbpedia.org/resource/England"/>
    <skos:prefLabel xml:lang="en">Water Meadow</skos:prefLabel>
    <skos:scopeNote xml:lang="en">Controlled irrigation to draw nutrient-rich silts and material onto valley-bottom grassland to increase hay yields and enable earlier mowing. Early modern agricultural improvement; normally now no longer operated though earthworks may survive.</skos:scopeNote>
  </skos:Concept>

</rdf:RDF>